@prefix owl: <http://www.w3.org/2002/07/owl#> .
@prefix rdfs: <http://www.w3.org/2000/01/rdf-schema#> .
@prefix dc11: <http://purl.org/dc/elements/1.1/> .
@prefix ns0: <http://www.wurvoc.org/vocabularies/WV/> .
@prefix dc: <http://purl.org/dc/terms/> .
@prefix ns1: <http://www.wurvoc.org/bibliography/om-2/> .
@prefix ns2: <http://www.ontology-of-units-of-measure.org/resource/om-2/> .
@prefix skos: <http://www.w3.org/2004/02/skos/core#> .
@prefix bibo: <http://purl.org/ontology/bibo/> .
@prefix foaf: <http://xmlns.com/foaf/0.1/> .
@prefix xsd: <http://www.w3.org/2001/XMLSchema#> .
@prefix rdf: <http://www.w3.org/1999/02/22-rdf-syntax-ns#> .

<http://www.ontology-of-units-of-measure.org/resource/om-2>
  a owl:Ontology ;
  rdfs:label "Ontology of units of Measure (OM)"@en, "測定単位のオントロジー (OM)"@ja ;
  owl:versionInfo "2.0.39"@en ;
  dc11:identifier "http://www.ontology-of-units-of-measure.org/vocabularies/om-2/" ;
  dc11:date "2023/03/17" ;
  rdfs:comment "The Ontology of units of Measure (OM) 2.0 models concepts and relations important to scientific research. It has a strong focus on units, quantities, measurements, and dimensions."@en, "測定単位のオントロジー (Ontology of units of Measure; OM) は，科学技術にとって重要な概念及び関係をモデル化する。OMは，単位・量・測定・次元に特に焦点を当てている。"@ja ;
  ns0:logo "http://www.wurvoc.org/images/vocabularies/om-logo.jpg" ;
  ns0:illustration "http://www.wurvoc.org/images/vocabularies/om-illustration.jpg" ;
  dc11:creator "Hajo Rijgersberg, Don Willems, Jan Top"@en ;
  dc:license <https://creativecommons.org/licenses/by/4.0/> ;
  ns1:reference <http://www.openisbn.com/isbn/9789462280618/> .

<http://www.ontology-of-units-of-measure.org/resource/om-2/alternativeLabel>
  a owl:AnnotationProperty ;
  rdfs:label "alternative label"@en, "標識の別名"@ja .

<http://www.ontology-of-units-of-measure.org/resource/om-2/longcomment>
  a owl:AnnotationProperty ;
  rdfs:label "longcomment"@en, "詳細な注釈"@ja ;
  ns2:alternativeLabel "long comment"@en, "has longcomment"@en, "詳細な注釈がある"@ja .

ns2:symbol
  a owl:AnnotationProperty ;
  rdfs:label "symbol"@en, "記号"@ja ;
  ns2:alternativeLabel "has symbol"@en, "記号を持つ"@ja .

ns2:alternativeSymbol
  a owl:AnnotationProperty ;
  rdfs:label "alternative symbol"@en, "別の記号"@ja ;
  ns2:alternativeLabel "has alternative symbol"@en, "別の記号を持つ"@ja .

ns2:abbreviation
  a owl:AnnotationProperty ;
  rdfs:label "abbreviation"@en, "略記"@ja ;
  ns2:alternativeLabel "has abbreviation"@en, "略記がある"@ja .
ns2:unofficialLabel
  a owl:AnnotationProperty ;
  rdfs:label "unofficial label"@en, "非公式な記号"@ja ;
  ns2:alternativeLabel "has unofficial label"@en, "非公式な記号を持つ"@ja ;
  rdfs:comment "Used to specify labels that are used in e.g. every day speech but are not defined in any standard." ;
  rdfs:subPropertyOf skos:hiddenLabel .

ns2:unofficialAbbreviation
  a owl:AnnotationProperty ;
  rdfs:label "unofficial abbreviation"@en, "非公式な略記"@ja ;
  ns2:alternativeLabel "has unofficial abbreviation"@en, "非公式な略記がある"@ja ;
  rdfs:comment "Used to specify abbreviations that are used in e.g. every day speech but are not defined in any standard." ;
  rdfs:subPropertyOf skos:hiddenLabel .
ns2:Quantity
  a owl:Class ;
  rdfs:label "quantity"@en, "量"@ja ;
  rdfs:comment "A quantity is a representation of a quantifiable (standardised) aspect (such as length, mass, and time) of a phenomenon (e.g., a star, a molecule, or a food product). Quantities are classified according to similarity in their (implicit) metrological aspect, e.g. the length of my table and the length of my chair are both classified as length."@en, "量とは，ある現象（例: 星・分子・食品）の定量化できる（標準化された）性質（例: 長さ・質量・時間）の表現である。量は（暗黙の）計量的類似性に従って分離される。例: 机の長さ及び椅子の長さは双方とも長さに分類される。"@ja .

ns2:hasPhenomenon
  a owl:ObjectProperty ;
  rdfs:label "has phenomenon"@en, "現象がある"@ja ;
  rdfs:domain ns2:Quantity .

ns2:hasContext
  a owl:ObjectProperty ;
  rdfs:label "has context"@en, "文脈を持つ"@ja ;
  rdfs:domain ns2:Quantity .

ns2:hasValue
  a owl:ObjectProperty ;
  rdfs:label "has value"@en, "値を持つ"@ja ;
  rdfs:domain ns2:Quantity ;
  rdfs:range [
    a owl:Class ;
    owl:unionOf (
     ns2:Measure
     ns2:Point
   )
  ] .

ns2:Measure
  a owl:Class ;
  rdfs:label "measure"@en ;
  rdfs:comment "A measure combines a number to a unit of measure. For example, \"3 m\" is a measure."@en .

ns2:Point
  a owl:Class ;
  rdfs:label "point"@en ;
  rdfs:comment "A point is an element of an interval scale or a ratio scale, for example, 273.16 on the Kelvin scale indicates the triple point of water thermodynamic temperature."@en .

ns2:commonlyHasUnit
  a owl:ObjectProperty ;
  rdfs:label "commonly has unit"@en, "通常は単位を持つ"@ja ;
  ns2:alternativeLabel "commonly has unit of measure"@en, "通常は測定単位を持つ"@ja ;
  rdfs:comment "This property indicates a commonly-used unit." ;
  rdfs:domain ns2:Quantity ;
  rdfs:range ns2:Unit .

ns2:hasAggregateFunction
  a owl:ObjectProperty ;
  rdfs:label "has aggregate function"@en, "集計関数を持つ"@ja ;
  rdfs:domain ns2:Quantity ;
  rdfs:range ns2:Function .

ns2:Function
  a owl:Class ;
  rdfs:label "function"@en, "関数"@ja .

ns2:first
  a ns2:Function ;
  rdfs:label "first"@en, "最初"@ja .

ns2:last
  a ns2:Function ;
  rdfs:label "last"@en, "最後"@ja .

ns2:minimum
  a ns2:Function ;
  rdfs:label "minimum"@en, "最小"@ja .

ns2:maximum
  a ns2:Function ;
  rdfs:label "maximum"@en, "最大"@ja .

ns2:sum
  a ns2:Function ;
  rdfs:label "sum"@en, "合計"@ja .

ns2:average
  a ns2:Function ;
  rdfs:label "average"@en, "平均"@ja .

ns2:count
  a ns2:Function ;
  rdfs:label "count"@en, "回数"@ja .

ns2:standardDeviation
  a ns2:Function ;
  rdfs:label "standard deviation"@en, "標準偏差"@ja .

ns2:product
  a ns2:Function ;
  rdfs:label "product"@en, "積"@ja .

ns2:median
  a ns2:Function ;
  rdfs:label "median"@en ;
  ns2:alternativeLabel "50th percentile"@en .

ns2:10thPercentile
  a ns2:Function ;
  rdfs:label "10th percentile"@en .

ns2:20thPercentile
  a ns2:Function ;
  rdfs:label "20th percentile"@en .

ns2:25thPercentile
  a ns2:Function ;
  rdfs:label "25th percentile"@en .

ns2:30thPercentile
  a ns2:Function ;
  rdfs:label "30th percentile"@en .

ns2:40thPercentile
  a ns2:Function ;
  rdfs:label "40th percentile"@en .

ns2:60thPercentile
  a ns2:Function ;
  rdfs:label "60th percentile"@en .

ns2:70thPercentile
  a ns2:Function ;
  rdfs:label "70th percentile"@en .

ns2:75thPercentile
  a ns2:Function ;
  rdfs:label "th percentile"@en .

ns2:80thPercentile
  a ns2:Function ;
  rdfs:label "80th percentile"@en .

ns2:90thPercentile
  a ns2:Function ;
  rdfs:label "90th percentile"@en .

ns2:hasQuantity
  a owl:ObjectProperty ;
  rdfs:label "has quantity"@en, "量を持つ"@ja ;
  rdfs:domain [
    a owl:Class ;
    owl:unionOf (
     ns2:SingularUnit
     ns2:FixedPoint
   )
  ] ;
  rdfs:range ns2:Quantity .

ns2:SingularUnit
  a owl:Class ;
  rdfs:label "singular unit"@en, "単数単位"@ja ;
  rdfs:subClassOf ns2:Unit .

ns2:FixedPoint
  a owl:Class ;
  rdfs:label "fixed point"@en ;
  rdfs:subClassOf ns2:Point, [
    a owl:Restriction ;
    owl:onProperty ns2:hasPoint ;
    owl:allValuesFrom [
      a owl:Class ;
      owl:unionOf ( ns2:FixedPoint )
    ]
  ] .

ns2:Unit
  a owl:Class ;
  rdfs:label "unit"@en, "単位"@ja ;
  ns2:alternativeLabel "unit of measure"@en, "測定単位"@ja, "unit of measurement"@en, "測定の単位"@ja ;
  rdfs:comment "A unit of measure is a definite magnitude of a quantity, defined and adopted by convention or by law. It is used as a standard for measurement of the same quantity, where any other value of the quantity can be expressed as a simple multiple of the unit. For example, length is a quantity; the metre is a unit of length that represents a definite predetermined length. When we say 10 metre (or 10 m), we actually mean 10 times the definite predetermined length called \"metre\"."@en, "測定単位とは，量の確定的な大きさであり，慣例又は法律によって定義し採用されている。同じ量の測定の標準として用いられ，他の如何なる量の値も当該単位の単純な倍数として表わせる。例えば，長さも量である; メートルは長さの単位であり，確定的な所定の長さを表している。10メートル（又は10 m）とは，「メートル」と呼ばれる確定的な所定の長さの10倍を，実際に意味している。"@ja .

ns2:PrefixedUnit
  a owl:Class ;
  rdfs:label "prefixed unit"@en, "補助単位"@ja ;
  rdfs:subClassOf ns2:Unit, [
    a owl:Restriction ;
    owl:onProperty ns2:hasUnit ;
    owl:allValuesFrom ns2:SingularUnit
  ] .

ns2:hasUnit
  a owl:ObjectProperty, owl:FunctionalProperty ;
  rdfs:label "has unit"@en, "単位を持つ"@ja ;
  rdfs:domain [
    a owl:Class ;
    owl:unionOf (
     ns2:PrefixedUnit
     ns2:UnitMultiple
     ns2:SingularUnit
     ns2:IntervalScale
     ns2:RatioScale
     ns2:Measure
   )
  ] ;
  rdfs:range ns2:Unit .

ns2:UnitMultiple
  a owl:Class ;
  rdfs:label "unit multiple"@en, "単位倍量"@ja ;
  rdfs:subClassOf ns2:Unit .

ns2:IntervalScale
  a owl:Class ;
  rdfs:label "interval scale"@en ;
  rdfs:subClassOf ns2:Scale .

ns2:RatioScale
  a owl:Class ;
  rdfs:label "ratio scale"@en ;
  rdfs:subClassOf ns2:Scale .

ns2:hasPrefix
  a owl:ObjectProperty, owl:FunctionalProperty ;
  rdfs:label "has prefix"@en, "補助単位を持つ"@ja ;
  rdfs:domain ns2:PrefixedUnit ;
  rdfs:range ns2:Prefix .

ns2:hasFactor
  a owl:DatatypeProperty, owl:FunctionalProperty ;
  rdfs:label "has factor"@en, "因子を持つ"@ja ;
  rdfs:domain [
    a owl:Class ;
    owl:unionOf (
     ns2:UnitMultiple
     ns2:SingularUnit
     ns2:Prefix
     ns2:Scale
   )
  ] ;
  rdfs:range xsd:float .

ns2:Prefix
  a owl:Class ;
  rdfs:label "prefix"@en ;
  rdfs:comment "A prefix is a name that precedes a basic unit of measure to indicate a decimal or binary multiple or fraction of the unit. Each prefix has a unique symbol that is prepended to the unit symbol. For example, an electric current of 0.000 000 001 ampere is written by using the SI-prefix nano as 1 nanoampere or 1 nA."@en .

ns2:Scale
  a owl:Class ;
  rdfs:label "scale"@en ;
  ns2:alternativeLabel "measurement scale"@en, "schaal"@nl, "meetschaal"@nl .

ns2:CompoundUnit
  a owl:Class ;
  rdfs:label "compound unit"@en, "複合単位"@ja ;
  rdfs:subClassOf ns2:Unit .

ns2:UnitMultiplication
  a owl:Class ;
  rdfs:label "unit multiplication"@en, "単位乗算"@ja ;
  rdfs:subClassOf ns2:CompoundUnit .

ns2:hasTerm1
  a owl:ObjectProperty ;
  rdfs:label "has term 1"@en ;
  rdfs:domain ns2:UnitMultiplication ;
  rdfs:range ns2:Unit .

ns2:hasTerm2
  a owl:ObjectProperty ;
  rdfs:label "has term 2"@en ;
  rdfs:domain ns2:UnitMultiplication ;
  rdfs:range ns2:Unit .

ns2:UnitExponentiation
  a owl:Class ;
  rdfs:label "unit exponentiation"@en ;
  rdfs:subClassOf ns2:CompoundUnit .

ns2:hasBase
  a owl:ObjectProperty ;
  rdfs:label "has base"@en ;
  rdfs:domain ns2:UnitExponentiation ;
  rdfs:range ns2:Unit .

ns2:hasExponent
  a owl:DatatypeProperty ;
  rdfs:label "has exponent"@en ;
  rdfs:domain ns2:UnitExponentiation ;
  rdfs:range xsd:integer .

ns2:UnitDivision
  a owl:Class ;
  rdfs:label "unit division"@en ;
  rdfs:subClassOf ns2:CompoundUnit .

ns2:hasNumerator
  a owl:ObjectProperty ;
  rdfs:label "has numerator"@en ;
  rdfs:domain ns2:UnitDivision ;
  rdfs:range ns2:Unit .

ns2:hasDenominator
  a owl:ObjectProperty ;
  rdfs:label "has denominator"@en ;
  rdfs:domain ns2:UnitDivision ;
  rdfs:range ns2:Unit .

ns2:hasNumericalValue
  a owl:DatatypeProperty, owl:FunctionalProperty ;
  rdfs:label "has numerical value"@en ;
  rdfs:domain [
    a owl:Class ;
    owl:unionOf (
     ns2:Measure
     ns2:Point
   )
  ] .

ns2:hasOff-Set
  a owl:DatatypeProperty ;
  rdfs:label "has off-set"@en ;
  rdfs:domain ns2:Scale ;
  rdfs:range xsd:float .

ns2:FixedZeroPoint
  a owl:Class ;
  rdfs:label "fixed zero point"@en ;
  rdfs:subClassOf ns2:FixedPoint .

ns2:hasPoint
  a owl:ObjectProperty ;
  rdfs:label "has point"@en ;
  rdfs:domain [
    a owl:Class ;
    owl:unionOf (
     ns2:IntervalScale
     ns2:RatioScale
     ns2:FixedPoint
   )
  ] ;
  rdfs:range ns2:Point .

ns2:hasScale
  a owl:ObjectProperty ;
  rdfs:label "has scale"@en ;
  rdfs:domain [
    a owl:Class ;
    owl:unionOf (
     ns2:Scale
     ns2:Quantity
     ns2:ApplicationArea
   )
  ] ;
  rdfs:range ns2:Scale .

ns2:ApplicationArea
  a owl:Class ;
  rdfs:label "application area"@en ;
  rdfs:comment "An application area groups quantities and units of measure for application areas such as scientific disciplines (e.g., thermodynamics, mechanics)."@en .

ns2:Dimension
  a owl:Class ;
  rdfs:label "dimension"@en ;
  rdfs:comment "Dimensions are abstract properties of units and quantities neglecting their vectorial or tensorial character and all numerical factors including their sign."@en .

ns2:hasDimension
  a owl:ObjectProperty ;
  rdfs:label "has dimension"@en ;
  rdfs:domain [
    a owl:Class ;
    owl:unionOf (
     ns2:Quantity
     ns2:Unit
     ns2:Scale
   )
  ] ;
  rdfs:range ns2:Dimension .

ns2:hasSILengthDimensionExponent
  a owl:DatatypeProperty ;
  rdfs:label "has SI length dimension exponent"@en ;
  rdfs:domain ns2:Dimension ;
  rdfs:range xsd:integer .

ns2:hasSIMassDimensionExponent
  a owl:DatatypeProperty ;
  rdfs:label "has SI mass dimension exponent"@en ;
  rdfs:domain ns2:Dimension ;
  rdfs:range xsd:integer .

ns2:hasSITimeDimensionExponent
  a owl:DatatypeProperty ;
  rdfs:label "has SI time dimension exponent"@en ;
  rdfs:domain ns2:Dimension ;
  rdfs:range xsd:integer .

ns2:hasSIElectricCurrentDimensionExponent
  a owl:DatatypeProperty ;
  rdfs:label "has SI electric current dimension exponent"@en ;
  rdfs:domain ns2:Dimension ;
  rdfs:range xsd:integer .

ns2:hasSIThermodynamicTemperatureDimensionExponent
  a owl:DatatypeProperty ;
  rdfs:label "has SI thermodynamic temperature dimension exponent"@en ;
  rdfs:domain ns2:Dimension ;
  rdfs:range xsd:integer .

ns2:hasSIAmountOfSubstanceDimensionExponent
  a owl:DatatypeProperty ;
  rdfs:label "has SI amount of substance dimension exponent"@en ;
  rdfs:domain ns2:Dimension ;
  rdfs:range xsd:integer .

ns2:hasSILuminousIntensityDimensionExponent
  a owl:DatatypeProperty ;
  rdfs:label "has SI luminous intensity dimension exponent"@en ;
  rdfs:domain ns2:Dimension ;
  rdfs:range xsd:integer .

ns2:SystemOfUnits
  a owl:Class ;
  rdfs:label "system of units"@en ;
  rdfs:comment "In order to achieve a coherent, interdependent set of units of measure in the wide variety of units that exist, units are organised in systems of units. A system of units is based on a set of units chosen by convention to be the system’s base units, units that are considered to be mutually independent (i.e., can’t be expressed in terms of each other)."@en .

ns2:hasBaseQuantity
  a owl:ObjectProperty ;
  rdfs:label "has base quantity"@en ;
  rdfs:domain ns2:SystemOfUnits ;
  rdfs:range ns2:Quantity .

ns2:hasBaseUnit
  a owl:ObjectProperty ;
  rdfs:label "has base unit"@en ;
  rdfs:domain ns2:SystemOfUnits ;
  rdfs:range ns2:Unit .

ns2:hasDerivedQuantity
  a owl:ObjectProperty ;
  rdfs:label "has derived quantity"@en ;
  rdfs:domain ns2:SystemOfUnits ;
  rdfs:range ns2:Quantity .

ns2:hasDerivedUnit
  a owl:ObjectProperty ;
  rdfs:label "has derived unit"@en ;
  rdfs:domain ns2:SystemOfUnits ;
  rdfs:range ns2:Unit .

ns2:usesQuantity
  a owl:ObjectProperty ;
  rdfs:label "uses quantity"@en ;
  rdfs:domain ns2:ApplicationArea ;
  rdfs:range ns2:Quantity .

ns2:usesUnit
  a owl:ObjectProperty ;
  rdfs:label "uses unit"@en ;
  rdfs:domain ns2:ApplicationArea ;
  rdfs:range ns2:Unit .

ns2:LaTeXCommand
  a owl:AnnotationProperty ;
  rdfs:label "LaTeX command"@en ;
  ns2:alternativeLabel "typeset by LaTeX command"@en ;
  rdfs:comment "OMLaTeX command that can be used to render this quantity or unit."@en .

ns2:LaTeXSymbol
  a owl:AnnotationProperty ;
  rdfs:label "LaTeX symbol"@en ;
  ns2:alternativeLabel "has LaTeX symbol"@en, "LaTeX formatted symbol"@en ;
  rdfs:comment "OMLaTeX formatted symbol may include commands such as \\unit and \\E as defined in OMLaTeX."@en .

ns2:alternativeLaTeXSymbol
  a owl:AnnotationProperty ;
  rdfs:label "alternative LaTeX symbol"@en ;
  ns2:alternativeLabel "has alternative LaTeX symbol"@en, "alternative LaTeX formatted symbol"@en ;
  rdfs:comment "An alternative OMLaTeX formatted symbol, which may include commands such as \\unit and \\E as defined in OMLaTeX."@en .

ns2:geometry
  a ns2:ApplicationArea ;
  rdfs:label "geometry"@en, "geometrie"@nl ;
  ns2:usesQuantity ns2:Length, ns2:Breadth, ns2:Height, ns2:Thickness, ns2:Width, ns2:Radius, ns2:Diameter, ns2:Circumference, ns2:Area, ns2:Volume, ns2:Angle, ns2:SolidAngle, ns2:LengthFraction, ns2:Slope ;
  ns2:usesUnit ns2:chain, ns2:cicero, ns2:fathom-USSurvey, ns2:fermi, ns2:foot-International, ns2:foot-USSurvey, ns2:furlong-International, ns2:inch-International, ns2:metre, ns2:micrometre, ns2:millimetre, ns2:centimetre, ns2:decimetre, ns2:decametre, ns2:hectometre, ns2:kilometre, ns2:megametre, ns2:gigametre, ns2:micron, ns2:mil-Length, ns2:mile-Statute, ns2:mile-USSurvey, ns2:nauticalMile-International, ns2:pica-ATA, ns2:pica-Postscript, ns2:pica-TeX, ns2:point-ATA, ns2:point-Didot, ns2:point-Postscript, ns2:point-TeX, ns2:rod-US, ns2:yard-International, ns2:angstrom, ns2:attometre, ns2:femtometre, ns2:picometre, ns2:nanometre, ns2:astronomicalUnit, ns2:lightYear, ns2:terametre, ns2:petametre, ns2:exametre, ns2:parsec, ns2:megaparsec, ns2:acre-International, ns2:acre-USSurvey, ns2:are, ns2:barn, ns2:centiare, ns2:circularMil, ns2:squareInch-International, ns2:squareFoot-International, ns2:squareYard-International, ns2:squareMile-International, ns2:hectare, ns2:squareCentimetre, ns2:squareDecametre, ns2:squareDecimetre, ns2:squareGigametre, ns2:squareHectometre, ns2:squareKilometre, ns2:squareMegametre, ns2:squareMetre, ns2:squareMicrometre, ns2:squareMillimetre, ns2:squareAttometre, ns2:squareFemtometre, ns2:squareNanometre, ns2:squarePicometre, ns2:squareExametre, ns2:squarePetametre, ns2:squareTerametre, ns2:acreFoot, ns2:barrel-US, ns2:bushel-US, ns2:cord, ns2:cubicCentimetre, ns2:cubicDecametre, ns2:cubicDecimetre, ns2:cubicGigametre, ns2:cubicHectometre, ns2:cubicKilometre, ns2:cubicMegametre, ns2:cubicMetre, ns2:cubicMicrometre, ns2:cubicMillimetre, ns2:cup-USCustomary, ns2:cubicParsec, ns2:cubicKiloparsec, ns2:dryGallon-US, ns2:dryPint-US, ns2:dryQuart-US, ns2:fluidOunce-Imperial, ns2:fluidOunce-US, ns2:gallon-Imperial, ns2:gallon-US, ns2:gill-Imperial, ns2:gill-US, ns2:litre, ns2:microlitre, ns2:millilitre, ns2:centilitre, ns2:decilitre, ns2:decalitre, ns2:hectolitre, ns2:kilolitre, ns2:megalitre, ns2:gigalitre, ns2:liquidPint-US, ns2:liquidQuart-US, ns2:peck-US, ns2:pint-Imperial, ns2:quart-Imperial, ns2:stere, ns2:tablespoon-US, ns2:teaspoon-US, ns2:dessertspoon, ns2:ton-Register, ns2:cubicAttometre, ns2:cubicFemtometre, ns2:cubicNanometre, ns2:cubicPicometre, ns2:attolitre, ns2:femtolitre, ns2:picolitre, ns2:nanolitre, ns2:cubicExametre, ns2:cubicPetametre, ns2:cubicTerametre, ns2:teralitre, ns2:petalitre, ns2:exalitre, ns2:degree, ns2:gon, ns2:metrePerMetre, ns2:mil-Angle, ns2:minute-Angle, ns2:radian, ns2:microradian, ns2:milliradian, ns2:centiradian, ns2:deciradian, ns2:revolution, ns2:second-Angle, ns2:attoradian, ns2:femtoradian, ns2:picoradian, ns2:nanoradian, ns2:millisecond-Angle, ns2:microsecond-Angle, ns2:degreeSquared, ns2:steradian, ns2:microsteradian, ns2:millisteradian, ns2:centisteradian, ns2:decisteradian, ns2:attosteradian, ns2:femtosteradian, ns2:picosteradian, ns2:nanosteradian, ns2:millimetrePerMetre .

ns2:Length
  a owl:Class ;
  rdfs:label "length"@en, "lengte"@nl, "长度"@zh ;
  rdfs:comment "Length is the amount of space between two geographical points along a curve. It is a base quantity in the International System of Units and other systems of units. Length is speed times time. The metre, a base unit of length in the International System of Units, is defined in terms of speed of light during a certain time interval."@en ;
  rdfs:subClassOf ns2:Quantity, [
    a owl:Restriction ;
    owl:onProperty ns2:hasValue ;
    owl:allValuesFrom [
      a owl:Restriction ;
      owl:onProperty ns2:hasUnit ;
      owl:allValuesFrom ns2:LengthUnit
    ]
  ], [
    a owl:Restriction ;
    owl:onProperty ns2:hasDimension ;
    owl:hasValue ns2:length-Dimension
  ] ;
  ns2:symbol "l" ;
  ns2:alternativeSymbol "L" ;
  ns2:commonlyHasUnit ns2:metre, ns2:attometre, ns2:centimetre, ns2:decametre, ns2:decimetre, ns2:exametre, ns2:femtometre, ns2:gigametre, ns2:hectometre, ns2:kilometre, ns2:megametre, ns2:micrometre, ns2:millimetre, ns2:nanometre, ns2:petametre, ns2:picometre, ns2:terametre, ns2:angstrom, ns2:chain, ns2:fathom-USSurvey, ns2:fermi, ns2:foot-International, ns2:foot-USSurvey, ns2:furlong-International, ns2:inch-International, ns2:micron, ns2:mil-Length, ns2:mile-Statute, ns2:mile-USSurvey, ns2:nauticalMile-International, ns2:rod-US, ns2:yard-International, ns2:astronomicalUnit, ns2:lightYear, ns2:parsec, ns2:solarRadius, ns2:gigaparsec, ns2:kiloparsec, ns2:megaparsec, ns2:cicero, ns2:pica-ATA, ns2:pica-Postscript, ns2:pica-TeX, ns2:point-ATA, ns2:point-Didot, ns2:point-Postscript, ns2:point-TeX .

ns2:Breadth
  a owl:Class ;
  rdfs:label "breadth"@en, "breedte"@nl ;
  rdfs:subClassOf ns2:Length ;
  ns2:symbol "b" ;
  ns2:commonlyHasUnit ns2:metre, ns2:attometre, ns2:centimetre, ns2:decametre, ns2:decimetre, ns2:exametre, ns2:femtometre, ns2:gigametre, ns2:hectometre, ns2:kilometre, ns2:megametre, ns2:micrometre, ns2:millimetre, ns2:nanometre, ns2:petametre, ns2:picometre, ns2:terametre, ns2:angstrom, ns2:chain, ns2:fathom-USSurvey, ns2:fermi, ns2:foot-International, ns2:foot-USSurvey, ns2:furlong-International, ns2:inch-International, ns2:micron, ns2:mil-Length, ns2:mile-Statute, ns2:mile-USSurvey, ns2:nauticalMile-International, ns2:rod-US, ns2:yard-International, ns2:astronomicalUnit, ns2:lightYear, ns2:parsec, ns2:solarRadius, ns2:gigaparsec, ns2:kiloparsec, ns2:megaparsec, ns2:cicero, ns2:pica-ATA, ns2:pica-Postscript, ns2:pica-TeX, ns2:point-ATA, ns2:point-Didot, ns2:point-Postscript, ns2:point-TeX .

ns2:Depth
  a owl:Class ;
  rdfs:label "depth"@en, "diepte"@nl ;
  rdfs:subClassOf ns2:Length ;
  ns2:symbol "d" ;
  ns2:commonlyHasUnit ns2:metre, ns2:attometre, ns2:centimetre, ns2:decametre, ns2:decimetre, ns2:exametre, ns2:femtometre, ns2:gigametre, ns2:hectometre, ns2:kilometre, ns2:megametre, ns2:micrometre, ns2:millimetre, ns2:nanometre, ns2:petametre, ns2:picometre, ns2:terametre, ns2:angstrom, ns2:chain, ns2:fathom-USSurvey, ns2:fermi, ns2:foot-International, ns2:foot-USSurvey, ns2:furlong-International, ns2:inch-International, ns2:micron, ns2:mil-Length, ns2:mile-Statute, ns2:mile-USSurvey, ns2:nauticalMile-International, ns2:rod-US, ns2:yard-International, ns2:astronomicalUnit, ns2:lightYear, ns2:parsec, ns2:solarRadius, ns2:gigaparsec, ns2:kiloparsec, ns2:megaparsec, ns2:cicero, ns2:pica-ATA, ns2:pica-Postscript, ns2:pica-TeX, ns2:point-ATA, ns2:point-Didot, ns2:point-Postscript, ns2:point-TeX .

ns2:Distance
  a owl:Class ;
  rdfs:label "distance"@en, "afstand"@nl, "距离"@zh ;
  rdfs:subClassOf ns2:Length ;
  ns2:symbol "d" ;
  ns2:commonlyHasUnit ns2:metre, ns2:attometre, ns2:centimetre, ns2:decametre, ns2:decimetre, ns2:exametre, ns2:femtometre, ns2:gigametre, ns2:hectometre, ns2:kilometre, ns2:megametre, ns2:micrometre, ns2:millimetre, ns2:nanometre, ns2:petametre, ns2:picometre, ns2:terametre, ns2:angstrom, ns2:chain, ns2:fathom-USSurvey, ns2:fermi, ns2:foot-International, ns2:foot-USSurvey, ns2:furlong-International, ns2:inch-International, ns2:micron, ns2:mil-Length, ns2:mile-Statute, ns2:mile-USSurvey, ns2:nauticalMile-International, ns2:rod-US, ns2:yard-International, ns2:astronomicalUnit, ns2:lightYear, ns2:parsec, ns2:solarRadius, ns2:gigaparsec, ns2:kiloparsec, ns2:megaparsec, ns2:cicero, ns2:pica-ATA, ns2:pica-Postscript, ns2:pica-TeX, ns2:point-ATA, ns2:point-Didot, ns2:point-Postscript, ns2:point-TeX .

ns2:Height
  a owl:Class ;
  rdfs:label "height"@en, "hoogte"@nl ;
  rdfs:subClassOf ns2:Length ;
  ns2:symbol "h" ;
  ns2:commonlyHasUnit ns2:metre, ns2:attometre, ns2:centimetre, ns2:decametre, ns2:decimetre, ns2:exametre, ns2:femtometre, ns2:gigametre, ns2:hectometre, ns2:kilometre, ns2:megametre, ns2:micrometre, ns2:millimetre, ns2:nanometre, ns2:petametre, ns2:picometre, ns2:terametre, ns2:angstrom, ns2:chain, ns2:fathom-USSurvey, ns2:fermi, ns2:foot-International, ns2:foot-USSurvey, ns2:furlong-International, ns2:inch-International, ns2:micron, ns2:mil-Length, ns2:mile-Statute, ns2:mile-USSurvey, ns2:nauticalMile-International, ns2:rod-US, ns2:yard-International, ns2:astronomicalUnit, ns2:lightYear, ns2:parsec, ns2:solarRadius, ns2:gigaparsec, ns2:kiloparsec, ns2:megaparsec, ns2:cicero, ns2:pica-ATA, ns2:pica-Postscript, ns2:pica-TeX, ns2:point-ATA, ns2:point-Didot, ns2:point-Postscript, ns2:point-TeX .

ns2:Thickness
  a owl:Class ;
  rdfs:label "thickness"@en, "dikte"@nl ;
  rdfs:subClassOf ns2:Length ;
  ns2:symbol "d" ;
  ns2:alternativeSymbol "δ" ;
  ns2:commonlyHasUnit ns2:metre, ns2:attometre, ns2:centimetre, ns2:decametre, ns2:decimetre, ns2:exametre, ns2:femtometre, ns2:gigametre, ns2:hectometre, ns2:kilometre, ns2:megametre, ns2:micrometre, ns2:millimetre, ns2:nanometre, ns2:petametre, ns2:picometre, ns2:terametre, ns2:angstrom, ns2:chain, ns2:fathom-USSurvey, ns2:fermi, ns2:foot-International, ns2:foot-USSurvey, ns2:furlong-International, ns2:inch-International, ns2:micron, ns2:mil-Length, ns2:mile-Statute, ns2:mile-USSurvey, ns2:nauticalMile-International, ns2:rod-US, ns2:yard-International, ns2:astronomicalUnit, ns2:lightYear, ns2:parsec, ns2:solarRadius, ns2:gigaparsec, ns2:kiloparsec, ns2:megaparsec, ns2:cicero, ns2:pica-ATA, ns2:pica-Postscript, ns2:pica-TeX, ns2:point-ATA, ns2:point-Didot, ns2:point-Postscript, ns2:point-TeX .

ns2:Width
  a owl:Class ;
  rdfs:label "width"@en, "breedte"@nl ;
  rdfs:subClassOf ns2:Length ;
  ns2:symbol "w" ;
  ns2:commonlyHasUnit ns2:metre, ns2:attometre, ns2:centimetre, ns2:decametre, ns2:decimetre, ns2:exametre, ns2:femtometre, ns2:gigametre, ns2:hectometre, ns2:kilometre, ns2:megametre, ns2:micrometre, ns2:millimetre, ns2:nanometre, ns2:petametre, ns2:picometre, ns2:terametre, ns2:angstrom, ns2:chain, ns2:fathom-USSurvey, ns2:fermi, ns2:foot-International, ns2:foot-USSurvey, ns2:furlong-International, ns2:inch-International, ns2:micron, ns2:mil-Length, ns2:mile-Statute, ns2:mile-USSurvey, ns2:nauticalMile-International, ns2:rod-US, ns2:yard-International, ns2:astronomicalUnit, ns2:lightYear, ns2:parsec, ns2:solarRadius, ns2:gigaparsec, ns2:kiloparsec, ns2:megaparsec, ns2:cicero, ns2:pica-ATA, ns2:pica-Postscript, ns2:pica-TeX, ns2:point-ATA, ns2:point-Didot, ns2:point-Postscript, ns2:point-TeX .

ns2:Radius
  a owl:Class ;
  rdfs:label "radius"@en, "straal"@nl, "半径"@zh ;
  ns2:alternativeLabel "radius"@nl ;
  rdfs:subClassOf ns2:Length ;
  ns2:symbol "r" ;
  ns2:commonlyHasUnit ns2:metre, ns2:attometre, ns2:centimetre, ns2:decametre, ns2:decimetre, ns2:exametre, ns2:femtometre, ns2:gigametre, ns2:hectometre, ns2:kilometre, ns2:megametre, ns2:micrometre, ns2:millimetre, ns2:nanometre, ns2:petametre, ns2:picometre, ns2:terametre, ns2:angstrom, ns2:chain, ns2:fathom-USSurvey, ns2:fermi, ns2:foot-International, ns2:foot-USSurvey, ns2:furlong-International, ns2:inch-International, ns2:micron, ns2:mil-Length, ns2:mile-Statute, ns2:mile-USSurvey, ns2:nauticalMile-International, ns2:rod-US, ns2:yard-International, ns2:astronomicalUnit, ns2:lightYear, ns2:parsec, ns2:solarRadius, ns2:gigaparsec, ns2:kiloparsec, ns2:megaparsec, ns2:cicero, ns2:pica-ATA, ns2:pica-Postscript, ns2:pica-TeX, ns2:point-ATA, ns2:point-Didot, ns2:point-Postscript, ns2:point-TeX .

ns2:Diameter
  a owl:Class ;
  rdfs:label "diameter"@en, "diameter"@nl, "直径"@zh ;
  rdfs:subClassOf ns2:Length ;
  ns2:symbol "d" ;
  ns2:commonlyHasUnit ns2:metre, ns2:attometre, ns2:centimetre, ns2:decametre, ns2:decimetre, ns2:exametre, ns2:femtometre, ns2:gigametre, ns2:hectometre, ns2:kilometre, ns2:megametre, ns2:micrometre, ns2:millimetre, ns2:nanometre, ns2:petametre, ns2:picometre, ns2:terametre, ns2:angstrom, ns2:chain, ns2:fathom-USSurvey, ns2:fermi, ns2:foot-International, ns2:foot-USSurvey, ns2:furlong-International, ns2:inch-International, ns2:micron, ns2:mil-Length, ns2:mile-Statute, ns2:mile-USSurvey, ns2:nauticalMile-International, ns2:rod-US, ns2:yard-International, ns2:astronomicalUnit, ns2:lightYear, ns2:parsec, ns2:solarRadius, ns2:gigaparsec, ns2:kiloparsec, ns2:megaparsec, ns2:cicero, ns2:pica-ATA, ns2:pica-Postscript, ns2:pica-TeX, ns2:point-ATA, ns2:point-Didot, ns2:point-Postscript, ns2:point-TeX .

ns2:Circumference
  a owl:Class ;
  rdfs:label "circumference"@en, "omtrek"@nl, "圆周"@zh ;
  rdfs:subClassOf ns2:Length ;
  ns2:symbol "C" ;
  ns2:commonlyHasUnit ns2:metre, ns2:attometre, ns2:centimetre, ns2:decametre, ns2:decimetre, ns2:exametre, ns2:femtometre, ns2:gigametre, ns2:hectometre, ns2:kilometre, ns2:megametre, ns2:micrometre, ns2:millimetre, ns2:nanometre, ns2:petametre, ns2:picometre, ns2:terametre, ns2:angstrom, ns2:chain, ns2:fathom-USSurvey, ns2:fermi, ns2:foot-International, ns2:foot-USSurvey, ns2:furlong-International, ns2:inch-International, ns2:micron, ns2:mil-Length, ns2:mile-Statute, ns2:mile-USSurvey, ns2:nauticalMile-International, ns2:rod-US, ns2:yard-International, ns2:astronomicalUnit, ns2:lightYear, ns2:parsec, ns2:solarRadius, ns2:gigaparsec, ns2:kiloparsec, ns2:megaparsec, ns2:cicero, ns2:pica-ATA, ns2:pica-Postscript, ns2:pica-TeX, ns2:point-ATA, ns2:point-Didot, ns2:point-Postscript, ns2:point-TeX .

ns2:Area
  a owl:Class ;
  rdfs:label "area"@en, "oppervlakte"@nl, "面积"@zh ;
  ns2:alternativeLabel "oppervlak"@nl ;
  rdfs:comment "Area expresses the two-dimensional size of a defined part of a surface, typically a region bounded by a closed curve. It is a derived quantity in the International System of Units. Area is length squared."@en ;
  rdfs:subClassOf ns2:Quantity, [
    a owl:Restriction ;
    owl:onProperty ns2:hasValue ;
    owl:allValuesFrom [
      a owl:Restriction ;
      owl:onProperty ns2:hasUnit ;
      owl:allValuesFrom ns2:AreaUnit
    ]
  ], [
    a owl:Restriction ;
    owl:onProperty ns2:hasDimension ;
    owl:hasValue ns2:area-Dimension
  ] ;
  ns2:symbol "A" ;
  ns2:alternativeSymbol "S" ;
  ns2:commonlyHasUnit ns2:squareMetre, ns2:squareAttometre, ns2:squareCentimetre, ns2:squareDecametre, ns2:squareDecimetre, ns2:squareExametre, ns2:squareFemtometre, ns2:squareGigametre, ns2:squareHectometre, ns2:squareKilometre, ns2:squareMegametre, ns2:squareMicrometre, ns2:squareMillimetre, ns2:squareNanometre, ns2:squarePetametre, ns2:squarePicometre, ns2:squareTerametre, ns2:are, ns2:centiare, ns2:hectare, ns2:acre-International, ns2:acre-USSurvey, ns2:barn, ns2:circularMil, ns2:squareInch-International, ns2:squareFoot-International, ns2:squareYard-International, ns2:squareMile-International .

ns2:Volume
  a owl:Class ;
  rdfs:label "volume"@en, "volume"@nl, "体积"@zh ;
  ns2:alternativeLabel "inhoud"@nl ;
  rdfs:comment "Volume is a measure of how much three-dimensional space any phenomenon occupies. It is a derived quantity in the International System of Units. Volume is length to the power 3."@en ;
  rdfs:subClassOf ns2:Quantity, [
    a owl:Restriction ;
    owl:onProperty ns2:hasValue ;
    owl:allValuesFrom [
      a owl:Restriction ;
      owl:onProperty ns2:hasUnit ;
      owl:allValuesFrom ns2:VolumeUnit
    ]
  ], [
    a owl:Restriction ;
    owl:onProperty ns2:hasDimension ;
    owl:hasValue ns2:volume-Dimension
  ] ;
  ns2:symbol "V" ;
  ns2:alternativeSymbol "v" ;
  ns2:commonlyHasUnit ns2:cubicMetre, ns2:cubicAttometre, ns2:cubicCentimetre, ns2:cubicDecametre, ns2:cubicDecimetre, ns2:cubicExametre, ns2:cubicFemtometre, ns2:cubicGigametre, ns2:cubicHectometre, ns2:cubicKilometre, ns2:cubicMegametre, ns2:cubicMicrometre, ns2:cubicMillimetre, ns2:cubicNanometre, ns2:cubicPetametre, ns2:cubicPicometre, ns2:cubicTerametre, ns2:litre, ns2:attolitre, ns2:centilitre, ns2:decalitre, ns2:decilitre, ns2:exalitre, ns2:femtolitre, ns2:gigalitre, ns2:hectolitre, ns2:kilolitre, ns2:megalitre, ns2:microlitre, ns2:millilitre, ns2:nanolitre, ns2:petalitre, ns2:picolitre, ns2:teralitre, ns2:acreFoot, ns2:barrel-US, ns2:bushel-US, ns2:cord, ns2:cup-USCustomary, ns2:dryGallon-US, ns2:dryPint-US, ns2:dryQuart-US, ns2:fluidOunce-Imperial, ns2:fluidOunce-US, ns2:gallon-Imperial, ns2:gallon-US, ns2:gill-Imperial, ns2:gill-US, ns2:liquidPint-US, ns2:liquidQuart-US, ns2:peck-US, ns2:pint-Imperial, ns2:quart-Imperial, ns2:stere, ns2:tablespoon-US, ns2:teaspoon-US, ns2:dessertspoon, ns2:ton-Register, ns2:cubicParsec, ns2:cubicKiloparsec .

ns2:Angle
  a owl:Class ;
  rdfs:label "angle"@en, "hoek"@nl, "角度"@zh ;
  ns2:alternativeLabel "plane angle"@en ;
  rdfs:comment "Angle is the ratio between an arc and its radius."@en ;
  rdfs:subClassOf ns2:Quantity, [
    a owl:Restriction ;
    owl:onProperty ns2:hasValue ;
    owl:allValuesFrom [
      a owl:Restriction ;
      owl:onProperty ns2:hasUnit ;
      owl:allValuesFrom ns2:AngleUnit
    ]
  ], [
    a owl:Restriction ;
    owl:onProperty ns2:hasDimension ;
    owl:hasValue ns2:dimensionOne
  ] ;
  ns2:symbol "α" ;
  ns2:alternativeSymbol "β", "γ", "θ", "φ" ;
  ns2:commonlyHasUnit ns2:metrePerMetre, ns2:radian, ns2:attoradian, ns2:centiradian, ns2:deciradian, ns2:femtoradian, ns2:microradian, ns2:milliradian, ns2:nanoradian, ns2:picoradian, ns2:degree, ns2:gon, ns2:mil-Angle, ns2:minute-Angle, ns2:revolution, ns2:second-Angle, ns2:millisecond-Angle, ns2:microsecond-Angle .

ns2:SolidAngle
  a owl:Class ;
  rdfs:label "solid angle"@en, "ruimtehoek"@nl, "立体角"@zh ;
  rdfs:comment "Solid angle is the ratio of the surface of a portion of a sphere enclosed by the conical surface that forms an angle to the square of the radius of the sphere."@en ;
  rdfs:subClassOf ns2:Quantity, [
    a owl:Restriction ;
    owl:onProperty ns2:hasValue ;
    owl:allValuesFrom [
      a owl:Restriction ;
      owl:onProperty ns2:hasUnit ;
      owl:allValuesFrom ns2:SolidAngleUnit
    ]
  ], [
    a owl:Restriction ;
    owl:onProperty ns2:hasDimension ;
    owl:hasValue ns2:dimensionOne
  ] ;
  ns2:symbol "Ω" ;
  ns2:alternativeSymbol "ω" ;
  ns2:commonlyHasUnit ns2:squareMetrePerSquareMetre, ns2:steradian, ns2:attosteradian, ns2:centisteradian, ns2:decisteradian, ns2:femtosteradian, ns2:microsteradian, ns2:millisteradian, ns2:nanosteradian, ns2:picosteradian, ns2:degreeSquared, ns2:second-AngleSquared .

ns2:AngularSize
  a owl:Class ;
  rdfs:label "angular size"@en ;
  rdfs:subClassOf ns2:SolidAngle ;
  ns2:commonlyHasUnit ns2:degreeSquared, ns2:second-AngleSquared .

ns2:LengthFraction
  a owl:Class ;
  rdfs:label "length fraction"@en, "lengtefractie"@nl ;
  rdfs:subClassOf ns2:Quantity, [
    a owl:Restriction ;
    owl:onProperty ns2:hasDimension ;
    owl:hasValue ns2:dimensionOne
  ] ;
  ns2:commonlyHasUnit ns2:metrePerMetre, ns2:millimetrePerMetre .

ns2:Slope
  a owl:Class ;
  rdfs:label "slope"@en ;
  rdfs:subClassOf ns2:LengthFraction .

ns2:SIPrefix
  a owl:Class ;
  rdfs:label "SI prefix"@en ;
  rdfs:subClassOf ns2:Prefix .

ns2:yocto
  a ns2:SIPrefix ;
  rdfs:label "yocto"@en, "yocto"@nl ;
  ns2:symbol "y" ;
  ns2:hasFactor "1e-24"^^xsd:float .

ns2:zepto
  a ns2:SIPrefix ;
  rdfs:label "zepto"@en, "zepto"@nl ;
  ns2:symbol "z" ;
  ns2:hasFactor "1e-21"^^xsd:float .

ns2:atto
  a ns2:SIPrefix ;
  rdfs:label "atto"@en, "atto"@nl ;
  ns2:symbol "a" ;
  ns2:hasFactor "1e-18"^^xsd:float .

ns2:femto
  a ns2:SIPrefix ;
  rdfs:label "femto"@en, "femto"@nl ;
  ns2:symbol "f" ;
  ns2:hasFactor "1e-15"^^xsd:float .

ns2:pico
  a ns2:SIPrefix ;
  rdfs:label "pico"@en, "pico"@nl ;
  ns2:symbol "p" ;
  ns2:hasFactor "1e-12"^^xsd:float .

ns2:nano
  a ns2:SIPrefix ;
  rdfs:label "nano"@en, "nano"@nl ;
  ns2:symbol "n" ;
  ns2:hasFactor "1e-9"^^xsd:float .

ns2:micro
  a ns2:SIPrefix ;
  rdfs:label "micro"@en, "micro"@nl ;
  ns2:symbol "μ" ;
  ns2:alternativeSymbol "u" ;
  ns2:hasFactor "1e-6"^^xsd:float .

ns2:milli
  a ns2:SIPrefix ;
  rdfs:label "milli"@en, "milli"@nl ;
  ns2:symbol "m" ;
  ns2:hasFactor "1e-3"^^xsd:float .

ns2:centi
  a ns2:SIPrefix ;
  rdfs:label "centi"@en, "centi"@nl ;
  ns2:symbol "c" ;
  ns2:hasFactor "1e-2"^^xsd:float .

ns2:deci
  a ns2:SIPrefix ;
  rdfs:label "deci"@en, "deci"@nl ;
  ns2:symbol "d" ;
  ns2:hasFactor "1e-1"^^xsd:float .

ns2:deca
  a ns2:SIPrefix ;
  rdfs:label "deca"@en, "deca"@nl ;
  ns2:alternativeLabel "deka"@en ;
  ns2:symbol "da" ;
  ns2:hasFactor "1e1"^^xsd:float .

ns2:hecto
  a ns2:SIPrefix ;
  rdfs:label "hecto"@en, "hecto"@nl ;
  ns2:symbol "h" ;
  ns2:hasFactor "1e2"^^xsd:float .

ns2:kilo
  a ns2:SIPrefix ;
  rdfs:label "kilo"@en, "kilo"@nl ;
  ns2:symbol "k" ;
  ns2:hasFactor "1e3"^^xsd:float .

ns2:mega
  a ns2:SIPrefix ;
  rdfs:label "mega"@en, "mega"@nl ;
  ns2:symbol "M" ;
  ns2:hasFactor "1e6"^^xsd:float .

ns2:giga
  a ns2:SIPrefix ;
  rdfs:label "giga"@en, "giga"@nl ;
  ns2:symbol "G" ;
  ns2:hasFactor "1e9"^^xsd:float .

ns2:tera
  a ns2:SIPrefix ;
  rdfs:label "tera"@en, "tera"@nl ;
  ns2:symbol "T" ;
  ns2:hasFactor "1e12"^^xsd:float .

ns2:peta
  a ns2:SIPrefix ;
  rdfs:label "peta"@en, "peta"@nl ;
  ns2:symbol "P" ;
  ns2:hasFactor "1e15"^^xsd:float .

ns2:exa
  a ns2:SIPrefix ;
  rdfs:label "exa"@en, "exa"@nl ;
  ns2:symbol "E" ;
  ns2:hasFactor "1e18"^^xsd:float .

ns2:zetta
  a ns2:SIPrefix ;
  rdfs:label "zetta"@en, "zetta"@nl ;
  ns2:symbol "Z" ;
  ns2:hasFactor "1e21"^^xsd:float .

ns2:yotta
  a ns2:SIPrefix ;
  rdfs:label "yotta"@en, "yotta"@nl ;
  ns2:symbol "Y" ;
  ns2:hasFactor "1e24"^^xsd:float .

ns2:metre
  a ns2:Unit, ns2:SingularUnit ;
  rdfs:label "metre"@en, "meter"@nl, "米"@zh ;
  ns2:alternativeLabel "meter"@en ;
  ns2:symbol "m" ;
  ns2:hasDimension ns2:length-Dimension ;
  rdfs:comment "The metre is a unit of length defined as the length of the path travelled by light in vacuum during a time interval of 1/299 792 458 of a second."@en ;
  ns2:longcomment "The metre is a unit of length defined as the length of the path travelled by light in vacuum during a time interval of 1/299 792 458 of a second. The metre is a base unit in the International System of Units." ;
  ns2:hasQuantity ns2:lengthOfThePathTravelledByLightInVacuumDuringATimeIntervalOf1299792458OfASecond .

ns2:pathTravelledByLightInVacuumDuringATimeIntervalOf1299792458OfASecond
  a owl:Thing ;
  rdfs:label "path travelled by light in vacuum during a time interval of 1/299 792 458 of a second"@en .

ns2:lengthOfThePathTravelledByLightInVacuumDuringATimeIntervalOf1299792458OfASecond
  a ns2:Length ;
  rdfs:label "length of the path travelled by light in vacuum during a time interval of 1/299 792 458 of a second"@en ;
  ns2:hasPhenomenon ns2:pathTravelledByLightInVacuumDuringATimeIntervalOf1299792458OfASecond .

ns2:LengthUnit
  a owl:Class ;
  rdfs:label "length unit"@en ;
  rdfs:subClassOf ns2:Unit ;
  owl:equivalentClass [
    a owl:Class ;
    owl:unionOf (
     _:genid40
     ns2:PrefixedMetre
   )
  ] .

ns2:angstrom
  a ns2:Unit, ns2:SingularUnit ;
  rdfs:label "ångström"@en, "ångström"@nl ;
  ns2:alternativeLabel "angstrom"@en, "angstrom"@nl ;
  rdfs:comment "The ångström is a unit of length defined as 1.0e-10 metre. The unit is often used for wavelengths of electromagnetic radiation or to express the sizes of atoms and molecules."@en ;
  ns2:symbol "Å" ;
  ns2:hasFactor "1.0e-10"^^xsd:float ;
  ns2:hasUnit ns2:metre ;
  ns2:hasDimension ns2:length-Dimension .

ns2:astronomicalUnit
  a ns2:Unit, ns2:SingularUnit ;
  rdfs:label "astronomical unit"@en ;
  rdfs:comment "The atronomical unit is a unit of length defined as 149 597 870 700 metre (IAU 2012 Resolution)."@en ;
  ns2:symbol "au" ;
  ns2:alternativeSymbol "AU" ;
  ns2:hasFactor "1.495978707e11"^^xsd:float ;
  ns2:hasUnit ns2:metre ;
  ns1:reference ns1:IAU_2012_Resolution_B2 ;
  ns2:hasDimension ns2:length-Dimension .

ns2:BirminghamGauge
  a ns2:Unit, ns2:SingularUnit ;
  rdfs:label "Birmingham gauge"@en ;
  ns2:symbol "G" ;
  ns2:alternativeSymbol "GA" ;
  ns2:hasDimension ns2:length-Dimension .

ns2:chain
  a ns2:Unit, ns2:SingularUnit ;
  rdfs:label "chain"@en ;
  rdfs:comment "The chain is a unit of length defined as 20.1168 metre."@en ;
  ns2:symbol "ch" ;
  ns2:hasFactor "20.1168"^^xsd:float ;
  ns2:hasUnit ns2:metre ;
  ns2:hasDimension ns2:length-Dimension .

ns2:cicero
  a ns2:Unit, ns2:SingularUnit ;
  rdfs:label "cicero"@en, "cicero"@nl ;
  rdfs:comment "The cicero is a unit of length defined as 12 point (Didot)."@en ;
  ns2:hasFactor "12"^^xsd:float ;
  ns2:hasUnit ns2:point-Didot ;
  ns2:hasDimension ns2:length-Dimension .

ns2:fathom-USSurvey
  a ns2:Unit, ns2:SingularUnit ;
  rdfs:label "fathom (US survey)"@en ;
  ns2:alternativeLabel "US survey fathom"@en ;
  rdfs:comment "The US survey fathom is a unit of length defined as 1.828804 metre."@en ;
  ns2:hasFactor "1.828804"^^xsd:float ;
  ns2:hasUnit ns2:metre ;
  ns2:hasDimension ns2:length-Dimension .

ns2:fermi
  a ns2:Unit, ns2:SingularUnit ;
  rdfs:label "fermi"@en, "fermi"@nl ;
  rdfs:comment "The fermi is a unit of length defined as 1.0e-15 metre."@en ;
  ns2:hasFactor "1.0e-15"^^xsd:float ;
  ns2:hasUnit ns2:metre ;
  ns2:hasDimension ns2:length-Dimension .

ns2:foot-International
  a ns2:Unit, ns2:SingularUnit ;
  rdfs:label "foot (international)"@en, "英尺（国际）"@zh ;
  ns2:alternativeLabel "international foot"@en ;
  rdfs:comment "The international foot is a unit of length defined as 3.048e-1 metre."@en ;
  ns2:symbol "ft" ;
  ns2:hasFactor "3.048e-1"^^xsd:float ;
  ns2:hasUnit ns2:metre ;
  ns2:hasDimension ns2:length-Dimension .

ns2:foot-USSurvey
  a ns2:Unit, ns2:SingularUnit ;
  rdfs:label "foot (US survey)"@en ;
  ns2:alternativeLabel "US survey foot"@en ;
  rdfs:comment "The US survey foot is a unit of length defined as 3.048006e-1 metre."@en ;
  ns2:symbol "ft" ;
  ns2:hasFactor "3.048006e-1"^^xsd:float ;
  ns2:hasUnit ns2:metre ;
  ns2:hasDimension ns2:length-Dimension .

ns2:FrenchGauge
  a ns2:Unit, ns2:SingularUnit ;
  rdfs:label "French gauge"@en ;
  ns2:symbol "Fr" ;
  ns2:alternativeSymbol "Fg", "FR", "F", "CH", "Ch" ;
  ns2:hasDimension ns2:length-Dimension .

ns2:furlong-International
  a ns2:Unit, ns2:SingularUnit ;
  rdfs:label "furlong (international)"@en ;
  ns2:alternativeLabel "international furlong"@en ;
  rdfs:comment "The international furlong is a unit of length defined as 201.168 metre."@en ;
  ns2:hasFactor "201.168"^^xsd:float ;
  ns2:hasUnit ns2:metre ;
  ns2:hasDimension ns2:length-Dimension .

ns2:inch-International
  a ns2:Unit, ns2:SingularUnit ;
  rdfs:label "inch (international)"@en, "英寸（国际）"@zh ;
  ns2:alternativeLabel "international inch"@en ;
  rdfs:comment "The international inch is a unit of length defined as 2.54e-2 metre."@en ;
  ns2:symbol "in" ;
  ns2:hasFactor "2.54e-2"^^xsd:float ;
  ns2:hasUnit ns2:metre ;
  ns2:hasDimension ns2:length-Dimension .

ns2:lightYear
  a ns2:Unit, ns2:SingularUnit ;
  rdfs:label "light year"@en, "lichtjaar"@nl ;
  ns2:alternativeLabel "lightyear"@en ;
  rdfs:comment "The light year is a unit of length defined as 9.46073e15 metre."@en ;
  ns2:symbol "ly" ;
  ns2:hasFactor "9.46073e15"^^xsd:float ;
  ns2:hasUnit ns2:metre ;
  ns2:hasDimension ns2:length-Dimension .

ns2:micron
  a ns2:Unit, ns2:SingularUnit ;
  rdfs:label "micron"@en, "micron"@nl ;
  rdfs:comment "The micron is a unit of length defined as 1.0e-6 metre."@en ;
  ns2:symbol "μ" ;
  ns2:hasFactor "1.0e-6"^^xsd:float ;
  ns2:hasUnit ns2:metre ;
  ns2:hasDimension ns2:length-Dimension .

ns2:mil-Length
  a ns2:Unit, ns2:SingularUnit ;
  rdfs:label "mil (length)"@en ;
  ns2:alternativeLabel "thou"@en ;
  rdfs:comment "The mil (length) is a unit of length defined as 2.54e-5 metre."@en ;
  ns2:hasFactor "2.54e-5"^^xsd:float ;
  ns2:hasUnit ns2:metre ;
  ns2:hasDimension ns2:length-Dimension .

ns2:mile-Statute
  a ns2:Unit, ns2:SingularUnit ;
  rdfs:label "mile (statute)"@en ;
  ns2:alternativeLabel "statute mile"@en ;
  rdfs:comment "The statute mile is a unit of length defined as 1.609344e3 metre."@en ;
  ns2:symbol "mi" ;
  ns2:hasFactor "1.609344e3"^^xsd:float ;
  ns2:hasUnit ns2:metre ;
  ns2:hasDimension ns2:length-Dimension .

ns2:mile-USSurvey
  a ns2:Unit, ns2:SingularUnit ;
  rdfs:label "mile (US survey)"@en ;
  ns2:alternativeLabel "US survey mile"@en ;
  rdfs:comment "The US survey mile is a unit of length defined as 1.609347e3 metre."@en ;
  ns2:hasFactor "1.609347e3"^^xsd:float ;
  ns2:hasUnit ns2:metre ;
  ns2:hasDimension ns2:length-Dimension .

ns2:nauticalMile-International
  a ns2:Unit, ns2:SingularUnit ;
  rdfs:label "nautical mile (international)"@en, "zeemijl (internationaal)"@nl, "海里（国际）"@zh ;
  ns2:alternativeLabel "international nautical mile"@en ;
  rdfs:comment "The international nautical mile is a unit of length defined as 1852 metre."@en ;
  ns2:symbol "nmi" ;
  ns2:alternativeSymbol "M", "NM", "nm" ;
  ns2:hasFactor "1852"^^xsd:float ;
  ns2:hasUnit ns2:metre ;
  ns2:hasDimension ns2:length-Dimension .

ns2:parsec
  a ns2:Unit, ns2:SingularUnit ;
  rdfs:label "parsec"@en ;
  rdfs:comment "The parsec is a unit of length defined as 3.08567758149137e16 metre."@en ;
  ns2:symbol "pc" ;
  ns2:hasFactor "3.08567758149137e16"^^xsd:float ;
  ns2:hasUnit ns2:metre ;
  ns2:hasDimension ns2:length-Dimension .

ns2:pica-ATA
  a ns2:Unit, ns2:SingularUnit ;
  rdfs:label "pica (ATA)"@en ;
  ns2:alternativeLabel "ATA pica"@en ;
  rdfs:comment "The ATA pica is a unit of length defined as 12 point (ATA)."@en ;
  ns2:hasFactor "12"^^xsd:float ;
  ns2:hasUnit ns2:point-ATA ;
  ns2:hasDimension ns2:length-Dimension .

ns2:pica-Postscript
  a ns2:Unit, ns2:SingularUnit ;
  rdfs:label "pica (Postscript)"@en ;
  ns2:alternativeLabel "Postscript pica"@en ;
  rdfs:comment "The Postscript pica is a unit of length defined as 12 point (Postscript)."@en ;
  ns2:hasFactor "12"^^xsd:float ;
  ns2:hasUnit ns2:point-Postscript ;
  ns2:hasDimension ns2:length-Dimension .

ns2:pica-TeX
  a ns2:Unit, ns2:SingularUnit ;
  rdfs:label "pica (TeX)"@en ;
  ns2:alternativeLabel "TeX pica"@en ;
  rdfs:comment "The TeX pica is a unit of length defined as 12 point (TeX)."@en ;
  ns2:hasFactor "12"^^xsd:float ;
  ns2:hasUnit ns2:point-TeX ;
  ns2:hasDimension ns2:length-Dimension .

ns2:point-ATA
  a ns2:Unit, ns2:SingularUnit ;
  rdfs:label "point (ATA)"@en ;
  ns2:alternativeLabel "ATA point"@en ;
  rdfs:comment "The ATA point is a unit of length defined as 0.3514598e-3 metre."@en ;
  ns2:symbol "pt" ;
  ns2:hasFactor "0.3514598e-3"^^xsd:float ;
  ns2:hasUnit ns2:metre ;
  ns2:hasDimension ns2:length-Dimension .

ns2:point-Didot
  a ns2:Unit, ns2:SingularUnit ;
  rdfs:label "point (Didot)"@en ;
  ns2:alternativeLabel "Didot point"@en ;
  rdfs:comment "The Didot point is a unit of length defined as 0.3759e-3 metre."@en ;
  ns2:symbol "pt" ;
  ns2:hasFactor "0.3759e-3"^^xsd:float ;
  ns2:hasUnit ns2:metre ;
  ns2:hasDimension ns2:length-Dimension .

ns2:point-Postscript
  a ns2:Unit, ns2:SingularUnit ;
  rdfs:label "point (Postscript)"@en ;
  ns2:alternativeLabel "Postscript point"@en ;
  rdfs:comment "The Postscript point is a unit of length defined as 0.013888888888888888888888888888889 inch."@en ;
  ns2:symbol "pt" ;
  ns2:hasFactor "0.013888888888888888888888888888889"^^xsd:float ;
  ns2:hasUnit ns2:inch-International ;
  ns2:hasDimension ns2:length-Dimension .

ns2:point-TeX
  a ns2:Unit, ns2:SingularUnit ;
  rdfs:label "point (TeX)"@en ;
  ns2:alternativeLabel "TeX point"@en ;
  rdfs:comment "The TeX point is a unit of length defined as 0.01383700013837000138370001383 inch."@en ;
  ns2:symbol "pt" ;
  ns2:hasFactor "0.013837000138370001383700013837"^^xsd:float ;
  ns2:hasUnit ns2:inch-International ;
  ns2:hasDimension ns2:length-Dimension .

ns2:rod-US
  a ns2:Unit, ns2:SingularUnit ;
  rdfs:label "rod (US)"@en ;
  ns2:alternativeLabel "US rod"@en, "perch"@en, "pole"@en ;
  rdfs:comment "The US rod is a unit of length defined as 5.029210 metre."@en ;
  ns2:symbol "rd" ;
  ns2:hasFactor "5.029210"^^xsd:float ;
  ns2:hasUnit ns2:metre ;
  ns2:hasDimension ns2:length-Dimension .

ns2:solarRadius
  a ns2:Unit, ns2:SingularUnit ;
  rdfs:label "solar radius"@en ;
  rdfs:comment "Solar radius is a unit used in astronomy to denote stellar or stellar system radii (http://en.wikipedia.org/wiki/solarRadius)."@en ;
  ns2:symbol "R_☉" ;
  ns2:LaTeXSymbol "R_{\\astrosun}" ;
  ns2:hasFactor "6.955e8"^^xsd:float ;
  ns2:hasUnit ns2:metre ;
  ns2:hasDimension ns2:length-Dimension .

ns2:yard-International
  a ns2:Unit, ns2:SingularUnit ;
  rdfs:label "yard (international)"@en, "码（国际）"@zh ;
  ns2:alternativeLabel "international yard"@en ;
  rdfs:comment "The international yard is a unit of length defined as 9.144e-1 metre."@en ;
  ns2:symbol "yd" ;
  ns2:hasFactor "9.144e-1"^^xsd:float ;
  ns2:hasUnit ns2:metre ;
  ns2:hasDimension ns2:length-Dimension .

ns2:gigaparsec
  a ns2:PrefixedUnit ;
  rdfs:label "gigaparsec"@en, "gigaparsec"@nl ;
  rdfs:comment "The gigaparsec is a unit of length defined as 1.0e9 parsec. Gebruikt voor de afstand op de schaal van het heelal."@en ;
  ns2:symbol "Gpc" ;
  ns2:hasPrefix ns2:giga ;
  ns2:hasUnit ns2:parsec ;
  ns2:hasDimension ns2:length-Dimension .

ns2:kiloparsec
  a ns2:PrefixedUnit ;
  rdfs:label "kiloparsec"@en, "kiloparsec"@nl ;
  rdfs:comment "The kiloparsec is a unit of length defined as 1.0e3 parsec. Gebruikt voor afstanden op de schaal van het melkwegstelsel."@en ;
  ns2:symbol "kpc" ;
  ns2:hasPrefix ns2:kilo ;
  ns2:hasUnit ns2:parsec ;
  ns2:hasDimension ns2:length-Dimension .

ns2:megaparsec
  a ns2:PrefixedUnit ;
  rdfs:label "megaparsec"@en, "megaparsec"@nl ;
  rdfs:comment "The megaparsec is a unit of length defined as 1.0e6 parsec. Gebruikt voor afstanden op de schaal van clusters."@en ;
  ns2:symbol "Mpc" ;
  ns2:hasPrefix ns2:mega ;
  ns2:hasUnit ns2:parsec ;
  ns2:hasDimension ns2:length-Dimension .

ns2:PrefixedMetre
  a owl:Class ;
  rdfs:label "prefixed metre"@en ;
  rdfs:subClassOf ns2:PrefixedUnit ;
  owl:equivalentClass [
    a owl:Class ;
    owl:intersectionOf (
     _:genid79
     _:genid81
     _:genid83
     _:genid85
   )
  ] .

ns2:yoctometre
  a ns2:PrefixedUnit ;
  rdfs:label "yoctometre"@en, "yoctometer"@nl ;
  rdfs:comment "The yoctometre is a unit of length defined as 1.0e-24 metre."@en ;
  ns2:symbol "ym" ;
  ns2:hasPrefix ns2:yocto ;
  ns2:hasUnit ns2:metre ;
  ns2:hasDimension ns2:length-Dimension .

ns2:zeptometre
  a ns2:PrefixedUnit ;
  rdfs:label "zeptometre"@en, "zeptometer"@nl ;
  rdfs:comment "The zeptometre is a unit of length defined as 1.0e-21 metre."@en ;
  ns2:symbol "zm" ;
  ns2:hasPrefix ns2:zepto ;
  ns2:hasUnit ns2:metre ;
  ns2:hasDimension ns2:length-Dimension .

ns2:attometre
  a ns2:PrefixedUnit ;
  rdfs:label "attometre"@en, "attometer"@nl ;
  rdfs:comment "The attometre is a unit of length defined as 1.0e-18 metre."@en ;
  ns2:symbol "am" ;
  ns2:hasPrefix ns2:atto ;
  ns2:hasUnit ns2:metre ;
  ns2:hasDimension ns2:length-Dimension .

ns2:femtometre
  a ns2:PrefixedUnit ;
  rdfs:label "femtometre"@en, "femtometer"@nl, "1/(10^15)米"@zh ;
  rdfs:comment "The femtometre is a unit of length defined as 1.0e-15 metre."@en ;
  ns2:symbol "fm" ;
  ns2:hasPrefix ns2:femto ;
  ns2:hasUnit ns2:metre ;
  ns2:hasDimension ns2:length-Dimension .

ns2:picometre
  a ns2:PrefixedUnit ;
  rdfs:label "picometre"@en, "picometer"@nl, "1/(10^12)米"@zh ;
  rdfs:comment "The picometre is a unit of length defined as 1.0e-12 metre."@en ;
  ns2:symbol "pm" ;
  ns2:hasPrefix ns2:pico ;
  ns2:hasUnit ns2:metre ;
  ns2:hasDimension ns2:length-Dimension .

ns2:nanometre
  a ns2:PrefixedUnit ;
  rdfs:label "nanometre"@en, "nanometer"@nl ;
  rdfs:comment "The nanometre is a unit of length defined as 1.0e-9 metre."@en ;
  ns2:symbol "nm" ;
  ns2:hasPrefix ns2:nano ;
  ns2:hasUnit ns2:metre ;
  ns2:hasDimension ns2:length-Dimension .

ns2:micrometre
  a ns2:PrefixedUnit ;
  rdfs:label "micrometre"@en, "micrometer"@nl, "微米"@zh ;
  rdfs:comment "The micrometre is a unit of length defined as 1.0e-6 metre."@en ;
  ns2:symbol "μm" ;
  ns2:hasPrefix ns2:micro ;
  ns2:hasUnit ns2:metre ;
  ns2:hasDimension ns2:length-Dimension .

ns2:millimetre
  a ns2:PrefixedUnit ;
  rdfs:label "millimetre"@en, "millimeter"@nl, "毫米"@zh ;
  rdfs:comment "The millimetre is a unit of length defined as 1.0e-3 metre."@en ;
  ns2:symbol "mm" ;
  ns2:hasPrefix ns2:milli ;
  ns2:hasUnit ns2:metre ;
  ns2:hasDimension ns2:length-Dimension .

ns2:centimetre
  a ns2:PrefixedUnit ;
  rdfs:label "centimetre"@en, "centimeter"@nl ;
  rdfs:comment "The centimetre is a unit of length defined as 1.0e-2 metre."@en ;
  ns2:symbol "cm" ;
  ns2:hasPrefix ns2:centi ;
  ns2:hasUnit ns2:metre ;
  ns2:hasDimension ns2:length-Dimension .

ns2:decimetre
  a ns2:PrefixedUnit ;
  rdfs:label "decimetre"@en, "decimeter"@nl ;
  rdfs:comment "The decimetre is a unit of length defined as 1.0e-1 metre."@en ;
  ns2:symbol "dm" ;
  ns2:hasPrefix ns2:deci ;
  ns2:hasUnit ns2:metre ;
  ns2:hasDimension ns2:length-Dimension .

ns2:decametre
  a ns2:PrefixedUnit ;
  rdfs:label "decametre"@en, "decameter"@nl ;
  rdfs:comment "The decametre is a unit of length defined as 1.0e1 metre."@en ;
  ns2:symbol "dam" ;
  ns2:hasPrefix ns2:deca ;
  ns2:hasUnit ns2:metre ;
  ns2:hasDimension ns2:length-Dimension .

ns2:hectometre
  a ns2:PrefixedUnit ;
  rdfs:label "hectometre"@en, "hectometer"@nl ;
  rdfs:comment "The hectometre is a unit of length defined as 1.0e2 metre."@en ;
  ns2:symbol "hm" ;
  ns2:hasPrefix ns2:hecto ;
  ns2:hasUnit ns2:metre ;
  ns2:hasDimension ns2:length-Dimension .

ns2:kilometre
  a ns2:PrefixedUnit ;
  rdfs:label "kilometre"@en, "kilometer"@nl, "公里"@zh ;
  rdfs:comment "The kilometre is a unit of length defined as 1.0e3 metre."@en ;
  ns2:symbol "km" ;
  ns2:hasPrefix ns2:kilo ;
  ns2:hasUnit ns2:metre ;
  ns2:hasDimension ns2:length-Dimension .

ns2:megametre
  a ns2:PrefixedUnit ;
  rdfs:label "megametre"@en, "megameter"@nl, "百万米"@zh ;
  rdfs:comment "The megametre is a unit of length defined as 1.0e6 metre."@en ;
  ns2:symbol "Mm" ;
  ns2:hasPrefix ns2:mega ;
  ns2:hasUnit ns2:metre ;
  ns2:hasDimension ns2:length-Dimension .

ns2:gigametre
  a ns2:PrefixedUnit ;
  rdfs:label "gigametre"@en, "gigameter"@nl, "10^9米"@zh ;
  rdfs:comment "The gigametre is a unit of length defined as 1.0e9 metre."@en ;
  ns2:symbol "Gm" ;
  ns2:hasPrefix ns2:giga ;
  ns2:hasUnit ns2:metre ;
  ns2:hasDimension ns2:length-Dimension .

ns2:terametre
  a ns2:PrefixedUnit ;
  rdfs:label "terametre"@en, "terameter"@nl, "10^12米"@zh ;
  rdfs:comment "The terametre is a unit of length defined as 1.0e12 metre."@en ;
  ns2:unofficialAbbreviation "10^9 km" ;
  ns2:symbol "Tm" ;
  ns2:hasPrefix ns2:tera ;
  ns2:hasUnit ns2:metre ;
  ns2:hasDimension ns2:length-Dimension .

ns2:petametre
  a ns2:PrefixedUnit ;
  rdfs:label "petametre"@en, "petameter"@nl, "10^15米"@zh ;
  rdfs:comment "The petametre is a unit of length defined as 1.0e15 metre."@en ;
  ns2:symbol "Pm" ;
  ns2:hasPrefix ns2:peta ;
  ns2:hasUnit ns2:metre ;
  ns2:hasDimension ns2:length-Dimension .

ns2:exametre
  a ns2:PrefixedUnit ;
  rdfs:label "exametre"@en, "exameter"@nl, "千兆兆米"@zh ;
  rdfs:comment "The exametre is a unit of length defined as 1.0e18 metre."@en ;
  ns2:symbol "Em" ;
  ns2:hasPrefix ns2:exa ;
  ns2:hasUnit ns2:metre ;
  ns2:hasDimension ns2:length-Dimension .

ns2:zettametre
  a ns2:PrefixedUnit ;
  rdfs:label "zettametre"@en, "zettameter"@nl ;
  rdfs:comment "The zettametre is a unit of length defined as 1.0e21 metre."@en ;
  ns2:symbol "Zm" ;
  ns2:hasPrefix ns2:zetta ;
  ns2:hasUnit ns2:metre ;
  ns2:hasDimension ns2:length-Dimension .

ns2:yottametre
  a ns2:PrefixedUnit ;
  rdfs:label "yottametre"@en, "yottameter"@nl, "10^24米"@zh ;
  rdfs:comment "The yottametre is a unit of length defined as 1.0e24 metre."@en ;
  ns2:symbol "Ym" ;
  ns2:hasPrefix ns2:yotta ;
  ns2:hasUnit ns2:metre ;
  ns2:hasDimension ns2:length-Dimension .

ns2:squareMetre
  a ns2:UnitExponentiation ;
  rdfs:label "square metre"@en, "vierkante meter"@nl, "平方米"@zh ;
  rdfs:comment "Square metre is a unit of area defined as the area of a square whose sides measure exactly one metre."@en ;
  ns2:longcomment "Square metre is a unit of area defined as the area of a square whose sides measure exactly one metre. Square metre is a derived unit in the International System of Units." ;
  ns2:symbol "m2" ;
  ns2:hasBase ns2:metre ;
  ns2:hasExponent 2 ;
  ns2:hasDimension ns2:area-Dimension .

ns2:AreaUnit
  a owl:Class ;
  rdfs:label "area unit"@en ;
  rdfs:subClassOf ns2:Unit ;
  owl:equivalentClass [
    a owl:Class ;
    owl:unionOf (
     _:genid88
     ns2:PrefixedAre
     ns2:SquarePrefixedMetre
   )
  ] .

ns2:acre-International
  a ns2:Unit, ns2:SingularUnit ;
  rdfs:label "acre (international)"@en, "英亩（国际）"@zh ;
  ns2:alternativeLabel "international acre"@en ;
  rdfs:comment "The international acre is a unit of area defined as 4.0468564224e3 square metre."@en ;
  ns2:symbol "ac" ;
  ns2:hasFactor "4.0468564224e3"^^xsd:float ;
  ns2:hasUnit ns2:squareMetre ;
  ns2:hasDimension ns2:area-Dimension .

ns2:acre-USSurvey
  a ns2:Unit, ns2:SingularUnit ;
  rdfs:label "acre (US survey)"@en, "英亩（美国调查）"@zh ;
  ns2:alternativeLabel "US survey acre"@en ;
  rdfs:comment "The US survey acre is a unit of area defined as 4.046872609874252e3 square metre."@en ;
  ns2:symbol "ac" ;
  ns2:hasFactor "4.046872609874252e3"^^xsd:float ;
  ns2:hasUnit ns2:squareMetre ;
  ns2:hasDimension ns2:area-Dimension .

ns2:are
  a ns2:Unit, ns2:SingularUnit ;
  rdfs:label "are"@en, "are"@nl ;
  rdfs:comment "The are is a unit of area defined as 100 square metre."@en ;
  ns2:symbol "a" ;
  ns2:hasFactor "1.0e2"^^xsd:float ;
  ns2:hasUnit ns2:squareMetre ;
  ns2:hasDimension ns2:area-Dimension .

ns2:barn
  a ns2:Unit, ns2:SingularUnit ;
  rdfs:label "barn"@en ;
  rdfs:comment "The barn is a unit of area defined as 1.0e-28 square metre."@en ;
  ns2:symbol "b" ;
  ns2:hasFactor "1.0e-28"^^xsd:float ;
  ns2:hasUnit ns2:squareMetre ;
  ns2:hasDimension ns2:area-Dimension .

ns2:circularMil
  a ns2:Unit, ns2:SingularUnit ;
  rdfs:label "circular mil"@en ;
  rdfs:comment "The cicular mil is a unit of area defined as 5.067075e-10 square metre."@en ;
  ns2:hasFactor "5.067075e-10"^^xsd:float ;
  ns2:hasUnit ns2:squareMetre ;
  ns2:hasDimension ns2:area-Dimension .

ns2:squareInch-International
  a ns2:UnitExponentiation ;
  rdfs:label "square inch (international)"@en ;
  ns2:symbol "in2" ;
  ns2:hasBase ns2:inch-International ;
  ns2:hasExponent 2 ;
  ns2:hasDimension ns2:area-Dimension .

ns2:squareFoot-International
  a ns2:UnitExponentiation ;
  rdfs:label "square foot (international)"@en ;
  ns2:symbol "ft2" ;
  ns2:hasBase ns2:foot-International ;
  ns2:hasExponent 2 ;
  ns2:hasDimension ns2:area-Dimension .

ns2:squareYard-International
  a ns2:UnitExponentiation ;
  rdfs:label "square yard (international)"@en ;
  ns2:symbol "yd2" ;
  ns2:hasBase ns2:yard-International ;
  ns2:hasExponent 2 ;
  ns2:hasDimension ns2:area-Dimension .

ns2:squareMile-International a ns2:UnitExponentiation .
ns2:PrefixedAre
  a owl:Class ;
  rdfs:label "prefixed are"@en ;
  rdfs:subClassOf ns2:PrefixedUnit ;
  owl:equivalentClass [
    a owl:Class ;
    owl:intersectionOf (
     _:genid114
     _:genid116
     _:genid118
     _:genid120
   )
  ] .

ns2:SquarePrefixedMetre
  a owl:Class ;
  rdfs:label "square prefixed metre"@en ;
  rdfs:subClassOf ns2:UnitExponentiation ;
  owl:equivalentClass [
    a owl:Class ;
    owl:intersectionOf (
     _:genid105
     _:genid107
     _:genid109
     _:genid111
   )
  ] .

ns2:squareYoctometre
  a ns2:SquarePrefixedMetre ;
  rdfs:label "square yoctometre"@en, "vierkante yoctometer"@nl ;
  ns2:symbol "ym2" ;
  ns2:hasBase ns2:yoctometre ;
  ns2:hasExponent 2 ;
  ns2:hasDimension ns2:area-Dimension .

ns2:squareZeptometre
  a ns2:SquarePrefixedMetre ;
  rdfs:label "square zeptometre"@en, "vierkante zeptometer"@nl ;
  ns2:symbol "zm2" ;
  ns2:hasBase ns2:zeptometre ;
  ns2:hasExponent 2 ;
  ns2:hasDimension ns2:area-Dimension .

ns2:squareAttometre
  a ns2:SquarePrefixedMetre ;
  rdfs:label "square attometre"@en, "vierkante attometer"@nl ;
  ns2:symbol "am2" ;
  ns2:hasBase ns2:attometre ;
  ns2:hasExponent 2 ;
  ns2:hasDimension ns2:area-Dimension .

ns2:squareFemtometre
  a ns2:SquarePrefixedMetre ;
  rdfs:label "square femtometre"@en, "vierkante femtometer"@nl ;
  ns2:symbol "fm2" ;
  ns2:hasBase ns2:femtometre ;
  ns2:hasExponent 2 ;
  ns2:hasDimension ns2:area-Dimension .

ns2:squarePicometre
  a ns2:SquarePrefixedMetre ;
  rdfs:label "square picometre"@en, "vierkante picometer"@nl ;
  ns2:symbol "pm2" ;
  ns2:hasBase ns2:picometre ;
  ns2:hasExponent 2 ;
  ns2:hasDimension ns2:area-Dimension .

ns2:squareNanometre
  a ns2:SquarePrefixedMetre ;
  rdfs:label "square nanometre"@en, "vierkante nanometer"@nl ;
  ns2:symbol "nm2" ;
  ns2:hasBase ns2:nanometre ;
  ns2:hasExponent 2 ;
  ns2:hasDimension ns2:area-Dimension .

ns2:squareMicrometre
  a ns2:SquarePrefixedMetre ;
  rdfs:label "square micrometre"@en, "vierkante micrometer"@nl ;
  ns2:symbol "μm2" ;
  ns2:hasBase ns2:micrometre ;
  ns2:hasExponent 2 ;
  ns2:hasDimension ns2:area-Dimension .

ns2:squareMillimetre
  a ns2:SquarePrefixedMetre ;
  rdfs:label "square millimetre"@en, "vierkante millimeter"@nl ;
  ns2:symbol "mm2" ;
  ns2:hasBase ns2:millimetre ;
  ns2:hasExponent 2 ;
  ns2:hasDimension ns2:area-Dimension .

ns2:squareCentimetre
  a ns2:SquarePrefixedMetre ;
  rdfs:label "square centimetre"@en, "vierkante centimeter"@nl ;
  ns2:symbol "cm2" ;
  ns2:hasBase ns2:centimetre ;
  ns2:hasExponent 2 ;
  ns2:hasDimension ns2:area-Dimension .

ns2:squareDecimetre
  a ns2:SquarePrefixedMetre ;
  rdfs:label "square decimetre"@en, "vierkante decimeter"@nl ;
  ns2:symbol "dm2" ;
  ns2:hasBase ns2:decimetre ;
  ns2:hasExponent 2 ;
  ns2:hasDimension ns2:area-Dimension .

ns2:squareDecametre
  a ns2:SquarePrefixedMetre ;
  rdfs:label "square decametre"@en, "vierkante decameter"@nl ;
  ns2:symbol "dam2" ;
  ns2:hasBase ns2:decametre ;
  ns2:hasExponent 2 ;
  ns2:hasDimension ns2:area-Dimension .

ns2:squareHectometre
  a ns2:SquarePrefixedMetre ;
  rdfs:label "square hectometre"@en, "vierkante hectometer"@nl ;
  ns2:symbol "hm2" ;
  ns2:hasBase ns2:hectometre ;
  ns2:hasExponent 2 ;
  ns2:hasDimension ns2:area-Dimension .

ns2:squareKilometre
  a ns2:SquarePrefixedMetre ;
  rdfs:label "square kilometre"@en, "vierkante kilometer"@nl ;
  ns2:unofficialAbbreviation "10^6 m2" ;
  ns2:symbol "km2" ;
  ns2:hasBase ns2:kilometre ;
  ns2:hasExponent 2 ;
  ns2:hasDimension ns2:area-Dimension .

ns2:squareMegametre
  a ns2:SquarePrefixedMetre ;
  rdfs:label "square megametre"@en, "vierkante megameter"@nl ;
  ns2:symbol "Mm2" ;
  ns2:hasBase ns2:megametre ;
  ns2:hasExponent 2 ;
  ns2:hasDimension ns2:area-Dimension .

ns2:squareGigametre
  a ns2:SquarePrefixedMetre ;
  rdfs:label "square gigametre"@en, "vierkante gigameter"@nl ;
  ns2:symbol "Gm2" ;
  ns2:hasBase ns2:gigametre ;
  ns2:hasExponent 2 ;
  ns2:hasDimension ns2:area-Dimension .

ns2:squareTerametre
  a ns2:SquarePrefixedMetre ;
  rdfs:label "square terametre"@en, "vierkante terameter"@nl ;
  ns2:symbol "Tm2" ;
  ns2:hasBase ns2:terametre ;
  ns2:hasExponent 2 ;
  ns2:hasDimension ns2:area-Dimension .

ns2:squarePetametre
  a ns2:SquarePrefixedMetre ;
  rdfs:label "square petametre"@en, "vierkante petameter"@nl ;
  ns2:symbol "Pm2" ;
  ns2:hasBase ns2:petametre ;
  ns2:hasExponent 2 ;
  ns2:hasDimension ns2:area-Dimension .

ns2:squareExametre
  a ns2:SquarePrefixedMetre ;
  rdfs:label "square exametre"@en, "vierkante exameter"@nl ;
  ns2:symbol "Em2" ;
  ns2:hasBase ns2:exametre ;
  ns2:hasExponent 2 ;
  ns2:hasDimension ns2:area-Dimension .

ns2:squareZettametre
  a ns2:SquarePrefixedMetre ;
  rdfs:label "square zettametre"@en, "vierkante zettameter"@nl ;
  ns2:symbol "Zm2" ;
  ns2:hasBase ns2:zettametre ;
  ns2:hasExponent 2 ;
  ns2:hasDimension ns2:area-Dimension .

ns2:squareYottametre
  a ns2:SquarePrefixedMetre ;
  rdfs:label "square yottametre"@en, "vierkante yottameter"@nl ;
  ns2:symbol "Ym2" ;
  ns2:hasBase ns2:yottametre ;
  ns2:hasExponent 2 ;
  ns2:hasDimension ns2:area-Dimension .

ns2:centiare
  a ns2:PrefixedUnit ;
  rdfs:label "centiare"@en, "centiare"@nl ;
  rdfs:comment "The centiare is a unit of area defined as 1.0e-2 are."@en ;
  ns2:symbol "ca" ;
  ns2:hasPrefix ns2:centi ;
  ns2:hasUnit ns2:are ;
  ns2:hasDimension ns2:area-Dimension .

ns2:hectare
  a ns2:PrefixedUnit ;
  rdfs:label "hectare"@en, "hectare"@nl ;
  rdfs:comment "The hectare is a unit of area defined as 1.0e2 are."@en ;
  ns2:symbol "ha" ;
  ns2:hasPrefix ns2:hecto ;
  ns2:hasUnit ns2:are ;
  ns2:hasDimension ns2:area-Dimension .

ns2:squareMile-Statute
  a ns2:UnitExponentiation ;
  rdfs:label "square mile (statute)"@en ;
  ns2:symbol "mi2" ;
  ns2:hasBase ns2:mile-International ;
  ns2:hasExponent 2 ;
  ns2:hasDimension ns2:area-Dimension .

ns2:cubicMetre
  a ns2:UnitExponentiation ;
  rdfs:label "cubic metre"@en, "kubieke meter"@nl ;
  rdfs:comment "Cubic metre is a unit of volume defined as the volume of a cube whose sides measure exactly one metre."@en ;
  ns2:longcomment "Cubic metre is a unit of volume defined as the volume of a cube whose sides measure exactly one metre. Cubic metre is a derived unit in the International System of Units." ;
  ns2:symbol "m3" ;
  ns2:hasBase ns2:metre ;
  ns2:hasExponent 3 ;
  ns2:hasDimension ns2:volume-Dimension .

ns2:VolumeUnit
  a owl:Class ;
  rdfs:label "volume unit"@en ;
  rdfs:subClassOf ns2:Unit ;
  owl:equivalentClass [
    a owl:Class ;
    owl:unionOf (
     _:genid123
     ns2:PrefixedLitre
     ns2:CubicPrefixedMetre
   )
  ] .

ns2:acreFoot
  a ns2:Unit, ns2:SingularUnit ;
  rdfs:label "acre foot"@en ;
  rdfs:comment "The acre foot is a unit of volume defined as 1.233489e3 cubic metre."@en ;
  ns2:hasFactor "1.233489e3"^^xsd:float ;
  ns2:hasUnit ns2:cubicMetre ;
  ns2:hasDimension ns2:volume-Dimension .

ns2:barrel-US
  a ns2:Unit, ns2:SingularUnit ;
  rdfs:label "barrel (US)"@en ;
  ns2:alternativeLabel "US barrel"@en ;
  rdfs:comment "The US barrel is a unit of volume defined as 1.589873e-1 cubic metre."@en ;
  ns2:symbol "bbl" ;
  ns2:hasFactor "1.589873e-1"^^xsd:float ;
  ns2:hasUnit ns2:cubicMetre ;
  ns2:hasDimension ns2:volume-Dimension .

ns2:bushel-US
  a ns2:Unit, ns2:SingularUnit ;
  rdfs:label "bushel (US)"@en ;
  ns2:alternativeLabel "US bushel"@en ;
  rdfs:comment "The US bushel is a unit of volume defined as 3.523907e-2 cubic metre."@en ;
  ns2:symbol "bu" ;
  ns2:hasFactor "3.523907e-2"^^xsd:float ;
  ns2:hasUnit ns2:cubicMetre ;
  ns2:hasDimension ns2:volume-Dimension .

ns2:cord
  a ns2:Unit, ns2:SingularUnit ;
  rdfs:label "cord"@en ;
  rdfs:comment "The cord is a unit of volume defined as 3.624556 cubic metre."@en ;
  ns2:hasFactor "3.624556"^^xsd:float ;
  ns2:hasUnit ns2:cubicMetre ;
  ns2:hasDimension ns2:volume-Dimension .

ns2:cup-USCustomary
  a ns2:Unit, ns2:SingularUnit ;
  rdfs:label "cup (US customary)"@en ;
  ns2:alternativeLabel "US customary cup"@en ;
  rdfs:comment "The US customary cup is a unit of volume defined as 2.365882e-4 cubic metre."@en ;
  ns2:hasFactor "2.365882e-4"^^xsd:float ;
  ns2:hasUnit ns2:cubicMetre ;
  ns2:hasDimension ns2:volume-Dimension ;
  ns2:LaTeXCommand "\\cupUnit" .

ns2:dryGallon-US
  a ns2:Unit, ns2:SingularUnit ;
  rdfs:label "dry gallon (US)"@en ;
  ns2:alternativeLabel "gallon (US dry)"@en, "US dry gallon"@en ;
  rdfs:comment "The US dry gallon is a unit of volume defined as 4.40488377086e-3 cubic metre."@en ;
  ns2:symbol "gal" ;
  ns2:hasFactor "4.40488377086e-3"^^xsd:float ;
  ns2:hasUnit ns2:cubicMetre ;
  ns2:hasDimension ns2:volume-Dimension .

ns2:dryPint-US
  a ns2:Unit, ns2:SingularUnit ;
  rdfs:label "dry pint (US)"@en ;
  ns2:alternativeLabel "pint (US dry)"@en, "US dry pint"@en ;
  rdfs:comment "The US dry pint is a unit of volume defined as 5.506105e-4 cubic metre."@en ;
  ns2:symbol "dry pt" ;
  ns2:hasFactor "5.506105e-4"^^xsd:float ;
  ns2:hasUnit ns2:cubicMetre ;
  ns2:hasDimension ns2:volume-Dimension .

ns2:dryQuart-US
  a ns2:Unit, ns2:SingularUnit ;
  rdfs:label "dry quart (US)"@en ;
  ns2:alternativeLabel "quart (US dry)"@en, "US dry quart"@en ;
  rdfs:comment "The US dry quart is a unit of volume defined as 1.101221e-3 cubic metre."@en ;
  ns2:symbol "dry qt" ;
  ns2:hasFactor "1.101221e-3"^^xsd:float ;
  ns2:hasUnit ns2:cubicMetre ;
  ns2:hasDimension ns2:volume-Dimension .

ns2:fluidOunce-Imperial
  a ns2:Unit, ns2:SingularUnit ;
  rdfs:label "fluid ounce (imperial)"@en ;
  ns2:alternativeLabel "ounce (imperial fluid)"@en, "imperial fluid ounce"@en ;
  rdfs:comment "The imperial fluid ounce is a unit of volume defined as 2.841306e-5 cubic metre."@en ;
  ns2:symbol "fl oz" ;
  ns2:hasFactor "2.841306e-5"^^xsd:float ;
  ns2:hasUnit ns2:cubicMetre ;
  ns2:hasDimension ns2:volume-Dimension .

ns2:fluidOunce-US
  a ns2:Unit, ns2:SingularUnit ;
  rdfs:label "fluid ounce (US)"@en ;
  ns2:alternativeLabel "ounce (US fluid)"@en, "US fluid ounce"@en ;
  rdfs:comment "The US fluid ounce is a unit of volume defined as 2.957353e-5 cubic metre."@en ;
  ns2:symbol "fl oz" ;
  ns2:hasFactor "2.957353e-5"^^xsd:float ;
  ns2:hasUnit ns2:cubicMetre ;
  ns2:hasDimension ns2:volume-Dimension .

ns2:gallon-Imperial
  a ns2:Unit, ns2:SingularUnit ;
  rdfs:label "gallon (imperial)"@en ;
  ns2:alternativeLabel "imperial gallon"@en ;
  rdfs:comment "The imperial gallon is a unit of volume defined as 4.54609e-3 cubic metre."@en ;
  ns2:symbol "gal" ;
  ns2:hasFactor "4.54609e-3"^^xsd:float ;
  ns2:hasUnit ns2:cubicMetre ;
  ns2:hasDimension ns2:volume-Dimension .

ns2:gallon-US
  a ns2:Unit, ns2:SingularUnit ;
  rdfs:label "gallon (US)"@en ;
  ns2:alternativeLabel "US gallon"@en ;
  rdfs:comment "The US gallon is a unit of volume defined as 3.785412e-3 cubic metre."@en ;
  ns2:symbol "gal" ;
  ns2:hasFactor "3.785412e-3"^^xsd:float ;
  ns2:hasUnit ns2:cubicMetre ;
  ns2:hasDimension ns2:volume-Dimension .

ns2:gill-Imperial
  a ns2:Unit, ns2:SingularUnit ;
  rdfs:label "gill (imperial)"@en ;
  ns2:alternativeLabel "imperial gill"@en ;
  rdfs:comment "The imperial gill is a unit of volume defined as 1.420653e-4 cubic metre."@en ;
  ns2:symbol "gi" ;
  ns2:hasFactor "1.420653e-4"^^xsd:float ;
  ns2:hasUnit ns2:cubicMetre ;
  ns2:hasDimension ns2:volume-Dimension .

ns2:gill-US
  a ns2:Unit, ns2:SingularUnit ;
  rdfs:label "gill (US)"@en ;
  ns2:alternativeLabel "US gill"@en ;
  rdfs:comment "The US gill is a unit of volume defined as 1.182941e-4 cubic metre."@en ;
  ns2:symbol "gi" ;
  ns2:hasFactor "1.182941e-4"^^xsd:float ;
  ns2:hasUnit ns2:cubicMetre ;
  ns2:hasDimension ns2:volume-Dimension .

ns2:litre
  a ns2:Unit, ns2:SingularUnit ;
  rdfs:label "litre"@en, "liter"@nl, "升"@zh ;
  ns2:alternativeLabel "liter"@en ;
  rdfs:comment "The litre is a unit of volume defined as 1.0e-3 cubic metre."@en ;
  ns2:symbol "l" ;
  ns2:alternativeSymbol "L" ;
  ns2:hasFactor "1.0e-3"^^xsd:float ;
  ns2:hasUnit ns2:cubicMetre ;
  ns2:hasDimension ns2:volume-Dimension .

ns2:liquidPint-US
  a ns2:Unit, ns2:SingularUnit ;
  rdfs:label "liquid pint (US)"@en ;
  ns2:alternativeLabel "pint (US liquid)"@en, "US liquid pint"@en ;
  rdfs:comment "The US liquid pint is a unit of volume defined as 4.731765e-4 cubic metre."@en ;
  ns2:symbol "liq pt" ;
  ns2:hasFactor "4.731765e-4"^^xsd:float ;
  ns2:hasUnit ns2:cubicMetre ;
  ns2:hasDimension ns2:volume-Dimension .

ns2:liquidQuart-US
  a ns2:Unit, ns2:SingularUnit ;
  rdfs:label "liquid quart (US)"@en ;
  ns2:alternativeLabel "quart (US liquid)"@en, "US liquid quart"@en ;
  rdfs:comment "The US liquid quart is a unit of volume defined as 9.463529e-4 cubic metre."@en ;
  ns2:symbol "liq qt" ;
  ns2:hasFactor "9.463529e-4"^^xsd:float ;
  ns2:hasUnit ns2:cubicMetre ;
  ns2:hasDimension ns2:volume-Dimension .

ns2:peck-US
  a ns2:Unit, ns2:SingularUnit ;
  rdfs:label "peck (US)"@en ;
  ns2:alternativeLabel "US peck"@en ;
  rdfs:comment "The US peck is a unit of volume defined as 8.809768e-3 cubic metre."@en ;
  ns2:symbol "pk" ;
  ns2:hasFactor "8.809768e-3"^^xsd:float ;
  ns2:hasUnit ns2:cubicMetre ;
  ns2:hasDimension ns2:volume-Dimension .

ns2:pint-Imperial
  a ns2:Unit, ns2:SingularUnit ;
  rdfs:label "pint (imperial)"@en ;
  ns2:alternativeLabel "imperial pint"@en ;
  rdfs:comment "The pint is a unit of volume defined as 568.26125 millilitre."@en ;
  ns2:hasFactor "568.26125"^^xsd:float ;
  ns2:hasUnit ns2:millilitre ;
  ns2:hasDimension ns2:volume-Dimension .

ns2:quart-Imperial
  a ns2:Unit, ns2:SingularUnit ;
  rdfs:label "quart (imperial)"@en ;
  ns2:alternativeLabel "imperial quart"@en ;
  rdfs:comment "The imperial quart is a unit of volume defined as 1.1365 litre."@en ;
  ns2:hasFactor "1.1365"^^xsd:float ;
  ns2:hasUnit ns2:litre ;
  ns2:hasDimension ns2:volume-Dimension .

ns2:stere
  a ns2:Unit, ns2:SingularUnit ;
  rdfs:label "stere"@en ;
  rdfs:comment "The stere is a unit of volume defined as cubic metre."@en ;
  ns2:hasUnit ns2:cubicMetre ;
  ns2:hasDimension ns2:volume-Dimension .

ns2:tablespoon-US
  a ns2:Unit, ns2:SingularUnit ;
  rdfs:label "tablespoon (US)"@en ;
  ns2:alternativeLabel "US tablespoon"@en ;
  rdfs:comment "The US tablespoon is a unit of volume defined as 1.478676e-5 cubic metre."@en ;
  ns2:hasFactor "1.478676e-5"^^xsd:float ;
  ns2:hasUnit ns2:cubicMetre ;
  ns2:hasDimension ns2:volume-Dimension .

ns2:teaspoon-US
  a ns2:Unit, ns2:SingularUnit ;
  rdfs:label "teaspoon (US)"@en ;
  ns2:alternativeLabel "US teaspoon"@en ;
  rdfs:comment "The US teaspoon is a unit of volume defined as 4.928922e-6 cubic metre."@en ;
  ns2:hasFactor "4.928922e-6"^^xsd:float ;
  ns2:hasUnit ns2:cubicMetre ;
  ns2:hasDimension ns2:volume-Dimension .

ns2:dessertspoon
  a ns2:Unit, ns2:SingularUnit ;
  rdfs:label "dessertspoon"@en ;
  rdfs:comment "The desserspoon is a unit of volume defined as 2 teaspoon."@en ;
  ns2:hasFactor "2"^^xsd:float ;
  ns2:hasUnit ns2:teaspoon-US ;
  ns2:hasDimension ns2:volume-Dimension .

ns2:ton-Register
  a ns2:Unit, ns2:SingularUnit ;
  rdfs:label "ton (register)"@en ;
  ns2:alternativeLabel "register ton"@en ;
  rdfs:comment "The register ton is a unit of volume defined as 100 cubic foot = 2.8316846592 cubic metre."@en ;
  ns2:hasDimension ns2:volume-Dimension .

ns2:cubicParsec
  a ns2:UnitExponentiation ;
  rdfs:label "cubic parsec"@en, "kubieke parsec"@nl ;
  ns2:symbol "pc3" ;
  ns2:hasBase ns2:parsec ;
  ns2:hasExponent 3 ;
  ns2:hasDimension ns2:volume-Dimension .

ns2:cubicKiloparsec
  a ns2:UnitExponentiation ;
  rdfs:label "cubic kiloparsec"@en, "kubieke kiloparsec"@nl ;
  ns2:symbol "kpc3" ;
  ns2:hasBase ns2:kiloparsec ;
  ns2:hasExponent 3 ;
  ns2:hasDimension ns2:volume-Dimension .

ns2:PrefixedLitre
  a owl:Class ;
  rdfs:label "prefixed litre"@en ;
  rdfs:subClassOf ns2:PrefixedUnit ;
  owl:equivalentClass [
    a owl:Class ;
    owl:intersectionOf (
     _:genid167
     _:genid169
     _:genid171
     _:genid173
   )
  ] .

ns2:CubicPrefixedMetre
  a owl:Class ;
  rdfs:label "cubic prefixed metre"@en ;
  rdfs:subClassOf ns2:UnitExponentiation ;
  owl:equivalentClass [
    a owl:Class ;
    owl:intersectionOf (
     _:genid158
     _:genid160
     _:genid162
     _:genid164
   )
  ] .

ns2:cubicYoctometre
  a ns2:CubicPrefixedMetre ;
  rdfs:label "cubic yoctometre"@en, "kubieke yoctometer"@nl ;
  ns2:symbol "ym3" ;
  ns2:hasBase ns2:yoctometre ;
  ns2:hasExponent 3 ;
  ns2:hasDimension ns2:volume-Dimension .

ns2:cubicZeptometre
  a ns2:CubicPrefixedMetre ;
  rdfs:label "cubic zeptometre"@en, "kubieke zeptometer"@nl ;
  ns2:symbol "zm3" ;
  ns2:hasBase ns2:zeptometre ;
  ns2:hasExponent 3 ;
  ns2:hasDimension ns2:volume-Dimension .

ns2:cubicAttometre
  a ns2:CubicPrefixedMetre ;
  rdfs:label "cubic attometre"@en, "kubieke attometer"@nl ;
  ns2:symbol "am3" ;
  ns2:hasBase ns2:attometre ;
  ns2:hasExponent 3 ;
  ns2:hasDimension ns2:volume-Dimension .

ns2:cubicFemtometre
  a ns2:CubicPrefixedMetre ;
  rdfs:label "cubic femtometre"@en, "kubieke femtometer"@nl ;
  ns2:symbol "fm3" ;
  ns2:hasBase ns2:femtometre ;
  ns2:hasExponent 3 ;
  ns2:hasDimension ns2:volume-Dimension .

ns2:cubicPicometre
  a ns2:CubicPrefixedMetre ;
  rdfs:label "cubic picometre"@en, "kubieke picometer"@nl ;
  ns2:symbol "pm3" ;
  ns2:hasBase ns2:picometre ;
  ns2:hasExponent 3 ;
  ns2:hasDimension ns2:volume-Dimension .

ns2:cubicNanometre
  a ns2:CubicPrefixedMetre ;
  rdfs:label "cubic nanometre"@en, "kubieke nanometer"@nl ;
  ns2:symbol "nm3" ;
  ns2:hasBase ns2:nanometre ;
  ns2:hasExponent 3 ;
  ns2:hasDimension ns2:volume-Dimension .

ns2:cubicMicrometre
  a ns2:CubicPrefixedMetre ;
  rdfs:label "cubic micrometre"@en, "kubieke micrometer"@nl ;
  ns2:symbol "μm3" ;
  ns2:hasBase ns2:micrometre ;
  ns2:hasExponent 3 ;
  ns2:hasDimension ns2:volume-Dimension .

ns2:cubicMillimetre
  a ns2:CubicPrefixedMetre ;
  rdfs:label "cubic millimetre"@en, "kubieke millimeter"@nl ;
  ns2:symbol "mm3" ;
  ns2:hasBase ns2:millimetre ;
  ns2:hasExponent 3 ;
  ns2:hasDimension ns2:volume-Dimension .

ns2:cubicCentimetre
  a ns2:CubicPrefixedMetre ;
  rdfs:label "cubic centimetre"@en, "kubieke centimeter"@nl ;
  ns2:symbol "cm3" ;
  ns2:hasBase ns2:centimetre ;
  ns2:hasExponent 3 ;
  ns2:hasDimension ns2:volume-Dimension .

ns2:cubicDecimetre
  a ns2:CubicPrefixedMetre ;
  rdfs:label "cubic decimetre"@en, "kubieke decimeter"@nl ;
  ns2:symbol "dm3" ;
  ns2:hasBase ns2:decimetre ;
  ns2:hasExponent 3 ;
  ns2:hasDimension ns2:volume-Dimension .

ns2:cubicDecametre
  a ns2:CubicPrefixedMetre ;
  rdfs:label "cubic decametre"@en, "kubieke decameter"@nl ;
  ns2:symbol "dam3" ;
  ns2:hasBase ns2:decametre ;
  ns2:hasExponent 3 ;
  ns2:hasDimension ns2:volume-Dimension .

ns2:cubicHectometre
  a ns2:CubicPrefixedMetre ;
  rdfs:label "cubic hectometre"@en, "kubieke hectometer"@nl ;
  ns2:symbol "hm3" ;
  ns2:hasBase ns2:hectometre ;
  ns2:hasExponent 3 ;
  ns2:hasDimension ns2:volume-Dimension .

ns2:cubicKilometre
  a ns2:CubicPrefixedMetre ;
  rdfs:label "cubic kilometre"@en, "kubieke kilometer"@nl ;
  ns2:symbol "km3" ;
  ns2:hasBase ns2:kilometre ;
  ns2:hasExponent 3 ;
  ns2:hasDimension ns2:volume-Dimension .

ns2:cubicMegametre
  a ns2:CubicPrefixedMetre ;
  rdfs:label "cubic megametre"@en, "kubieke megameter"@nl ;
  ns2:symbol "Mm3" ;
  ns2:hasBase ns2:megametre ;
  ns2:hasExponent 3 ;
  ns2:hasDimension ns2:volume-Dimension .

ns2:cubicGigametre
  a ns2:CubicPrefixedMetre ;
  rdfs:label "cubic gigametre"@en, "kubieke gigameter"@nl ;
  ns2:symbol "Gm3" ;
  ns2:hasBase ns2:gigametre ;
  ns2:hasExponent 3 ;
  ns2:hasDimension ns2:volume-Dimension .

ns2:cubicTerametre
  a ns2:CubicPrefixedMetre ;
  rdfs:label "cubic terametre"@en, "kubieke terameter"@nl ;
  ns2:symbol "Tm3" ;
  ns2:hasBase ns2:terametre ;
  ns2:hasExponent 3 ;
  ns2:hasDimension ns2:volume-Dimension .

ns2:cubicPetametre
  a ns2:CubicPrefixedMetre ;
  rdfs:label "cubic petametre"@en, "kubieke petameter"@nl ;
  ns2:symbol "Pm3" ;
  ns2:hasBase ns2:petametre ;
  ns2:hasExponent 3 ;
  ns2:hasDimension ns2:volume-Dimension .

ns2:cubicExametre
  a ns2:CubicPrefixedMetre ;
  rdfs:label "cubic exametre"@en, "kubieke exameter"@nl ;
  ns2:symbol "Em3" ;
  ns2:hasBase ns2:exametre ;
  ns2:hasExponent 3 ;
  ns2:hasDimension ns2:volume-Dimension .

ns2:cubicZettametre
  a ns2:CubicPrefixedMetre ;
  rdfs:label "cubic zettametre"@en, "kubieke zettameter"@nl ;
  ns2:symbol "Zm3" ;
  ns2:hasBase ns2:zettametre ;
  ns2:hasExponent 3 ;
  ns2:hasDimension ns2:volume-Dimension .

ns2:cubicYottametre
  a ns2:CubicPrefixedMetre ;
  rdfs:label "cubic yottametre"@en, "kubieke yottameter"@nl ;
  ns2:symbol "Ym3" ;
  ns2:hasBase ns2:yottametre ;
  ns2:hasExponent 3 ;
  ns2:hasDimension ns2:volume-Dimension .

ns2:yoctolitre
  a ns2:PrefixedUnit ;
  rdfs:label "yoctolitre"@en, "yoctoliter"@nl ;
  ns2:symbol "yl" ;
  ns2:hasPrefix ns2:yocto ;
  ns2:hasUnit ns2:litre ;
  ns2:hasDimension ns2:volume-Dimension .

ns2:zeptolitre
  a ns2:PrefixedUnit ;
  rdfs:label "zeptolitre"@en, "zeptoliter"@nl ;
  ns2:symbol "zl" ;
  ns2:hasPrefix ns2:zepto ;
  ns2:hasUnit ns2:litre ;
  ns2:hasDimension ns2:volume-Dimension .

ns2:attolitre
  a ns2:PrefixedUnit ;
  rdfs:label "attolitre"@en, "attoliter"@nl ;
  ns2:symbol "al" ;
  ns2:hasPrefix ns2:atto ;
  ns2:hasUnit ns2:litre ;
  ns2:hasDimension ns2:volume-Dimension .

ns2:femtolitre
  a ns2:PrefixedUnit ;
  rdfs:label "femtolitre"@en, "femtoliter"@nl ;
  ns2:symbol "fl" ;
  ns2:hasPrefix ns2:femto ;
  ns2:hasUnit ns2:litre ;
  ns2:hasDimension ns2:volume-Dimension .

ns2:picolitre
  a ns2:PrefixedUnit ;
  rdfs:label "picolitre"@en, "picoliter"@nl ;
  ns2:symbol "pl" ;
  ns2:hasPrefix ns2:pico ;
  ns2:hasUnit ns2:litre ;
  ns2:hasDimension ns2:volume-Dimension .

ns2:nanolitre
  a ns2:PrefixedUnit ;
  rdfs:label "nanolitre"@en, "nanoliter"@nl ;
  ns2:symbol "nl" ;
  ns2:hasPrefix ns2:nano ;
  ns2:hasUnit ns2:litre ;
  ns2:hasDimension ns2:volume-Dimension .

ns2:microlitre
  a ns2:PrefixedUnit ;
  rdfs:label "microlitre"@en, "microliter"@nl ;
  ns2:symbol "μl" ;
  ns2:unofficialAbbreviation "ul" ;
  ns2:hasPrefix ns2:micro ;
  ns2:hasUnit ns2:litre ;
  ns2:hasDimension ns2:volume-Dimension .

ns2:millilitre
  a ns2:PrefixedUnit ;
  rdfs:label "millilitre"@en, "milliliter"@nl ;
  ns2:symbol "ml" ;
  ns2:hasPrefix ns2:milli ;
  ns2:hasUnit ns2:litre ;
  ns2:hasDimension ns2:volume-Dimension .

ns2:centilitre
  a ns2:PrefixedUnit ;
  rdfs:label "centilitre"@en, "centiliter"@nl ;
  ns2:symbol "cl" ;
  ns2:hasPrefix ns2:centi ;
  ns2:hasUnit ns2:litre ;
  ns2:hasDimension ns2:volume-Dimension .

ns2:decilitre
  a ns2:PrefixedUnit ;
  rdfs:label "decilitre"@en, "deciliter"@nl ;
  ns2:symbol "dl" ;
  ns2:hasPrefix ns2:deci ;
  ns2:hasUnit ns2:litre ;
  ns2:hasDimension ns2:volume-Dimension .

ns2:decalitre
  a ns2:PrefixedUnit ;
  rdfs:label "decalitre"@en, "decaliter"@nl ;
  ns2:symbol "dal" ;
  ns2:hasPrefix ns2:deca ;
  ns2:hasUnit ns2:litre ;
  ns2:hasDimension ns2:volume-Dimension .

ns2:hectolitre
  a ns2:PrefixedUnit ;
  rdfs:label "hectolitre"@en, "hectoliter"@nl ;
  ns2:symbol "hl" ;
  ns2:hasPrefix ns2:hecto ;
  ns2:hasUnit ns2:litre ;
  ns2:hasDimension ns2:volume-Dimension .

ns2:kilolitre
  a ns2:PrefixedUnit ;
  rdfs:label "kilolitre"@en, "kiloliter"@nl ;
  ns2:symbol "kl" ;
  ns2:hasPrefix ns2:kilo ;
  ns2:hasUnit ns2:litre ;
  ns2:hasDimension ns2:volume-Dimension .

ns2:megalitre
  a ns2:PrefixedUnit ;
  rdfs:label "megalitre"@en, "megaliter"@nl ;
  ns2:symbol "Ml" ;
  ns2:hasPrefix ns2:mega ;
  ns2:hasUnit ns2:litre ;
  ns2:hasDimension ns2:volume-Dimension .

ns2:gigalitre
  a ns2:PrefixedUnit ;
  rdfs:label "gigalitre"@en, "gigaliter"@nl ;
  ns2:symbol "Gl" ;
  ns2:hasPrefix ns2:giga ;
  ns2:hasUnit ns2:litre ;
  ns2:hasDimension ns2:volume-Dimension .

ns2:teralitre
  a ns2:PrefixedUnit ;
  rdfs:label "teralitre"@en, "teraliter"@nl ;
  ns2:symbol "Tl" ;
  ns2:hasPrefix ns2:tera ;
  ns2:hasUnit ns2:litre ;
  ns2:hasDimension ns2:volume-Dimension .

ns2:petalitre
  a ns2:PrefixedUnit ;
  rdfs:label "petalitre"@en, "petaliter"@nl ;
  ns2:symbol "Pl" ;
  ns2:hasPrefix ns2:peta ;
  ns2:hasUnit ns2:litre ;
  ns2:hasDimension ns2:volume-Dimension .

ns2:exalitre
  a ns2:PrefixedUnit ;
  rdfs:label "exalitre"@en, "exaliter"@nl ;
  ns2:symbol "El" ;
  ns2:hasPrefix ns2:exa ;
  ns2:hasUnit ns2:litre ;
  ns2:hasDimension ns2:volume-Dimension .

ns2:zettalitre
  a ns2:PrefixedUnit ;
  rdfs:label "zettalitre"@en, "zettaliter"@nl ;
  ns2:symbol "Zl" ;
  ns2:hasPrefix ns2:zetta ;
  ns2:hasUnit ns2:litre ;
  ns2:hasDimension ns2:volume-Dimension .

ns2:yottalitre
  a ns2:PrefixedUnit ;
  rdfs:label "yottalitre"@en, "yottaliter"@nl ;
  ns2:symbol "Yl" ;
  ns2:hasPrefix ns2:yotta ;
  ns2:hasUnit ns2:litre ;
  ns2:hasDimension ns2:volume-Dimension .

ns2:_25Millilitre
  a ns2:UnitMultiple ;
  rdfs:label "25 millilitre"@en, "25 milliliter"@nl ;
  ns2:symbol "25 ml" ;
  ns2:hasFactor "25"^^xsd:float ;
  ns2:hasUnit ns2:millilitre ;
  ns2:hasDimension ns2:volume-Dimension .

ns2:bar-Food
  a ns2:Unit ;
  rdfs:label "bar (food)"@en, "reep"@nl .

ns2:bottle
  a ns2:Unit ;
  rdfs:label "bottle"@en, "fles"@nl .

ns2:bowl
  a ns2:Unit ;
  rdfs:label "bowl"@en, "schaaltje"@nl .

ns2:cup
  a ns2:Unit ;
  rdfs:label "cup"@en, "kopje"@nl .

ns2:dash
  a ns2:Unit ;
  rdfs:label "dash"@en, "scheutje"@nl .

ns2:deepBowl
  a ns2:Unit ;
  rdfs:label "deep bowl"@en, "diep bord"@nl .

ns2:drop
  a ns2:Unit ;
  rdfs:label "drop"@en, "druppel"@nl .

ns2:fillet
  a ns2:Unit ;
  rdfs:label "fillet"@en, "filet"@nl .

ns2:glass
  a ns2:Unit ;
  rdfs:label "glass"@en, "glas"@nl .

ns2:handful
  a ns2:Unit ;
  rdfs:label "handful"@en, "handje"@nl .

ns2:piece
  a ns2:Unit ;
  rdfs:label "piece"@en, "stuks"@nl .

ns2:pinch
  a ns2:Unit ;
  rdfs:label "pinch"@en, "mespunt"@nl .

ns2:portion
  a ns2:Unit ;
  rdfs:label "portion"@en, "portie"@nl .

ns2:scoop
  a ns2:Unit ;
  rdfs:label "scoop"@en, "bolletje"@nl .

ns2:servingSpoon
  a ns2:Unit ;
  rdfs:label "serving spoon"@en, "opscheplepel"@nl .

ns2:slice
  a ns2:Unit ;
  rdfs:label "slice"@en, "snee"@nl .

ns2:spread
  a ns2:Unit ;
  rdfs:label "spread"@en, "broodbelegging"@nl .

ns2:wedge
  a ns2:Unit ;
  rdfs:label "wedge"@en, "punt"@nl .

ns2:wineGlass
  a ns2:Unit ;
  rdfs:label "wine glass"@en, "wijnglas"@nl .

ns2:radian
  a ns2:Unit, ns2:SingularUnit ;
  rdfs:label "radian"@en, "radiaal"@nl, "弧度"@zh ;
  rdfs:comment "The radian is a unit of angle defined as the angle subtended at the center of a circle by an arc that is equal in length to the radius of the circle."@en ;
  ns2:longcomment "The radian is a unit of angle defined as the angle subtended at the center of a circle by an arc that is equal in length to the radius of the circle. The radian is a derived unit in the International System of Units." ;
  ns2:symbol "rad" ;
  ns2:hasUnit ns2:metrePerMetre ;
  ns2:hasDimension ns2:dimensionOne .

ns2:AngleUnit
  a owl:Class ;
  rdfs:label "angle unit"@en ;
  rdfs:subClassOf ns2:Unit ;
  owl:equivalentClass [
    a owl:Class ;
    owl:unionOf (
     _:genid176
     ns2:PrefixedRadian
   )
  ] .

ns2:degree
  a ns2:Unit, ns2:SingularUnit ;
  rdfs:label "degree"@en, "graad"@nl, "度"@zh ;
  rdfs:comment "The degree is a unit of angle defined as 1.745329e-2 radian."@en ;
  ns2:symbol "°" ;
  ns2:hasFactor "1.745329e-2"^^xsd:float ;
  ns2:hasUnit ns2:radian ;
  ns2:hasDimension ns2:dimensionOne .

ns2:gon
  a ns2:Unit, ns2:SingularUnit ;
  rdfs:label "gon"@en ;
  ns2:alternativeLabel "grade"@en ;
  rdfs:comment "The gon is a unit of angle defined as 1.570796e-2 radian."@en ;
  ns2:symbol "gon" ;
  ns2:hasFactor "1.570796e-2"^^xsd:float ;
  ns2:hasUnit ns2:radian ;
  ns2:hasDimension ns2:dimensionOne .

ns2:mil-Angle
  a ns2:Unit, ns2:SingularUnit ;
  rdfs:label "mil (angle)"@en ;
  rdfs:comment "The mil (angle) is a unit of angle defined as 9.817477e-4 radian."@en ;
  ns2:hasFactor "9.817477e-4"^^xsd:float ;
  ns2:hasUnit ns2:radian ;
  ns2:hasDimension ns2:dimensionOne .

ns2:minute-Angle
  a ns2:Unit, ns2:SingularUnit ;
  rdfs:label "minute (angle)"@en, "minuut (hoek)"@nl, "分钟（角）"@zh ;
  ns2:alternativeLabel "minute of arc"@en, "arcminute"@en, "arcminuut"@nl ;
  rdfs:comment "The minute (angle) is a unit of angle defined as 2.908882e-4 radian."@en ;
  ns2:symbol "'" ;
  ns2:hasFactor "2.908882e-4"^^xsd:float ;
  ns2:hasUnit ns2:radian ;
  ns2:hasDimension ns2:dimensionOne .

ns2:revolution
  a ns2:Unit, ns2:SingularUnit ;
  rdfs:label "revolution"@en ;
  rdfs:comment "The revolution is a unit of angle defined as 6.283185 radian."@en ;
  ns2:symbol "r" ;
  ns2:hasFactor "6.283185"^^xsd:float ;
  ns2:hasUnit ns2:radian ;
  ns2:hasDimension ns2:dimensionOne .

ns2:second-Angle
  a ns2:Unit, ns2:SingularUnit ;
  rdfs:label "second (angle)"@en, "seconde (hoek)"@nl, "秒（角度）"@zh ;
  ns2:alternativeLabel "second of arc"@en, "arcsecond"@en, "boogseconde"@nl ;
  rdfs:comment "The second (angle) is a unit of angle defined as 4.848137e-6 radian."@en ;
  ns2:symbol "\"" ;
  ns2:hasFactor "4.848137e-6"^^xsd:float ;
  ns2:hasUnit ns2:radian ;
  ns2:hasDimension ns2:dimensionOne .

ns2:millisecond-Angle
  a ns2:PrefixedUnit ;
  rdfs:label "millisecond (angle)"@en, "milliseconde (hoek)"@nl ;
  ns2:alternativeLabel "millisecond of arc"@en, "milliarcsecond"@en, "milliboogseconde"@nl ;
  rdfs:comment "The millisecond (angle) is a unit of length defined as 1.0e-3 second (angle). Used in astronomy (measurements of positions of stars, galaxies, etc.) to represent the error."@en ;
  ns2:symbol "mas" ;
  ns2:hasPrefix ns2:milli ;
  ns2:hasUnit ns2:second-Angle ;
  ns2:hasDimension ns2:dimensionOne .

ns2:microsecond-Angle
  a ns2:PrefixedUnit ;
  rdfs:label "microsecond (angle)"@en, "microseconde (hoek)"@nl ;
  ns2:alternativeLabel "microsecond of arc"@en, "microarcsecond"@en, "microboogseconde"@nl ;
  rdfs:comment "The microsecond (angle) is a unit of length defined as 1.0e-6 second (angle). Used in astronomy (measurements of positions of stars, galaxies, etc.) to represent the error."@en ;
  ns2:symbol "μas" ;
  ns2:hasPrefix ns2:milli ;
  ns2:hasUnit ns2:second-Angle ;
  ns2:hasDimension ns2:dimensionOne .

ns2:metrePerMetre
  a ns2:UnitDivision ;
  rdfs:label "metre per metre"@en, "meter per meter"@nl ;
  ns2:symbol "m/m" ;
  ns2:alternativeSymbol "m m-1", "m·m-1" ;
  ns2:hasNumerator ns2:metre ;
  ns2:hasDenominator ns2:metre ;
  ns2:hasDimension ns2:dimensionOne .

ns2:PrefixedRadian
  a owl:Class ;
  rdfs:label "prefixed radian"@en ;
  rdfs:subClassOf ns2:PrefixedUnit ;
  owl:equivalentClass [
    a owl:Class ;
    owl:intersectionOf (
     _:genid192
     _:genid194
     _:genid196
     _:genid198
   )
  ] .

ns2:yoctoradian
  a ns2:PrefixedUnit ;
  rdfs:label "yoctoradian"@en, "yoctoradiaal"@nl ;
  ns2:symbol "yrad" ;
  ns2:hasPrefix ns2:yocto ;
  ns2:hasUnit ns2:radian ;
  ns2:hasDimension ns2:dimensionOne .

ns2:zeptoradian
  a ns2:PrefixedUnit ;
  rdfs:label "zeptoradian"@en, "zeptoradiaal"@nl ;
  ns2:symbol "zrad" ;
  ns2:hasPrefix ns2:zepto ;
  ns2:hasUnit ns2:radian ;
  ns2:hasDimension ns2:dimensionOne .

ns2:attoradian
  a ns2:PrefixedUnit ;
  rdfs:label "attoradian"@en, "attoradiaal"@nl ;
  ns2:symbol "arad" ;
  ns2:hasPrefix ns2:atto ;
  ns2:hasUnit ns2:radian ;
  ns2:hasDimension ns2:dimensionOne .

ns2:femtoradian
  a ns2:PrefixedUnit ;
  rdfs:label "femtoradian"@en, "femtoradiaal"@nl ;
  ns2:symbol "frad" ;
  ns2:hasPrefix ns2:femto ;
  ns2:hasUnit ns2:radian ;
  ns2:hasDimension ns2:dimensionOne .

ns2:picoradian
  a ns2:PrefixedUnit ;
  rdfs:label "picoradian"@en, "picoradiaal"@nl ;
  ns2:symbol "prad" ;
  ns2:hasPrefix ns2:pico ;
  ns2:hasUnit ns2:radian ;
  ns2:hasDimension ns2:dimensionOne .

ns2:nanoradian
  a ns2:PrefixedUnit ;
  rdfs:label "nanoradian"@en, "nanoradiaal"@nl ;
  ns2:symbol "nrad" ;
  ns2:hasPrefix ns2:nano ;
  ns2:hasUnit ns2:radian ;
  ns2:hasDimension ns2:dimensionOne .

ns2:microradian
  a ns2:PrefixedUnit ;
  rdfs:label "microradian"@en, "microradiaal"@nl ;
  ns2:symbol "μrad" ;
  ns2:hasPrefix ns2:micro ;
  ns2:hasUnit ns2:radian ;
  ns2:hasDimension ns2:dimensionOne .

ns2:milliradian
  a ns2:PrefixedUnit ;
  rdfs:label "milliradian"@en, "milliradiaal"@nl ;
  ns2:symbol "mrad" ;
  ns2:hasPrefix ns2:milli ;
  ns2:hasUnit ns2:radian ;
  ns2:hasDimension ns2:dimensionOne .

ns2:centiradian
  a ns2:PrefixedUnit ;
  rdfs:label "centiradian"@en, "centiradiaal"@nl ;
  ns2:symbol "crad" ;
  ns2:hasPrefix ns2:centi ;
  ns2:hasUnit ns2:radian ;
  ns2:hasDimension ns2:dimensionOne .

ns2:deciradian
  a ns2:PrefixedUnit ;
  rdfs:label "deciradian"@en, "deciradiaal"@nl ;
  ns2:symbol "drad" ;
  ns2:hasPrefix ns2:deci ;
  ns2:hasUnit ns2:radian ;
  ns2:hasDimension ns2:dimensionOne .

ns2:steradian
  a ns2:Unit, ns2:SingularUnit ;
  rdfs:label "steradian"@en, "steradiaal"@nl, "球面度"@zh ;
  rdfs:comment "The steradian is a unit of solid angle defined as the solid angle subtended at the center of a sphere by a portion of the surface of the sphere that has an area equal to the square of the radius of the sphere."@en ;
  ns2:longcomment "The steradian is a unit of solid angle defined as the solid angle subtended at the center of a sphere by a portion of the surface of the sphere that has an area equal to the square of the radius of the sphere. The steradian is a derived unit in the International System of Units." ;
  ns2:symbol "sr" ;
  ns2:hasUnit ns2:squareMetrePerSquareMetre ;
  ns2:hasDimension ns2:dimensionOne .

ns2:SolidAngleUnit
  a owl:Class ;
  rdfs:label "solid angle unit"@en ;
  rdfs:subClassOf ns2:Unit ;
  owl:equivalentClass [
    a owl:Class ;
    owl:unionOf (
     _:genid201
     ns2:PrefixedSteradian
   )
  ] .

ns2:squareMetrePerSquareMetre
  a ns2:UnitDivision ;
  rdfs:label "square metre per square metre"@en, "vierkante meter per vierkante meter"@nl ;
  ns2:symbol "m2/m2" ;
  ns2:alternativeSymbol "m2 m-2", "m2·m-2" ;
  ns2:hasNumerator ns2:squareMetre ;
  ns2:hasDenominator ns2:squareMetre ;
  ns2:hasDimension ns2:dimensionOne .

ns2:degreeSquared
  a ns2:UnitExponentiation ;
  rdfs:label "degree squared"@en ;
  ns2:hasBase ns2:degree ;
  ns2:hasExponent 2 ;
  ns2:hasDimension ns2:dimensionOne .

ns2:second-AngleSquared
  a ns2:UnitExponentiation ;
  rdfs:label "second (angle) squared"@en ;
  ns2:alternativeLabel "arcsecond squared"@en ;
  ns2:symbol "arcsec2" ;
  ns2:hasBase ns2:second-Angle ;
  ns2:hasExponent 2 ;
  ns2:hasDimension ns2:dimensionOne .

ns2:PrefixedSteradian
  a owl:Class ;
  rdfs:label "prefixed steradian"@en ;
  rdfs:subClassOf ns2:PrefixedUnit ;
  owl:equivalentClass [
    a owl:Class ;
    owl:intersectionOf (
     _:genid211
     _:genid213
     _:genid215
     _:genid217
   )
  ] .

ns2:yoctosteradian
  a ns2:PrefixedUnit ;
  rdfs:label "yoctosteradian"@en, "yoctosteradiaal"@nl ;
  ns2:symbol "ysr" ;
  ns2:hasPrefix ns2:yocto ;
  ns2:hasUnit ns2:steradian ;
  ns2:hasDimension ns2:dimensionOne .

ns2:zeptosteradian
  a ns2:PrefixedUnit ;
  rdfs:label "zeptosteradian"@en, "zeptosteradiaal"@nl ;
  ns2:symbol "zsr" ;
  ns2:hasPrefix ns2:zepto ;
  ns2:hasUnit ns2:steradian ;
  ns2:hasDimension ns2:dimensionOne .

ns2:attosteradian
  a ns2:PrefixedUnit ;
  rdfs:label "attosteradian"@en, "attosteradiaal"@nl ;
  ns2:symbol "asr" ;
  ns2:hasPrefix ns2:atto ;
  ns2:hasUnit ns2:steradian ;
  ns2:hasDimension ns2:dimensionOne .

ns2:femtosteradian
  a ns2:PrefixedUnit ;
  rdfs:label "femtosteradian"@en, "femtosteradiaal"@nl ;
  ns2:symbol "fsr" ;
  ns2:hasPrefix ns2:femto ;
  ns2:hasUnit ns2:steradian ;
  ns2:hasDimension ns2:dimensionOne .

ns2:picosteradian
  a ns2:PrefixedUnit ;
  rdfs:label "picosteradian"@en, "picosteradiaal"@nl ;
  ns2:symbol "psr" ;
  ns2:hasPrefix ns2:pico ;
  ns2:hasUnit ns2:steradian ;
  ns2:hasDimension ns2:dimensionOne .

ns2:nanosteradian
  a ns2:PrefixedUnit ;
  rdfs:label "nanosteradian"@en, "nanosteradiaal"@nl ;
  ns2:symbol "nsr" ;
  ns2:hasPrefix ns2:nano ;
  ns2:hasUnit ns2:steradian ;
  ns2:hasDimension ns2:dimensionOne .

ns2:microsteradian
  a ns2:PrefixedUnit ;
  rdfs:label "microsteradian"@en, "microsteradiaal"@nl ;
  ns2:symbol "μsr" ;
  ns2:hasPrefix ns2:micro ;
  ns2:hasUnit ns2:steradian ;
  ns2:hasDimension ns2:dimensionOne .

ns2:millisteradian
  a ns2:PrefixedUnit ;
  rdfs:label "millisteradian"@en, "millisteradiaal"@nl ;
  ns2:symbol "msr" ;
  ns2:hasPrefix ns2:milli ;
  ns2:hasUnit ns2:steradian ;
  ns2:hasDimension ns2:dimensionOne .

ns2:centisteradian
  a ns2:PrefixedUnit ;
  rdfs:label "centisteradian"@en, "centisteradiaal"@nl ;
  ns2:symbol "csr" ;
  ns2:hasPrefix ns2:centi ;
  ns2:hasUnit ns2:steradian ;
  ns2:hasDimension ns2:dimensionOne .

ns2:decisteradian
  a ns2:PrefixedUnit ;
  rdfs:label "decisteradian"@en, "decisteradiaal"@nl ;
  ns2:symbol "dsr" ;
  ns2:hasPrefix ns2:deci ;
  ns2:hasUnit ns2:steradian ;
  ns2:hasDimension ns2:dimensionOne .

ns2:millimetrePerMetre
  a ns2:UnitDivision ;
  rdfs:label "millimetre per metre"@en, "millimeter per meter"@nl ;
  ns2:symbol "mm/m" ;
  ns2:alternativeSymbol "mm m-1", "mm·m-1" ;
  ns2:hasNumerator ns2:millimetre ;
  ns2:hasDenominator ns2:metre ;
  ns2:hasDimension ns2:dimensionOne .

ns2:length-Dimension
  a ns2:Dimension ;
  rdfs:label "length dimension"@en, "lengtedimensie"@nl ;
  ns2:symbol "L" ;
  ns2:hasSILengthDimensionExponent 1 ;
  ns2:hasSIMassDimensionExponent 0 ;
  ns2:hasSITimeDimensionExponent 0 ;
  ns2:hasSIElectricCurrentDimensionExponent 0 ;
  ns2:hasSIThermodynamicTemperatureDimensionExponent 0 ;
  ns2:hasSIAmountOfSubstanceDimensionExponent 0 ;
  ns2:hasSILuminousIntensityDimensionExponent 0 .

ns2:area-Dimension
  a ns2:Dimension ;
  rdfs:label "area dimension"@en, "oppervlaktedimensie"@nl ;
  ns2:hasSILengthDimensionExponent 2 ;
  ns2:hasSIMassDimensionExponent 0 ;
  ns2:hasSITimeDimensionExponent 0 ;
  ns2:hasSIElectricCurrentDimensionExponent 0 ;
  ns2:hasSIThermodynamicTemperatureDimensionExponent 0 ;
  ns2:hasSIAmountOfSubstanceDimensionExponent 0 ;
  ns2:hasSILuminousIntensityDimensionExponent 0 .

ns2:volume-Dimension
  a ns2:Dimension ;
  rdfs:label "volume dimension"@en, "volumedimensie"@nl ;
  ns2:hasSILengthDimensionExponent 3 ;
  ns2:hasSIMassDimensionExponent 0 ;
  ns2:hasSITimeDimensionExponent 0 ;
  ns2:hasSIElectricCurrentDimensionExponent 0 ;
  ns2:hasSIThermodynamicTemperatureDimensionExponent 0 ;
  ns2:hasSIAmountOfSubstanceDimensionExponent 0 ;
  ns2:hasSILuminousIntensityDimensionExponent 0 .

ns2:dimensionOne
  a ns2:Dimension ;
  rdfs:label "dimensionOne"@en ;
  ns2:symbol "1" ;
  ns2:hasSILengthDimensionExponent 0 ;
  ns2:hasSIMassDimensionExponent 0 ;
  ns2:hasSITimeDimensionExponent 0 ;
  ns2:hasSIElectricCurrentDimensionExponent 0 ;
  ns2:hasSIThermodynamicTemperatureDimensionExponent 0 ;
  ns2:hasSIAmountOfSubstanceDimensionExponent 0 ;
  ns2:hasSILuminousIntensityDimensionExponent 0 .

ns2:centimetre-Gram-SecondSystemOfUnits
  a ns2:SystemOfUnits ;
  rdfs:label "centimetre-gram-second system of units"@en, "centimeter-gram-seconde-systeem"@nl ;
  ns2:abbreviation "cgs"^^xsd:string, "CGS"^^xsd:string ;
  ns2:hasBaseQuantity ns2:Length, ns2:Mass, ns2:Time ;
  ns2:hasDerivedQuantity ns2:Frequency, ns2:Force, ns2:Energy, ns2:Pressure, ns2:DynamicViscosity, ns2:KinematicViscosity, ns2:Acceleration, ns2:Luminance, ns2:Illuminance ;
  ns2:hasBaseUnit ns2:centimetre, ns2:gram, ns2:second-Time ;
  ns2:hasDerivedUnit ns2:hertz, ns2:dyne, ns2:erg, ns2:microbar, ns2:poise, ns2:stokes, ns2:gal, ns2:stilb, ns2:phot .

ns2:centimetre-Gram-SecondElectromagneticSystemOfUnits
  a ns2:SystemOfUnits ;
  rdfs:label "centimetre-gram-second electromagnetic system of units"@en, "centimeter-gram-seconde electromagnetische systeem"@nl ;
  ns2:alternativeLabel "centimetre, gram, second electromagnetic system of units"@en, "CGS electromagnetic system of units"@en, "electromagnetic CGS system of units"@en ;
  ns2:abbreviation "emu"^^xsd:string, "EMU"^^xsd:string ;
  ns2:hasBaseQuantity ns2:Length, ns2:Mass, ns2:Time ;
  ns2:hasDerivedQuantity ns2:ElectricCurrent, ns2:ElectricCharge, ns2:Capacitance, ns2:Inductance, ns2:ElectricalConductance, ns2:ElectricalResistance, ns2:ElectricPotential, ns2:MagneticField, ns2:MagneticFluxDensity, ns2:MagneticFlux, ns2:MagnetomotiveForce ;
  ns2:hasBaseUnit ns2:centimetre, ns2:gram, ns2:second-Time ;
  ns2:hasDerivedUnit ns2:abampere, ns2:abcoulomb, ns2:abfarad, ns2:abhenry, ns2:abmho, ns2:abohm, ns2:abvolt, ns2:oersted, ns2:gauss, ns2:maxwell, ns2:gilbert .

ns2:centimetre-Gram-SecondElectrostaticSystemOfUnits
  a ns2:SystemOfUnits ;
  rdfs:label "centimetre-gram-second electrostatic system of units"@en, "centimeter-gram-seconde electrostatische systeem"@nl ;
  ns2:alternativeLabel "CGS electrostatic system of units"@en, "electrostatic CGS system of units"@en ;
  ns2:abbreviation "esu"^^xsd:string, "ESU"^^xsd:string ;
  ns2:hasBaseQuantity ns2:Length, ns2:Mass, ns2:Time ;
  ns2:hasDerivedQuantity ns2:ElectricCharge, ns2:ElectricCurrent, ns2:ElectricPotential, ns2:MagneticFluxDensity, ns2:Capacitance, ns2:Inductance, ns2:ElectricalConductance, ns2:ElectricalResistance, ns2:MagneticFlux, ns2:MagnetomotiveForce ;
  ns2:hasBaseUnit ns2:centimetre, ns2:gram, ns2:second-Time ;
  ns2:hasDerivedUnit ns2:statcoulomb, ns2:statampere, ns2:statvolt, ns2:stattesla, ns2:statfarad, ns2:stathenry, ns2:statmho, ns2:statohm, ns2:statweber .

ns2:centimetre-Gram-Second-BiotSystemOfUnits
  a ns2:SystemOfUnits ;
  rdfs:label "centimetre-gram-second-biot system of units"@en, "centimeter-gram-seconde-biot-systeem"@nl ;
  ns2:abbreviation "cm-g-s-Bi"^^xsd:string ;
  ns2:hasBaseQuantity ns2:Length, ns2:Mass, ns2:Time, ns2:ElectricCurrent ;
  ns2:hasBaseUnit ns2:centimetre, ns2:gram, ns2:second-Time, ns2:biot .

ns2:centimetre-Gram-Second-FranklinSystemOfUnits
  a ns2:SystemOfUnits ;
  rdfs:label "centimetre-gram-second-franklin system of units"@en, "centimeter-gram-seconde-franklin-systeem"@nl ;
  ns2:abbreviation "cm-g-s-Fr"^^xsd:string ;
  ns2:hasBaseQuantity ns2:Length, ns2:Mass, ns2:Time, ns2:ElectricCharge ;
  ns2:hasBaseUnit ns2:centimetre, ns2:gram, ns2:second-Time, ns2:franklin .

ns2:GaussianSystemOfUnits
  a ns2:SystemOfUnits ;
  rdfs:label "Gaussian system of units"@en, "Gaussische eenhedenstelsel"@nl, "高斯系统单位"@zh ;
  ns2:alternativeLabel "Gaussian CGS system of units"@en, "mixed CGS system of units"@en, "symmetrised CGS system of units"@en ;
  ns2:hasBaseQuantity ns2:Length, ns2:Mass, ns2:Time ;
  ns2:hasDerivedQuantity ns2:ElectricCharge, ns2:ElectricCurrent, ns2:ElectricPotential, ns2:MagneticFluxDensity, ns2:Capacitance, ns2:Inductance, ns2:ElectricalConductance, ns2:ElectricalResistance, ns2:MagneticFlux, ns2:MagneticField, ns2:MagnetomotiveForce ;
  ns2:hasBaseUnit ns2:centimetre, ns2:gram, ns2:second-Time ;
  ns2:hasDerivedUnit ns2:statcoulomb, ns2:abampere, ns2:statampere, ns2:statvolt, ns2:stattesla, ns2:statfarad, ns2:stathenry, ns2:statmho, ns2:statohm, ns2:statweber, ns2:abcoulomb, ns2:abfarad, ns2:abhenry, ns2:abmho, ns2:abohm, ns2:abvolt, ns2:oersted, ns2:gauss, ns2:maxwell, ns2:gilbert .

ns2:InternationalSystemOfUnits
  a ns2:SystemOfUnits ;
  rdfs:label "International System of Units"@en, "Internationale Stelsel van Eenheden"@nl, "国际单位制"@zh ;
  ns2:abbreviation "SI" ;
  ns2:hasBaseQuantity ns2:Length, ns2:Mass, ns2:Time, ns2:ElectricCurrent, ns2:ThermodynamicTemperature, ns2:AmountOfSubstance, ns2:LuminousIntensity ;
  ns2:hasDerivedQuantity ns2:Area, ns2:Volume, ns2:Angle, ns2:SolidAngle, ns2:Speed, ns2:Acceleration, ns2:Force, ns2:Momentum, ns2:Frequency, ns2:Wavenumber, ns2:AngularSpeed, ns2:AngularAcceleration, ns2:AngularMomentum, ns2:Density, ns2:SpecificVolume, ns2:Energy, ns2:Power, ns2:Torque, ns2:Pressure, ns2:Action, ns2:SurfaceTension, ns2:DynamicViscosity, ns2:Irradiance, ns2:HeatCapacity, ns2:SpecificHeatCapacity, ns2:ElectricCharge, ns2:CurrentDensity, ns2:ElectricPotential, ns2:MagneticFluxDensity, ns2:Capacitance, ns2:Inductance, ns2:ElectricalConductance, ns2:ElectricalResistance, ns2:ElectricalConductivity, ns2:ElectricalResistivity, ns2:MagneticFlux, ns2:MagnetomotiveForce, ns2:PermeabilityOfFreeSpace, ns2:Permittivity, ns2:Luminance, ns2:LuminousFlux, ns2:LuminousEnergy, ns2:Illuminance, ns2:Exposure, ns2:LuminousEfficacy, ns2:AbsorbedDose, ns2:AbsorbedDoseRate, ns2:DoseEquivalent, ns2:Activity, ns2:MolarMass, ns2:MolarHeatCapacity, ns2:CatalyticActivity ;
  ns2:hasBaseUnit ns2:metre, ns2:kilogram, ns2:second-Time, ns2:ampere, ns2:kelvin, ns2:mole, ns2:candela ;
  ns2:hasDerivedUnit ns2:squareMetre, ns2:cubicMetre, ns2:metrePerSecond-Time, ns2:metrePerSecond-TimeSquared, ns2:reciprocalMetre, ns2:kilogramPerCubicmetre, ns2:gramPerCubicmetre, ns2:milligramPerCubicmetre, ns2:gramPerCubicCentimetre, ns2:microgramPerCubicCentimetre, ns2:kilogramPerCubicDecimetre, ns2:cubicMetrePerKilogram, ns2:litrePerKilogram, ns2:amperePerSquareMetre, ns2:amperePerMetre, ns2:molePerCubicmetre, ns2:candelaPerSquareMetre, ns2:radian, ns2:steradian, ns2:hertz, ns2:newton, ns2:pascal, ns2:joule, ns2:watt, ns2:coulomb, ns2:volt, ns2:farad, ns2:ohm, ns2:siemens, ns2:weber, ns2:tesla, ns2:henry, ns2:degreeCelsius, ns2:lumen, ns2:lux, ns2:becquerel, ns2:gray, ns2:sievert, ns2:katal, ns2:radianPerSecond-Time, ns2:radianPerSecond-TimeSquared, ns2:pascalSecond-Time, ns2:newtonMetre, ns2:wattPerSquareMetre, ns2:wattPerSteradian, ns2:wattPerSquareMetreSteradian, ns2:joulePerKelvin, ns2:joulePerKelvinKilogram, ns2:joulePerKilogram, ns2:wattPerMetreKelvin, ns2:joulePerCubicmetre, ns2:voltPerMetre, ns2:coulombPerCubicmetre, ns2:coulombPerSquareMetre, ns2:faradPerMetre, ns2:henryPerMetre, ns2:joulePerMole, ns2:joulePerKelvinMole, ns2:coulombPerKilogram, ns2:grayPerSecond-Time, ns2:milligrayPerSecond-Time, ns2:yoctometre, ns2:zeptometre, ns2:attometre, ns2:picometre, ns2:femtometre, ns2:nanometre, ns2:micrometre, ns2:millimetre, ns2:centimetre, ns2:decimetre, ns2:decametre, ns2:hectometre, ns2:kilometre, ns2:megametre, ns2:gigametre, ns2:terametre, ns2:petametre, ns2:exametre, ns2:zettametre, ns2:yottametre, ns2:yoctogram, ns2:zeptogram, ns2:attogram, ns2:picogram, ns2:femtogram, ns2:nanogram, ns2:microgram, ns2:milligram, ns2:centigram, ns2:decigram, ns2:gram, ns2:decagram, ns2:hectogram, ns2:megagram, ns2:gigagram, ns2:teragram, ns2:petagram, ns2:exagram, ns2:zettagram, ns2:yottagram, ns2:yoctosecond-Time, ns2:zeptosecond-Time, ns2:attosecond-Time, ns2:picosecond-Time, ns2:femtosecond-Time, ns2:nanosecond-Time, ns2:microsecond-Time, ns2:millisecond-Time, ns2:centisecond-Time, ns2:decisecond-Time, ns2:decasecond-Time, ns2:hectosecond-Time, ns2:kilosecond-Time, ns2:megasecond-Time, ns2:gigasecond-Time, ns2:terasecond-Time, ns2:petasecond-Time, ns2:exasecond-Time, ns2:zettasecond-Time, ns2:yottasecond-Time, ns2:yoctoampere, ns2:zeptoampere, ns2:attoampere, ns2:picoampere, ns2:femtoampere, ns2:nanoampere, ns2:microampere, ns2:milliampere, ns2:centiampere, ns2:deciampere, ns2:decaampere, ns2:hectoampere, ns2:kiloampere, ns2:megaampere, ns2:gigaampere, ns2:teraampere, ns2:petaampere, ns2:exaampere, ns2:zettaampere, ns2:yottaampere, ns2:yoctokelvin, ns2:zeptokelvin, ns2:attokelvin, ns2:picokelvin, ns2:femtokelvin, ns2:nanokelvin, ns2:microkelvin, ns2:millikelvin, ns2:centikelvin, ns2:decikelvin, ns2:decakelvin, ns2:hectokelvin, ns2:kilokelvin, ns2:megakelvin, ns2:gigakelvin, ns2:terakelvin, ns2:petakelvin, ns2:exakelvin, ns2:zettakelvin, ns2:yottakelvin, ns2:yoctomole, ns2:zeptomole, ns2:attomole, ns2:picomole, ns2:femtomole, ns2:nanomole, ns2:micromole, ns2:millimole, ns2:centimole, ns2:decimole, ns2:decamole, ns2:hectomole, ns2:kilomole, ns2:megamole, ns2:gigamole, ns2:teramole, ns2:petamole, ns2:examole, ns2:zettamole, ns2:yottamole, ns2:yoctocandela, ns2:zeptocandela, ns2:attocandela, ns2:picocandela, ns2:femtocandela, ns2:nanocandela, ns2:microcandela, ns2:millicandela, ns2:centicandela, ns2:decicandela, ns2:decacandela, ns2:hectocandela, ns2:kilocandela, ns2:megacandela, ns2:gigacandela, ns2:teracandela, ns2:petacandela, ns2:exacandela, ns2:zettacandela, ns2:yottacandela, ns2:squareYoctometre, ns2:squareZeptometre, ns2:squareAttometre, ns2:squarePicometre, ns2:squareFemtometre, ns2:squareNanometre, ns2:squareMicrometre, ns2:squareMillimetre, ns2:squareCentimetre, ns2:squareDecimetre, ns2:squareDecametre, ns2:squareHectometre, ns2:squareKilometre, ns2:squareMegametre, ns2:squareGigametre, ns2:squareTerametre, ns2:squarePetametre, ns2:squareExametre, ns2:squareZettametre, ns2:squareYottametre, ns2:cubicYoctometre, ns2:cubicZeptometre, ns2:cubicAttometre, ns2:cubicPicometre, ns2:cubicFemtometre, ns2:cubicNanometre, ns2:cubicMicrometre, ns2:cubicMillimetre, ns2:cubicCentimetre, ns2:cubicDecimetre, ns2:cubicDecametre, ns2:cubicHectometre, ns2:cubicKilometre, ns2:cubicMegametre, ns2:cubicGigametre, ns2:cubicTerametre, ns2:cubicPetametre, ns2:cubicExametre, ns2:cubicZettametre, ns2:cubicYottametre, ns2:yoctometrePerSecond-Time, ns2:zeptometrePerSecond-Time, ns2:attometrePerSecond-Time, ns2:picometrePerSecond-Time, ns2:femtometrePerSecond-Time, ns2:nanometrePerSecond-Time, ns2:micrometrePerSecond-Time, ns2:millimetrePerSecond-Time, ns2:centimetrePerSecond-Time, ns2:decimetrePerSecond-Time, ns2:decametrePerSecond-Time, ns2:hectometrePerSecond-Time, ns2:kilometrePerSecond-Time, ns2:megametrePerSecond-Time, ns2:gigametrePerSecond-Time, ns2:terametrePerSecond-Time, ns2:petametrePerSecond-Time, ns2:exametrePerSecond-Time, ns2:zettametrePerSecond-Time, ns2:yottametrePerSecond-Time, ns2:metrePerYoctosecond-Time, ns2:metrePerZeptosecond-Time, ns2:metrePerAttosecond-Time, ns2:metrePerPicosecond-Time, ns2:metrePerFemtosecond-Time, ns2:metrePerNanosecond-Time, ns2:metrePerMicrosecond-Time, ns2:metrePerMillisecond-Time, ns2:metrePerCentisecond-Time, ns2:metrePerDecisecond-Time, ns2:metrePerDecasecond-Time, ns2:metrePerHectosecond-Time, ns2:metrePerKilosecond-Time, ns2:metrePerMegasecond-Time, ns2:metrePerGigasecond-Time, ns2:metrePerTerasecond-Time, ns2:metrePerPetasecond-Time, ns2:metrePerExasecond-Time, ns2:metrePerZettasecond-Time, ns2:metrePerYottasecond-Time, ns2:yoctometrePerSecond-TimeSquared, ns2:zeptometrePerSecond-TimeSquared, ns2:attometrePerSecond-TimeSquared, ns2:picometrePerSecond-TimeSquared, ns2:femtometrePerSecond-TimeSquared, ns2:nanometrePerSecond-TimeSquared, ns2:micrometrePerSecond-TimeSquared, ns2:millimetrePerSecond-TimeSquared, ns2:centimetrePerSecond-TimeSquared, ns2:decimetrePerSecond-TimeSquared, ns2:decametrePerSecond-TimeSquared, ns2:hectometrePerSecond-TimeSquared, ns2:kilometrePerSecond-TimeSquared, ns2:megametrePerSecond-TimeSquared, ns2:gigametrePerSecond-TimeSquared, ns2:terametrePerSecond-TimeSquared, ns2:petametrePerSecond-TimeSquared, ns2:exametrePerSecond-TimeSquared, ns2:zettametrePerSecond-TimeSquared, ns2:yottametrePerSecond-TimeSquared, ns2:metrePerYoctosecond-TimeSquared, ns2:metrePerZeptosecond-TimeSquared, ns2:metrePerAttosecond-TimeSquared, ns2:metrePerPicosecond-TimeSquared, ns2:metrePerFemtosecond-TimeSquared, ns2:metrePerNanosecond-TimeSquared, ns2:metrePerMicrosecond-TimeSquared, ns2:metrePerMillisecond-TimeSquared, ns2:metrePerCentisecond-TimeSquared, ns2:metrePerDecisecond-TimeSquared, ns2:metrePerDecasecond-TimeSquared, ns2:metrePerHectosecond-TimeSquared, ns2:metrePerKilosecond-TimeSquared, ns2:metrePerMegasecond-TimeSquared, ns2:metrePerGigasecond-TimeSquared, ns2:metrePerTerasecond-TimeSquared, ns2:metrePerPetasecond-TimeSquared, ns2:metrePerExasecond-TimeSquared, ns2:metrePerZettasecond-TimeSquared, ns2:metrePerYottasecond-TimeSquared, ns2:yoctoradian, ns2:zeptoradian, ns2:attoradian, ns2:picoradian, ns2:femtoradian, ns2:nanoradian, ns2:microradian, ns2:milliradian, ns2:centiradian, ns2:deciradian, ns2:yoctosteradian, ns2:zeptosteradian, ns2:attosteradian, ns2:picosteradian, ns2:femtosteradian, ns2:nanosteradian, ns2:microsteradian, ns2:millisteradian, ns2:centisteradian, ns2:decisteradian, ns2:yoctohertz, ns2:zeptohertz, ns2:attohertz, ns2:picohertz, ns2:femtohertz, ns2:nanohertz, ns2:microhertz, ns2:millihertz, ns2:centihertz, ns2:decihertz, ns2:decahertz, ns2:hectohertz, ns2:kilohertz, ns2:megahertz, ns2:gigahertz, ns2:terahertz, ns2:petahertz, ns2:exahertz, ns2:zettahertz, ns2:yottahertz, ns2:yoctonewton, ns2:zeptonewton, ns2:attonewton, ns2:piconewton, ns2:femtonewton, ns2:nanonewton, ns2:micronewton, ns2:millinewton, ns2:centinewton, ns2:decinewton, ns2:decanewton, ns2:hectonewton, ns2:kilonewton, ns2:meganewton, ns2:giganewton, ns2:teranewton, ns2:petanewton, ns2:exanewton, ns2:zettanewton, ns2:yottanewton, ns2:yoctopascal, ns2:zeptopascal, ns2:attopascal, ns2:picopascal, ns2:femtopascal, ns2:nanopascal, ns2:micropascal, ns2:millipascal, ns2:centipascal, ns2:decipascal, ns2:decapascal, ns2:hectopascal, ns2:kilopascal, ns2:megapascal, ns2:gigapascal, ns2:terapascal, ns2:petapascal, ns2:exapascal, ns2:zettapascal, ns2:yottapascal, ns2:yoctojoule, ns2:zeptojoule, ns2:attojoule, ns2:picojoule, ns2:femtojoule, ns2:nanojoule, ns2:microjoule, ns2:millijoule, ns2:centijoule, ns2:decijoule, ns2:decajoule, ns2:hectojoule, ns2:kilojoule, ns2:megajoule, ns2:gigajoule, ns2:terajoule, ns2:petajoule, ns2:exajoule, ns2:zettajoule, ns2:yottajoule, ns2:yoctowatt, ns2:zeptowatt, ns2:attowatt, ns2:picowatt, ns2:femtowatt, ns2:nanowatt, ns2:microwatt, ns2:milliwatt, ns2:centiwatt, ns2:deciwatt, ns2:decawatt, ns2:hectowatt, ns2:kilowatt, ns2:megawatt, ns2:gigawatt, ns2:terawatt, ns2:petawatt, ns2:exawatt, ns2:zettawatt, ns2:yottawatt, ns2:yoctocoulomb, ns2:zeptocoulomb, ns2:attocoulomb, ns2:picocoulomb, ns2:femtocoulomb, ns2:nanocoulomb, ns2:microcoulomb, ns2:millicoulomb, ns2:centicoulomb, ns2:decicoulomb, ns2:decacoulomb, ns2:hectocoulomb, ns2:kilocoulomb, ns2:megacoulomb, ns2:gigacoulomb, ns2:teracoulomb, ns2:petacoulomb, ns2:exacoulomb, ns2:zettacoulomb, ns2:yottacoulomb, ns2:yoctovolt, ns2:zeptovolt, ns2:attovolt, ns2:picovolt, ns2:femtovolt, ns2:nanovolt, ns2:microvolt, ns2:millivolt, ns2:centivolt, ns2:decivolt, ns2:decavolt, ns2:hectovolt, ns2:kilovolt, ns2:megavolt, ns2:gigavolt, ns2:teravolt, ns2:petavolt, ns2:exavolt, ns2:zettavolt, ns2:yottavolt, ns2:yoctofarad, ns2:zeptofarad, ns2:attofarad, ns2:picofarad, ns2:femtofarad, ns2:nanofarad, ns2:microfarad, ns2:millifarad, ns2:centifarad, ns2:decifarad, ns2:decafarad, ns2:hectofarad, ns2:kilofarad, ns2:megafarad, ns2:gigafarad, ns2:terafarad, ns2:petafarad, ns2:exafarad, ns2:zettafarad, ns2:yottafarad, ns2:yoctoohm, ns2:zeptoohm, ns2:attoohm, ns2:picoohm, ns2:femtoohm, ns2:nanoohm, ns2:microohm, ns2:milliohm, ns2:centiohm, ns2:deciohm, ns2:decaohm, ns2:hectoohm, ns2:kilohm, ns2:megohm, ns2:gigaohm, ns2:teraohm, ns2:petaohm, ns2:exaohm, ns2:zettaohm, ns2:yottaohm, ns2:yoctosiemens, ns2:zeptosiemens, ns2:attosiemens, ns2:picosiemens, ns2:femtosiemens, ns2:nanosiemens, ns2:microsiemens, ns2:millisiemens, ns2:centisiemens, ns2:decisiemens, ns2:decasiemens, ns2:hectosiemens, ns2:kilosiemens, ns2:megasiemens, ns2:gigasiemens, ns2:terasiemens, ns2:petasiemens, ns2:exasiemens, ns2:zettasiemens, ns2:yottasiemens, ns2:yoctoweber, ns2:zeptoweber, ns2:attoweber, ns2:picoweber, ns2:femtoweber, ns2:nanoweber, ns2:microweber, ns2:milliweber, ns2:centiweber, ns2:deciweber, ns2:decaweber, ns2:hectoweber, ns2:kiloweber, ns2:megaweber, ns2:gigaweber, ns2:teraweber, ns2:petaweber, ns2:exaweber, ns2:zettaweber, ns2:yottaweber, ns2:yoctotesla, ns2:zeptotesla, ns2:attotesla, ns2:picotesla, ns2:femtotesla, ns2:nanotesla, ns2:microtesla, ns2:millitesla, ns2:centitesla, ns2:decitesla, ns2:decatesla, ns2:hectotesla, ns2:kilotesla, ns2:megatesla, ns2:gigatesla, ns2:teratesla, ns2:petatesla, ns2:exatesla, ns2:zettatesla, ns2:yottatesla, ns2:yoctohenry, ns2:zeptohenry, ns2:attohenry, ns2:picohenry, ns2:femtohenry, ns2:nanohenry, ns2:microhenry, ns2:millihenry, ns2:centihenry, ns2:decihenry, ns2:decahenry, ns2:hectohenry, ns2:kilohenry, ns2:megahenry, ns2:gigahenry, ns2:terahenry, ns2:petahenry, ns2:exahenry, ns2:zettahenry, ns2:yottahenry, ns2:yoctodegreeCelsius, ns2:zeptodegreeCelsius, ns2:attodegreeCelsius, ns2:picodegreeCelsius, ns2:femtodegreeCelsius, ns2:nanodegreeCelsius, ns2:microdegreeCelsius, ns2:millidegreeCelsius, ns2:centidegreeCelsius, ns2:decidegreeCelsius, ns2:yoctolumen, ns2:zeptolumen, ns2:attolumen, ns2:picolumen, ns2:femtolumen, ns2:nanolumen, ns2:microlumen, ns2:millilumen, ns2:centilumen, ns2:decilumen, ns2:decalumen, ns2:hectolumen, ns2:kilolumen, ns2:megalumen, ns2:gigalumen, ns2:teralumen, ns2:petalumen, ns2:exalumen, ns2:zettalumen, ns2:yottalumen, ns2:yoctolux, ns2:zeptolux, ns2:attolux, ns2:picolux, ns2:femtolux, ns2:nanolux, ns2:microlux, ns2:millilux, ns2:centilux, ns2:decilux, ns2:decalux, ns2:hectolux, ns2:kilolux, ns2:megalux, ns2:gigalux, ns2:teralux, ns2:petalux, ns2:exalux, ns2:zettalux, ns2:yottalux, ns2:yoctobecquerel, ns2:zeptobecquerel, ns2:attobecquerel, ns2:picobecquerel, ns2:femtobecquerel, ns2:nanobecquerel, ns2:microbecquerel, ns2:millibecquerel, ns2:centibecquerel, ns2:decibecquerel, ns2:decabecquerel, ns2:hectobecquerel, ns2:kilobecquerel, ns2:megabecquerel, ns2:gigabecquerel, ns2:terabecquerel, ns2:petabecquerel, ns2:exabecquerel, ns2:zettabecquerel, ns2:yottabecquerel, ns2:yoctogray, ns2:zeptogray, ns2:attogray, ns2:picogray, ns2:femtogray, ns2:nanogray, ns2:microgray, ns2:milligray, ns2:centigray, ns2:decigray, ns2:decagray, ns2:hectogray, ns2:kilogray, ns2:megagray, ns2:gigagray, ns2:teragray, ns2:petagray, ns2:exagray, ns2:zettagray, ns2:yottagray, ns2:yoctosievert, ns2:zeptosievert, ns2:attosievert, ns2:picosievert, ns2:femtosievert, ns2:nanosievert, ns2:microsievert, ns2:millisievert, ns2:centisievert, ns2:decisievert, ns2:decasievert, ns2:hectosievert, ns2:kilosievert, ns2:megasievert, ns2:gigasievert, ns2:terasievert, ns2:petasievert, ns2:exasievert, ns2:zettasievert, ns2:yottasievert, ns2:yoctokatal, ns2:zeptokatal, ns2:attokatal, ns2:picokatal, ns2:femtokatal, ns2:nanokatal, ns2:microkatal, ns2:millikatal, ns2:centikatal, ns2:decikatal, ns2:decakatal, ns2:hectokatal, ns2:kilokatal, ns2:megakatal, ns2:gigakatal, ns2:terakatal, ns2:petakatal, ns2:exakatal, ns2:zettakatal, ns2:yottakatal, ns2:kilojoulePerHectogram .

ns2:metre-Kilogram-Second-AmpereSystemOfUnits
  a ns2:SystemOfUnits ;
  rdfs:label "metre-kilogram-second-ampere system of units"@en, "meter-kilogram-seconde-ampère-systeem"@nl ;
  ns2:alternativeLabel "Giorgi system of units"@en, "Giorgi-stelsel"@nl ;
  ns2:abbreviation "m-kg-s-A"^^xsd:string ;
  ns2:hasBaseQuantity ns2:Length, ns2:Mass, ns2:Time, ns2:ElectricCurrent ;
  ns2:hasDerivedQuantity ns2:Frequency, ns2:Force, ns2:Energy, ns2:Power, ns2:ElectricCharge, ns2:ElectricPotential, ns2:Capacitance, ns2:ElectricalResistance, ns2:Inductance, ns2:MagneticFlux, ns2:MagneticFluxDensity, ns2:MagnetomotiveForce ;
  ns2:hasBaseUnit ns2:metre, ns2:kilogram, ns2:second-Time, ns2:ampere ;
  ns2:hasDerivedUnit ns2:hertz, ns2:newton, ns2:joule, ns2:watt, ns2:coulomb, ns2:volt, ns2:farad, ns2:ohm, ns2:henry, ns2:weber, ns2:tesla .

ns2:mechanics
  a ns2:ApplicationArea ;
  rdfs:label "mechanics"@en, "mechanica"@nl ;
  ns2:usesQuantity ns2:Wavelength, ns2:Time, ns2:Period, ns2:Mass, ns2:Wavenumber, ns2:Frequency, ns2:AngularSpeed, ns2:Speed, ns2:Velocity, ns2:Acceleration, ns2:AngularAcceleration, ns2:Density, ns2:SpecificVolume, ns2:Momentum, ns2:Action, ns2:AngularMomentum, ns2:MomentOfInertia, ns2:Force, ns2:Impulse, ns2:Weight, ns2:Torque, ns2:Pressure, ns2:DynamicViscosity, ns2:KinematicViscosity, ns2:Energy, ns2:Enthalpy, ns2:KineticEnergy, ns2:PotentialEnergy, ns2:Work, ns2:Power, ns2:MassFraction, ns2:AreaFraction, ns2:VolumeFraction ;
  ns2:usesUnit ns2:kayser, ns2:reciprocalMetre, ns2:day, ns2:hour, ns2:minute-Time, ns2:second-Time, ns2:microsecond-Time, ns2:millisecond-Time, ns2:centisecond-Time, ns2:decisecond-Time, ns2:decasecond-Time, ns2:hectosecond-Time, ns2:kilosecond-Time, ns2:megasecond-Time, ns2:gigasecond-Time, ns2:year, ns2:gigayear, ns2:attosecond-Time, ns2:femtosecond-Time, ns2:picosecond-Time, ns2:nanosecond-Time, ns2:shake, ns2:day-Sidereal, ns2:hour-Sidereal, ns2:minute-Sidereal, ns2:second-Sidereal, ns2:terasecond-Time, ns2:petasecond-Time, ns2:exasecond-Time, ns2:year-Sidereal, ns2:year-Tropical, ns2:hertz, ns2:reciprocalSecond-Time, ns2:microhertz, ns2:millihertz, ns2:centihertz, ns2:decihertz, ns2:decahertz, ns2:hectohertz, ns2:kilohertz, ns2:megahertz, ns2:gigahertz, ns2:attohertz, ns2:femtohertz, ns2:picohertz, ns2:nanohertz, ns2:terahertz, ns2:petahertz, ns2:exahertz, ns2:centimetrePerSecond-Time, ns2:decametrePerSecond-Time, ns2:decimetrePerSecond-Time, ns2:gigametrePerSecond-Time, ns2:hectometrePerSecond-Time, ns2:kilometrePerSecond-Time, ns2:megametrePerSecond-Time, ns2:metrePerCentisecond-Time, ns2:metrePerDecasecond-Time, ns2:metrePerDecisecond-Time, ns2:metrePerGigasecond-Time, ns2:metrePerHectosecond-Time, ns2:metrePerKilosecond-Time, ns2:metrePerMegasecond-Time, ns2:metrePerMicrosecond-Time, ns2:metrePerMillisecond-Time, ns2:metrePerSecond-Time, ns2:micrometrePerSecond-Time, ns2:millimetrePerSecond-Time, ns2:millimetrePerHour, ns2:kilometrePerHour, ns2:centimetrePerDay, ns2:metrePerDay, ns2:millimetrePerDay, ns2:knot-International, ns2:nauticalMile-InternationalPerHour, ns2:attometrePerSecond-Time, ns2:femtometrePerSecond-Time, ns2:nanometrePerSecond-Time, ns2:picometrePerSecond-Time, ns2:metrePerExasecond-Time, ns2:metrePerPetasecond-Time, ns2:metrePerTerasecond-Time, ns2:exametrePerSecond-Time, ns2:metrePerAttosecond-Time, ns2:metrePerFemtosecond-Time, ns2:metrePerNanosecond-Time, ns2:metrePerPicosecond-Time, ns2:petametrePerSecond-Time, ns2:terametrePerSecond-Time, ns2:centimetrePerSecond-TimeSquared, ns2:decametrePerSecond-TimeSquared, ns2:decimetrePerSecond-TimeSquared, ns2:gal, ns2:gigametrePerSecond-TimeSquared, ns2:hectometrePerSecond-TimeSquared, ns2:kilometrePerSecond-TimeSquared, ns2:megametrePerSecond-TimeSquared, ns2:metrePerCentisecond-TimeSquared, ns2:metrePerDecasecond-TimeSquared, ns2:metrePerDecisecond-TimeSquared, ns2:metrePerGigasecond-TimeSquared, ns2:metrePerHectosecond-TimeSquared, ns2:metrePerKilosecond-TimeSquared, ns2:metrePerMegasecond-TimeSquared, ns2:metrePerMicrosecond-TimeSquared, ns2:metrePerMillisecond-TimeSquared, ns2:metrePerSecond-TimeSquared, ns2:micrometrePerSecond-TimeSquared, ns2:millimetrePerSecond-TimeSquared, ns2:attometrePerSecond-TimeSquared, ns2:femtometrePerSecond-TimeSquared, ns2:nanometrePerSecond-TimeSquared, ns2:picometrePerSecond-TimeSquared, ns2:metrePerExasecond-TimeSquared, ns2:metrePerPetasecond-TimeSquared, ns2:metrePerTerasecond-TimeSquared, ns2:exametrePerSecond-TimeSquared, ns2:petametrePerSecond-TimeSquared, ns2:terametrePerSecond-TimeSquared, ns2:metrePerAttosecond-TimeSquared, ns2:metrePerFemtosecond-TimeSquared, ns2:metrePerNanosecond-TimeSquared, ns2:metrePerPicosecond-TimeSquared, ns2:radianPerSecond-TimeSquared .

ns2:Displacement
  a owl:Class ;
  rdfs:label "displacement"@en, "verplaatsing"@nl ;
  rdfs:subClassOf ns2:Length ;
  ns2:symbol "d" ;
  ns2:commonlyHasUnit ns2:metre, ns2:attometre, ns2:centimetre, ns2:decametre, ns2:decimetre, ns2:exametre, ns2:femtometre, ns2:gigametre, ns2:hectometre, ns2:kilometre, ns2:megametre, ns2:micrometre, ns2:millimetre, ns2:nanometre, ns2:petametre, ns2:picometre, ns2:terametre, ns2:angstrom, ns2:chain, ns2:fathom-USSurvey, ns2:fermi, ns2:foot-International, ns2:foot-USSurvey, ns2:furlong-International, ns2:inch-International, ns2:micron, ns2:mil-Length, ns2:mile-Statute, ns2:mile-USSurvey, ns2:nauticalMile-International, ns2:rod-US, ns2:yard-International, ns2:astronomicalUnit, ns2:lightYear, ns2:parsec, ns2:solarRadius, ns2:gigaparsec, ns2:kiloparsec, ns2:megaparsec, ns2:cicero, ns2:pica-ATA, ns2:pica-Postscript, ns2:pica-TeX, ns2:point-ATA, ns2:point-Didot, ns2:point-Postscript, ns2:point-TeX .

ns2:Wavelength
  a owl:Class ;
  rdfs:label "wavelength"@en, "golflengte"@nl ;
  rdfs:subClassOf ns2:Length ;
  ns2:symbol "λ" ;
  ns2:commonlyHasUnit ns2:metre, ns2:attometre, ns2:centimetre, ns2:decametre, ns2:decimetre, ns2:exametre, ns2:femtometre, ns2:gigametre, ns2:hectometre, ns2:kilometre, ns2:megametre, ns2:micrometre, ns2:millimetre, ns2:nanometre, ns2:petametre, ns2:picometre, ns2:terametre, ns2:angstrom, ns2:chain, ns2:fathom-USSurvey, ns2:fermi, ns2:foot-International, ns2:foot-USSurvey, ns2:furlong-International, ns2:inch-International, ns2:micron, ns2:mil-Length, ns2:mile-Statute, ns2:mile-USSurvey, ns2:nauticalMile-International, ns2:rod-US, ns2:yard-International, ns2:astronomicalUnit, ns2:lightYear, ns2:parsec, ns2:solarRadius, ns2:gigaparsec, ns2:kiloparsec, ns2:megaparsec, ns2:cicero, ns2:pica-ATA, ns2:pica-Postscript, ns2:pica-TeX, ns2:point-ATA, ns2:point-Didot, ns2:point-Postscript, ns2:point-TeX .

ns2:Time
  a owl:Class ;
  rdfs:label "time"@en, "tijd"@nl, "时间"@zh ;
  rdfs:comment "Time is a base quantity in the International System of Units and other systems of units. It is measured by numbers of repetitions of cyclical events."@en ;
  rdfs:subClassOf ns2:Quantity, [
    a owl:Restriction ;
    owl:onProperty ns2:hasValue ;
    owl:allValuesFrom [
      a owl:Restriction ;
      owl:onProperty ns2:hasUnit ;
      owl:allValuesFrom ns2:TimeUnit
    ]
  ], [
    a owl:Restriction ;
    owl:onProperty ns2:hasDimension ;
    owl:hasValue ns2:time-Dimension
  ] ;
  ns2:symbol "t" ;
  ns2:commonlyHasUnit ns2:second-Time, ns2:attosecond-Time, ns2:centisecond-Time, ns2:decasecond-Time, ns2:decisecond-Time, ns2:exasecond-Time, ns2:femtosecond-Time, ns2:gigasecond-Time, ns2:hectosecond-Time, ns2:kilosecond-Time, ns2:megasecond-Time, ns2:microsecond-Time, ns2:millisecond-Time, ns2:nanosecond-Time, ns2:petasecond-Time, ns2:picosecond-Time, ns2:terasecond-Time, ns2:day, ns2:hour, ns2:minute-Time, ns2:shake, ns2:year, ns2:day-Sidereal, ns2:gigayear, ns2:hour-Sidereal, ns2:minute-Sidereal, ns2:second-Sidereal, ns2:year-Sidereal, ns2:year-Tropical .

ns2:Date
  a owl:Class ;
  rdfs:label "date"@en, "datum"@nl ;
  rdfs:subClassOf ns2:Time ;
  ns2:commonlyHasUnit ns2:second-Time, ns2:attosecond-Time, ns2:centisecond-Time, ns2:decasecond-Time, ns2:decisecond-Time, ns2:exasecond-Time, ns2:femtosecond-Time, ns2:gigasecond-Time, ns2:hectosecond-Time, ns2:kilosecond-Time, ns2:megasecond-Time, ns2:microsecond-Time, ns2:millisecond-Time, ns2:nanosecond-Time, ns2:petasecond-Time, ns2:picosecond-Time, ns2:terasecond-Time, ns2:day, ns2:hour, ns2:minute-Time, ns2:shake, ns2:year, ns2:day-Sidereal, ns2:gigayear, ns2:hour-Sidereal, ns2:minute-Sidereal, ns2:second-Sidereal, ns2:year-Sidereal, ns2:year-Tropical .

ns2:Duration
  a owl:Class ;
  rdfs:label "duration"@en, "duur"@nl ;
  rdfs:subClassOf ns2:Time ;
  ns2:commonlyHasUnit ns2:second-Time, ns2:attosecond-Time, ns2:centisecond-Time, ns2:decasecond-Time, ns2:decisecond-Time, ns2:exasecond-Time, ns2:femtosecond-Time, ns2:gigasecond-Time, ns2:hectosecond-Time, ns2:kilosecond-Time, ns2:megasecond-Time, ns2:microsecond-Time, ns2:millisecond-Time, ns2:nanosecond-Time, ns2:petasecond-Time, ns2:picosecond-Time, ns2:terasecond-Time, ns2:day, ns2:hour, ns2:minute-Time, ns2:shake, ns2:year, ns2:day-Sidereal, ns2:gigayear, ns2:hour-Sidereal, ns2:minute-Sidereal, ns2:second-Sidereal, ns2:year-Sidereal, ns2:year-Tropical .

ns2:Period
  a owl:Class ;
  rdfs:label "period"@en, "periode"@nl ;
  rdfs:subClassOf ns2:Time ;
  ns2:symbol "T" ;
  ns2:commonlyHasUnit ns2:second-Time, ns2:attosecond-Time, ns2:centisecond-Time, ns2:decasecond-Time, ns2:decisecond-Time, ns2:exasecond-Time, ns2:femtosecond-Time, ns2:gigasecond-Time, ns2:hectosecond-Time, ns2:kilosecond-Time, ns2:megasecond-Time, ns2:microsecond-Time, ns2:millisecond-Time, ns2:nanosecond-Time, ns2:petasecond-Time, ns2:picosecond-Time, ns2:terasecond-Time, ns2:day, ns2:hour, ns2:minute-Time, ns2:shake, ns2:year, ns2:day-Sidereal, ns2:gigayear, ns2:hour-Sidereal, ns2:minute-Sidereal, ns2:second-Sidereal, ns2:year-Sidereal, ns2:year-Tropical .

ns2:Mass
  a owl:Class ;
  rdfs:label "mass"@en, "massa"@nl, "质量"@zh ;
  ns2:unofficialLabel "weight" ;
  rdfs:comment "Mass is the amount of matter of a phenomenon. It is a base quantity in the International System of Units. Mass is force divided by acceleration."@en ;
  rdfs:subClassOf ns2:Quantity, [
    a owl:Restriction ;
    owl:onProperty ns2:hasValue ;
    owl:allValuesFrom [
      a owl:Restriction ;
      owl:onProperty ns2:hasUnit ;
      owl:allValuesFrom ns2:MassUnit
    ]
  ], [
    a owl:Restriction ;
    owl:onProperty ns2:hasDimension ;
    owl:hasValue ns2:mass-Dimension
  ] ;
  ns2:symbol "m" ;
  ns2:commonlyHasUnit ns2:gram, ns2:attogram, ns2:exagram, ns2:centigram, ns2:decagram, ns2:decigram, ns2:femtogram, ns2:gigagram, ns2:hectogram, ns2:kilogram, ns2:megagram, ns2:microgram, ns2:milligram, ns2:nanogram, ns2:petagram, ns2:picogram, ns2:teragram, ns2:tonne, ns2:kilotonne, ns2:megatonne, ns2:unifiedAtomicMassUnit, ns2:nanounifiedAtomicMassUnit, ns2:carat-Mass, ns2:grain, ns2:hundredweight-British, ns2:hundredweight-US, ns2:InternationalUnit, ns2:milligramRAE, ns2:ounceAvoirdupois, ns2:ounceApothecaries, ns2:pennyweight-Troy, ns2:poundApothecaries, ns2:poundAvoirdupois, ns2:slug, ns2:ton-ShortAssay, ns2:ton-Long, ns2:ton-Short, ns2:solarMass .

ns2:AtomicMass
  a owl:Class ;
  rdfs:label "atomic mass"@en ;
  rdfs:subClassOf ns2:Mass ;
  ns2:symbol "m_a" ;
  ns2:commonlyHasUnit ns2:unifiedAtomicMassUnit, ns2:nanounifiedAtomicMassUnit .

ns2:QuantityOfDimensionOne
  a owl:Class ;
  rdfs:label "quantity of dimension one"@en ;
  rdfs:subClassOf ns2:Quantity, [
    a owl:Restriction ;
    owl:onProperty ns2:hasDimension ;
    owl:hasValue ns2:dimensionOne
  ], [
    a owl:Restriction ;
    owl:onProperty ns2:hasValue ;
    owl:allValuesFrom [
      a owl:Restriction ;
      owl:onProperty ns2:hasUnit ;
      owl:allValuesFrom ns2:QuantityOfDimensionOneUnit
    ]
  ] ;
  ns2:commonlyHasUnit ns2:one, ns2:percent, ns2:partsPerMillion, ns2:halfDozen, ns2:dozen, ns2:hundredCount, ns2:gross, ns2:thousandPiece .

ns2:Number
  a owl:Class ;
  rdfs:label "number"@en ;
  rdfs:subClassOf ns2:Quantity, [
    a owl:Restriction ;
    owl:onProperty ns2:hasDimension ;
    owl:hasValue ns2:dimensionOne
  ], [
    a owl:Restriction ;
    owl:onProperty ns2:hasValue ;
    owl:allValuesFrom [
      a owl:Restriction ;
      owl:onProperty ns2:hasUnit ;
      owl:allValuesFrom ns2:NumberUnit
    ]
  ] ;
  ns2:symbol "N" ;
  ns2:unofficialAbbreviation "nr", "no", "#" ;
  ns2:commonlyHasUnit ns2:one .

ns2:Ratio
  a owl:Class ;
  rdfs:label "ratio"@en ;
  rdfs:subClassOf ns2:Quantity, [
    a owl:Restriction ;
    owl:onProperty ns2:hasDimension ;
    owl:hasValue ns2:dimensionOne
  ], [
    a owl:Restriction ;
    owl:onProperty ns2:hasValue ;
    owl:allValuesFrom [
      a owl:Restriction ;
      owl:onProperty ns2:hasUnit ;
      owl:allValuesFrom ns2:RatioUnit
    ]
  ] ;
  ns2:commonlyHasUnit ns2:one, ns2:percent, ns2:partsPerMillion .

ns2:Percentage
  a owl:Class ;
  rdfs:label "percentage"@en ;
  rdfs:subClassOf ns2:Ratio, [
    a owl:Restriction ;
    owl:onProperty ns2:hasValue ;
    owl:allValuesFrom [
      a owl:Restriction ;
      owl:onProperty ns2:hasUnit ;
      owl:allValuesFrom ns2:PercentageUnit
    ]
  ] ;
  ns2:commonlyHasUnit ns2:one, ns2:percent .

ns2:NumberDensity
  a owl:Class ;
  rdfs:label "number density"@en ;
  rdfs:subClassOf ns2:Quantity, [
    a owl:Restriction ;
    owl:onProperty ns2:hasValue ;
    owl:allValuesFrom [
      a owl:Restriction ;
      owl:onProperty ns2:hasUnit ;
      owl:allValuesFrom ns2:NumberDensityUnit
    ]
  ], [
    a owl:Restriction ;
    owl:onProperty ns2:hasDimension ;
    owl:hasValue ns2:numberDensity-Dimension
  ] ;
  ns2:symbol "n" ;
  ns2:commonlyHasUnit ns2:reciprocalCubicMetre, ns2:reciprocalCubicCentimetre, ns2:reciprocalLitre, ns2:reciprocalCubicParsec .

ns2:ColumnNumberDensity
  a owl:Class ;
  rdfs:label "column number density"@en ;
  rdfs:subClassOf ns2:Quantity, [
    a owl:Restriction ;
    owl:onProperty ns2:hasValue ;
    owl:allValuesFrom [
      a owl:Restriction ;
      owl:onProperty ns2:hasUnit ;
      owl:allValuesFrom ns2:ColumnNumberDensityUnit
    ]
  ], [
    a owl:Restriction ;
    owl:onProperty ns2:hasDimension ;
    owl:hasValue ns2:columnNumberDensity-Dimension
  ] ;
  ns2:unofficialLabel "number density", "density" ;
  ns2:commonlyHasUnit ns2:reciprocalSquareMetre, ns2:reciprocalSquareCentimetre .

ns2:Wavenumber
  a owl:Class ;
  rdfs:label "wavenumber"@en, "golfgetal"@nl ;
  rdfs:comment "Wavenumber is the number of repeating units of a propagating wave (the number of times a wave has the same phase) per unit of space."@en ;
  rdfs:subClassOf ns2:Quantity, [
    a owl:Restriction ;
    owl:onProperty ns2:hasValue ;
    owl:allValuesFrom [
      a owl:Restriction ;
      owl:onProperty ns2:hasUnit ;
      owl:allValuesFrom ns2:WavenumberUnit
    ]
  ], [
    a owl:Restriction ;
    owl:onProperty ns2:hasDimension ;
    owl:hasValue ns2:wavenumber-Dimension
  ] ;
  ns2:symbol "σ" ;
  ns2:commonlyHasUnit ns2:reciprocalMetre, ns2:kayser .

ns2:AngularDisplacement
  a owl:Class ;
  rdfs:label "angular displacement"@en ;
  rdfs:subClassOf ns2:Angle ;
  ns2:commonlyHasUnit ns2:radian, ns2:attoradian, ns2:centiradian, ns2:deciradian, ns2:femtoradian, ns2:microradian, ns2:milliradian, ns2:nanoradian, ns2:picoradian, ns2:degree, ns2:gon, ns2:mil-Angle, ns2:minute-Angle, ns2:revolution, ns2:second-Angle, ns2:millisecond-Angle, ns2:microsecond-Angle, ns2:metrePerMetre .

ns2:Frequency
  a owl:Class ;
  rdfs:label "frequency"@en, "frequentie"@nl, "频率"@zh ;
  ns2:unofficialAbbreviation "freq" ;
  rdfs:comment "Frequency is a measure of the number of occurrences of a repeating event per unit time."@en ;
  rdfs:subClassOf ns2:Quantity, [
    a owl:Restriction ;
    owl:onProperty ns2:hasValue ;
    owl:allValuesFrom [
      a owl:Restriction ;
      owl:onProperty ns2:hasUnit ;
      owl:allValuesFrom ns2:FrequencyUnit
    ]
  ], [
    a owl:Restriction ;
    owl:onProperty ns2:hasDimension ;
    owl:hasValue ns2:frequency-Dimension
  ] ;
  ns2:symbol "f" ;
  ns2:alternativeSymbol "ν" ;
  ns2:commonlyHasUnit ns2:reciprocalSecond-Time, ns2:hertz, ns2:attohertz, ns2:centihertz, ns2:decahertz, ns2:decihertz, ns2:exahertz, ns2:femtohertz, ns2:gigahertz, ns2:hectohertz, ns2:kilohertz, ns2:megahertz, ns2:microhertz, ns2:millihertz, ns2:nanohertz, ns2:petahertz, ns2:picohertz, ns2:terahertz, ns2:reciprocalMinute-Time, ns2:reciprocalHour, ns2:reciprocalDay, ns2:reciprocalYear .

ns2:Acceleration
  a owl:Class ;
  rdfs:label "acceleration"@en, "versnelling"@nl ;
  ns2:alternativeLabel "acceleratie"@nl ;
  rdfs:subClassOf ns2:Quantity, [
    a owl:Restriction ;
    owl:onProperty ns2:hasValue ;
    owl:allValuesFrom [
      a owl:Restriction ;
      owl:onProperty ns2:hasUnit ;
      owl:allValuesFrom ns2:AccelerationUnit
    ]
  ], [
    a owl:Restriction ;
    owl:onProperty ns2:hasDimension ;
    owl:hasValue ns2:acceleration-Dimension
  ] ;
  ns2:symbol "a" ;
  ns2:commonlyHasUnit ns2:metrePerSecond-TimeSquared, ns2:attometrePerSecond-TimeSquared, ns2:centimetrePerSecond-TimeSquared, ns2:decametrePerSecond-TimeSquared, ns2:decimetrePerSecond-TimeSquared, ns2:exametrePerSecond-TimeSquared, ns2:femtometrePerSecond-TimeSquared, ns2:gigametrePerSecond-TimeSquared, ns2:hectometrePerSecond-TimeSquared, ns2:kilometrePerSecond-TimeSquared, ns2:megametrePerSecond-TimeSquared, ns2:metrePerAttosecond-TimeSquared, ns2:metrePerCentisecond-TimeSquared, ns2:metrePerDecasecond-TimeSquared, ns2:metrePerDecisecond-TimeSquared, ns2:metrePerExasecond-TimeSquared, ns2:metrePerFemtosecond-TimeSquared, ns2:metrePerGigasecond-TimeSquared, ns2:metrePerHectosecond-TimeSquared, ns2:metrePerKilosecond-TimeSquared, ns2:metrePerMegasecond-TimeSquared, ns2:metrePerMicrosecond-TimeSquared, ns2:metrePerMillisecond-TimeSquared, ns2:metrePerNanosecond-TimeSquared, ns2:metrePerPetasecond-TimeSquared, ns2:metrePerPicosecond-TimeSquared, ns2:metrePerTerasecond-TimeSquared, ns2:micrometrePerSecond-TimeSquared, ns2:millimetrePerSecond-TimeSquared, ns2:nanometrePerSecond-TimeSquared, ns2:petametrePerSecond-TimeSquared, ns2:picometrePerSecond-TimeSquared, ns2:terametrePerSecond-TimeSquared, ns2:gal .

ns2:GravitationalAcceleration
  a owl:Class ;
  rdfs:label "gravitational acceleration"@en, "valversnelling"@nl ;
  ns2:alternativeLabel "acceleration of free fall"@en, "zwaarteveldsterkte"@nl, "gravitatieveldsterkte"@nl ;
  rdfs:subClassOf ns2:Acceleration ;
  ns2:symbol "g" ;
  ns2:commonlyHasUnit ns2:metrePerSecond-TimeSquared, ns2:attometrePerSecond-TimeSquared, ns2:centimetrePerSecond-TimeSquared, ns2:decametrePerSecond-TimeSquared, ns2:decimetrePerSecond-TimeSquared, ns2:exametrePerSecond-TimeSquared, ns2:femtometrePerSecond-TimeSquared, ns2:gigametrePerSecond-TimeSquared, ns2:hectometrePerSecond-TimeSquared, ns2:kilometrePerSecond-TimeSquared, ns2:megametrePerSecond-TimeSquared, ns2:metrePerAttosecond-TimeSquared, ns2:metrePerCentisecond-TimeSquared, ns2:metrePerDecasecond-TimeSquared, ns2:metrePerDecisecond-TimeSquared, ns2:metrePerExasecond-TimeSquared, ns2:metrePerFemtosecond-TimeSquared, ns2:metrePerGigasecond-TimeSquared, ns2:metrePerHectosecond-TimeSquared, ns2:metrePerKilosecond-TimeSquared, ns2:metrePerMegasecond-TimeSquared, ns2:metrePerMicrosecond-TimeSquared, ns2:metrePerMillisecond-TimeSquared, ns2:metrePerNanosecond-TimeSquared, ns2:metrePerPetasecond-TimeSquared, ns2:metrePerPicosecond-TimeSquared, ns2:metrePerTerasecond-TimeSquared, ns2:micrometrePerSecond-TimeSquared, ns2:millimetrePerSecond-TimeSquared, ns2:nanometrePerSecond-TimeSquared, ns2:petametrePerSecond-TimeSquared, ns2:picometrePerSecond-TimeSquared, ns2:terametrePerSecond-TimeSquared, ns2:gal .

ns2:Density
  a owl:Class ;
  rdfs:label "density"@en, "dichtheid"@nl, "密度"@zh ;
  ns2:alternativeLabel "mass density"@en, "soortelijke massa"@nl, "concentration (w/v)"@en ;
  rdfs:comment "Density is the concentration of matter. It is a derived quantity in the International System of Units. Density is mass divided by volume."@en ;
  rdfs:subClassOf ns2:Quantity, [
    a owl:Restriction ;
    owl:onProperty ns2:hasValue ;
    owl:allValuesFrom [
      a owl:Restriction ;
      owl:onProperty ns2:hasUnit ;
      owl:allValuesFrom ns2:DensityUnit
    ]
  ], [
    a owl:Restriction ;
    owl:onProperty ns2:hasDimension ;
    owl:hasValue ns2:density-Dimension
  ] ;
  ns2:symbol "ρ" ;
  ns2:commonlyHasUnit ns2:kilogramPerCubicmetre, ns2:gramPerCubicmetre, ns2:milligramPerCubicmetre, ns2:gramPerCubicCentimetre, ns2:microgramPerCubicCentimetre, ns2:kilogramPerCubicDecimetre, ns2:gramPerLitre, ns2:attogramPerLitre, ns2:centigramPerLitre, ns2:decagramPerLitre, ns2:decigramPerLitre, ns2:exagramPerLitre, ns2:femtogramPerLitre, ns2:gigagramPerLitre, ns2:hectogramPerLitre, ns2:kilogramPerLitre, ns2:megagramPerLitre, ns2:microgramPerLitre, ns2:milligramPerLitre, ns2:nanogramPerLitre, ns2:petagramPerLitre, ns2:picogramPerLitre, ns2:teragramPerLitre, ns2:gramPerAttolitre, ns2:gramPerCentilitre, ns2:gramPerDecalitre, ns2:gramPerDecilitre, ns2:gramPerExalitre, ns2:gramPerFemtolitre, ns2:gramPerGigalitre, ns2:gramPerHectolitre, ns2:gramPerKilolitre, ns2:gramPerMegalitre, ns2:gramPerMicrolitre, ns2:gramPerMillilitre, ns2:gramPerNanolitre, ns2:gramPerPetalitre, ns2:gramPerPicolitre, ns2:gramPerTeralitre .

ns2:SpecificVolume
  a owl:Class ;
  rdfs:label "specific volume"@en, "soortelijk volume"@nl ;
  ns2:alternativeLabel "specifiek volume"@nl, "concentration (v/w)"@en ;
  rdfs:comment "Specific volume is volume per unit mass."@en ;
  rdfs:subClassOf ns2:Quantity, [
    a owl:Restriction ;
    owl:onProperty ns2:hasValue ;
    owl:allValuesFrom [
      a owl:Restriction ;
      owl:onProperty ns2:hasUnit ;
      owl:allValuesFrom ns2:SpecificVolumeUnit
    ]
  ], [
    a owl:Restriction ;
    owl:onProperty ns2:hasDimension ;
    owl:hasValue ns2:specificVolume-Dimension
  ] ;
  ns2:symbol "v" ;
  ns2:commonlyHasUnit ns2:cubicMetrePerKilogram, ns2:litrePerKilogram .

ns2:Speed
  a owl:Class ;
  rdfs:label "speed"@en, "snelheid (scalair)"@nl, "速度"@zh ;
  rdfs:comment "Speed is the time rate of motion measured by the distance moved over in unit time."@en ;
  rdfs:subClassOf ns2:Quantity, [
    a owl:Restriction ;
    owl:onProperty ns2:hasValue ;
    owl:allValuesFrom [
      a owl:Restriction ;
      owl:onProperty ns2:hasUnit ;
      owl:allValuesFrom ns2:SpeedUnit
    ]
  ], [
    a owl:Restriction ;
    owl:onProperty ns2:hasDimension ;
    owl:hasValue ns2:speed-Dimension
  ] ;
  ns2:symbol "v" ;
  ns2:alternativeSymbol "u" ;
  ns2:commonlyHasUnit ns2:metrePerSecond-Time, ns2:attometrePerSecond-Time, ns2:centimetrePerSecond-Time, ns2:decametrePerSecond-Time, ns2:decimetrePerSecond-Time, ns2:exametrePerSecond-Time, ns2:femtometrePerSecond-Time, ns2:gigametrePerSecond-Time, ns2:hectometrePerSecond-Time, ns2:kilometrePerSecond-Time, ns2:megametrePerSecond-Time, ns2:metrePerAttosecond-Time, ns2:metrePerCentisecond-Time, ns2:metrePerDecasecond-Time, ns2:metrePerDecisecond-Time, ns2:metrePerExasecond-Time, ns2:metrePerFemtosecond-Time, ns2:metrePerGigasecond-Time, ns2:metrePerHectosecond-Time, ns2:metrePerKilosecond-Time, ns2:metrePerMegasecond-Time, ns2:metrePerMicrosecond-Time, ns2:metrePerMillisecond-Time, ns2:metrePerNanosecond-Time, ns2:metrePerPetasecond-Time, ns2:metrePerPicosecond-Time, ns2:metrePerTerasecond-Time, ns2:micrometrePerSecond-Time, ns2:millimetrePerSecond-Time, ns2:nanometrePerSecond-Time, ns2:petametrePerSecond-Time, ns2:picometrePerSecond-Time, ns2:terametrePerSecond-Time, ns2:knot-International, ns2:millimetrePerHour, ns2:kilometrePerHour, ns2:centimetrePerDay, ns2:metrePerDay, ns2:millimetrePerDay, ns2:mile-StatutePerHour, ns2:nauticalMile-InternationalPerHour .

ns2:Velocity
  a owl:Class ;
  rdfs:label "velocity"@en, "snelheid (vector)"@nl ;
  rdfs:comment "Velocity is the rate of change of position."@en ;
  rdfs:subClassOf ns2:Speed ;
  ns2:symbol "u" ;
  ns2:alternativeSymbol "v", "w" ;
  ns2:commonlyHasUnit ns2:metrePerSecond-Time, ns2:attometrePerSecond-Time, ns2:centimetrePerSecond-Time, ns2:decametrePerSecond-Time, ns2:decimetrePerSecond-Time, ns2:exametrePerSecond-Time, ns2:femtometrePerSecond-Time, ns2:gigametrePerSecond-Time, ns2:hectometrePerSecond-Time, ns2:kilometrePerSecond-Time, ns2:megametrePerSecond-Time, ns2:metrePerAttosecond-Time, ns2:metrePerCentisecond-Time, ns2:metrePerDecasecond-Time, ns2:metrePerDecisecond-Time, ns2:metrePerExasecond-Time, ns2:metrePerFemtosecond-Time, ns2:metrePerGigasecond-Time, ns2:metrePerHectosecond-Time, ns2:metrePerKilosecond-Time, ns2:metrePerMegasecond-Time, ns2:metrePerMicrosecond-Time, ns2:metrePerMillisecond-Time, ns2:metrePerNanosecond-Time, ns2:metrePerPetasecond-Time, ns2:metrePerPicosecond-Time, ns2:metrePerTerasecond-Time, ns2:micrometrePerSecond-Time, ns2:millimetrePerSecond-Time, ns2:nanometrePerSecond-Time, ns2:petametrePerSecond-Time, ns2:picometrePerSecond-Time, ns2:terametrePerSecond-Time, ns2:knot-International, ns2:millimetrePerHour, ns2:kilometrePerHour, ns2:centimetrePerDay, ns2:metrePerDay, ns2:millimetrePerDay, ns2:mile-StatutePerHour, ns2:nauticalMile-InternationalPerHour .

ns2:AverageSpeed
  a owl:Class ;
  rdfs:label "average speed"@en ;
  rdfs:subClassOf ns2:Speed ;
  ns2:symbol "u" ;
  owl:equivalentClass [
    a owl:Class ;
    owl:intersectionOf ( _:genid228 )
  ] ;
  ns2:commonlyHasUnit ns2:metrePerSecond-Time, ns2:attometrePerSecond-Time, ns2:centimetrePerSecond-Time, ns2:decametrePerSecond-Time, ns2:decimetrePerSecond-Time, ns2:exametrePerSecond-Time, ns2:femtometrePerSecond-Time, ns2:gigametrePerSecond-Time, ns2:hectometrePerSecond-Time, ns2:kilometrePerSecond-Time, ns2:megametrePerSecond-Time, ns2:metrePerAttosecond-Time, ns2:metrePerCentisecond-Time, ns2:metrePerDecasecond-Time, ns2:metrePerDecisecond-Time, ns2:metrePerExasecond-Time, ns2:metrePerFemtosecond-Time, ns2:metrePerGigasecond-Time, ns2:metrePerHectosecond-Time, ns2:metrePerKilosecond-Time, ns2:metrePerMegasecond-Time, ns2:metrePerMicrosecond-Time, ns2:metrePerMillisecond-Time, ns2:metrePerNanosecond-Time, ns2:metrePerPetasecond-Time, ns2:metrePerPicosecond-Time, ns2:metrePerTerasecond-Time, ns2:micrometrePerSecond-Time, ns2:millimetrePerSecond-Time, ns2:nanometrePerSecond-Time, ns2:petametrePerSecond-Time, ns2:picometrePerSecond-Time, ns2:terametrePerSecond-Time, ns2:knot-International, ns2:millimetrePerHour, ns2:kilometrePerHour, ns2:centimetrePerDay, ns2:metrePerDay, ns2:millimetrePerDay, ns2:mile-StatutePerHour, ns2:nauticalMile-InternationalPerHour .

ns2:DrainageSpeed
  a owl:Class ;
  rdfs:label "drainage speed"@en ;
  rdfs:subClassOf ns2:Speed ;
  ns2:commonlyHasUnit ns2:metrePerSecond-Time, ns2:attometrePerSecond-Time, ns2:centimetrePerSecond-Time, ns2:decametrePerSecond-Time, ns2:decimetrePerSecond-Time, ns2:exametrePerSecond-Time, ns2:femtometrePerSecond-Time, ns2:gigametrePerSecond-Time, ns2:hectometrePerSecond-Time, ns2:kilometrePerSecond-Time, ns2:megametrePerSecond-Time, ns2:metrePerAttosecond-Time, ns2:metrePerCentisecond-Time, ns2:metrePerDecasecond-Time, ns2:metrePerDecisecond-Time, ns2:metrePerExasecond-Time, ns2:metrePerFemtosecond-Time, ns2:metrePerGigasecond-Time, ns2:metrePerHectosecond-Time, ns2:metrePerKilosecond-Time, ns2:metrePerMegasecond-Time, ns2:metrePerMicrosecond-Time, ns2:metrePerMillisecond-Time, ns2:metrePerNanosecond-Time, ns2:metrePerPetasecond-Time, ns2:metrePerPicosecond-Time, ns2:metrePerTerasecond-Time, ns2:micrometrePerSecond-Time, ns2:millimetrePerSecond-Time, ns2:nanometrePerSecond-Time, ns2:petametrePerSecond-Time, ns2:picometrePerSecond-Time, ns2:terametrePerSecond-Time, ns2:knot-International, ns2:millimetrePerHour, ns2:kilometrePerHour, ns2:centimetrePerDay, ns2:metrePerDay, ns2:millimetrePerDay, ns2:mile-StatutePerHour, ns2:nauticalMile-InternationalPerHour .

ns2:Force
  a owl:Class ;
  rdfs:label "force"@en, "kracht"@nl, "力"@zh ;
  rdfs:comment "Force is the extent to which an object with mass can be caused to accelerate. It is a derived quantity in the International System of Units. Force is mass times acceleration."@en ;
  rdfs:subClassOf ns2:Quantity, [
    a owl:Restriction ;
    owl:onProperty ns2:hasValue ;
    owl:allValuesFrom [
      a owl:Restriction ;
      owl:onProperty ns2:hasUnit ;
      owl:allValuesFrom ns2:ForceUnit
    ]
  ], [
    a owl:Restriction ;
    owl:onProperty ns2:hasDimension ;
    owl:hasValue ns2:force-Dimension
  ] ;
  ns2:symbol "F" ;
  ns2:commonlyHasUnit ns2:metreKilogramPerSecond-TimeSquared, ns2:newton, ns2:attonewton, ns2:centinewton, ns2:decanewton, ns2:decinewton, ns2:exanewton, ns2:femtonewton, ns2:giganewton, ns2:hectonewton, ns2:kilonewton, ns2:meganewton, ns2:micronewton, ns2:millinewton, ns2:nanonewton, ns2:petanewton, ns2:piconewton, ns2:teranewton, ns2:dyne, ns2:kip, ns2:poundal, ns2:pound-Force, ns2:ton-Force-Short .

ns2:Friction
  a owl:Class ;
  rdfs:label "friction"@en, "wrijving"@nl ;
  rdfs:comment "Friction is a force that resists the relative motion of solid surfaces, fluid layers, or material elements sliding against each other."@en ;
  rdfs:subClassOf ns2:Force ;
  ns2:commonlyHasUnit ns2:metreKilogramPerSecond-TimeSquared, ns2:newton, ns2:attonewton, ns2:centinewton, ns2:decanewton, ns2:decinewton, ns2:exanewton, ns2:femtonewton, ns2:giganewton, ns2:hectonewton, ns2:kilonewton, ns2:meganewton, ns2:micronewton, ns2:millinewton, ns2:nanonewton, ns2:petanewton, ns2:piconewton, ns2:teranewton, ns2:dyne, ns2:kip, ns2:poundal, ns2:pound-Force, ns2:ton-Force-Short .

ns2:Thrust
  a owl:Class ;
  rdfs:label "thrust"@en, "stuwkracht"@nl ;
  rdfs:comment "Thrust is a reaction force that is caused by an accelerated mass expelled by a system in one direction."@en ;
  rdfs:subClassOf ns2:Force ;
  ns2:commonlyHasUnit ns2:metreKilogramPerSecond-TimeSquared, ns2:newton, ns2:attonewton, ns2:centinewton, ns2:decanewton, ns2:decinewton, ns2:exanewton, ns2:femtonewton, ns2:giganewton, ns2:hectonewton, ns2:kilonewton, ns2:meganewton, ns2:micronewton, ns2:millinewton, ns2:nanonewton, ns2:petanewton, ns2:piconewton, ns2:teranewton, ns2:dyne, ns2:kip, ns2:poundal, ns2:pound-Force, ns2:ton-Force-Short .

ns2:Weight
  a owl:Class ;
  rdfs:label "weight"@en, "gewicht"@nl ;
  rdfs:comment "Weight is a force that attracts a body towards another (reference) body."@en ;
  rdfs:subClassOf ns2:Force ;
  ns2:symbol "G" ;
  ns2:alternativeSymbol "W", "P" ;
  ns2:commonlyHasUnit ns2:metreKilogramPerSecond-TimeSquared, ns2:newton, ns2:attonewton, ns2:centinewton, ns2:decanewton, ns2:decinewton, ns2:exanewton, ns2:femtonewton, ns2:giganewton, ns2:hectonewton, ns2:kilonewton, ns2:meganewton, ns2:micronewton, ns2:millinewton, ns2:nanonewton, ns2:petanewton, ns2:piconewton, ns2:teranewton, ns2:dyne, ns2:kip, ns2:poundal, ns2:pound-Force, ns2:ton-Force-Short .

ns2:Pressure
  a owl:Class ;
  rdfs:label "pressure"@en, "druk"@nl, "压力"@zh ;
  rdfs:comment "Pressure is the force applied to or distributed over a surface. It is a derived quantity in the International System of Units. Pressure is force divided by area."@en ;
  rdfs:subClassOf ns2:Quantity, [
    a owl:Restriction ;
    owl:onProperty ns2:hasValue ;
    owl:allValuesFrom [
      a owl:Restriction ;
      owl:onProperty ns2:hasUnit ;
      owl:allValuesFrom ns2:PressureUnit
    ]
  ], [
    a owl:Restriction ;
    owl:onProperty ns2:hasDimension ;
    owl:hasValue ns2:pressure-Dimension
  ] ;
  ns2:symbol "p" ;
  ns2:alternativeSymbol "P" ;
  ns2:commonlyHasUnit ns2:newtonPerSquareMetre, ns2:kilogramSecond-TimeToThePower-2ReciprocalMetre, ns2:pascal, ns2:attopascal, ns2:centipascal, ns2:decapascal, ns2:decipascal, ns2:exapascal, ns2:femtopascal, ns2:gigapascal, ns2:hectopascal, ns2:kilopascal, ns2:megapascal, ns2:micropascal, ns2:millipascal, ns2:nanopascal, ns2:petapascal, ns2:picopascal, ns2:terapascal, ns2:bar, ns2:decibar, ns2:microbar, ns2:millibar, ns2:metreOfMercury, ns2:centimetreOfMercury, ns2:millimetreOfMercury, ns2:atmosphere-Standard, ns2:atmosphere-Technical, ns2:barye, ns2:torr .

ns2:Energy
  a owl:Class ;
  rdfs:label "energy"@en, "energie"@nl, "能量"@zh ;
  rdfs:comment "Energy can be defined as the ability to do work. It is a derived quantity in the International System of Units."@en ;
  rdfs:subClassOf ns2:Quantity, [
    a owl:Restriction ;
    owl:onProperty ns2:hasValue ;
    owl:allValuesFrom [
      a owl:Restriction ;
      owl:onProperty ns2:hasUnit ;
      owl:allValuesFrom ns2:EnergyUnit
    ]
  ], [
    a owl:Restriction ;
    owl:onProperty ns2:hasDimension ;
    owl:hasValue ns2:energy-Dimension
  ] ;
  ns2:symbol "E" ;
  ns2:alternativeSymbol "W" ;
  ns2:commonlyHasUnit ns2:newtonMetre, ns2:micronewtonMetre, ns2:millinewtonMetre, ns2:joule, ns2:attojoule, ns2:centijoule, ns2:decajoule, ns2:decijoule, ns2:exajoule, ns2:femtojoule, ns2:gigajoule, ns2:hectojoule, ns2:kilojoule, ns2:megajoule, ns2:microjoule, ns2:millijoule, ns2:nanojoule, ns2:petajoule, ns2:picojoule, ns2:terajoule, ns2:electronvolt, ns2:gigaelectronvolt, ns2:kiloelectronvolt, ns2:megaelectronvolt, ns2:calorie-Mean, ns2:kilocalorie-Mean, ns2:BritishThermalUnit-39F, ns2:BritishThermalUnit-59F, ns2:BritishThermalUnit-60F, ns2:BritishThermalUnit-InternationalTable, ns2:BritishThermalUnit-Mean, ns2:BritishThermalUnit-Thermochemical, ns2:calorie-15C, ns2:calorie-20C, ns2:calorie-InternationalTable, ns2:calorie-Thermochemical, ns2:erg, ns2:footPoundal, ns2:quad, ns2:wattHour, ns2:kilowattHour, ns2:megawattHour, ns2:gigawattHour, ns2:terawattHour, ns2:therm-EC, ns2:therm-US, ns2:tonOfTNT, ns2:megaerg .

ns2:Enthalpy
  a owl:Class ;
  rdfs:label "enthalpy"@en, "enthalpie"@nl, "焓"@zh ;
  rdfs:comment "Enthalpy is the sum of the internal energy of a system plus the product of the pressure-volume work done on the system."@en ;
  rdfs:subClassOf ns2:Energy ;
  ns2:symbol "H" ;
  ns2:commonlyHasUnit ns2:newtonMetre, ns2:micronewtonMetre, ns2:millinewtonMetre, ns2:joule, ns2:attojoule, ns2:centijoule, ns2:decajoule, ns2:decijoule, ns2:exajoule, ns2:femtojoule, ns2:gigajoule, ns2:hectojoule, ns2:kilojoule, ns2:megajoule, ns2:microjoule, ns2:millijoule, ns2:nanojoule, ns2:petajoule, ns2:picojoule, ns2:terajoule, ns2:electronvolt, ns2:gigaelectronvolt, ns2:kiloelectronvolt, ns2:megaelectronvolt, ns2:calorie-Mean, ns2:kilocalorie-Mean, ns2:BritishThermalUnit-39F, ns2:BritishThermalUnit-59F, ns2:BritishThermalUnit-60F, ns2:BritishThermalUnit-InternationalTable, ns2:BritishThermalUnit-Mean, ns2:BritishThermalUnit-Thermochemical, ns2:calorie-15C, ns2:calorie-20C, ns2:calorie-InternationalTable, ns2:calorie-Thermochemical, ns2:erg, ns2:footPoundal, ns2:quad, ns2:wattHour, ns2:kilowattHour, ns2:megawattHour, ns2:gigawattHour, ns2:terawattHour, ns2:therm-EC, ns2:therm-US, ns2:tonOfTNT, ns2:megaerg .

ns2:KineticEnergy
  a owl:Class ;
  rdfs:label "kinetic energy"@en, "kinetische energie"@nl, "动能"@zh ;
  ns2:alternativeLabel "bewegingsenergie"@nl ;
  rdfs:comment "Kinetic energy is energy due to motion."@en ;
  rdfs:subClassOf ns2:Energy ;
  ns2:symbol "E_k" ;
  ns2:alternativeSymbol "T", "K" ;
  ns2:commonlyHasUnit ns2:newtonMetre, ns2:micronewtonMetre, ns2:millinewtonMetre, ns2:joule, ns2:attojoule, ns2:centijoule, ns2:decajoule, ns2:decijoule, ns2:exajoule, ns2:femtojoule, ns2:gigajoule, ns2:hectojoule, ns2:kilojoule, ns2:megajoule, ns2:microjoule, ns2:millijoule, ns2:nanojoule, ns2:petajoule, ns2:picojoule, ns2:terajoule, ns2:electronvolt, ns2:gigaelectronvolt, ns2:kiloelectronvolt, ns2:megaelectronvolt, ns2:calorie-Mean, ns2:kilocalorie-Mean, ns2:BritishThermalUnit-39F, ns2:BritishThermalUnit-59F, ns2:BritishThermalUnit-60F, ns2:BritishThermalUnit-InternationalTable, ns2:BritishThermalUnit-Mean, ns2:BritishThermalUnit-Thermochemical, ns2:calorie-15C, ns2:calorie-20C, ns2:calorie-InternationalTable, ns2:calorie-Thermochemical, ns2:erg, ns2:footPoundal, ns2:quad, ns2:wattHour, ns2:kilowattHour, ns2:megawattHour, ns2:gigawattHour, ns2:terawattHour, ns2:therm-EC, ns2:therm-US, ns2:tonOfTNT, ns2:megaerg .

ns2:PotentialEnergy
  a owl:Class ;
  rdfs:label "potential energy"@en, "potentiële energie"@nl, "势能"@zh ;
  rdfs:comment "Potential energy is energy due to position of one body with respect to another or to the relative parts of the same body."@en ;
  rdfs:subClassOf ns2:Energy ;
  ns2:symbol "E_p" ;
  ns2:alternativeSymbol "V", "Φ", "U" ;
  ns2:commonlyHasUnit ns2:newtonMetre, ns2:micronewtonMetre, ns2:millinewtonMetre, ns2:joule, ns2:attojoule, ns2:centijoule, ns2:decajoule, ns2:decijoule, ns2:exajoule, ns2:femtojoule, ns2:gigajoule, ns2:hectojoule, ns2:kilojoule, ns2:megajoule, ns2:microjoule, ns2:millijoule, ns2:nanojoule, ns2:petajoule, ns2:picojoule, ns2:terajoule, ns2:electronvolt, ns2:gigaelectronvolt, ns2:kiloelectronvolt, ns2:megaelectronvolt, ns2:calorie-Mean, ns2:kilocalorie-Mean, ns2:BritishThermalUnit-39F, ns2:BritishThermalUnit-59F, ns2:BritishThermalUnit-60F, ns2:BritishThermalUnit-InternationalTable, ns2:BritishThermalUnit-Mean, ns2:BritishThermalUnit-Thermochemical, ns2:calorie-15C, ns2:calorie-20C, ns2:calorie-InternationalTable, ns2:calorie-Thermochemical, ns2:erg, ns2:footPoundal, ns2:quad, ns2:wattHour, ns2:kilowattHour, ns2:megawattHour, ns2:gigawattHour, ns2:terawattHour, ns2:therm-EC, ns2:therm-US, ns2:tonOfTNT, ns2:megaerg .

ns2:Work
  a owl:Class ;
  rdfs:label "work"@en, "arbeid"@nl, "工作"@zh ;
  rdfs:comment "Work is the energy when a force acts against resistance to produce motion in a body."@en ;
  rdfs:subClassOf ns2:Energy ;
  ns2:symbol "W" ;
  ns2:alternativeSymbol "A" ;
  ns2:commonlyHasUnit ns2:newtonMetre, ns2:micronewtonMetre, ns2:millinewtonMetre, ns2:joule, ns2:attojoule, ns2:centijoule, ns2:decajoule, ns2:decijoule, ns2:exajoule, ns2:femtojoule, ns2:gigajoule, ns2:hectojoule, ns2:kilojoule, ns2:megajoule, ns2:microjoule, ns2:millijoule, ns2:nanojoule, ns2:petajoule, ns2:picojoule, ns2:terajoule, ns2:electronvolt, ns2:gigaelectronvolt, ns2:kiloelectronvolt, ns2:megaelectronvolt, ns2:calorie-Mean, ns2:kilocalorie-Mean, ns2:BritishThermalUnit-39F, ns2:BritishThermalUnit-59F, ns2:BritishThermalUnit-60F, ns2:BritishThermalUnit-InternationalTable, ns2:BritishThermalUnit-Mean, ns2:BritishThermalUnit-Thermochemical, ns2:calorie-15C, ns2:calorie-20C, ns2:calorie-InternationalTable, ns2:calorie-Thermochemical, ns2:erg, ns2:footPoundal, ns2:quad, ns2:wattHour, ns2:kilowattHour, ns2:megawattHour, ns2:gigawattHour, ns2:terawattHour, ns2:therm-EC, ns2:therm-US, ns2:tonOfTNT, ns2:megaerg .

ns2:Torque
  a owl:Class ;
  rdfs:label "torque"@en, "koppel"@nl, "扭矩"@zh ;
  rdfs:comment "Torque is the effectiveness of a force to produce rotation about an axis, measured by the product of the force and the perpendicular distance from the line of action of the force to the axis."@en ;
  rdfs:subClassOf ns2:Quantity, [
    a owl:Restriction ;
    owl:onProperty ns2:hasValue ;
    owl:allValuesFrom [
      a owl:Restriction ;
      owl:onProperty ns2:hasUnit ;
      owl:allValuesFrom ns2:TorqueUnit
    ]
  ], [
    a owl:Restriction ;
    owl:onProperty ns2:hasDimension ;
    owl:hasValue ns2:energy-Dimension
  ] ;
  ns2:symbol "T" ;
  ns2:commonlyHasUnit ns2:newtonMetre, ns2:micronewtonMetre, ns2:millinewtonMetre .

ns2:MomentOfForce
  a owl:Class ;
  rdfs:label "moment of force"@en ;
  ns2:alternativeLabel "moment"@en ;
  rdfs:comment "Moment of force is the effectiveness of a force to produce rotation about an axis measured by the product of the force and the perpendicular distance from the line of action of the force to the axis."@en ;
  rdfs:subClassOf ns2:Quantity, [
    a owl:Restriction ;
    owl:onProperty ns2:hasValue ;
    owl:allValuesFrom [
      a owl:Restriction ;
      owl:onProperty ns2:hasUnit ;
      owl:allValuesFrom ns2:MomentOfForceUnit
    ]
  ], [
    a owl:Restriction ;
    owl:onProperty ns2:hasDimension ;
    owl:hasValue ns2:energy-Dimension
  ] ;
  ns2:symbol "M" ;
  ns2:commonlyHasUnit ns2:newtonMetre, ns2:micronewtonMetre, ns2:millinewtonMetre .

ns2:Power
  a owl:Class ;
  rdfs:label "power"@en, "vermogen"@nl, "功率"@zh ;
  rdfs:comment "Power is the time rate at which work is done. It is a derived quantity in the International System of Units. Power is energy divided by time."@en ;
  rdfs:subClassOf ns2:Quantity, [
    a owl:Restriction ;
    owl:onProperty ns2:hasValue ;
    owl:allValuesFrom [
      a owl:Restriction ;
      owl:onProperty ns2:hasUnit ;
      owl:allValuesFrom ns2:PowerUnit
    ]
  ], [
    a owl:Restriction ;
    owl:onProperty ns2:hasDimension ;
    owl:hasValue ns2:power-Dimension
  ] ;
  ns2:symbol "P" ;
  ns2:commonlyHasUnit ns2:joulePerSecond-Time, ns2:watt, ns2:attowatt, ns2:centiwatt, ns2:decawatt, ns2:deciwatt, ns2:exawatt, ns2:femtowatt, ns2:gigawatt, ns2:hectowatt, ns2:kilowatt, ns2:megawatt, ns2:microwatt, ns2:milliwatt, ns2:nanowatt, ns2:petawatt, ns2:picowatt, ns2:terawatt, ns2:horsepower-Boiler, ns2:horsepower-British, ns2:horsepower-Electric, ns2:horsepower-Metric, ns2:horsepower-Water, ns2:tonOfRefrigeration, ns2:solarLuminosity .

ns2:SpecificEnergy
  a owl:Class ;
  rdfs:label "specific energy"@en ;
  rdfs:comment "Specific energy is energy per unit mass."@en ;
  rdfs:subClassOf ns2:Quantity, [
    a owl:Restriction ;
    owl:onProperty ns2:hasValue ;
    owl:allValuesFrom [
      a owl:Restriction ;
      owl:onProperty ns2:hasUnit ;
      owl:allValuesFrom ns2:SpecificEnergyUnit
    ]
  ], [
    a owl:Restriction ;
    owl:onProperty ns2:hasDimension ;
    owl:hasValue ns2:specificEnergyOrAbsorbedDoseOrDoseEquivalent-Dimension
  ] ;
  ns2:commonlyHasUnit ns2:joulePerKilogram, ns2:kilocalorie-MeanPerHectogram, ns2:kilojoulePerHectogram .

ns2:AngularSpeed
  a owl:Class ;
  rdfs:label "angular speed"@en, "hoeksnelheid"@nl ;
  ns2:alternativeLabel "angular frequency"@en, "hoekfrequentie"@nl ;
  ns2:symbol "ω" ;
  ns2:alternativeSymbol "Ω" ;
  rdfs:subClassOf ns2:Quantity, [
    a owl:Restriction ;
    owl:onProperty ns2:hasValue ;
    owl:allValuesFrom [
      a owl:Restriction ;
      owl:onProperty ns2:hasUnit ;
      owl:allValuesFrom ns2:AngularSpeedUnit
    ]
  ], [
    a owl:Restriction ;
    owl:onProperty ns2:hasDimension ;
    owl:hasValue ns2:angularSpeed-Dimension
  ] ;
  ns2:commonlyHasUnit ns2:radianPerSecond-Time, ns2:millisecond-AnglePerYear .

ns2:AngularVelocity
  a owl:Class ;
  rdfs:label "angular velocity"@en ;
  rdfs:subClassOf ns2:AngularSpeed ;
  ns2:symbol "ω" ;
  ns2:commonlyHasUnit ns2:radianPerSecond-Time .

ns2:AngularAcceleration
  a owl:Class ;
  rdfs:label "angular acceleration"@en, "hoekversnelling"@nl ;
  rdfs:subClassOf ns2:Quantity, [
    a owl:Restriction ;
    owl:onProperty ns2:hasValue ;
    owl:allValuesFrom [
      a owl:Restriction ;
      owl:onProperty ns2:hasUnit ;
      owl:allValuesFrom ns2:AngularAccelerationUnit
    ]
  ], [
    a owl:Restriction ;
    owl:onProperty ns2:hasDimension ;
    owl:hasValue ns2:angularAcceleration-Dimension
  ] ;
  ns2:symbol "α" ;
  ns2:commonlyHasUnit ns2:radianPerSecond-TimeSquared .

ns2:DynamicViscosity
  a owl:Class ;
  rdfs:label "dynamic viscosity"@en, "dynamische viscositeit"@nl ;
  ns2:unofficialLabel "viscosity" ;
  rdfs:comment "Viscosity is the definite resistance to change of form of many materials."@en ;
  rdfs:subClassOf ns2:Quantity, [
    a owl:Restriction ;
    owl:onProperty ns2:hasValue ;
    owl:allValuesFrom [
      a owl:Restriction ;
      owl:onProperty ns2:hasUnit ;
      owl:allValuesFrom ns2:DynamicViscosityUnit
    ]
  ], [
    a owl:Restriction ;
    owl:onProperty ns2:hasDimension ;
    owl:hasValue ns2:dynamicViscosity-Dimension
  ] ;
  ns2:symbol "μ" ;
  ns2:alternativeSymbol "η" ;
  ns2:commonlyHasUnit ns2:pascalSecond-Time, ns2:poise, ns2:centipoise .

ns2:KinematicViscosity
  a owl:Class ;
  rdfs:label "kinematic viscosity"@en, "kinematische viscositeit"@nl ;
  ns2:unofficialLabel "viscosity" ;
  rdfs:comment "Kinematic viscosity is the ratio of viscosity to density."@en ;
  rdfs:subClassOf ns2:Quantity, [
    a owl:Restriction ;
    owl:onProperty ns2:hasValue ;
    owl:allValuesFrom [
      a owl:Restriction ;
      owl:onProperty ns2:hasUnit ;
      owl:allValuesFrom ns2:KinematicViscosityUnit
    ]
  ], [
    a owl:Restriction ;
    owl:onProperty ns2:hasDimension ;
    owl:hasValue ns2:kinematicViscosityOrThermalDiffusivity-Dimension
  ] ;
  ns2:symbol "ν" ;
  ns2:commonlyHasUnit ns2:squareMetrePerSecond-Time, ns2:stokes, ns2:centistokes .

ns2:PowerDensity
  a owl:Class ;
  rdfs:label "power density"@en ;
  rdfs:subClassOf ns2:Quantity, [
    a owl:Restriction ;
    owl:onProperty ns2:hasValue ;
    owl:allValuesFrom [
      a owl:Restriction ;
      owl:onProperty ns2:hasUnit ;
      owl:allValuesFrom ns2:PowerDensityUnit
    ]
  ], [
    a owl:Restriction ;
    owl:onProperty ns2:hasDimension ;
    owl:hasValue ns2:powerDensity-Dimension
  ] ;
  ns2:commonlyHasUnit ns2:wattPerSquareMetre .

ns2:EnergyDensity
  a owl:Class ;
  rdfs:label "energy density"@en, "energiedichtheid"@nl ;
  rdfs:comment "Energy density is the amount of energy stored in a given system or region of space per unit volume."@en ;
  rdfs:subClassOf ns2:Quantity, [
    a owl:Restriction ;
    owl:onProperty ns2:hasValue ;
    owl:allValuesFrom [
      a owl:Restriction ;
      owl:onProperty ns2:hasUnit ;
      owl:allValuesFrom ns2:EnergyDensityUnit
    ]
  ], [
    a owl:Restriction ;
    owl:onProperty ns2:hasDimension ;
    owl:hasValue ns2:energyDensity-Dimension
  ] ;
  ns2:commonlyHasUnit ns2:joulePerCubicmetre .

ns2:Action
  a owl:Class ;
  rdfs:label "action"@en, "actie"@nl ;
  rdfs:subClassOf ns2:Quantity, [
    a owl:Restriction ;
    owl:onProperty ns2:hasValue ;
    owl:allValuesFrom [
      a owl:Restriction ;
      owl:onProperty ns2:hasUnit ;
      owl:allValuesFrom ns2:ActionUnit
    ]
  ], [
    a owl:Restriction ;
    owl:onProperty ns2:hasDimension ;
    owl:hasValue ns2:actionOrAngularMomentum-Dimension
  ] ;
  ns2:commonlyHasUnit ns2:jouleSecond-Time, ns2:ergSecond-Time .

ns2:AngularMomentum
  a owl:Class ;
  rdfs:label "angular momentum"@en, "impulsmoment"@nl ;
  ns2:alternativeLabel "draaiimpuls"@nl, "hoekmoment"@nl, "draaimoment"@nl ;
  rdfs:subClassOf ns2:Quantity, [
    a owl:Restriction ;
    owl:onProperty ns2:hasValue ;
    owl:allValuesFrom [
      a owl:Restriction ;
      owl:onProperty ns2:hasUnit ;
      owl:allValuesFrom ns2:AngularMomentumUnit
    ]
  ], [
    a owl:Restriction ;
    owl:onProperty ns2:hasDimension ;
    owl:hasValue ns2:actionOrAngularMomentum-Dimension
  ] ;
  ns2:symbol "L" ;
  ns2:alternativeSymbol "J" ;
  ns2:commonlyHasUnit ns2:jouleSecond-Time, ns2:ergSecond-Time .

ns2:Fluidity
  a owl:Class ;
  rdfs:label "fluidity"@en ;
  rdfs:subClassOf ns2:Quantity, [
    a owl:Restriction ;
    owl:onProperty ns2:hasValue ;
    owl:allValuesFrom [
      a owl:Restriction ;
      owl:onProperty ns2:hasUnit ;
      owl:allValuesFrom ns2:FluidityUnit
    ]
  ], [
    a owl:Restriction ;
    owl:onProperty ns2:hasDimension ;
    owl:hasValue ns2:fluidity-Dimension
  ] ;
  ns2:commonlyHasUnit ns2:reciprocalPascalSecond-Time, ns2:rhe .

ns2:MassFraction
  a owl:Class ;
  rdfs:label "mass fraction"@en, "massafractie"@nl ;
  ns2:alternativeLabel "concentration (w/w)"@en ;
  rdfs:subClassOf ns2:Quantity, [
    a owl:Restriction ;
    owl:onProperty ns2:hasDimension ;
    owl:hasValue ns2:dimensionOne
  ], [
    a owl:Restriction ;
    owl:onProperty ns2:hasValue ;
    owl:allValuesFrom [
      a owl:Restriction ;
      owl:onProperty ns2:hasUnit ;
      owl:allValuesFrom ns2:MassFractionUnit
    ]
  ] ;
  ns2:symbol "w" ;
  ns2:commonlyHasUnit ns2:one, ns2:percent, ns2:partsPerMillion, ns2:gramPerGram, ns2:gramPerKilogram, ns2:gramPerHectogram, ns2:kilogramPerKilogram, ns2:milligramPerHectogram, ns2:milligramPerKilogram, ns2:microgramPerHectogram .

ns2:Momentum
  a owl:Class ;
  rdfs:label "momentum"@en, "impuls"@nl ;
  ns2:alternativeLabel "linear momentum"@en ;
  rdfs:comment "Momentum is the product of mass and velocity of an object."@en ;
  rdfs:subClassOf ns2:Quantity, [
    a owl:Restriction ;
    owl:onProperty ns2:hasValue ;
    owl:allValuesFrom [
      a owl:Restriction ;
      owl:onProperty ns2:hasUnit ;
      owl:allValuesFrom ns2:MomentumUnit
    ]
  ] ;
  ns2:symbol "p" ;
  ns2:commonlyHasUnit ns2:metreKilogramPerSecond-Time .

ns2:MomentOfInertia
  a owl:Class ;
  rdfs:label "moment of inertia"@en, "traagheidsmoment"@nl ;
  ns2:alternativeLabel "massatraagheidsmoment"@nl ;
  rdfs:comment "Moment of inertia is a measure of the effectiveness of mass in rotation."@en ;
  rdfs:subClassOf ns2:Quantity, [
    a owl:Restriction ;
    owl:onProperty ns2:hasValue ;
    owl:allValuesFrom [
      a owl:Restriction ;
      owl:onProperty ns2:hasUnit ;
      owl:allValuesFrom ns2:MomentOfInertiaUnit
    ]
  ] ;
  ns2:symbol "I" ;
  ns2:alternativeSymbol "J" ;
  ns2:commonlyHasUnit ns2:kilogramSquareMetre .

ns2:RelativeHumidity
  a owl:Class ;
  rdfs:label "relative humidity"@en, "relatieve luchtvochtigheid"@nl ;
  rdfs:subClassOf ns2:Quantity, [
    a owl:Restriction ;
    owl:onProperty ns2:hasDimension ;
    owl:hasValue ns2:dimensionOne
  ], [
    a owl:Restriction ;
    owl:onProperty ns2:hasValue ;
    owl:allValuesFrom [
      a owl:Restriction ;
      owl:onProperty ns2:hasUnit ;
      owl:allValuesFrom ns2:RelativeHumidityUnit
    ]
  ] ;
  ns2:symbol "RH" ;
  ns2:commonlyHasUnit ns2:one, ns2:percent .

ns2:AreaFraction
  a owl:Class ;
  rdfs:label "area fraction"@en, "oppervlaktefractie"@nl ;
  rdfs:subClassOf ns2:Quantity, [
    a owl:Restriction ;
    owl:onProperty ns2:hasDimension ;
    owl:hasValue ns2:dimensionOne
  ], [
    a owl:Restriction ;
    owl:onProperty ns2:hasValue ;
    owl:allValuesFrom [
      a owl:Restriction ;
      owl:onProperty ns2:hasUnit ;
      owl:allValuesFrom ns2:AreaFractionUnit
    ]
  ] ;
  ns2:commonlyHasUnit ns2:one, ns2:percent, ns2:partsPerMillion, ns2:squareMetrePerSquareMetre .

ns2:Coverage
  a owl:Class ;
  rdfs:label "coverage"@en ;
  rdfs:subClassOf ns2:AreaFraction ;
  ns2:commonlyHasUnit ns2:one, ns2:percent, ns2:partsPerMillion, ns2:squareMetrePerSquareMetre .

ns2:VolumetricFlowRate
  a owl:Class ;
  rdfs:label "volumetric flow rate"@en ;
  ns2:alternativeLabel "volume flow rate"@en, "volume flow"@en, "flow rate"@en ;
  rdfs:subClassOf ns2:Quantity, [
    a owl:Restriction ;
    owl:onProperty ns2:hasValue ;
    owl:allValuesFrom [
      a owl:Restriction ;
      owl:onProperty ns2:hasUnit ;
      owl:allValuesFrom ns2:VolumetricFlowRateUnit
    ]
  ], [
    a owl:Restriction ;
    owl:onProperty ns2:hasDimension ;
    owl:hasValue ns2:volumetricFlowRate-Dimension
  ] ;
  ns2:commonlyHasUnit ns2:cubicMetrePerSecond-Time, ns2:cubicMetrePerYear, ns2:litrePerHour .

ns2:VolumeFraction
  a owl:Class ;
  rdfs:label "volume fraction"@en, "volumefractie"@nl ;
  ns2:alternativeLabel "concentration (v/v)"@en ;
  rdfs:subClassOf ns2:Quantity, [
    a owl:Restriction ;
    owl:onProperty ns2:hasDimension ;
    owl:hasValue ns2:dimensionOne
  ], [
    a owl:Restriction ;
    owl:onProperty ns2:hasValue ;
    owl:allValuesFrom [
      a owl:Restriction ;
      owl:onProperty ns2:hasUnit ;
      owl:allValuesFrom ns2:VolumeFractionUnit
    ]
  ] ;
  ns2:symbol "φ" ;
  ns2:commonlyHasUnit ns2:one, ns2:percent, ns2:partsPerMillion, ns2:cubicMetrePerCubicmetre, ns2:cubicMillimetrePerCubicMillimetre, ns2:cubicCentimetrePerCubicCentimetre .

ns2:Overrun
  a owl:Class ;
  rdfs:label "overrun"@en ;
  rdfs:subClassOf ns2:VolumeFraction ;
  ns2:commonlyHasUnit ns2:one, ns2:percent, ns2:partsPerMillion, ns2:cubicMetrePerCubicmetre, ns2:cubicMillimetrePerCubicMillimetre, ns2:cubicCentimetrePerCubicCentimetre .

ns2:MassFlow
  a owl:Class ;
  rdfs:label "mass flow"@en ;
  rdfs:comment "Mass flow is the movement of substances at equal rates or as a single body."@en ;
  rdfs:subClassOf ns2:Quantity, [
    a owl:Restriction ;
    owl:onProperty ns2:hasValue ;
    owl:allValuesFrom [
      a owl:Restriction ;
      owl:onProperty ns2:hasUnit ;
      owl:allValuesFrom ns2:MassFlowUnit
    ]
  ], [
    a owl:Restriction ;
    owl:onProperty ns2:hasDimension ;
    owl:hasValue ns2:massFlow-Dimension
  ] ;
  ns2:commonlyHasUnit ns2:kilogramPerSecond-Time .

ns2:MassPerEnergy
  a owl:Class ;
  rdfs:label "mass per energy"@en ;
  rdfs:subClassOf ns2:Quantity, [
    a owl:Restriction ;
    owl:onProperty ns2:hasValue ;
    owl:allValuesFrom [
      a owl:Restriction ;
      owl:onProperty ns2:hasUnit ;
      owl:allValuesFrom ns2:MassPerEnergyUnit
    ]
  ] .

ns2:Impulse
  a owl:Class ;
  rdfs:label "impulse"@en, "stoot"@nl ;
  rdfs:comment "Impulse is the integral of a force with respect to time."@en ;
  rdfs:subClassOf ns2:Quantity ;
  ns2:symbol "I" .

ns2:AreaDensity
  a owl:Class ;
  rdfs:label "area density"@en, "oppervlaktedichtheid"@nl ;
  rdfs:subClassOf ns2:Quantity, [
    a owl:Restriction ;
    owl:onProperty ns2:hasValue ;
    owl:allValuesFrom [
      a owl:Restriction ;
      owl:onProperty ns2:hasUnit ;
      owl:allValuesFrom ns2:AreaDensityUnit
    ]
  ] ;
  ns2:commonlyHasUnit ns2:gramPerSquareMetre, ns2:kilogramPerSquareMetre, ns2:kilogramPerHectare, ns2:ounceAvoirdupoisPerSquareYard-International .

ns2:AreaDensityRate
  a owl:Class ;
  rdfs:label "area density rate"@en ;
  rdfs:subClassOf ns2:Quantity, [
    a owl:Restriction ;
    owl:onProperty ns2:hasValue ;
    owl:allValuesFrom [
      a owl:Restriction ;
      owl:onProperty ns2:hasUnit ;
      owl:allValuesFrom ns2:AreaDensityRateUnit
    ]
  ] ;
  ns2:commonlyHasUnit ns2:kilogramPerHectareDay .

ns2:second-Time
  a ns2:Unit, ns2:SingularUnit ;
  rdfs:label "second"@en, "seconde"@nl, "秒"@zh ;
  ns2:unofficialAbbreviation "sec" ;
  ns2:symbol "s" ;
  ns2:hasDimension ns2:time-Dimension ;
  rdfs:comment "The second is a unit of time defined as the duration of 9 192 631 770 periods of the radiation corresponding to the transition between the two hyperfine levels of the ground state of the cesium 133 atom."@en ;
  ns2:longcomment "The second is a unit of time defined as the duration of 9 192 631 770 periods of the radiation corresponding to the transition between the two hyperfine levels of the ground state of the cesium 133 atom. The second is a base unit in the International System of Units." ;
  ns2:hasQuantity ns2:durationOf9192631770PeriodsOfTheRadiationCorrespondingToTheTransitionBetweenTheTwoHyperfineLevelsOfTheGroundStateOfTheCesium133Atom .

ns2:_9192631770PeriodsOfTheRadiationCorrespondingToTheTransitionBetweenTheTwoHyperfineLevelsOfTheGroundStateOfTheCesium133Atom
  a owl:Thing ;
  rdfs:label "9 192 631 770 periods of the radiation corresponding to the transition between the two hyperfine levels of the ground state of the cesium 133 atom"@en .

ns2:durationOf9192631770PeriodsOfTheRadiationCorrespondingToTheTransitionBetweenTheTwoHyperfineLevelsOfTheGroundStateOfTheCesium133Atom
  a ns2:Duration ;
  rdfs:label "duration of 9 192 631 770 periods of the radiation corresponding to the transition between the two hyperfine levels of the ground state of the cesium 133 atom"@en ;
  ns2:hasPhenomenon ns2:_9192631770PeriodsOfTheRadiationCorrespondingToTheTransitionBetweenTheTwoHyperfineLevelsOfTheGroundStateOfTheCesium133Atom .

ns2:TimeUnit
  a owl:Class ;
  rdfs:label "time unit"@en ;
  rdfs:subClassOf ns2:Unit ;
  owl:equivalentClass [
    a owl:Class ;
    owl:unionOf (
     _:genid235
     ns2:PrefixedSecond-Time
   )
  ] .

ns2:day
  a ns2:Unit, ns2:SingularUnit ;
  rdfs:label "day"@en, "dag"@nl, "天"@zh ;
  rdfs:comment "The day is a unit of time defined as 86400 second."@en ;
  ns2:symbol "d" ;
  ns2:LaTeXCommand "\\dayUnit" ;
  ns2:hasFactor "86400"^^xsd:float ;
  ns2:hasUnit ns2:second-Time ;
  ns2:hasDimension ns2:time-Dimension .

ns2:day-Sidereal
  a ns2:Unit, ns2:SingularUnit ;
  rdfs:label "day (sidereal)"@en ;
  ns2:alternativeLabel "sidereal day"@en ;
  rdfs:comment "The sidereal day is a unit of time defined as 8.616409e4 second."@en ;
  ns2:hasFactor "8.616409e4"^^xsd:float ;
  ns2:hasUnit ns2:second-Time ;
  ns2:hasDimension ns2:time-Dimension .

ns2:hour
  a ns2:Unit, ns2:SingularUnit ;
  rdfs:label "hour"@en, "uur"@nl, "小时"@zh ;
  rdfs:comment "The hour is a unit of time defined as 3600 second."@en ;
  ns2:symbol "h" ;
  ns2:alternativeSymbol "u" ;
  ns2:hasFactor "3.6e3"^^xsd:float ;
  ns2:hasUnit ns2:second-Time ;
  ns2:hasDimension ns2:time-Dimension .

ns2:hour-Sidereal
  a ns2:Unit, ns2:SingularUnit ;
  rdfs:label "hour (sidereal)"@en ;
  ns2:alternativeLabel "sidereal hour"@en ;
  ns2:hasFactor "3.590170e3"^^xsd:float ;
  ns2:hasUnit ns2:second-Time ;
  ns2:hasDimension ns2:time-Dimension .

ns2:minute-Time
  a ns2:Unit, ns2:SingularUnit ;
  rdfs:label "minute"@en, "minuut"@nl, "分钟"@zh ;
  rdfs:comment "The minute (time) is a unit of time defined as 60 second."@en ;
  ns2:symbol "min" ;
  ns2:hasFactor "6.0e1"^^xsd:float ;
  ns2:hasUnit ns2:second-Time ;
  ns2:hasDimension ns2:time-Dimension .

ns2:minute-Sidereal
  a ns2:Unit, ns2:SingularUnit ;
  rdfs:label "minute (sidereal)"@en ;
  ns2:alternativeLabel "sidereal minute"@en ;
  rdfs:comment "The sidereal minute is a unit of time defined as 5.983617e1 second."@en ;
  ns2:hasFactor "5.983617e1"^^xsd:float ;
  ns2:hasUnit ns2:second-Time ;
  ns2:hasDimension ns2:time-Dimension .

ns2:second-Sidereal
  a ns2:Unit, ns2:SingularUnit ;
  rdfs:label "second (sidereal)"@en ;
  ns2:alternativeLabel "sidereal second"@en, "second (sidereal)"@en ;
  rdfs:comment "The sidereal second is a unit of time defined as 9.972696e-1 second."@en ;
  ns2:hasFactor "9.972696e-1"^^xsd:float ;
  ns2:hasUnit ns2:second-Time ;
  ns2:hasDimension ns2:time-Dimension .

ns2:shake
  a ns2:Unit, ns2:SingularUnit ;
  rdfs:label "shake"@en ;
  rdfs:comment "The shake is a unit of time defined as 1.0e-8 second."@en ;
  ns2:hasFactor "1.0e-8"^^xsd:float ;
  ns2:hasUnit ns2:second-Time ;
  ns2:hasDimension ns2:time-Dimension .

ns2:year
  a ns2:Unit, ns2:SingularUnit ;
  rdfs:label "year"@en, "jaar"@nl ;
  rdfs:comment "The year is a unit of time defined as 31556952 second."@en ;
  ns2:LaTeXCommand "\\yearUnit" ;
  ns2:symbol "a" ;
  ns2:alternativeSymbol "y", "yr" ;
  ns2:hasFactor "31556952"^^xsd:float ;
  ns2:hasUnit ns2:second-Time ;
  ns2:hasDimension ns2:time-Dimension .

ns2:year-Sidereal
  a ns2:Unit, ns2:SingularUnit ;
  rdfs:label "year (sidereal)"@en ;
  ns2:alternativeLabel "sidereal year"@en ;
  rdfs:comment "The sidereal year is a unit of time defined as 3.155815e7 second."@en ;
  ns2:hasFactor "3.155815e7"^^xsd:float ;
  ns2:hasUnit ns2:second-Time ;
  ns2:hasDimension ns2:time-Dimension .

ns2:year-Tropical
  a ns2:Unit, ns2:SingularUnit ;
  rdfs:label "year (tropical)"@en ;
  ns2:alternativeLabel "tropical year"@en ;
  rdfs:comment "The tropical year is a unit of time defined as 3.155693e7 second."@en ;
  ns2:hasFactor "3.155693e7"^^xsd:float ;
  ns2:hasUnit ns2:second-Time ;
  ns2:hasDimension ns2:time-Dimension .

ns2:gigayear
  a ns2:PrefixedUnit ;
  rdfs:label "gigayear"@en, "gigajaar"@nl ;
  ns2:symbol "Gyr" ;
  ns2:hasPrefix ns2:giga ;
  ns2:hasUnit ns2:year ;
  ns2:hasDimension ns2:time-Dimension .

ns2:PrefixedSecond-Time
  a owl:Class ;
  rdfs:label "prefixed second (time)"@en ;
  rdfs:subClassOf ns2:PrefixedUnit ;
  owl:equivalentClass [
    a owl:Class ;
    owl:intersectionOf (
     _:genid254
     _:genid256
     _:genid258
     _:genid260
   )
  ] .

ns2:yoctosecond-Time
  a ns2:PrefixedUnit ;
  rdfs:label "yoctosecond"@en, "yoctoseconde"@nl ;
  ns2:symbol "ys" ;
  ns2:hasPrefix ns2:yocto ;
  ns2:hasUnit ns2:second-Time ;
  ns2:hasDimension ns2:time-Dimension .

ns2:zeptosecond-Time
  a ns2:PrefixedUnit ;
  rdfs:label "zeptosecond"@en, "zeptoseconde"@nl ;
  ns2:symbol "zs" ;
  ns2:hasPrefix ns2:zepto ;
  ns2:hasUnit ns2:second-Time ;
  ns2:hasDimension ns2:time-Dimension .

ns2:attosecond-Time
  a ns2:PrefixedUnit ;
  rdfs:label "attosecond"@en, "attoseconde"@nl ;
  ns2:symbol "as" ;
  ns2:hasPrefix ns2:atto ;
  ns2:hasUnit ns2:second-Time ;
  ns2:hasDimension ns2:time-Dimension .

ns2:femtosecond-Time
  a ns2:PrefixedUnit ;
  rdfs:label "femtosecond"@en, "femtoseconde"@nl ;
  ns2:symbol "fs" ;
  ns2:hasPrefix ns2:femto ;
  ns2:hasUnit ns2:second-Time ;
  ns2:hasDimension ns2:time-Dimension .

ns2:picosecond-Time
  a ns2:PrefixedUnit ;
  rdfs:label "picosecond"@en, "picoseconde"@nl ;
  ns2:symbol "ps" ;
  ns2:hasPrefix ns2:pico ;
  ns2:hasUnit ns2:second-Time ;
  ns2:hasDimension ns2:time-Dimension .

ns2:nanosecond-Time
  a ns2:PrefixedUnit ;
  rdfs:label "nanosecond"@en, "nanoseconde"@nl ;
  ns2:symbol "ns" ;
  ns2:hasPrefix ns2:nano ;
  ns2:hasUnit ns2:second-Time ;
  ns2:hasDimension ns2:time-Dimension .

ns2:microsecond-Time
  a ns2:PrefixedUnit ;
  rdfs:label "microsecond"@en, "microseconde"@nl ;
  ns2:symbol "μs" ;
  ns2:hasPrefix ns2:micro ;
  ns2:hasUnit ns2:second-Time ;
  ns2:hasDimension ns2:time-Dimension .

ns2:millisecond-Time
  a ns2:PrefixedUnit ;
  rdfs:label "millisecond"@en, "milliseconde"@nl ;
  ns2:symbol "ms" ;
  ns2:hasPrefix ns2:milli ;
  ns2:hasUnit ns2:second-Time ;
  ns2:hasDimension ns2:time-Dimension .

ns2:centisecond-Time
  a ns2:PrefixedUnit ;
  rdfs:label "centisecond"@en, "centiseconde"@nl ;
  ns2:symbol "cs" ;
  ns2:hasPrefix ns2:centi ;
  ns2:hasUnit ns2:second-Time ;
  ns2:hasDimension ns2:time-Dimension .

ns2:decisecond-Time
  a ns2:PrefixedUnit ;
  rdfs:label "decisecond"@en, "deciseconde"@nl ;
  ns2:symbol "ds" ;
  ns2:hasPrefix ns2:deci ;
  ns2:hasUnit ns2:second-Time ;
  ns2:hasDimension ns2:time-Dimension .

ns2:decasecond-Time
  a ns2:PrefixedUnit ;
  rdfs:label "decasecond"@en, "decaseconde"@nl ;
  ns2:symbol "das" ;
  ns2:hasPrefix ns2:deca ;
  ns2:hasUnit ns2:second-Time ;
  ns2:hasDimension ns2:time-Dimension .

ns2:hectosecond-Time
  a ns2:PrefixedUnit ;
  rdfs:label "hectosecond"@en, "hectoseconde"@nl ;
  ns2:symbol "hs" ;
  ns2:hasPrefix ns2:hecto ;
  ns2:hasUnit ns2:second-Time ;
  ns2:hasDimension ns2:time-Dimension .

ns2:kilosecond-Time
  a ns2:PrefixedUnit ;
  rdfs:label "kilosecond"@en, "kiloseconde"@nl ;
  ns2:symbol "ks" ;
  ns2:hasPrefix ns2:kilo ;
  ns2:hasUnit ns2:second-Time ;
  ns2:hasDimension ns2:time-Dimension .

ns2:megasecond-Time
  a ns2:PrefixedUnit ;
  rdfs:label "megasecond"@en, "megaseconde"@nl ;
  ns2:symbol "Ms" ;
  ns2:hasPrefix ns2:mega ;
  ns2:hasUnit ns2:second-Time ;
  ns2:hasDimension ns2:time-Dimension .

ns2:gigasecond-Time
  a ns2:PrefixedUnit ;
  rdfs:label "gigasecond"@en, "gigaseconde"@nl ;
  ns2:symbol "Gs" ;
  ns2:hasPrefix ns2:giga ;
  ns2:hasUnit ns2:second-Time ;
  ns2:hasDimension ns2:time-Dimension .

ns2:terasecond-Time
  a ns2:PrefixedUnit ;
  rdfs:label "terasecond"@en, "teraseconde"@nl ;
  ns2:symbol "Ts" ;
  ns2:hasPrefix ns2:tera ;
  ns2:hasUnit ns2:second-Time ;
  ns2:hasDimension ns2:time-Dimension .

ns2:petasecond-Time
  a ns2:PrefixedUnit ;
  rdfs:label "petasecond"@en, "petaseconde"@nl ;
  ns2:symbol "Ps" ;
  ns2:hasPrefix ns2:peta ;
  ns2:hasUnit ns2:second-Time ;
  ns2:hasDimension ns2:time-Dimension .

ns2:exasecond-Time
  a ns2:PrefixedUnit ;
  rdfs:label "exasecond"@en, "exaseconde"@nl ;
  ns2:symbol "Es" ;
  ns2:hasPrefix ns2:exa ;
  ns2:hasUnit ns2:second-Time ;
  ns2:hasDimension ns2:time-Dimension .

ns2:zettasecond-Time
  a ns2:PrefixedUnit ;
  rdfs:label "zettasecond"@en, "zettaseconde"@nl ;
  ns2:symbol "Zs" ;
  ns2:hasPrefix ns2:zetta ;
  ns2:hasUnit ns2:second-Time ;
  ns2:hasDimension ns2:time-Dimension .

ns2:yottasecond-Time
  a ns2:PrefixedUnit ;
  rdfs:label "yottasecond"@en, "yottaseconde"@nl ;
  ns2:symbol "Ys" ;
  ns2:hasPrefix ns2:yotta ;
  ns2:hasUnit ns2:second-Time ;
  ns2:hasDimension ns2:time-Dimension .

ns2:month
  a ns2:Unit, ns2:SingularUnit ;
  rdfs:label "month"@en, "maand"@nl, "月"@zh ;
  rdfs:comment "The month is a unit of time."@en ;
  ns2:hasDimension ns2:time-Dimension ;
  ns2:LaTeXCommand "\\monthUnit" .

ns2:week
  a ns2:Unit, ns2:SingularUnit ;
  rdfs:label "week"@en, "week"@nl ;
  rdfs:comment "The week is a unit of time defined as 6.04800e5 second."@en ;
  ns2:hasFactor "6.04800e5"^^xsd:float ;
  ns2:hasUnit ns2:second-Time ;
  ns2:hasDimension ns2:time-Dimension .

ns2:gram
  a ns2:Unit, ns2:SingularUnit ;
  rdfs:label "gram"@en, "gram"@nl, "克"@zh ;
  rdfs:comment "The gram is a unit of mass defined as 1.0e-3 kilogram."@en ;
  ns2:symbol "g" ;
  ns2:hasFactor "1.0e-3"^^xsd:float ;
  ns2:hasUnit ns2:kilogram ;
  ns2:hasDimension ns2:mass-Dimension .

ns2:MassUnit
  a owl:Class ;
  rdfs:label "mass unit"@en ;
  rdfs:subClassOf ns2:Unit ;
  owl:equivalentClass [
    a owl:Class ;
    owl:unionOf (
     _:genid263
     ns2:PrefixedGram
     ns2:PrefixedTonne
     ns2:PrefixedUnifiedAtomicMassUnit
   )
  ] .

ns2:carat-Mass
  a ns2:Unit, ns2:SingularUnit ;
  rdfs:label "carat (mass)"@en, "karaat (massa)"@nl ;
  rdfs:comment "The carat (mass) is a unit of mass defined as 2.0e-4 kilogram."@en ;
  ns2:hasFactor "2.0e-4"^^xsd:float ;
  ns2:hasUnit ns2:kilogram ;
  ns2:hasDimension ns2:mass-Dimension .

ns2:grain
  a ns2:Unit, ns2:SingularUnit ;
  rdfs:label "grain"@en ;
  rdfs:comment "The grain is a unit of mass defined as 6.479891e-5 kilogram."@en ;
  ns2:symbol "gr" ;
  ns2:hasFactor "6.479891e-5"^^xsd:float ;
  ns2:hasUnit ns2:kilogram ;
  ns2:hasDimension ns2:mass-Dimension .

ns2:hundredweight-British
  a ns2:Unit, ns2:SingularUnit ;
  rdfs:label "hundredweight (British)"@en ;
  ns2:alternativeLabel "British hundredweight"@en ;
  rdfs:comment "The British hundredweight is a unit of mass defined as 5.080235e1 kilogram."@en ;
  ns2:hasFactor "5.080235e1"^^xsd:float ;
  ns2:hasUnit ns2:kilogram ;
  ns2:hasDimension ns2:mass-Dimension .

ns2:hundredweight-US
  a ns2:Unit, ns2:SingularUnit ;
  rdfs:label "hundredweight (US)"@en ;
  ns2:alternativeLabel "US hundredweight"@en ;
  rdfs:comment "The US hundredweight is a unit of mass defined as 4.535924e1 kilogram."@en ;
  ns2:hasFactor "4.535924e1"^^xsd:float ;
  ns2:hasUnit ns2:kilogram ;
  ns2:hasDimension ns2:mass-Dimension .

ns2:InternationalUnit
  a ns2:Unit, ns2:SingularUnit ;
  rdfs:label "International Unit"@en, "国际单位"@zh ;
  ns2:symbol "IU" ;
  ns2:hasDimension ns2:mass-Dimension .

ns2:milligramRAE
  a ns2:Unit, ns2:SingularUnit ;
  rdfs:label "milligram RAE"@en ;
  ns2:hasDimension ns2:mass-Dimension .

ns2:ounceApothecaries
  a ns2:Unit, ns2:SingularUnit ;
  rdfs:label "ounce (apothecaries')"@en ;
  ns2:alternativeLabel "apothecaries' ounce"@en, "troy ounce"@en, "ounce (troy)"@en ;
  rdfs:comment "The apothecaries' ounce is a unit of mass defined as 3.110348e-2 kilogram."@en ;
  ns2:symbol "oz (ap.)" ;
  ns2:alternativeSymbol "oz (apoth)" ;
  ns2:hasFactor "3.110348e-2"^^xsd:float ;
  ns2:hasUnit ns2:kilogram ;
  ns2:hasDimension ns2:mass-Dimension .

ns2:ounceAvoirdupois
  a ns2:Unit, ns2:SingularUnit ;
  rdfs:label "ounce (avoirdupois)"@en ;
  ns2:alternativeLabel "avoirdupois ounce"@en ;
  rdfs:comment "The avoirdupois ounce is a unit of mass defined as 2.834952e-2 kilogram."@en ;
  ns2:symbol "oz" ;
  ns2:alternativeSymbol "oz (av.)", "oz avdp" ;
  ns2:hasFactor "2.834952e-2"^^xsd:float ;
  ns2:hasUnit ns2:kilogram ;
  ns2:hasDimension ns2:mass-Dimension .

ns2:pennyweight-Troy
  a ns2:Unit, ns2:SingularUnit ;
  rdfs:label "pennyweight (Troy)"@en ;
  ns2:alternativeLabel "Troy pennyweight"@en ;
  rdfs:comment "The Troy pennyweight is a unit of mass defined as 1.555174e-3 kilogram."@en ;
  ns2:symbol "dwt" ;
  ns2:hasFactor "1.555174e-3"^^xsd:float ;
  ns2:hasUnit ns2:kilogram ;
  ns2:hasDimension ns2:mass-Dimension .

ns2:poundApothecaries
  a ns2:Unit, ns2:SingularUnit ;
  rdfs:label "pound (apthecaries')"@en ;
  ns2:alternativeLabel "apothecaries' pound"@en, "troy pound"@en, "pound (troy)"@en ;
  rdfs:comment "The apothecaries' pound is a unit of mass defined as 3.732417e-1 kilogram."@en ;
  ns2:symbol "lb" ;
  ns2:hasFactor "3.732417e-1"^^xsd:float ;
  ns2:hasUnit ns2:kilogram ;
  ns2:hasDimension ns2:mass-Dimension .

ns2:poundAvoirdupois
  a ns2:Unit, ns2:SingularUnit ;
  rdfs:label "pound (avoirdupois)"@en ;
  ns2:alternativeLabel "avoirdupois pound"@en ;
  rdfs:comment "The avoirdupois pound is a unit of mass defined as 4.535924e-1 kilogram."@en ;
  ns2:symbol "lb" ;
  ns2:hasFactor "4.5359237e-1"^^xsd:float ;
  ns2:hasUnit ns2:kilogram ;
  ns2:hasDimension ns2:mass-Dimension .

ns2:slug
  a ns2:Unit, ns2:SingularUnit ;
  rdfs:label "slug"@en, "金属块"@zh ;
  rdfs:comment "The slug is a unit of mass defined as 1.459390e1 kilogram."@en ;
  ns2:symbol "slug" ;
  ns2:hasFactor "1.459390e1"^^xsd:float ;
  ns2:hasUnit ns2:kilogram ;
  ns2:hasDimension ns2:mass-Dimension .

ns2:solarMass
  a ns2:Unit, ns2:SingularUnit ;
  rdfs:label "solar mass"@en, "zonsmassa"@nl ;
  rdfs:comment "Solar mass is a unit used in astronomy to denote stellar or galactic masses (http://en.wikipedia.org/wiki/SolarMass)."@en ;
  ns2:symbol "M_☉" ;
  ns2:LaTeXSymbol "M_{\\astrosun}" ;
  ns2:hasFactor "1.98892e30"^^xsd:float ;
  ns2:hasUnit ns2:kilogram ;
  ns2:hasDimension ns2:mass-Dimension .

ns2:ton-ShortAssay
  a ns2:Unit, ns2:SingularUnit ;
  rdfs:label "ton (short assay)"@en ;
  ns2:alternativeLabel "short assay ton"@en ;
  rdfs:comment "The short assay ton is a unit of mass defined as 2.916667e-2 kilogram."@en ;
  ns2:hasFactor "2.916667e-2"^^xsd:float ;
  ns2:hasUnit ns2:kilogram ;
  ns2:hasDimension ns2:mass-Dimension .

ns2:ton-Long
  a ns2:Unit, ns2:SingularUnit ;
  rdfs:label "ton (long)"@en ;
  ns2:alternativeLabel "long ton"@en ;
  rdfs:comment "The long ton is a unit of mass defined as 1.016047e3 kilogram."@en ;
  ns2:hasFactor "1.016047e3"^^xsd:float ;
  ns2:hasUnit ns2:kilogram ;
  ns2:hasDimension ns2:mass-Dimension .

ns2:ton-Short
  a ns2:Unit, ns2:SingularUnit ;
  rdfs:label "ton (short)"@en ;
  ns2:alternativeLabel "short ton"@en ;
  rdfs:comment "The short ton is a unit of mass defined as 9.071847e2 kilogram."@en ;
  ns2:hasFactor "9.071847e2"^^xsd:float ;
  ns2:hasUnit ns2:kilogram ;
  ns2:hasDimension ns2:mass-Dimension .

ns2:tonne
  a ns2:Unit, ns2:SingularUnit ;
  rdfs:label "tonne"@en, "ton"@nl, "公吨"@zh ;
  ns2:alternativeLabel "metric ton"@en ;
  rdfs:comment "The tonne is a unit of mass defined as 1000 kilogram."@en ;
  ns2:symbol "t" ;
  ns2:hasFactor "1.0e3"^^xsd:float ;
  ns2:hasUnit ns2:kilogram ;
  ns2:hasDimension ns2:mass-Dimension .

ns2:unifiedAtomicMassUnit
  a ns2:Unit, ns2:SingularUnit ;
  rdfs:label "unified atomic mass unit"@en ;
  rdfs:comment "The unified atomic mass unit is a unit of mass defined as 1.660538782(83)e-27 kilogram."@en ;
  ns2:symbol "u" ;
  ns2:hasDimension ns2:mass-Dimension .

ns2:PrefixedGram
  a owl:Class ;
  rdfs:label "prefixed gram"@en ;
  rdfs:subClassOf ns2:PrefixedUnit ;
  owl:equivalentClass [
    a owl:Class ;
    owl:intersectionOf (
     _:genid290
     _:genid292
     _:genid294
     _:genid296
   )
  ] .

ns2:PrefixedTonne
  a owl:Class ;
  rdfs:label "prefixed tonne"@en ;
  rdfs:subClassOf ns2:PrefixedUnit ;
  owl:equivalentClass [
    a owl:Class ;
    owl:intersectionOf (
     _:genid299
     _:genid301
     _:genid303
     _:genid305
   )
  ] .

ns2:PrefixedUnifiedAtomicMassUnit
  a owl:Class ;
  rdfs:label "prefixed unified atomic mass unit"@en ;
  rdfs:subClassOf ns2:PrefixedUnit ;
  owl:equivalentClass [
    a owl:Class ;
    owl:intersectionOf (
     _:genid308
     _:genid310
     _:genid312
     _:genid314
   )
  ] .

ns2:yoctogram
  a ns2:PrefixedUnit ;
  rdfs:label "yoctogram"@en, "yoctogram"@nl ;
  rdfs:comment "The yoctogram is a unit of mass defined as 1.0e-24 gram."@en ;
  ns2:symbol "yg" ;
  ns2:hasPrefix ns2:yocto ;
  ns2:hasUnit ns2:gram ;
  ns2:hasDimension ns2:mass-Dimension .

ns2:zeptogram
  a ns2:PrefixedUnit ;
  rdfs:label "zeptogram"@en, "zeptogram"@nl ;
  rdfs:comment "The zeptgram is a unit of mass defined as 1.0e-21 gram."@en ;
  ns2:symbol "zg" ;
  ns2:hasPrefix ns2:zepto ;
  ns2:hasUnit ns2:gram ;
  ns2:hasDimension ns2:mass-Dimension .

ns2:attogram
  a ns2:PrefixedUnit ;
  rdfs:label "attogram"@en, "attogram"@nl ;
  rdfs:comment "The attogram is a unit of mass defined as 1.0e-18 gram."@en ;
  ns2:symbol "ag" ;
  ns2:hasPrefix ns2:atto ;
  ns2:hasUnit ns2:gram ;
  ns2:hasDimension ns2:mass-Dimension .

ns2:femtogram
  a ns2:PrefixedUnit ;
  rdfs:label "femtogram"@en, "femtogram"@nl ;
  rdfs:comment "The femtogram is a unit of mass defined as 1.0e-15 gram."@en ;
  ns2:symbol "fg" ;
  ns2:hasPrefix ns2:femto ;
  ns2:hasUnit ns2:gram ;
  ns2:hasDimension ns2:mass-Dimension .

ns2:picogram
  a ns2:PrefixedUnit ;
  rdfs:label "picogram"@en, "picogram"@nl ;
  rdfs:comment "The picogram is a unit of mass defined as 1.0e-12 gram."@en ;
  ns2:symbol "pg" ;
  ns2:hasPrefix ns2:pico ;
  ns2:hasUnit ns2:gram ;
  ns2:hasDimension ns2:mass-Dimension .

ns2:nanogram
  a ns2:PrefixedUnit ;
  rdfs:label "nanogram"@en, "nanogram"@nl, "纳克"@zh ;
  rdfs:comment "The nanogram is a unit of mass defined as 1.0e-9 gram."@en ;
  ns2:symbol "ng" ;
  ns2:hasPrefix ns2:nano ;
  ns2:hasUnit ns2:gram ;
  ns2:hasDimension ns2:mass-Dimension .

ns2:microgram
  a ns2:PrefixedUnit ;
  rdfs:label "microgram"@en, "microgram"@nl, "微克"@zh ;
  rdfs:comment "The microgram is a unit of mass defined as 1.0e-6 gram."@en ;
  ns2:symbol "μg" ;
  ns2:unofficialAbbreviation "mcg", "ug" ;
  ns2:hasPrefix ns2:micro ;
  ns2:hasUnit ns2:gram ;
  ns2:hasDimension ns2:mass-Dimension .

ns2:milligram
  a ns2:PrefixedUnit ;
  rdfs:label "milligram"@en, "milligram"@nl, "毫克"@zh ;
  rdfs:comment "The milligram is a unit of mass defined as 1.0e-3 gram."@en ;
  ns2:symbol "mg" ;
  ns2:hasPrefix ns2:milli ;
  ns2:hasUnit ns2:gram ;
  ns2:hasDimension ns2:mass-Dimension .

ns2:centigram
  a ns2:PrefixedUnit ;
  rdfs:label "centigram"@en, "centigram"@nl, "百分之一克"@zh ;
  rdfs:comment "The centigram is a unit of mass defined as 1.0e-2 gram."@en ;
  ns2:symbol "cg" ;
  ns2:hasPrefix ns2:centi ;
  ns2:hasUnit ns2:gram ;
  ns2:hasDimension ns2:mass-Dimension .

ns2:decigram
  a ns2:PrefixedUnit ;
  rdfs:label "decigram"@en, "decigram"@nl, "十分之一克"@zh ;
  rdfs:comment "The decigram is a unit of mass defined as 1.0e-1 gram."@en ;
  ns2:symbol "dg" ;
  ns2:hasPrefix ns2:deci ;
  ns2:hasUnit ns2:gram ;
  ns2:hasDimension ns2:mass-Dimension .

ns2:decagram
  a ns2:PrefixedUnit ;
  rdfs:label "decagram"@en, "decagram"@nl ;
  rdfs:comment "The decagram is a unit of mass defined as 1.0e1 gram."@en ;
  ns2:symbol "dag" ;
  ns2:hasPrefix ns2:deca ;
  ns2:hasUnit ns2:gram ;
  ns2:hasDimension ns2:mass-Dimension .

ns2:hectogram
  a ns2:PrefixedUnit ;
  rdfs:label "hectogram"@en, "hectogram"@nl ;
  ns2:alternativeLabel "100 gram"@en ;
  rdfs:comment "The hectogram is a unit of mass defined as 1.0e2 gram."@en ;
  ns2:symbol "hg" ;
  ns2:hasPrefix ns2:hecto ;
  ns2:hasUnit ns2:gram ;
  ns2:hasDimension ns2:mass-Dimension .

ns2:kilogram
  a ns2:PrefixedUnit ;
  rdfs:label "kilogram"@en, "kilogram"@nl, "公斤"@zh ;
  ns2:symbol "kg" ;
  ns2:hasPrefix ns2:kilo ;
  ns2:hasUnit ns2:gram ;
  ns2:hasDimension ns2:mass-Dimension ;
  rdfs:comment "The kilogram is a unit of mass defined as the mass of the international prototype of the kilogram."@en ;
  ns2:longcomment "The kilogram is a unit of mass defined as the mass of the international prototype of the kilogram. The kilogram is a base unit in the International System of Units." ;
  ns2:hasQuantity ns2:massOfTheInternationalPrototypeOfTheKilogram .

ns2:internationalPrototypeOfTheKilogram
  a owl:Thing ;
  rdfs:label "international prototype of the kilogram"@en .

ns2:massOfTheInternationalPrototypeOfTheKilogram
  a ns2:Mass ;
  rdfs:label "mass of the international prototype of the kilogram"@en ;
  ns2:hasPhenomenon ns2:internationalPrototypeOfTheKilogram .

ns2:megagram
  a ns2:PrefixedUnit ;
  rdfs:label "megagram"@en, "megagram"@nl ;
  rdfs:comment "The megagram is a unit of mass defined as 1.0e6 gram."@en ;
  ns2:symbol "Mg" ;
  ns2:hasPrefix ns2:mega ;
  ns2:hasUnit ns2:gram ;
  ns2:hasDimension ns2:mass-Dimension .

ns2:gigagram
  a ns2:PrefixedUnit ;
  rdfs:label "gigagram"@en, "gigagram"@nl ;
  rdfs:comment "The gigagram is a unit of mass defined as 1.0e9 gram."@en ;
  ns2:symbol "Gg" ;
  ns2:hasPrefix ns2:giga ;
  ns2:hasUnit ns2:gram ;
  ns2:hasDimension ns2:mass-Dimension .

ns2:teragram
  a ns2:PrefixedUnit ;
  rdfs:label "teragram"@en, "teragram"@nl, "10^12克"@zh ;
  rdfs:comment "The teragram is a unit of mass defined as 1.0e12 gram."@en ;
  ns2:symbol "Tg" ;
  ns2:hasPrefix ns2:tera ;
  ns2:hasUnit ns2:gram ;
  ns2:hasDimension ns2:mass-Dimension .

ns2:petagram
  a ns2:PrefixedUnit ;
  rdfs:label "petagram"@en, "petagram"@nl, "10^15克"@zh ;
  rdfs:comment "The petagram is a unit of mass defined as 1.0e15 gram."@en ;
  ns2:symbol "Pg" ;
  ns2:hasPrefix ns2:peta ;
  ns2:hasUnit ns2:gram ;
  ns2:hasDimension ns2:mass-Dimension .

ns2:exagram
  a ns2:PrefixedUnit ;
  rdfs:label "exagram"@en, "exagram"@nl, "千兆兆克"@zh ;
  rdfs:comment "The exagram is a unit of mass defined as 1.0e18 gram."@en ;
  ns2:symbol "Eg" ;
  ns2:hasPrefix ns2:exa ;
  ns2:hasUnit ns2:gram ;
  ns2:hasDimension ns2:mass-Dimension .

ns2:zettagram
  a ns2:PrefixedUnit ;
  rdfs:label "zettagram"@en, "zettagram"@nl, "10^21克"@zh ;
  rdfs:comment "The zettagram is a unit of mass defined as 1.0e21 gram."@en ;
  ns2:symbol "ZG" ;
  ns2:hasPrefix ns2:zetta ;
  ns2:hasUnit ns2:gram ;
  ns2:hasDimension ns2:mass-Dimension .

ns2:yottagram
  a ns2:PrefixedUnit ;
  rdfs:label "yottagram"@en, "yottagram"@nl ;
  rdfs:comment "The yottagram is a unit of mass defined as 1.0e24 gram."@en ;
  ns2:symbol "YG" ;
  ns2:hasPrefix ns2:yotta ;
  ns2:hasUnit ns2:gram ;
  ns2:hasDimension ns2:mass-Dimension .

ns2:kilotonne
  a ns2:PrefixedUnit ;
  rdfs:label "kilotonne"@en, "kiloton"@nl ;
  ns2:symbol "kt" ;
  ns2:hasPrefix ns2:kilo ;
  ns2:hasUnit ns2:tonne ;
  ns2:hasDimension ns2:mass-Dimension .

ns2:megatonne
  a ns2:PrefixedUnit ;
  rdfs:label "megatonne"@en, "megaton"@nl ;
  ns2:symbol "Mt" ;
  ns2:hasPrefix ns2:mega ;
  ns2:hasUnit ns2:tonne ;
  ns2:hasDimension ns2:mass-Dimension .

ns2:nanounifiedAtomicMassUnit
  a ns2:PrefixedUnit ;
  rdfs:label "nanounified atomic mass unit"@en ;
  ns2:symbol "nu" ;
  ns2:hasPrefix ns2:nano ;
  ns2:hasUnit ns2:unifiedAtomicMassUnit ;
  ns2:hasDimension ns2:mass-Dimension .

ns2:one
  a ns2:Unit, ns2:SingularUnit ;
  rdfs:label "one"@en ;
  ns2:alternativeLabel "unit one"@en ;
  rdfs:comment "Unit one is a unit of dimension one."@en ;
  ns2:symbol "1" ;
  ns2:hasDimension ns2:dimensionOne .

ns2:QuantityOfDimensionOneUnit
  a owl:Class ;
  rdfs:label "quantity of dimension one unit"@en ;
  rdfs:subClassOf ns2:Unit ;
  owl:equivalentClass [
    a owl:Class ;
    owl:oneOf (
     ns2:one
     ns2:percent
     ns2:partsPerMillion
     ns2:halfDozen
     ns2:dozen
     ns2:hundredCount
     ns2:gross
     ns2:thousandPiece
   )
  ] .

ns2:percent
  a ns2:Unit, ns2:SingularUnit ;
  rdfs:label "percent"@en, "procent"@nl, "百分"@zh ;
  rdfs:comment "The percent is a unit of dimension one defined as 1/100."@en ;
  ns2:symbol "%" ;
  ns2:LaTeXSymbol "\\%" ;
  ns2:hasFactor "0.01"^^xsd:float ;
  ns2:hasUnit ns2:one ;
  ns2:hasDimension ns2:dimensionOne .

ns2:partsPerMillion
  a ns2:Unit, ns2:SingularUnit ;
  rdfs:label "parts per million"@en ;
  rdfs:comment "Parts per million is a unit of dimension one defined as 1/1 000 000."@en ;
  ns2:symbol "ppm" ;
  ns2:hasFactor "0.000001"^^xsd:float ;
  ns2:hasUnit ns2:one ;
  ns2:hasDimension ns2:dimensionOne .

ns2:halfDozen
  a ns2:Unit, ns2:SingularUnit ;
  rdfs:label "half dozen"@en ;
  rdfs:comment "Half dozen is a unit of dimension one defined as 6."@en ;
  ns2:hasFactor "6"^^xsd:float ;
  ns2:hasUnit ns2:one ;
  ns2:hasDimension ns2:dimensionOne .

ns2:dozen
  a ns2:Unit, ns2:SingularUnit ;
  rdfs:label "dozen"@en ;
  rdfs:comment "Dozen is a unit of dimension one defined as 12."@en ;
  ns2:hasFactor "12"^^xsd:float ;
  ns2:hasUnit ns2:one ;
  ns2:hasDimension ns2:dimensionOne .

ns2:hundredCount
  a ns2:Unit, ns2:SingularUnit ;
  rdfs:label "hundred count"@en ;
  rdfs:comment "Hundred count is a unit of dimension one defined as 100."@en ;
  ns2:hasFactor "100"^^xsd:float ;
  ns2:hasUnit ns2:one ;
  ns2:hasDimension ns2:dimensionOne .

ns2:gross
  a ns2:Unit, ns2:SingularUnit ;
  rdfs:label "gross"@en ;
  rdfs:comment "Gross is a unit of dimension one defined as 144."@en ;
  ns2:hasFactor "144"^^xsd:float ;
  ns2:hasUnit ns2:one ;
  ns2:hasDimension ns2:dimensionOne .

ns2:thousandPiece
  a ns2:Unit, ns2:SingularUnit ;
  rdfs:label "thousand piece"@en ;
  rdfs:comment "Thousand is a unit of dimension one defined as 1000."@en ;
  ns2:hasFactor "1000"^^xsd:float ;
  ns2:hasUnit ns2:one ;
  ns2:hasDimension ns2:dimensionOne .

ns2:NumberUnit
  a owl:Class ;
  rdfs:label "number unit"@en ;
  rdfs:subClassOf ns2:Unit ;
  owl:equivalentClass [
    a owl:Class ;
    owl:oneOf (
     ns2:one
     ns2:halfDozen
     ns2:dozen
     ns2:hundredCount
     ns2:gross
     ns2:thousandPiece
   )
  ] .

ns2:RatioUnit
  a owl:Class ;
  rdfs:label "ratio unit"@en ;
  rdfs:subClassOf ns2:Unit ;
  owl:equivalentClass [
    a owl:Class ;
    owl:oneOf (
     ns2:one
     ns2:percent
     ns2:partsPerMillion
   )
  ] .

ns2:PercentageUnit
  a owl:Class ;
  rdfs:label "percentage unit"@en ;
  rdfs:subClassOf ns2:Unit ;
  owl:equivalentClass [
    a owl:Class ;
    owl:oneOf ( ns2:percent )
  ] .

ns2:MassFractionUnit
  a owl:Class ;
  rdfs:label "mass fraction unit"@en ;
  rdfs:subClassOf ns2:Unit ;
  owl:equivalentClass [
    a owl:Class ;
    owl:oneOf (
     ns2:one
     ns2:partsPerMillion
     ns2:percent
     ns2:gramPerGram
     ns2:gramPerKilogram
     ns2:gramPerHectogram
     ns2:kilogramPerKilogram
     ns2:milligramPerHectogram
     ns2:milligramPerKilogram
     ns2:microgramPerHectogram
   )
  ] .

ns2:gramPerGram
  a ns2:UnitDivision ;
  rdfs:label "gram per gram"@en, "gram per gram"@nl ;
  ns2:symbol "g/g" ;
  ns2:alternativeSymbol "g g-1", "g·g-1" ;
  ns2:hasNumerator ns2:gram ;
  ns2:hasDenominator ns2:gram ;
  ns2:hasDimension ns2:dimensionOne .

ns2:gramPerKilogram
  a ns2:UnitDivision ;
  rdfs:label "gram per kilogram"@en, "gram per kilogram"@nl ;
  ns2:symbol "g/kg" ;
  ns2:alternativeSymbol "g kg-1", "g·kg-1" ;
  ns2:hasNumerator ns2:gram ;
  ns2:hasDenominator ns2:kilogram ;
  ns2:hasFactor "0.001"^^xsd:float ;
  ns2:hasUnit ns2:one ;
  ns2:hasDimension ns2:dimensionOne .

ns2:gramPerHectogram
  a ns2:UnitDivision ;
  rdfs:label "gram per hectogram"@en, "gram per hectogram"@nl ;
  ns2:alternativeLabel "gram per 100 gram"@en, "gram per 100 gram"@nl ;
  ns2:symbol "g/hg" ;
  ns2:alternativeSymbol "g/100 g", "g hg-1", "g·hg-1" ;
  ns2:hasNumerator ns2:gram ;
  ns2:hasDenominator ns2:hectogram ;
  ns2:hasDimension ns2:dimensionOne .

ns2:kilogramPerKilogram
  a ns2:UnitDivision ;
  rdfs:label "kilogram per kilogram"@en, "kilogram per kilogram"@nl ;
  ns2:symbol "kg/kg" ;
  ns2:alternativeSymbol "kg kg-1", "kg·kg-1" ;
  ns2:hasNumerator ns2:kilogram ;
  ns2:hasDenominator ns2:kilogram ;
  ns2:hasDimension ns2:dimensionOne .

ns2:milligramPerHectogram
  a ns2:UnitDivision ;
  rdfs:label "milligram per hectogram"@en, "milligram per hectogram"@nl ;
  ns2:alternativeLabel "milligram per 100 gram"@en, "milligram per 100 gram"@nl ;
  ns2:symbol "mg/hg" ;
  ns2:alternativeSymbol "mg/100 g", "mg hg-1", "mg·hg-1" ;
  ns2:hasNumerator ns2:milligram ;
  ns2:hasDenominator ns2:hectogram ;
  ns2:hasDimension ns2:dimensionOne .

ns2:milligramPerKilogram
  a ns2:UnitDivision ;
  rdfs:label "milligram per kilogram"@en, "milligram per kilogram"@nl ;
  ns2:symbol "mg/kg" ;
  ns2:alternativeSymbol "mg kg-1", "mg·kg-1" ;
  ns2:hasNumerator ns2:milligram ;
  ns2:hasDenominator ns2:kilogram ;
  ns2:hasDimension ns2:dimensionOne .

ns2:microgramPerHectogram
  a ns2:UnitDivision ;
  rdfs:label "microgram per hectogram"@en, "microgram per hectogram"@nl ;
  ns2:alternativeLabel "microgram per 100 gram"@en, "microgram per 100 gram"@nl ;
  ns2:symbol "μg/hg" ;
  ns2:alternativeSymbol "μg/100 g", "μg hg-1", "μg·hg-1" ;
  ns2:hasNumerator ns2:microgram ;
  ns2:hasDenominator ns2:hectogram ;
  ns2:hasDimension ns2:dimensionOne .

ns2:AreaFractionUnit
  a owl:Class ;
  rdfs:label "area fraction unit"@en ;
  rdfs:subClassOf ns2:Unit ;
  owl:equivalentClass [
    a owl:Class ;
    owl:oneOf (
     ns2:one
     ns2:partsPerMillion
     ns2:percent
     ns2:squareMetrePerSquareMetre
   )
  ] .

ns2:VolumeFractionUnit
  a owl:Class ;
  rdfs:label "volume fraction unit"@en ;
  rdfs:subClassOf ns2:Unit ;
  owl:equivalentClass [
    a owl:Class ;
    owl:oneOf (
     ns2:one
     ns2:partsPerMillion
     ns2:percent
     ns2:cubicCentimetrePerCubicCentimetre
     ns2:cubicMetrePerCubicmetre
     ns2:cubicMillimetrePerCubicMillimetre
   )
  ] .

ns2:cubicCentimetrePerCubicCentimetre
  a ns2:UnitDivision ;
  rdfs:label "cubic centimetre per cubic centimetre"@en, "kubieke centimeter per kubieke centimeter"@nl ;
  ns2:symbol "cm3/cm3" ;
  ns2:alternativeSymbol "cm3 cm-3", "cm3·cm-3" ;
  ns2:hasNumerator ns2:cubicCentimetre ;
  ns2:hasDenominator ns2:cubicCentimetre ;
  ns2:hasDimension ns2:dimensionOne .

ns2:cubicMetrePerCubicmetre
  a ns2:UnitDivision ;
  rdfs:label "cubic metre per cubic metre"@en, "kubieke meter per kubieke meter"@nl ;
  ns2:symbol "m3/m3" ;
  ns2:alternativeSymbol "m3 m-3", "m3·m-3" ;
  ns2:hasNumerator ns2:cubicMetre ;
  ns2:hasDenominator ns2:cubicMetre ;
  ns2:hasDimension ns2:dimensionOne .

ns2:cubicMillimetrePerCubicMillimetre
  a ns2:UnitDivision ;
  rdfs:label "cubic millimetre per cubic millimetre"@en, "kubieke millimeter per kubieke millimeter"@nl ;
  ns2:symbol "mm3/mm3" ;
  ns2:alternativeSymbol "mm3 mm-3", "mm3·mm-3" ;
  ns2:hasNumerator ns2:cubicMillimetre ;
  ns2:hasDenominator ns2:cubicMillimetre ;
  ns2:hasDimension ns2:dimensionOne .

ns2:RelativeHumidityUnit
  a owl:Class ;
  rdfs:label "relative humidity unit"@en ;
  rdfs:subClassOf ns2:Unit ;
  owl:equivalentClass [
    a owl:Class ;
    owl:oneOf (
     ns2:one
     ns2:percent
   )
  ] .

ns2:reciprocalSecond-Time
  a ns2:UnitExponentiation ;
  rdfs:label "reciprocal second"@en, "omgekeerde seconde"@nl ;
  ns2:symbol "s-1" ;
  ns2:hasBase ns2:second-Time ;
  ns2:hasExponent -1 ;
  ns2:hasDimension ns2:frequency-Dimension .

ns2:FrequencyUnit
  a owl:Class ;
  rdfs:label "frequency unit"@en ;
  rdfs:subClassOf ns2:Unit ;
  owl:equivalentClass [
    a owl:Class ;
    owl:unionOf (
     _:genid381
     ns2:PrefixedHertz
   )
  ] .

ns2:hertz
  a ns2:Unit, ns2:SingularUnit ;
  rdfs:label "hertz"@en, "hertz"@nl, "赫兹"@zh ;
  rdfs:comment "The hertz is a unit of frequency defined as 1 divided by second."@en ;
  ns2:longcomment "The hertz is a unit of frequency defined as 1 divided by second. The hertz is a derived unit in the International System of Units." ;
  ns2:symbol "Hz" ;
  ns2:hasUnit ns2:reciprocalSecond-Time ;
  ns2:hasDimension ns2:frequency-Dimension .

ns2:reciprocalMinute-Time
  a ns2:UnitExponentiation ;
  rdfs:label "reciprocal minute"@en, "omgekeerde minuut"@nl ;
  ns2:symbol "min-1" ;
  ns2:hasBase ns2:minute-Time ;
  ns2:hasExponent -1 ;
  ns2:hasDimension ns2:frequency-Dimension .

ns2:reciprocalHour
  a ns2:UnitExponentiation ;
  rdfs:label "reciprocal hour"@en, "omgekeerd uur"@nl ;
  ns2:symbol "h-1" ;
  ns2:hasBase ns2:hour ;
  ns2:hasExponent -1 ;
  ns2:hasDimension ns2:frequency-Dimension .

ns2:reciprocalDay
  a ns2:UnitExponentiation ;
  rdfs:label "reciprocal day"@en, "omgekeerde dag"@nl ;
  ns2:symbol "d-1" ;
  ns2:hasBase ns2:day ;
  ns2:hasExponent -1 ;
  ns2:hasDimension ns2:frequency-Dimension .

ns2:reciprocalYear
  a ns2:UnitExponentiation ;
  rdfs:label "reciprocal year"@en, "omgekeerd jaar"@nl ;
  ns2:symbol "a-1" ;
  ns2:hasBase ns2:year ;
  ns2:hasExponent -1 ;
  ns2:hasDimension ns2:frequency-Dimension .

ns2:PrefixedHertz
  a owl:Class ;
  rdfs:label "prefixed hertz"@en ;
  rdfs:subClassOf ns2:PrefixedUnit ;
  owl:equivalentClass [
    a owl:Class ;
    owl:intersectionOf (
     _:genid393
     _:genid395
     _:genid397
     _:genid399
   )
  ] .

ns2:yoctohertz
  a ns2:PrefixedUnit ;
  rdfs:label "yoctohertz"@en, "yoctohertz"@nl ;
  rdfs:comment "The yoctohertz is a unit of frequency defined as 1.0e-24 hertz."@en ;
  ns2:symbol "yHz" ;
  ns2:hasPrefix ns2:yocto ;
  ns2:hasUnit ns2:hertz ;
  ns2:hasDimension ns2:frequency-Dimension .

ns2:zeptohertz
  a ns2:PrefixedUnit ;
  rdfs:label "zeptohertz"@en, "zeptohertz"@nl ;
  rdfs:comment "The zepthertz is a unit of frequency defined as 1.0e-21 hertz."@en ;
  ns2:symbol "zHz" ;
  ns2:hasPrefix ns2:zepto ;
  ns2:hasUnit ns2:hertz ;
  ns2:hasDimension ns2:frequency-Dimension .

ns2:attohertz
  a ns2:PrefixedUnit ;
  rdfs:label "attohertz"@en, "attohertz"@nl ;
  rdfs:comment "The attohertz is a unit of frequency defined as 1.0e-18 hertz."@en ;
  ns2:symbol "aHz" ;
  ns2:hasPrefix ns2:atto ;
  ns2:hasUnit ns2:hertz ;
  ns2:hasDimension ns2:frequency-Dimension .

ns2:femtohertz
  a ns2:PrefixedUnit ;
  rdfs:label "femtohertz"@en, "femtohertz"@nl ;
  rdfs:comment "The femtohertz is a unit of frequency defined as 1.0e-15 hertz."@en ;
  ns2:symbol "fHz" ;
  ns2:hasPrefix ns2:femto ;
  ns2:hasUnit ns2:hertz ;
  ns2:hasDimension ns2:frequency-Dimension .

ns2:picohertz
  a ns2:PrefixedUnit ;
  rdfs:label "picohertz"@en, "picohertz"@nl ;
  rdfs:comment "The picohertz is a unit of frequency defined as 1.0e-12 hertz."@en ;
  ns2:symbol "pHz" ;
  ns2:hasPrefix ns2:pico ;
  ns2:hasUnit ns2:hertz ;
  ns2:hasDimension ns2:frequency-Dimension .

ns2:nanohertz
  a ns2:PrefixedUnit ;
  rdfs:label "nanohertz"@en, "nanohertz"@nl ;
  rdfs:comment "The nanohertz is a unit of frequency defined as 1.0e-9 hertz."@en ;
  ns2:symbol "nHz" ;
  ns2:hasPrefix ns2:nano ;
  ns2:hasUnit ns2:hertz ;
  ns2:hasDimension ns2:frequency-Dimension .

ns2:microhertz
  a ns2:PrefixedUnit ;
  rdfs:label "microhertz"@en, "microhertz"@nl ;
  rdfs:comment "The microhertz is a unit of frequency defined as 1.0e-6 hertz."@en ;
  ns2:symbol "μHz" ;
  ns2:hasPrefix ns2:micro ;
  ns2:hasUnit ns2:hertz ;
  ns2:hasDimension ns2:frequency-Dimension .

ns2:millihertz
  a ns2:PrefixedUnit ;
  rdfs:label "millihertz"@en, "millihertz"@nl ;
  rdfs:comment "The millihertz is a unit of frequency defined as 1.0e-3 hertz."@en ;
  ns2:symbol "mHz" ;
  ns2:hasPrefix ns2:milli ;
  ns2:hasUnit ns2:hertz ;
  ns2:hasDimension ns2:frequency-Dimension .

ns2:centihertz
  a ns2:PrefixedUnit ;
  rdfs:label "centihertz"@en, "centihertz"@nl ;
  rdfs:comment "The centihertz is a unit of frequency defined as 1.0e-2 hertz."@en ;
  ns2:symbol "cHz" ;
  ns2:hasPrefix ns2:centi ;
  ns2:hasUnit ns2:hertz ;
  ns2:hasDimension ns2:frequency-Dimension .

ns2:decihertz
  a ns2:PrefixedUnit ;
  rdfs:label "decihertz"@en, "decihertz"@nl ;
  rdfs:comment "The decihertz is a unit of frequency defined as 1.0e-1 hertz."@en ;
  ns2:symbol "dHz" ;
  ns2:hasPrefix ns2:deci ;
  ns2:hasUnit ns2:hertz ;
  ns2:hasDimension ns2:frequency-Dimension .

ns2:decahertz
  a ns2:PrefixedUnit ;
  rdfs:label "decahertz"@en, "decahertz"@nl ;
  rdfs:comment "The decahertz is a unit of frequency defined as 1.0e1 hertz."@en ;
  ns2:symbol "daHz" ;
  ns2:hasPrefix ns2:deca ;
  ns2:hasUnit ns2:hertz ;
  ns2:hasDimension ns2:frequency-Dimension .

ns2:hectohertz
  a ns2:PrefixedUnit ;
  rdfs:label "hectohertz"@en, "hectohertz"@nl ;
  rdfs:comment "The hectohertz is a unit of frequency defined as 1.0e2 hertz."@en ;
  ns2:symbol "hHz" ;
  ns2:hasPrefix ns2:hecto ;
  ns2:hasUnit ns2:hertz ;
  ns2:hasDimension ns2:frequency-Dimension .

ns2:kilohertz
  a ns2:PrefixedUnit ;
  rdfs:label "kilohertz"@en, "kilohertz"@nl ;
  rdfs:comment "The kilohertz is a unit of frequency defined as 1.0e3 hertz."@en ;
  ns2:symbol "kHz" ;
  ns2:hasPrefix ns2:kilo ;
  ns2:hasUnit ns2:hertz ;
  ns2:hasDimension ns2:frequency-Dimension .

ns2:megahertz
  a ns2:PrefixedUnit ;
  rdfs:label "megahertz"@en, "megahertz"@nl ;
  rdfs:comment "The megahertz is a unit of frequency defined as 1.0e6 hertz."@en ;
  ns2:symbol "MHz" ;
  ns2:hasPrefix ns2:mega ;
  ns2:hasUnit ns2:hertz ;
  ns2:hasDimension ns2:frequency-Dimension .

ns2:gigahertz
  a ns2:PrefixedUnit ;
  rdfs:label "gigahertz"@en, "gigahertz"@nl ;
  rdfs:comment "The gigahertz is a unit of frequency defined as 1.0e9 hertz."@en ;
  ns2:symbol "GHz" ;
  ns2:hasPrefix ns2:giga ;
  ns2:hasUnit ns2:hertz ;
  ns2:hasDimension ns2:frequency-Dimension .

ns2:terahertz
  a ns2:PrefixedUnit ;
  rdfs:label "terahertz"@en, "terahertz"@nl ;
  rdfs:comment "The terahertz is a unit of frequency defined as 1.0e12 hertz."@en ;
  ns2:symbol "THz" ;
  ns2:hasPrefix ns2:tera ;
  ns2:hasUnit ns2:hertz ;
  ns2:hasDimension ns2:frequency-Dimension .

ns2:petahertz
  a ns2:PrefixedUnit ;
  rdfs:label "petahertz"@en, "petahertz"@nl ;
  rdfs:comment "The petahertz is a unit of frequency defined as 1.0e15 hertz."@en ;
  ns2:symbol "PHz" ;
  ns2:hasPrefix ns2:peta ;
  ns2:hasUnit ns2:hertz ;
  ns2:hasDimension ns2:frequency-Dimension .

ns2:exahertz
  a ns2:PrefixedUnit ;
  rdfs:label "exahertz"@en, "exahertz"@nl ;
  rdfs:comment "The exahertz is a unit of frequency defined as 1.0e18 hertz."@en ;
  ns2:symbol "EHz" ;
  ns2:hasPrefix ns2:exa ;
  ns2:hasUnit ns2:hertz ;
  ns2:hasDimension ns2:frequency-Dimension .

ns2:zettahertz
  a ns2:PrefixedUnit ;
  rdfs:label "zettahertz"@en, "zettahertz"@nl ;
  rdfs:comment "The zettahertz is a unit of frequency defined as 1.0e21 hertz."@en ;
  ns2:symbol "ZHz" ;
  ns2:hasPrefix ns2:zetta ;
  ns2:hasUnit ns2:hertz ;
  ns2:hasDimension ns2:frequency-Dimension .

ns2:yottahertz
  a ns2:PrefixedUnit ;
  rdfs:label "yottahertz"@en, "yottahertz"@nl ;
  rdfs:comment "The yottahertz is a unit of frequency defined as 1.0e24 hertz."@en ;
  ns2:symbol "YHz" ;
  ns2:hasPrefix ns2:yotta ;
  ns2:hasUnit ns2:hertz ;
  ns2:hasDimension ns2:frequency-Dimension .

ns2:reciprocalCubicMetre
  a ns2:UnitExponentiation ;
  rdfs:label "reciprocal cubic metre"@en, "omgekeerde kubieke meter"@nl ;
  ns2:symbol "m-3" ;
  ns2:hasBase ns2:metre ;
  ns2:hasExponent -3 ;
  ns2:hasDimension ns2:numberDensity-Dimension .

ns2:NumberDensityUnit
  a owl:Class ;
  rdfs:label "number density unit"@en ;
  rdfs:subClassOf ns2:Unit ;
  owl:equivalentClass [
    a owl:Class ;
    owl:oneOf (
     ns2:reciprocalCubicCentimetre
     ns2:reciprocalLitre
     ns2:reciprocalCubicMetre
     ns2:reciprocalCubicParsec
   )
  ] .

ns2:reciprocalCubicCentimetre
  a ns2:UnitExponentiation ;
  rdfs:label "reciprocal cubic centimetre"@en, "omgekeerde kubieke centimeter"@nl ;
  ns2:symbol "cm-3" ;
  ns2:hasBase ns2:centimetre ;
  ns2:hasExponent -3 ;
  ns2:hasDimension ns2:numberDensity-Dimension .

ns2:reciprocalLitre
  a ns2:UnitExponentiation ;
  rdfs:label "reciprocal litre"@en, "omgekeerde liter"@nl ;
  ns2:symbol "l-1" ;
  ns2:hasBase ns2:litre ;
  ns2:hasExponent -1 ;
  ns2:hasDimension ns2:numberDensity-Dimension .

ns2:reciprocalCubicParsec
  a ns2:UnitExponentiation ;
  rdfs:label "reciprocal cubic parsec"@en, "omgekeerde kubieke parsec"@nl ;
  ns2:symbol "pc-3" ;
  ns2:hasBase ns2:parsec ;
  ns2:hasExponent -3 ;
  ns2:hasDimension ns2:numberDensity-Dimension .

ns2:reciprocalMetre
  a ns2:UnitExponentiation ;
  rdfs:label "reciprocal metre"@en, "omgekeerder meter"@nl ;
  rdfs:comment "Reciprocal metre is a unit of wavenumber defined as 1 divided by metre."@en ;
  ns2:longcomment "Reciprocal metre is a unit of wavenumber defined as 1 divided by metre. Reciprocal metre is a derived unit in the International System of Units." ;
  ns2:symbol "m-1" ;
  ns2:hasBase ns2:metre ;
  ns2:hasExponent -1 ;
  ns2:hasDimension ns2:wavenumber-Dimension .

ns2:WavenumberUnit
  a owl:Class ;
  rdfs:label "wave number unit"@en ;
  rdfs:subClassOf ns2:Unit ;
  owl:equivalentClass [
    a owl:Class ;
    owl:oneOf (
     ns2:kayser
     ns2:reciprocalMetre
   )
  ] .

ns2:kayser
  a ns2:Unit, ns2:SingularUnit ;
  rdfs:label "kayser"@en, "kayser"@nl ;
  ns2:alternativeLabel "rydberg"@en, "rydberg"@nl ;
  rdfs:comment "The kayser is a unit of wavenumber defined as 100 reciprocal metre."@en ;
  ns2:hasFactor "1.0e2"^^xsd:float ;
  ns2:hasUnit ns2:reciprocalMetre ;
  ns2:hasDimension ns2:wavenumber-Dimension .

ns2:metrePerSecond-TimeSquared
  a ns2:UnitDivision ;
  rdfs:label "metre per second squared"@en, "meter per seconde kwadraat"@nl ;
  rdfs:comment "Metre per second squared is a unit of acceleration defined as metre divided by second squared."@en ;
  ns2:longcomment "Metre per second squared is a unit of acceleration defined as metre divided by second squared. Metre per second squared is a derived unit in the International System of Units." ;
  ns2:symbol "m/s2" ;
  ns2:alternativeSymbol "m s-2", "m·s-2" ;
  ns2:hasNumerator ns2:metre ;
  ns2:hasDenominator ns2:second-TimeSquared ;
  ns2:hasDimension ns2:acceleration-Dimension .

ns2:AccelerationUnit
  a owl:Class ;
  rdfs:label "acceleration unit"@en ;
  rdfs:subClassOf ns2:Unit ;
  owl:equivalentClass [
    a owl:Class ;
    owl:unionOf (
     _:genid414
     ns2:PrefixedMetrePerSecond-TimeSquared
     ns2:MetrePerPrefixedSecond-TimeSquared
     ns2:PrefixedMetrePerPrefixedSecond-TimeSquared
   )
  ] .

ns2:gal
  a ns2:Unit, ns2:SingularUnit ;
  rdfs:label "gal"@en, "gal"@nl ;
  ns2:alternativeLabel "galileo"@en, "galileo"@nl ;
  rdfs:comment "The gal is a unit of acceleration defined as centimetre per second (time) squared."@en ;
  ns2:symbol "Gal" ;
  ns2:hasUnit ns2:centimetrePerSecond-TimeSquared ;
  ns2:hasDimension ns2:acceleration-Dimension .

ns2:PrefixedMetrePerSecond-TimeSquared
  a owl:Class ;
  rdfs:label "prefixed metre per second (time) squared"@en ;
  rdfs:subClassOf ns2:UnitDivision ;
  owl:equivalentClass [
    a owl:Class ;
    owl:intersectionOf (
     _:genid424
     _:genid426
     _:genid428
     _:genid430
   )
  ] .

ns2:MetrePerPrefixedSecond-TimeSquared
  a owl:Class ;
  rdfs:label "metre per prefixed second (time) squared"@en ;
  rdfs:subClassOf ns2:UnitDivision ;
  owl:equivalentClass [
    a owl:Class ;
    owl:intersectionOf (
     _:genid433
     _:genid435
     _:genid437
     _:genid439
   )
  ] .

ns2:PrefixedMetrePerPrefixedSecond-TimeSquared
  a owl:Class ;
  rdfs:label "prefixed metre per prefixed secon (time) squared"@en ;
  rdfs:subClassOf ns2:UnitDivision ;
  owl:equivalentClass [
    a owl:Class ;
    owl:intersectionOf (
     _:genid442
     _:genid444
     _:genid446
     _:genid448
   )
  ] .

ns2:yoctometrePerSecond-TimeSquared
  a ns2:PrefixedMetrePerSecond-TimeSquared ;
  rdfs:label "yoctometre per second squared"@en, "yoctometer per seconde kwadraat"@nl ;
  rdfs:comment "Yoctometre per second squared is a unit of acceleration defined as yoctometre divided by second squared."@en ;
  ns2:symbol "ym/s2" ;
  ns2:alternativeSymbol "ym s-2", "ym·s-2" ;
  ns2:hasNumerator ns2:yoctometre ;
  ns2:hasDenominator ns2:second-TimeSquared ;
  ns2:hasDimension ns2:acceleration-Dimension .

ns2:zeptometrePerSecond-TimeSquared
  a ns2:PrefixedMetrePerSecond-TimeSquared ;
  rdfs:label "zeptometre per second squared"@en, "zeptometer per seconde kwadraat"@nl ;
  rdfs:comment "Zeptometre per second squared is a unit of acceleration defined as zeptometre divided by second squared."@en ;
  ns2:symbol "zm/s2" ;
  ns2:alternativeSymbol "zm s-2", "zm·s-2" ;
  ns2:hasNumerator ns2:zeptometre ;
  ns2:hasDenominator ns2:second-TimeSquared ;
  ns2:hasDimension ns2:acceleration-Dimension .

ns2:attometrePerSecond-TimeSquared
  a ns2:PrefixedMetrePerSecond-TimeSquared ;
  rdfs:label "attometre per second squared"@en, "attometer per seconde kwadraat"@nl ;
  rdfs:comment "Attometre per second squared is a unit of acceleration defined as attometre divided by second squared."@en ;
  ns2:symbol "am/s2" ;
  ns2:alternativeSymbol "am s-2", "am·s-2" ;
  ns2:hasNumerator ns2:attometre ;
  ns2:hasDenominator ns2:second-TimeSquared ;
  ns2:hasDimension ns2:acceleration-Dimension .

ns2:femtometrePerSecond-TimeSquared
  a ns2:PrefixedMetrePerSecond-TimeSquared ;
  rdfs:label "femtometre per second squared"@en, "femtometer per seconde kwadraat"@nl ;
  rdfs:comment "Femtometre per second squared is a unit of acceleration defined as femtometre divided by second squared."@en ;
  ns2:symbol "fm/s2" ;
  ns2:alternativeSymbol "fm s-2", "fm·s-2" ;
  ns2:hasNumerator ns2:femtometre ;
  ns2:hasDenominator ns2:second-TimeSquared ;
  ns2:hasDimension ns2:acceleration-Dimension .

ns2:picometrePerSecond-TimeSquared
  a ns2:PrefixedMetrePerSecond-TimeSquared ;
  rdfs:label "picometre per second squared"@en, "picometer per seconde kwadraat"@nl ;
  rdfs:comment "Picometre per second squared is a unit of acceleration defined as picometre divided by second squared."@en ;
  ns2:symbol "pm/s2" ;
  ns2:alternativeSymbol "pm s-2", "pm·s-2" ;
  ns2:hasNumerator ns2:picometre ;
  ns2:hasDenominator ns2:second-TimeSquared ;
  ns2:hasDimension ns2:acceleration-Dimension .

ns2:nanometrePerSecond-TimeSquared
  a ns2:PrefixedMetrePerSecond-TimeSquared ;
  rdfs:label "nanometre per second squared"@en, "nanometer per seconde kwadraat"@nl ;
  rdfs:comment "Nanometre per second squared is a unit of acceleration defined as nanometre divided by second squared."@en ;
  ns2:symbol "nm/s2" ;
  ns2:alternativeSymbol "nm s-2", "nm·s-2" ;
  ns2:hasNumerator ns2:nanometre ;
  ns2:hasDenominator ns2:second-TimeSquared ;
  ns2:hasDimension ns2:acceleration-Dimension .

ns2:micrometrePerSecond-TimeSquared
  a ns2:PrefixedMetrePerSecond-TimeSquared ;
  rdfs:label "micrometre per second squared"@en, "micrometer per seconde kwadraat"@nl ;
  rdfs:comment "Micrometre per second squared is a unit of acceleration defined as micrometre divided by second squared."@en ;
  ns2:symbol "μm/s2" ;
  ns2:alternativeSymbol "μm s-2", "μm·s-2" ;
  ns2:hasNumerator ns2:micrometre ;
  ns2:hasDenominator ns2:second-TimeSquared ;
  ns2:hasDimension ns2:acceleration-Dimension .

ns2:millimetrePerSecond-TimeSquared
  a ns2:PrefixedMetrePerSecond-TimeSquared ;
  rdfs:label "millimetre per second squared"@en, "millimeter per seconde kwadraat"@nl ;
  rdfs:comment "Millimetre per second squared is a unit of acceleration defined as millimetre divided by second squared."@en ;
  ns2:symbol "mm/s2" ;
  ns2:alternativeSymbol "mm s-2", "mm·s-2" ;
  ns2:hasNumerator ns2:millimetre ;
  ns2:hasDenominator ns2:second-TimeSquared ;
  ns2:hasDimension ns2:acceleration-Dimension .

ns2:centimetrePerSecond-TimeSquared
  a ns2:PrefixedMetrePerSecond-TimeSquared ;
  rdfs:label "centimetre per second squared"@en, "centimeter per seconde kwadraat"@nl ;
  rdfs:comment "Centimetre per second squared is a unit of acceleration defined as centimetre divided by second squared."@en ;
  ns2:symbol "cm/s2" ;
  ns2:alternativeSymbol "cm s-2", "cm·s-2" ;
  ns2:hasNumerator ns2:centimetre ;
  ns2:hasDenominator ns2:second-TimeSquared ;
  ns2:hasDimension ns2:acceleration-Dimension .

ns2:decimetrePerSecond-TimeSquared
  a ns2:PrefixedMetrePerSecond-TimeSquared ;
  rdfs:label "decimetre per second squared"@en, "decimeter per seconde kwadraat"@nl ;
  rdfs:comment "Decimetre per second squared is a unit of acceleration defined as decimetre divided by second squared."@en ;
  ns2:symbol "dm/s2" ;
  ns2:alternativeSymbol "dm s-2", "dm·s-2" ;
  ns2:hasNumerator ns2:decimetre ;
  ns2:hasDenominator ns2:second-TimeSquared ;
  ns2:hasDimension ns2:acceleration-Dimension .

ns2:decametrePerSecond-TimeSquared
  a ns2:PrefixedMetrePerSecond-TimeSquared ;
  rdfs:label "decametre per second squared"@en, "decameter per seconde kwadraat"@nl ;
  rdfs:comment "Decametre per second squared is a unit of acceleration defined as decametre divided by second squared."@en ;
  ns2:symbol "dam/s2" ;
  ns2:alternativeSymbol "dam s-2", "dam·s-2" ;
  ns2:hasNumerator ns2:decametre ;
  ns2:hasDenominator ns2:second-TimeSquared ;
  ns2:hasDimension ns2:acceleration-Dimension .

ns2:hectometrePerSecond-TimeSquared
  a ns2:PrefixedMetrePerSecond-TimeSquared ;
  rdfs:label "hectometre per second squared"@en, "hectometer per seconde kwadraat"@nl ;
  rdfs:comment "Hectometre per second squared is a unit of acceleration defined as hectometre divided by second squared."@en ;
  ns2:symbol "hm/s2" ;
  ns2:alternativeSymbol "hm s-2", "hm·s-2" ;
  ns2:hasNumerator ns2:hectometre ;
  ns2:hasDenominator ns2:second-TimeSquared ;
  ns2:hasDimension ns2:acceleration-Dimension .

ns2:kilometrePerSecond-TimeSquared
  a ns2:PrefixedMetrePerSecond-TimeSquared ;
  rdfs:label "kilometre per second squared"@en, "kilometer per seconde kwadraat"@nl ;
  rdfs:comment "Kilometre per second squared is a unit of acceleration defined as kilometre divided by second squared."@en ;
  ns2:symbol "km/s2" ;
  ns2:alternativeSymbol "km s-2", "km·s-2" ;
  ns2:hasNumerator ns2:kilometre ;
  ns2:hasDenominator ns2:second-TimeSquared ;
  ns2:hasDimension ns2:acceleration-Dimension .

ns2:megametrePerSecond-TimeSquared
  a ns2:PrefixedMetrePerSecond-TimeSquared ;
  rdfs:label "megametre per second squared"@en, "megameter per seconde kwadraat"@nl ;
  rdfs:comment "Megametre per second squared is a unit of acceleration defined as megametre divided by second squared."@en ;
  ns2:symbol "Mm/s2" ;
  ns2:alternativeSymbol "Mm s-2", "Mm·s-2" ;
  ns2:hasNumerator ns2:megametre ;
  ns2:hasDenominator ns2:second-TimeSquared ;
  ns2:hasDimension ns2:acceleration-Dimension .

ns2:gigametrePerSecond-TimeSquared
  a ns2:PrefixedMetrePerSecond-TimeSquared ;
  rdfs:label "gigametre per second squared"@en, "gigameter per seconde kwadraat"@nl ;
  rdfs:comment "Gigametre per second squared is a unit of acceleration defined as gigametre divided by second squared."@en ;
  ns2:symbol "Gm/s2" ;
  ns2:alternativeSymbol "Gm s-2", "Gm·s-2" ;
  ns2:hasNumerator ns2:gigametre ;
  ns2:hasDenominator ns2:second-TimeSquared ;
  ns2:hasDimension ns2:acceleration-Dimension .

ns2:terametrePerSecond-TimeSquared
  a ns2:PrefixedMetrePerSecond-TimeSquared ;
  rdfs:label "terametre per second squared"@en, "terameter per seconde kwadraat"@nl ;
  rdfs:comment "Terametre per second squared is a unit of acceleration defined as terametre divided by second squared."@en ;
  ns2:symbol "Tm/s2" ;
  ns2:alternativeSymbol "Tm s-2", "Tm·s-2" ;
  ns2:hasNumerator ns2:terametre ;
  ns2:hasDenominator ns2:second-TimeSquared ;
  ns2:hasDimension ns2:acceleration-Dimension .

ns2:petametrePerSecond-TimeSquared
  a ns2:PrefixedMetrePerSecond-TimeSquared ;
  rdfs:label "petametre per second squared"@en, "petameter per seconde kwadraat"@nl ;
  rdfs:comment "Petametre per second squared is a unit of acceleration defined as petametre divided by second squared."@en ;
  ns2:symbol "Pm/s2" ;
  ns2:alternativeSymbol "Pm s-2", "Pm·s-2" ;
  ns2:hasNumerator ns2:petametre ;
  ns2:hasDenominator ns2:second-TimeSquared ;
  ns2:hasDimension ns2:acceleration-Dimension .

ns2:exametrePerSecond-TimeSquared
  a ns2:PrefixedMetrePerSecond-TimeSquared ;
  rdfs:label "exametre per second squared"@en, "exameter per seconde kwadraat"@nl ;
  rdfs:comment "Exametre per second squared is a unit of acceleration defined as exametre divided by second squared."@en ;
  ns2:symbol "Em/s2" ;
  ns2:alternativeSymbol "Em s-2", "Em·s-2" ;
  ns2:hasNumerator ns2:exametre ;
  ns2:hasDenominator ns2:second-TimeSquared ;
  ns2:hasDimension ns2:acceleration-Dimension .

ns2:zettametrePerSecond-TimeSquared
  a ns2:PrefixedMetrePerSecond-TimeSquared ;
  rdfs:label "zettametre per second squared"@en, "zettameter per seconde kwadraat"@nl ;
  rdfs:comment "Zettametre per second squared is a unit of acceleration defined as zettametre divided by second squared."@en ;
  ns2:symbol "Zm/s2" ;
  ns2:alternativeSymbol "Zm s-2", "Zm·s-2" ;
  ns2:hasNumerator ns2:zettametre ;
  ns2:hasDenominator ns2:second-TimeSquared ;
  ns2:hasDimension ns2:acceleration-Dimension .

ns2:yottametrePerSecond-TimeSquared
  a ns2:PrefixedMetrePerSecond-TimeSquared ;
  rdfs:label "yottametre per second squared"@en, "yottameter per seconde kwadraat"@nl ;
  rdfs:comment "Yottametre per second squared is a unit of acceleration defined as yottametre divided by second squared."@en ;
  ns2:symbol "Ym/s2" ;
  ns2:alternativeSymbol "Ym s-2", "Ym·s-2" ;
  ns2:hasNumerator ns2:yottametre ;
  ns2:hasDenominator ns2:second-TimeSquared ;
  ns2:hasDimension ns2:acceleration-Dimension .

ns2:metrePerYoctosecond-TimeSquared
  a ns2:MetrePerPrefixedSecond-TimeSquared ;
  rdfs:label "metre per yoctosecond squared"@en, "meter per yoctoseconde kwadraat"@nl ;
  rdfs:comment "Metre per yoctosecond squared is a unit of acceleration defined as metre divided by yoctosecond squared."@en ;
  ns2:symbol "m/ys2" ;
  ns2:alternativeSymbol "m ys-2", "m·ys-2" ;
  ns2:hasNumerator ns2:metre ;
  ns2:hasDenominator ns2:yoctosecond-TimeSquared ;
  ns2:hasDimension ns2:acceleration-Dimension .

ns2:metrePerZeptosecond-TimeSquared
  a ns2:MetrePerPrefixedSecond-TimeSquared ;
  rdfs:label "metre per zeptosecond squared"@en, "meter per zeptoseconde kwadraat"@nl ;
  rdfs:comment "Metre per zeptosecond squared is a unit of acceleration defined as metre divided by zeptosecond squared."@en ;
  ns2:symbol "m/zs2" ;
  ns2:alternativeSymbol "m zs-2", "m·zs-2" ;
  ns2:hasNumerator ns2:metre ;
  ns2:hasDenominator ns2:zeptosecond-TimeSquared ;
  ns2:hasDimension ns2:acceleration-Dimension .

ns2:metrePerAttosecond-TimeSquared
  a ns2:MetrePerPrefixedSecond-TimeSquared ;
  rdfs:label "metre per attosecond squared"@en, "meter per attoseconde kwadraat"@nl ;
  rdfs:comment "Metre per attosecond squared is a unit of acceleration defined as metre divided by attosecond squared."@en ;
  ns2:symbol "m/as2" ;
  ns2:alternativeSymbol "m as-2", "m·as-2" ;
  ns2:hasNumerator ns2:metre ;
  ns2:hasDenominator ns2:attosecond-TimeSquared ;
  ns2:hasDimension ns2:acceleration-Dimension .

ns2:metrePerFemtosecond-TimeSquared
  a ns2:MetrePerPrefixedSecond-TimeSquared ;
  rdfs:label "metre per femtosecond squared"@en, "meter per femtoseconde kwadraat"@nl ;
  rdfs:comment "Metre per femtosecond squared is a unit of acceleration defined as metre divided by femtosecond squared."@en ;
  ns2:symbol "m/fs2" ;
  ns2:alternativeSymbol "m fs-2", "m·fs-2" ;
  ns2:hasNumerator ns2:metre ;
  ns2:hasDenominator ns2:femtosecond-TimeSquared ;
  ns2:hasDimension ns2:acceleration-Dimension .

ns2:metrePerPicosecond-TimeSquared
  a ns2:MetrePerPrefixedSecond-TimeSquared ;
  rdfs:label "metre per picosecond squared"@en, "meter per picoseconde kwadraat"@nl ;
  rdfs:comment "Metre per picosecond squared is a unit of acceleration defined as metre divided by picosecond squared."@en ;
  ns2:symbol "m/ps2" ;
  ns2:alternativeSymbol "m ps-2", "m·ps-2" ;
  ns2:hasNumerator ns2:metre ;
  ns2:hasDenominator ns2:picosecond-TimeSquared ;
  ns2:hasDimension ns2:acceleration-Dimension .

ns2:metrePerNanosecond-TimeSquared
  a ns2:MetrePerPrefixedSecond-TimeSquared ;
  rdfs:label "metre per nanosecond squared"@en, "meter per nanoseconde kwadraat"@nl ;
  rdfs:comment "Metre per nanosecond squared is a unit of acceleration defined as metre divided by nanosecond squared."@en ;
  ns2:symbol "m/ns2" ;
  ns2:alternativeSymbol "m ns-2", "m·ns-2" ;
  ns2:hasNumerator ns2:metre ;
  ns2:hasDenominator ns2:nanosecond-TimeSquared ;
  ns2:hasDimension ns2:acceleration-Dimension .

ns2:metrePerMicrosecond-TimeSquared
  a ns2:MetrePerPrefixedSecond-TimeSquared ;
  rdfs:label "metre per microsecond squared"@en, "meter per microseconde kwadraat"@nl ;
  rdfs:comment "Metre per microsecond squared is a unit of acceleration defined as metre divided by microsecond squared."@en ;
  ns2:symbol "m/μs2" ;
  ns2:alternativeSymbol "m μs-2", "m·μs-2" ;
  ns2:hasNumerator ns2:metre ;
  ns2:hasDenominator ns2:microsecond-TimeSquared ;
  ns2:hasDimension ns2:acceleration-Dimension .

ns2:metrePerMillisecond-TimeSquared
  a ns2:MetrePerPrefixedSecond-TimeSquared ;
  rdfs:label "metre per millisecond squared"@en, "meter per milliseconde kwadraat"@nl ;
  rdfs:comment "Metre per millisecond squared is a unit of acceleration defined as metre divided by millisecond squared."@en ;
  ns2:symbol "m/ms2" ;
  ns2:alternativeSymbol "m ms-2", "m·ms-2" ;
  ns2:hasNumerator ns2:metre ;
  ns2:hasDenominator ns2:millisecond-TimeSquared ;
  ns2:hasDimension ns2:acceleration-Dimension .

ns2:metrePerCentisecond-TimeSquared
  a ns2:MetrePerPrefixedSecond-TimeSquared ;
  rdfs:label "metre per centisecond squared"@en, "meter per centiseconde kwadraat"@nl ;
  rdfs:comment "Metre per centisecond squared is a unit of acceleration defined as metre divided by centisecond squared."@en ;
  ns2:symbol "m/cs2" ;
  ns2:alternativeSymbol "m cs-2", "m·cs-2" ;
  ns2:hasNumerator ns2:metre ;
  ns2:hasDenominator ns2:centisecond-TimeSquared ;
  ns2:hasDimension ns2:acceleration-Dimension .

ns2:metrePerDecisecond-TimeSquared
  a ns2:MetrePerPrefixedSecond-TimeSquared ;
  rdfs:label "metre per decisecond squared"@en, "meter per deciseconde kwadraat"@nl ;
  rdfs:comment "Metre per decisecond squared is a unit of acceleration defined as metre divided by decisecond squared."@en ;
  ns2:symbol "m/ds2" ;
  ns2:alternativeSymbol "m ds-2", "m·ds-2" ;
  ns2:hasNumerator ns2:metre ;
  ns2:hasDenominator ns2:decisecond-TimeSquared ;
  ns2:hasDimension ns2:acceleration-Dimension .

ns2:metrePerDecasecond-TimeSquared
  a ns2:MetrePerPrefixedSecond-TimeSquared ;
  rdfs:label "metre per decasecond squared"@en, "meter per decaseconde kwadraat"@nl ;
  rdfs:comment "Metre per decasecond squared is a unit of acceleration defined as metre divided by decasecond squared."@en ;
  ns2:symbol "m/das2" ;
  ns2:alternativeSymbol "m das-2", "m·das-2" ;
  ns2:hasNumerator ns2:metre ;
  ns2:hasDenominator ns2:decasecond-TimeSquared ;
  ns2:hasDimension ns2:acceleration-Dimension .

ns2:metrePerHectosecond-TimeSquared
  a ns2:MetrePerPrefixedSecond-TimeSquared ;
  rdfs:label "metre per hectosecond squared"@en, "meter per hectoseconde kwadraat"@nl ;
  rdfs:comment "Metre per hectosecond squared is a unit of acceleration defined as metre divided by hectosecond squared."@en ;
  ns2:symbol "m/hs2" ;
  ns2:alternativeSymbol "m hs-2", "m·hs-2" ;
  ns2:hasNumerator ns2:metre ;
  ns2:hasDenominator ns2:hectosecond-TimeSquared ;
  ns2:hasDimension ns2:acceleration-Dimension .

ns2:metrePerKilosecond-TimeSquared
  a ns2:MetrePerPrefixedSecond-TimeSquared ;
  rdfs:label "metre per kilosecond squared"@en, "meter per kiloseconde kwadraat"@nl ;
  rdfs:comment "Metre per kilosecond squared is a unit of acceleration defined as metre divided by kilosecond squared."@en ;
  ns2:symbol "m/ks2" ;
  ns2:alternativeSymbol "m ks-2", "m·ks-2" ;
  ns2:hasNumerator ns2:metre ;
  ns2:hasDenominator ns2:kilosecond-TimeSquared ;
  ns2:hasDimension ns2:acceleration-Dimension .

ns2:metrePerMegasecond-TimeSquared
  a ns2:MetrePerPrefixedSecond-TimeSquared ;
  rdfs:label "metre per megasecond squared"@en, "meter per megaseconde kwadraat"@nl ;
  rdfs:comment "Metre per megasecond squared is a unit of acceleration defined as metre divided by megasecond squared."@en ;
  ns2:symbol "m/Ms2" ;
  ns2:alternativeSymbol "m Ms-2", "m·Ms-2" ;
  ns2:hasNumerator ns2:metre ;
  ns2:hasDenominator ns2:megasecond-TimeSquared ;
  ns2:hasDimension ns2:acceleration-Dimension .

ns2:metrePerGigasecond-TimeSquared
  a ns2:MetrePerPrefixedSecond-TimeSquared ;
  rdfs:label "metre per gigasecond squared"@en, "meter per gigaseconde kwadraat"@nl ;
  rdfs:comment "Metre per gigasecond squared is a unit of acceleration defined as metre divided by gigasecond squared."@en ;
  ns2:symbol "m/Gs2" ;
  ns2:alternativeSymbol "m Gs-2", "m·Gs-2" ;
  ns2:hasNumerator ns2:metre ;
  ns2:hasDenominator ns2:gigasecond-TimeSquared ;
  ns2:hasDimension ns2:acceleration-Dimension .

ns2:metrePerTerasecond-TimeSquared
  a ns2:MetrePerPrefixedSecond-TimeSquared ;
  rdfs:label "metre per terasecond squared"@en, "meter per teraseconde kwadraat"@nl ;
  rdfs:comment "Metre per terasecond squared is a unit of acceleration defined as metre divided by terasecond squared."@en ;
  ns2:symbol "m/Ts2" ;
  ns2:alternativeSymbol "m Ts-2", "m·Ts-2" ;
  ns2:hasNumerator ns2:metre ;
  ns2:hasDenominator ns2:terasecond-TimeSquared ;
  ns2:hasDimension ns2:acceleration-Dimension .

ns2:metrePerPetasecond-TimeSquared
  a ns2:MetrePerPrefixedSecond-TimeSquared ;
  rdfs:label "metre per petasecond squared"@en, "meter per petaseconde kwadraat"@nl ;
  rdfs:comment "Metre per petasecond squared is a unit of acceleration defined as metre divided by petasecond squared."@en ;
  ns2:symbol "m/Ps2" ;
  ns2:alternativeSymbol "m Ps-2", "m·Ps-2" ;
  ns2:hasNumerator ns2:metre ;
  ns2:hasDenominator ns2:petasecond-TimeSquared ;
  ns2:hasDimension ns2:acceleration-Dimension .

ns2:metrePerExasecond-TimeSquared
  a ns2:MetrePerPrefixedSecond-TimeSquared ;
  rdfs:label "metre per exasecond squared"@en, "meter per exaseconde kwadraat"@nl ;
  rdfs:comment "Metre per exasecond squared is a unit of acceleration defined as metre divided by exasecond squared."@en ;
  ns2:symbol "m/Es2" ;
  ns2:alternativeSymbol "m Es-2", "m·Es-2" ;
  ns2:hasNumerator ns2:metre ;
  ns2:hasDenominator ns2:exasecond-TimeSquared ;
  ns2:hasDimension ns2:acceleration-Dimension .

ns2:metrePerZettasecond-TimeSquared
  a ns2:MetrePerPrefixedSecond-TimeSquared ;
  rdfs:label "metre per zettasecond squared"@en, "meter per zettaseconde kwadraat"@nl ;
  rdfs:comment "Metre per zettasecond squared is a unit of acceleration defined as metre divided by zettasecond squared."@en ;
  ns2:symbol "m/Zs2" ;
  ns2:alternativeSymbol "m Zs-2", "m·Zs-2" ;
  ns2:hasNumerator ns2:metre ;
  ns2:hasDenominator ns2:zettasecond-TimeSquared ;
  ns2:hasDimension ns2:acceleration-Dimension .

ns2:metrePerYottasecond-TimeSquared
  a ns2:MetrePerPrefixedSecond-TimeSquared ;
  rdfs:label "metre per yottasecond squared"@en, "meter per yottaseconde kwadraat"@nl ;
  rdfs:comment "Metre per yottasecond squared is a unit of acceleration defined as metre divided by yottasecond squared."@en ;
  ns2:symbol "m/Ys2" ;
  ns2:alternativeSymbol "m Ys-2", "m·Ys-2" ;
  ns2:hasNumerator ns2:metre ;
  ns2:hasDenominator ns2:yottasecond-TimeSquared ;
  ns2:hasDimension ns2:acceleration-Dimension .

ns2:kilogramPerCubicmetre
  a ns2:UnitDivision ;
  rdfs:label "kilogram per cubic metre"@en, "kilogram per kubieke meter"@nl ;
  rdfs:comment "Kilogram per cubic metre is a unit of density defined as kilogram divided by cubic metre."@en ;
  ns2:longcomment "Kilogram per cubic metre is a unit of density defined as kilogram divided by cubic metre. Kilogram per cubic metre is a derived unit in the International System of Units." ;
  ns2:symbol "kg/m3" ;
  ns2:alternativeSymbol "kg m-3", "kg·m-3" ;
  ns2:hasNumerator ns2:kilogram ;
  ns2:hasDenominator ns2:cubicMetre ;
  ns2:hasDimension ns2:density-Dimension .

ns2:DensityUnit
  a owl:Class ;
  rdfs:label "density unit"@en ;
  rdfs:subClassOf ns2:Unit ;
  owl:equivalentClass [
    a owl:Class ;
    owl:unionOf (
     _:genid451
     ns2:PrefixedGramPerLitre
     ns2:GramPerPrefixedLitre
     ns2:PrefixedGramPerPrefixedLitre
   )
  ] .

ns2:gramPerCubicmetre
  a ns2:UnitDivision ;
  rdfs:label "gram per cubic metre"@en, "gram per kubieke meter"@nl ;
  rdfs:comment "Gram per cubic metre is a unit of density defined as gram divided by cubic metre."@en ;
  ns2:longcomment "Gram per cubic metre is a unit of density defined as gram divided by cubic metre. Gram per cubic metre is a derived unit in the International System of Units." ;
  ns2:symbol "g/m3" ;
  ns2:alternativeSymbol "g m-3", "g·m-3" ;
  ns2:hasNumerator ns2:gram ;
  ns2:hasDenominator ns2:cubicMetre ;
  ns2:hasDimension ns2:density-Dimension .

ns2:milligramPerCubicmetre
  a ns2:UnitDivision ;
  rdfs:label "milligram per cubic metre"@en, "milligram per kubieke meter"@nl ;
  rdfs:comment "Milligram per cubic metre is a unit of density defined as milligram divided by cubic metre."@en ;
  ns2:longcomment "Milligram per cubic metre is a unit of density defined as milligram divided by cubic metre. Milligram per cubic metre is a derived unit in the International System of Units." ;
  ns2:symbol "mg/m3" ;
  ns2:alternativeSymbol "mg m-3", "mg·m-3" ;
  ns2:hasNumerator ns2:milligram ;
  ns2:hasDenominator ns2:cubicMetre ;
  ns2:hasDimension ns2:density-Dimension .

ns2:gramPerCubicCentimetre
  a ns2:UnitDivision ;
  rdfs:label "gram per cubic centimetre"@en, "gram per kubieke centimeter"@nl ;
  rdfs:comment "Gram per cubic centimetre is a unit of density defined as gram divided by cubic centimetre."@en ;
  ns2:longcomment "Gram per cubic centimetre is a unit of density defined as gram divided by cubic centimetre. Gram per cubic centimetre is a derived unit in the International System of Units." ;
  ns2:symbol "g/cm3" ;
  ns2:alternativeSymbol "g cm-3", "g·cm-3" ;
  ns2:hasNumerator ns2:gram ;
  ns2:hasDenominator ns2:cubicCentimetre ;
  ns2:hasDimension ns2:density-Dimension .

ns2:microgramPerCubicCentimetre
  a ns2:UnitDivision ;
  rdfs:label "microgram per cubic centimetre"@en, "microgram per kubieke centimeter"@nl ;
  rdfs:comment "Microram per cubic centimetre is a unit of density defined as microgram divided by cubic centimetre."@en ;
  ns2:longcomment "Microgram per cubic centimetre is a unit of density defined as microgram divided by cubic centimetre. Microgram per cubic centimetre is a derived unit in the International System of Units." ;
  ns2:symbol "μg/cm3" ;
  ns2:alternativeSymbol "μg cm-3", "μg·cm-3" ;
  ns2:hasNumerator ns2:microgram ;
  ns2:hasDenominator ns2:cubicCentimetre ;
  ns2:hasDimension ns2:density-Dimension .

ns2:kilogramPerCubicDecimetre
  a ns2:UnitDivision ;
  rdfs:label "kilogram per cubic decimetre"@en, "kilogram per kubieke decimeter"@nl ;
  rdfs:comment "Kilogram per cubic decimetre is a unit of density defined as kilogram divided by cubic decimetre."@en ;
  ns2:longcomment "Kilogram per cubic decimetre is a unit of density defined as kilogram divided by cubic decimetre. Kilogram per cubic decimetre is a derived unit in the International System of Units." ;
  ns2:symbol "kg/dm3" ;
  ns2:alternativeSymbol "kg dm-3", "kg·dm-3" ;
  ns2:hasNumerator ns2:kilogram ;
  ns2:hasDenominator ns2:cubicDecimetre ;
  ns2:hasDimension ns2:density-Dimension .

ns2:gramPerLitre
  a ns2:UnitDivision ;
  rdfs:label "gram per litre"@en, "gram per liter"@nl ;
  rdfs:comment "Gram per litre is a unit of density defined as gram divided by litre."@en ;
  ns2:longcomment "Gram per litre is a unit of density defined as gram divided by litre. Gram per litre is a derived unit in the International System of Units." ;
  ns2:symbol "g/l" ;
  ns2:alternativeSymbol "g l-1", "g·l-1" ;
  ns2:hasNumerator ns2:gram ;
  ns2:hasDenominator ns2:litre ;
  ns2:hasDimension ns2:density-Dimension .

ns2:solarMassPerCubicParsec
  a ns2:UnitDivision ;
  rdfs:label "solar mass per cubic parsec"@en, "zonsmassa per kubieke parsec"@nl ;
  rdfs:comment "The mass (in solar masses) per cubic parsec."@en ;
  ns2:symbol "M_☉/pc3" ;
  ns2:alternativeSymbol "M_☉ pc-3", "M_☉·pc-3" ;
  ns2:LaTeXSymbol "M_{\\astrosun} pc^{-3}" ;
  ns2:hasNumerator ns2:solarMass ;
  ns2:hasDenominator ns2:cubicParsec ;
  ns2:hasDimension ns2:density-Dimension .

ns2:PrefixedGramPerLitre
  a owl:Class ;
  rdfs:label "prefixed gram per litre"@en ;
  rdfs:subClassOf ns2:UnitDivision ;
  owl:equivalentClass [
    a owl:Class ;
    owl:intersectionOf (
     _:genid467
     _:genid469
     _:genid471
     _:genid473
   )
  ] .

ns2:GramPerPrefixedLitre
  a owl:Class ;
  rdfs:label "gram per prefixed litre"@en ;
  rdfs:subClassOf ns2:UnitDivision ;
  owl:equivalentClass [
    a owl:Class ;
    owl:intersectionOf (
     _:genid476
     _:genid478
     _:genid480
     _:genid482
   )
  ] .

ns2:PrefixedGramPerPrefixedLitre
  a owl:Class ;
  rdfs:label "prefixed gram per prefixed litre"@en ;
  rdfs:subClassOf ns2:UnitDivision ;
  owl:equivalentClass [
    a owl:Class ;
    owl:intersectionOf (
     _:genid485
     _:genid487
     _:genid489
     _:genid491
   )
  ] .

ns2:yoctogramPerLitre
  a ns2:PrefixedGramPerLitre ;
  rdfs:label "yoctogram per litre"@en, "yoctogram per liter"@nl ;
  rdfs:comment "Yoctogram per litre is a unit of density defined as yoctogram divided by litre."@en ;
  ns2:symbol "yg/l" ;
  ns2:alternativeSymbol "yg l-1", "yg·l-1" ;
  ns2:hasNumerator ns2:yoctogram ;
  ns2:hasDenominator ns2:litre ;
  ns2:hasDimension ns2:density-Dimension .

ns2:zeptogramPerLitre
  a ns2:PrefixedGramPerLitre ;
  rdfs:label "zeptogram per litre"@en, "zeptogram per liter"@nl ;
  rdfs:comment "Zeptogram per litre is a unit of density defined as zeptogram divided by litre."@en ;
  ns2:symbol "zg/l" ;
  ns2:alternativeSymbol "zg l-1", "zg·l-1" ;
  ns2:hasNumerator ns2:zeptogram ;
  ns2:hasDenominator ns2:litre ;
  ns2:hasDimension ns2:density-Dimension .

ns2:attogramPerLitre
  a ns2:PrefixedGramPerLitre ;
  rdfs:label "attogram per litre"@en, "attogram per liter"@nl ;
  rdfs:comment "Attogram per litre is a unit of density defined as attogram divided by litre."@en ;
  ns2:symbol "ag/l" ;
  ns2:alternativeSymbol "ag l-1", "ag·l-1" ;
  ns2:hasNumerator ns2:attogram ;
  ns2:hasDenominator ns2:litre ;
  ns2:hasDimension ns2:density-Dimension .

ns2:femtogramPerLitre
  a ns2:PrefixedGramPerLitre ;
  rdfs:label "femtogram per litre"@en, "femtogram per liter"@nl ;
  rdfs:comment "Femtogram per litre is a unit of density defined as femtogram divided by litre."@en ;
  ns2:symbol "fg/l" ;
  ns2:alternativeSymbol "fm s-1", "fm·s-1" ;
  ns2:hasNumerator ns2:femtogram ;
  ns2:hasDenominator ns2:litre ;
  ns2:hasDimension ns2:density-Dimension .

ns2:picogramPerLitre
  a ns2:PrefixedGramPerLitre ;
  rdfs:label "picogram per litre"@en, "picogram per liter"@nl ;
  rdfs:comment "Picogram per litre is a unit of density defined as picogram divided by litre."@en ;
  ns2:symbol "pg/l" ;
  ns2:alternativeSymbol "pg l-1", "pg·l-1" ;
  ns2:hasNumerator ns2:picogram ;
  ns2:hasDenominator ns2:litre ;
  ns2:hasDimension ns2:density-Dimension .

ns2:nanogramPerLitre
  a ns2:PrefixedGramPerLitre ;
  rdfs:label "nanogram per litre"@en, "nanogram per liter"@nl ;
  rdfs:comment "Nanogram per litre is a unit of density defined as nanogram divided by litre."@en ;
  ns2:symbol "ng/l" ;
  ns2:alternativeSymbol "ng l-1", "ng·l-1" ;
  ns2:hasNumerator ns2:nanogram ;
  ns2:hasDenominator ns2:litre ;
  ns2:hasDimension ns2:density-Dimension .

ns2:microgramPerLitre
  a ns2:PrefixedGramPerLitre ;
  rdfs:label "microgram per litre"@en, "microgram per liter"@nl ;
  rdfs:comment "Microgram per litre is a unit of density defined as microgram divided by litre."@en ;
  ns2:symbol "μg/l" ;
  ns2:alternativeSymbol "μg l-1", "μg·l-1" ;
  ns2:hasNumerator ns2:microgram ;
  ns2:hasDenominator ns2:litre ;
  ns2:hasDimension ns2:density-Dimension .

ns2:milligramPerLitre
  a ns2:PrefixedGramPerLitre ;
  rdfs:label "milligram per litre"@en, "milligram per liter"@nl ;
  rdfs:comment "Milligram per litre is a unit of density defined as milligram divided by litre."@en ;
  ns2:symbol "mg/l" ;
  ns2:alternativeSymbol "mg l-1", "mg·l-1" ;
  ns2:hasNumerator ns2:milligram ;
  ns2:hasDenominator ns2:litre ;
  ns2:hasDimension ns2:density-Dimension .

ns2:centigramPerLitre
  a ns2:PrefixedGramPerLitre ;
  rdfs:label "centigram per litre"@en, "centigram per liter"@nl ;
  rdfs:comment "Centigram per litre is a unit of density defined as centigram divided by litre."@en ;
  ns2:symbol "cg/l" ;
  ns2:alternativeSymbol "cg l-1", "cg·l-1" ;
  ns2:hasNumerator ns2:centigram ;
  ns2:hasDenominator ns2:litre ;
  ns2:hasDimension ns2:density-Dimension .

ns2:decigramPerLitre
  a ns2:PrefixedGramPerLitre ;
  rdfs:label "decigram per litre"@en, "decigram per liter"@nl ;
  rdfs:comment "Decigram per litre is a unit of density defined as decigram divided by litre."@en ;
  ns2:symbol "dg/l" ;
  ns2:alternativeSymbol "dg l-1", "dg·l-1" ;
  ns2:hasNumerator ns2:decigram ;
  ns2:hasDenominator ns2:litre ;
  ns2:hasDimension ns2:density-Dimension .

ns2:decagramPerLitre
  a ns2:PrefixedGramPerLitre ;
  rdfs:label "decagram per litre"@en, "decagram per liter"@nl ;
  rdfs:comment "Decagram per litre is a unit of density defined as decagram divided by litre."@en ;
  ns2:symbol "dag/l" ;
  ns2:alternativeSymbol "dag l-1", "dag·l-1" ;
  ns2:hasNumerator ns2:decagram ;
  ns2:hasDenominator ns2:litre ;
  ns2:hasDimension ns2:density-Dimension .

ns2:hectogramPerLitre
  a ns2:PrefixedGramPerLitre ;
  rdfs:label "hectogram per litre"@en, "hectogram per liter"@nl ;
  rdfs:comment "Hectogram per litre is a unit of density defined as hectogram divided by litre."@en ;
  ns2:symbol "hg/l" ;
  ns2:alternativeSymbol "hg l-1", "hg·l-1" ;
  ns2:hasNumerator ns2:hectogram ;
  ns2:hasDenominator ns2:litre ;
  ns2:hasDimension ns2:density-Dimension .

ns2:kilogramPerLitre
  a ns2:PrefixedGramPerLitre ;
  rdfs:label "kilogram per litre"@en, "kilogram per liter"@nl ;
  rdfs:comment "Kilogram per litre is a unit of density defined as kilogram divided by litre."@en ;
  ns2:symbol "kg/l" ;
  ns2:alternativeSymbol "kg l-1", "kg·l-1" ;
  ns2:hasNumerator ns2:kilogram ;
  ns2:hasDenominator ns2:litre ;
  ns2:hasDimension ns2:density-Dimension .

ns2:megagramPerLitre
  a ns2:PrefixedGramPerLitre ;
  rdfs:label "megagram per litre"@en, "megagram per liter"@nl ;
  rdfs:comment "Megagram per litre is a unit of density defined as megagram divided by litre."@en ;
  ns2:symbol "Mg/l" ;
  ns2:alternativeSymbol "Mg l-1", "Mg·l-1" ;
  ns2:hasNumerator ns2:megagram ;
  ns2:hasDenominator ns2:litre ;
  ns2:hasDimension ns2:density-Dimension .

ns2:gigagramPerLitre
  a ns2:PrefixedGramPerLitre ;
  rdfs:label "gigagram per litre"@en, "gigagram per liter"@nl ;
  rdfs:comment "Gigagram per litre is a unit of density defined as gigagram divided by litre."@en ;
  ns2:symbol "Gg/l" ;
  ns2:alternativeSymbol "Gg l-1", "Gg·l-1" ;
  ns2:hasNumerator ns2:gigagram ;
  ns2:hasDenominator ns2:litre ;
  ns2:hasDimension ns2:density-Dimension .

ns2:teragramPerLitre
  a ns2:PrefixedGramPerLitre ;
  rdfs:label "teragram per litre"@en, "teragram per liter"@nl ;
  rdfs:comment "Teragram per litre is a unit of density defined as teragram divided by litre."@en ;
  ns2:symbol "Tg/l" ;
  ns2:alternativeSymbol "Tg l-1", "Tg·l-1" ;
  ns2:hasNumerator ns2:teragram ;
  ns2:hasDenominator ns2:litre ;
  ns2:hasDimension ns2:density-Dimension .

ns2:petagramPerLitre
  a ns2:PrefixedGramPerLitre ;
  rdfs:label "petagram per litre"@en, "petagram per liter"@nl ;
  rdfs:comment "Petagram per litre is a unit of density defined as petagram divided by litre."@en ;
  ns2:symbol "Pg/l" ;
  ns2:alternativeSymbol "Pg l-1", "Pg·l-1" ;
  ns2:hasNumerator ns2:petagram ;
  ns2:hasDenominator ns2:litre ;
  ns2:hasDimension ns2:density-Dimension .

ns2:exagramPerLitre
  a ns2:PrefixedGramPerLitre ;
  rdfs:label "exagram per litre"@en, "exagram per liter"@nl ;
  rdfs:comment "Exagram per litre is a unit of density defined as exagram divided by litre."@en ;
  ns2:symbol "Eg/l" ;
  ns2:alternativeSymbol "Eg l-1", "Eg·l-1" ;
  ns2:hasNumerator ns2:exagram ;
  ns2:hasDenominator ns2:litre ;
  ns2:hasDimension ns2:density-Dimension .

ns2:zettagramPerLitre
  a ns2:PrefixedGramPerLitre ;
  rdfs:label "zettagram per litre"@en, "zettagram per liter"@nl ;
  rdfs:comment "Zettagram per litre is a unit of density defined as zettagram divided by litre."@en ;
  ns2:symbol "Zg/l" ;
  ns2:alternativeSymbol "Zg l-1", "Zg·l-1" ;
  ns2:hasNumerator ns2:zettagram ;
  ns2:hasDenominator ns2:litre ;
  ns2:hasDimension ns2:density-Dimension .

ns2:yottagramPerLitre
  a ns2:PrefixedGramPerLitre ;
  rdfs:label "yottagram per litre"@en, "yottagram per liter"@nl ;
  rdfs:comment "Yottagram per litre is a unit of density defined as yottagram divided by litre."@en ;
  ns2:symbol "Yg/l" ;
  ns2:alternativeSymbol "Yg l-1", "Yg·l-1" ;
  ns2:hasNumerator ns2:yottagram ;
  ns2:hasDenominator ns2:litre ;
  ns2:hasDimension ns2:density-Dimension .

ns2:gramPerYoctolitre
  a ns2:GramPerPrefixedLitre ;
  rdfs:label "gram per yoctolitre"@en, "gram per yoctoliter"@nl ;
  rdfs:comment "Gram per yoctolitre is a unit of density defined as gram divided by yoctolitre."@en ;
  ns2:symbol "g/yl" ;
  ns2:alternativeSymbol "g yl-1", "g·yl-1" ;
  ns2:hasNumerator ns2:gram ;
  ns2:hasDenominator ns2:yoctolitre ;
  ns2:hasDimension ns2:density-Dimension .

ns2:gramPerZeptolitre
  a ns2:GramPerPrefixedLitre ;
  rdfs:label "gram per zeptolitre"@en, "gram per zeptoliter"@nl ;
  rdfs:comment "Gram per zeptolitre is a unit of density defined as gram divided by zeptolitre."@en ;
  ns2:symbol "g/zl" ;
  ns2:alternativeSymbol "g zl-1", "g·zl-1" ;
  ns2:hasNumerator ns2:gram ;
  ns2:hasDenominator ns2:zeptolitre ;
  ns2:hasDimension ns2:density-Dimension .

ns2:gramPerAttolitre
  a ns2:GramPerPrefixedLitre ;
  rdfs:label "gram per attolitre"@en, "gram per attoliter"@nl ;
  rdfs:comment "Gram per attolitre is a unit of density defined as gram divided by attolitre."@en ;
  ns2:symbol "g/al" ;
  ns2:alternativeSymbol "g al-1", "g·al-1" ;
  ns2:hasNumerator ns2:gram ;
  ns2:hasDenominator ns2:attolitre ;
  ns2:hasDimension ns2:density-Dimension .

ns2:gramPerFemtolitre
  a ns2:GramPerPrefixedLitre ;
  rdfs:label "gram per femtolitre"@en, "gram per femtoliter"@nl ;
  rdfs:comment "Gram per femtolitre is a unit of density defined as gram divided by femtolitre."@en ;
  ns2:symbol "g/fl" ;
  ns2:alternativeSymbol "g fl-1", "g·fl-1" ;
  ns2:hasNumerator ns2:gram ;
  ns2:hasDenominator ns2:femtolitre ;
  ns2:hasDimension ns2:density-Dimension .

ns2:gramPerPicolitre
  a ns2:GramPerPrefixedLitre ;
  rdfs:label "gram per picolitre"@en, "gram per picoliter"@nl ;
  rdfs:comment "Gram per picolitre is a unit of density defined as gram divided by picolitre."@en ;
  ns2:symbol "g/pl" ;
  ns2:alternativeSymbol "g pl-1", "g·pl-1" ;
  ns2:hasNumerator ns2:gram ;
  ns2:hasDenominator ns2:picolitre ;
  ns2:hasDimension ns2:density-Dimension .

ns2:gramPerNanolitre
  a ns2:GramPerPrefixedLitre ;
  rdfs:label "gram per nanolitre"@en, "gram per nanoliter"@nl ;
  rdfs:comment "Gram per nanolitre is a unit of density defined as gram divided by nanolitre."@en ;
  ns2:symbol "g/nl" ;
  ns2:alternativeSymbol "g nl-1", "g·nl-1" ;
  ns2:hasNumerator ns2:gram ;
  ns2:hasDenominator ns2:nanolitre ;
  ns2:hasDimension ns2:density-Dimension .

ns2:gramPerMicrolitre
  a ns2:GramPerPrefixedLitre ;
  rdfs:label "gram per microlitre"@en, "gram per microliter"@nl ;
  rdfs:comment "Gram per microlitre is a unit of density defined as gram divided by microlitre."@en ;
  ns2:symbol "g/μl" ;
  ns2:alternativeSymbol "g μl-1", "g·μl-1" ;
  ns2:hasNumerator ns2:gram ;
  ns2:hasDenominator ns2:microlitre ;
  ns2:hasDimension ns2:density-Dimension .

ns2:gramPerMillilitre
  a ns2:GramPerPrefixedLitre ;
  rdfs:label "gram per millilitre"@en, "gram per milliliter"@nl ;
  rdfs:comment "Gram per millilitre is a unit of density defined as gram divided by millilitre."@en ;
  ns2:symbol "g/ml" ;
  ns2:alternativeSymbol "g ml-1", "g·ml-1" ;
  ns2:hasNumerator ns2:gram ;
  ns2:hasDenominator ns2:millilitre ;
  ns2:hasDimension ns2:density-Dimension .

ns2:gramPerCentilitre
  a ns2:GramPerPrefixedLitre ;
  rdfs:label "gram per centilitre"@en, "gram per centiliter"@nl ;
  rdfs:comment "Gram per centilitre is a unit of density defined as gram divided by centilitre."@en ;
  ns2:symbol "g/cl" ;
  ns2:alternativeSymbol "g cl-1", "g·cl-1" ;
  ns2:hasNumerator ns2:gram ;
  ns2:hasDenominator ns2:centilitre ;
  ns2:hasDimension ns2:density-Dimension .

ns2:gramPerDecilitre
  a ns2:GramPerPrefixedLitre ;
  rdfs:label "gram per decilitre"@en, "gram per deciliter"@nl ;
  rdfs:comment "Gram per decilitre is a unit of density defined as gram divided by decilitre."@en ;
  ns2:symbol "g/dl" ;
  ns2:alternativeSymbol "g dl-1", "g·dl-1" ;
  ns2:hasNumerator ns2:gram ;
  ns2:hasDenominator ns2:decilitre ;
  ns2:hasDimension ns2:density-Dimension .

ns2:gramPerDecalitre
  a ns2:GramPerPrefixedLitre ;
  rdfs:label "gram per decalitre"@en, "gram per decaliter"@nl ;
  rdfs:comment "Gram per decalitre is a unit of density defined as gram divided by decalitre."@en ;
  ns2:symbol "g/dal" ;
  ns2:alternativeSymbol "g dal-1", "g·dal-1" ;
  ns2:hasNumerator ns2:gram ;
  ns2:hasDenominator ns2:decalitre ;
  ns2:hasDimension ns2:density-Dimension .

ns2:gramPerHectolitre
  a ns2:GramPerPrefixedLitre ;
  rdfs:label "gram per hectolitre"@en, "gram per hectoliter"@nl ;
  rdfs:comment "Gram per hectolitre is a unit of density defined as gram divided by hectolitre."@en ;
  ns2:symbol "g/hl" ;
  ns2:alternativeSymbol "g hl-1", "g·hl-1" ;
  ns2:hasNumerator ns2:gram ;
  ns2:hasDenominator ns2:hectolitre ;
  ns2:hasDimension ns2:density-Dimension .

ns2:gramPerKilolitre
  a ns2:GramPerPrefixedLitre ;
  rdfs:label "gram per kilolitre"@en, "gram per kiloliter"@nl ;
  rdfs:comment "Gram per kilolitre is a unit of density defined as gram divided by kilolitre."@en ;
  ns2:symbol "g/kl" ;
  ns2:alternativeSymbol "g kl-1", "g·kl-1" ;
  ns2:hasNumerator ns2:gram ;
  ns2:hasDenominator ns2:kilolitre ;
  ns2:hasDimension ns2:density-Dimension .

ns2:gramPerMegalitre
  a ns2:GramPerPrefixedLitre ;
  rdfs:label "gram per megalitre"@en, "gram per megaliter"@nl ;
  rdfs:comment "Gram per megalitre is a unit of density defined as gram divided by megalitre."@en ;
  ns2:symbol "g/Ml" ;
  ns2:alternativeSymbol "g Ml-1", "g·Ml-1" ;
  ns2:hasNumerator ns2:gram ;
  ns2:hasDenominator ns2:megalitre ;
  ns2:hasDimension ns2:density-Dimension .

ns2:gramPerGigalitre
  a ns2:GramPerPrefixedLitre ;
  rdfs:label "gram per gigalitre"@en, "gram per gigaliter"@nl ;
  rdfs:comment "Gram per gigalitre is a unit of density defined as gram divided by gigalitre."@en ;
  ns2:symbol "g/Gl" ;
  ns2:alternativeSymbol "g Gl-1", "g·Gl-1" ;
  ns2:hasNumerator ns2:gram ;
  ns2:hasDenominator ns2:gigalitre ;
  ns2:hasDimension ns2:density-Dimension .

ns2:gramPerTeralitre
  a ns2:GramPerPrefixedLitre ;
  rdfs:label "gram per teralitre"@en, "gram per teraliter"@nl ;
  rdfs:comment "Gram per teralitre is a unit of density defined as gram divided by teralitre."@en ;
  ns2:symbol "g/Tl" ;
  ns2:alternativeSymbol "g Tl-1", "g·Tl-1" ;
  ns2:hasNumerator ns2:gram ;
  ns2:hasDenominator ns2:teralitre ;
  ns2:hasDimension ns2:density-Dimension .

ns2:gramPerPetalitre
  a ns2:GramPerPrefixedLitre ;
  rdfs:label "gram per petalitre"@en, "gram per petaliter"@nl ;
  rdfs:comment "Gram per petalitre is a unit of density defined as gram divided by petalitre."@en ;
  ns2:symbol "g/Pl" ;
  ns2:alternativeSymbol "g Pl-1", "g·Pl-1" ;
  ns2:hasNumerator ns2:gram ;
  ns2:hasDenominator ns2:petalitre ;
  ns2:hasDimension ns2:density-Dimension .

ns2:gramPerExalitre
  a ns2:GramPerPrefixedLitre ;
  rdfs:label "gram per exalitre"@en, "gram per exaliter"@nl ;
  rdfs:comment "Gram per exalitre is a unit of density defined as gram divided by exalitre."@en ;
  ns2:symbol "g/El" ;
  ns2:alternativeSymbol "g El-1", "g·El-1" ;
  ns2:hasNumerator ns2:gram ;
  ns2:hasDenominator ns2:exalitre ;
  ns2:hasDimension ns2:density-Dimension .

ns2:gramPerZettalitre
  a ns2:GramPerPrefixedLitre ;
  rdfs:label "gram per zettalitre"@en, "gram per zettaliter"@nl ;
  rdfs:comment "Gram per zettalitre is a unit of density defined as gram divided by zettalitre."@en ;
  ns2:symbol "g/Zl" ;
  ns2:alternativeSymbol "g Zl-1", "g·Zl-1" ;
  ns2:hasNumerator ns2:gram ;
  ns2:hasDenominator ns2:zettalitre ;
  ns2:hasDimension ns2:density-Dimension .

ns2:gramPerYottalitre
  a ns2:GramPerPrefixedLitre ;
  rdfs:label "gram per yottalitre"@en, "gram per yottaliter"@nl ;
  rdfs:comment "Gram per yottalitre is a unit of density defined as gram divided by yottalitre."@en ;
  ns2:symbol "g/Yl" ;
  ns2:alternativeSymbol "g Yl-1", "g·Yl-1" ;
  ns2:hasNumerator ns2:gram ;
  ns2:hasDenominator ns2:yottalitre ;
  ns2:hasDimension ns2:density-Dimension .

ns2:cubicMetrePerKilogram
  a ns2:UnitDivision ;
  rdfs:label "cubic metre per kilogram"@en, "kubieke meter per kilogram"@nl ;
  rdfs:comment "Cubic metre per kilogram is a unit of specific volume defined as cubic metre divided by kilogram."@en ;
  ns2:longcomment "Cubic metre per kilogram is a unit of specific volume defined as cubic metre divided by kilogram. Cubic metre per kilogram is a derived unit in the International System of Units." ;
  ns2:symbol "m3/kg" ;
  ns2:alternativeSymbol "m3 kg-1", "m3·kg-1" ;
  ns2:hasNumerator ns2:cubicMetre ;
  ns2:hasDenominator ns2:kilogram ;
  ns2:hasDimension ns2:specificVolume-Dimension .

ns2:SpecificVolumeUnit
  a owl:Class ;
  rdfs:label "specific volume unit"@en ;
  rdfs:subClassOf ns2:Unit ;
  owl:equivalentClass [
    a owl:Class ;
    owl:oneOf (
     ns2:cubicMetrePerKilogram
     ns2:litrePerKilogram
   )
  ] .

ns2:litrePerKilogram
  a ns2:UnitDivision ;
  rdfs:label "litre per kilogram"@en, "liter per kilogram"@nl ;
  rdfs:comment "Litre per kilogram is a unit of specific volume defined as litre divided by kilogram."@en ;
  ns2:longcomment "Litre per kilogram is a unit of specific volume defined as litre divided by kilogram. Litre per kilogram is a derived unit in the International System of Units." ;
  ns2:symbol "l/kg" ;
  ns2:alternativeSymbol "l kg-1", "l·kg-1" ;
  ns2:hasNumerator ns2:litre ;
  ns2:hasDenominator ns2:kilogram ;
  ns2:hasDimension ns2:specificVolume-Dimension .

ns2:metrePerSecond-Time
  a ns2:UnitDivision ;
  rdfs:label "metre per second"@en, "meter per seconde"@nl ;
  rdfs:comment "Metre per second is a unit of speed defined as metre divided by second."@en ;
  ns2:longcomment "Metre per second is a unit of speed defined as metre divided by second. Metre per second is a derived unit in the International System of Units." ;
  ns2:symbol "m/s" ;
  ns2:alternativeSymbol "m s-1", "m·s-1", "mps" ;
  ns2:hasNumerator ns2:metre ;
  ns2:hasDenominator ns2:second-Time ;
  ns2:hasDimension ns2:speed-Dimension .

ns2:SpeedUnit
  a owl:Class ;
  rdfs:label "speed unit"@en ;
  rdfs:subClassOf ns2:Unit ;
  owl:equivalentClass [
    a owl:Class ;
    owl:unionOf (
     _:genid499
     ns2:PrefixedMetrePerSecond-Time
     ns2:MetrePerPrefixedSecond-Time
     ns2:PrefixedMetrePerPrefixedSecond-Time
   )
  ] .

ns2:knot-International
  a ns2:Unit, ns2:SingularUnit ;
  rdfs:label "knot (international)"@en, "knoop (internationaal)"@nl, "海里/小时（国际）"@zh ;
  ns2:alternativeLabel "international knot"@en ;
  rdfs:comment "The international knot is a unit of speed defined as nautical mile per hour."@en ;
  ns2:hasUnit ns2:nauticalMile-InternationalPerHour ;
  ns2:hasDimension ns2:speed-Dimension .

ns2:millimetrePerHour
  a ns2:UnitDivision ;
  rdfs:label "millimetre per hour"@en, "millimeter per uur"@nl ;
  rdfs:comment "Millimetre per hour is a unit of speed defined as millimetre divided by hour."@en ;
  ns2:symbol "mm/h" ;
  ns2:alternativeSymbol "mm h-1", "mm·h-1" ;
  ns2:hasNumerator ns2:millimetre ;
  ns2:hasDenominator ns2:hour ;
  ns2:hasDimension ns2:speed-Dimension .

ns2:kilometrePerHour
  a ns2:UnitDivision ;
  rdfs:label "kilometre per hour"@en, "kilometer per uur"@nl ;
  rdfs:comment "Kilometre per hour is a unit of speed defined as kilometre divided by hour."@en ;
  ns2:symbol "km/h" ;
  ns2:alternativeSymbol "km h-1", "km·h-1" ;
  ns2:hasNumerator ns2:kilometre ;
  ns2:hasDenominator ns2:hour ;
  ns2:hasDimension ns2:speed-Dimension .

ns2:centimetrePerDay
  a ns2:UnitDivision ;
  rdfs:label "centimetre per day"@en, "centimeter per dag"@nl ;
  rdfs:comment "Centimetre per day is a unit of speed defined as centimetre divided by day."@en ;
  ns2:symbol "cm/d" ;
  ns2:alternativeSymbol "cm d-1", "cm·d-1" ;
  ns2:hasNumerator ns2:centimetre ;
  ns2:hasDenominator ns2:day .

ns2:metrePerDay
  a ns2:UnitDivision ;
  rdfs:label "metre per day"@en, "meter per dag"@nl ;
  rdfs:comment "Metre per day is a unit of speed defined as metre divided by day."@en ;
  ns2:symbol "m/d" ;
  ns2:alternativeSymbol "m d-1", "m·d-1" ;
  ns2:hasNumerator ns2:metre ;
  ns2:hasDenominator ns2:day .

ns2:millimetrePerDay
  a ns2:UnitDivision ;
  rdfs:label "millimetre per day"@en, "millimeter per dag"@nl ;
  rdfs:comment "Millimetre per day is a unit of speed defined as millimetre divided by day."@en ;
  ns2:symbol "mm/d" ;
  ns2:alternativeSymbol "mm d-1", "mm·d-1" ;
  ns2:hasNumerator ns2:millimetre ;
  ns2:hasDenominator ns2:day ;
  ns2:hasDimension ns2:speed-Dimension .

ns2:mile-StatutePerHour
  a ns2:UnitDivision ;
  rdfs:label "mile (statute) per hour"@en, "mijl per uur"@nl ;
  rdfs:comment "Mile (statute) per hour is a unit of speed defined as mile (statute) divided by hour."@en ;
  ns2:symbol "mi/h" ;
  ns2:alternativeSymbol "mi h-1", "mi·h-1" ;
  ns2:hasNumerator ns2:mile-Statute ;
  ns2:hasDenominator ns2:hour ;
  ns2:hasDimension ns2:speed-Dimension .

ns2:nauticalMile-InternationalPerHour
  a ns2:UnitDivision ;
  rdfs:label "nautical mile per hour"@en, "zeemijl per uur"@nl ;
  rdfs:comment "Nautical mile per hour is a unit of speed defined as nautical mile divided by hour."@en ;
  ns2:symbol "nmi/h", "M/h" ;
  ns2:alternativeSymbol "nmi h-1", "nmi·h-1", "M h-1", "M·h-1", "NM/h", "NM h-1", "NM·h-1", "nm/h", "nm h-1", "nm·h-1" ;
  ns2:hasNumerator ns2:nauticalMile-International ;
  ns2:hasDenominator ns2:hour ;
  ns2:hasDimension ns2:speed-Dimension .

ns2:PrefixedMetrePerSecond-Time
  a owl:Class ;
  rdfs:label "prefixed metre per second (time)"@en ;
  rdfs:subClassOf ns2:UnitDivision ;
  owl:equivalentClass [
    a owl:Class ;
    owl:intersectionOf (
     _:genid516
     _:genid518
     _:genid520
     _:genid522
   )
  ] .

ns2:MetrePerPrefixedSecond-Time
  a owl:Class ;
  rdfs:label "metre per prefixed second (time)"@en ;
  rdfs:subClassOf ns2:UnitDivision ;
  owl:equivalentClass [
    a owl:Class ;
    owl:intersectionOf (
     _:genid525
     _:genid527
     _:genid529
     _:genid531
   )
  ] .

ns2:PrefixedMetrePerPrefixedSecond-Time
  a owl:Class ;
  rdfs:label "prefixed metre per prefixed second (time)"@en ;
  rdfs:subClassOf ns2:UnitDivision ;
  owl:equivalentClass [
    a owl:Class ;
    owl:intersectionOf (
     _:genid534
     _:genid536
     _:genid538
     _:genid540
   )
  ] .

ns2:yoctometrePerSecond-Time
  a ns2:PrefixedMetrePerSecond-Time ;
  rdfs:label "yoctometre per second"@en, "yoctometer per seconde"@nl ;
  rdfs:comment "Yoctometre per second is a unit of speed defined as yoctometre divided by second."@en ;
  ns2:symbol "ym/s" ;
  ns2:alternativeSymbol "ym s-1", "ym·s-1" ;
  ns2:hasNumerator ns2:yoctometre ;
  ns2:hasDenominator ns2:second-Time ;
  ns2:hasDimension ns2:speed-Dimension .

ns2:zeptometrePerSecond-Time
  a ns2:PrefixedMetrePerSecond-Time ;
  rdfs:label "zeptometre per second"@en, "zeptometer per seconde"@nl ;
  rdfs:comment "Zeptometre per second is a unit of speed defined as zeptometre divided by second."@en ;
  ns2:symbol "zm/s" ;
  ns2:alternativeSymbol "zm s-1", "zm·s-1" ;
  ns2:hasNumerator ns2:zeptometre ;
  ns2:hasDenominator ns2:second-Time ;
  ns2:hasDimension ns2:speed-Dimension .

ns2:attometrePerSecond-Time
  a ns2:PrefixedMetrePerSecond-Time ;
  rdfs:label "attometre per second"@en, "attometer per seconde"@nl ;
  rdfs:comment "Attometre per second is a unit of speed defined as attometre divided by second."@en ;
  ns2:symbol "am/s" ;
  ns2:alternativeSymbol "am s-1", "am·s-1" ;
  ns2:hasNumerator ns2:attometre ;
  ns2:hasDenominator ns2:second-Time ;
  ns2:hasDimension ns2:speed-Dimension .

ns2:femtometrePerSecond-Time
  a ns2:PrefixedMetrePerSecond-Time ;
  rdfs:label "femtometre per second"@en, "femtometer per seconde"@nl ;
  rdfs:comment "Femtometre per second is a unit of speed defined as femtometre divided by second."@en ;
  ns2:symbol "fm/s" ;
  ns2:alternativeSymbol "fm s-1", "fm·s-1" ;
  ns2:hasNumerator ns2:femtometre ;
  ns2:hasDenominator ns2:second-Time ;
  ns2:hasDimension ns2:speed-Dimension .

ns2:picometrePerSecond-Time
  a ns2:PrefixedMetrePerSecond-Time ;
  rdfs:label "picometre per second"@en, "picometer per seconde"@nl ;
  rdfs:comment "Picometre per second is a unit of speed defined as picometre divided by second."@en ;
  ns2:symbol "pm/s" ;
  ns2:alternativeSymbol "pm·s-1", "pm s-1" ;
  ns2:hasNumerator ns2:picometre ;
  ns2:hasDenominator ns2:second-Time ;
  ns2:hasDimension ns2:speed-Dimension .

ns2:nanometrePerSecond-Time
  a ns2:PrefixedMetrePerSecond-Time ;
  rdfs:label "nanometre per second"@en, "nanometer per seconde"@nl ;
  rdfs:comment "Nanometre per second is a unit of speed defined as nanometre divided by second."@en ;
  ns2:symbol "nm/s" ;
  ns2:alternativeSymbol "nm s-1", "nm·s-1" ;
  ns2:hasNumerator ns2:nanometre ;
  ns2:hasDenominator ns2:second-Time ;
  ns2:hasDimension ns2:speed-Dimension .

ns2:micrometrePerSecond-Time
  a ns2:PrefixedMetrePerSecond-Time ;
  rdfs:label "micrometre per second"@en, "micrometer per seconde"@nl ;
  rdfs:comment "Micrometre per second is a unit of speed defined as micrometre divided by second."@en ;
  ns2:symbol "μm/s" ;
  ns2:alternativeSymbol "μm·s-1", "μm s-1" ;
  ns2:hasNumerator ns2:micrometre ;
  ns2:hasDenominator ns2:second-Time ;
  ns2:hasDimension ns2:speed-Dimension .

ns2:millimetrePerSecond-Time
  a ns2:PrefixedMetrePerSecond-Time ;
  rdfs:label "millimetre per second"@en, "millimeter per seconde"@nl ;
  rdfs:comment "Millimetre per second is a unit of speed defined as millimetre divided by second."@en ;
  ns2:symbol "mm/s" ;
  ns2:alternativeSymbol "mm s-1", "mm·s-1" ;
  ns2:hasNumerator ns2:millimetre ;
  ns2:hasDenominator ns2:second-Time ;
  ns2:hasDimension ns2:speed-Dimension .

ns2:centimetrePerSecond-Time
  a ns2:PrefixedMetrePerSecond-Time ;
  rdfs:label "centimetre per second"@en, "centimeter per seconde"@nl ;
  rdfs:comment "Centimetre per second is a unit of speed defined as centimetre divided by second."@en ;
  ns2:symbol "cm/s" ;
  ns2:alternativeSymbol "cm s-1", "cm·s-1" ;
  ns2:hasNumerator ns2:centimetre ;
  ns2:hasDenominator ns2:second-Time ;
  ns2:hasDimension ns2:speed-Dimension .

ns2:decimetrePerSecond-Time
  a ns2:PrefixedMetrePerSecond-Time ;
  rdfs:label "decimetre per second"@en, "decimeter per seconde"@nl ;
  rdfs:comment "Decimetre per second is a unit of speed defined as decimetre divided by second."@en ;
  ns2:symbol "dm/s" ;
  ns2:alternativeSymbol "dm s-1", "dm·s-1" ;
  ns2:hasNumerator ns2:decimetre ;
  ns2:hasDenominator ns2:second-Time ;
  ns2:hasDimension ns2:speed-Dimension .

ns2:decametrePerSecond-Time
  a ns2:PrefixedMetrePerSecond-Time ;
  rdfs:label "decametre per second"@en, "decameter per seconde"@nl ;
  rdfs:comment "Decametre per second is a unit of speed defined as decametre divided by second."@en ;
  ns2:symbol "dam/s" ;
  ns2:alternativeSymbol "dam s-1", "dam·s-1" ;
  ns2:hasNumerator ns2:decametre ;
  ns2:hasDenominator ns2:second-Time ;
  ns2:hasDimension ns2:speed-Dimension .

ns2:hectometrePerSecond-Time
  a ns2:PrefixedMetrePerSecond-Time ;
  rdfs:label "hectometre per second"@en, "hectometer per seconde"@nl ;
  rdfs:comment "Hectometre per second is a unit of speed defined as hectometre divided by second."@en ;
  ns2:symbol "hm/s" ;
  ns2:alternativeSymbol "hm s-1", "hm·s-1" ;
  ns2:hasNumerator ns2:hectometre ;
  ns2:hasDenominator ns2:second-Time ;
  ns2:hasDimension ns2:speed-Dimension .

ns2:kilometrePerSecond-Time
  a ns2:PrefixedMetrePerSecond-Time ;
  rdfs:label "kilometre per second"@en, "kilometer per seconde"@nl ;
  rdfs:comment "Kilometre per second is a unit of speed defined as kilometre divided by second."@en ;
  ns2:symbol "km/s" ;
  ns2:alternativeSymbol "km s-1", "km·s-1" ;
  ns2:hasNumerator ns2:kilometre ;
  ns2:hasDenominator ns2:second-Time ;
  ns2:hasDimension ns2:speed-Dimension .

ns2:megametrePerSecond-Time
  a ns2:PrefixedMetrePerSecond-Time ;
  rdfs:label "megametre per second"@en, "megameter per seconde"@nl ;
  rdfs:comment "Megametre per second is a unit of speed defined as megametre divided by second."@en ;
  ns2:symbol "Mm/s" ;
  ns2:alternativeSymbol "Mm s-1", "Mm·s-1" ;
  ns2:hasNumerator ns2:megametre ;
  ns2:hasDenominator ns2:second-Time ;
  ns2:hasDimension ns2:speed-Dimension .

ns2:gigametrePerSecond-Time
  a ns2:PrefixedMetrePerSecond-Time ;
  rdfs:label "gigametre per second"@en, "gigameter per seconde"@nl ;
  rdfs:comment "Gigametre per second is a unit of speed defined as gigametre divided by second."@en ;
  ns2:symbol "Gm/s" ;
  ns2:alternativeSymbol "Gm s-1", "Gm·s-1" ;
  ns2:hasNumerator ns2:gigametre ;
  ns2:hasDenominator ns2:second-Time ;
  ns2:hasDimension ns2:speed-Dimension .

ns2:terametrePerSecond-Time
  a ns2:PrefixedMetrePerSecond-Time ;
  rdfs:label "terametre per second"@en, "terameter per seconde"@nl ;
  rdfs:comment "Terametre per second is a unit of speed defined as terametre divided by second."@en ;
  ns2:symbol "Tm/s" ;
  ns2:alternativeSymbol "Tm s-1", "Tm·s-1" ;
  ns2:hasNumerator ns2:terametre ;
  ns2:hasDenominator ns2:second-Time ;
  ns2:hasDimension ns2:speed-Dimension .

ns2:petametrePerSecond-Time
  a ns2:PrefixedMetrePerSecond-Time ;
  rdfs:label "petametre per second"@en, "petameter per seconde"@nl ;
  rdfs:comment "Petametre per second is a unit of speed defined as petametre divided by second."@en ;
  ns2:symbol "Pm/s" ;
  ns2:alternativeSymbol "Pm s-1", "Pm·s-1" ;
  ns2:hasNumerator ns2:petametre ;
  ns2:hasDenominator ns2:second-Time ;
  ns2:hasDimension ns2:speed-Dimension .

ns2:exametrePerSecond-Time
  a ns2:PrefixedMetrePerSecond-Time ;
  rdfs:label "exametre per second"@en, "exameter per seconde"@nl ;
  rdfs:comment "Exametre per second is a unit of speed defined as exametre divided by second."@en ;
  ns2:symbol "Em/s" ;
  ns2:alternativeSymbol "Em s-1", "Em·s-1" ;
  ns2:hasNumerator ns2:exametre ;
  ns2:hasDenominator ns2:second-Time ;
  ns2:hasDimension ns2:speed-Dimension .

ns2:zettametrePerSecond-Time
  a ns2:PrefixedMetrePerSecond-Time ;
  rdfs:label "zettametre per second"@en, "zettameter per seconde"@nl ;
  rdfs:comment "Zettametre per second is a unit of speed defined as zettametre divided by second."@en ;
  ns2:symbol "Zm/s" ;
  ns2:alternativeSymbol "Zm s-1", "Zm·s-1" ;
  ns2:hasNumerator ns2:zettametre ;
  ns2:hasDenominator ns2:second-Time ;
  ns2:hasDimension ns2:speed-Dimension .

ns2:yottametrePerSecond-Time
  a ns2:PrefixedMetrePerSecond-Time ;
  rdfs:label "yottametre per second"@en, "yottameter per seconde"@nl ;
  rdfs:comment "Yottametre per second is a unit of speed defined as yottametre divided by second."@en ;
  ns2:symbol "Ym/s" ;
  ns2:alternativeSymbol "Ym s-1", "Ym·s-1" ;
  ns2:hasNumerator ns2:yottametre ;
  ns2:hasDenominator ns2:second-Time ;
  ns2:hasDimension ns2:speed-Dimension .

ns2:metrePerYoctosecond-Time
  a ns2:MetrePerPrefixedSecond-Time ;
  rdfs:label "metre per yoctosecond"@en, "meter per yoctoseconde"@nl ;
  rdfs:comment "Metre per yoctosecond is a unit of speed defined as metre divided by yoctosecond."@en ;
  ns2:symbol "m/ys" ;
  ns2:alternativeSymbol "m ys-1", "m·ys-1" ;
  ns2:hasNumerator ns2:metre ;
  ns2:hasDenominator ns2:yoctosecond-Time ;
  ns2:hasDimension ns2:speed-Dimension .

ns2:metrePerZeptosecond-Time
  a ns2:MetrePerPrefixedSecond-Time ;
  rdfs:label "metre per zeptosecond"@en, "meter per zeptoseconde"@nl ;
  rdfs:comment "Metre per zeptosecond is a unit of speed defined as metre divided by zeptosecond."@en ;
  ns2:symbol "m/zs" ;
  ns2:alternativeSymbol "m zs-1", "m·zs-1" ;
  ns2:hasNumerator ns2:metre ;
  ns2:hasDenominator ns2:zeptosecond-Time ;
  ns2:hasDimension ns2:speed-Dimension .

ns2:metrePerAttosecond-Time
  a ns2:MetrePerPrefixedSecond-Time ;
  rdfs:label "metre per attosecond"@en, "meter per attoseconde"@nl ;
  rdfs:comment "Metre per attosecond is a unit of speed defined as metre divided by attosecond."@en ;
  ns2:symbol "m/as" ;
  ns2:alternativeSymbol "m as-1", "m·as-1" ;
  ns2:hasNumerator ns2:metre ;
  ns2:hasDenominator ns2:attosecond-Time ;
  ns2:hasDimension ns2:speed-Dimension .

ns2:metrePerFemtosecond-Time
  a ns2:MetrePerPrefixedSecond-Time ;
  rdfs:label "metre per femtosecond"@en, "meter per femtoseconde"@nl ;
  rdfs:comment "Metre per femtosecond is a unit of speed defined as metre divided by femtosecond."@en ;
  ns2:symbol "m/fs" ;
  ns2:alternativeSymbol "m fs-1", "m·fs-1" ;
  ns2:hasNumerator ns2:metre ;
  ns2:hasDenominator ns2:femtosecond-Time ;
  ns2:hasDimension ns2:speed-Dimension .

ns2:metrePerPicosecond-Time
  a ns2:MetrePerPrefixedSecond-Time ;
  rdfs:label "metre per picosecond"@en, "meter per picoseconde"@nl ;
  rdfs:comment "Metre per picosecond is a unit of speed defined as metre divided by picosecond."@en ;
  ns2:symbol "m/ps" ;
  ns2:alternativeSymbol "m ps-1", "m·ps-1" ;
  ns2:hasNumerator ns2:metre ;
  ns2:hasDenominator ns2:picosecond-Time ;
  ns2:hasDimension ns2:speed-Dimension .

ns2:metrePerNanosecond-Time
  a ns2:MetrePerPrefixedSecond-Time ;
  rdfs:label "metre per nanosecond"@en, "meter per nanoseconde"@nl ;
  rdfs:comment "Metre per nanosecond is a unit of speed defined as metre divided by nanosecond."@en ;
  ns2:symbol "m/ns" ;
  ns2:alternativeSymbol "m ns-1", "m·ns-1" ;
  ns2:hasNumerator ns2:metre ;
  ns2:hasDenominator ns2:nanosecond-Time ;
  ns2:hasDimension ns2:speed-Dimension .

ns2:metrePerMicrosecond-Time
  a ns2:MetrePerPrefixedSecond-Time ;
  rdfs:label "metre per microsecond"@en, "meter per microseconde"@nl ;
  rdfs:comment "Metre per microsecond is a unit of speed defined as metre divided by microsecond."@en ;
  ns2:symbol "m/μs" ;
  ns2:alternativeSymbol "m μs-1", "m·μs-1" ;
  ns2:hasNumerator ns2:metre ;
  ns2:hasDenominator ns2:microsecond-Time ;
  ns2:hasDimension ns2:speed-Dimension .

ns2:metrePerMillisecond-Time
  a ns2:MetrePerPrefixedSecond-Time ;
  rdfs:label "metre per millisecond"@en, "meter per milliseconde"@nl ;
  rdfs:comment "Metre per millisecond is a unit of speed defined as metre divided by millisecond."@en ;
  ns2:symbol "m/ms" ;
  ns2:alternativeSymbol "m ms-1", "m·ms-1" ;
  ns2:hasNumerator ns2:metre ;
  ns2:hasDenominator ns2:millisecond-Time ;
  ns2:hasDimension ns2:speed-Dimension .

ns2:metrePerCentisecond-Time
  a ns2:MetrePerPrefixedSecond-Time ;
  rdfs:label "metre per centisecond"@en, "meter per centiseconde"@nl ;
  rdfs:comment "Metre per centisecond is a unit of speed defined as metre divided by centisecond."@en ;
  ns2:symbol "m/cs" ;
  ns2:alternativeSymbol "m cs-1", "m·cs-1" ;
  ns2:hasNumerator ns2:metre ;
  ns2:hasDenominator ns2:centisecond-Time ;
  ns2:hasDimension ns2:speed-Dimension .

ns2:metrePerDecisecond-Time
  a ns2:MetrePerPrefixedSecond-Time ;
  rdfs:label "metre per decisecond"@en, "meter per deciseconde"@nl ;
  rdfs:comment "Metre per decisecond is a unit of speed defined as metre divided by decisecond."@en ;
  ns2:symbol "m/ds" ;
  ns2:alternativeSymbol "m ds-1", "m·ds-1" ;
  ns2:hasNumerator ns2:metre ;
  ns2:hasDenominator ns2:decisecond-Time ;
  ns2:hasDimension ns2:speed-Dimension .

ns2:metrePerDecasecond-Time
  a ns2:MetrePerPrefixedSecond-Time ;
  rdfs:label "metre per decasecond"@en, "meter per decaseconde"@nl ;
  rdfs:comment "Metre per decasecond is a unit of speed defined as metre divided by decasecond."@en ;
  ns2:symbol "m/das" ;
  ns2:alternativeSymbol "m das-1", "m·das-1" ;
  ns2:hasNumerator ns2:metre ;
  ns2:hasDenominator ns2:decasecond-Time ;
  ns2:hasDimension ns2:speed-Dimension .

ns2:metrePerHectosecond-Time
  a ns2:MetrePerPrefixedSecond-Time ;
  rdfs:label "metre per hectosecond"@en, "meter per hectoseconde"@nl ;
  rdfs:comment "Metre per hectosecond is a unit of speed defined as metre divided by hectosecond."@en ;
  ns2:symbol "m/hs" ;
  ns2:alternativeSymbol "m hs-1", "m·hs-1" ;
  ns2:hasNumerator ns2:metre ;
  ns2:hasDenominator ns2:hectosecond-Time ;
  ns2:hasDimension ns2:speed-Dimension .

ns2:metrePerKilosecond-Time
  a ns2:MetrePerPrefixedSecond-Time ;
  rdfs:label "metre per kilosecond"@en, "meter per kiloseconde"@nl ;
  rdfs:comment "Metre per kilosecond is a unit of speed defined as metre divided by kilosecond."@en ;
  ns2:symbol "m/ks" ;
  ns2:alternativeSymbol "m ks-1", "m·ks-1" ;
  ns2:hasNumerator ns2:metre ;
  ns2:hasDenominator ns2:kilosecond-Time ;
  ns2:hasDimension ns2:speed-Dimension .

ns2:metrePerMegasecond-Time
  a ns2:MetrePerPrefixedSecond-Time ;
  rdfs:label "metre per megasecond"@en, "meter per megaseconde"@nl ;
  rdfs:comment "Metre per megasecond is a unit of speed defined as metre divided by megasecond."@en ;
  ns2:symbol "m/Ms" ;
  ns2:alternativeSymbol "m Ms-1", "m·Ms-1" ;
  ns2:hasNumerator ns2:metre ;
  ns2:hasDenominator ns2:megasecond-Time ;
  ns2:hasDimension ns2:speed-Dimension .

ns2:metrePerGigasecond-Time
  a ns2:MetrePerPrefixedSecond-Time ;
  rdfs:label "metre per gigasecond"@en, "meter per gigaseconde"@nl ;
  rdfs:comment "Metre per gigasecond is a unit of speed defined as metre divided by gigasecond."@en ;
  ns2:symbol "m/Gs" ;
  ns2:alternativeSymbol "m Gs-1", "m·Gs-1" ;
  ns2:hasNumerator ns2:metre ;
  ns2:hasDenominator ns2:gigasecond-Time ;
  ns2:hasDimension ns2:speed-Dimension .

ns2:metrePerTerasecond-Time
  a ns2:MetrePerPrefixedSecond-Time ;
  rdfs:label "metre per terasecond"@en, "meter per teraseconde"@nl ;
  rdfs:comment "Metre per terasecond is a unit of speed defined as metre divided by terasecond."@en ;
  ns2:symbol "m/Ts" ;
  ns2:alternativeSymbol "m Ts-1", "m·Ts-1" ;
  ns2:hasNumerator ns2:metre ;
  ns2:hasDenominator ns2:terasecond-Time ;
  ns2:hasDimension ns2:speed-Dimension .

ns2:metrePerPetasecond-Time
  a ns2:MetrePerPrefixedSecond-Time ;
  rdfs:label "metre per petasecond"@en, "meter per petaseconde"@nl ;
  rdfs:comment "Metre per petasecond is a unit of speed defined as metre divided by petasecond."@en ;
  ns2:symbol "m/Ps" ;
  ns2:alternativeSymbol "m Ps-1", "m·Ps-1" ;
  ns2:hasNumerator ns2:metre ;
  ns2:hasDenominator ns2:petasecond-Time ;
  ns2:hasDimension ns2:speed-Dimension .

ns2:metrePerExasecond-Time
  a ns2:MetrePerPrefixedSecond-Time ;
  rdfs:label "metre per exasecond"@en, "meter per exaseconde"@nl ;
  rdfs:comment "Metre per exasecond is a unit of speed defined as metre divided by exasecond."@en ;
  ns2:symbol "m/Es" ;
  ns2:alternativeSymbol "m Es-1", "m·Es-1" ;
  ns2:hasNumerator ns2:metre ;
  ns2:hasDenominator ns2:exasecond-Time ;
  ns2:hasDimension ns2:speed-Dimension .

ns2:metrePerZettasecond-Time
  a ns2:MetrePerPrefixedSecond-Time ;
  rdfs:label "metre per zettasecond"@en, "meter per zettaseconde"@nl ;
  rdfs:comment "Metre per zettasecond is a unit of speed defined as metre divided by zettasecond."@en ;
  ns2:symbol "m/Zs" ;
  ns2:alternativeSymbol "m Zs-1", "m·Zs-1" ;
  ns2:hasNumerator ns2:metre ;
  ns2:hasDenominator ns2:zettasecond-Time ;
  ns2:hasDimension ns2:speed-Dimension .

ns2:metrePerYottasecond-Time
  a ns2:MetrePerPrefixedSecond-Time ;
  rdfs:label "metre per yottasecond"@en, "meter per yottaseconde"@nl ;
  rdfs:comment "Metre per yottasecond is a unit of speed defined as metre divided by yottasecond."@en ;
  ns2:symbol "m/Ys" ;
  ns2:alternativeSymbol "m Ys-1", "m·Ys-1" ;
  ns2:hasNumerator ns2:metre ;
  ns2:hasDenominator ns2:yottasecond-Time ;
  ns2:hasDimension ns2:speed-Dimension .

ns2:metreKilogramPerSecond-TimeSquared
  a ns2:UnitDivision ;
  rdfs:label "metre kilogram per second squared"@en, "meter kilogram per seconde kwadraat"@nl ;
  ns2:symbol "m kg/s2" ;
  ns2:alternativeSymbol "m·kg/s2", "m kg s-2", "m·kg·s-2" ;
  ns2:hasNumerator ns2:metreKilogram ;
  ns2:hasDenominator ns2:second-TimeSquared ;
  ns2:hasDimension ns2:force-Dimension .

ns2:ForceUnit
  a owl:Class ;
  rdfs:label "force unit"@en ;
  rdfs:subClassOf ns2:Unit ;
  owl:equivalentClass [
    a owl:Class ;
    owl:unionOf (
     _:genid543
     ns2:PrefixedNewton
   )
  ] .

ns2:dyne
  a ns2:Unit, ns2:SingularUnit ;
  rdfs:label "dyne"@en, "dyne"@nl, "达因"@zh ;
  rdfs:comment "The dyne is a unit of force defined as 1.0e-5 newton."@en ;
  ns2:symbol "dyn" ;
  ns2:hasFactor "1.0e-5"^^xsd:float ;
  ns2:hasUnit ns2:newton ;
  ns2:hasDimension ns2:force-Dimension .

ns2:kip
  a ns2:Unit, ns2:SingularUnit ;
  rdfs:label "kip"@en, "kip"@nl ;
  rdfs:comment "The kip is a unit of force defined as 4.448222e3 newton."@en ;
  ns2:hasFactor "4.448222e3"^^xsd:float ;
  ns2:hasUnit ns2:newton ;
  ns2:hasDimension ns2:force-Dimension .

ns2:newton
  a ns2:Unit, ns2:SingularUnit ;
  rdfs:label "newton"@en, "newton"@nl, "牛顿"@zh ;
  rdfs:comment "The newton is a unit of force defined as kilogram timesmetre divided by second squared."@en ;
  ns2:longcomment "The newton is a unit of force defined as kilogram times metre divided by second squared. The newton is a derived unit in the International System of Units." ;
  ns2:symbol "N" ;
  ns2:hasUnit ns2:metreKilogramPerSecond-TimeSquared ;
  ns2:hasDimension ns2:force-Dimension .

ns2:poundal
  a ns2:Unit, ns2:SingularUnit ;
  rdfs:label "poundal"@en ;
  rdfs:comment "The poundal is a unit of force defined as 1.382550e-1 newton."@en ;
  ns2:hasFactor "1.382550e-1"^^xsd:float ;
  ns2:hasUnit ns2:newton ;
  ns2:hasDimension ns2:force-Dimension .

ns2:pound-Force
  a ns2:Unit, ns2:SingularUnit ;
  rdfs:label "pound-force"@en ;
  rdfs:comment "The pound-force is a unit of force defined as 4.448222 newton."@en ;
  ns2:symbol "lbf" ;
  ns2:hasFactor "4.448222"^^xsd:float ;
  ns2:hasUnit ns2:newton ;
  ns2:hasDimension ns2:force-Dimension .

ns2:ton-Force-Short
  a ns2:Unit, ns2:SingularUnit ;
  rdfs:label "ton-force (short)"@en ;
  ns2:alternativeLabel "short ton-force"@en ;
  rdfs:comment "The short ton-force is a unit of force defined as 8.896443e3 newton."@en ;
  ns2:hasFactor "8.896443e3"^^xsd:float ;
  ns2:hasUnit ns2:newton ;
  ns2:hasDimension ns2:force-Dimension .

ns2:PrefixedNewton
  a owl:Class ;
  rdfs:label "prefixed newton"@en ;
  rdfs:subClassOf ns2:PrefixedUnit ;
  owl:equivalentClass [
    a owl:Class ;
    owl:intersectionOf (
     _:genid556
     _:genid558
     _:genid560
     _:genid562
   )
  ] .

ns2:yoctonewton
  a ns2:PrefixedUnit ;
  rdfs:label "yoctonewton"@en, "yoctonewton"@nl ;
  ns2:symbol "yN" ;
  ns2:hasPrefix ns2:yocto ;
  ns2:hasUnit ns2:newton ;
  ns2:hasDimension ns2:force-Dimension .

ns2:zeptonewton
  a ns2:PrefixedUnit ;
  rdfs:label "zeptonewton"@en, "zeptonewton"@nl ;
  ns2:symbol "zN" ;
  ns2:hasPrefix ns2:zepto ;
  ns2:hasUnit ns2:newton ;
  ns2:hasDimension ns2:force-Dimension .

ns2:attonewton
  a ns2:PrefixedUnit ;
  rdfs:label "attonewton"@en, "attonewton"@nl ;
  ns2:symbol "aN" ;
  ns2:hasPrefix ns2:atto ;
  ns2:hasUnit ns2:newton ;
  ns2:hasDimension ns2:force-Dimension .

ns2:femtonewton
  a ns2:PrefixedUnit ;
  rdfs:label "femtonewton"@en, "femtonewton"@nl ;
  ns2:symbol "fN" ;
  ns2:hasPrefix ns2:femto ;
  ns2:hasUnit ns2:newton ;
  ns2:hasDimension ns2:force-Dimension .

ns2:piconewton
  a ns2:PrefixedUnit ;
  rdfs:label "piconewton"@en, "piconewton"@nl ;
  ns2:symbol "pN" ;
  ns2:hasPrefix ns2:pico ;
  ns2:hasUnit ns2:newton ;
  ns2:hasDimension ns2:force-Dimension .

ns2:nanonewton
  a ns2:PrefixedUnit ;
  rdfs:label "nanonewton"@en, "nanonewton"@nl ;
  ns2:symbol "nN" ;
  ns2:hasPrefix ns2:nano ;
  ns2:hasUnit ns2:newton ;
  ns2:hasDimension ns2:force-Dimension .

ns2:micronewton
  a ns2:PrefixedUnit ;
  rdfs:label "micronewton"@en, "micronewton"@nl ;
  ns2:symbol "μN" ;
  ns2:hasPrefix ns2:micro ;
  ns2:hasUnit ns2:newton ;
  ns2:hasDimension ns2:force-Dimension .

ns2:millinewton
  a ns2:PrefixedUnit ;
  rdfs:label "millinewton"@en, "millinewton"@nl ;
  ns2:symbol "mN" ;
  ns2:hasPrefix ns2:milli ;
  ns2:hasUnit ns2:newton ;
  ns2:hasDimension ns2:force-Dimension .

ns2:centinewton
  a ns2:PrefixedUnit ;
  rdfs:label "centinewton"@en, "centinewton"@nl ;
  ns2:symbol "cN" ;
  ns2:hasPrefix ns2:centi ;
  ns2:hasUnit ns2:newton ;
  ns2:hasDimension ns2:force-Dimension .

ns2:decinewton
  a ns2:PrefixedUnit ;
  rdfs:label "decinewton"@en, "decinewton"@nl ;
  ns2:symbol "dN" ;
  ns2:hasPrefix ns2:deci ;
  ns2:hasUnit ns2:newton ;
  ns2:hasDimension ns2:force-Dimension .

ns2:decanewton
  a ns2:PrefixedUnit ;
  rdfs:label "decanewton"@en, "decanewton"@nl ;
  ns2:symbol "daN" ;
  ns2:hasPrefix ns2:deca ;
  ns2:hasUnit ns2:newton ;
  ns2:hasDimension ns2:force-Dimension .

ns2:hectonewton
  a ns2:PrefixedUnit ;
  rdfs:label "hectonewton"@en, "hectonewton"@nl ;
  ns2:symbol "hN" ;
  ns2:hasPrefix ns2:hecto ;
  ns2:hasUnit ns2:newton ;
  ns2:hasDimension ns2:force-Dimension .

ns2:kilonewton
  a ns2:PrefixedUnit ;
  rdfs:label "kilonewton"@en, "kilonewton"@nl ;
  ns2:symbol "kN" ;
  ns2:hasPrefix ns2:kilo ;
  ns2:hasUnit ns2:newton ;
  ns2:hasDimension ns2:force-Dimension .

ns2:meganewton
  a ns2:PrefixedUnit ;
  rdfs:label "meganewton"@en, "meganewton"@nl ;
  ns2:symbol "MN" ;
  ns2:hasPrefix ns2:mega ;
  ns2:hasUnit ns2:newton ;
  ns2:hasDimension ns2:force-Dimension .

ns2:giganewton
  a ns2:PrefixedUnit ;
  rdfs:label "giganewton"@en, "giganewton"@nl ;
  ns2:symbol "GN" ;
  ns2:hasPrefix ns2:giga ;
  ns2:hasUnit ns2:newton ;
  ns2:hasDimension ns2:force-Dimension .

ns2:teranewton
  a ns2:PrefixedUnit ;
  rdfs:label "teranewton"@en, "teranewton"@nl ;
  ns2:symbol "TN" ;
  ns2:hasPrefix ns2:tera ;
  ns2:hasUnit ns2:newton ;
  ns2:hasDimension ns2:force-Dimension .

ns2:petanewton
  a ns2:PrefixedUnit ;
  rdfs:label "petanewton"@en, "petanewton"@nl ;
  ns2:symbol "PN" ;
  ns2:hasPrefix ns2:peta ;
  ns2:hasUnit ns2:newton ;
  ns2:hasDimension ns2:force-Dimension .

ns2:exanewton
  a ns2:PrefixedUnit ;
  rdfs:label "exanewton"@en, "exanewton"@nl ;
  ns2:symbol "EN" ;
  ns2:hasPrefix ns2:exa ;
  ns2:hasUnit ns2:newton ;
  ns2:hasDimension ns2:force-Dimension .

ns2:zettanewton
  a ns2:PrefixedUnit ;
  rdfs:label "zettanewton"@en, "zettanewton"@nl ;
  ns2:symbol "ZN" ;
  ns2:hasPrefix ns2:zetta ;
  ns2:hasUnit ns2:newton ;
  ns2:hasDimension ns2:force-Dimension .

ns2:yottanewton
  a ns2:PrefixedUnit ;
  rdfs:label "yottanewton"@en, "yottanewton"@nl ;
  ns2:symbol "YN" ;
  ns2:hasPrefix ns2:yotta ;
  ns2:hasUnit ns2:newton ;
  ns2:hasDimension ns2:force-Dimension .

ns2:newtonPerSquareMetre
  a ns2:UnitDivision ;
  rdfs:label "newton per square metre"@en, "newton per vierkante meter"@nl ;
  ns2:symbol "N/m2" ;
  ns2:alternativeSymbol "N m-2", "N·m-2" ;
  ns2:hasNumerator ns2:newton ;
  ns2:hasDenominator ns2:squareMetre ;
  ns2:hasDimension ns2:pressure-Dimension .

ns2:PressureUnit
  a owl:Class ;
  rdfs:label "pressure unit"@en ;
  rdfs:subClassOf ns2:Unit ;
  owl:equivalentClass [
    a owl:Class ;
    owl:unionOf (
     _:genid565
     ns2:PrefixedPascal
   )
  ] .

ns2:atmosphere-Standard
  a ns2:SingularUnit, ns2:Unit ;
  rdfs:label "atmosphere (standard)"@en, "atmosfeer (standaard)"@nl ;
  ns2:alternativeLabel "standard atmosphere"@en ;
  rdfs:comment "The standard atmosphere is a unit of pressure defined as 1.01325e5 pascal."@en ;
  ns2:symbol "atm" ;
  ns2:hasFactor "1.01325e5"^^xsd:float ;
  ns2:hasUnit ns2:pascal ;
  ns2:hasDimension ns2:pressure-Dimension .

ns2:atmosphere-Technical
  a ns2:SingularUnit, ns2:Unit ;
  rdfs:label "atmosphere (technical)"@en ;
  ns2:alternativeLabel "technical atmosphere"@en ;
  rdfs:comment "The technical atmosphere is a unit of pressure defined as 9.80665e4 pascal."@en ;
  ns2:symbol "at" ;
  ns2:hasFactor "9.80665e4"^^xsd:float ;
  ns2:hasUnit ns2:pascal ;
  ns2:hasDimension ns2:pressure-Dimension .

ns2:bar
  a ns2:SingularUnit, ns2:Unit ;
  rdfs:label "bar"@en, "bar"@nl, "巴（压力计量单位）"@zh ;
  rdfs:comment "The bar is a unit of pressure defined as 100 000 pascal."@en ;
  ns2:LaTeXCommand "\\barUnit" ;
  ns2:symbol "bar" ;
  ns2:hasFactor "1.0e5"^^xsd:float ;
  ns2:hasUnit ns2:pascal ;
  ns2:hasDimension ns2:pressure-Dimension .

ns2:barye
  a ns2:SingularUnit, ns2:Unit ;
  rdfs:label "barye"@en, "barye"@nl ;
  rdfs:comment "The barye is a unit of pressure defined as 0.1 pascal."@en ;
  ns2:symbol "ba" ;
  ns2:hasFactor "1.0e-1"^^xsd:float ;
  ns2:hasUnit ns2:pascal ;
  ns2:hasDimension ns2:pressure-Dimension .

ns2:metreOfMercury
  a ns2:SingularUnit, ns2:Unit ;
  rdfs:label "metre of mercury"@en, "meter kwik"@nl ;
  rdfs:comment "The metre of mercury is a unit of pressure defined as 133 322 pascal."@en ;
  ns2:symbol "m Hg" ;
  ns2:hasFactor "1.33322e5"^^xsd:float ;
  ns2:hasUnit ns2:pascal ;
  ns2:hasDimension ns2:pressure-Dimension .

ns2:pascal
  a ns2:SingularUnit, ns2:Unit ;
  rdfs:label "pascal"@en, "pascal"@nl ;
  rdfs:comment "The pascal is a unit of pressure and stress defined as newton divided by square metre = joule divided by cubic metre = kilogram divided by metre second squared."@en ;
  ns2:longcomment "The pascal is a unit of pressure and stress defined as newton divided by square metre = joule divided by cubic metre = kilogram divided by metre second squared. The pascal is a derived unit in the International System of Units." ;
  ns2:symbol "Pa" ;
  ns2:hasUnit ns2:newtonPerSquareMetre ;
  ns2:hasDimension ns2:pressure-Dimension .

ns2:torr
  a ns2:SingularUnit, ns2:Unit ;
  rdfs:label "torr"@en, "torr"@nl ;
  rdfs:comment "The torr is a unit of pressure defined as 1.333224e2 pascal."@en ;
  ns2:symbol "Torr" ;
  ns2:hasFactor "1.33322368421053e2"^^xsd:float ;
  ns2:hasUnit ns2:pascal ;
  ns2:hasDimension ns2:pressure-Dimension .

ns2:decibar
  a ns2:PrefixedUnit ;
  rdfs:label "decibar"@en, "decibar"@nl ;
  rdfs:comment "The decibar is a unit of pressure defined as 1.0e-1 bar."@en ;
  ns2:symbol "dbar" ;
  ns2:hasPrefix ns2:deci ;
  ns2:hasUnit ns2:bar ;
  ns2:hasDimension ns2:pressure-Dimension .

ns2:microbar
  a ns2:PrefixedUnit ;
  rdfs:label "microbar"@en, "microbar"@nl, "微巴"@zh ;
  rdfs:comment "The microbar is a unit of pressure defined as 1.0e-6 bar."@en ;
  ns2:symbol "μbar" ;
  ns2:hasPrefix ns2:micro ;
  ns2:hasUnit ns2:bar ;
  ns2:hasDimension ns2:pressure-Dimension .

ns2:millibar
  a ns2:PrefixedUnit ;
  rdfs:label "millibar"@en, "millibar"@nl ;
  rdfs:comment "The millibar is a unit of pressure defined as 1.0e-3 bar."@en ;
  ns2:symbol "mbar" ;
  ns2:hasPrefix ns2:milli ;
  ns2:hasUnit ns2:bar ;
  ns2:hasDimension ns2:pressure-Dimension .

ns2:centimetreOfMercury
  a ns2:PrefixedUnit ;
  rdfs:label "centimetre of mercury"@en, "centimeter kwik"@nl ;
  rdfs:comment "The centimetre of mercury is a unit of pressure defined as 1.0e-2 metre of mercury."@en ;
  ns2:symbol "cm Hg" ;
  ns2:hasPrefix ns2:centi ;
  ns2:hasUnit ns2:metreOfMercury ;
  ns2:hasDimension ns2:pressure-Dimension .

ns2:millimetreOfMercury
  a ns2:PrefixedUnit ;
  rdfs:label "millimetre of mercury"@en, "millimeter kwik"@nl ;
  rdfs:comment "The millimetre of mercury is a unit of pressure defined as 1.0e-3 metre of mercury."@en ;
  ns2:symbol "mm Hg" ;
  ns2:hasPrefix ns2:milli ;
  ns2:hasUnit ns2:metreOfMercury ;
  ns2:hasDimension ns2:pressure-Dimension .

ns2:kilogramSecond-TimeToThePower-2ReciprocalMetre
  a ns2:UnitMultiplication ;
  rdfs:label "reciprocal metre kilogram second to the power -2"@en, "omgekeerde meter kilogram seconde tot de macht -2"@nl ;
  ns2:symbol "m-1 kg s-2" ;
  ns2:alternativeSymbol "m-1·kg·s-2" ;
  ns2:hasTerm1 ns2:kilogramSecond-TimeToThePower-2 ;
  ns2:hasTerm2 ns2:reciprocalMetre ;
  ns2:hasDimension ns2:pressure-Dimension .

ns2:PrefixedPascal
  a owl:Class ;
  rdfs:label "prefixed pascal"@en ;
  rdfs:subClassOf ns2:PrefixedUnit ;
  owl:equivalentClass [
    a owl:Class ;
    owl:intersectionOf (
     _:genid607
     _:genid609
     _:genid611
     _:genid613
   )
  ] .

ns2:StressUnit
  a owl:Class ;
  rdfs:label "stress unit"@en ;
  rdfs:subClassOf ns2:Unit ;
  owl:equivalentClass [
    a owl:Class ;
    owl:unionOf (
     _:genid583
     ns2:PrefixedPascal
   )
  ] .

ns2:Stress
  a owl:Class ;
  rdfs:subClassOf [
    a owl:Restriction ;
    owl:onProperty ns2:hasValue ;
    owl:allValuesFrom [
      a owl:Restriction ;
      owl:onProperty ns2:hasUnit ;
      owl:allValuesFrom ns2:StressUnit
    ]
  ], ns2:Quantity, [
    a owl:Restriction ;
    owl:onProperty ns2:hasDimension ;
    owl:hasValue ns2:pressure-Dimension
  ] ;
  rdfs:label "stress"@en, "mechanische spanning"@nl ;
  rdfs:comment "Stress is a force that produces or tends to produce deformation in a body measured by the force applied per unit area."@en ;
  ns2:symbol "σ" ;
  ns2:commonlyHasUnit ns2:newtonPerSquareMetre, ns2:kilogramSecond-TimeToThePower-2ReciprocalMetre, ns2:pascal, ns2:attopascal, ns2:centipascal, ns2:decapascal, ns2:decipascal, ns2:exapascal, ns2:femtopascal, ns2:gigapascal, ns2:hectopascal, ns2:kilopascal, ns2:megapascal, ns2:micropascal, ns2:millipascal, ns2:nanopascal, ns2:petapascal, ns2:picopascal, ns2:terapascal, ns2:bar, ns2:decibar, ns2:microbar, ns2:millibar, ns2:metreOfMercury, ns2:centimetreOfMercury, ns2:millimetreOfMercury, ns2:atmosphere-Standard, ns2:atmosphere-Technical, ns2:barye, ns2:torr .

ns2:DynamicModulus
  a owl:Class ;
  rdfs:subClassOf [
    a owl:Restriction ;
    owl:onProperty ns2:hasValue ;
    owl:allValuesFrom [
      a owl:Restriction ;
      owl:onProperty ns2:hasUnit ;
      owl:allValuesFrom ns2:StressUnit
    ]
  ], ns2:Quantity, [
    a owl:Restriction ;
    owl:onProperty ns2:hasDimension ;
    owl:hasValue ns2:pressure-Dimension
  ] ;
  rdfs:label "dynamic modulus"@en ;
  ns2:symbol "E" ;
  ns2:commonlyHasUnit ns2:newtonPerSquareMetre, ns2:kilogramSecond-TimeToThePower-2ReciprocalMetre, ns2:pascal, ns2:attopascal, ns2:centipascal, ns2:decapascal, ns2:decipascal, ns2:exapascal, ns2:femtopascal, ns2:gigapascal, ns2:hectopascal, ns2:kilopascal, ns2:megapascal, ns2:micropascal, ns2:millipascal, ns2:nanopascal, ns2:petapascal, ns2:picopascal, ns2:terapascal, ns2:bar, ns2:decibar, ns2:microbar, ns2:millibar, ns2:metreOfMercury, ns2:centimetreOfMercury, ns2:millimetreOfMercury, ns2:atmosphere-Standard, ns2:atmosphere-Technical, ns2:barye, ns2:torr .

ns2:yoctopascal
  a ns2:PrefixedUnit ;
  rdfs:label "yoctopascal"@en, "yoctopascal"@nl ;
  ns2:symbol "yPa" ;
  ns2:hasPrefix ns2:yocto ;
  ns2:hasUnit ns2:pascal ;
  ns2:hasDimension ns2:pressure-Dimension .

ns2:zeptopascal
  a ns2:PrefixedUnit ;
  rdfs:label "zeptopascal"@en, "zeptopascal"@nl ;
  ns2:symbol "zPa" ;
  ns2:hasPrefix ns2:zepto ;
  ns2:hasUnit ns2:pascal ;
  ns2:hasDimension ns2:pressure-Dimension .

ns2:attopascal
  a ns2:PrefixedUnit ;
  rdfs:label "attopascal"@en, "attopascal"@nl ;
  ns2:symbol "aPa" ;
  ns2:hasPrefix ns2:atto ;
  ns2:hasUnit ns2:pascal ;
  ns2:hasDimension ns2:pressure-Dimension .

ns2:femtopascal
  a ns2:PrefixedUnit ;
  rdfs:label "femtopascal"@en, "femtopascal"@nl ;
  ns2:symbol "fPa" ;
  ns2:hasPrefix ns2:femto ;
  ns2:hasUnit ns2:pascal ;
  ns2:hasDimension ns2:pressure-Dimension .

ns2:picopascal
  a ns2:PrefixedUnit ;
  rdfs:label "picopascal"@en, "picopascal"@nl ;
  ns2:symbol "pPa" ;
  ns2:hasPrefix ns2:pico ;
  ns2:hasUnit ns2:pascal ;
  ns2:hasDimension ns2:pressure-Dimension .

ns2:nanopascal
  a ns2:PrefixedUnit ;
  rdfs:label "nanopascal"@en, "nanopascal"@nl ;
  ns2:symbol "nPa" ;
  ns2:hasPrefix ns2:nano ;
  ns2:hasUnit ns2:pascal ;
  ns2:hasDimension ns2:pressure-Dimension .

ns2:micropascal
  a ns2:PrefixedUnit ;
  rdfs:label "micropascal"@en, "micropascal"@nl ;
  ns2:symbol "μPa" ;
  ns2:hasPrefix ns2:micro ;
  ns2:hasUnit ns2:pascal ;
  ns2:hasDimension ns2:pressure-Dimension .

ns2:millipascal
  a ns2:PrefixedUnit ;
  rdfs:label "millipascal"@en, "millipascal"@nl ;
  ns2:symbol "mPa" ;
  ns2:hasPrefix ns2:milli ;
  ns2:hasUnit ns2:pascal ;
  ns2:hasDimension ns2:pressure-Dimension .

ns2:centipascal
  a ns2:PrefixedUnit ;
  rdfs:label "centipascal"@en, "centipascal"@nl ;
  ns2:symbol "cPa" ;
  ns2:hasPrefix ns2:centi ;
  ns2:hasUnit ns2:pascal ;
  ns2:hasDimension ns2:pressure-Dimension .

ns2:decipascal
  a ns2:PrefixedUnit ;
  rdfs:label "decipascal"@en, "decipascal"@nl ;
  ns2:symbol "dPa" ;
  ns2:hasPrefix ns2:deci ;
  ns2:hasUnit ns2:pascal ;
  ns2:hasDimension ns2:pressure-Dimension .

ns2:decapascal
  a ns2:PrefixedUnit ;
  rdfs:label "decapascal"@en, "decapascal"@nl ;
  ns2:symbol "daPa" ;
  ns2:hasPrefix ns2:deca ;
  ns2:hasUnit ns2:pascal ;
  ns2:hasDimension ns2:pressure-Dimension .

ns2:hectopascal
  a ns2:PrefixedUnit ;
  rdfs:label "hectopascal"@en, "hectopascal"@nl ;
  ns2:symbol "hPa" ;
  ns2:hasPrefix ns2:hecto ;
  ns2:hasUnit ns2:pascal ;
  ns2:hasDimension ns2:pressure-Dimension .

ns2:kilopascal
  a ns2:PrefixedUnit ;
  rdfs:label "kilopascal"@en, "kilopascal"@nl ;
  ns2:symbol "kPa" ;
  ns2:hasPrefix ns2:kilo ;
  ns2:hasUnit ns2:pascal ;
  ns2:hasDimension ns2:pressure-Dimension .

ns2:megapascal
  a ns2:PrefixedUnit ;
  rdfs:label "megapascal"@en, "megapascal"@nl ;
  ns2:symbol "MPa" ;
  ns2:hasPrefix ns2:mega ;
  ns2:hasUnit ns2:pascal ;
  ns2:hasDimension ns2:pressure-Dimension .

ns2:gigapascal
  a ns2:PrefixedUnit ;
  rdfs:label "gigapascal"@en, "gigapascal"@nl ;
  ns2:symbol "GPa" ;
  ns2:hasPrefix ns2:giga ;
  ns2:hasUnit ns2:pascal ;
  ns2:hasDimension ns2:pressure-Dimension .

ns2:terapascal
  a ns2:PrefixedUnit ;
  rdfs:label "terapascal"@en, "terapascal"@nl ;
  ns2:symbol "TPa" ;
  ns2:hasPrefix ns2:tera ;
  ns2:hasUnit ns2:pascal ;
  ns2:hasDimension ns2:pressure-Dimension .

ns2:petapascal
  a ns2:PrefixedUnit ;
  rdfs:label "petapascal"@en, "petapascal"@nl ;
  ns2:symbol "PPa" ;
  ns2:hasPrefix ns2:peta ;
  ns2:hasUnit ns2:pascal ;
  ns2:hasDimension ns2:pressure-Dimension .

ns2:exapascal
  a ns2:PrefixedUnit ;
  rdfs:label "exapascal"@en, "exapascal"@nl ;
  ns2:symbol "EPa" ;
  ns2:hasPrefix ns2:exa ;
  ns2:hasUnit ns2:pascal ;
  ns2:hasDimension ns2:pressure-Dimension .

ns2:zettapascal
  a ns2:PrefixedUnit ;
  rdfs:label "zettapascal"@en, "zettapascal"@nl ;
  ns2:symbol "ZPa" ;
  ns2:hasPrefix ns2:zetta ;
  ns2:hasUnit ns2:pascal ;
  ns2:hasDimension ns2:pressure-Dimension .

ns2:yottapascal
  a ns2:PrefixedUnit ;
  rdfs:label "yottapascal"@en, "yottapascal"@nl ;
  ns2:symbol "YPa" ;
  ns2:hasPrefix ns2:yotta ;
  ns2:hasUnit ns2:pascal ;
  ns2:hasDimension ns2:pressure-Dimension .

ns2:TorqueUnit
  a owl:Class ;
  rdfs:label "torque unit"@en ;
  rdfs:subClassOf ns2:Unit ;
  owl:equivalentClass [
    a owl:Class ;
    owl:oneOf (
     ns2:newtonMetre
     ns2:micronewtonMetre
     ns2:millinewtonMetre
   )
  ] .

ns2:newtonMetre
  a ns2:UnitMultiplication ;
  rdfs:label "newton metre"@en, "newton meter"@nl ;
  ns2:symbol "N m" ;
  ns2:alternativeSymbol "N·m" ;
  ns2:hasTerm1 ns2:newton ;
  ns2:hasTerm2 ns2:metre ;
  ns2:hasDimension ns2:energy-Dimension .

ns2:micronewtonMetre
  a ns2:UnitMultiplication ;
  rdfs:label "micronewton metre"@en, "micronewton meter"@nl ;
  ns2:symbol "μN m" ;
  ns2:alternativeSymbol "μN·m" ;
  ns2:hasTerm1 ns2:micronewton ;
  ns2:hasTerm2 ns2:metre ;
  ns2:hasDimension ns2:energy-Dimension .

ns2:millinewtonMetre
  a ns2:UnitMultiplication ;
  rdfs:label "millinewton metre"@en, "millinewton meter"@nl ;
  ns2:symbol "mN m" ;
  ns2:alternativeSymbol "mN·m" ;
  ns2:hasTerm1 ns2:millinewton ;
  ns2:hasTerm2 ns2:metre ;
  ns2:hasDimension ns2:energy-Dimension .

ns2:MomentOfForceUnit
  a owl:Class ;
  rdfs:label "moment of force unit"@en ;
  rdfs:subClassOf ns2:Unit ;
  owl:equivalentClass [
    a owl:Class ;
    owl:oneOf (
     ns2:newtonMetre
     ns2:micronewtonMetre
     ns2:millinewtonMetre
   )
  ] .

ns2:EnergyUnit
  a owl:Class ;
  rdfs:label "energy unit"@en ;
  rdfs:subClassOf ns2:Unit ;
  owl:equivalentClass [
    a owl:Class ;
    owl:unionOf (
     _:genid628
     ns2:PrefixedJoule
     ns2:PrefixedElectronvolt
     ns2:PrefixedCalorie-Mean
   )
  ] .

ns2:BritishThermalUnit-39F
  a ns2:Unit, ns2:SingularUnit ;
  rdfs:label "British thermal unit (39 °F)"@en, "英国热力单位（39°F）"@zh ;
  ns2:alternativeLabel "39 °F British thermal unit"@en ;
  ns2:LaTeXCommand "\\BritishTermalUnitThirtyNineF" ;
  ns2:symbol "Btu" ;
  ns2:hasDimension ns2:energy-Dimension .

ns2:BritishThermalUnit-59F
  a ns2:Unit, ns2:SingularUnit ;
  rdfs:label "British thermal unit (59 °F)"@en, "英国热力单位（59°F）"@zh ;
  ns2:alternativeLabel "59 °F British thermal unit"@en ;
  ns2:LaTeXCommand "\\BritishTermalUnitFiftyNineF" ;
  ns2:symbol "Btu" ;
  ns2:hasDimension ns2:energy-Dimension .

ns2:BritishThermalUnit-60F
  a ns2:Unit, ns2:SingularUnit ;
  rdfs:label "British thermal unit (60 °F)"@en, "英国热力单位（60°F）"@zh ;
  ns2:alternativeLabel "60 °F British thermal unit"@en ;
  ns2:LaTeXCommand "\\BritishTermalUnitSixtyF" ;
  ns2:symbol "Btu" ;
  ns2:hasDimension ns2:energy-Dimension .

ns2:BritishThermalUnit-InternationalTable
  a ns2:Unit, ns2:SingularUnit ;
  rdfs:label "British thermal unit (International Table)"@en, "英国热力单位（国际表）"@zh ;
  ns2:alternativeLabel "International Table British thermal unit"@en ;
  ns2:symbol "Btu_IT" ;
  ns2:LaTeXSymbol "Btu_{IT}" ;
  ns2:hasDimension ns2:energy-Dimension .

ns2:BritishThermalUnit-Mean
  a ns2:Unit, ns2:SingularUnit ;
  rdfs:label "British thermal unit (mean)"@en, "英国热力单位（平均）"@zh ;
  ns2:alternativeLabel "mean British thermal unit"@en ;
  ns2:symbol "Btu" ;
  ns2:hasDimension ns2:energy-Dimension .

ns2:BritishThermalUnit-Thermochemical
  a ns2:Unit, ns2:SingularUnit ;
  rdfs:label "British thermal unit (thermochemical)"@en, "英国热力单位（热力化学）"@zh ;
  ns2:alternativeLabel "thermochemical British thermal unit"@en ;
  ns2:symbol "Btu_th" ;
  ns2:LaTeXSymbol "BTU_{th}" ;
  ns2:hasDimension ns2:energy-Dimension .

ns2:calorie-15C
  a ns2:Unit, ns2:SingularUnit ;
  rdfs:label "calorie (15 °C)"@en, "calorie (15 °C)"@nl ;
  ns2:alternativeLabel "15 °C calorie"@en, "15 °C calorie"@nl ;
  ns2:symbol "cal_15" ;
  ns2:LaTeXSymbol "cal_{15}" ;
  ns2:hasDimension ns2:energy-Dimension .

ns2:calorie-20C
  a ns2:Unit, ns2:SingularUnit ;
  rdfs:label "calorie (20 °C)"@en, "calorie (20 °C)"@nl ;
  ns2:alternativeLabel "20 °C calorie"@en, "20 °C calorie"@nl ;
  ns2:LaTeXCommand "\\calorieTwentyC" ;
  ns2:symbol "cal_20" ;
  ns2:LaTeXSymbol "cal_{20}" ;
  ns2:hasDimension ns2:energy-Dimension .

ns2:calorie-InternationalTable
  a ns2:Unit, ns2:SingularUnit ;
  rdfs:label "calorie (International Table)"@en ;
  ns2:alternativeLabel "calorie (International Steam Table)"@en, "International Table calorie"@en, "International Steam Table calorie"@en ;
  ns2:symbol "cal_IT" ;
  ns2:LaTeXSymbol "cal_{IT}" ;
  ns2:hasDimension ns2:energy-Dimension .

ns2:calorie-Mean
  a ns2:Unit, ns2:SingularUnit ;
  rdfs:label "calorie (mean)"@en ;
  ns2:alternativeLabel "mean calorie"@en ;
  rdfs:comment "The mean calorie is a unit of energy defined as 4.19002 joule."@en ;
  ns2:symbol "cal" ;
  ns2:alternativeSymbol "c" ;
  ns2:hasFactor "4.19002"^^xsd:float ;
  ns2:hasUnit ns2:joule ;
  ns2:hasDimension ns2:energy-Dimension .

ns2:calorie-Thermochemical
  a ns2:Unit, ns2:SingularUnit ;
  rdfs:label "calorie (thermochemical)"@en ;
  ns2:alternativeLabel "thermochemical calorie"@en ;
  ns2:symbol "cal_th" ;
  ns2:LaTeXSymbol "cal_{th}" ;
  ns2:hasDimension ns2:energy-Dimension .

ns2:electronvolt
  a ns2:Unit, ns2:SingularUnit ;
  rdfs:label "electronvolt"@en, "electronvolt"@nl, "电子伏特"@zh ;
  rdfs:comment "The electronvolt is a unit of energy defined as 1.602177e-19 joule."@en ;
  ns2:symbol "eV" ;
  ns2:hasFactor "1.602177e-19"^^xsd:float ;
  ns2:hasUnit ns2:joule ;
  ns2:hasDimension ns2:energy-Dimension .

ns2:erg
  a ns2:Unit, ns2:SingularUnit ;
  rdfs:label "erg"@en, "erg"@nl, "尔格"@zh ;
  rdfs:comment "The erg is a unit of energy defined as 1.0e-7 joule."@en ;
  ns2:symbol "erg" ;
  ns2:hasFactor "1.0e-7"^^xsd:float ;
  ns2:hasUnit ns2:joule ;
  ns2:hasDimension ns2:energy-Dimension .

ns2:footPoundal
  a ns2:Unit, ns2:SingularUnit ;
  rdfs:label "foot poundal"@en ;
  rdfs:comment "The foot poundal is a unit of energy defined as 4.214011e-2 joule."@en ;
  ns2:hasFactor "4.214011e-2"^^xsd:float ;
  ns2:hasUnit ns2:joule ;
  ns2:hasDimension ns2:energy-Dimension .

ns2:joule
  a ns2:Unit, ns2:SingularUnit ;
  rdfs:label "joule"@en, "joule"@nl, "焦耳"@zh ;
  rdfs:comment "The joule is a unit of energy defined as kilogram times square metre divided by second squared."@en ;
  ns2:longcomment "The joule is a unit of energy defined as kilogram times square metre divided by second squared. The joule is a derived unit in the International System of Units." ;
  ns2:symbol "J" ;
  ns2:hasUnit ns2:newtonMetre ;
  ns2:hasDimension ns2:energy-Dimension .

ns2:quad
  a ns2:Unit, ns2:SingularUnit ;
  rdfs:label "quad"@en ;
  rdfs:comment "The quad is a unit of energy defined as 1.0e15 British thermal unit (International Table)."@en ;
  ns2:hasFactor "1.0e15"^^xsd:float ;
  ns2:hasUnit ns2:BritishThermalUnit-InternationalTable ;
  ns2:hasDimension ns2:energy-Dimension ;
  ns2:LaTeXCommand "\\quadUnit" .

ns2:gigaelectronvolt
  a ns2:PrefixedUnit ;
  rdfs:label "gigaelectronvolt"@en, "gigaelectronvolt"@nl ;
  rdfs:comment "The gigaelectronvolt is a unit of energy defined as 1.0e9 electronvolt."@en ;
  ns2:symbol "GeV" ;
  ns2:hasPrefix ns2:giga ;
  ns2:hasUnit ns2:electronvolt ;
  ns2:hasDimension ns2:energy-Dimension .

ns2:kiloelectronvolt
  a ns2:PrefixedUnit ;
  rdfs:label "kiloelectronvolt"@en, "kiloelectronvolt"@nl ;
  rdfs:comment "The kiloelectronvolt is a unit of energy defined as 1.0e3 electronvolt."@en ;
  ns2:symbol "keV" ;
  ns2:hasPrefix ns2:kilo ;
  ns2:hasUnit ns2:electronvolt ;
  ns2:hasDimension ns2:energy-Dimension .

ns2:megaelectronvolt
  a ns2:PrefixedUnit ;
  rdfs:label "megaelectronvolt"@en, "megaelectronvolt"@nl ;
  rdfs:comment "The megaelectronvolt is a unit of energy defined as 1.0e6 electronvolt."@en ;
  ns2:symbol "MeV" ;
  ns2:hasPrefix ns2:mega ;
  ns2:hasUnit ns2:electronvolt ;
  ns2:hasDimension ns2:energy-Dimension .

ns2:wattHour
  a ns2:UnitMultiplication ;
  rdfs:label "watt hour"@en ;
  ns2:alternativeLabel "watt-hour"@en, "watthour"@en ;
  ns2:symbol "W h" ;
  ns2:alternativeSymbol "W·h", "Wh" ;
  ns2:hasTerm1 ns2:watt ;
  ns2:hasTerm2 ns2:hour ;
  ns2:hasDimension ns2:energy-Dimension .

ns2:kilowattHour
  a ns2:UnitMultiplication ;
  rdfs:label "kilowatt hour"@en ;
  ns2:alternativeLabel "kilowatt-hour"@en, "kilowatthour"@en ;
  ns2:symbol "kW h" ;
  ns2:alternativeSymbol "kW·h", "kWh" ;
  ns2:hasTerm1 ns2:kilowatt ;
  ns2:hasTerm2 ns2:hour ;
  ns2:hasDimension ns2:energy-Dimension .

ns2:terawattHour
  a ns2:UnitMultiplication ;
  rdfs:label "terawatt hour"@en ;
  ns2:alternativeLabel "terawatt-hour"@en, "terawatthour"@en ;
  ns2:symbol "TW h" ;
  ns2:alternativeSymbol "TW·h", "TWh" ;
  ns2:hasTerm1 ns2:terawatt ;
  ns2:hasTerm2 ns2:hour ;
  ns2:hasDimension ns2:energy-Dimension .

ns2:therm-EC
  a ns2:Unit, ns2:SingularUnit ;
  rdfs:label "therm (EC)"@en ;
  ns2:alternativeLabel "EC therm"@en ;
  rdfs:comment "The EC therm is a unit of energy defined as 1.05506e8 joule."@en ;
  ns2:hasFactor "1.05506e8"^^xsd:float ;
  ns2:hasUnit ns2:joule ;
  ns2:hasDimension ns2:energy-Dimension .

ns2:therm-US
  a ns2:Unit, ns2:SingularUnit ;
  rdfs:label "therm (US)"@en ;
  ns2:alternativeLabel "US therm"@en ;
  rdfs:comment "The US therm is a unit of energy defined as 1.054804e8 joule."@en ;
  ns2:hasFactor "1.054804e8"^^xsd:float ;
  ns2:hasUnit ns2:joule ;
  ns2:hasDimension ns2:energy-Dimension .

ns2:tonOfTNT
  a ns2:Unit, ns2:SingularUnit ;
  rdfs:label "ton of TNT"@en ;
  rdfs:comment "The ton of TNT is a unit of energy defined as 4.184e9 joule."@en ;
  ns2:hasFactor "4.184e9"^^xsd:float ;
  ns2:hasUnit ns2:joule ;
  ns2:hasDimension ns2:energy-Dimension .

ns2:PrefixedJoule
  a owl:Class ;
  rdfs:label "prefixed joule"@en ;
  rdfs:subClassOf ns2:PrefixedUnit ;
  owl:equivalentClass [
    a owl:Class ;
    owl:intersectionOf (
     _:genid664
     _:genid666
     _:genid668
     _:genid670
   )
  ] .

ns2:PrefixedElectronvolt
  a owl:Class ;
  rdfs:label "prefixed electronvolt"@en ;
  rdfs:subClassOf ns2:PrefixedUnit ;
  owl:equivalentClass [
    a owl:Class ;
    owl:intersectionOf (
     _:genid673
     _:genid675
     _:genid677
     _:genid679
   )
  ] .

ns2:PrefixedCalorie-Mean
  a owl:Class ;
  rdfs:label "prefixed calorie (mean)"@en ;
  rdfs:subClassOf ns2:PrefixedUnit ;
  owl:equivalentClass [
    a owl:Class ;
    owl:intersectionOf (
     _:genid682
     _:genid684
     _:genid686
     _:genid688
   )
  ] .

ns2:yoctojoule
  a ns2:PrefixedUnit ;
  rdfs:label "yoctojoule"@en, "yoctojoule"@nl ;
  rdfs:comment "The yoctojoule is a unit of energy defined as 1.0e-24 joule."@en ;
  ns2:symbol "yJ" ;
  ns2:hasPrefix ns2:yocto ;
  ns2:hasUnit ns2:joule ;
  ns2:hasDimension ns2:energy-Dimension .

ns2:zeptojoule
  a ns2:PrefixedUnit ;
  rdfs:label "zeptojoule"@en, "zeptojoule"@nl ;
  rdfs:comment "The zeptjoule is a unit of energy defined as 1.0e-21 joule."@en ;
  ns2:symbol "zJ" ;
  ns2:hasPrefix ns2:zepto ;
  ns2:hasUnit ns2:joule ;
  ns2:hasDimension ns2:energy-Dimension .

ns2:attojoule
  a ns2:PrefixedUnit ;
  rdfs:label "attojoule"@en, "attojoule"@nl ;
  rdfs:comment "The attojoule is a unit of energy defined as 1.0e-18 joule."@en ;
  ns2:symbol "aJ" ;
  ns2:hasPrefix ns2:atto ;
  ns2:hasUnit ns2:joule ;
  ns2:hasDimension ns2:energy-Dimension .

ns2:femtojoule
  a ns2:PrefixedUnit ;
  rdfs:label "femtojoule"@en, "femtojoule"@nl ;
  rdfs:comment "The femtojoule is a unit of energy defined as 1.0e-15 joule."@en ;
  ns2:symbol "fJ" ;
  ns2:hasPrefix ns2:femto ;
  ns2:hasUnit ns2:joule ;
  ns2:hasDimension ns2:energy-Dimension .

ns2:picojoule
  a ns2:PrefixedUnit ;
  rdfs:label "picojoule"@en, "picojoule"@nl ;
  rdfs:comment "The picojoule is a unit of energy defined as 1.0e-12 joule."@en ;
  ns2:symbol "pJ" ;
  ns2:hasPrefix ns2:pico ;
  ns2:hasUnit ns2:joule ;
  ns2:hasDimension ns2:energy-Dimension .

ns2:nanojoule
  a ns2:PrefixedUnit ;
  rdfs:label "nanojoule"@en, "nanojoule"@nl ;
  rdfs:comment "The nanojoule is a unit of energy defined as 1.0e-9 joule."@en ;
  ns2:symbol "nJ" ;
  ns2:hasPrefix ns2:nano ;
  ns2:hasUnit ns2:joule ;
  ns2:hasDimension ns2:energy-Dimension .

ns2:microjoule
  a ns2:PrefixedUnit ;
  rdfs:label "microjoule"@en, "microjoule"@nl ;
  rdfs:comment "The microjoule is a unit of energy defined as 1.0e-6 joule."@en ;
  ns2:symbol "μJ" ;
  ns2:hasPrefix ns2:micro ;
  ns2:hasUnit ns2:joule ;
  ns2:hasDimension ns2:energy-Dimension .

ns2:millijoule
  a ns2:PrefixedUnit ;
  rdfs:label "millijoule"@en, "millijoule"@nl ;
  rdfs:comment "The millijoule is a unit of energy defined as 1.0e-3 joule."@en ;
  ns2:symbol "mJ" ;
  ns2:hasPrefix ns2:milli ;
  ns2:hasUnit ns2:joule ;
  ns2:hasDimension ns2:energy-Dimension .

ns2:centijoule
  a ns2:PrefixedUnit ;
  rdfs:label "centijoule"@en, "centijoule"@nl ;
  rdfs:comment "The centijoule is a unit of energy defined as 1.0e-2 joule."@en ;
  ns2:symbol "cJ" ;
  ns2:hasPrefix ns2:centi ;
  ns2:hasUnit ns2:joule ;
  ns2:hasDimension ns2:energy-Dimension .

ns2:decijoule
  a ns2:PrefixedUnit ;
  rdfs:label "decijoule"@en, "decijoule"@nl ;
  rdfs:comment "The decijoule is a unit of energy defined as 1.0e-1 joule."@en ;
  ns2:symbol "dJ" ;
  ns2:hasPrefix ns2:deci ;
  ns2:hasUnit ns2:joule ;
  ns2:hasDimension ns2:energy-Dimension .

ns2:decajoule
  a ns2:PrefixedUnit ;
  rdfs:label "decajoule"@en, "decajoule"@nl ;
  rdfs:comment "The decajoule is a unit of energy defined as 1.0e1 joule."@en ;
  ns2:symbol "daJ" ;
  ns2:hasPrefix ns2:deca ;
  ns2:hasUnit ns2:joule ;
  ns2:hasDimension ns2:energy-Dimension .

ns2:hectojoule
  a ns2:PrefixedUnit ;
  rdfs:label "hectojoule"@en, "hectojoule"@nl ;
  rdfs:comment "The hectojoule is a unit of energy defined as 1.0e2 joule."@en ;
  ns2:symbol "hJ" ;
  ns2:hasPrefix ns2:hecto ;
  ns2:hasUnit ns2:joule ;
  ns2:hasDimension ns2:energy-Dimension .

ns2:kilojoule
  a ns2:PrefixedUnit ;
  rdfs:label "kilojoule"@en, "kilojoule"@nl ;
  rdfs:comment "The kilojoule is a unit of energy defined as 1.0e3 joule."@en ;
  ns2:symbol "kJ" ;
  ns2:hasPrefix ns2:kilo ;
  ns2:hasUnit ns2:joule ;
  ns2:hasDimension ns2:energy-Dimension .

ns2:megajoule
  a ns2:PrefixedUnit ;
  rdfs:label "megajoule"@en, "megajoule"@nl ;
  rdfs:comment "The megajoule is a unit of energy defined as 1.0e6 joule."@en ;
  ns2:symbol "MJ" ;
  ns2:hasPrefix ns2:mega ;
  ns2:hasUnit ns2:joule ;
  ns2:hasDimension ns2:energy-Dimension .

ns2:gigajoule
  a ns2:PrefixedUnit ;
  rdfs:label "gigajoule"@en, "gigajoule"@nl ;
  rdfs:comment "The gigajoule is a unit of energy defined as 1.0e9 joule."@en ;
  ns2:symbol "GJ" ;
  ns2:hasPrefix ns2:giga ;
  ns2:hasUnit ns2:joule ;
  ns2:hasDimension ns2:energy-Dimension .

ns2:terajoule
  a ns2:PrefixedUnit ;
  rdfs:label "terajoule"@en, "terajoule"@nl ;
  rdfs:comment "The terajoule is a unit of energy defined as 1.0e12 joule."@en ;
  ns2:symbol "TJ" ;
  ns2:hasPrefix ns2:tera ;
  ns2:hasUnit ns2:joule ;
  ns2:hasDimension ns2:energy-Dimension .

ns2:petajoule
  a ns2:PrefixedUnit ;
  rdfs:label "petajoule"@en, "petajoule"@nl ;
  rdfs:comment "The petajoule is a unit of energy defined as 1.0e15 joule."@en ;
  ns2:symbol "PJ" ;
  ns2:hasPrefix ns2:peta ;
  ns2:hasUnit ns2:joule ;
  ns2:hasDimension ns2:energy-Dimension .

ns2:exajoule
  a ns2:PrefixedUnit ;
  rdfs:label "exajoule"@en, "exajoule"@nl ;
  rdfs:comment "The exajoule is a unit of energy defined as 1.0e18 joule."@en ;
  ns2:symbol "EJ" ;
  ns2:hasPrefix ns2:exa ;
  ns2:hasUnit ns2:joule ;
  ns2:hasDimension ns2:energy-Dimension .

ns2:zettajoule
  a ns2:PrefixedUnit ;
  rdfs:label "zettajoule"@en, "zettajoule"@nl ;
  rdfs:comment "The zettajoule is a unit of energy defined as 1.0e21 joule."@en ;
  ns2:symbol "ZJ" ;
  ns2:hasPrefix ns2:zetta ;
  ns2:hasUnit ns2:joule ;
  ns2:hasDimension ns2:energy-Dimension .

ns2:yottajoule
  a ns2:PrefixedUnit ;
  rdfs:label "yottajoule"@en, "yottajoule"@nl ;
  rdfs:comment "The yottajoule is a unit of energy defined as 1.0e24 joule."@en ;
  ns2:symbol "YJ" ;
  ns2:hasPrefix ns2:yotta ;
  ns2:hasUnit ns2:joule ;
  ns2:hasDimension ns2:energy-Dimension .

ns2:kilocalorie-Mean
  a ns2:PrefixedUnit ;
  rdfs:label "kilocalorie (mean)"@en ;
  rdfs:comment "The kilocalorie (mean) is a unit of energy defined as 1.0e3 calorie (mean)."@en ;
  ns2:symbol "kcal" ;
  ns2:hasPrefix ns2:kilo ;
  ns2:hasUnit ns2:calorie-Mean ;
  ns2:hasDimension ns2:energy-Dimension .

ns2:megaerg
  a ns2:PrefixedUnit ;
  rdfs:label "megaerg"@en ;
  ns2:alternativeLabel "megalerg"@en ;
  rdfs:comment "The megaerg is a unit of energy defined as 1.0e6 erg."@en ;
  ns2:symbol "Merg" ;
  ns2:hasPrefix ns2:mega ;
  ns2:hasUnit ns2:erg ;
  ns2:hasDimension ns2:energy-Dimension .

ns2:megawattHour
  a ns2:UnitMultiplication ;
  rdfs:label "megawatt hour"@en ;
  ns2:alternativeLabel "megawatt-hour"@en, "megawatthour"@en ;
  ns2:symbol "MW h" ;
  ns2:alternativeSymbol "MW·h", "MWh" ;
  ns2:hasTerm1 ns2:megawatt ;
  ns2:hasTerm2 ns2:hour ;
  ns2:hasDimension ns2:energy-Dimension .

ns2:gigawattHour
  a ns2:UnitMultiplication ;
  rdfs:label "gigawatt hour"@en ;
  ns2:alternativeLabel "gigawatt-hour"@en, "gigawatthour"@en ;
  ns2:symbol "GW h" ;
  ns2:alternativeSymbol "GW·h", "GWh" ;
  ns2:hasTerm1 ns2:gigawatt ;
  ns2:hasTerm2 ns2:hour ;
  ns2:hasDimension ns2:energy-Dimension .

ns2:joulePerSecond-Time
  a ns2:UnitDivision ;
  rdfs:label "joule per second"@en, "joule per seconde"@nl ;
  ns2:symbol "J/s" ;
  ns2:alternativeSymbol "J s-1", "J·s-1" ;
  ns2:hasNumerator ns2:joule ;
  ns2:hasDenominator ns2:second-Time ;
  ns2:hasDimension ns2:power-Dimension .

ns2:PowerUnit
  a owl:Class ;
  rdfs:label "power unit"@en ;
  rdfs:subClassOf ns2:Unit ;
  owl:equivalentClass [
    a owl:Class ;
    owl:unionOf (
     _:genid691
     ns2:PrefixedWatt
   )
  ] .

ns2:horsepower-Boiler
  a ns2:Unit, ns2:SingularUnit ;
  rdfs:label "horsepower (boiler)"@en ;
  ns2:alternativeLabel "boiler horsepower"@en ;
  rdfs:comment "The boiler horsepower is a unit of power defined as 9.80950e3 watt."@en ;
  ns2:hasFactor "9.80950e3"^^xsd:float ;
  ns2:hasUnit ns2:watt ;
  ns2:hasDimension ns2:power-Dimension .

ns2:horsepower-British
  a ns2:Unit, ns2:SingularUnit ;
  rdfs:label "horsepower (British)"@en ;
  ns2:alternativeLabel "British horsepower"@en, "imperial horsepower"@en ;
  rdfs:comment "The British horsepower is a unit of power defined as 7.4570e2 watt."@en ;
  ns2:hasFactor "7.4570e2"^^xsd:float ;
  ns2:hasUnit ns2:watt ;
  ns2:hasDimension ns2:power-Dimension .

ns2:horsepower-Electric
  a ns2:Unit, ns2:SingularUnit ;
  rdfs:label "horsepower (electric)"@en ;
  ns2:alternativeLabel "electric horsepower"@en ;
  rdfs:comment "The electric horsepower is a unit of power defined as 7.46e2 watt."@en ;
  ns2:hasFactor "7.46e2"^^xsd:float ;
  ns2:hasUnit ns2:watt ;
  ns2:hasDimension ns2:power-Dimension .

ns2:horsepower-Metric
  a ns2:Unit, ns2:SingularUnit ;
  rdfs:label "horsepower (metric)"@en ;
  ns2:alternativeLabel "metric horsepower"@en ;
  rdfs:comment "The metric horsepower is a unit of power defined as 7.354988e2 watt."@en ;
  ns2:symbol "PS" ;
  ns2:hasFactor "7.354988e2"^^xsd:float ;
  ns2:hasUnit ns2:watt ;
  ns2:hasDimension ns2:power-Dimension .

ns2:horsepower-Water
  a ns2:Unit, ns2:SingularUnit ;
  rdfs:label "horsepower (water)"@en ;
  ns2:alternativeLabel "water horsepower"@en ;
  rdfs:comment "The water horsepower is a unit of power defined as 7.46043e2 watt."@en ;
  ns2:hasFactor "7.46043e2"^^xsd:float ;
  ns2:hasUnit ns2:watt ;
  ns2:hasDimension ns2:power-Dimension .

ns2:kilocalorie-MeanPerDay
  a ns2:Unit, ns2:UnitDivision ;
  rdfs:label "kilocalorie (mean) per day"@en ;
  ns2:symbol "kcal/d" ;
  ns2:alternativeSymbol "kcal d-1", "kcal·d-1" ;
  ns2:hasNumerator ns2:kilocalorie-Mean ;
  ns2:hasDenominator ns2:day ;
  ns2:hasDimension ns2:power-Dimension .

ns2:solarLuminosity
  a ns2:Unit, ns2:SingularUnit ;
  rdfs:label "solar luminosity"@en ;
  rdfs:comment "Solar luminosity is a unit used in astronomy to denote stellar or galactic radiant fluxes (http://en.wikipedia.org/wiki/SolarLuminosity)."@en ;
  ns2:symbol "L_☉" ;
  ns2:LaTeXSymbol "L_{\\astrosun}" ;
  ns2:hasFactor "3.839e26"^^xsd:float ;
  ns2:hasUnit ns2:watt ;
  ns2:hasDimension ns2:power-Dimension .

ns2:tonOfRefrigeration
  a ns2:Unit, ns2:SingularUnit ;
  rdfs:label "ton of refrigeration"@en ;
  rdfs:comment "The ton of refrigeration is a unit of power defined as 3.516853e3 watt."@en ;
  ns2:hasFactor "3.516853e3"^^xsd:float ;
  ns2:hasUnit ns2:watt ;
  ns2:hasDimension ns2:power-Dimension .

ns2:watt
  a ns2:Unit, ns2:SingularUnit ;
  rdfs:label "watt"@en, "watt"@nl ;
  rdfs:comment "The watt is a unit of power defined as joule divided by second = newton times metre divided by second = volt times ampere = kilogram times square metre divided by second to the power 3."@en ;
  ns2:longcomment "The watt is a unit of power defined as joule divided by second = newton times metre divided by second = volt times ampere = kilogram times square metre divided by second to the power 3. The watt is a derived unit in the International System of Units." ;
  ns2:symbol "W" ;
  ns2:hasUnit ns2:joulePerSecond-Time ;
  ns2:hasDimension ns2:power-Dimension .

ns2:PrefixedWatt
  a owl:Class ;
  rdfs:label "prefixed watt"@en ;
  rdfs:subClassOf ns2:PrefixedUnit ;
  owl:equivalentClass [
    a owl:Class ;
    owl:intersectionOf (
     _:genid707
     _:genid709
     _:genid711
     _:genid713
   )
  ] .

ns2:yoctowatt
  a ns2:PrefixedUnit ;
  rdfs:label "yoctowatt"@en, "yoctowatt"@nl ;
  ns2:symbol "yW" ;
  ns2:hasPrefix ns2:yocto ;
  ns2:hasUnit ns2:watt ;
  ns2:hasDimension ns2:power-Dimension .

ns2:zeptowatt
  a ns2:PrefixedUnit ;
  rdfs:label "zeptowatt"@en, "zeptowatt"@nl ;
  ns2:symbol "zW" ;
  ns2:hasPrefix ns2:zepto ;
  ns2:hasUnit ns2:watt ;
  ns2:hasDimension ns2:power-Dimension .

ns2:attowatt
  a ns2:PrefixedUnit ;
  rdfs:label "attowatt"@en, "attowatt"@nl ;
  ns2:symbol "aW" ;
  ns2:hasPrefix ns2:atto ;
  ns2:hasUnit ns2:watt ;
  ns2:hasDimension ns2:power-Dimension .

ns2:femtowatt
  a ns2:PrefixedUnit ;
  rdfs:label "femtowatt"@en, "femtowatt"@nl ;
  ns2:symbol "fW" ;
  ns2:hasPrefix ns2:femto ;
  ns2:hasUnit ns2:watt ;
  ns2:hasDimension ns2:power-Dimension .

ns2:picowatt
  a ns2:PrefixedUnit ;
  rdfs:label "picowatt"@en, "picowatt"@nl ;
  ns2:symbol "pW" ;
  ns2:hasPrefix ns2:pico ;
  ns2:hasUnit ns2:watt ;
  ns2:hasDimension ns2:power-Dimension .

ns2:nanowatt
  a ns2:PrefixedUnit ;
  rdfs:label "nanowatt"@en, "nanowatt"@nl ;
  ns2:symbol "nW" ;
  ns2:hasPrefix ns2:nano ;
  ns2:hasUnit ns2:watt ;
  ns2:hasDimension ns2:power-Dimension .

ns2:microwatt
  a ns2:PrefixedUnit ;
  rdfs:label "microwatt"@en, "microwatt"@nl ;
  ns2:symbol "μW" ;
  ns2:hasPrefix ns2:micro ;
  ns2:hasUnit ns2:watt ;
  ns2:hasDimension ns2:power-Dimension .

ns2:milliwatt
  a ns2:PrefixedUnit ;
  rdfs:label "milliwatt"@en, "milliwatt"@nl ;
  ns2:symbol "mW" ;
  ns2:hasPrefix ns2:milli ;
  ns2:hasUnit ns2:watt ;
  ns2:hasDimension ns2:power-Dimension .

ns2:centiwatt
  a ns2:PrefixedUnit ;
  rdfs:label "centiwatt"@en, "centiwatt"@nl ;
  ns2:symbol "cW" ;
  ns2:hasPrefix ns2:centi ;
  ns2:hasUnit ns2:watt ;
  ns2:hasDimension ns2:power-Dimension .

ns2:deciwatt
  a ns2:PrefixedUnit ;
  rdfs:label "deciwatt"@en, "deciwatt"@nl ;
  ns2:symbol "dW" ;
  ns2:hasPrefix ns2:deci ;
  ns2:hasUnit ns2:watt ;
  ns2:hasDimension ns2:power-Dimension .

ns2:decawatt
  a ns2:PrefixedUnit ;
  rdfs:label "decawatt"@en, "decawatt"@nl ;
  ns2:symbol "daW" ;
  ns2:hasPrefix ns2:deca ;
  ns2:hasUnit ns2:watt ;
  ns2:hasDimension ns2:power-Dimension .

ns2:hectowatt
  a ns2:PrefixedUnit ;
  rdfs:label "hectowatt"@en, "hectowatt"@nl ;
  ns2:symbol "hW" ;
  ns2:hasPrefix ns2:hecto ;
  ns2:hasUnit ns2:watt ;
  ns2:hasDimension ns2:power-Dimension .

ns2:kilowatt
  a ns2:PrefixedUnit ;
  rdfs:label "kilowatt"@en, "kilowatt"@nl ;
  ns2:symbol "kW" ;
  ns2:hasPrefix ns2:kilo ;
  ns2:hasUnit ns2:watt ;
  ns2:hasDimension ns2:power-Dimension .

ns2:megawatt
  a ns2:PrefixedUnit ;
  rdfs:label "megawatt"@en, "megawatt"@nl ;
  ns2:symbol "MW" ;
  ns2:hasPrefix ns2:mega ;
  ns2:hasUnit ns2:watt ;
  ns2:hasDimension ns2:power-Dimension .

ns2:gigawatt
  a ns2:PrefixedUnit ;
  rdfs:label "gigawatt"@en, "gigawatt"@nl ;
  ns2:symbol "GW" ;
  ns2:hasPrefix ns2:giga ;
  ns2:hasUnit ns2:watt ;
  ns2:hasDimension ns2:power-Dimension .

ns2:terawatt
  a ns2:PrefixedUnit ;
  rdfs:label "terawatt"@en, "terawatt"@nl ;
  ns2:symbol "TW" ;
  ns2:hasPrefix ns2:tera ;
  ns2:hasUnit ns2:watt ;
  ns2:hasDimension ns2:power-Dimension .

ns2:petawatt
  a ns2:PrefixedUnit ;
  rdfs:label "petawatt"@en, "petawatt"@nl ;
  ns2:symbol "PW" ;
  ns2:hasPrefix ns2:peta ;
  ns2:hasUnit ns2:watt ;
  ns2:hasDimension ns2:power-Dimension .

ns2:exawatt
  a ns2:PrefixedUnit ;
  rdfs:label "exawatt"@en, "exawatt"@nl ;
  ns2:symbol "EW" ;
  ns2:hasPrefix ns2:exa ;
  ns2:hasUnit ns2:watt ;
  ns2:hasDimension ns2:power-Dimension .

ns2:zettawatt
  a ns2:PrefixedUnit ;
  rdfs:label "zettawatt"@en, "zettawatt"@nl ;
  ns2:symbol "ZW" ;
  ns2:hasPrefix ns2:zetta ;
  ns2:hasUnit ns2:watt ;
  ns2:hasDimension ns2:power-Dimension .

ns2:yottawatt
  a ns2:PrefixedUnit ;
  rdfs:label "yottawatt"@en, "yottawatt"@nl ;
  ns2:symbol "YW" ;
  ns2:hasPrefix ns2:yotta ;
  ns2:hasUnit ns2:watt ;
  ns2:hasDimension ns2:power-Dimension .

ns2:RadiantFlux
  a owl:Class ;
  ns2:commonlyHasUnit ns2:attowatt, ns2:centiwatt, ns2:decawatt, ns2:deciwatt, ns2:exawatt, ns2:femtowatt, ns2:gigawatt, ns2:hectowatt, ns2:kilowatt, ns2:megawatt, ns2:microwatt, ns2:milliwatt, ns2:nanowatt, ns2:petawatt, ns2:picowatt, ns2:terawatt, ns2:joulePerSecond-Time, ns2:watt, ns2:horsepower-Boiler, ns2:horsepower-British, ns2:horsepower-Electric, ns2:horsepower-Metric, ns2:horsepower-Water, ns2:tonOfRefrigeration, ns2:solarLuminosity ;
  rdfs:label "radiant flux"@en ;
  ns2:alternativeLabel "radiant energy flux"@en, "radiant power"@en ;
  rdfs:comment "Radiant flux is the measure of the total power of electromagnetic radiation."@en ;
  rdfs:subClassOf ns2:Power ;
  ns2:symbol "Φ" ;
  ns2:alternativeSymbol "Φ_e", "P" .

ns2:joulePerKilogram
  a ns2:UnitDivision ;
  rdfs:label "joule per kilogram"@en, "joule per kilogram"@nl, "焦耳每千克"@zh ;
  ns2:symbol "J/kg" ;
  ns2:alternativeSymbol "J kg-1", "J·kg-1" ;
  ns2:hasNumerator ns2:joule ;
  ns2:hasDenominator ns2:kilogram ;
  ns2:hasDimension ns2:specificEnergyOrAbsorbedDoseOrDoseEquivalent-Dimension .

ns2:kilocalorie-MeanPerHectogram
  a ns2:UnitDivision ;
  rdfs:label "kilocalorie (mean) per hectogram"@en ;
  ns2:alternativeLabel "kilocalorie per 100 gram"@en ;
  ns2:symbol "kcal/hg" ;
  ns2:alternativeSymbol "kcal/100 g", "kcal hg-1", "kcal·hg-1" ;
  ns2:hasNumerator ns2:kilocalorie-Mean ;
  ns2:hasDenominator ns2:hectogram ;
  ns2:hasDimension ns2:specificEnergyOrAbsorbedDoseOrDoseEquivalent-Dimension .

ns2:kilojoulePerHectogram
  a ns2:UnitDivision ;
  rdfs:label "kilojoule per hectogram"@en, "kilojoule per hectogram"@nl ;
  ns2:alternativeLabel "kilojoule per 100 gram"@en, "kilojoule per 100 gram"@nl ;
  ns2:symbol "kJ/hg" ;
  ns2:alternativeSymbol "kJ/100 g", "kJ hg-1", "kJ·hg-1" ;
  ns2:hasNumerator ns2:kilojoule ;
  ns2:hasDenominator ns2:hectogram ;
  ns2:hasDimension ns2:specificEnergyOrAbsorbedDoseOrDoseEquivalent-Dimension .

ns2:SpecificEnergyUnit
  a owl:Class ;
  rdfs:label "specific energy unit"@en ;
  rdfs:subClassOf ns2:Unit ;
  owl:equivalentClass [
    a owl:Class ;
    owl:oneOf (
     ns2:joulePerKilogram
     ns2:kilocalorie-MeanPerHectogram
     ns2:kilojoulePerHectogram
   )
  ] .

ns2:radianPerSecond-Time
  a ns2:UnitDivision ;
  rdfs:label "radian per second"@en, "radiaal per seconde"@nl ;
  ns2:symbol "rad/s" ;
  ns2:alternativeSymbol "rad s-1", "rad·s-1" ;
  ns2:hasNumerator ns2:radian ;
  ns2:hasDenominator ns2:second-Time ;
  ns2:hasDimension ns2:angularSpeed-Dimension .

ns2:AngularSpeedUnit
  a owl:Class ;
  rdfs:label "angular speed unit"@en ;
  rdfs:subClassOf ns2:Unit ;
  owl:equivalentClass [
    a owl:Class ;
    owl:oneOf (
     ns2:millisecond-AnglePerYear
     ns2:radianPerSecond-Time
   )
  ] .

ns2:millisecond-AnglePerYear
  a ns2:UnitDivision ;
  rdfs:label "millisecond (angle) per year"@en, "milliseconde (hoek) per jaar"@nl ;
  rdfs:comment "Wordt gebruikt om de waargenomen verandering van de positie van sterren uit te drukken (de proper motion)."@nl ;
  ns2:symbol "mas/yr" ;
  ns2:hasNumerator ns2:millisecond-Angle ;
  ns2:hasDenominator ns2:year ;
  ns2:hasDimension ns2:angularSpeed-Dimension .

ns2:radianPerSecond-TimeSquared
  a ns2:UnitDivision ;
  rdfs:label "radian per second squared"@en, "radiaal per seconde kwadraat"@nl ;
  ns2:symbol "rad/s2" ;
  ns2:alternativeSymbol "rad s-2", "rad·s-2" ;
  ns2:hasNumerator ns2:radian ;
  ns2:hasDenominator ns2:second-TimeSquared ;
  ns2:hasDimension ns2:angularAcceleration-Dimension .

ns2:AngularAccelerationUnit
  a owl:Class ;
  rdfs:label "angular acceleration unit"@en ;
  rdfs:subClassOf ns2:Unit ;
  owl:equivalentClass [
    a owl:Class ;
    owl:oneOf ( ns2:radianPerSecond-TimeSquared )
  ] .

ns2:pascalSecond-Time
  a ns2:UnitMultiplication ;
  rdfs:label "pascal second"@en, "pascal seconde"@nl ;
  ns2:symbol "Pa s" ;
  ns2:alternativeSymbol "Pa·s" ;
  ns2:hasTerm1 ns2:pascal ;
  ns2:hasTerm2 ns2:second-Time ;
  ns2:hasDimension ns2:dynamicViscosity-Dimension .

ns2:DynamicViscosityUnit
  a owl:Class ;
  rdfs:label "dynamic viscosity unit"@en ;
  rdfs:subClassOf ns2:Unit ;
  owl:equivalentClass [
    a owl:Class ;
    owl:unionOf (
     _:genid731
     ns2:PrefixedPoise
   )
  ] .

ns2:poise
  a ns2:Unit, ns2:SingularUnit ;
  rdfs:label "poise"@en, "poise"@nl ;
  rdfs:comment "The poise is a unit of dynamic viscosity defined as 1.0e-1 pascal second (time)."@en ;
  ns2:symbol "P" ;
  ns2:hasFactor "1.0e-1"^^xsd:float ;
  ns2:hasUnit ns2:pascalSecond-Time ;
  ns2:hasDimension ns2:dynamicViscosity-Dimension .

ns2:PrefixedPoise
  a owl:Class ;
  rdfs:label "prefixed poise"@en ;
  rdfs:subClassOf ns2:PrefixedUnit ;
  owl:equivalentClass [
    a owl:Class ;
    owl:intersectionOf (
     _:genid739
     _:genid741
     _:genid743
     _:genid745
   )
  ] .

ns2:centipoise
  a ns2:PrefixedUnit ;
  rdfs:label "centipoise"@en, "centipoise"@nl ;
  ns2:symbol "cP" ;
  ns2:hasPrefix ns2:centi ;
  ns2:hasUnit ns2:poise ;
  ns2:hasDimension ns2:dynamicViscosity-Dimension .

ns2:squareMetrePerSecond-Time
  a ns2:UnitDivision ;
  rdfs:label "square metre per second"@en, "vierkante meter per seconde"@nl ;
  ns2:symbol "m2/s" ;
  ns2:alternativeSymbol "m2 s-1", "m2·s-1" ;
  ns2:hasNumerator ns2:squareMetre ;
  ns2:hasDenominator ns2:second-Time ;
  ns2:hasDimension ns2:kinematicViscosityOrThermalDiffusivity-Dimension .

ns2:KinematicViscosityUnit
  a owl:Class ;
  rdfs:label "kinematic viscosity unit"@en ;
  rdfs:subClassOf ns2:Unit ;
  owl:equivalentClass [
    a owl:Class ;
    owl:unionOf (
     _:genid748
     ns2:PrefixedStokes
   )
  ] .

ns2:stokes
  a ns2:Unit, ns2:SingularUnit ;
  rdfs:label "stokes"@en, "stokes"@nl ;
  rdfs:comment "The stokes is a unit of kinematic viscosity defined as 1.0e-4 square metre per second (time)."@en ;
  ns2:symbol "St" ;
  ns2:hasFactor "1.0e-4"^^xsd:float ;
  ns2:hasUnit ns2:squareMetrePerSecond-Time ;
  ns2:hasDimension ns2:kinematicViscosityOrThermalDiffusivity-Dimension .

ns2:PrefixedStokes
  a owl:Class ;
  rdfs:label "prefixed stokes"@en ;
  rdfs:subClassOf ns2:PrefixedUnit ;
  owl:equivalentClass [
    a owl:Class ;
    owl:intersectionOf (
     _:genid756
     _:genid758
     _:genid760
     _:genid762
   )
  ] .

ns2:centistokes
  a ns2:PrefixedUnit ;
  rdfs:label "centistokes"@en, "centistokes"@nl ;
  ns2:symbol "cSt" ;
  ns2:hasPrefix ns2:centi ;
  ns2:hasUnit ns2:stokes ;
  ns2:hasDimension ns2:kinematicViscosityOrThermalDiffusivity-Dimension .

ns2:wattPerSquareMetre
  a ns2:UnitDivision ;
  rdfs:label "watt per square metre"@en, "watt per vierkante meter"@nl ;
  ns2:symbol "W/m2" ;
  ns2:alternativeSymbol "W m-2", "W·m-2" ;
  ns2:hasNumerator ns2:watt ;
  ns2:hasDenominator ns2:squareMetre ;
  ns2:hasDimension ns2:powerDensity-Dimension .

ns2:Irradiance
  a owl:Class ;
  ns2:commonlyHasUnit ns2:wattPerSquareMetre ;
  rdfs:label "irradiance"@en ;
  rdfs:comment "Irradiance is the power of electromagnetic radiation at a surface per unit area."@en ;
  rdfs:subClassOf ns2:PowerDensity ;
  ns2:symbol "E" ;
  ns2:alternativeSymbol "E_e" .

ns2:PowerDensityUnit
  a owl:Class ;
  rdfs:label "power density unit"@en ;
  rdfs:subClassOf ns2:Unit ;
  owl:equivalentClass [
    a owl:Class ;
    owl:oneOf ( ns2:wattPerSquareMetre )
  ] .

ns2:wattPerSteradian
  a ns2:UnitDivision ;
  rdfs:label "watt per steradian"@en, "watt per steradiaal"@nl ;
  ns2:symbol "W/sr" ;
  ns2:alternativeSymbol "W sr-1", "W·sr-1" ;
  ns2:hasNumerator ns2:watt ;
  ns2:hasDenominator ns2:steradian .

ns2:RadiantIntensity
  a owl:Class ;
  ns2:commonlyHasUnit ns2:wattPerSteradian ;
  rdfs:subClassOf [
    a owl:Restriction ;
    owl:onProperty ns2:hasValue ;
    owl:allValuesFrom [
      a owl:Restriction ;
      owl:onProperty ns2:hasUnit ;
      owl:allValuesFrom ns2:RadiantIntensityUnit
    ]
  ], ns2:Quantity ;
  rdfs:label "radiant intensity"@en ;
  ns2:symbol "I" ;
  ns2:alternativeSymbol "I_e" .

ns2:RadiantIntensityUnit
  a owl:Class ;
  rdfs:label "radiant intensity unit"@en ;
  rdfs:subClassOf ns2:Unit ;
  owl:equivalentClass [
    a owl:Class ;
    owl:oneOf ( ns2:wattPerSteradian )
  ] .

ns2:wattPerSquareMetreSteradian
  a ns2:UnitDivision ;
  rdfs:label "watt per square metre steradian"@en, "watt per vierkante meter steradiaal"@nl ;
  ns2:symbol "W/(m2 sr)" ;
  ns2:alternativeSymbol "W/(m2·sr)", "W m-2 sr-1", "W·m-2·sr-1" ;
  ns2:hasNumerator ns2:watt ;
  ns2:hasDenominator ns2:squareMetreSteradian ;
  ns2:hasDimension ns2:radiance-Dimension .

ns2:Radiance
  a owl:Class ;
  ns2:commonlyHasUnit ns2:wattPerSquareMetreSteradian ;
  rdfs:subClassOf [
    a owl:Restriction ;
    owl:onProperty ns2:hasValue ;
    owl:allValuesFrom [
      a owl:Restriction ;
      owl:onProperty ns2:hasUnit ;
      owl:allValuesFrom ns2:RadianceUnit
    ]
  ], ns2:Quantity, [
    a owl:Restriction ;
    owl:onProperty ns2:hasDimension ;
    owl:hasValue ns2:radiance-Dimension
  ] ;
  rdfs:label "radiance"@en ;
  rdfs:comment "Radiance is a radiometric measure that describes the amount of light that passes through or is emitted from a particular area and falls within a given solid angle in a specified direction."@en ;
  ns2:symbol "L" ;
  ns2:alternativeSymbol "L_e" .

ns2:RadianceUnit
  a owl:Class ;
  rdfs:label "radiance unit"@en ;
  rdfs:subClassOf ns2:Unit ;
  owl:equivalentClass [
    a owl:Class ;
    owl:oneOf ( ns2:wattPerSquareMetreSteradian )
  ] .

ns2:joulePerCubicmetre
  a ns2:UnitDivision ;
  rdfs:label "joule per cubic metre"@en, "joule per kubieke meter"@nl ;
  ns2:symbol "J/m3" ;
  ns2:alternativeSymbol "J m-3", "J·m-3" ;
  ns2:hasNumerator ns2:joule ;
  ns2:hasDenominator ns2:cubicMetre ;
  ns2:hasDimension ns2:energyDensity-Dimension .

ns2:EnergyDensityUnit
  a owl:Class ;
  rdfs:label "energy density unit"@en ;
  rdfs:subClassOf ns2:Unit ;
  owl:equivalentClass [
    a owl:Class ;
    owl:oneOf ( ns2:joulePerCubicmetre )
  ] .

ns2:jouleSecond-Time
  a ns2:UnitMultiplication ;
  rdfs:label "joule second"@en, "joule seconde"@nl ;
  ns2:symbol "J s" ;
  ns2:alternativeSymbol "J·s" ;
  ns2:hasTerm1 ns2:joule ;
  ns2:hasTerm2 ns2:second-Time ;
  ns2:hasDimension ns2:actionOrAngularMomentum-Dimension .

ns2:ActionUnit
  a owl:Class ;
  rdfs:label "action unit"@en ;
  rdfs:subClassOf ns2:Unit ;
  owl:equivalentClass [
    a owl:Class ;
    owl:oneOf (
     ns2:ergSecond-Time
     ns2:jouleSecond-Time
   )
  ] .

ns2:ergSecond-Time
  a ns2:UnitMultiplication ;
  rdfs:label "erg second"@en, "erg seconde"@nl ;
  ns2:symbol "erg s" ;
  ns2:alternativeSymbol "erg·s" ;
  ns2:hasTerm1 ns2:erg ;
  ns2:hasTerm2 ns2:second-Time ;
  ns2:hasDimension ns2:actionOrAngularMomentum-Dimension .

ns2:AngularMomentumUnit
  a owl:Class ;
  rdfs:label "angular momentum unit"@en ;
  rdfs:subClassOf ns2:Unit ;
  owl:equivalentClass [
    a owl:Class ;
    owl:oneOf (
     ns2:ergSecond-Time
     ns2:jouleSecond-Time
   )
  ] .

ns2:reciprocalPascalSecond-Time
  a ns2:UnitExponentiation ;
  rdfs:label "reciprocal pascal second"@en, "omgekeerde pascal seconde"@nl ;
  ns2:symbol "Pa-1 s-1" ;
  ns2:alternativeSymbol "Pa-1·s-1", "(Pa s)-1", "(Pa·s)-1" ;
  ns2:hasBase ns2:pascalSecond-Time ;
  ns2:hasExponent -1 ;
  ns2:hasDimension ns2:fluidity-Dimension .

ns2:FluidityUnit
  a owl:Class ;
  rdfs:label "fluidity unit"@en ;
  rdfs:subClassOf ns2:Unit ;
  owl:equivalentClass [
    a owl:Class ;
    owl:oneOf (
     ns2:rhe
     ns2:reciprocalPascalSecond-Time
   )
  ] .

ns2:rhe
  a ns2:Unit, ns2:SingularUnit ;
  rdfs:label "rhe"@en, "rhe"@nl ;
  rdfs:comment "The rhe is a unit of fluidity defined as 10 reciprocal pascal second (time)."@en ;
  ns2:hasFactor "1.0e1"^^xsd:float ;
  ns2:hasUnit ns2:reciprocalPascalSecond-Time ;
  ns2:hasDimension ns2:fluidity-Dimension .

ns2:metreKilogramPerSecond-Time
  a ns2:UnitDivision ;
  rdfs:label "metre kilogram per second"@en, "meter kilogram per seconde"@nl ;
  ns2:symbol "m kg/s" ;
  ns2:alternativeSymbol "m·kg/s", "m kg s-1", "m·kg·s-1" ;
  ns2:hasNumerator ns2:metreKilogram ;
  ns2:hasDenominator ns2:second-Time .

ns2:MomentumUnit
  a owl:Class ;
  rdfs:label "momentum unit"@en ;
  rdfs:subClassOf ns2:Unit ;
  owl:equivalentClass [
    a owl:Class ;
    owl:oneOf ( ns2:metreKilogramPerSecond-Time )
  ] .

ns2:kilogramSquareMetre
  a ns2:UnitMultiplication ;
  rdfs:label "kilogram square metre"@en, "kilogram vierkante meter"@nl ;
  ns2:symbol "kg m2" ;
  ns2:alternativeSymbol "kg·m2" ;
  ns2:hasTerm1 ns2:kilogram ;
  ns2:hasTerm2 ns2:squareMetre .

ns2:MomentOfInertiaUnit
  a owl:Class ;
  rdfs:label "moment of inertia unit"@en ;
  rdfs:subClassOf ns2:Unit ;
  owl:equivalentClass [
    a owl:Class ;
    owl:oneOf ( ns2:kilogramSquareMetre )
  ] .

ns2:ShearRate
  a owl:Class ;
  ns2:commonlyHasUnit ns2:reciprocalSecond-Time ;
  rdfs:subClassOf [
    a owl:Restriction ;
    owl:onProperty ns2:hasValue ;
    owl:allValuesFrom [
      a owl:Restriction ;
      owl:onProperty ns2:hasUnit ;
      owl:allValuesFrom ns2:ShearRateUnit
    ]
  ], ns2:Quantity ;
  rdfs:label "shear rate"@en ;
  ns2:symbol "S" .

ns2:ShearRateUnit
  a owl:Class ;
  rdfs:label "shear rate unit"@en ;
  rdfs:subClassOf ns2:Unit ;
  owl:equivalentClass [
    a owl:Class ;
    owl:oneOf ( ns2:reciprocalSecond-Time )
  ] .

ns2:newtonPerMetre
  a ns2:UnitDivision ;
  rdfs:label "newton per metre"@en, "newton per meter"@nl ;
  ns2:symbol "N/m" ;
  ns2:alternativeSymbol "N m-1", "N·m-1" ;
  ns2:hasNumerator ns2:newton ;
  ns2:hasDenominator ns2:metre ;
  ns2:hasDimension ns2:surfaceTension-Dimension .

ns2:SurfaceTension
  a owl:Class ;
  ns2:commonlyHasUnit ns2:newtonPerMetre ;
  rdfs:subClassOf [
    a owl:Restriction ;
    owl:onProperty ns2:hasValue ;
    owl:allValuesFrom [
      a owl:Restriction ;
      owl:onProperty ns2:hasUnit ;
      owl:allValuesFrom ns2:SurfaceTensionUnit
    ]
  ], ns2:Quantity, [
    a owl:Restriction ;
    owl:onProperty ns2:hasDimension ;
    owl:hasValue ns2:surfaceTension-Dimension
  ] ;
  rdfs:label "surface tension"@en, "oppervlaktespanning"@nl ;
  rdfs:comment "Surface tension is an attractive property of the surface of a liquid."@en ;
  ns2:symbol "γ" ;
  ns2:alternativeSymbol "σ" .

ns2:SurfaceTensionUnit
  a owl:Class ;
  rdfs:label "surface tension unit"@en ;
  rdfs:subClassOf ns2:Unit ;
  owl:equivalentClass [
    a owl:Class ;
    owl:oneOf ( ns2:newtonPerMetre )
  ] .

ns2:cubicMetrePerSecond-Time
  a ns2:UnitDivision ;
  rdfs:label "cubic metre per second"@en, "kubieke meter per seconde"@nl ;
  ns2:symbol "m3/s" ;
  ns2:alternativeSymbol "m3 s-1", "m3·s-1" ;
  ns2:hasNumerator ns2:cubicMetre ;
  ns2:hasDenominator ns2:second-Time ;
  ns2:hasDimension ns2:volumetricFlowRate-Dimension .

ns2:VolumetricFlowRateUnit
  a owl:Class ;
  rdfs:label "volumetric flow rate unit"@en ;
  rdfs:subClassOf ns2:Unit ;
  owl:equivalentClass [
    a owl:Class ;
    owl:oneOf (
     ns2:cubicMetrePerSecond-Time
     ns2:cubicMetrePerYear
     ns2:litrePerHour
   )
  ] .

ns2:cubicMetrePerYear
  a ns2:UnitDivision ;
  rdfs:label "cubic metre per year"@en, "kubieke meter per jaar"@nl ;
  ns2:hasNumerator ns2:cubicMetre ;
  ns2:hasDenominator ns2:year ;
  ns2:hasDimension ns2:volumetricFlowRate-Dimension .

ns2:litrePerHour
  a ns2:UnitDivision ;
  rdfs:label "litre per hour"@en, "liter per uur"@nl ;
  ns2:symbol "l/h" ;
  ns2:alternativeSymbol "l h-1", "l·h-1" ;
  ns2:hasNumerator ns2:litre ;
  ns2:hasDenominator ns2:hour .

ns2:reciprocalWatt
  a ns2:UnitExponentiation ;
  rdfs:label "reciprocal watt"@en, "omgekeerde watt"@nl ;
  ns2:symbol "W-1" ;
  ns2:hasBase ns2:watt ;
  ns2:hasExponent -1 .

ns2:Detectivity
  a owl:Class ;
  ns2:commonlyHasUnit ns2:reciprocalWatt ;
  rdfs:subClassOf [
    a owl:Restriction ;
    owl:onProperty ns2:hasValue ;
    owl:allValuesFrom [
      a owl:Restriction ;
      owl:onProperty ns2:hasUnit ;
      owl:allValuesFrom ns2:DetectivityUnit
    ]
  ], ns2:Quantity ;
  rdfs:label "detectivity"@en ;
  rdfs:comment "Reciprocal of Noise equivalent power. The signal-to-noise ratio for incident radiation of unit intensity."@en ;
  ns1:reference ns1:Astrophysical_Techniques_chapter1 ;
  ns2:symbol "D" .

ns2:DetectivityUnit
  a owl:Class ;
  rdfs:label "detectivity unit"@en ;
  rdfs:subClassOf ns2:Unit ;
  owl:equivalentClass [
    a owl:Class ;
    owl:oneOf ( ns2:reciprocalWatt )
  ] .

ns2:kilogramPerSecond-Time
  a ns2:UnitDivision ;
  rdfs:label "kilogram per second"@en, "kilogram per seconde"@nl ;
  ns2:symbol "kg/s" ;
  ns2:alternativeSymbol "kg s-1", "kg·s-1" ;
  ns2:hasNumerator ns2:kilogram ;
  ns2:hasDenominator ns2:second-Time ;
  ns2:hasDimension ns2:massFlow-Dimension .

ns2:gramPerDay
  a ns2:UnitDivision ;
  rdfs:label "gram per day"@en, "gram per dag"@nl ;
  ns2:symbol "g/d" ;
  ns2:alternativeSymbol "g d-1", "g·d-1" ;
  ns2:hasNumerator ns2:gram ;
  ns2:hasDenominator ns2:day ;
  ns2:hasDimension ns2:massFlow-Dimension .

ns2:milligramPerDay
  a ns2:UnitDivision ;
  rdfs:label "milligram per day"@en, "milligram per dag"@nl ;
  ns2:symbol "mg/d" ;
  ns2:alternativeSymbol "mg d-1", "mg·d-1" ;
  ns2:hasNumerator ns2:milligram ;
  ns2:hasDenominator ns2:day ;
  ns2:hasDimension ns2:massFlow-Dimension .

ns2:MassFlowUnit
  a owl:Class ;
  rdfs:label "mass flow unit"@en ;
  rdfs:subClassOf ns2:Unit ;
  owl:equivalentClass [
    a owl:Class ;
    owl:oneOf (
     ns2:gramPerDay
     ns2:kilogramPerSecond-Time
     ns2:milligramPerDay
   )
  ] .

ns2:metreKilogram
  a ns2:UnitMultiplication ;
  rdfs:label "metre kilogram"@en, "meter kilogram"@nl ;
  ns2:symbol "m kg" ;
  ns2:alternativeSymbol "m·kg" ;
  ns2:hasTerm1 ns2:metre ;
  ns2:hasTerm2 ns2:kilogram .

ns2:PrefixedMetrePrefixedGram
  a owl:Class ;
  rdfs:label "prefixed metre prefixed gram"@en ;
  rdfs:subClassOf ns2:UnitMultiplication ;
  owl:equivalentClass [
    a owl:Class ;
    owl:intersectionOf (
     _:genid828
     _:genid830
     _:genid832
     _:genid834
   )
  ] .

ns2:reciprocalGram
  a ns2:UnitExponentiation ;
  rdfs:label "reciprocal gram"@en, "omgekeerde gram"@nl ;
  ns2:symbol "g-1" ;
  ns2:hasBase ns2:gram ;
  ns2:hasExponent -1 .

ns2:kilogramSecond-TimeToThePower-2
  a ns2:UnitMultiplication ;
  rdfs:label "kilogram second to the power -2"@en, "kilogram seconde tot de macht -2"@nl ;
  ns2:symbol "kg s-2" ;
  ns2:alternativeSymbol "kg·s-2" ;
  ns2:hasTerm1 ns2:kilogram ;
  ns2:hasTerm2 ns2:second-TimeToThePower-2 .

ns2:gramPerJoule
  a ns2:UnitDivision ;
  rdfs:label "gram per joule"@en, "gram per joule"@nl ;
  rdfs:comment "Gram per joule is a unit of mass per energy."@en ;
  ns2:longcomment "Gram per joule is a unit of mass per energy defined as gram divided by joule. Gram per joule is a derived unit in the International System of Units." ;
  ns2:symbol "g/J" ;
  ns2:alternativeSymbol "g J-1", "g·J-1" ;
  ns2:hasNumerator ns2:gram ;
  ns2:hasDenominator ns2:joule .

ns2:kilogramPerGigajoule
  a ns2:UnitDivision ;
  rdfs:label "kilogram per gigajoule"@en, "kilogram per gigajoule"@nl ;
  rdfs:comment "Kilogram per gigajoule is a unit of mass per energy."@en ;
  ns2:longcomment "Kilogram per gigajoule is a unit of mass per energy defined as kilogram divided by gigajoule. Kilogram per gigajoule is a derived unit in the International System of Units." ;
  ns2:symbol "kg/GJ" ;
  ns2:alternativeSymbol "kg GJ-1", "kg·GJ-1" ;
  ns2:hasNumerator ns2:kilogram ;
  ns2:hasDenominator ns2:gigajoule .

ns2:microgramPerJoule
  a ns2:UnitDivision ;
  rdfs:label "microgram per joule"@en, "microgram per joule"@nl ;
  ns2:symbol "mg/J" ;
  ns2:alternativeSymbol "mg J-1", "mg·J-1" ;
  ns2:hasNumerator ns2:microgram ;
  ns2:hasDenominator ns2:joule .

ns2:MassPerEnergyUnit
  a owl:Class ;
  rdfs:label "mass per energy unit"@en ;
  rdfs:subClassOf ns2:Unit ;
  owl:equivalentClass [
    a owl:Class ;
    owl:oneOf (
     ns2:gramPerJoule
     ns2:kilogramPerGigaJoule
     ns2:microgramPerJoule
   )
  ] .

ns2:kilogramPerGigaJoule a ns2:UnitDivision .
ns2:gramPerMetre
  a ns2:UnitDivision ;
  rdfs:label "gram per metre"@en, "gram per meter"@nl ;
  ns2:symbol "g/m" ;
  ns2:alternativeSymbol "g m-1", "g·m-1" ;
  ns2:hasNumerator ns2:gram ;
  ns2:hasDenominator ns2:metre .

ns2:milligramPerKilometre
  a ns2:UnitDivision ;
  rdfs:label "milligram per kilometre"@en, "milligram per kilometer"@nl ;
  ns2:symbol "mg/km" ;
  ns2:alternativeSymbol "mg km-1", "mg·km-1" ;
  ns2:hasNumerator ns2:milligram ;
  ns2:hasDenominator ns2:kilometre .

ns2:gramPerSquareMetre
  a ns2:UnitDivision ;
  rdfs:label "gram per square metre"@en, "gram per vierkante meter"@nl ;
  ns2:symbol "g/m2" ;
  ns2:alternativeSymbol "g m-2", "g·m-2" ;
  ns2:hasNumerator ns2:gram ;
  ns2:hasDenominator ns2:squareMetre .

ns2:AreaDensityUnit
  a owl:Class ;
  rdfs:label "area density unit"@en ;
  rdfs:subClassOf ns2:Unit ;
  owl:equivalentClass [
    a owl:Class ;
    owl:unionOf ( _:genid843 )
  ] .

ns2:kilogramPerSquareMetre
  a ns2:UnitDivision ;
  rdfs:label "kilogram per square metre"@en, "kilogram per vierkante meter"@nl ;
  ns2:symbol "kg/m2" ;
  ns2:alternativeSymbol "kg m-2", "kg·m-2" ;
  ns2:hasNumerator ns2:kilogram ;
  ns2:hasDenominator ns2:squareMetre .

ns2:kilogramPerHectare
  a ns2:UnitDivision ;
  rdfs:label "kilogram per hectare"@en, "kilogram per hectare"@nl ;
  ns2:symbol "kg/ha" ;
  ns2:alternativeSymbol "kg ha-1", "kg·ha-1" ;
  ns2:hasNumerator ns2:kilogram ;
  ns2:hasDenominator ns2:hectare .

ns2:ounceAvoirdupoisPerSquareYard-International
  a ns2:UnitDivision ;
  rdfs:label "ounce (avoirdupois) per square yard (international)"@en ;
  ns2:symbol "oz/yd2" ;
  ns2:alternativeSymbol "oz yd-2", "oz·yd-1" ;
  ns2:hasNumerator ns2:ounceAvoirdupois ;
  ns2:hasDenominator ns2:squareYard-International .

ns2:hectareDay
  a ns2:UnitMultiplication ;
  rdfs:label "hectare day"@en, "hectare dag"@nl ;
  ns2:symbol "ha d" ;
  ns2:alternativeSymbol "ha·d" ;
  ns2:hasTerm1 ns2:hectare ;
  ns2:hasTerm2 ns2:day .

ns2:kilogramPerHectareDay
  a ns2:UnitDivision ;
  rdfs:label "kilogram per hectare day"@en, "kilogram per hectare dag"@nl ;
  ns2:symbol "kg/(ha d)" ;
  ns2:alternativeSymbol "kg ha-1 d-1", "kg·ha-1·d-1" ;
  ns2:hasNumerator ns2:kilogram ;
  ns2:hasDenominator ns2:hectareDay .

ns2:AreaDensityRateUnit
  a owl:Class ;
  rdfs:label "area density rate unit"@en ;
  rdfs:subClassOf ns2:Unit ;
  owl:equivalentClass [
    a owl:Class ;
    owl:unionOf ( _:genid852 )
  ] .

ns2:joulePerSquareMetre
  a ns2:UnitDivision ;
  rdfs:label "joule per square metre"@en, "joule per vierkante meter"@nl ;
  ns2:symbol "J/m2" ;
  ns2:alternativeSymbol "J m-2", "J·m-2" ;
  ns2:hasNumerator ns2:joule ;
  ns2:hasDenominator ns2:squareMetre .

ns2:megajoulePerSquareMetre
  a ns2:UnitDivision ;
  rdfs:label "megajoule per square metre"@en, "megajoule per vierkante meter"@nl ;
  ns2:symbol "MJ/m2" ;
  ns2:alternativeSymbol "MJ m-2", "MJ·m-2" ;
  ns2:hasNumerator ns2:megajoule ;
  ns2:hasDenominator ns2:squareMetre .

ns2:joulePerSquareMetreSecond-Time
  a ns2:UnitDivision ;
  rdfs:label "joule per square metre second"@en, "joule per vierkante meter seconde"@nl ;
  ns2:symbol "J/(m2 s)" ;
  ns2:alternativeSymbol "J m-2 s-1", "J·m-2·s-1" ;
  ns2:hasNumerator ns2:joule ;
  ns2:hasDenominator ns2:squareMetreSecond-Time .

ns2:joulePerSquareMetreDay
  a ns2:UnitDivision ;
  rdfs:label "joule per square metre day"@en, "joule per vierkante meter dag"@nl ;
  ns2:symbol "J/(m2 d)" ;
  ns2:alternativeSymbol "J m-2 d-1", "J·m-2·d-1" ;
  ns2:hasNumerator ns2:joule ;
  ns2:hasDenominator ns2:squareMetreDay .

ns2:kilojoulePerSquareMetreDay
  a ns2:UnitDivision ;
  rdfs:label "kilojoule per square metre day"@en, "kilojoule per vierkante meter dag"@nl ;
  ns2:symbol "kJ/(m2 d)" ;
  ns2:alternativeSymbol "kJ m-2 d-1", "kJ·m-2·d-1" ;
  ns2:hasNumerator ns2:kilojoule ;
  ns2:hasDenominator ns2:squareMetreDay .

ns2:megajoulePerSquareMetreDay
  a ns2:UnitDivision ;
  rdfs:label "megajoule per square metre day"@en, "megajoule per vierkante meter dag"@nl ;
  ns2:symbol "MJ/(m2 d)" ;
  ns2:alternativeSymbol "MJ m-2 d-1", "MJ·m-2·d-1" ;
  ns2:hasNumerator ns2:megajoule ;
  ns2:hasDenominator ns2:squareMetreDay .

ns2:gramPerSquareMetreSecond-Time
  a ns2:UnitDivision ;
  rdfs:label "gram per square metre second"@en, "gram per vierkante meter seconde"@nl ;
  ns2:symbol "g/(m2 s)" ;
  ns2:alternativeSymbol "g m-2 s-1", "g·m-2·s-1" ;
  ns2:hasNumerator ns2:gram ;
  ns2:hasDenominator ns2:squareMetreSecond-Time .

ns2:gramPerSquareMetreDay
  a ns2:UnitDivision ;
  rdfs:label "gram per square metre day"@en, "gram per vierkante meter dag"@nl ;
  ns2:symbol "g/(m2 d)" ;
  ns2:alternativeSymbol "g m-2 d-1", "g·m-2·d-1" ;
  ns2:hasNumerator ns2:gram ;
  ns2:hasDenominator ns2:squareMetreDay .

ns2:microgramPerSquareMetreSecond-Time
  a ns2:UnitDivision ;
  rdfs:label "microgram per square metre second"@en, "microgram per vierkante meter seconde"@nl ;
  ns2:symbol "mg/(m2 s)" ;
  ns2:alternativeSymbol "mg m-2 s-1", "mg·m-2·s-1" ;
  ns2:hasNumerator ns2:microgram ;
  ns2:hasDenominator ns2:squareMetreSecond-Time .

ns2:tonnePerCubicmetre
  a ns2:UnitDivision ;
  rdfs:label "tonne per cubic metre"@en, "ton per kubieke meter"@nl ;
  ns2:symbol "t/m3" ;
  ns2:alternativeSymbol "t m-3", "t·m-3" ;
  ns2:hasNumerator ns2:tonne ;
  ns2:hasDenominator ns2:cubicMetre .

ns2:wattSquareMetre
  a ns2:UnitMultiplication ;
  rdfs:label "watt square metre"@en, "watt vierkante meter"@nl ;
  ns2:symbol "W m2" ;
  ns2:alternativeSymbol "W·m2" ;
  ns2:hasTerm1 ns2:watt ;
  ns2:hasTerm2 ns2:squareMetre .

ns2:reciprocalSquareMetreReciprocalGram
  a ns2:UnitMultiplication ;
  rdfs:label "reciprocal square metre reciprocal gram"@en, "omgekeerde vierkante meter omgekeerde gram"@nl ;
  ns2:symbol "m-2 g-1" ;
  ns2:alternativeSymbol "m-2·g-1" ;
  ns2:hasTerm1 ns2:reciprocalSquareMetre ;
  ns2:hasTerm2 ns2:reciprocalGram .

ns2:gramPerMegajoule
  a ns2:UnitDivision ;
  rdfs:label "gram per megajoule"@en, "gram per megajoule"@nl ;
  ns2:symbol "g/MJ" ;
  ns2:alternativeSymbol "g MJ-1", "g·MJ-1" ;
  ns2:hasNumerator ns2:gram ;
  ns2:hasDenominator ns2:megajoule .

ns2:wattPerCubicmetre
  a ns2:UnitDivision ;
  rdfs:label "watt per cubic metre"@en, "watt per kubieke meter"@nl ;
  ns2:symbol "W/m3" ;
  ns2:alternativeSymbol "W m-3", "W·m-3" ;
  ns2:hasNumerator ns2:watt ;
  ns2:hasDenominator ns2:cubicMetre .

ns2:wattPerHertz
  a ns2:UnitDivision ;
  rdfs:label "watt per hertz"@en, "watt per hertz"@nl ;
  ns2:symbol "W/Hz" ;
  ns2:alternativeSymbol "W Hz-1", "W·Hz-1" ;
  ns2:hasNumerator ns2:watt ;
  ns2:hasDenominator ns2:hertz .

ns2:wattPerNanometre
  a ns2:UnitDivision ;
  rdfs:label "watt per nanometre"@en, "watt per nanometer"@nl ;
  ns2:symbol "W/nm" ;
  ns2:alternativeSymbol "W nm-1", "W·nm-1" ;
  ns2:hasNumerator ns2:watt ;
  ns2:hasDenominator ns2:nanometre .

ns2:wattPerSquareMetreHertz
  a ns2:UnitDivision ;
  rdfs:label "watt per square metre hertz"@en, "watt per vierkante meter hertz"@nl ;
  ns2:symbol "W/(m2 Hz)" ;
  ns2:alternativeSymbol "W m-2 Hz-1", "W·m-2·Hz-1" ;
  ns2:hasNumerator ns2:watt ;
  ns2:hasDenominator ns2:squareMetreHertz .

ns2:wattPerSquareMetreNanometre
  a ns2:UnitDivision ;
  rdfs:label "watt per square metre nanometre"@en, "watt per vierkante meter nanometer"@nl ;
  ns2:symbol "W/(m2 nm)" ;
  ns2:alternativeSymbol "W m-2 nm-1", "W·m-2·nm-1" ;
  ns2:hasNumerator ns2:watt ;
  ns2:hasDenominator ns2:squareMetreNanometre .

ns2:wattPerSteradianSquareMetre
  a ns2:UnitDivision ;
  rdfs:label "watt per steradian square metre"@en, "watt per steradiaal vierkante meter"@nl ;
  ns2:symbol "W/(sr m2)" ;
  ns2:alternativeSymbol "W sr-1 m-2", "W·sr-1·m-2" ;
  ns2:hasNumerator ns2:watt ;
  ns2:hasDenominator ns2:steradianSquareMetre .

ns2:wattPerSteradianSquareMetreHertz
  a ns2:UnitDivision ;
  rdfs:label "watt per steradian square metre hertz"@en, "watt per steradiaal vierkante meter hertz"@nl ;
  ns2:symbol "W/(sr m2 Hz)" ;
  ns2:alternativeSymbol "W sr-1 m-2 Hz-1", "W·sr-1·m-2·Hz-1" ;
  ns2:hasNumerator ns2:watt ;
  ns2:hasDenominator ns2:steradianSquareMetreHertz .

ns2:squareMetrePerGram
  a ns2:UnitDivision ;
  rdfs:label "square metre per gram"@en, "vierkante meter per gram"@nl ;
  ns2:symbol "m2/g" ;
  ns2:alternativeSymbol "m2 g-1", "m2·g-1" ;
  ns2:hasNumerator ns2:squareMetre ;
  ns2:hasDenominator ns2:gram .

ns2:megametrePerKilojoule
  a ns2:UnitDivision ;
  rdfs:label "megametre per kilojoule"@en ;
  ns2:alternativeLabel "1000 kilometre per kilojoule"@en ;
  ns2:unofficialAbbreviation "1000 km/kJ" ;
  ns2:symbol "Mm/kJ" ;
  ns2:hasNumerator ns2:megametre ;
  ns2:hasDenominator ns2:kilojoule .

ns2:megaeuroPerPetajoule
  a ns2:UnitDivision ;
  rdfs:label "megaeuro per petajoule"@en ;
  ns2:hasNumerator ns2:megaeuro ;
  ns2:hasDenominator ns2:petajoule .

ns2:megaeuroPerMegawatt
  a ns2:UnitDivision ;
  rdfs:label "megaeuro per megawatt"@en ;
  ns2:hasNumerator ns2:megaeuro ;
  ns2:hasDenominator ns2:megawatt .

ns2:gramPerSquareMetreMetre
  a ns2:UnitDivision ;
  rdfs:label "gram per square metre metre"@en ;
  ns2:symbol "g/(m2 m)" ;
  ns2:alternativeSymbol "g m-2 m-1", "g·m-2·m-1" ;
  ns2:hasNumerator ns2:gramPerSquareMetre ;
  ns2:hasDenominator ns2:metre .

ns2:gramPerSquareMetreCentimetre
  a ns2:UnitDivision ;
  rdfs:label "gram per square metre centimetre"@en ;
  ns2:symbol "g/(m2 cm)" ;
  ns2:alternativeSymbol "g m-2 cm-1", "g·m-2·cm-1" ;
  ns2:hasNumerator ns2:gramPerSquareMetre ;
  ns2:hasDenominator ns2:centimetre .

ns2:tonnePerHectare
  a ns2:UnitDivision ;
  rdfs:label "tonne per hectare"@en ;
  ns2:symbol "t/ha" ;
  ns2:alternativeSymbol "t ha-1", "t·ha-1" ;
  ns2:hasNumerator ns2:tonne ;
  ns2:hasDenominator ns2:hectare .

ns2:metrePerSecond-TimePerMetre
  a ns2:UnitDivision ;
  rdfs:label "metre per second per metre"@en, "meter per seconde per metre"@nl ;
  ns2:symbol "m/s/m" ;
  ns2:hasNumerator ns2:metrePerSecond-Time ;
  ns2:hasDenominator ns2:metre .

ns2:metrePerCubicMetre
  a ns2:UnitDivision ;
  rdfs:label "metre per cubic metre"@en, "meter per kubieke meter"@nl ;
  ns2:symbol "m/m3" ;
  ns2:alternativeSymbol "m m-3", "m·m-3" ;
  ns2:hasNumerator ns2:metre ;
  ns2:hasDenominator ns2:cubicMetre .

ns2:centimetrePerCubicCentimetre
  a ns2:UnitDivision ;
  rdfs:label "centimetre per cubic centimetre"@en, "centimeter per kubieke centimeter"@nl ;
  ns2:symbol "cm/cm3" ;
  ns2:alternativeSymbol "cm cm-3", "cm·cm-3" ;
  ns2:hasNumerator ns2:centimetre ;
  ns2:hasDenominator ns2:cubicCentimetre .

ns2:squareMetreSecond-Time
  a ns2:UnitMultiplication ;
  rdfs:label "square metre second"@en, "vierkante meter seconde"@nl ;
  ns2:symbol "m2 s" ;
  ns2:alternativeSymbol "m2·s" ;
  ns2:hasTerm1 ns2:squareMetre ;
  ns2:hasTerm2 ns2:second-Time .

ns2:squareMetreDay
  a ns2:UnitMultiplication ;
  rdfs:label "square metre day"@en, "vierkante meter dag"@nl ;
  ns2:symbol "m2 d" ;
  ns2:alternativeSymbol "m2·d" ;
  ns2:hasTerm1 ns2:squareMetre ;
  ns2:hasTerm2 ns2:day .

ns2:second-TimePerDay
  a ns2:UnitDivision ;
  rdfs:label "second per day"@en, "seconde per dag"@nl ;
  ns2:symbol "s/d" ;
  ns2:alternativeSymbol "s d-1", "s·d-1" ;
  ns2:hasNumerator ns2:second-Time ;
  ns2:hasDenominator ns2:day .

ns2:reciprocalSquareMetreReciprocalMetre
  a ns2:UnitMultiplication ;
  rdfs:label "reciprocal square metre reciprocal metre"@en, "omgekeerde vierkante meter omgekeerde meter"@nl ;
  ns2:symbol "m-2 m-1" ;
  ns2:alternativeSymbol "m-2·m-1" ;
  ns2:hasTerm1 ns2:reciprocalSquareMetre ;
  ns2:hasTerm2 ns2:reciprocalMetre .

ns2:squareMetreHertz
  a ns2:UnitMultiplication ;
  rdfs:label "square metre hertz"@en, "vierkante meter hertz"@nl ;
  ns2:symbol "m2 Hz" ;
  ns2:alternativeSymbol "m2·Hz" ;
  ns2:hasTerm1 ns2:squareMetre ;
  ns2:hasTerm2 ns2:hertz .

ns2:squareMetreNanometre
  a ns2:UnitMultiplication ;
  rdfs:label "square metre nanometre"@en, "vierkante meter nanometer"@nl ;
  ns2:symbol "m2 nm" ;
  ns2:alternativeSymbol "m2·nm" ;
  ns2:hasTerm1 ns2:squareMetre ;
  ns2:hasTerm2 ns2:nanometre .

ns2:reciprocalSquareMetre
  a ns2:UnitExponentiation ;
  rdfs:label "reciprocal square metre"@en, "omgekeerde vierkante meter"@nl ;
  ns2:symbol "m-2" ;
  ns2:hasBase ns2:metre ;
  ns2:hasExponent -2 ;
  ns2:hasDimension ns2:columnNumberDensity-Dimension .

ns2:reciprocalSquareCentimetre
  a ns2:UnitExponentiation ;
  rdfs:label "reciprocal square centimetre"@en, "omgekeerde vierkante centimeter"@nl ;
  ns2:symbol "cm-2" ;
  ns2:hasBase ns2:centimetre ;
  ns2:hasExponent -2 ;
  ns2:hasDimension ns2:columnNumberDensity-Dimension .

ns2:ColumnNumberDensityUnit
  a owl:Class ;
  rdfs:label "column number density unit"@en ;
  rdfs:subClassOf ns2:Unit ;
  owl:equivalentClass [
    a owl:Class ;
    owl:oneOf (
     ns2:reciprocalSquareCentimetre
     ns2:reciprocalSquareMetre
   )
  ] .

ns2:partsPerMillionPerYear
  a ns2:UnitDivision ;
  rdfs:label "parts per million per year"@en ;
  ns2:symbol "ppm/a" ;
  ns2:alternativeSymbol "ppm a-1", "ppm·a-1", "ppm/y", "ppm y-1", "ppm·y-1", "ppm/yr", "ppm yr-1", "ppm·yr-1" ;
  ns2:hasNumerator ns2:partsPerMillion ;
  ns2:hasDenominator ns2:year .

ns2:reciprocalPartsPerMillionPerYear
  a ns2:UnitExponentiation ;
  rdfs:label "reciprocal parts per million"@en ;
  ns2:symbol "ppm-1" ;
  ns2:hasBase ns2:partsPerMillion ;
  ns2:hasExponent -1 .

ns2:second-TimePerSquareMetre
  a ns2:UnitDivision ;
  rdfs:label "second per square metre"@en ;
  ns2:symbol "s/m2" ;
  ns2:alternativeSymbol "s m-2", "s·m-2" ;
  ns2:hasNumerator ns2:second-Time ;
  ns2:hasDenominator ns2:squareMetre .

ns2:squareMetrePerSquareMetreDay
  a ns2:UnitDivision ;
  rdfs:label "square metre per square metre day"@en ;
  ns2:symbol "m2/(m2 d)" ;
  ns2:alternativeSymbol "m2 m-2 d-1", "m2·m-2·d-1" ;
  ns2:hasNumerator ns2:squareMetrePerSquareMetre ;
  ns2:hasDenominator ns2:day .

ns2:second-TimeSquared
  a ns2:UnitExponentiation ;
  rdfs:label "second squared"@en, "seconde kwadraat"@nl ;
  ns2:symbol "s2" ;
  ns2:hasBase ns2:second-Time ;
  ns2:hasExponent 2 .

ns2:yoctosecond-TimeSquared
  a ns2:PrefixedSecond-TimeSquared ;
  rdfs:label "yoctosecond squared"@en, "yoctoseconde kwadraat"@nl ;
  ns2:symbol "ys2" ;
  ns2:hasBase ns2:yoctosecond-Time ;
  ns2:hasExponent 2 .

ns2:zeptosecond-TimeSquared
  a ns2:PrefixedSecond-TimeSquared ;
  rdfs:label "zeptosecond squared"@en, "zeptoseconde kwadraat"@nl ;
  ns2:symbol "zs2" ;
  ns2:hasBase ns2:zeptosecond-Time ;
  ns2:hasExponent 2 .

ns2:attosecond-TimeSquared
  a ns2:PrefixedSecond-TimeSquared ;
  rdfs:label "attosecond squared"@en, "attoseconde kwadraat"@nl ;
  ns2:symbol "as2" ;
  ns2:hasBase ns2:attosecond-Time ;
  ns2:hasExponent 2 .

ns2:femtosecond-TimeSquared
  a ns2:PrefixedSecond-TimeSquared ;
  rdfs:label "femtosecond squared"@en, "femtoseconde kwadraat"@nl ;
  ns2:symbol "fs2" ;
  ns2:hasBase ns2:femtosecond-Time ;
  ns2:hasExponent 2 .

ns2:picosecond-TimeSquared
  a ns2:PrefixedSecond-TimeSquared ;
  rdfs:label "picosecond squared"@en, "picoseconde kwadraat"@nl ;
  ns2:symbol "ps2" ;
  ns2:hasBase ns2:picosecond-Time ;
  ns2:hasExponent 2 .

ns2:nanosecond-TimeSquared
  a ns2:PrefixedSecond-TimeSquared ;
  rdfs:label "nanosecond squared"@en, "nanoseconde kwadraat"@nl ;
  ns2:symbol "ns2" ;
  ns2:hasBase ns2:nanosecond-Time ;
  ns2:hasExponent 2 .

ns2:microsecond-TimeSquared
  a ns2:PrefixedSecond-TimeSquared ;
  rdfs:label "microsecond squared"@en, "microseconde kwadraat"@nl ;
  ns2:symbol "μs2" ;
  ns2:hasBase ns2:microsecond-Time ;
  ns2:hasExponent 2 .

ns2:millisecond-TimeSquared
  a ns2:PrefixedSecond-TimeSquared ;
  rdfs:label "millisecond squared"@en, "milliseconde kwadraat"@nl ;
  ns2:symbol "ms2" ;
  ns2:hasBase ns2:millisecond-Time ;
  ns2:hasExponent 2 .

ns2:centisecond-TimeSquared
  a ns2:PrefixedSecond-TimeSquared ;
  rdfs:label "centisecond squared"@en, "centiseconde kwadraat"@nl ;
  ns2:symbol "cs2" ;
  ns2:hasBase ns2:centisecond-Time ;
  ns2:hasExponent 2 .

ns2:decisecond-TimeSquared
  a ns2:PrefixedSecond-TimeSquared ;
  rdfs:label "decisecond squared"@en, "deciseconde kwadraat"@nl ;
  ns2:symbol "ds2" ;
  ns2:hasBase ns2:decisecond-Time ;
  ns2:hasExponent 2 .

ns2:decasecond-TimeSquared
  a ns2:PrefixedSecond-TimeSquared ;
  rdfs:label "decasecond squared"@en, "decaseconde kwadraat"@nl ;
  ns2:symbol "das2" ;
  ns2:hasBase ns2:decasecond-Time ;
  ns2:hasExponent 2 .

ns2:hectosecond-TimeSquared
  a ns2:PrefixedSecond-TimeSquared ;
  rdfs:label "hectosecond squared"@en, "hectoseconde kwadraat"@nl ;
  ns2:symbol "hs2" ;
  ns2:hasBase ns2:hectosecond-Time ;
  ns2:hasExponent 2 .

ns2:kilosecond-TimeSquared
  a ns2:PrefixedSecond-TimeSquared ;
  rdfs:label "kilosecond squared"@en, "kiloseconde kwadraat"@nl ;
  ns2:symbol "ks2" ;
  ns2:hasBase ns2:kilosecond-Time ;
  ns2:hasExponent 2 .

ns2:megasecond-TimeSquared
  a ns2:PrefixedSecond-TimeSquared ;
  rdfs:label "megasecond squared"@en, "megaseconde kwadraat"@nl ;
  ns2:symbol "Ms2" ;
  ns2:hasBase ns2:megasecond-Time ;
  ns2:hasExponent 2 .

ns2:gigasecond-TimeSquared
  a ns2:PrefixedSecond-TimeSquared ;
  rdfs:label "gigasecond squared"@en, "gigaseconde kwadraat"@nl ;
  ns2:symbol "Gs2" ;
  ns2:hasBase ns2:gigasecond-Time ;
  ns2:hasExponent 2 .

ns2:terasecond-TimeSquared
  a ns2:PrefixedSecond-TimeSquared ;
  rdfs:label "terasecond squared"@en, "teraseconde kwadraat"@nl ;
  ns2:symbol "Ts2" ;
  ns2:hasBase ns2:terasecond-Time ;
  ns2:hasExponent 2 .

ns2:petasecond-TimeSquared
  a ns2:PrefixedSecond-TimeSquared ;
  rdfs:label "petasecond squared"@en, "petaseconde kwadraat"@nl ;
  ns2:symbol "Ps2" ;
  ns2:hasBase ns2:petasecond-Time ;
  ns2:hasExponent 2 .

ns2:exasecond-TimeSquared
  a ns2:PrefixedSecond-TimeSquared ;
  rdfs:label "exasecond squared"@en, "exaseconde kwadraat"@nl ;
  ns2:symbol "Es2" ;
  ns2:hasBase ns2:exasecond-Time ;
  ns2:hasExponent 2 .

ns2:zettasecond-TimeSquared
  a ns2:PrefixedSecond-TimeSquared ;
  rdfs:label "zettasecond squared"@en, "zettaseconde kwadraat"@nl ;
  ns2:symbol "Zs2" ;
  ns2:hasBase ns2:zettasecond-Time ;
  ns2:hasExponent 2 .

ns2:yottasecond-TimeSquared
  a ns2:PrefixedSecond-TimeSquared ;
  rdfs:label "yottasecond squared"@en, "yottaseconde kwadraat"@nl ;
  ns2:symbol "Ys2" ;
  ns2:hasBase ns2:yottasecond-Time ;
  ns2:hasExponent 2 .

ns2:PrefixedSecond-TimeSquared
  a owl:Class ;
  rdfs:label "prefixed second (time) squared"@en ;
  rdfs:subClassOf ns2:UnitExponentiation ;
  owl:equivalentClass [
    a owl:Class ;
    owl:intersectionOf (
     _:genid863
     _:genid865
     _:genid867
     _:genid869
   )
  ] .

ns2:second-TimeToThePower-2
  a ns2:UnitExponentiation ;
  rdfs:label "second to the power -2"@en, "seconde tot de macht -2"@nl ;
  ns2:symbol "s-2" ;
  ns2:hasBase ns2:second-Time ;
  ns2:hasExponent -2 .

ns2:steradianSquareMetre
  a ns2:UnitMultiplication ;
  rdfs:label "steradian square metre"@en, "steradiaal vierkante meter"@nl ;
  ns2:symbol "sr m2" ;
  ns2:alternativeSymbol "sr·m2" ;
  ns2:hasTerm1 ns2:steradian ;
  ns2:hasTerm2 ns2:squareMetre .

ns2:steradianSquareMetreHertz
  a ns2:UnitMultiplication ;
  rdfs:label "steradian square metre hertz"@en, "steradiaal vierkante meter hertz"@nl ;
  ns2:symbol "sr m2 Hz" ;
  ns2:alternativeSymbol "sr·m2·Hz" ;
  ns2:hasTerm1 ns2:steradianSquareMetre ;
  ns2:hasTerm2 ns2:hertz .

ns2:squareMetreSteradian
  a ns2:UnitMultiplication ;
  rdfs:label "square metre steradian"@en, "vierkante meter steradian"@nl ;
  ns2:symbol "m2 sr" ;
  ns2:alternativeSymbol "m2·sr" ;
  ns2:hasTerm1 ns2:squareMetre ;
  ns2:hasTerm2 ns2:steradian .

ns2:litrePer100Kilometre
  a ns2:UnitDivision ;
  rdfs:label "litre per 100 kilometre"@en, "liter per 100 kilometer"@nl ;
  ns2:alternativeLabel "litre per 100 kilometre"@en, "liter per 100 kilometer"@nl ;
  ns2:symbol "l/100 km" ;
  ns2:hasNumerator ns2:litre ;
  ns2:hasDenominator ns2:_100Kilometre .

ns2:_100Kilometre
  a ns2:UnitMultiple ;
  rdfs:label "100 kilometre"@en, "100 kilometer"@nl ;
  ns2:symbol "100 km" ;
  ns2:hasFactor "100"^^xsd:float ;
  ns2:hasUnit ns2:kilometre ;
  ns2:hasDimension ns2:length-Dimension .

ns2:time-Dimension
  a ns2:Dimension ;
  rdfs:label "time dimension"@en, "dimensie van tijd"@nl ;
  ns2:symbol "T" ;
  ns2:hasSILengthDimensionExponent 0 ;
  ns2:hasSIMassDimensionExponent 0 ;
  ns2:hasSITimeDimensionExponent 1 ;
  ns2:hasSIElectricCurrentDimensionExponent 0 ;
  ns2:hasSIThermodynamicTemperatureDimensionExponent 0 ;
  ns2:hasSIAmountOfSubstanceDimensionExponent 0 ;
  ns2:hasSILuminousIntensityDimensionExponent 0 .

ns2:mass-Dimension
  a ns2:Dimension ;
  rdfs:label "mass dimension"@en, "massadimensie"@nl ;
  ns2:symbol "M" ;
  ns2:hasSILengthDimensionExponent 0 ;
  ns2:hasSIMassDimensionExponent 1 ;
  ns2:hasSITimeDimensionExponent 0 ;
  ns2:hasSIElectricCurrentDimensionExponent 0 ;
  ns2:hasSIThermodynamicTemperatureDimensionExponent 0 ;
  ns2:hasSIAmountOfSubstanceDimensionExponent 0 ;
  ns2:hasSILuminousIntensityDimensionExponent 0 .

ns2:numberDensity-Dimension
  a ns2:Dimension ;
  rdfs:label "number density dimension"@en ;
  ns2:hasSILengthDimensionExponent -3 ;
  ns2:hasSIMassDimensionExponent 0 ;
  ns2:hasSITimeDimensionExponent 0 ;
  ns2:hasSIElectricCurrentDimensionExponent 0 ;
  ns2:hasSIThermodynamicTemperatureDimensionExponent 0 ;
  ns2:hasSIAmountOfSubstanceDimensionExponent 0 ;
  ns2:hasSILuminousIntensityDimensionExponent 0 .

ns2:columnNumberDensity-Dimension
  a ns2:Dimension ;
  rdfs:label "column number density dimension"@en ;
  ns2:hasSILengthDimensionExponent -2 ;
  ns2:hasSIMassDimensionExponent 0 ;
  ns2:hasSITimeDimensionExponent 0 ;
  ns2:hasSIElectricCurrentDimensionExponent 0 ;
  ns2:hasSIThermodynamicTemperatureDimensionExponent 0 ;
  ns2:hasSIAmountOfSubstanceDimensionExponent 0 ;
  ns2:hasSILuminousIntensityDimensionExponent 0 .

ns2:wavenumber-Dimension
  a ns2:Dimension ;
  rdfs:label "wavenumber dimension"@en, "golfgetaldimensie"@nl ;
  ns2:hasSILengthDimensionExponent -1 ;
  ns2:hasSIMassDimensionExponent 0 ;
  ns2:hasSITimeDimensionExponent 0 ;
  ns2:hasSIElectricCurrentDimensionExponent 0 ;
  ns2:hasSIThermodynamicTemperatureDimensionExponent 0 ;
  ns2:hasSIAmountOfSubstanceDimensionExponent 0 ;
  ns2:hasSILuminousIntensityDimensionExponent 0 .

ns2:frequency-Dimension
  a ns2:Dimension ;
  rdfs:label "frequency dimension"@en ;
  ns2:hasSILengthDimensionExponent 0 ;
  ns2:hasSIMassDimensionExponent 0 ;
  ns2:hasSITimeDimensionExponent -1 ;
  ns2:hasSIElectricCurrentDimensionExponent 0 ;
  ns2:hasSIThermodynamicTemperatureDimensionExponent 0 ;
  ns2:hasSIAmountOfSubstanceDimensionExponent 0 ;
  ns2:hasSILuminousIntensityDimensionExponent 0 .

ns2:acceleration-Dimension
  a ns2:Dimension ;
  rdfs:label "acceleration dimension"@en, "versnellingdimensie"@nl ;
  ns2:hasSILengthDimensionExponent 1 ;
  ns2:hasSIMassDimensionExponent 0 ;
  ns2:hasSITimeDimensionExponent -2 ;
  ns2:hasSIElectricCurrentDimensionExponent 0 ;
  ns2:hasSIThermodynamicTemperatureDimensionExponent 0 ;
  ns2:hasSIAmountOfSubstanceDimensionExponent 0 ;
  ns2:hasSILuminousIntensityDimensionExponent 0 .

ns2:density-Dimension
  a ns2:Dimension ;
  rdfs:label "density dimension"@en, "dichtheiddimensie"@nl ;
  ns2:hasSILengthDimensionExponent -3 ;
  ns2:hasSIMassDimensionExponent 1 ;
  ns2:hasSITimeDimensionExponent 0 ;
  ns2:hasSIElectricCurrentDimensionExponent 0 ;
  ns2:hasSIThermodynamicTemperatureDimensionExponent 0 ;
  ns2:hasSIAmountOfSubstanceDimensionExponent 0 ;
  ns2:hasSILuminousIntensityDimensionExponent 0 .

ns2:specificVolume-Dimension
  a ns2:Dimension ;
  rdfs:label "specific volume dimension"@en ;
  ns2:hasSILengthDimensionExponent 3 ;
  ns2:hasSIMassDimensionExponent -1 ;
  ns2:hasSITimeDimensionExponent 0 ;
  ns2:hasSIElectricCurrentDimensionExponent 0 ;
  ns2:hasSIThermodynamicTemperatureDimensionExponent 0 ;
  ns2:hasSIAmountOfSubstanceDimensionExponent 0 ;
  ns2:hasSILuminousIntensityDimensionExponent 0 .

ns2:speed-Dimension
  a ns2:Dimension ;
  rdfs:label "speed dimension"@en, "snelheiddimensie"@nl ;
  ns2:hasSILengthDimensionExponent 1 ;
  ns2:hasSIMassDimensionExponent 0 ;
  ns2:hasSITimeDimensionExponent -1 ;
  ns2:hasSIElectricCurrentDimensionExponent 0 ;
  ns2:hasSIThermodynamicTemperatureDimensionExponent 0 ;
  ns2:hasSIAmountOfSubstanceDimensionExponent 0 ;
  ns2:hasSILuminousIntensityDimensionExponent 0 .

ns2:force-Dimension
  a ns2:Dimension ;
  rdfs:label "force dimension"@en, "krachtdimensie"@nl ;
  ns2:hasSILengthDimensionExponent 1 ;
  ns2:hasSIMassDimensionExponent 1 ;
  ns2:hasSITimeDimensionExponent -2 ;
  ns2:hasSIElectricCurrentDimensionExponent 0 ;
  ns2:hasSIThermodynamicTemperatureDimensionExponent 0 ;
  ns2:hasSIAmountOfSubstanceDimensionExponent 0 ;
  ns2:hasSILuminousIntensityDimensionExponent 0 .

ns2:pressure-Dimension
  a ns2:Dimension ;
  rdfs:label "pressure dimension"@en ;
  ns2:hasSILengthDimensionExponent -1 ;
  ns2:hasSIMassDimensionExponent 1 ;
  ns2:hasSITimeDimensionExponent -2 ;
  ns2:hasSIElectricCurrentDimensionExponent 0 ;
  ns2:hasSIThermodynamicTemperatureDimensionExponent 0 ;
  ns2:hasSIAmountOfSubstanceDimensionExponent 0 ;
  ns2:hasSILuminousIntensityDimensionExponent 0 .

ns2:energy-Dimension
  a ns2:Dimension ;
  rdfs:label "energy dimension"@en ;
  ns2:hasSILengthDimensionExponent 2 ;
  ns2:hasSIMassDimensionExponent 1 ;
  ns2:hasSITimeDimensionExponent -2 ;
  ns2:hasSIElectricCurrentDimensionExponent 0 ;
  ns2:hasSIThermodynamicTemperatureDimensionExponent 0 ;
  ns2:hasSIAmountOfSubstanceDimensionExponent 0 ;
  ns2:hasSILuminousIntensityDimensionExponent 0 .

ns2:power-Dimension
  a ns2:Dimension ;
  rdfs:label "power dimension"@en ;
  ns2:hasSILengthDimensionExponent 2 ;
  ns2:hasSIMassDimensionExponent 1 ;
  ns2:hasSITimeDimensionExponent -3 ;
  ns2:hasSIElectricCurrentDimensionExponent 0 ;
  ns2:hasSIThermodynamicTemperatureDimensionExponent 0 ;
  ns2:hasSIAmountOfSubstanceDimensionExponent 0 ;
  ns2:hasSILuminousIntensityDimensionExponent 0 .

ns2:specificEnergyOrAbsorbedDoseOrDoseEquivalent-Dimension
  a ns2:Dimension ;
  rdfs:label "specific energy, absorbed dose, or dose equivalent dimension"@en ;
  ns2:hasSILengthDimensionExponent 2 ;
  ns2:hasSIMassDimensionExponent 0 ;
  ns2:hasSITimeDimensionExponent -2 ;
  ns2:hasSIElectricCurrentDimensionExponent 0 ;
  ns2:hasSIThermodynamicTemperatureDimensionExponent 0 ;
  ns2:hasSIAmountOfSubstanceDimensionExponent 0 ;
  ns2:hasSILuminousIntensityDimensionExponent 0 .

ns2:angularSpeed-Dimension
  a ns2:Dimension ;
  rdfs:label "angular speed dimension"@en ;
  ns2:hasSILengthDimensionExponent 0 ;
  ns2:hasSIMassDimensionExponent 0 ;
  ns2:hasSITimeDimensionExponent -1 ;
  ns2:hasSIElectricCurrentDimensionExponent 0 ;
  ns2:hasSIThermodynamicTemperatureDimensionExponent 0 ;
  ns2:hasSIAmountOfSubstanceDimensionExponent 0 ;
  ns2:hasSILuminousIntensityDimensionExponent 0 .

ns2:angularAcceleration-Dimension
  a ns2:Dimension ;
  rdfs:label "angular acceleration dimension"@en ;
  ns2:hasSILengthDimensionExponent 0 ;
  ns2:hasSIMassDimensionExponent 0 ;
  ns2:hasSITimeDimensionExponent -2 ;
  ns2:hasSIElectricCurrentDimensionExponent 0 ;
  ns2:hasSIThermodynamicTemperatureDimensionExponent 0 ;
  ns2:hasSIAmountOfSubstanceDimensionExponent 0 ;
  ns2:hasSILuminousIntensityDimensionExponent 0 .

ns2:dynamicViscosity-Dimension
  a ns2:Dimension ;
  rdfs:label "dynamic viscosity dimension"@en ;
  ns2:hasSILengthDimensionExponent -1 ;
  ns2:hasSIMassDimensionExponent 1 ;
  ns2:hasSITimeDimensionExponent -1 ;
  ns2:hasSIElectricCurrentDimensionExponent 0 ;
  ns2:hasSIThermodynamicTemperatureDimensionExponent 0 ;
  ns2:hasSIAmountOfSubstanceDimensionExponent 0 ;
  ns2:hasSILuminousIntensityDimensionExponent 0 .

ns2:kinematicViscosityOrThermalDiffusivity-Dimension
  a ns2:Dimension ;
  rdfs:label "kinematic viscosity dimension"@en ;
  ns2:hasSILengthDimensionExponent 2 ;
  ns2:hasSIMassDimensionExponent 0 ;
  ns2:hasSITimeDimensionExponent -1 ;
  ns2:hasSIElectricCurrentDimensionExponent 0 ;
  ns2:hasSIThermodynamicTemperatureDimensionExponent 0 ;
  ns2:hasSIAmountOfSubstanceDimensionExponent 0 ;
  ns2:hasSILuminousIntensityDimensionExponent 0 .

ns2:powerDensity-Dimension
  a ns2:Dimension ;
  rdfs:label "power density dimension"@en ;
  ns2:hasSILengthDimensionExponent 0 ;
  ns2:hasSIMassDimensionExponent 1 ;
  ns2:hasSITimeDimensionExponent -3 ;
  ns2:hasSIElectricCurrentDimensionExponent 0 ;
  ns2:hasSIThermodynamicTemperatureDimensionExponent 0 ;
  ns2:hasSIAmountOfSubstanceDimensionExponent 0 ;
  ns2:hasSILuminousIntensityDimensionExponent 0 .

ns2:energyDensity-Dimension
  a ns2:Dimension ;
  rdfs:label "energy density dimension"@en ;
  ns2:hasSILengthDimensionExponent -1 ;
  ns2:hasSIMassDimensionExponent 1 ;
  ns2:hasSITimeDimensionExponent -2 ;
  ns2:hasSIElectricCurrentDimensionExponent 0 ;
  ns2:hasSIThermodynamicTemperatureDimensionExponent 0 ;
  ns2:hasSIAmountOfSubstanceDimensionExponent 0 ;
  ns2:hasSILuminousIntensityDimensionExponent 0 .

ns2:actionOrAngularMomentum-Dimension
  a ns2:Dimension ;
  rdfs:label "action or angular momentum dimension"@en ;
  ns2:hasSILengthDimensionExponent 2 ;
  ns2:hasSIMassDimensionExponent 1 ;
  ns2:hasSITimeDimensionExponent -1 ;
  ns2:hasSIElectricCurrentDimensionExponent 0 ;
  ns2:hasSIThermodynamicTemperatureDimensionExponent 0 ;
  ns2:hasSIAmountOfSubstanceDimensionExponent 0 ;
  ns2:hasSILuminousIntensityDimensionExponent 0 .

ns2:fluidity-Dimension
  a ns2:Dimension ;
  rdfs:label "fluidity dimension"@en ;
  ns2:hasSILengthDimensionExponent 1 ;
  ns2:hasSIMassDimensionExponent -1 ;
  ns2:hasSITimeDimensionExponent 1 ;
  ns2:hasSIElectricCurrentDimensionExponent 0 ;
  ns2:hasSIThermodynamicTemperatureDimensionExponent 0 ;
  ns2:hasSIAmountOfSubstanceDimensionExponent 0 ;
  ns2:hasSILuminousIntensityDimensionExponent 0 .

ns2:volumetricFlowRate-Dimension
  a ns2:Dimension ;
  rdfs:label "volumetric flow rate dimension"@en ;
  ns2:hasSILengthDimensionExponent 3 ;
  ns2:hasSIMassDimensionExponent 0 ;
  ns2:hasSITimeDimensionExponent -1 ;
  ns2:hasSIElectricCurrentDimensionExponent 0 ;
  ns2:hasSIThermodynamicTemperatureDimensionExponent 0 ;
  ns2:hasSIAmountOfSubstanceDimensionExponent 0 ;
  ns2:hasSILuminousIntensityDimensionExponent 0 .

ns2:massFlow-Dimension
  a ns2:Dimension ;
  rdfs:label "mass flow dimension"@en ;
  ns2:hasSILengthDimensionExponent 0 ;
  ns2:hasSIMassDimensionExponent 1 ;
  ns2:hasSITimeDimensionExponent -1 ;
  ns2:hasSIElectricCurrentDimensionExponent 0 ;
  ns2:hasSIThermodynamicTemperatureDimensionExponent 0 ;
  ns2:hasSIAmountOfSubstanceDimensionExponent 0 ;
  ns2:hasSILuminousIntensityDimensionExponent 0 .

ns2:thermodynamics
  a ns2:ApplicationArea ;
  rdfs:label "thermodynamics"@en, "thermodynamica"@nl ;
  ns2:usesQuantity ns2:Temperature, ns2:ThermodynamicTemperature, ns2:CelsiusTemperature, ns2:FahrenheitTemperature, ns2:RankineTemperature, ns2:ReaumurTemperature, ns2:Heat, ns2:InternalEnergy, ns2:HeatFluxDensity, ns2:Entropy, ns2:HeatCapacity, ns2:SpecificHeatCapacity, ns2:HeatFlowRate, ns2:SpecificEntropy, ns2:ThermalConductivity, ns2:ThermalResistance, ns2:TemperatureRate, ns2:HeatTransferCoefficient ;
  ns2:usesUnit ns2:kelvin, ns2:attokelvin, ns2:centikelvin, ns2:decakelvin, ns2:decikelvin, ns2:exakelvin, ns2:femtokelvin, ns2:gigakelvin, ns2:hectokelvin, ns2:kilokelvin, ns2:megakelvin, ns2:microkelvin, ns2:millikelvin, ns2:nanokelvin, ns2:petakelvin, ns2:picokelvin, ns2:terakelvin, ns2:degreeCelsius, ns2:attodegreeCelsius, ns2:centidegreeCelsius, ns2:decidegreeCelsius, ns2:femtodegreeCelsius, ns2:microdegreeCelsius, ns2:millidegreeCelsius, ns2:nanodegreeCelsius, ns2:picodegreeCelsius, ns2:degreeFahrenheit, ns2:degreeRankine, ns2:degreeReaumur, ns2:joulePerKelvin, ns2:joulePerKelvinKilogram, ns2:wattPerMetreKelvin, ns2:squareMetreKelvinPerWatt, ns2:degreeCelsiusPerMinute-Time, ns2:wattPerSquareMetreKelvin .

ns2:Temperature
  a owl:Class ;
  rdfs:label "temperature"@en, "temperatuur"@nl, "温度"@zh ;
  rdfs:comment "Temperature is the extent to which an object is hot."@en ;
  ns2:unofficialAbbreviation "temp" ;
  rdfs:subClassOf ns2:Quantity, [
    a owl:Restriction ;
    owl:onProperty ns2:hasScale ;
    owl:allValuesFrom [
      a owl:Class ;
      owl:oneOf (
       ns2:CelsiusScale
       ns2:FahrenheitScale
       ns2:ReaumurScale
       ns2:KelvinScale
       ns2:RankineScale
     )
    ]
  ], [
    a owl:Restriction ;
    owl:onProperty ns2:hasValue ;
    owl:allValuesFrom [
      a owl:Restriction ;
      owl:onProperty ns2:hasUnit ;
      owl:allValuesFrom [
        a owl:Class ;
        owl:unionOf (
         ns2:TemperatureUnit
         ns2:Temperature_scale
       )
      ]
    ]
  ], [
    a owl:Restriction ;
    owl:onProperty ns2:hasDimension ;
    owl:hasValue ns2:thermodynamicTemperature-Dimension
  ] ;
  ns2:symbol "T" ;
  ns2:alternativeSymbol "t", "θ" ;
  ns2:commonlyHasUnit ns2:kelvin, ns2:attokelvin, ns2:centikelvin, ns2:decakelvin, ns2:decikelvin, ns2:exakelvin, ns2:femtokelvin, ns2:gigakelvin, ns2:hectokelvin, ns2:kilokelvin, ns2:megakelvin, ns2:microkelvin, ns2:millikelvin, ns2:nanokelvin, ns2:petakelvin, ns2:picokelvin, ns2:terakelvin, ns2:degreeCelsius, ns2:attodegreeCelsius, ns2:centidegreeCelsius, ns2:decidegreeCelsius, ns2:femtodegreeCelsius, ns2:microdegreeCelsius, ns2:millidegreeCelsius, ns2:nanodegreeCelsius, ns2:picodegreeCelsius, ns2:degreeFahrenheit, ns2:degreeRankine, ns2:degreeReaumur .

ns2:ThermodynamicTemperature
  a owl:Class ;
  rdfs:label "thermodynamic temperature"@en, "absolute temperatuur"@nl ;
  ns2:alternativeLabel "thermodynamische temperatuur"@nl ;
  rdfs:comment "Thermodynamic temperature is the absolute measure of temperature. Its zero point is the temperature at which the particle constituents of matter have minimal motion and can be no colder. Thermodynamic temperature is a base quantity in the International System of Units."@en ;
  rdfs:subClassOf ns2:Temperature, [
    a owl:Restriction ;
    owl:onProperty ns2:hasScale ;
    owl:hasValue ns2:KelvinScale
  ], [
    a owl:Restriction ;
    owl:onProperty ns2:hasValue ;
    owl:allValuesFrom [
      a owl:Restriction ;
      owl:onProperty ns2:hasUnit ;
      owl:allValuesFrom [
        a owl:Class ;
        owl:unionOf (
         ns2:ThermodynamicTemperatureUnit
         ns2:ThermodynamicTemperatureScale
       )
      ]
    ]
  ] ;
  ns2:symbol "T" ;
  ns2:commonlyHasUnit ns2:kelvin, ns2:attokelvin, ns2:centikelvin, ns2:decakelvin, ns2:decikelvin, ns2:exakelvin, ns2:femtokelvin, ns2:gigakelvin, ns2:hectokelvin, ns2:kilokelvin, ns2:megakelvin, ns2:microkelvin, ns2:millikelvin, ns2:nanokelvin, ns2:petakelvin, ns2:picokelvin, ns2:terakelvin .

ns2:CelsiusTemperature
  a owl:Class ;
  rdfs:label "Celsius temperature"@en, "Celsiustemperatuur"@nl ;
  rdfs:subClassOf ns2:Temperature, [
    a owl:Restriction ;
    owl:onProperty ns2:hasScale ;
    owl:hasValue ns2:CelsiusScale
  ], [
    a owl:Restriction ;
    owl:onProperty ns2:hasValue ;
    owl:allValuesFrom [
      a owl:Restriction ;
      owl:onProperty ns2:hasUnit ;
      owl:allValuesFrom [
        a owl:Class ;
        owl:unionOf (
         ns2:CelsiusTemperatureUnit
         ns2:CelsiusTemperatureScale
       )
      ]
    ]
  ] ;
  ns2:symbol "t" ;
  ns2:alternativeSymbol "θ" ;
  ns2:commonlyHasUnit ns2:degreeCelsius, ns2:attodegreeCelsius, ns2:centidegreeCelsius, ns2:decidegreeCelsius, ns2:femtodegreeCelsius, ns2:microdegreeCelsius, ns2:millidegreeCelsius, ns2:nanodegreeCelsius, ns2:picodegreeCelsius .

ns2:FahrenheitTemperature
  a owl:Class ;
  rdfs:label "Fahrenheit temperature"@en, "Fahrenheittemperatuur"@nl ;
  rdfs:subClassOf ns2:Temperature, [
    a owl:Restriction ;
    owl:onProperty ns2:hasScale ;
    owl:hasValue ns2:FahrenheitScale
  ], [
    a owl:Restriction ;
    owl:onProperty ns2:hasValue ;
    owl:allValuesFrom [
      a owl:Restriction ;
      owl:onProperty ns2:hasUnit ;
      owl:allValuesFrom [
        a owl:Class ;
        owl:unionOf (
         ns2:FahrenheitTemperatureUnit
         ns2:FahrenheitTemperatureScale
       )
      ]
    ]
  ] ;
  ns2:symbol "T" ;
  ns2:commonlyHasUnit ns2:degreeFahrenheit .

ns2:RankineTemperature
  a owl:Class ;
  rdfs:label "Rankine temperature"@en, "Rankinetemperatuur"@nl ;
  rdfs:subClassOf ns2:Temperature, [
    a owl:Restriction ;
    owl:onProperty ns2:hasScale ;
    owl:hasValue ns2:RankineScale
  ], [
    a owl:Restriction ;
    owl:onProperty ns2:hasValue ;
    owl:allValuesFrom [
      a owl:Restriction ;
      owl:onProperty ns2:hasUnit ;
      owl:allValuesFrom [
        a owl:Class ;
        owl:unionOf (
         ns2:RankineTemperatureUnit
         ns2:RankineTemperatureScale
       )
      ]
    ]
  ] ;
  ns2:symbol "T" ;
  ns2:commonlyHasUnit ns2:degreeRankine .

ns2:ReaumurTemperature
  a owl:Class ;
  rdfs:label "Réaumur temperature"@en, "Réaumurtemperatuur"@nl ;
  rdfs:subClassOf ns2:Temperature, [
    a owl:Restriction ;
    owl:onProperty ns2:hasScale ;
    owl:hasValue ns2:ReaumurScale
  ], [
    a owl:Restriction ;
    owl:onProperty ns2:hasValue ;
    owl:allValuesFrom [
      a owl:Restriction ;
      owl:onProperty ns2:hasUnit ;
      owl:allValuesFrom [
        a owl:Class ;
        owl:unionOf (
         ns2:ReaumurTemperatureUnit
         ns2:ReaumurTemperatureScale
       )
      ]
    ]
  ] ;
  ns2:symbol "T" ;
  ns2:commonlyHasUnit ns2:degreeReaumur .

ns2:Heat
  a owl:Class ;
  rdfs:label "heat"@en, "warmte"@nl ;
  ns2:alternativeLabel "quantity of heat"@en ;
  rdfs:comment "Heat is any flow of energy from one body or system to another due to a difference in temperature."@en ;
  rdfs:subClassOf ns2:Energy ;
  ns2:symbol "Q" ;
  ns2:commonlyHasUnit ns2:newtonMetre, ns2:micronewtonMetre, ns2:millinewtonMetre, ns2:joule, ns2:attojoule, ns2:centijoule, ns2:decajoule, ns2:decijoule, ns2:exajoule, ns2:femtojoule, ns2:gigajoule, ns2:hectojoule, ns2:kilojoule, ns2:megajoule, ns2:microjoule, ns2:millijoule, ns2:nanojoule, ns2:petajoule, ns2:picojoule, ns2:terajoule, ns2:electronvolt, ns2:gigaelectronvolt, ns2:kiloelectronvolt, ns2:megaelectronvolt, ns2:calorie-Mean, ns2:kilocalorie-Mean, ns2:BritishThermalUnit-39F, ns2:BritishThermalUnit-59F, ns2:BritishThermalUnit-60F, ns2:BritishThermalUnit-InternationalTable, ns2:BritishThermalUnit-Mean, ns2:BritishThermalUnit-Thermochemical, ns2:calorie-15C, ns2:calorie-20C, ns2:calorie-InternationalTable, ns2:calorie-Thermochemical, ns2:erg, ns2:footPoundal, ns2:quad, ns2:wattHour, ns2:kilowattHour, ns2:megawattHour, ns2:gigawattHour, ns2:terawattHour, ns2:therm-EC, ns2:therm-US, ns2:tonOfTNT, ns2:megaerg .

ns2:InternalEnergy
  a owl:Class ;
  rdfs:label "internal energy"@en, "inwendige energie"@nl ;
  rdfs:comment "The internal energy of a thermodynamic system, or a body with well-defined boundaries is the total of the kinetic energy due to the motion of molecules (translational, rotational, vibrational) and the potential energy associated with the vibrational and electric energy of atoms within molecules or crystals."@en ;
  rdfs:subClassOf ns2:Energy ;
  ns2:symbol "U" ;
  ns2:commonlyHasUnit ns2:newtonMetre, ns2:micronewtonMetre, ns2:millinewtonMetre, ns2:joule, ns2:attojoule, ns2:centijoule, ns2:decajoule, ns2:decijoule, ns2:exajoule, ns2:femtojoule, ns2:gigajoule, ns2:hectojoule, ns2:kilojoule, ns2:megajoule, ns2:microjoule, ns2:millijoule, ns2:nanojoule, ns2:petajoule, ns2:picojoule, ns2:terajoule, ns2:electronvolt, ns2:gigaelectronvolt, ns2:kiloelectronvolt, ns2:megaelectronvolt, ns2:calorie-Mean, ns2:kilocalorie-Mean, ns2:BritishThermalUnit-39F, ns2:BritishThermalUnit-59F, ns2:BritishThermalUnit-60F, ns2:BritishThermalUnit-InternationalTable, ns2:BritishThermalUnit-Mean, ns2:BritishThermalUnit-Thermochemical, ns2:calorie-15C, ns2:calorie-20C, ns2:calorie-InternationalTable, ns2:calorie-Thermochemical, ns2:erg, ns2:footPoundal, ns2:quad, ns2:wattHour, ns2:kilowattHour, ns2:megawattHour, ns2:gigawattHour, ns2:terawattHour, ns2:therm-EC, ns2:therm-US, ns2:tonOfTNT, ns2:megaerg .

ns2:HeatFluxDensity
  a owl:Class ;
  rdfs:label "heat flux density"@en ;
  rdfs:subClassOf ns2:PowerDensity ;
  ns2:commonlyHasUnit ns2:wattPerSquareMetre .

ns2:Entropy
  a owl:Class ;
  rdfs:label "entropy"@en, "entropie"@nl, "熵单位"@zh ;
  rdfs:comment "Entropy is a measure of the unavailability of a system’s energy to do work."@en ;
  rdfs:subClassOf ns2:Quantity, [
    a owl:Restriction ;
    owl:onProperty ns2:hasValue ;
    owl:allValuesFrom [
      a owl:Restriction ;
      owl:onProperty ns2:hasUnit ;
      owl:allValuesFrom ns2:EntropyUnit
    ]
  ], [
    a owl:Restriction ;
    owl:onProperty ns2:hasDimension ;
    owl:hasValue ns2:entropyOrHeatCapacity-Dimension
  ] ;
  ns2:symbol "S" ;
  ns2:commonlyHasUnit ns2:joulePerKelvin .

ns2:HeatCapacity
  a owl:Class ;
  rdfs:label "heat capacity"@en, "warmtecapaciteit"@nl, "热容量"@zh ;
  rdfs:comment "Heat capacity is the heat required to increase the temperature of a system or substance one unit temperature."@en ;
  rdfs:subClassOf ns2:Quantity, [
    a owl:Restriction ;
    owl:onProperty ns2:hasValue ;
    owl:allValuesFrom [
      a owl:Restriction ;
      owl:onProperty ns2:hasUnit ;
      owl:allValuesFrom ns2:HeatCapacityUnit
    ]
  ], [
    a owl:Restriction ;
    owl:onProperty ns2:hasDimension ;
    owl:hasValue ns2:entropyOrHeatCapacity-Dimension
  ] ;
  ns2:symbol "C_p" ;
  ns2:alternativeSymbol "C_v" ;
  ns2:commonlyHasUnit ns2:joulePerKelvin .

ns2:SpecificHeatCapacity
  a owl:Class ;
  rdfs:label "specific heat capacity"@en, "soortelijke warmte"@nl ;
  ns2:alternativeLabel "specifieke warmte"@nl, "specifieke warmtecapaciteit"@nl ;
  rdfs:subClassOf ns2:Quantity, [
    a owl:Restriction ;
    owl:onProperty ns2:hasValue ;
    owl:allValuesFrom [
      a owl:Restriction ;
      owl:onProperty ns2:hasUnit ;
      owl:allValuesFrom ns2:SpecificHeatCapacityUnit
    ]
  ], [
    a owl:Restriction ;
    owl:onProperty ns2:hasDimension ;
    owl:hasValue ns2:specificEntropyOrSpecificHeatCapacity-Dimension
  ] ;
  ns2:symbol "c_p" ;
  ns2:alternativeSymbol "c_v" ;
  ns2:commonlyHasUnit ns2:joulePerKelvinKilogram .

ns2:HeatFlowRate
  a owl:Class ;
  rdfs:label "heat flow rate"@en ;
  rdfs:subClassOf ns2:Power ;
  ns2:symbol "Φ" ;
  ns2:alternativeSymbol "q" ;
  ns2:commonlyHasUnit ns2:joulePerSecond-Time, ns2:watt, ns2:attowatt, ns2:centiwatt, ns2:decawatt, ns2:deciwatt, ns2:exawatt, ns2:femtowatt, ns2:gigawatt, ns2:hectowatt, ns2:kilowatt, ns2:megawatt, ns2:microwatt, ns2:milliwatt, ns2:nanowatt, ns2:petawatt, ns2:picowatt, ns2:terawatt, ns2:horsepower-Boiler, ns2:horsepower-British, ns2:horsepower-Electric, ns2:horsepower-Metric, ns2:horsepower-Water, ns2:tonOfRefrigeration, ns2:solarLuminosity .

ns2:SpecificEntropy
  a owl:Class ;
  rdfs:label "specific entropy"@en ;
  rdfs:subClassOf ns2:Quantity, [
    a owl:Restriction ;
    owl:onProperty ns2:hasValue ;
    owl:allValuesFrom [
      a owl:Restriction ;
      owl:onProperty ns2:hasUnit ;
      owl:allValuesFrom ns2:SpecificEntropyUnit
    ]
  ], [
    a owl:Restriction ;
    owl:onProperty ns2:hasDimension ;
    owl:hasValue ns2:specificEntropyOrSpecificHeatCapacity-Dimension
  ] ;
  ns2:commonlyHasUnit ns2:joulePerKelvinKilogram .

ns2:ThermalConductivity
  a owl:Class ;
  rdfs:label "thermal conductivity"@en, "thermische geleidbaarheid"@nl ;
  rdfs:comment "Termal conductivity indicates the ability of a material to conduct heat."@en ;
  rdfs:subClassOf ns2:Quantity, [
    a owl:Restriction ;
    owl:onProperty ns2:hasValue ;
    owl:allValuesFrom [
      a owl:Restriction ;
      owl:onProperty ns2:hasUnit ;
      owl:allValuesFrom ns2:ThermalConductivityUnit
    ]
  ], [
    a owl:Restriction ;
    owl:onProperty ns2:hasDimension ;
    owl:hasValue ns2:thermalConductivity-Dimension
  ] ;
  ns2:symbol "κ" ;
  ns2:alternativeSymbol "k", "K", "λ" ;
  ns2:commonlyHasUnit ns2:wattPerMetreKelvin .

ns2:ThermalDiffusivity
  a owl:Class ;
  rdfs:label "thermal diffusivity"@en ;
  rdfs:subClassOf ns2:Quantity, [
    a owl:Restriction ;
    owl:onProperty ns2:hasValue ;
    owl:allValuesFrom [
      a owl:Restriction ;
      owl:onProperty ns2:hasUnit ;
      owl:allValuesFrom ns2:ThermalDiffusivityUnit
    ]
  ] ;
  ns2:hasDimension ns2:kinematicViscosityOrThermalDiffusivity-Dimension ;
  ns2:commonlyHasUnit ns2:squareMetrePerSecond-Time .

ns2:ThermalDiffusivityUnit
  a owl:Class ;
  rdfs:label "thermal diffusivity unit"@en ;
  rdfs:subClassOf ns2:Unit ;
  owl:equivalentClass [
    a owl:Class ;
    owl:oneOf ( ns2:squareMetrePerSecond-Time )
  ] .

ns2:ThermalInsulance
  a owl:Class ;
  rdfs:label "thermal insulance"@en ;
  rdfs:subClassOf ns2:Quantity, [
    a owl:Restriction ;
    owl:onProperty ns2:hasValue ;
    owl:allValuesFrom [
      a owl:Restriction ;
      owl:onProperty ns2:hasUnit ;
      owl:allValuesFrom ns2:ThermalInsulanceUnit
    ]
  ], [
    a owl:Restriction ;
    owl:onProperty ns2:hasDimension ;
    owl:hasValue ns2:thermalInsulance-Dimension
  ] ;
  ns2:commonlyHasUnit ns2:squareMetreKelvinPerWatt .

ns2:ThermalResistance
  a owl:Class ;
  rdfs:label "thermal resistance"@en ;
  rdfs:subClassOf ns2:Quantity, [
    a owl:Restriction ;
    owl:onProperty ns2:hasValue ;
    owl:allValuesFrom [
      a owl:Restriction ;
      owl:onProperty ns2:hasUnit ;
      owl:allValuesFrom ns2:ThermalResistanceUnit
    ]
  ], [
    a owl:Restriction ;
    owl:onProperty ns2:hasDimension ;
    owl:hasValue ns2:thermalResistance-Dimension
  ] ;
  ns2:commonlyHasUnit ns2:kelvinPerWatt .

ns2:TemperatureRate
  a owl:Class ;
  rdfs:label "temperature rate"@en, "temperatuur-rate"@nl ;
  ns2:unofficialLabel "heating rate" ;
  rdfs:subClassOf ns2:Quantity, [
    a owl:Restriction ;
    owl:onProperty ns2:hasValue ;
    owl:allValuesFrom [
      a owl:Restriction ;
      owl:onProperty ns2:hasUnit ;
      owl:allValuesFrom ns2:TemperatureRateUnit
    ]
  ] ;
  ns2:commonlyHasUnit ns2:degreeCelsiusPerHour, ns2:degreeCelsiusPerMinute-Time, ns2:degreeCelsiusPerSecond-Time .

ns2:HeatTransferCoefficient
  a owl:Class ;
  rdfs:label "heat transfer coefficient"@en ;
  rdfs:subClassOf ns2:Quantity, [
    a owl:Restriction ;
    owl:onProperty ns2:hasValue ;
    owl:allValuesFrom [
      a owl:Restriction ;
      owl:onProperty ns2:hasUnit ;
      owl:allValuesFrom ns2:HeatTransferCoefficientUnit
    ]
  ], [
    a owl:Restriction ;
    owl:onProperty ns2:hasDimension ;
    owl:hasValue ns2:heatTransferCoefficient-Dimension
  ] ;
  ns2:commonlyHasUnit ns2:wattPerSquareMetreKelvin .

ns2:VolumetricHeatCapacity
  a owl:Class ;
  rdfs:label "volumetric heat capacity"@en ;
  rdfs:subClassOf ns2:Quantity, [
    a owl:Restriction ;
    owl:onProperty ns2:hasValue ;
    owl:allValuesFrom [
      a owl:Restriction ;
      owl:onProperty ns2:hasUnit ;
      owl:allValuesFrom ns2:VolumetricHeatCapacityUnit
    ]
  ], [
    a owl:Restriction ;
    owl:onProperty ns2:hasDimension ;
    owl:hasValue ns2:volumetricHeatCapacity-Dimension
  ] ;
  ns2:commonlyHasUnit ns2:joulePerCubicMetreKelvin .

ns2:kelvin
  a ns2:Unit, ns2:SingularUnit ;
  rdfs:label "kelvin"@en, "kelvin"@nl, "开"@zh ;
  ns2:symbol "K" ;
  ns2:hasDimension ns2:thermodynamicTemperature-Dimension ;
  rdfs:comment "The kelvin is a unit of temperature defined as 1/273.16 of the thermodynamic temperature of the triple point of water."@en ;
  ns2:longcomment "The kelvin is a unit of temperature defined as 1/273.16 of the thermodynamic temperature of the triple point of water. The kelvin is a base unit in the International System of Units." ;
  ns2:hasQuantity ns2:_127316OfTheThermodynamicTemperatureOfTheTriplePointOfWater .

ns2:triplePointOfWater
  a owl:Thing ;
  rdfs:label "triple point of water"@en .

ns2:_127316OfTheThermodynamicTemperatureOfTheTriplePointOfWater
  a ns2:ThermodynamicTemperature ;
  rdfs:label "1/273.16 of the thermodynamic temperature of the triple point of water"@en .

ns2:ThermodynamicTemperatureUnit
  a owl:Class ;
  rdfs:label "thermodynamic temperature unit"@en ;
  rdfs:subClassOf ns2:TemperatureUnit ;
  owl:equivalentClass [
    a owl:Class ;
    owl:unionOf (
     _:genid904
     ns2:PrefixedKelvin
   )
  ] .

ns2:PrefixedKelvin
  a owl:Class ;
  rdfs:label "prefixed kelvin"@en ;
  rdfs:subClassOf ns2:PrefixedUnit ;
  owl:equivalentClass [
    a owl:Class ;
    owl:intersectionOf (
     _:genid919
     _:genid921
     _:genid923
     _:genid925
   )
  ] .

ns2:TemperatureUnit
  a owl:Class ;
  rdfs:label "temperature unit"@en ;
  rdfs:subClassOf ns2:Unit ;
  owl:equivalentClass [
    a owl:Class ;
    owl:unionOf (
     _:genid909
     ns2:PrefixedDegreeCelsius
     ns2:PrefixedKelvin
   )
  ] .

ns2:degreeCelsius
  a ns2:Unit, ns2:SingularUnit ;
  rdfs:label "degree Celsius"@en, "graad Celsius"@nl, "摄氏度"@zh ;
  ns2:alternativeLabel "centigrade"@en ;
  rdfs:comment "The degree Celsius is a unit of temperature defined as 1 kelvin."@en ;
  ns2:longcomment "The degree Celsius is a unit of temperature defined as 1 kelvin. The degree Celsius is a derived unit in the International System of Units." ;
  ns2:symbol "°C" ;
  ns2:hasUnit ns2:kelvin ;
  ns2:hasDimension ns2:thermodynamicTemperature-Dimension .

ns2:degreeFahrenheit
  a ns2:Unit, ns2:SingularUnit ;
  rdfs:label "degree Fahrenheit"@en, "graad Fahrenheit"@nl ;
  rdfs:comment "The degree Fahrenheit is a unit of temperature defined as 5.555556e-1 kelvin."@en ;
  ns2:symbol "°F" ;
  ns2:hasFactor "5.555556e-1"^^xsd:float ;
  ns2:hasUnit ns2:kelvin ;
  ns2:hasDimension ns2:thermodynamicTemperature-Dimension .

ns2:degreeRankine
  a ns2:Unit, ns2:SingularUnit ;
  rdfs:label "degree Rankine"@en, "graad Rankine"@nl ;
  rdfs:comment "The degree Rankine is a unit of temperature defined as 5.555556e-1 kelvin."@en ;
  ns2:symbol "°R" ;
  ns2:alternativeSymbol "°Ra" ;
  ns2:hasFactor "5.555556e-1"^^xsd:float ;
  ns2:hasUnit ns2:kelvin ;
  ns2:hasDimension ns2:thermodynamicTemperature-Dimension .

ns2:degreeReaumur
  a ns2:Unit, ns2:SingularUnit ;
  rdfs:label "degree Réaumur"@en, "graad Réaumur"@nl ;
  rdfs:comment "The degree Réaumur is a unit of temperature defined as 1.25 kelvin."@en ;
  ns2:symbol "°Ré" ;
  ns2:alternativeSymbol "°Re", "°R" ;
  ns2:hasFactor "1.25"^^xsd:float ;
  ns2:hasUnit ns2:kelvin ;
  ns2:hasDimension ns2:thermodynamicTemperature-Dimension .

ns2:PrefixedDegreeCelsius
  a owl:Class ;
  rdfs:label "prefixed degree Celsius"@en ;
  rdfs:subClassOf ns2:PrefixedUnit ;
  owl:equivalentClass [
    a owl:Class ;
    owl:intersectionOf (
     _:genid933
     _:genid935
     _:genid937
     _:genid939
   )
  ] .

ns2:yoctokelvin
  a ns2:PrefixedUnit ;
  rdfs:label "yoctokelvin"@en, "yoctokelvin"@nl ;
  rdfs:comment "The yoctokelvin is a unit of temperature defined as 1.0e-24 kelvin."@en ;
  ns2:symbol "yK" ;
  ns2:hasPrefix ns2:yocto ;
  ns2:hasUnit ns2:kelvin ;
  ns2:hasDimension ns2:thermodynamicTemperature-Dimension .

ns2:zeptokelvin
  a ns2:PrefixedUnit ;
  rdfs:label "zeptokelvin"@en, "zeptokelvin"@nl ;
  rdfs:comment "The zeptkelvin is a unit of temperature defined as 1.0e-21 kelvin."@en ;
  ns2:symbol "zK" ;
  ns2:hasPrefix ns2:zepto ;
  ns2:hasUnit ns2:kelvin ;
  ns2:hasDimension ns2:thermodynamicTemperature-Dimension .

ns2:attokelvin
  a ns2:PrefixedUnit ;
  rdfs:label "attokelvin"@en, "attokelvin"@nl ;
  rdfs:comment "The attokelvin is a unit of temperature defined as 1.0e-18 kelvin."@en ;
  ns2:symbol "aK" ;
  ns2:hasPrefix ns2:atto ;
  ns2:hasUnit ns2:kelvin ;
  ns2:hasDimension ns2:thermodynamicTemperature-Dimension .

ns2:femtokelvin
  a ns2:PrefixedUnit ;
  rdfs:label "femtokelvin"@en, "femtokelvin"@nl ;
  rdfs:comment "The femtokelvin is a unit of temperature defined as 1.0e-15 kelvin."@en ;
  ns2:symbol "fK" ;
  ns2:hasPrefix ns2:femto ;
  ns2:hasUnit ns2:kelvin ;
  ns2:hasDimension ns2:thermodynamicTemperature-Dimension .

ns2:picokelvin
  a ns2:PrefixedUnit ;
  rdfs:label "picokelvin"@en, "picokelvin"@nl ;
  rdfs:comment "The picokelvin is a unit of temperature defined as 1.0e-12 kelvin."@en ;
  ns2:symbol "pK" ;
  ns2:hasPrefix ns2:pico ;
  ns2:hasUnit ns2:kelvin ;
  ns2:hasDimension ns2:thermodynamicTemperature-Dimension .

ns2:nanokelvin
  a ns2:PrefixedUnit ;
  rdfs:label "nanokelvin"@en, "nanokelvin"@nl ;
  rdfs:comment "The nanokelvin is a unit of temperature defined as 1.0e-9 kelvin."@en ;
  ns2:symbol "nK" ;
  ns2:hasPrefix ns2:nano ;
  ns2:hasUnit ns2:kelvin ;
  ns2:hasDimension ns2:thermodynamicTemperature-Dimension .

ns2:microkelvin
  a ns2:PrefixedUnit ;
  rdfs:label "microkelvin"@en, "microkelvin"@nl ;
  rdfs:comment "The microkelvin is a unit of temperature defined as 1.0e-6 kelvin."@en ;
  ns2:symbol "μK" ;
  ns2:hasPrefix ns2:micro ;
  ns2:hasUnit ns2:kelvin ;
  ns2:hasDimension ns2:thermodynamicTemperature-Dimension .

ns2:millikelvin
  a ns2:PrefixedUnit ;
  rdfs:label "millikelvin"@en, "millikelvin"@nl ;
  rdfs:comment "The millikelvin is a unit of temperature defined as 1.0e-3 kelvin."@en ;
  ns2:symbol "mK" ;
  ns2:hasPrefix ns2:milli ;
  ns2:hasUnit ns2:kelvin ;
  ns2:hasDimension ns2:thermodynamicTemperature-Dimension .

ns2:centikelvin
  a ns2:PrefixedUnit ;
  rdfs:label "centikelvin"@en, "centikelvin"@nl ;
  rdfs:comment "The centikelvin is a unit of temperature defined as 1.0e-2 kelvin."@en ;
  ns2:symbol "cK" ;
  ns2:hasPrefix ns2:centi ;
  ns2:hasUnit ns2:kelvin ;
  ns2:hasDimension ns2:thermodynamicTemperature-Dimension .

ns2:decikelvin
  a ns2:PrefixedUnit ;
  rdfs:label "decikelvin"@en, "decikelvin"@nl ;
  rdfs:comment "The decikelvin is a unit of temperature defined as 1.0e-1 kelvin."@en ;
  ns2:symbol "dK" ;
  ns2:hasPrefix ns2:deci ;
  ns2:hasUnit ns2:kelvin ;
  ns2:hasDimension ns2:thermodynamicTemperature-Dimension .

ns2:decakelvin
  a ns2:PrefixedUnit ;
  rdfs:label "decakelvin"@en, "decakelvin"@nl ;
  rdfs:comment "The decakelvin is a unit of thermodynamic temperature defined as 1.0e1 kelvin."@en ;
  ns2:symbol "daK" ;
  ns2:hasPrefix ns2:deca ;
  ns2:hasUnit ns2:kelvin ;
  ns2:hasDimension ns2:thermodynamicTemperature-Dimension .

ns2:hectokelvin
  a ns2:PrefixedUnit ;
  rdfs:label "hectokelvin"@en, "hectokelvin"@nl ;
  rdfs:comment "The hectokelvin is a unit of thermodynamic temperature defined as 1.0e2 kelvin."@en ;
  ns2:symbol "hK" ;
  ns2:hasPrefix ns2:hecto ;
  ns2:hasUnit ns2:kelvin ;
  ns2:hasDimension ns2:thermodynamicTemperature-Dimension .

ns2:kilokelvin
  a ns2:PrefixedUnit ;
  rdfs:label "kilokelvin"@en, "kilokelvin"@nl ;
  rdfs:comment "The kilokelvin is a unit of thermodynamic temperature defined as 1.0e3 kelvin."@en ;
  ns2:symbol "kK" ;
  ns2:hasPrefix ns2:kilo ;
  ns2:hasUnit ns2:kelvin ;
  ns2:hasDimension ns2:thermodynamicTemperature-Dimension .

ns2:megakelvin
  a ns2:PrefixedUnit ;
  rdfs:label "megakelvin"@en, "megakelvin"@nl ;
  rdfs:comment "The megakelvin is a unit of thermodynamic temperature defined as 1.0e6 kelvin."@en ;
  ns2:symbol "MK" ;
  ns2:hasPrefix ns2:mega ;
  ns2:hasUnit ns2:kelvin ;
  ns2:hasDimension ns2:thermodynamicTemperature-Dimension .

ns2:gigakelvin
  a ns2:PrefixedUnit ;
  rdfs:label "gigakelvin"@en, "gigakelvin"@nl ;
  rdfs:comment "The gigakelvin is a unit of thermodynamic temperature defined as 1.0e9 kelvin."@en ;
  ns2:symbol "GK" ;
  ns2:hasPrefix ns2:giga ;
  ns2:hasUnit ns2:kelvin ;
  ns2:hasDimension ns2:thermodynamicTemperature-Dimension .

ns2:terakelvin
  a ns2:PrefixedUnit ;
  rdfs:label "terakelvin"@en, "terakelvin"@nl ;
  rdfs:comment "The terakelvin is a unit of thermodynamic temperature defined as 1.0e12 kelvin."@en ;
  ns2:symbol "TK" ;
  ns2:hasPrefix ns2:tera ;
  ns2:hasUnit ns2:kelvin ;
  ns2:hasDimension ns2:thermodynamicTemperature-Dimension .

ns2:petakelvin
  a ns2:PrefixedUnit ;
  rdfs:label "petakelvin"@en, "petakelvin"@nl ;
  rdfs:comment "The petakelvin is a unit of thermodynamic temperature defined as 1.0e15 kelvin."@en ;
  ns2:symbol "PK" ;
  ns2:hasPrefix ns2:peta ;
  ns2:hasUnit ns2:kelvin ;
  ns2:hasDimension ns2:thermodynamicTemperature-Dimension .

ns2:exakelvin
  a ns2:PrefixedUnit ;
  rdfs:label "exakelvin"@en, "exakelvin"@nl ;
  rdfs:comment "The exakelvin is a unit of thermodynamic temperature defined as 1.0e18 kelvin."@en ;
  ns2:symbol "EK" ;
  ns2:hasPrefix ns2:exa ;
  ns2:hasUnit ns2:kelvin ;
  ns2:hasDimension ns2:thermodynamicTemperature-Dimension .

ns2:zettakelvin
  a ns2:PrefixedUnit ;
  rdfs:label "zettakelvin"@en, "zettakelvin"@nl ;
  rdfs:comment "The zettakelvin is a unit of thermodynamic temperature defined as 1.0e21 kelvin."@en ;
  ns2:symbol "ZK" ;
  ns2:hasPrefix ns2:zetta ;
  ns2:hasUnit ns2:kelvin ;
  ns2:hasDimension ns2:thermodynamicTemperature-Dimension .

ns2:yottakelvin
  a ns2:PrefixedUnit ;
  rdfs:label "yottakelvin"@en, "yottakelvin"@nl ;
  rdfs:comment "The yottakelvin is a unit of thermodynamic temperature defined as 1.0e24 kelvin."@en ;
  ns2:symbol "YK" ;
  ns2:hasPrefix ns2:yotta ;
  ns2:hasUnit ns2:kelvin ;
  ns2:hasDimension ns2:thermodynamicTemperature-Dimension .

ns2:CelsiusTemperatureUnit
  a owl:Class ;
  rdfs:label "Celsius temperature unit"@en ;
  rdfs:subClassOf ns2:TemperatureUnit ;
  owl:equivalentClass [
    a owl:Class ;
    owl:unionOf (
     _:genid928
     ns2:PrefixedDegreeCelsius
   )
  ] .

ns2:yoctodegreeCelsius
  a ns2:PrefixedUnit ;
  rdfs:label "yoctodegree Celsius"@en, "yoctograad Celsius"@nl ;
  rdfs:comment "The yoctodegree Celsius is a unit of temperature defined as 1.0e-24 degree Celsius."@en ;
  ns2:symbol "y°C" ;
  ns2:hasPrefix ns2:yocto ;
  ns2:hasUnit ns2:degreeCelsius ;
  ns2:hasDimension ns2:thermodynamicTemperature-Dimension .

ns2:zeptodegreeCelsius
  a ns2:PrefixedUnit ;
  rdfs:label "zeptodegree Celsius"@en, "zeptograad Celsius"@nl ;
  rdfs:comment "The zeptdegree Celsius is a unit of temperature defined as 1.0e-21 degree Celsius."@en ;
  ns2:symbol "z°C" ;
  ns2:hasPrefix ns2:zepto ;
  ns2:hasUnit ns2:degreeCelsius ;
  ns2:hasDimension ns2:thermodynamicTemperature-Dimension .

ns2:attodegreeCelsius
  a ns2:PrefixedUnit ;
  rdfs:label "attodegree Celsius"@en, "attograad Celsius"@nl ;
  rdfs:comment "The attodegree Celsius is a unit of temperature defined as 1.0e-18 degree Celsius."@en ;
  ns2:symbol "a°C" ;
  ns2:hasPrefix ns2:atto ;
  ns2:hasUnit ns2:degreeCelsius ;
  ns2:hasDimension ns2:thermodynamicTemperature-Dimension .

ns2:femtodegreeCelsius
  a ns2:PrefixedUnit ;
  rdfs:label "femtodegree Celsius"@en, "femtograad Celsius"@nl ;
  rdfs:comment "The femtodegree Celsius is a unit of temperature defined as 1.0e-15 degree Celsius."@en ;
  ns2:symbol "f°C" ;
  ns2:hasPrefix ns2:femto ;
  ns2:hasUnit ns2:degreeCelsius ;
  ns2:hasDimension ns2:thermodynamicTemperature-Dimension .

ns2:picodegreeCelsius
  a ns2:PrefixedUnit ;
  rdfs:label "picodegree Celsius"@en, "picograad Celsius"@nl ;
  rdfs:comment "The picodegree Celsius is a unit of temperature defined as 1.0e-12 degree Celsius."@en ;
  ns2:symbol "p°C" ;
  ns2:hasPrefix ns2:pico ;
  ns2:hasUnit ns2:degreeCelsius ;
  ns2:hasDimension ns2:thermodynamicTemperature-Dimension .

ns2:nanodegreeCelsius
  a ns2:PrefixedUnit ;
  rdfs:label "nanodegree Celsius"@en, "nanograad Celsius"@nl ;
  rdfs:comment "The nanodegree Celsius is a unit of temperature defined as 1.0e-9 degree Celsius."@en ;
  ns2:symbol "n°C" ;
  ns2:hasPrefix ns2:nano ;
  ns2:hasUnit ns2:degreeCelsius ;
  ns2:hasDimension ns2:thermodynamicTemperature-Dimension .

ns2:microdegreeCelsius
  a ns2:PrefixedUnit ;
  rdfs:label "microdegree Celsius"@en, "micrograad Celsius"@nl ;
  rdfs:comment "The microdegree Celsius is a unit of temperature defined as 1.0e-6 degree Celsius."@en ;
  ns2:symbol "μ°C" ;
  ns2:hasPrefix ns2:micro ;
  ns2:hasUnit ns2:degreeCelsius ;
  ns2:hasDimension ns2:thermodynamicTemperature-Dimension .

ns2:millidegreeCelsius
  a ns2:PrefixedUnit ;
  rdfs:label "millidegree Celsius"@en, "milligraad Celsius"@nl ;
  rdfs:comment "The millidegree Celsius is a unit of temperature defined as 1.0e-3 degree Celsius."@en ;
  ns2:symbol "m°C" ;
  ns2:hasPrefix ns2:milli ;
  ns2:hasUnit ns2:degreeCelsius ;
  ns2:hasDimension ns2:thermodynamicTemperature-Dimension .

ns2:centidegreeCelsius
  a ns2:PrefixedUnit ;
  rdfs:label "centidegree Celsius"@en, "centigraad Celsius"@nl ;
  rdfs:comment "The centidegree Celsius is a unit of temperature defined as 1.0e-2 degree Celsius."@en ;
  ns2:symbol "c°C" ;
  ns2:hasPrefix ns2:centi ;
  ns2:hasUnit ns2:degreeCelsius ;
  ns2:hasDimension ns2:thermodynamicTemperature-Dimension .

ns2:decidegreeCelsius
  a ns2:PrefixedUnit ;
  rdfs:label "decidegree Celsius"@en, "decigraad Celsius"@nl ;
  rdfs:comment "The decidegree Celsius is a unit of temperature defined as 1.0e-1 degree Celsius."@en ;
  ns2:symbol "d°C" ;
  ns2:hasPrefix ns2:deci ;
  ns2:hasUnit ns2:degreeCelsius ;
  ns2:hasDimension ns2:thermodynamicTemperature-Dimension .

ns2:FahrenheitTemperatureUnit
  a owl:Class ;
  rdfs:label "Fahrenheit temperature unit"@en ;
  rdfs:subClassOf ns2:TemperatureUnit ;
  owl:equivalentClass [
    a owl:Class ;
    owl:unionOf ( _:genid942 )
  ] .

ns2:RankineTemperatureUnit
  a owl:Class ;
  rdfs:label "Rankine temperature unit"@en ;
  rdfs:subClassOf ns2:TemperatureUnit ;
  owl:equivalentClass [
    a owl:Class ;
    owl:unionOf ( _:genid946 )
  ] .

ns2:ReaumurTemperatureUnit
  a owl:Class ;
  rdfs:label "Réaumur temperature unit"@en ;
  rdfs:subClassOf ns2:TemperatureUnit ;
  owl:equivalentClass [
    a owl:Class ;
    owl:unionOf ( _:genid950 )
  ] .

ns2:joulePerKelvin
  a ns2:UnitDivision ;
  rdfs:label "joule per kelvin"@en, "joule per kelvin"@nl ;
  ns2:symbol "J/K" ;
  ns2:alternativeSymbol "J K-1", "J·K-1" ;
  ns2:hasNumerator ns2:joule ;
  ns2:hasDenominator ns2:kelvin ;
  ns2:hasDimension ns2:entropyOrHeatCapacity-Dimension .

ns2:EntropyUnit
  a owl:Class ;
  rdfs:label "entropy unit"@en ;
  rdfs:subClassOf ns2:Unit ;
  owl:equivalentClass [
    a owl:Class ;
    owl:oneOf ( ns2:joulePerKelvin )
  ] .

ns2:HeatCapacityUnit
  a owl:Class ;
  rdfs:label "heat capacity unit"@en ;
  rdfs:subClassOf ns2:Unit ;
  owl:equivalentClass [
    a owl:Class ;
    owl:oneOf ( ns2:joulePerKelvin )
  ] .

ns2:joulePerKelvinKilogram
  a ns2:UnitDivision ;
  rdfs:label "joule per kelvin kilogram"@en, "joule per kelvin kilogram"@nl ;
  ns2:symbol "J/(K kg)" ;
  ns2:alternativeSymbol "J/(K·kg)", "J K-1 kg-1", "J·K-1·kg-1" ;
  ns2:hasNumerator ns2:joule ;
  ns2:hasDenominator ns2:kelvinKilogram ;
  ns2:hasDimension ns2:specificEntropyOrSpecificHeatCapacity-Dimension .

ns2:SpecificEntropyUnit
  a owl:Class ;
  rdfs:label "specific entropy unit"@en ;
  rdfs:subClassOf ns2:Unit ;
  owl:equivalentClass [
    a owl:Class ;
    owl:oneOf ( ns2:joulePerKelvinKilogram )
  ] .

ns2:SpecificHeatCapacityUnit
  a owl:Class ;
  rdfs:label "specific heat capacity unit"@en ;
  rdfs:subClassOf ns2:Unit ;
  owl:equivalentClass [
    a owl:Class ;
    owl:oneOf ( ns2:joulePerKelvinKilogram )
  ] .

ns2:wattPerMetreKelvin
  a ns2:UnitDivision ;
  rdfs:label "watt per metre kelvin"@en, "watt per meter kelvin"@nl ;
  ns2:symbol "W/(m K)" ;
  ns2:alternativeSymbol "W/(m·K)", "W m-1 K-1", "W·m-1·K-1" ;
  ns2:hasNumerator ns2:watt ;
  ns2:hasDenominator ns2:metreKelvin ;
  ns2:hasDimension ns2:thermalConductivity-Dimension .

ns2:ThermalConductivityUnit
  a owl:Class ;
  rdfs:label "thermal conductivity unit"@en ;
  rdfs:subClassOf ns2:Unit ;
  owl:equivalentClass [
    a owl:Class ;
    owl:oneOf ( ns2:wattPerMetreKelvin )
  ] .

ns2:squareMetreKelvin
  a ns2:UnitMultiplication ;
  rdfs:label "square metre kelvin"@en, "vierkante meter kelvin"@nl ;
  ns2:symbol "m2 K" ;
  ns2:alternativeSymbol "m2·K" ;
  ns2:hasTerm1 ns2:squareMetre ;
  ns2:hasTerm2 ns2:kelvin .

ns2:squareMetreKelvinPerWatt
  a ns2:UnitDivision ;
  rdfs:label "square metre kelvin per watt"@en, "vierkante meter kelvin per watt"@nl ;
  ns2:symbol "m2 K/W" ;
  ns2:alternativeSymbol "m2·K/W", "m2 K W-1", "m2·K·W-1" ;
  ns2:hasNumerator ns2:squareMetreKelvin ;
  ns2:hasDenominator ns2:watt ;
  ns2:hasDimension ns2:thermalInsulance-Dimension .

ns2:ThermalInsulanceUnit
  a owl:Class ;
  rdfs:label "thermal insulance unit"@en ;
  rdfs:subClassOf ns2:Unit ;
  owl:equivalentClass [
    a owl:Class ;
    owl:oneOf ( ns2:squareMetreKelvinPerWatt )
  ] .

ns2:kelvinPerWatt
  a ns2:UnitDivision ;
  rdfs:label "kelvin per watt"@en, "kelvin per watt"@nl ;
  ns2:symbol "K/W" ;
  ns2:alternativeSymbol "K W-1", "K·W-1" ;
  ns2:hasNumerator ns2:kelvin ;
  ns2:hasDenominator ns2:watt ;
  ns2:hasDimension ns2:thermalResistance-Dimension .

ns2:ThermalResistanceUnit
  a owl:Class ;
  rdfs:label "thermal resistance unit"@en ;
  rdfs:subClassOf ns2:Unit ;
  owl:equivalentClass [
    a owl:Class ;
    owl:oneOf ( ns2:kelvinPerWatt )
  ] .

ns2:wattPerSquareMetreKelvin
  a ns2:UnitDivision ;
  rdfs:label "watt per square metre kelvin"@en, "watt per vierkante meter kelvin"@nl ;
  ns2:symbol "W/m2 K" ;
  ns2:alternativeSymbol "W/(m2·K)", "W-1 m2 K", "W-1·m2·K" ;
  ns2:hasNumerator ns2:watt ;
  ns2:hasDenominator ns2:squareMetreKelvin ;
  ns2:hasDimension ns2:heatTransferCoefficient-Dimension .

ns2:HeatTransferCoefficientUnit
  a owl:Class ;
  rdfs:label "heat transfer coefficient unit"@en ;
  rdfs:subClassOf ns2:Unit ;
  owl:equivalentClass [
    a owl:Class ;
    owl:oneOf ( ns2:wattPerSquareMetreKelvin )
  ] .

ns2:degreeCelsiusPerHour
  a ns2:UnitDivision ;
  rdfs:label "degree Celsius per hour"@en, "graad Celsius per uur"@nl ;
  ns2:symbol "°C/h" ;
  ns2:alternativeSymbol "°C h-1", "°C·h-1" ;
  ns2:hasNumerator ns2:degreeCelsius ;
  ns2:hasDenominator ns2:hour .

ns2:degreeCelsiusPerMinute-Time
  a ns2:UnitDivision ;
  rdfs:label "degree Celsius per minute"@en, "graad Celsius per minuut"@nl ;
  ns2:symbol "°C/min" ;
  ns2:alternativeSymbol "°C min-1", "°C·min-1" ;
  ns2:hasNumerator ns2:degreeCelsius ;
  ns2:hasDenominator ns2:minute-Time .

ns2:degreeCelsiusPerSecond-Time
  a ns2:UnitDivision ;
  rdfs:label "degree Celsius per second"@en, "graad Celsius per seconde"@nl ;
  ns2:symbol "°C/s" ;
  ns2:alternativeSymbol "°C s-1", "°C·s-1" ;
  ns2:hasNumerator ns2:degreeCelsius ;
  ns2:hasDenominator ns2:second-Time .

ns2:TemperatureRateUnit
  a owl:Class ;
  rdfs:label "temperature rate unit"@en ;
  rdfs:subClassOf ns2:Unit ;
  owl:equivalentClass [
    a owl:Class ;
    owl:oneOf (
     ns2:degreeCelsiusPerHour
     ns2:degreeCelsiusPerMinute-Time
     ns2:degreeCelsiusPerSecond-Time
   )
  ] .

ns2:kelvinKilogram
  a ns2:UnitMultiplication ;
  rdfs:label "kelvin kilogram"@en, "kelvin kilogram"@nl ;
  ns2:symbol "K kg" ;
  ns2:alternativeSymbol "K·kg" ;
  ns2:hasTerm1 ns2:kelvin ;
  ns2:hasTerm2 ns2:kilogram .

ns2:metreKelvin
  a ns2:UnitMultiplication ;
  rdfs:label "metre kelvin"@en, "meter kelvin"@nl ;
  ns2:symbol "m K" ;
  ns2:alternativeSymbol "m·K" ;
  ns2:hasTerm1 ns2:metre ;
  ns2:hasTerm2 ns2:kelvin .

ns2:pascalSecond-TimeSquareMetre
  a ns2:UnitMultiplication ;
  rdfs:label "pascal second square metre"@en, "pascal seconde vierkante meter"@nl ;
  ns2:symbol "Pa s m2" ;
  ns2:alternativeSymbol "Pa·s·m2" ;
  ns2:hasTerm1 ns2:pascalSecond-Time ;
  ns2:hasTerm2 ns2:squareMetre .

ns2:reciprocalAtmosphere-Standard
  a ns2:UnitExponentiation ;
  rdfs:label "reciprocal atmosphere (standard)"@en, "omgekeerde atmosfeer (standaard)"@nl ;
  ns2:symbol "atm-1" ;
  ns2:hasBase ns2:atmosphere-Standard ;
  ns2:hasExponent -1 .

ns2:degreeCelsiusDay
  a ns2:UnitMultiplication ;
  rdfs:label "degree Celsius day"@en, "graad Celsius dag"@nl ;
  ns2:symbol "°C d" ;
  ns2:alternativeSymbol "°C·d" ;
  ns2:hasTerm1 ns2:degreeCelsius ;
  ns2:hasTerm2 ns2:day .

ns2:reciprocalKelvin
  a ns2:UnitExponentiation ;
  rdfs:label "reciprocal kelvin"@en, "omgekeerde kelvin"@nl ;
  ns2:symbol "K-1" ;
  ns2:hasBase ns2:kelvin ;
  ns2:hasExponent -1 .

ns2:reciprocalDegreeCelsius
  a ns2:UnitExponentiation ;
  rdfs:label "reciprocal degree Celsius"@en, "omgekeerde graad Celsius"@nl ;
  ns2:symbol "°C-1" ;
  ns2:hasBase ns2:degreeCelsius ;
  ns2:hasExponent -1 .

ns2:reciprocalDegreeCelsiusDay
  a ns2:UnitExponentiation ;
  rdfs:label "reciprocal degree Celsius day"@en, "omgekeerde graad Celsius dag"@nl ;
  ns2:symbol "(°C d)-1" ;
  ns2:hasBase ns2:degreeCelsiusDay ;
  ns2:hasExponent -1 .

ns2:cubicMetreKelvin
  a ns2:UnitMultiplication ;
  rdfs:label "cubic metre kelvin"@en ;
  ns2:symbol "m3 K" ;
  ns2:alternativeSymbol "m3·K" ;
  ns2:hasTerm1 ns2:cubicMetre ;
  ns2:hasTerm2 ns2:kelvin .

ns2:joulePerCubicMetreKelvin
  a ns2:UnitDivision ;
  rdfs:label "joule per cubic metre kelvin"@en, "joule per kubieke meter kelvin"@nl ;
  ns2:symbol "J/m3 K" ;
  ns2:alternativeSymbol "J/(m3·K)", "J-1 m3 K", "J-1·m3·K" ;
  ns2:hasNumerator ns2:joule ;
  ns2:hasDenominator ns2:cubicMetreKelvin ;
  ns2:hasDimension ns2:volumetricHeatCapacity-Dimension .

ns2:VolumetricHeatCapacityUnit
  a owl:Class ;
  rdfs:label "volumetric heat capacity unit"@en ;
  rdfs:subClassOf ns2:Unit ;
  owl:equivalentClass [
    a owl:Class ;
    owl:oneOf ( ns2:joulePerCubicMetreKelvin )
  ] .

ns2:KelvinScale
  a ns2:RatioScale ;
  rdfs:label "Kelvin scale"@en, "Kelvinschaal"@nl, "开氏温标"@zh ;
  ns2:alternativeLabel "International Kelvin Temperature scale of 1990"@en ;
  ns2:hasDimension ns2:thermodynamicTemperature-Dimension ;
  ns2:hasPoint ns2:_3To5OnTheKelvinScale, ns2:_13.8033OnTheKelvinScale, ns2:approximately17OnTheKelvinScale, ns2:approximately203OnTheKelvinScale, ns2:_24.5561OnTheKelvinScale, ns2:_54.3584OnTheKelvinScale, ns2:_83.8058OnTheKelvinScale, ns2:_234.3156OnTheKelvinScale, ns2:_273.16OnTheKelvinScale, ns2:_302.9146OnTheKelvinScale, ns2:_429.7485OnTheKelvinScale, ns2:_505.078OnTheKelvinScale, ns2:_692.677OnTheKelvinScale, ns2:_933.473OnTheKelvinScale, ns2:_1234.93OnTheKelvinScale, ns2:_1337.33OnTheKelvinScale, ns2:_1357.77OnTheKelvinScale ;
  ns2:hasUnit ns2:kelvin .

ns2:thermodynamicTemperatureOfTheTriplePointOfWater
  a ns2:ThermodynamicTemperature ;
  rdfs:label "triple point of water thermodynamic temperature"@en ;
  ns2:hasPhenomenon ns2:triplePointOfWater .

ns2:_3To5OnTheKelvinScale
  a ns2:FixedPoint ;
  rdfs:label "3 to 5 on the Kelvin scale"@en ;
  ns2:hasNumericalValue "3 to 5" ;
  ns2:hasScale ns2:KelvinScale .

ns2:_13.8033OnTheKelvinScale
  a ns2:FixedPoint ;
  rdfs:label "13.8033 on the Kelvin scale"@en ;
  ns2:hasNumericalValue "13.8033" ;
  ns2:hasScale ns2:KelvinScale .

ns2:approximately17OnTheKelvinScale
  a ns2:FixedPoint ;
  rdfs:label "~17 on the Kelvin scale"@en ;
  ns2:hasNumericalValue "~17" ;
  ns2:hasScale ns2:KelvinScale .

ns2:approximately203OnTheKelvinScale
  a ns2:FixedPoint ;
  rdfs:label "~20.3 on the Kelvin scale"@en ;
  ns2:hasNumericalValue "~20.3" ;
  ns2:hasScale ns2:KelvinScale .

ns2:_24.5561OnTheKelvinScale
  a ns2:FixedPoint ;
  rdfs:label "24.5561 on the Kelvin scale"@en ;
  ns2:hasNumericalValue "24.5561" ;
  ns2:hasScale ns2:KelvinScale .

ns2:_54.3584OnTheKelvinScale
  a ns2:FixedPoint ;
  rdfs:label "54.3584 on the Kelvin scale"@en ;
  ns2:hasNumericalValue "54.3584" ;
  ns2:hasScale ns2:KelvinScale .

ns2:_83.8058OnTheKelvinScale
  a ns2:FixedPoint ;
  rdfs:label "83.8058 on the Kelvin scale"@en ;
  ns2:hasNumericalValue "83.8058" ;
  ns2:hasScale ns2:KelvinScale .

ns2:_234.3156OnTheKelvinScale
  a ns2:FixedPoint ;
  rdfs:label "234.3156 on the Kelvin scale"@en ;
  ns2:hasNumericalValue "234.3156" ;
  ns2:hasScale ns2:KelvinScale .

ns2:_273.16OnTheKelvinScale
  a ns2:FixedPoint ;
  rdfs:label "273.16 on the Kelvin scale"@en ;
  ns2:hasNumericalValue "273.16" ;
  ns2:hasScale ns2:KelvinScale ;
  ns2:hasQuantity ns2:thermodynamicTemperatureOfTheTriplePointOfWater .

ns2:_302.9146OnTheKelvinScale
  a ns2:FixedPoint ;
  rdfs:label "302.9146 on the Kelvin scale"@en ;
  ns2:hasNumericalValue "302.9146" ;
  ns2:hasScale ns2:KelvinScale .

ns2:_429.7485OnTheKelvinScale
  a ns2:FixedPoint ;
  rdfs:label "429.7485 on the Kelvin scale"@en ;
  ns2:hasNumericalValue "429.7485" ;
  ns2:hasScale ns2:KelvinScale .

ns2:_505.078OnTheKelvinScale
  a ns2:FixedPoint ;
  rdfs:label "505.078 on the Kelvin scale"@en ;
  ns2:hasNumericalValue "505.078" ;
  ns2:hasScale ns2:KelvinScale .

ns2:_692.677OnTheKelvinScale
  a ns2:FixedPoint ;
  rdfs:label "692.677 on the Kelvin scale"@en ;
  ns2:hasNumericalValue "692.677" ;
  ns2:hasScale ns2:KelvinScale .

ns2:_933.473OnTheKelvinScale
  a ns2:FixedPoint ;
  rdfs:label "933.473 on the Kelvin scale"@en ;
  ns2:hasNumericalValue "933.473" ;
  ns2:hasScale ns2:KelvinScale .

ns2:_1234.93OnTheKelvinScale
  a ns2:FixedPoint ;
  rdfs:label "1234.93 on the Kelvin scale"@en ;
  ns2:hasNumericalValue "1234.93" ;
  ns2:hasScale ns2:KelvinScale .

ns2:_1337.33OnTheKelvinScale
  a ns2:FixedPoint ;
  rdfs:label "1337.33 on the Kelvin scale"@en ;
  ns2:hasNumericalValue "1337.33" ;
  ns2:hasScale ns2:KelvinScale .

ns2:_1357.77OnTheKelvinScale
  a ns2:FixedPoint ;
  rdfs:label "1357.77 on the Kelvin scale"@en ;
  ns2:hasNumericalValue "1357.77" ;
  ns2:hasScale ns2:KelvinScale .

ns2:ThermodynamicTemperatureScale
  a owl:Class ;
  rdfs:label "thermodynamic temperature scale"@en ;
  rdfs:subClassOf ns2:Scale ;
  owl:equivalentClass [
    a owl:Class ;
    owl:oneOf ( ns2:KelvinScale )
  ] .

ns2:CelsiusScale
  a ns2:IntervalScale ;
  rdfs:label "Celsius scale"@en, "Celsiusschaal"@nl, "摄氏温标"@zh ;
  ns2:alternativeLabel "International Celsius Temperature scale of 1990"@en ;
  ns2:hasDimension ns2:thermodynamicTemperature-Dimension ;
  ns2:hasPoint ns2:_-270.15To-268.15OnTheCelsiusScale, ns2:_-259.3467OnTheCelsiusScale, ns2:approximately-256.15OnTheCelsiusScale, ns2:approximately-252.85OnTheCelsiusScale, ns2:_-248.5939OnTheCelsiusScale, ns2:_-218.7916OnTheCelsiusScale, ns2:_-189.3442OnTheCelsiusScale, ns2:_-38.8344OnTheCelsiusScale, ns2:_0.01OnTheCelsiusScale, ns2:_29.7646OnTheCelsiusScale, ns2:_156.5985OnTheCelsiusScale, ns2:_231.928OnTheCelsiusScale, ns2:_419.527OnTheCelsiusScale, ns2:_660.323OnTheCelsiusScale, ns2:_961.78OnTheCelsiusScale, ns2:_1064.18OnTheCelsiusScale, ns2:_1084.62OnTheCelsiusScale ;
  ns2:hasFactor "1"^^xsd:float ;
  ns2:hasOff-Set "-273.15"^^xsd:float ;
  ns2:hasScale ns2:KelvinScale ;
  ns2:hasUnit ns2:degreeCelsius .

ns2:_-270.15To-268.15OnTheCelsiusScale
  a ns2:FixedPoint ;
  rdfs:label "-270.15 to -268.15 on the Celsius scale"@en, "-270.15至-268.15摄氏度"@zh ;
  rdfs:comment "One of the fixed points defining the Celsius scale"@en ;
  ns2:hasNumericalValue "-270.15 to -268.15" ;
  ns2:hasScale ns2:CelsiusScale ;
  ns2:hasPoint ns2:_3To5OnTheKelvinScale .

ns2:_-259.3467OnTheCelsiusScale
  a ns2:FixedPoint ;
  rdfs:label "-259.3467 on the Celsius scale"@en, "-259.3467摄氏度"@zh ;
  ns2:hasNumericalValue "-259.3467" ;
  ns2:hasScale ns2:CelsiusScale ;
  ns2:hasPoint ns2:_13.8033OnTheKelvinScale .

ns2:approximately-256.15OnTheCelsiusScale
  a ns2:FixedPoint ;
  rdfs:label "~-256.15 on the Celsius scale"@en, "〜-256.15摄氏度"@zh ;
  ns2:hasNumericalValue "~-256.15" ;
  ns2:hasScale ns2:CelsiusScale ;
  ns2:hasPoint ns2:approximately17OnTheKelvinScale .

ns2:approximately-252.85OnTheCelsiusScale
  a ns2:FixedPoint ;
  rdfs:label "~-252.85 on the Celsius scale"@en, "〜-252.85摄氏度"@zh ;
  ns2:hasNumericalValue "~-252.85" ;
  ns2:hasScale ns2:CelsiusScale ;
  ns2:hasPoint ns2:approximately203OnTheKelvinScale .

ns2:_-248.5939OnTheCelsiusScale
  a ns2:FixedPoint ;
  rdfs:label "-248.5939 on the Celsius scale"@en, "-248.5939摄氏度"@zh ;
  ns2:hasNumericalValue "-248.5939" ;
  ns2:hasScale ns2:CelsiusScale ;
  ns2:hasPoint ns2:_24.5561OnTheKelvinScale .

ns2:_-218.7916OnTheCelsiusScale
  a ns2:FixedPoint ;
  rdfs:label "-218.7916 on the Celsius scale"@en, "-218.7916摄氏度"@zh ;
  ns2:hasNumericalValue "-218.7916" ;
  ns2:hasScale ns2:CelsiusScale ;
  ns2:hasPoint ns2:_54.3584OnTheKelvinScale .

ns2:_-189.3442OnTheCelsiusScale
  a ns2:FixedPoint ;
  rdfs:label "-189.3442 on the Celsius scale"@en, "-189.3442摄氏度"@zh ;
  ns2:hasNumericalValue "-189.3442" ;
  ns2:hasScale ns2:CelsiusScale ;
  ns2:hasPoint ns2:_83.8058OnTheKelvinScale .

ns2:_-38.8344OnTheCelsiusScale
  a ns2:FixedPoint ;
  rdfs:label "-38.8344 on the Celsius scale"@en, "-38.8344摄氏度"@zh ;
  ns2:hasNumericalValue "-38.8344" ;
  ns2:hasScale ns2:CelsiusScale ;
  ns2:hasPoint ns2:_234.3156OnTheKelvinScale .

ns2:_0.01OnTheCelsiusScale
  a ns2:FixedPoint ;
  rdfs:label "0.01 on the Celsius scale"@en, "0.01摄氏度"@zh ;
  ns2:hasNumericalValue "0.01" ;
  ns2:hasScale ns2:CelsiusScale ;
  ns2:hasPoint ns2:_273.16OnTheKelvinScale .

ns2:_29.7646OnTheCelsiusScale
  a ns2:FixedPoint ;
  rdfs:label "29.7646 on the Celsius scale"@en, "29.7646摄氏度"@zh ;
  ns2:hasNumericalValue "29.7646" ;
  ns2:hasScale ns2:CelsiusScale ;
  ns2:hasPoint ns2:_302.9146OnTheKelvinScale .

ns2:_156.5985OnTheCelsiusScale
  a ns2:FixedPoint ;
  rdfs:label "156.5985 on the Celsius scale"@en, "156.5985摄氏度"@zh ;
  ns2:hasNumericalValue "156.5985" ;
  ns2:hasScale ns2:CelsiusScale ;
  ns2:hasPoint ns2:_429.7485OnTheKelvinScale .

ns2:_231.928OnTheCelsiusScale
  a ns2:FixedPoint ;
  rdfs:label "231.928 on the Celsius scale"@en, "231.928摄氏度"@zh ;
  ns2:hasNumericalValue "231.928" ;
  ns2:hasScale ns2:CelsiusScale ;
  ns2:hasPoint ns2:_505.078OnTheKelvinScale .

ns2:_419.527OnTheCelsiusScale
  a ns2:FixedPoint ;
  rdfs:label "419.527 on the Celsius scale"@en, "419.527摄氏度"@zh ;
  ns2:hasNumericalValue "419.527" ;
  ns2:hasScale ns2:CelsiusScale ;
  ns2:hasPoint ns2:_692.677OnTheKelvinScale .

ns2:_660.323OnTheCelsiusScale
  a ns2:FixedPoint ;
  rdfs:label "660.323 on the Celsius scale"@en, "660.323摄氏度"@zh ;
  ns2:hasNumericalValue "660.323" ;
  ns2:hasScale ns2:CelsiusScale ;
  ns2:hasPoint ns2:_933.473OnTheKelvinScale .

ns2:_961.78OnTheCelsiusScale
  a ns2:FixedPoint ;
  rdfs:label "961.78 on the Celsius scale"@en, "961.78摄氏度"@zh ;
  ns2:hasNumericalValue "961.78" ;
  ns2:hasScale ns2:CelsiusScale ;
  ns2:hasPoint ns2:_1234.93OnTheKelvinScale .

ns2:_1064.18OnTheCelsiusScale
  a ns2:FixedPoint ;
  rdfs:label "1064.18 on the Celsius scale"@en, "1064.18摄氏度"@zh ;
  ns2:hasNumericalValue "1064.18" ;
  ns2:hasScale ns2:CelsiusScale ;
  ns2:hasPoint ns2:_1337.33OnTheKelvinScale .

ns2:_1084.62OnTheCelsiusScale
  a ns2:FixedPoint ;
  rdfs:label "1084.62 on the Celsius scale"@en, "1084.62摄氏度"@zh ;
  ns2:hasNumericalValue "1084.62" ;
  ns2:hasScale ns2:CelsiusScale ;
  ns2:hasPoint ns2:_1357.77OnTheKelvinScale .

ns2:CelsiusTemperatureScale
  a owl:Class ;
  rdfs:label "Celsius temperature scale"@en ;
  rdfs:subClassOf ns2:Scale ;
  owl:equivalentClass [
    a owl:Class ;
    owl:oneOf ( ns2:CelsiusScale )
  ] .

ns2:FahrenheitScale
  a ns2:IntervalScale ;
  rdfs:label "Fahrenheit scale"@en, "Fahrenheitschaal"@nl, "华氏温标"@zh ;
  ns2:hasFactor "1.8"^^xsd:float ;
  ns2:hasOff-Set "-459.67"^^xsd:float ;
  ns2:hasScale ns2:KelvinScale ;
  ns2:hasUnit ns2:degreeFahrenheit ;
  ns2:hasDimension ns2:thermodynamicTemperature-Dimension .

ns2:RankineScale
  a ns2:RatioScale ;
  rdfs:label "Rankine scale"@en, "Rankineschaal"@nl, "兰金规模"@zh ;
  ns2:hasFactor "1.8"^^xsd:float ;
  ns2:hasOff-Set "0"^^xsd:float ;
  ns2:hasScale ns2:KelvinScale ;
  ns2:hasUnit ns2:degreeRankine ;
  ns2:hasDimension ns2:thermodynamicTemperature-Dimension .

ns2:ReaumurScale
  a ns2:IntervalScale ;
  rdfs:label "Réaumur scale"@en, "Réaumurschaal"@nl, "列氏温标"@zh ;
  ns2:hasFactor "1"^^xsd:float ;
  ns2:hasOff-Set "-218.52"^^xsd:float ;
  ns2:hasScale ns2:KelvinScale ;
  ns2:hasUnit ns2:degreeReaumur ;
  ns2:hasDimension ns2:thermodynamicTemperature-Dimension .

ns2:Temperature_scale
  a owl:Class ;
  rdfs:subClassOf ns2:Scale ;
  owl:equivalentClass [
    a owl:Class ;
    owl:oneOf (
     ns2:CelsiusScale
     ns2:FahrenheitScale
     ns2:ReaumurScale
     ns2:KelvinScale
     ns2:RankineScale
   )
  ] .

ns2:FahrenheitTemperatureScale
  a owl:Class ;
  rdfs:label "Fahrenheit temperature scale"@en ;
  rdfs:subClassOf ns2:Scale ;
  owl:equivalentClass [
    a owl:Class ;
    owl:oneOf ( ns2:FahrenheitScale )
  ] .

ns2:RankineTemperatureScale
  a owl:Class ;
  rdfs:label "Rankine temperature scale"@en ;
  rdfs:subClassOf ns2:Scale ;
  owl:equivalentClass [
    a owl:Class ;
    owl:oneOf ( ns2:RankineScale )
  ] .

ns2:ReaumurTemperatureScale
  a owl:Class ;
  rdfs:label "Réaumur temperature scale"@en ;
  rdfs:subClassOf ns2:Scale ;
  owl:equivalentClass [
    a owl:Class ;
    owl:oneOf ( ns2:ReaumurScale )
  ] .

ns2:thermodynamicTemperature-Dimension
  a ns2:Dimension ;
  rdfs:label "thermodynamic temperature dimension"@en, "absolute-temperatuurdimensie"@nl ;
  ns2:symbol "Θ" ;
  ns2:hasSILengthDimensionExponent 0 ;
  ns2:hasSIMassDimensionExponent 0 ;
  ns2:hasSITimeDimensionExponent 0 ;
  ns2:hasSIElectricCurrentDimensionExponent 0 ;
  ns2:hasSIThermodynamicTemperatureDimensionExponent 1 ;
  ns2:hasSIAmountOfSubstanceDimensionExponent 0 ;
  ns2:hasSILuminousIntensityDimensionExponent 0 .

ns2:entropyOrHeatCapacity-Dimension
  a ns2:Dimension ;
  rdfs:label "entropy or heat capacity dimension"@en ;
  ns2:hasSILengthDimensionExponent 2 ;
  ns2:hasSIMassDimensionExponent 1 ;
  ns2:hasSITimeDimensionExponent -2 ;
  ns2:hasSIElectricCurrentDimensionExponent 0 ;
  ns2:hasSIThermodynamicTemperatureDimensionExponent -1 ;
  ns2:hasSIAmountOfSubstanceDimensionExponent 0 ;
  ns2:hasSILuminousIntensityDimensionExponent 0 .

ns2:specificEntropyOrSpecificHeatCapacity-Dimension
  a ns2:Dimension ;
  rdfs:label "specific entropy or specific heat capacity dimension"@en ;
  ns2:hasSILengthDimensionExponent 2 ;
  ns2:hasSIMassDimensionExponent 0 ;
  ns2:hasSITimeDimensionExponent -2 ;
  ns2:hasSIElectricCurrentDimensionExponent 0 ;
  ns2:hasSIThermodynamicTemperatureDimensionExponent -1 ;
  ns2:hasSIAmountOfSubstanceDimensionExponent 0 ;
  ns2:hasSILuminousIntensityDimensionExponent 0 .

ns2:thermalConductivity-Dimension
  a ns2:Dimension ;
  rdfs:label "thermal conductivity dimension"@en ;
  ns2:hasSILengthDimensionExponent 1 ;
  ns2:hasSIMassDimensionExponent 1 ;
  ns2:hasSITimeDimensionExponent -3 ;
  ns2:hasSIElectricCurrentDimensionExponent 0 ;
  ns2:hasSIThermodynamicTemperatureDimensionExponent -1 ;
  ns2:hasSIAmountOfSubstanceDimensionExponent 0 ;
  ns2:hasSILuminousIntensityDimensionExponent 0 .

ns2:thermalInsulance-Dimension
  a ns2:Dimension ;
  rdfs:label "thermal insulance dimension"@en ;
  ns2:hasSILengthDimensionExponent 0 ;
  ns2:hasSIMassDimensionExponent -1 ;
  ns2:hasSITimeDimensionExponent 3 ;
  ns2:hasSIElectricCurrentDimensionExponent 0 ;
  ns2:hasSIThermodynamicTemperatureDimensionExponent 1 ;
  ns2:hasSIAmountOfSubstanceDimensionExponent 0 ;
  ns2:hasSILuminousIntensityDimensionExponent 0 .

ns2:thermalResistance-Dimension
  a ns2:Dimension ;
  rdfs:label "thermal resistance dimension"@en ;
  ns2:hasSILengthDimensionExponent -2 ;
  ns2:hasSIMassDimensionExponent -1 ;
  ns2:hasSITimeDimensionExponent 3 ;
  ns2:hasSIElectricCurrentDimensionExponent 0 ;
  ns2:hasSIThermodynamicTemperatureDimensionExponent 1 ;
  ns2:hasSIAmountOfSubstanceDimensionExponent 0 ;
  ns2:hasSILuminousIntensityDimensionExponent 0 .

ns2:heatTransferCoefficient-Dimension
  a ns2:Dimension ;
  rdfs:label "heat transfer coefficient dimension"@en ;
  ns2:hasSILengthDimensionExponent 0 ;
  ns2:hasSIMassDimensionExponent 1 ;
  ns2:hasSITimeDimensionExponent -3 ;
  ns2:hasSIElectricCurrentDimensionExponent 0 ;
  ns2:hasSIThermodynamicTemperatureDimensionExponent -1 ;
  ns2:hasSIAmountOfSubstanceDimensionExponent 0 ;
  ns2:hasSILuminousIntensityDimensionExponent 0 .

ns2:volumetricHeatCapacity-Dimension
  a ns2:Dimension ;
  rdfs:label "volumetric heat capacity dimension"@en ;
  ns2:hasSILengthDimensionExponent -1 ;
  ns2:hasSIMassDimensionExponent 1 ;
  ns2:hasSITimeDimensionExponent -2 ;
  ns2:hasSIElectricCurrentDimensionExponent 0 ;
  ns2:hasSIThermodynamicTemperatureDimensionExponent -1 ;
  ns2:hasSIAmountOfSubstanceDimensionExponent 0 ;
  ns2:hasSILuminousIntensityDimensionExponent 0 .

ns2:electromagnetism
  a ns2:ApplicationArea ;
  rdfs:label "electromagnetism"@en, "elektromagnetisme"@nl ;
  ns2:usesQuantity ns2:ElectricCurrent, ns2:CurrentDensity, ns2:ElectricCharge, ns2:ElectricPotential, ns2:ElectromotiveForce, ns2:PotentialDifference, ns2:Capacitance, ns2:ElectricalResistance, ns2:ElectricalConductance, ns2:ElectricField, ns2:ElectricChargeDensity, ns2:ElectricFluxDensity, ns2:MagneticField, ns2:MagneticFlux, ns2:MagneticFluxDensity, ns2:Permeance-Electromagnetic, ns2:Inductance, ns2:PermeabilityOfFreeSpace, ns2:Permittivity, ns2:ElectricDipoleMoment, ns2:Reluctance, ns2:Admittance, ns2:ElectricalResistivity, ns2:ElectricalConductivity, ns2:MagnetomotiveForce ;
  ns2:usesUnit ns2:ampere, ns2:attoampere, ns2:centiampere, ns2:decaampere, ns2:deciampere, ns2:exaampere, ns2:femtoampere, ns2:gigaampere, ns2:hectoampere, ns2:kiloampere, ns2:megaampere, ns2:microampere, ns2:milliampere, ns2:nanoampere, ns2:petaampere, ns2:picoampere, ns2:teraampere, ns2:abampere, ns2:biot, ns2:gilbert, ns2:statampere, ns2:amperePerSquareMetre, ns2:second-TimeAmpere, ns2:coulomb, ns2:attocoulomb, ns2:centicoulomb, ns2:decacoulomb, ns2:decicoulomb, ns2:exacoulomb, ns2:femtocoulomb, ns2:gigacoulomb, ns2:hectocoulomb, ns2:kilocoulomb, ns2:megacoulomb, ns2:microcoulomb, ns2:millicoulomb, ns2:nanocoulomb, ns2:petacoulomb, ns2:picocoulomb, ns2:teracoulomb, ns2:abcoulomb, ns2:faraday, ns2:franklin, ns2:statcoulomb, ns2:wattPerAmpere, ns2:volt, ns2:attovolt, ns2:centivolt, ns2:decavolt, ns2:decivolt, ns2:exavolt, ns2:femtovolt, ns2:gigavolt, ns2:hectovolt, ns2:kilovolt, ns2:megavolt, ns2:microvolt, ns2:millivolt, ns2:nanovolt, ns2:petavolt, ns2:picovolt, ns2:teravolt, ns2:abvolt, ns2:statvolt, ns2:coulombPerVolt, ns2:farad, ns2:attofarad, ns2:centifarad, ns2:decafarad, ns2:decifarad, ns2:exafarad, ns2:femtofarad, ns2:gigafarad, ns2:hectofarad, ns2:kilofarad, ns2:megafarad, ns2:microfarad, ns2:millifarad, ns2:nanofarad, ns2:petafarad, ns2:picofarad, ns2:terafarad, ns2:abfarad, ns2:statfarad, ns2:voltPerAmpere, ns2:ohm, ns2:attoohm, ns2:centiohm, ns2:decaohm, ns2:deciohm, ns2:exaohm, ns2:femtoohm, ns2:gigaohm, ns2:hectoohm, ns2:kilohm, ns2:megohm, ns2:microohm, ns2:milliohm, ns2:nanoohm, ns2:petaohm, ns2:picoohm, ns2:teraohm, ns2:abohm, ns2:statohm, ns2:amperePerVolt, ns2:siemens, ns2:attosiemens, ns2:centisiemens, ns2:decasiemens, ns2:decisiemens, ns2:exasiemens, ns2:femtosiemens, ns2:gigasiemens, ns2:hectosiemens, ns2:kilosiemens, ns2:megasiemens, ns2:microsiemens, ns2:millisiemens, ns2:nanosiemens, ns2:petasiemens, ns2:picosiemens, ns2:terasiemens, ns2:abmho, ns2:mho, ns2:statmho, ns2:newtonPerCoulomb, ns2:voltPerMetre, ns2:coulombPerCubicmetre, ns2:coulombPerSquareMetre, ns2:amperePerMetre, ns2:oersted, ns2:voltSecond-Time, ns2:weber, ns2:attoweber, ns2:centiweber, ns2:decaweber, ns2:deciweber, ns2:exaweber, ns2:femtoweber, ns2:gigaweber, ns2:hectoweber, ns2:kiloweber, ns2:megaweber, ns2:microweber, ns2:milliweber, ns2:nanoweber, ns2:petaweber, ns2:picoweber, ns2:teraweber, ns2:maxwell, ns2:statweber, ns2:unitPole, ns2:weberPerSquareMetre, ns2:tesla, ns2:attotesla, ns2:centitesla, ns2:decatesla, ns2:decitesla, ns2:exatesla, ns2:femtotesla, ns2:gigatesla, ns2:hectotesla, ns2:kilotesla, ns2:megatesla, ns2:microtesla, ns2:millitesla, ns2:nanotesla, ns2:petatesla, ns2:picotesla, ns2:teratesla, ns2:gamma, ns2:gauss, ns2:stattesla, ns2:milligauss, ns2:weberPerAmpere, ns2:henry, ns2:attohenry, ns2:centihenry, ns2:decahenry, ns2:decihenry, ns2:exahenry, ns2:femtohenry, ns2:gigahenry, ns2:hectohenry, ns2:kilohenry, ns2:megahenry, ns2:microhenry, ns2:millihenry, ns2:nanohenry, ns2:petahenry, ns2:picohenry, ns2:terahenry, ns2:abhenry, ns2:stathenry, ns2:henryPerMetre, ns2:faradPerMetre, ns2:coulombMetre, ns2:debye, ns2:reciprocalHenry, ns2:ohmMetre, ns2:siemensPerMetre .

ns2:ElectricCurrent
  a owl:Class ;
  rdfs:label "electric current"@en ;
  ns2:alternativeLabel "current"@en ;
  rdfs:comment "Electric current is the flow of electric charge. It is a base quantity in the International System of Units. Electric current is electric charge divided by time."@en ;
  rdfs:subClassOf ns2:Quantity, [
    a owl:Restriction ;
    owl:onProperty ns2:hasValue ;
    owl:allValuesFrom [
      a owl:Restriction ;
      owl:onProperty ns2:hasUnit ;
      owl:allValuesFrom ns2:ElectricCurrentUnit
    ]
  ], [
    a owl:Restriction ;
    owl:onProperty ns2:hasDimension ;
    owl:hasValue ns2:electricCurrent-Dimension
  ] ;
  ns2:symbol "I" ;
  ns2:alternativeSymbol "i" ;
  ns2:commonlyHasUnit ns2:ampere, ns2:attoampere, ns2:centiampere, ns2:decaampere, ns2:deciampere, ns2:exaampere, ns2:femtoampere, ns2:gigaampere, ns2:hectoampere, ns2:kiloampere, ns2:megaampere, ns2:microampere, ns2:milliampere, ns2:nanoampere, ns2:petaampere, ns2:picoampere, ns2:teraampere, ns2:abampere, ns2:biot, ns2:statampere .

ns2:CurrentDensity
  a owl:Class ;
  rdfs:label "current density"@en ;
  rdfs:comment "Current density is the density of flow of a conserved charge. It is a derived quantity in the International System of Units. Current density is electric current divided by area."@en ;
  rdfs:subClassOf ns2:Quantity, [
    a owl:Restriction ;
    owl:onProperty ns2:hasValue ;
    owl:allValuesFrom [
      a owl:Restriction ;
      owl:onProperty ns2:hasUnit ;
      owl:allValuesFrom ns2:CurrentDensityUnit
    ]
  ], [
    a owl:Restriction ;
    owl:onProperty ns2:hasDimension ;
    owl:hasValue ns2:currentDensity-Dimension
  ] ;
  ns2:symbol "J" ;
  ns2:alternativeSymbol "j" ;
  ns2:commonlyHasUnit ns2:amperePerSquareMetre .

ns2:ElectricCharge
  a owl:Class ;
  rdfs:label "electric charge"@en, "electrische lading"@nl ;
  ns2:alternativeLabel "quantity of electricity"@en, "lading"@nl ;
  rdfs:comment "Electric charge is a conserved property of some subatomic particles, which determines their electromagnetic interaction. It is a derived quantity in the International System of Units. Electric charge is electric current times time."@en ;
  rdfs:subClassOf ns2:Quantity, [
    a owl:Restriction ;
    owl:onProperty ns2:hasValue ;
    owl:allValuesFrom [
      a owl:Restriction ;
      owl:onProperty ns2:hasUnit ;
      owl:allValuesFrom ns2:ElectricChargeUnit
    ]
  ], [
    a owl:Restriction ;
    owl:onProperty ns2:hasDimension ;
    owl:hasValue ns2:electricCharge-Dimension
  ] ;
  ns2:symbol "Q" ;
  ns2:alternativeSymbol "q" ;
  ns2:commonlyHasUnit ns2:second-TimeAmpere, ns2:coulomb, ns2:attocoulomb, ns2:centicoulomb, ns2:decacoulomb, ns2:decicoulomb, ns2:exacoulomb, ns2:femtocoulomb, ns2:gigacoulomb, ns2:hectocoulomb, ns2:kilocoulomb, ns2:megacoulomb, ns2:microcoulomb, ns2:millicoulomb, ns2:nanocoulomb, ns2:petacoulomb, ns2:picocoulomb, ns2:teracoulomb, ns2:abcoulomb, ns2:faraday, ns2:franklin, ns2:statcoulomb, ns2:amperehour, ns2:milliamperehour .

ns2:ElectricPotential
  a owl:Class ;
  rdfs:label "electric potential"@en, "electrische potentiaal"@nl ;
  ns2:alternativeLabel "voltage"@en, "voltage"@nl ;
  rdfs:comment "Electric potential is the potential energy per unit charge associated with static (time-invariant) electric field."@en ;
  rdfs:subClassOf ns2:Quantity, [
    a owl:Restriction ;
    owl:onProperty ns2:hasValue ;
    owl:allValuesFrom [
      a owl:Restriction ;
      owl:onProperty ns2:hasUnit ;
      owl:allValuesFrom ns2:ElectricPotentialUnit
    ]
  ], [
    a owl:Restriction ;
    owl:onProperty ns2:hasDimension ;
    owl:hasValue ns2:electricPotential-Dimension
  ] ;
  ns2:symbol "V" ;
  ns2:alternativeSymbol "φ" ;
  ns2:commonlyHasUnit ns2:wattPerAmpere, ns2:volt, ns2:attovolt, ns2:centivolt, ns2:decavolt, ns2:decivolt, ns2:exavolt, ns2:femtovolt, ns2:gigavolt, ns2:hectovolt, ns2:kilovolt, ns2:megavolt, ns2:microvolt, ns2:millivolt, ns2:nanovolt, ns2:petavolt, ns2:picovolt, ns2:teravolt, ns2:abvolt, ns2:statvolt .

ns2:ElectromotiveForce
  a owl:Class ;
  rdfs:label "electromotive force"@en ;
  rdfs:comment "Electromotive force is that which causes a flow of current."@en ;
  rdfs:subClassOf ns2:ElectricPotential ;
  ns2:symbol "E" ;
  ns2:alternativeSymbol "emf" ;
  ns2:commonlyHasUnit ns2:wattPerAmpere, ns2:volt, ns2:attovolt, ns2:centivolt, ns2:decavolt, ns2:decivolt, ns2:exavolt, ns2:femtovolt, ns2:gigavolt, ns2:hectovolt, ns2:kilovolt, ns2:megavolt, ns2:microvolt, ns2:millivolt, ns2:nanovolt, ns2:petavolt, ns2:picovolt, ns2:teravolt, ns2:abvolt, ns2:statvolt .

ns2:PotentialDifference
  a owl:Class ;
  rdfs:label "potential difference"@en, "potentiaalverschil"@nl ;
  rdfs:subClassOf ns2:ElectricPotential ;
  ns2:symbol "U" ;
  ns2:alternativeSymbol "V" ;
  ns2:commonlyHasUnit ns2:wattPerAmpere, ns2:volt, ns2:attovolt, ns2:centivolt, ns2:decavolt, ns2:decivolt, ns2:exavolt, ns2:femtovolt, ns2:gigavolt, ns2:hectovolt, ns2:kilovolt, ns2:megavolt, ns2:microvolt, ns2:millivolt, ns2:nanovolt, ns2:petavolt, ns2:picovolt, ns2:teravolt, ns2:abvolt, ns2:statvolt .

ns2:Capacitance
  a owl:Class ;
  rdfs:label "capacitance"@en, "capaciteit"@nl ;
  ns2:alternativeLabel "electric capacitance"@en, "electrische capaciteit"@nl ;
  rdfs:comment "Capacitance is the ability to hold electrical charge. It is a derived quantity in the International System of Units. Capacitance is electric charge divided by electric potential."@en ;
  rdfs:subClassOf ns2:Quantity, [
    a owl:Restriction ;
    owl:onProperty ns2:hasValue ;
    owl:allValuesFrom [
      a owl:Restriction ;
      owl:onProperty ns2:hasUnit ;
      owl:allValuesFrom ns2:CapacitanceUnit
    ]
  ], [
    a owl:Restriction ;
    owl:onProperty ns2:hasDimension ;
    owl:hasValue ns2:capacitance-Dimension
  ] ;
  ns2:symbol "C" ;
  ns2:commonlyHasUnit ns2:coulombPerVolt, ns2:farad, ns2:attofarad, ns2:centifarad, ns2:decafarad, ns2:decifarad, ns2:exafarad, ns2:femtofarad, ns2:gigafarad, ns2:hectofarad, ns2:kilofarad, ns2:megafarad, ns2:microfarad, ns2:millifarad, ns2:nanofarad, ns2:petafarad, ns2:picofarad, ns2:terafarad, ns2:abfarad, ns2:statfarad .

ns2:ElectricalResistance
  a owl:Class ;
  rdfs:label "electrical resistance"@en ;
  ns2:alternativeLabel "electric resistance"@en, "resistance"@en ;
  rdfs:comment "Electrical resistance is the degree to which an object opposes an electric current through it. It is a derived quantity in the International System of Units.  Electrical resistance is electric potential divided by electric current."@en ;
  rdfs:subClassOf ns2:Quantity, [
    a owl:Restriction ;
    owl:onProperty ns2:hasValue ;
    owl:allValuesFrom [
      a owl:Restriction ;
      owl:onProperty ns2:hasUnit ;
      owl:allValuesFrom ns2:ElectricalResistanceUnit
    ]
  ], [
    a owl:Restriction ;
    owl:onProperty ns2:hasDimension ;
    owl:hasValue ns2:electricalResistance-Dimension
  ] ;
  ns2:symbol "R" ;
  ns2:commonlyHasUnit ns2:voltPerAmpere, ns2:ohm, ns2:attoohm, ns2:centiohm, ns2:decaohm, ns2:deciohm, ns2:exaohm, ns2:femtoohm, ns2:gigaohm, ns2:hectoohm, ns2:kilohm, ns2:megohm, ns2:microohm, ns2:milliohm, ns2:nanoohm, ns2:petaohm, ns2:picoohm, ns2:teraohm, ns2:abohm, ns2:statohm .

ns2:ElectricalConductance
  a owl:Class ;
  rdfs:label "electrical conductance"@en ;
  ns2:alternativeLabel "electric conductance"@en, "conductance"@en ;
  rdfs:comment "Electrical conductance is a measure of how easily electricity flows along a certain path through an electrical element."@en ;
  rdfs:subClassOf ns2:Quantity, [
    a owl:Restriction ;
    owl:onProperty ns2:hasValue ;
    owl:allValuesFrom [
      a owl:Restriction ;
      owl:onProperty ns2:hasUnit ;
      owl:allValuesFrom ns2:ElectricalConductanceUnit
    ]
  ], [
    a owl:Restriction ;
    owl:onProperty ns2:hasDimension ;
    owl:hasValue ns2:electricalConductance-Dimension
  ] ;
  ns2:symbol "G" ;
  ns2:commonlyHasUnit ns2:amperePerVolt, ns2:siemens, ns2:attosiemens, ns2:centisiemens, ns2:decasiemens, ns2:decisiemens, ns2:exasiemens, ns2:femtosiemens, ns2:gigasiemens, ns2:hectosiemens, ns2:kilosiemens, ns2:megasiemens, ns2:microsiemens, ns2:millisiemens, ns2:nanosiemens, ns2:petasiemens, ns2:picosiemens, ns2:terasiemens, ns2:abmho, ns2:mho, ns2:statmho .

ns2:ElectricField
  a owl:Class ;
  rdfs:label "electric field"@en, "electrisch veld"@nl ;
  ns2:alternativeLabel "electric field strength"@en ;
  rdfs:comment "Electric field is a property of the space surrounding an electric charge or in the presence of a time-varying magnetic field which exerts a forceon other electrically charged objects."@en ;
  rdfs:subClassOf ns2:Quantity, [
    a owl:Restriction ;
    owl:onProperty ns2:hasValue ;
    owl:allValuesFrom [
      a owl:Restriction ;
      owl:onProperty ns2:hasUnit ;
      owl:allValuesFrom ns2:ElectricFieldUnit
    ]
  ], [
    a owl:Restriction ;
    owl:onProperty ns2:hasDimension ;
    owl:hasValue ns2:electricField-Dimension
  ] ;
  ns2:symbol "E" ;
  ns2:commonlyHasUnit ns2:newtonPerCoulomb, ns2:voltPerMetre .

ns2:ElectricChargeDensity
  a owl:Class ;
  rdfs:label "electric charge density"@en ;
  ns2:alternativeLabel "charge density"@en ;
  rdfs:comment "Electric charge density is the amount of electric charge in a volume. It is a derived quantity in the International System of Units. Electric charge density is electric charge divided by volume."@en ;
  rdfs:subClassOf ns2:Quantity, [
    a owl:Restriction ;
    owl:onProperty ns2:hasValue ;
    owl:allValuesFrom [
      a owl:Restriction ;
      owl:onProperty ns2:hasUnit ;
      owl:allValuesFrom ns2:ElectricChargeDensityUnit
    ]
  ], [
    a owl:Restriction ;
    owl:onProperty ns2:hasDimension ;
    owl:hasValue ns2:electricChargeDensity-Dimension
  ] ;
  ns2:commonlyHasUnit ns2:coulombPerCubicmetre .

ns2:ElectricFluxDensity
  a owl:Class ;
  rdfs:label "electric flux density"@en ;
  rdfs:subClassOf ns2:Quantity, [
    a owl:Restriction ;
    owl:onProperty ns2:hasValue ;
    owl:allValuesFrom [
      a owl:Restriction ;
      owl:onProperty ns2:hasUnit ;
      owl:allValuesFrom ns2:ElectricFluxDensityUnit
    ]
  ], [
    a owl:Restriction ;
    owl:onProperty ns2:hasDimension ;
    owl:hasValue ns2:electricFluxDensity-Dimension
  ] ;
  ns2:commonlyHasUnit ns2:coulombPerSquareMetre .

ns2:MagneticFlux
  a owl:Class ;
  rdfs:label "magnetic flux"@en ;
  rdfs:comment "Magnetic flux through any area perpendicular to a magnetic field is the product of the area by the field strength."@en ;
  rdfs:subClassOf ns2:Quantity, [
    a owl:Restriction ;
    owl:onProperty ns2:hasValue ;
    owl:allValuesFrom [
      a owl:Restriction ;
      owl:onProperty ns2:hasUnit ;
      owl:allValuesFrom ns2:MagneticFluxUnit
    ]
  ], [
    a owl:Restriction ;
    owl:onProperty ns2:hasDimension ;
    owl:hasValue ns2:magneticFlux-Dimension
  ] ;
  ns2:symbol "Φ" ;
  ns2:commonlyHasUnit ns2:voltSecond-Time, ns2:weber, ns2:attoweber, ns2:centiweber, ns2:decaweber, ns2:deciweber, ns2:exaweber, ns2:femtoweber, ns2:gigaweber, ns2:hectoweber, ns2:kiloweber, ns2:megaweber, ns2:microweber, ns2:milliweber, ns2:nanoweber, ns2:petaweber, ns2:picoweber, ns2:teraweber, ns2:maxwell, ns2:statweber, ns2:unitPole .

ns2:MagneticField
  a owl:Class ;
  rdfs:label "magnetic field"@en ;
  ns2:alternativeLabel "magnetic field strength"@en, "magnetic field intensity"@en, "magnetizing field"@en ;
  rdfs:subClassOf ns2:Quantity, [
    a owl:Restriction ;
    owl:onProperty ns2:hasValue ;
    owl:allValuesFrom [
      a owl:Restriction ;
      owl:onProperty ns2:hasUnit ;
      owl:allValuesFrom ns2:MagneticFieldUnit
    ]
  ], [
    a owl:Restriction ;
    owl:onProperty ns2:hasDimension ;
    owl:hasValue ns2:MagneticField-Dimension
  ] ;
  ns2:symbol "H" ;
  ns2:commonlyHasUnit ns2:amperePerMetre, ns2:oersted .

ns2:MagneticFluxDensity
  a owl:Class ;
  rdfs:label "magnetic flux density"@en ;
  ns2:alternativeLabel "magnetic field"@en, "magnetic induction"@en ;
  rdfs:subClassOf ns2:Quantity, [
    a owl:Restriction ;
    owl:onProperty ns2:hasValue ;
    owl:allValuesFrom [
      a owl:Restriction ;
      owl:onProperty ns2:hasUnit ;
      owl:allValuesFrom ns2:MagneticFluxDensityUnit
    ]
  ], [
    a owl:Restriction ;
    owl:onProperty ns2:hasDimension ;
    owl:hasValue ns2:magneticFluxDensity-Dimension
  ] ;
  ns2:symbol "B" ;
  ns2:commonlyHasUnit ns2:weberPerSquareMetre, ns2:tesla, ns2:attotesla, ns2:centitesla, ns2:decatesla, ns2:decitesla, ns2:exatesla, ns2:femtotesla, ns2:gigatesla, ns2:hectotesla, ns2:kilotesla, ns2:megatesla, ns2:microtesla, ns2:millitesla, ns2:nanotesla, ns2:petatesla, ns2:picotesla, ns2:teratesla, ns2:gamma, ns2:gauss, ns2:stattesla, ns2:milligauss .

ns2:Permeance-Electromagnetic
  a owl:Class ;
  rdfs:label "permeance (electromagnetic)"@en ;
  ns2:alternativeLabel "electromagnetic permeance"@en ;
  rdfs:comment "Electromagnetic permeance is a measure of flux for a number of current-turns in magnetic circuit."@en ;
  rdfs:subClassOf ns2:Quantity, [
    a owl:Restriction ;
    owl:onProperty ns2:hasValue ;
    owl:allValuesFrom [
      a owl:Restriction ;
      owl:onProperty ns2:hasUnit ;
      owl:allValuesFrom ns2:Permeance-ElectromagneticUnit
    ]
  ], [
    a owl:Restriction ;
    owl:onProperty ns2:hasDimension ;
    owl:hasValue ns2:inductanceOrPermeance-Electromagnetic-Dimension
  ] ;
  ns2:symbol "Λ" ;
  ns2:commonlyHasUnit ns2:weberPerAmpere, ns2:attohenry, ns2:centihenry, ns2:decahenry, ns2:decihenry, ns2:exahenry, ns2:femtohenry, ns2:gigahenry, ns2:hectohenry, ns2:kilohenry, ns2:megahenry, ns2:microhenry, ns2:millihenry, ns2:nanohenry, ns2:petahenry, ns2:picohenry, ns2:terahenry .

ns2:Inductance
  a owl:Class ;
  rdfs:label "inductance"@en ;
  rdfs:comment "Inductance is that property in an electrical circuit where a change in the current flowing through that circuit induces an electromotive force that opposes the change in current."@en ;
  rdfs:subClassOf ns2:Quantity, [
    a owl:Restriction ;
    owl:onProperty ns2:hasValue ;
    owl:allValuesFrom [
      a owl:Restriction ;
      owl:onProperty ns2:hasUnit ;
      owl:allValuesFrom ns2:InductanceUnit
    ]
  ], [
    a owl:Restriction ;
    owl:onProperty ns2:hasDimension ;
    owl:hasValue ns2:inductanceOrPermeance-Electromagnetic-Dimension
  ] ;
  ns2:commonlyHasUnit ns2:weberPerAmpere, ns2:henry, ns2:attohenry, ns2:centihenry, ns2:decahenry, ns2:decihenry, ns2:exahenry, ns2:femtohenry, ns2:gigahenry, ns2:hectohenry, ns2:kilohenry, ns2:megahenry, ns2:microhenry, ns2:millihenry, ns2:nanohenry, ns2:petahenry, ns2:picohenry, ns2:terahenry, ns2:abhenry, ns2:stathenry .

ns2:PermeabilityOfFreeSpace
  a owl:Class ;
  rdfs:label "permeability of free space"@en ;
  ns2:alternativeLabel "vacuum permeability"@en ;
  rdfs:subClassOf ns2:Quantity, [
    a owl:Restriction ;
    owl:onProperty ns2:hasValue ;
    owl:allValuesFrom [
      a owl:Restriction ;
      owl:onProperty ns2:hasUnit ;
      owl:allValuesFrom ns2:PermeabilityOfFreeSpaceUnit
    ]
  ], [
    a owl:Restriction ;
    owl:onProperty ns2:hasDimension ;
    owl:hasValue ns2:permeabilityOfFreeSpace-Dimension
  ] ;
  ns2:symbol "μ" ;
  ns2:commonlyHasUnit ns2:henryPerMetre .

ns2:Permittivity
  a owl:Class ;
  rdfs:label "permittivity"@en ;
  rdfs:subClassOf ns2:Quantity, [
    a owl:Restriction ;
    owl:onProperty ns2:hasValue ;
    owl:allValuesFrom [
      a owl:Restriction ;
      owl:onProperty ns2:hasUnit ;
      owl:allValuesFrom ns2:PermittivityUnit
    ]
  ], [
    a owl:Restriction ;
    owl:onProperty ns2:hasDimension ;
    owl:hasValue ns2:permittivity-Dimension
  ] ;
  ns2:symbol "ε" ;
  ns2:commonlyHasUnit ns2:faradPerMetre .

ns2:ElectricDipoleMoment
  a owl:Class ;
  rdfs:label "electric dipole moment"@en ;
  rdfs:comment "Electric dipole moment is a measure of the polarity of a system of electric charges."@en ;
  rdfs:subClassOf ns2:Quantity, [
    a owl:Restriction ;
    owl:onProperty ns2:hasValue ;
    owl:allValuesFrom [
      a owl:Restriction ;
      owl:onProperty ns2:hasUnit ;
      owl:allValuesFrom ns2:ElectricDipoleMomentUnit
    ]
  ], [
    a owl:Restriction ;
    owl:onProperty ns2:hasDimension ;
    owl:hasValue ns2:electricDipoleMoment-Dimension
  ] ;
  ns2:symbol "p" ;
  ns2:commonlyHasUnit ns2:coulombMetre, ns2:debye .

ns2:Reluctance
  a owl:Class ;
  rdfs:label "reluctance"@en ;
  rdfs:subClassOf ns2:Quantity, [
    a owl:Restriction ;
    owl:onProperty ns2:hasValue ;
    owl:allValuesFrom [
      a owl:Restriction ;
      owl:onProperty ns2:hasUnit ;
      owl:allValuesFrom ns2:ReluctanceUnit
    ]
  ], [
    a owl:Restriction ;
    owl:onProperty ns2:hasDimension ;
    owl:hasValue ns2:reluctance-Dimension
  ] ;
  ns2:symbol "τ" ;
  ns2:commonlyHasUnit ns2:reciprocalHenry .

ns2:Admittance
  a owl:Class ;
  rdfs:label "admittance"@en ;
  rdfs:comment "Admittance is a measure of how easily a circuit or device will allow a current to flow. It is electric current divided by electric potential."@en ;
  rdfs:subClassOf ns2:Quantity ;
  ns2:symbol "Y" .

ns2:ElectricalResistivity
  a owl:Class ;
  rdfs:label "electrical resistivity"@en ;
  rdfs:subClassOf ns2:Quantity, [
    a owl:Restriction ;
    owl:onProperty ns2:hasValue ;
    owl:allValuesFrom [
      a owl:Restriction ;
      owl:onProperty ns2:hasUnit ;
      owl:allValuesFrom ns2:ElectricalResistivityUnit
    ]
  ], [
    a owl:Restriction ;
    owl:onProperty ns2:hasDimension ;
    owl:hasValue ns2:electricalResistivity-Dimension
  ] ;
  ns2:commonlyHasUnit ns2:ohmMetre .

ns2:ElectricalConductivity
  a owl:Class ;
  rdfs:label "electrical conductivity"@en ;
  rdfs:subClassOf ns2:Quantity, [
    a owl:Restriction ;
    owl:onProperty ns2:hasValue ;
    owl:allValuesFrom [
      a owl:Restriction ;
      owl:onProperty ns2:hasUnit ;
      owl:allValuesFrom ns2:ElectricalConductivityUnit
    ]
  ], [
    a owl:Restriction ;
    owl:onProperty ns2:hasDimension ;
    owl:hasValue ns2:electricalConductivity-Dimension
  ] ;
  ns2:commonlyHasUnit ns2:siemensPerMetre .

ns2:MagnetomotiveForce
  a owl:Class ;
  rdfs:label "magnetomotive force"@en ;
  rdfs:subClassOf ns2:Quantity, [
    a owl:Restriction ;
    owl:onProperty ns2:hasValue ;
    owl:allValuesFrom [
      a owl:Restriction ;
      owl:onProperty ns2:hasUnit ;
      owl:allValuesFrom ns2:MagnetomotiveForceUnit
    ]
  ], [
    a owl:Restriction ;
    owl:onProperty ns2:hasDimension ;
    owl:hasValue ns2:electricCurrent-Dimension
  ] ;
  ns2:symbol "F" ;
  ns2:commonlyHasUnit ns2:ampere, ns2:attoampere, ns2:centiampere, ns2:decaampere, ns2:deciampere, ns2:exaampere, ns2:femtoampere, ns2:gigaampere, ns2:hectoampere, ns2:kiloampere, ns2:megaampere, ns2:microampere, ns2:milliampere, ns2:nanoampere, ns2:petaampere, ns2:picoampere, ns2:teraampere, ns2:gilbert .

ns2:ampere
  a ns2:Unit, ns2:SingularUnit ;
  rdfs:label "ampere"@en, "ampère"@nl ;
  ns2:symbol "A" ;
  ns2:hasDimension ns2:electricCurrent-Dimension ;
  rdfs:comment "The ampere is a unit of electric current defined as the constant current that produces an attractive force of 2e–7 newton per metre of length between two straight, parallel conductors of infinite length and negligible circular cross section placed one metre apart in a vacuum."@en ;
  ns2:longcomment "The ampere is a unit of electric current defined as the constant current that produces an attractive force of 2e–7 newton per metre of length between two straight, parallel conductors of infinite length and negligible circular cross section placed one metre apart in a vacuum. The ampere is a base unit in the International System of Units." ;
  ns2:hasQuantity ns2:constantCurrentThatProducesAnAttractiveForceOf2e-7NewtonPerMetreOfLengthBetweenTwoStraightParallelConductorsOfInfiniteLengthAndNegligibleCircularCrossSectionPlacedOneMetreApartInAVacuum .

ns2:constantCurrentThatProducesAnAttractiveForceOf2e-7NewtonPerMetreOfLengthBetweenTwoStraightParallelConductorsOfInfiniteLengthAndNegligibleCircularCrossSectionPlacedOneMetreApartInAVacuum
  a ns2:ElectricCurrent ;
  rdfs:label "constant current that produces an attractive force of 2e–7 newton per metre of length between two straight, parallel conductors of infinite length and negligible circular cross section placed one metre apart in a vacuum"@en .

ns2:ElectricCurrentUnit
  a owl:Class ;
  rdfs:label "electric current unit"@en ;
  rdfs:subClassOf ns2:Unit ;
  owl:equivalentClass [
    a owl:Class ;
    owl:unionOf (
     _:genid1064
     ns2:PrefixedAmpere
   )
  ] .

ns2:abampere
  a ns2:Unit, ns2:SingularUnit ;
  rdfs:label "abampere"@en, "abampère"@nl ;
  rdfs:comment "The abampere is a unit of electric current defined as 10 ampere."@en ;
  ns2:symbol "abA" ;
  ns2:hasFactor "1.0e1"^^xsd:float ;
  ns2:hasUnit ns2:ampere ;
  ns2:hasDimension ns2:electricCurrent-Dimension .

ns2:biot
  a ns2:Unit, ns2:SingularUnit ;
  rdfs:label "biot"@en, "biot"@nl ;
  rdfs:comment "The biot is a unit of electric current defined as 10 ampere."@en ;
  ns2:symbol "Bi" ;
  ns2:hasFactor "1.0e1"^^xsd:float ;
  ns2:hasUnit ns2:ampere ;
  ns2:hasDimension ns2:electricCurrent-Dimension .

ns2:statampere
  a ns2:Unit, ns2:SingularUnit ;
  rdfs:label "statampere"@en, "statampère"@nl ;
  rdfs:comment "The statampere is a unit of electric current defined as 3.335641e-10 ampere."@en ;
  ns2:symbol "statA" ;
  ns2:hasFactor "3.335641e-10"^^xsd:float ;
  ns2:hasUnit ns2:ampere ;
  ns2:hasDimension ns2:electricCurrent-Dimension .

ns2:PrefixedAmpere
  a owl:Class ;
  rdfs:label "prefixed ampere"@en ;
  rdfs:subClassOf ns2:PrefixedUnit ;
  owl:equivalentClass [
    a owl:Class ;
    owl:intersectionOf (
     _:genid1081
     _:genid1083
     _:genid1085
     _:genid1087
   )
  ] .

ns2:MagnetomotiveForceUnit
  a owl:Class ;
  rdfs:label "magnetomotive force unit"@en ;
  rdfs:subClassOf ns2:Unit ;
  owl:equivalentClass [
    a owl:Class ;
    owl:unionOf (
     _:genid1072
     ns2:PrefixedAmpere
   )
  ] .

ns2:gilbert
  a ns2:Unit, ns2:SingularUnit ;
  rdfs:label "gilbert"@en, "gilbert"@nl ;
  rdfs:comment "The gilbert is a unit of electric current defined as 7.957747e-1 ampere."@en ;
  ns2:symbol "Gb" ;
  ns2:hasFactor "7.957747e-1"^^xsd:float ;
  ns2:hasUnit ns2:ampere ;
  ns2:hasDimension ns2:electricCurrent-Dimension .

ns2:yoctoampere
  a ns2:PrefixedUnit ;
  rdfs:label "yoctoampere"@en, "yoctoampère"@nl ;
  rdfs:comment "The yoctoampere is a unit of electric current defined as 1.0e-24 ampere."@en ;
  ns2:symbol "yA" ;
  ns2:hasPrefix ns2:yocto ;
  ns2:hasUnit ns2:ampere ;
  ns2:hasDimension ns2:electricCurrent-Dimension .

ns2:zeptoampere
  a ns2:PrefixedUnit ;
  rdfs:label "zeptoampere"@en, "zeptoampère"@nl ;
  rdfs:comment "The zeptampere is a unit of electric current defined as 1.0e-21 ampere."@en ;
  ns2:symbol "zA" ;
  ns2:hasPrefix ns2:zepto ;
  ns2:hasUnit ns2:ampere ;
  ns2:hasDimension ns2:electricCurrent-Dimension .

ns2:attoampere
  a ns2:PrefixedUnit ;
  rdfs:label "attoampere"@en, "attoampère"@nl ;
  rdfs:comment "The attoampere is a unit of electric current defined as 1.0e-18 ampere."@en ;
  ns2:symbol "aA" ;
  ns2:hasPrefix ns2:atto ;
  ns2:hasUnit ns2:ampere ;
  ns2:hasDimension ns2:electricCurrent-Dimension .

ns2:femtoampere
  a ns2:PrefixedUnit ;
  rdfs:label "femtoampere"@en, "femtoampère"@nl ;
  rdfs:comment "The femtoampere is a unit of electric current defined as 1.0e-15 ampere."@en ;
  ns2:symbol "fA" ;
  ns2:hasPrefix ns2:femto ;
  ns2:hasUnit ns2:ampere ;
  ns2:hasDimension ns2:electricCurrent-Dimension .

ns2:picoampere
  a ns2:PrefixedUnit ;
  rdfs:label "picoampere"@en, "picoampère"@nl ;
  rdfs:comment "The picoampere is a unit of electric current defined as 1.0e-12 ampere."@en ;
  ns2:symbol "pA" ;
  ns2:hasPrefix ns2:pico ;
  ns2:hasUnit ns2:ampere ;
  ns2:hasDimension ns2:electricCurrent-Dimension .

ns2:nanoampere
  a ns2:PrefixedUnit ;
  rdfs:label "nanoampere"@en, "nanoampère"@nl ;
  rdfs:comment "The nanoampere is a unit of electric current defined as 1.0e-9 ampere."@en ;
  ns2:symbol "nA" ;
  ns2:hasPrefix ns2:nano ;
  ns2:hasUnit ns2:ampere ;
  ns2:hasDimension ns2:electricCurrent-Dimension .

ns2:microampere
  a ns2:PrefixedUnit ;
  rdfs:label "microampere"@en, "microampère"@nl ;
  rdfs:comment "The microampere is a unit of electric current defined as 1.0e-6 ampere."@en ;
  ns2:symbol "μA" ;
  ns2:hasPrefix ns2:micro ;
  ns2:hasUnit ns2:ampere ;
  ns2:hasDimension ns2:electricCurrent-Dimension .

ns2:milliampere
  a ns2:PrefixedUnit ;
  rdfs:label "milliampere"@en, "milliampère"@nl ;
  rdfs:comment "The milliampere is a unit of electric current defined as 1.0e-3 ampere."@en ;
  ns2:symbol "mA" ;
  ns2:hasPrefix ns2:milli ;
  ns2:hasUnit ns2:ampere ;
  ns2:hasDimension ns2:electricCurrent-Dimension .

ns2:centiampere
  a ns2:PrefixedUnit ;
  rdfs:label "centiampere"@en, "centiampère"@nl ;
  rdfs:comment "The centiampere is a unit of electric current defined as 1.0e-2 ampere."@en ;
  ns2:symbol "cA" ;
  ns2:hasPrefix ns2:centi ;
  ns2:hasUnit ns2:ampere ;
  ns2:hasDimension ns2:electricCurrent-Dimension .

ns2:deciampere
  a ns2:PrefixedUnit ;
  rdfs:label "deciampere"@en, "deciampère"@nl ;
  rdfs:comment "The deciampere is a unit of electric current defined as 1.0e-1 ampere."@en ;
  ns2:symbol "dA" ;
  ns2:hasPrefix ns2:deci ;
  ns2:hasUnit ns2:ampere ;
  ns2:hasDimension ns2:electricCurrent-Dimension .

ns2:decaampere
  a ns2:PrefixedUnit ;
  rdfs:label "decaampere"@en, "decaampère"@nl ;
  rdfs:comment "The decaampere is a unit of electric current defined as 1.0e1 ampere."@en ;
  ns2:symbol "daA" ;
  ns2:hasPrefix ns2:deca ;
  ns2:hasUnit ns2:ampere ;
  ns2:hasDimension ns2:electricCurrent-Dimension .

ns2:hectoampere
  a ns2:PrefixedUnit ;
  rdfs:label "hectoampere"@en, "hectoampère"@nl ;
  rdfs:comment "The hectoampere is a unit of electric current defined as 1.0e2 ampere."@en ;
  ns2:symbol "hA" ;
  ns2:hasPrefix ns2:hecto ;
  ns2:hasUnit ns2:ampere ;
  ns2:hasDimension ns2:electricCurrent-Dimension .

ns2:kiloampere
  a ns2:PrefixedUnit ;
  rdfs:label "kiloampere"@en, "kiloampère"@nl ;
  rdfs:comment "The kiloampere is a unit of electric current defined as 1.0e3 ampere."@en ;
  ns2:symbol "kA" ;
  ns2:hasPrefix ns2:kilo ;
  ns2:hasUnit ns2:ampere ;
  ns2:hasDimension ns2:electricCurrent-Dimension .

ns2:megaampere
  a ns2:PrefixedUnit ;
  rdfs:label "megaampere"@en, "megaampère"@nl ;
  rdfs:comment "The megaampere is a unit of electric current defined as 1.0e6 ampere."@en ;
  ns2:symbol "MA" ;
  ns2:hasPrefix ns2:mega ;
  ns2:hasUnit ns2:ampere ;
  ns2:hasDimension ns2:electricCurrent-Dimension .

ns2:gigaampere
  a ns2:PrefixedUnit ;
  rdfs:label "gigaampere"@en, "gigaampère"@nl ;
  rdfs:comment "The gigaampere is a unit of electric current defined as 1.0e9 ampere."@en ;
  ns2:symbol "GA" ;
  ns2:hasPrefix ns2:giga ;
  ns2:hasUnit ns2:ampere ;
  ns2:hasDimension ns2:electricCurrent-Dimension .

ns2:teraampere
  a ns2:PrefixedUnit ;
  rdfs:label "teraampere"@en, "teraampère"@nl ;
  rdfs:comment "The teraampere is a unit of electric current defined as 1.0e12 ampere."@en ;
  ns2:symbol "TA" ;
  ns2:hasPrefix ns2:tera ;
  ns2:hasUnit ns2:ampere ;
  ns2:hasDimension ns2:electricCurrent-Dimension .

ns2:petaampere
  a ns2:PrefixedUnit ;
  rdfs:label "petaampere"@en, "petaampère"@nl ;
  rdfs:comment "The petaampere is a unit of electric current defined as 1.0e15 ampere."@en ;
  ns2:symbol "PA" ;
  ns2:hasPrefix ns2:peta ;
  ns2:hasUnit ns2:ampere ;
  ns2:hasDimension ns2:electricCurrent-Dimension .

ns2:exaampere
  a ns2:PrefixedUnit ;
  rdfs:label "exaampere"@en, "exaampère"@nl ;
  rdfs:comment "The exaampere is a unit of electric current defined as 1.0e18 ampere."@en ;
  ns2:symbol "EA" ;
  ns2:hasPrefix ns2:exa ;
  ns2:hasUnit ns2:ampere ;
  ns2:hasDimension ns2:electricCurrent-Dimension .

ns2:zettaampere
  a ns2:PrefixedUnit ;
  rdfs:label "zettaampere"@en, "zettaampère"@nl ;
  rdfs:comment "The zettaampere is a unit of electric current defined as 1.0e21 ampere."@en ;
  ns2:symbol "ZA" ;
  ns2:hasPrefix ns2:zetta ;
  ns2:hasUnit ns2:ampere ;
  ns2:hasDimension ns2:electricCurrent-Dimension .

ns2:yottaampere
  a ns2:PrefixedUnit ;
  rdfs:label "yottaampere"@en, "yottaampère"@nl ;
  rdfs:comment "The yottaampere is a unit of electric current defined as 1.0e24 ampere."@en ;
  ns2:symbol "YA" ;
  ns2:hasPrefix ns2:yotta ;
  ns2:hasUnit ns2:ampere ;
  ns2:hasDimension ns2:electricCurrent-Dimension .

ns2:amperePerSquareMetre
  a ns2:UnitDivision ;
  rdfs:label "ampere per square metre"@en, "ampère per vierkante meter"@nl ;
  rdfs:comment "Ampere per square metre is a unit of current density defined as ampere divided by square metre."@en ;
  ns2:longcomment "Ampere per square metre is a unit of current density defined as ampere divided by square metre. Ampere per square metre is a derived unit in the International System of Units." ;
  ns2:symbol "A/m2" ;
  ns2:alternativeSymbol "A m-2", "A·m-2" ;
  ns2:hasNumerator ns2:ampere ;
  ns2:hasDenominator ns2:squareMetre ;
  ns2:hasDimension ns2:currentDensity-Dimension .

ns2:CurrentDensityUnit
  a owl:Class ;
  rdfs:label "current density unit"@en ;
  rdfs:subClassOf ns2:Unit ;
  owl:equivalentClass [
    a owl:Class ;
    owl:oneOf ( ns2:amperePerSquareMetre )
  ] .

ns2:second-TimeAmpere
  a ns2:UnitMultiplication ;
  rdfs:label "second ampere"@en, "seconde ampère"@nl ;
  ns2:symbol "s A" ;
  ns2:alternativeSymbol "s·A" ;
  ns2:hasTerm1 ns2:second-Time ;
  ns2:hasTerm2 ns2:ampere ;
  ns2:hasDimension ns2:electricCharge-Dimension .

ns2:ElectricChargeUnit
  a owl:Class ;
  rdfs:label "electric charge unit"@en ;
  rdfs:subClassOf ns2:Unit ;
  owl:equivalentClass [
    a owl:Class ;
    owl:unionOf (
     _:genid1094
     ns2:PrefixedCoulomb
   )
  ] .

ns2:abcoulomb
  a ns2:Unit, ns2:SingularUnit ;
  rdfs:label "abcoulomb"@en, "abcoulomb"@nl ;
  rdfs:comment "The abcoulomb is a unit of electric charge defined as 10 coulomb."@en ;
  ns2:symbol "abC" ;
  ns2:hasFactor "1.0e1"^^xsd:float ;
  ns2:hasUnit ns2:coulomb ;
  ns2:hasDimension ns2:electricCharge-Dimension .

ns2:coulomb
  a ns2:Unit, ns2:SingularUnit ;
  rdfs:label "coulomb"@en, "coulomb"@nl ;
  rdfs:comment "The coulomb is a unit of electric charge defined as ampere times second = farad times volt."@en ;
  ns2:longcomment "The coulomb is a unit of electric charge defined as ampere times second = farad times volt. The coulomb is a derived unit in the International System of Units." ;
  ns2:symbol "C" ;
  ns2:hasUnit ns2:second-TimeAmpere ;
  ns2:hasDimension ns2:electricCharge-Dimension .

ns2:faraday
  a ns2:Unit, ns2:SingularUnit ;
  rdfs:label "faraday"@en, "faraday"@nl ;
  rdfs:comment "The faraday is a unit of electric charge defined as 9.648531e4 coulomb."@en ;
  ns2:hasDimension ns2:electricCharge-Dimension .

ns2:franklin
  a ns2:Unit, ns2:SingularUnit ;
  rdfs:label "franklin"@en, "franklin"@nl ;
  rdfs:comment "The franklin is a unit of electric charge defined as 3.335641e-10 coulomb."@en ;
  ns2:symbol "Fr" ;
  ns2:hasFactor "3.335641e-10"^^xsd:float ;
  ns2:hasUnit ns2:coulomb ;
  ns2:hasDimension ns2:electricCharge-Dimension .

ns2:statcoulomb
  a ns2:Unit, ns2:SingularUnit ;
  rdfs:label "statcoulomb"@en, "statcoulomb"@nl ;
  rdfs:comment "The statcoulomb is a unit of electric charge defined as 3.335641e-10 coulomb."@en ;
  ns2:symbol "statC" ;
  ns2:hasFactor "3.335641e-10"^^xsd:float ;
  ns2:hasUnit ns2:coulomb ;
  ns2:hasDimension ns2:electricCharge-Dimension .

ns2:ampereHour
  a ns2:UnitMultiplication ;
  rdfs:label "ampere hour"@en, "ampère-uur"@nl ;
  ns2:symbol "A h" ;
  ns2:alternativeSymbol "A·h", "Ah" ;
  ns2:hasTerm1 ns2:ampere ;
  ns2:hasTerm2 ns2:hour ;
  ns2:hasDimension ns2:electricCharge-Dimension .

ns2:milliampereHour
  a ns2:UnitMultiplication ;
  rdfs:label "milliampere hour"@en, "milliampère-uur"@nl ;
  ns2:symbol "mA h" ;
  ns2:alternativeSymbol "mA·h", "mAh" ;
  ns2:hasTerm1 ns2:milliampere ;
  ns2:hasTerm2 ns2:hour ;
  ns2:hasDimension ns2:electricCharge-Dimension .

ns2:PrefixedCoulomb
  a owl:Class ;
  rdfs:label "prefixed coulomb"@en ;
  rdfs:subClassOf ns2:PrefixedUnit ;
  owl:equivalentClass [
    a owl:Class ;
    owl:intersectionOf (
     _:genid1108
     _:genid1110
     _:genid1112
     _:genid1114
   )
  ] .

ns2:yoctocoulomb
  a ns2:PrefixedUnit ;
  rdfs:label "yoctocoulomb"@en, "yoctocoulomb"@nl ;
  rdfs:comment "The yoctocoulomb is a unit of electric charge defined as 1.0e-24 coulomb."@en ;
  ns2:symbol "yC" ;
  ns2:hasPrefix ns2:yocto ;
  ns2:hasUnit ns2:coulomb ;
  ns2:hasDimension ns2:electricCharge-Dimension .

ns2:zeptocoulomb
  a ns2:PrefixedUnit ;
  rdfs:label "zeptocoulomb"@en, "zeptocoulomb"@nl ;
  rdfs:comment "The zeptcoulomb is a unit of electric charge defined as 1.0e-21 coulomb."@en ;
  ns2:symbol "zC" ;
  ns2:hasPrefix ns2:zepto ;
  ns2:hasUnit ns2:coulomb ;
  ns2:hasDimension ns2:electricCharge-Dimension .

ns2:attocoulomb
  a ns2:PrefixedUnit ;
  rdfs:label "attocoulomb"@en, "attocoulomb"@nl ;
  rdfs:comment "The attocoulomb is a unit of electric charge defined as 1.0e-18 coulomb."@en ;
  ns2:symbol "aC" ;
  ns2:hasPrefix ns2:atto ;
  ns2:hasUnit ns2:coulomb ;
  ns2:hasDimension ns2:electricCharge-Dimension .

ns2:femtocoulomb
  a ns2:PrefixedUnit ;
  rdfs:label "femtocoulomb"@en, "femtocoulomb"@nl ;
  rdfs:comment "The femtocoulomb is a unit of electric charge defined as 1.0e-15 coulomb."@en ;
  ns2:symbol "fC" ;
  ns2:hasPrefix ns2:femto ;
  ns2:hasUnit ns2:coulomb ;
  ns2:hasDimension ns2:electricCharge-Dimension .

ns2:picocoulomb
  a ns2:PrefixedUnit ;
  rdfs:label "picocoulomb"@en, "picocoulomb"@nl ;
  rdfs:comment "The picocoulomb is a unit of electric charge defined as 1.0e-12 coulomb."@en ;
  ns2:symbol "pC" ;
  ns2:hasPrefix ns2:pico ;
  ns2:hasUnit ns2:coulomb ;
  ns2:hasDimension ns2:electricCharge-Dimension .

ns2:nanocoulomb
  a ns2:PrefixedUnit ;
  rdfs:label "nanocoulomb"@en, "nanocoulomb"@nl ;
  rdfs:comment "The nanocoulomb is a unit of electric charge defined as 1.0e-9 coulomb."@en ;
  ns2:symbol "nC" ;
  ns2:hasPrefix ns2:nano ;
  ns2:hasUnit ns2:coulomb ;
  ns2:hasDimension ns2:electricCharge-Dimension .

ns2:microcoulomb
  a ns2:PrefixedUnit ;
  rdfs:label "microcoulomb"@en, "microcoulomb"@nl ;
  rdfs:comment "The microcoulomb is a unit of electric charge defined as 1.0e-6 coulomb."@en ;
  ns2:symbol "μC" ;
  ns2:hasPrefix ns2:micro ;
  ns2:hasUnit ns2:coulomb ;
  ns2:hasDimension ns2:electricCharge-Dimension .

ns2:millicoulomb
  a ns2:PrefixedUnit ;
  rdfs:label "millicoulomb"@en, "millicoulomb"@nl ;
  rdfs:comment "The millicoulomb is a unit of electric charge defined as 1.0e-3 coulomb."@en ;
  ns2:symbol "mC" ;
  ns2:hasPrefix ns2:milli ;
  ns2:hasUnit ns2:coulomb ;
  ns2:hasDimension ns2:electricCharge-Dimension .

ns2:centicoulomb
  a ns2:PrefixedUnit ;
  rdfs:label "centicoulomb"@en, "centicoulomb"@nl ;
  rdfs:comment "The centicoulomb is a unit of electric charge defined as 1.0e-2 coulomb."@en ;
  ns2:symbol "cC" ;
  ns2:hasPrefix ns2:centi ;
  ns2:hasUnit ns2:coulomb ;
  ns2:hasDimension ns2:electricCharge-Dimension .

ns2:decicoulomb
  a ns2:PrefixedUnit ;
  rdfs:label "decicoulomb"@en, "decicoulomb"@nl ;
  rdfs:comment "The decicoulomb is a unit of electric charge defined as 1.0e-1 coulomb."@en ;
  ns2:symbol "dC" ;
  ns2:hasPrefix ns2:deci ;
  ns2:hasUnit ns2:coulomb ;
  ns2:hasDimension ns2:electricCharge-Dimension .

ns2:decacoulomb
  a ns2:PrefixedUnit ;
  rdfs:label "decacoulomb"@en, "decacoulomb"@nl ;
  rdfs:comment "The decacoulomb is a unit of electric charge defined as 1.0e1 coulomb."@en ;
  ns2:symbol "daC" ;
  ns2:hasPrefix ns2:deca ;
  ns2:hasUnit ns2:coulomb ;
  ns2:hasDimension ns2:electricCharge-Dimension .

ns2:hectocoulomb
  a ns2:PrefixedUnit ;
  rdfs:label "hectocoulomb"@en, "hectocoulomb"@nl ;
  rdfs:comment "The hectocoulomb is a unit of electric charge defined as 1.0e2 coulomb."@en ;
  ns2:symbol "hC" ;
  ns2:hasPrefix ns2:hecto ;
  ns2:hasUnit ns2:coulomb ;
  ns2:hasDimension ns2:electricCharge-Dimension .

ns2:kilocoulomb
  a ns2:PrefixedUnit ;
  rdfs:label "kilocoulomb"@en, "kilocoulomb"@nl ;
  rdfs:comment "The kilocoulomb is a unit of electric charge defined as 1.0e3 coulomb."@en ;
  ns2:symbol "kC" ;
  ns2:hasPrefix ns2:kilo ;
  ns2:hasUnit ns2:coulomb ;
  ns2:hasDimension ns2:electricCharge-Dimension .

ns2:megacoulomb
  a ns2:PrefixedUnit ;
  rdfs:label "megacoulomb"@en, "megacoulomb"@nl ;
  rdfs:comment "The megacoulomb is a unit of electric charge defined as 1.0e6 coulomb."@en ;
  ns2:symbol "MC" ;
  ns2:hasPrefix ns2:mega ;
  ns2:hasUnit ns2:coulomb ;
  ns2:hasDimension ns2:electricCharge-Dimension .

ns2:gigacoulomb
  a ns2:PrefixedUnit ;
  rdfs:label "gigacoulomb"@en, "gigacoulomb"@nl ;
  rdfs:comment "The gigacoulomb is a unit of electric charge defined as 1.0e9 coulomb."@en ;
  ns2:symbol "GC" ;
  ns2:hasPrefix ns2:giga ;
  ns2:hasUnit ns2:coulomb ;
  ns2:hasDimension ns2:electricCharge-Dimension .

ns2:teracoulomb
  a ns2:PrefixedUnit ;
  rdfs:label "teracoulomb"@en, "teracoulomb"@nl ;
  rdfs:comment "The teracoulomb is a unit of electric charge defined as 1.0e12 coulomb."@en ;
  ns2:symbol "TC" ;
  ns2:hasPrefix ns2:tera ;
  ns2:hasUnit ns2:coulomb ;
  ns2:hasDimension ns2:electricCharge-Dimension .

ns2:petacoulomb
  a ns2:PrefixedUnit ;
  rdfs:label "petacoulomb"@en, "petacoulomb"@nl ;
  rdfs:comment "The petacoulomb is a unit of electric charge defined as 1.0e15 coulomb."@en ;
  ns2:symbol "PC" ;
  ns2:hasPrefix ns2:peta ;
  ns2:hasUnit ns2:coulomb ;
  ns2:hasDimension ns2:electricCharge-Dimension .

ns2:exacoulomb
  a ns2:PrefixedUnit ;
  rdfs:label "exacoulomb"@en, "exacoulomb"@nl ;
  rdfs:comment "The exacoulomb is a unit of electric charge defined as 1.0e18 coulomb."@en ;
  ns2:symbol "EC" ;
  ns2:hasPrefix ns2:exa ;
  ns2:hasUnit ns2:coulomb ;
  ns2:hasDimension ns2:electricCharge-Dimension .

ns2:zettacoulomb
  a ns2:PrefixedUnit ;
  rdfs:label "zettacoulomb"@en, "zettacoulomb"@nl ;
  rdfs:comment "The zettacoulomb is a unit of electric charge defined as 1.0e21 coulomb."@en ;
  ns2:symbol "ZC" ;
  ns2:hasPrefix ns2:zetta ;
  ns2:hasUnit ns2:coulomb ;
  ns2:hasDimension ns2:electricCharge-Dimension .

ns2:yottacoulomb
  a ns2:PrefixedUnit ;
  rdfs:label "yottacoulomb"@en, "yottacoulomb"@nl ;
  rdfs:comment "The yottacoulomb is a unit of electric charge defined as 1.0e24 coulomb."@en ;
  ns2:symbol "YC" ;
  ns2:hasPrefix ns2:yotta ;
  ns2:hasUnit ns2:coulomb ;
  ns2:hasDimension ns2:electricCharge-Dimension .

ns2:wattPerAmpere
  a ns2:UnitDivision ;
  rdfs:label "watt per ampere"@en, "watt per ampère"@nl ;
  ns2:symbol "W/A" ;
  ns2:alternativeSymbol "W A-1", "W·A-1" ;
  ns2:hasNumerator ns2:watt ;
  ns2:hasDenominator ns2:ampere ;
  ns2:hasDimension ns2:electricPotential-Dimension .

ns2:ElectricPotentialUnit
  a owl:Class ;
  rdfs:label "electric potential unit"@en ;
  rdfs:subClassOf ns2:Unit ;
  owl:equivalentClass [
    a owl:Class ;
    owl:unionOf (
     _:genid1117
     ns2:PrefixedVolt
   )
  ] .

ns2:abvolt
  a ns2:SingularUnit, ns2:Unit ;
  rdfs:label "abvolt"@en, "abvolt"@nl ;
  rdfs:comment "The abvolt is a unit of electric potential defined as 1.0e-8 volt."@en ;
  ns2:symbol "abV" ;
  ns2:hasFactor "1.0e-8"^^xsd:float ;
  ns2:hasUnit ns2:volt ;
  ns2:hasDimension ns2:electricPotential-Dimension .

ns2:statvolt
  a ns2:SingularUnit, ns2:Unit ;
  rdfs:label "statvolt"@en, "statvolt"@nl ;
  rdfs:comment "The statvolt is a unit of electric potential defined as 2.997925e2 volt."@en ;
  ns2:symbol "statV" ;
  ns2:hasFactor "2.997925e2"^^xsd:float ;
  ns2:hasUnit ns2:volt ;
  ns2:hasDimension ns2:electricPotential-Dimension .

ns2:volt
  a ns2:SingularUnit, ns2:Unit ;
  rdfs:label "volt"@en, "volt"@nl ;
  rdfs:comment "The volt is a unit of electric potential defined as watt divided by ampere = joule divided by coulomb = newton times metre divided by ampere times second = kilogram times square metre divided by ampere times second to the power 3."@en ;
  ns2:longcomment "The volt is a unit of electric potential defined as watt divided by ampere = joule divided by coulomb = newton times metre divided by ampere times second = kilogram times square metre divided by ampere times second to the power 3. The volt is a derived unit in the International System of Units." ;
  ns2:symbol "V" ;
  ns2:hasUnit ns2:wattPerAmpere ;
  ns2:hasDimension ns2:electricPotential-Dimension .

ns2:PrefixedVolt
  a owl:Class ;
  rdfs:label "prefixed volt"@en ;
  rdfs:subClassOf ns2:PrefixedUnit ;
  owl:equivalentClass [
    a owl:Class ;
    owl:intersectionOf (
     _:genid1127
     _:genid1129
     _:genid1131
     _:genid1133
   )
  ] .

ns2:yoctovolt
  a ns2:PrefixedUnit ;
  rdfs:label "yoctovolt"@en, "yoctovolt"@nl ;
  ns2:symbol "yV" ;
  ns2:hasPrefix ns2:yocto ;
  ns2:hasUnit ns2:volt ;
  ns2:hasDimension ns2:electricPotential-Dimension .

ns2:zeptovolt
  a ns2:PrefixedUnit ;
  rdfs:label "zeptovolt"@en, "zeptovolt"@nl ;
  ns2:symbol "zV" ;
  ns2:hasPrefix ns2:zepto ;
  ns2:hasUnit ns2:volt ;
  ns2:hasDimension ns2:electricPotential-Dimension .

ns2:attovolt
  a ns2:PrefixedUnit ;
  rdfs:label "attovolt"@nl, "attovolt"@en ;
  ns2:symbol "aV" ;
  ns2:hasPrefix ns2:atto ;
  ns2:hasUnit ns2:volt ;
  ns2:hasDimension ns2:electricPotential-Dimension .

ns2:femtovolt
  a ns2:PrefixedUnit ;
  rdfs:label "femtovolt"@nl, "femtovolt"@en ;
  ns2:symbol "fV" ;
  ns2:hasPrefix ns2:femto ;
  ns2:hasUnit ns2:volt ;
  ns2:hasDimension ns2:electricPotential-Dimension .

ns2:picovolt
  a ns2:PrefixedUnit ;
  rdfs:label "picovolt"@nl, "picovolt"@en ;
  ns2:symbol "pV" ;
  ns2:hasPrefix ns2:pico ;
  ns2:hasUnit ns2:volt ;
  ns2:hasDimension ns2:electricPotential-Dimension .

ns2:nanovolt
  a ns2:PrefixedUnit ;
  rdfs:label "nanovolt"@nl, "nanovolt"@en ;
  ns2:symbol "nV" ;
  ns2:hasPrefix ns2:nano ;
  ns2:hasUnit ns2:volt ;
  ns2:hasDimension ns2:electricPotential-Dimension .

ns2:microvolt
  a ns2:PrefixedUnit ;
  rdfs:label "microvolt"@nl, "microvolt"@en ;
  ns2:symbol "μV" ;
  ns2:hasPrefix ns2:micro ;
  ns2:hasUnit ns2:volt ;
  ns2:hasDimension ns2:electricPotential-Dimension .

ns2:millivolt
  a ns2:PrefixedUnit ;
  rdfs:label "millivolt"@en, "millivolt"@nl ;
  ns2:symbol "mV" ;
  ns2:hasPrefix ns2:milli ;
  ns2:hasUnit ns2:volt ;
  ns2:hasDimension ns2:electricPotential-Dimension .

ns2:centivolt
  a ns2:PrefixedUnit ;
  rdfs:label "centivolt"@en, "centivolt"@nl ;
  ns2:symbol "cV" ;
  ns2:hasPrefix ns2:centi ;
  ns2:hasUnit ns2:volt ;
  ns2:hasDimension ns2:electricPotential-Dimension .

ns2:decivolt
  a ns2:PrefixedUnit ;
  rdfs:label "decivolt"@en, "decivolt"@nl ;
  ns2:symbol "dV" ;
  ns2:hasPrefix ns2:deci ;
  ns2:hasUnit ns2:volt ;
  ns2:hasDimension ns2:electricPotential-Dimension .

ns2:decavolt
  a ns2:PrefixedUnit ;
  rdfs:label "decavolt"@en, "decavolt"@nl ;
  ns2:symbol "daV" ;
  ns2:hasPrefix ns2:deca ;
  ns2:hasUnit ns2:volt ;
  ns2:hasDimension ns2:electricPotential-Dimension .

ns2:hectovolt
  a ns2:PrefixedUnit ;
  rdfs:label "hectovolt"@en, "hectovolt"@nl ;
  ns2:symbol "hV" ;
  ns2:hasPrefix ns2:hecto ;
  ns2:hasUnit ns2:volt ;
  ns2:hasDimension ns2:electricPotential-Dimension .

ns2:kilovolt
  a ns2:PrefixedUnit ;
  rdfs:label "kilovolt"@en, "kilovolt"@nl ;
  ns2:symbol "kV" ;
  ns2:hasPrefix ns2:kilo ;
  ns2:hasUnit ns2:volt ;
  ns2:hasDimension ns2:electricPotential-Dimension .

ns2:megavolt
  a ns2:PrefixedUnit ;
  rdfs:label "megavolt"@en, "megavolt"@nl ;
  ns2:symbol "MV" ;
  ns2:hasPrefix ns2:mega ;
  ns2:hasUnit ns2:volt ;
  ns2:hasDimension ns2:electricPotential-Dimension .

ns2:gigavolt
  a ns2:PrefixedUnit ;
  rdfs:label "gigavolt"@en, "gigavolt"@nl ;
  ns2:symbol "GV" ;
  ns2:hasPrefix ns2:giga ;
  ns2:hasUnit ns2:volt ;
  ns2:hasDimension ns2:electricPotential-Dimension .

ns2:teravolt
  a ns2:PrefixedUnit ;
  rdfs:label "teravolt"@en, "teravolt"@nl ;
  ns2:symbol "TV" ;
  ns2:hasPrefix ns2:tera ;
  ns2:hasUnit ns2:volt ;
  ns2:hasDimension ns2:electricPotential-Dimension .

ns2:petavolt
  a ns2:PrefixedUnit ;
  rdfs:label "petavolt"@en, "petavolt"@nl ;
  ns2:symbol "PV" ;
  ns2:hasPrefix ns2:peta ;
  ns2:hasUnit ns2:volt ;
  ns2:hasDimension ns2:electricPotential-Dimension .

ns2:exavolt
  a ns2:PrefixedUnit ;
  rdfs:label "exavolt"@en, "exavolt"@nl ;
  ns2:symbol "EV" ;
  ns2:hasPrefix ns2:exa ;
  ns2:hasUnit ns2:volt ;
  ns2:hasDimension ns2:electricPotential-Dimension .

ns2:zettavolt
  a ns2:PrefixedUnit ;
  rdfs:label "zettavolt"@en, "zettavolt"@nl ;
  ns2:symbol "ZV" ;
  ns2:hasPrefix ns2:zetta ;
  ns2:hasUnit ns2:volt ;
  ns2:hasDimension ns2:electricPotential-Dimension .

ns2:yottavolt
  a ns2:PrefixedUnit ;
  rdfs:label "yottavolt"@en, "yottavolt"@nl ;
  ns2:symbol "YV" ;
  ns2:hasPrefix ns2:yotta ;
  ns2:hasUnit ns2:volt ;
  ns2:hasDimension ns2:electricPotential-Dimension .

ns2:coulombPerVolt
  a ns2:UnitDivision ;
  rdfs:label "coulomb per volt"@en, "coulomb per volt"@nl ;
  ns2:symbol "C/V" ;
  ns2:alternativeSymbol "C V-1", "C·V-1" ;
  ns2:hasNumerator ns2:coulomb ;
  ns2:hasDenominator ns2:volt ;
  ns2:hasDimension ns2:capacitance-Dimension .

ns2:CapacitanceUnit
  a owl:Class ;
  rdfs:label "capacitance unit"@en ;
  rdfs:subClassOf ns2:Unit ;
  owl:equivalentClass [
    a owl:Class ;
    owl:unionOf (
     _:genid1136
     ns2:PrefixedFarad
   )
  ] .

ns2:abfarad
  a ns2:Unit, ns2:SingularUnit ;
  rdfs:label "abfarad"@en, "abfarad"@nl ;
  rdfs:comment "The abfarad is a unit of capacitance defined as 1.0e9 farad."@en ;
  ns2:symbol "abF" ;
  ns2:hasFactor "1.0e9"^^xsd:float ;
  ns2:hasUnit ns2:farad ;
  ns2:hasDimension ns2:capacitance-Dimension .

ns2:farad
  a ns2:Unit, ns2:SingularUnit ;
  rdfs:label "farad"@en, "farad"@nl ;
  rdfs:comment "The farad is a unit of capacitance defined as ampere times second divided by volt = coulomb divided by volt = coulomb squared divided by joule = coulomb squared divided by newton times metre = second squared times coulomb squared divided by square metre times kilogram = second to the power 4 times ampere squared divided by square metre times kilogram."@en ;
  ns2:longcomment "The farad is a unit of capacitance defined as ampere times second divided by volt = coulomb divided by volt = coulomb squared divided by joule = coulomb squared divided by newton times metre = second squared times coulomb squared divided by square metre times kilogram = second to the power 4 times ampere squared divided by square metre times kilogram. The farad is a derived unit in the International System of Units." ;
  ns2:symbol "F" ;
  ns2:hasUnit ns2:coulombPerVolt ;
  ns2:hasDimension ns2:capacitance-Dimension .

ns2:statfarad
  a ns2:Unit, ns2:SingularUnit ;
  rdfs:label "statfarad"@en, "statfarad"@nl ;
  rdfs:comment "The statfarad is a unit of capacitance defined as 1.112650e-12 farad."@en ;
  ns2:symbol "statF" ;
  ns2:hasFactor "1.112650e-12"^^xsd:float ;
  ns2:hasUnit ns2:farad ;
  ns2:hasDimension ns2:capacitance-Dimension .

ns2:PrefixedFarad
  a owl:Class ;
  rdfs:label "prefixed farad"@en ;
  rdfs:subClassOf ns2:PrefixedUnit ;
  owl:equivalentClass [
    a owl:Class ;
    owl:intersectionOf (
     _:genid1146
     _:genid1148
     _:genid1150
     _:genid1152
   )
  ] .

ns2:yoctofarad
  a ns2:PrefixedUnit ;
  rdfs:label "yoctofarad"@en, "yoctofarad"@nl ;
  rdfs:comment "The yoctofarad is a unit of capacitance defined as 1.0e-24 farad."@en ;
  ns2:symbol "yF" ;
  ns2:hasPrefix ns2:yocto ;
  ns2:hasUnit ns2:farad ;
  ns2:hasDimension ns2:capacitance-Dimension .

ns2:zeptofarad
  a ns2:PrefixedUnit ;
  rdfs:label "zeptofarad"@en, "zeptofarad"@nl ;
  rdfs:comment "The zeptfarad is a unit of capacitance defined as 1.0e-21 farad."@en ;
  ns2:symbol "zF" ;
  ns2:hasPrefix ns2:zepto ;
  ns2:hasUnit ns2:farad ;
  ns2:hasDimension ns2:capacitance-Dimension .

ns2:attofarad
  a ns2:PrefixedUnit ;
  rdfs:label "attofarad"@en, "attofarad"@nl ;
  rdfs:comment "The attofarad is a unit of capacitance defined as 1.0e-18 farad."@en ;
  ns2:symbol "aF" ;
  ns2:hasPrefix ns2:atto ;
  ns2:hasUnit ns2:farad ;
  ns2:hasDimension ns2:capacitance-Dimension .

ns2:femtofarad
  a ns2:PrefixedUnit ;
  rdfs:label "femtofarad"@en, "femtofarad"@nl ;
  rdfs:comment "The femtofarad is a unit of capacitance defined as 1.0e-15 farad."@en ;
  ns2:symbol "fF" ;
  ns2:hasPrefix ns2:femto ;
  ns2:hasUnit ns2:farad ;
  ns2:hasDimension ns2:capacitance-Dimension .

ns2:picofarad
  a ns2:PrefixedUnit ;
  rdfs:label "picofarad"@en, "picofarad"@nl ;
  rdfs:comment "The picofarad is a unit of capacitance defined as 1.0e-12 farad."@en ;
  ns2:symbol "pF" ;
  ns2:hasPrefix ns2:pico ;
  ns2:hasUnit ns2:farad ;
  ns2:hasDimension ns2:capacitance-Dimension .

ns2:nanofarad
  a ns2:PrefixedUnit ;
  rdfs:label "nanofarad"@en, "nanofarad"@nl ;
  rdfs:comment "The nanofarad is a unit of capacitance defined as 1.0e-9 farad."@en ;
  ns2:symbol "nF" ;
  ns2:hasPrefix ns2:nano ;
  ns2:hasUnit ns2:farad ;
  ns2:hasDimension ns2:capacitance-Dimension .

ns2:microfarad
  a ns2:PrefixedUnit ;
  rdfs:label "microfarad"@en, "microfarad"@nl ;
  rdfs:comment "The microfarad is a unit of capacitance defined as 1.0e-6 farad."@en ;
  ns2:symbol "μF" ;
  ns2:hasPrefix ns2:micro ;
  ns2:hasUnit ns2:farad ;
  ns2:hasDimension ns2:capacitance-Dimension .

ns2:millifarad
  a ns2:PrefixedUnit ;
  rdfs:label "millifarad"@en, "millifarad"@nl ;
  rdfs:comment "The millifarad is a unit of capacitance defined as 1.0e-3 farad."@en ;
  ns2:symbol "mF" ;
  ns2:hasPrefix ns2:milli ;
  ns2:hasUnit ns2:farad ;
  ns2:hasDimension ns2:capacitance-Dimension .

ns2:centifarad
  a ns2:PrefixedUnit ;
  rdfs:label "centifarad"@en, "centifarad"@nl ;
  rdfs:comment "The centifarad is a unit of capacitance defined as 1.0e-2 farad."@en ;
  ns2:symbol "cF" ;
  ns2:hasPrefix ns2:centi ;
  ns2:hasUnit ns2:farad ;
  ns2:hasDimension ns2:capacitance-Dimension .

ns2:decifarad
  a ns2:PrefixedUnit ;
  rdfs:label "decifarad"@en, "decifarad"@nl ;
  rdfs:comment "The decifarad is a unit of capacitance defined as 1.0e-1 farad."@en ;
  ns2:symbol "dF" ;
  ns2:hasPrefix ns2:deci ;
  ns2:hasUnit ns2:farad ;
  ns2:hasDimension ns2:capacitance-Dimension .

ns2:decafarad
  a ns2:PrefixedUnit ;
  rdfs:label "decafarad"@en, "decafarad"@nl ;
  rdfs:comment "The decafarad is a unit of capacitance defined as 1.0e1 farad."@en ;
  ns2:symbol "daF" ;
  ns2:hasPrefix ns2:deca ;
  ns2:hasUnit ns2:farad ;
  ns2:hasDimension ns2:capacitance-Dimension .

ns2:hectofarad
  a ns2:PrefixedUnit ;
  rdfs:label "hectofarad"@en, "hectofarad"@nl ;
  rdfs:comment "The hectofarad is a unit of capacitance defined as 1.0e2 farad."@en ;
  ns2:symbol "hF" ;
  ns2:hasPrefix ns2:hecto ;
  ns2:hasUnit ns2:farad ;
  ns2:hasDimension ns2:capacitance-Dimension .

ns2:kilofarad
  a ns2:PrefixedUnit ;
  rdfs:label "kilofarad"@en, "kilofarad"@nl ;
  rdfs:comment "The kilofarad is a unit of capacitance defined as 1.0e3 farad."@en ;
  ns2:symbol "kF" ;
  ns2:hasPrefix ns2:kilo ;
  ns2:hasUnit ns2:farad ;
  ns2:hasDimension ns2:capacitance-Dimension .

ns2:megafarad
  a ns2:PrefixedUnit ;
  rdfs:label "megafarad"@en, "megafarad"@nl ;
  rdfs:comment "The megafarad is a unit of capacitance defined as 1.0e6 farad."@en ;
  ns2:symbol "MF" ;
  ns2:hasPrefix ns2:mega ;
  ns2:hasUnit ns2:farad ;
  ns2:hasDimension ns2:capacitance-Dimension .

ns2:gigafarad
  a ns2:PrefixedUnit ;
  rdfs:label "gigafarad"@en, "gigafarad"@nl ;
  rdfs:comment "The gigafarad is a unit of capacitance defined as 1.0e9 farad."@en ;
  ns2:symbol "GF" ;
  ns2:hasPrefix ns2:giga ;
  ns2:hasUnit ns2:farad ;
  ns2:hasDimension ns2:capacitance-Dimension .

ns2:terafarad
  a ns2:PrefixedUnit ;
  rdfs:label "terafarad"@en, "terafarad"@nl ;
  rdfs:comment "The terafarad is a unit of capacitance defined as 1.0e12 farad."@en ;
  ns2:symbol "TF" ;
  ns2:hasPrefix ns2:tera ;
  ns2:hasUnit ns2:farad ;
  ns2:hasDimension ns2:capacitance-Dimension .

ns2:petafarad
  a ns2:PrefixedUnit ;
  rdfs:label "petafarad"@en, "petafarad"@nl ;
  rdfs:comment "The petafarad is a unit of capacitance defined as 1.0e15 farad."@en ;
  ns2:symbol "PF" ;
  ns2:hasPrefix ns2:peta ;
  ns2:hasUnit ns2:farad ;
  ns2:hasDimension ns2:capacitance-Dimension .

ns2:exafarad
  a ns2:PrefixedUnit ;
  rdfs:label "exafarad"@en, "exafarad"@nl ;
  rdfs:comment "The exafarad is a unit of capacitance defined as 1.0e18 farad."@en ;
  ns2:symbol "EF" ;
  ns2:hasPrefix ns2:exa ;
  ns2:hasUnit ns2:farad ;
  ns2:hasDimension ns2:capacitance-Dimension .

ns2:zettafarad
  a ns2:PrefixedUnit ;
  rdfs:label "zettafarad"@en, "zettafarad"@nl ;
  rdfs:comment "The zettafarad is a unit of capacitance defined as 1.0e21 farad."@en ;
  ns2:symbol "ZF" ;
  ns2:hasPrefix ns2:zetta ;
  ns2:hasUnit ns2:farad ;
  ns2:hasDimension ns2:capacitance-Dimension .

ns2:yottafarad
  a ns2:PrefixedUnit ;
  rdfs:label "yottafarad"@en, "yottafarad"@nl ;
  rdfs:comment "The yottafarad is a unit of capacitance defined as 1.0e24 farad."@en ;
  ns2:symbol "YF" ;
  ns2:hasPrefix ns2:yotta ;
  ns2:hasUnit ns2:farad ;
  ns2:hasDimension ns2:capacitance-Dimension .

ns2:voltPerAmpere
  a ns2:UnitDivision ;
  rdfs:label "volt per ampere"@en, "volt per ampère"@nl ;
  ns2:symbol "V/A" ;
  ns2:alternativeSymbol "V A-1", "V·A-1" ;
  ns2:hasNumerator ns2:volt ;
  ns2:hasDenominator ns2:ampere ;
  ns2:hasDimension ns2:electricalResistance-Dimension .

ns2:ElectricalResistanceUnit
  a owl:Class ;
  rdfs:label "electrical resistance unit"@en ;
  rdfs:subClassOf ns2:Unit ;
  owl:equivalentClass [
    a owl:Class ;
    owl:unionOf (
     _:genid1155
     ns2:PrefixedOhm
   )
  ] .

ns2:abohm
  a ns2:Unit, ns2:SingularUnit ;
  rdfs:label "abohm"@en, "abohm"@nl ;
  rdfs:comment "The abohm is a unit of electrical resistance defined as 1.0e-9 ohm."@en ;
  ns2:symbol "abΩ" ;
  ns2:hasFactor "1.0e-9"^^xsd:float ;
  ns2:hasUnit ns2:ohm ;
  ns2:hasDimension ns2:electricalResistance-Dimension .

ns2:ohm
  a ns2:Unit, ns2:SingularUnit ;
  rdfs:label "ohm"@en, "ohm"@nl ;
  rdfs:comment "The ohm is a unit of electrical resistance defined as volt divided by ampere = square metre times kilogram divided by second to the power 3 times ampere squared."@en ;
  ns2:longcomment "The ohm is a unit of electrical resistance defined as volt divided by ampere = square metre times kilogram divided by second to the power 3 times ampere squared. The ohm is a derived unit in the International System of Units." ;
  ns2:symbol "Ω" ;
  ns2:hasUnit ns2:voltPerAmpere ;
  ns2:hasDimension ns2:electricalResistance-Dimension .

ns2:statohm
  a ns2:Unit, ns2:SingularUnit ;
  rdfs:label "statohm"@en, "statohm"@nl ;
  rdfs:comment "The statohm is a unit of electrical resistance defined as 8.987552e11 ohm."@en ;
  ns2:symbol "statΩ" ;
  ns2:hasFactor "8.987552e11"^^xsd:float ;
  ns2:hasUnit ns2:ohm ;
  ns2:hasDimension ns2:electricalResistance-Dimension .

ns2:PrefixedOhm
  a owl:Class ;
  rdfs:label "prefixed ohm"@en ;
  rdfs:subClassOf ns2:PrefixedUnit ;
  owl:equivalentClass [
    a owl:Class ;
    owl:intersectionOf (
     _:genid1165
     _:genid1167
     _:genid1169
     _:genid1171
   )
  ] .

ns2:yoctoohm
  a ns2:PrefixedUnit ;
  rdfs:label "yoctoohm"@en, "yoctoohm"@nl ;
  ns2:symbol "yΩ" ;
  ns2:hasPrefix ns2:yocto ;
  ns2:hasUnit ns2:ohm ;
  ns2:hasDimension ns2:electricalResistance-Dimension .

ns2:zeptoohm
  a ns2:PrefixedUnit ;
  rdfs:label "zeptoohm"@en, "zeptoohm"@nl ;
  ns2:symbol "zΩ" ;
  ns2:hasPrefix ns2:zepto ;
  ns2:hasUnit ns2:ohm ;
  ns2:hasDimension ns2:electricalResistance-Dimension .

ns2:attoohm
  a ns2:PrefixedUnit ;
  rdfs:label "attoohm"@en, "attoohm"@nl ;
  ns2:symbol "aΩ" ;
  ns2:hasPrefix ns2:atto ;
  ns2:hasUnit ns2:ohm ;
  ns2:hasDimension ns2:electricalResistance-Dimension .

ns2:femtoohm
  a ns2:PrefixedUnit ;
  rdfs:label "femtoohm"@en, "femtoohm"@nl ;
  ns2:symbol "fΩ" ;
  ns2:hasPrefix ns2:femto ;
  ns2:hasUnit ns2:ohm ;
  ns2:hasDimension ns2:electricalResistance-Dimension .

ns2:picoohm
  a ns2:PrefixedUnit ;
  rdfs:label "picoohm"@en, "picoohm"@nl ;
  ns2:symbol "pΩ" ;
  ns2:hasPrefix ns2:pico ;
  ns2:hasUnit ns2:ohm ;
  ns2:hasDimension ns2:electricalResistance-Dimension .

ns2:nanoohm
  a ns2:PrefixedUnit ;
  rdfs:label "nanoohm"@en, "nanoohm"@nl ;
  ns2:symbol "nΩ" ;
  ns2:hasPrefix ns2:nano ;
  ns2:hasUnit ns2:ohm ;
  ns2:hasDimension ns2:electricalResistance-Dimension .

ns2:microohm
  a ns2:PrefixedUnit ;
  rdfs:label "microohm"@en, "microohm"@nl ;
  ns2:symbol "μΩ" ;
  ns2:hasPrefix ns2:micro ;
  ns2:hasUnit ns2:ohm ;
  ns2:hasDimension ns2:electricalResistance-Dimension .

ns2:milliohm
  a ns2:PrefixedUnit ;
  rdfs:label "milliohm"@en, "milliohm"@nl ;
  ns2:symbol "mΩ" ;
  ns2:hasPrefix ns2:milli ;
  ns2:hasUnit ns2:ohm ;
  ns2:hasDimension ns2:electricalResistance-Dimension .

ns2:centiohm
  a ns2:PrefixedUnit ;
  rdfs:label "centiohm"@en, "centiohm"@nl ;
  ns2:symbol "cΩ" ;
  ns2:hasPrefix ns2:centi ;
  ns2:hasUnit ns2:ohm ;
  ns2:hasDimension ns2:electricalResistance-Dimension .

ns2:deciohm
  a ns2:PrefixedUnit ;
  rdfs:label "deciohm"@en, "deciohm"@nl ;
  ns2:symbol "dΩ" ;
  ns2:hasPrefix ns2:deci ;
  ns2:hasUnit ns2:ohm ;
  ns2:hasDimension ns2:electricalResistance-Dimension .

ns2:decaohm
  a ns2:PrefixedUnit ;
  rdfs:label "decaohm"@en, "decaohm"@nl ;
  ns2:symbol "daΩ" ;
  ns2:hasPrefix ns2:deca ;
  ns2:hasUnit ns2:ohm ;
  ns2:hasDimension ns2:electricalResistance-Dimension .

ns2:hectoohm
  a ns2:PrefixedUnit ;
  rdfs:label "hectoohm"@en, "hectoohm"@nl ;
  ns2:symbol "hΩ" ;
  ns2:hasPrefix ns2:hecto ;
  ns2:hasUnit ns2:ohm ;
  ns2:hasDimension ns2:electricalResistance-Dimension .

ns2:kilohm
  a ns2:PrefixedUnit ;
  rdfs:label "kilohm"@en, "kilohm"@nl ;
  ns2:alternativeLabel "kiloohm"@en ;
  ns2:symbol "kΩ" ;
  ns2:hasPrefix ns2:kilo ;
  ns2:hasUnit ns2:ohm ;
  ns2:hasDimension ns2:electricalResistance-Dimension .

ns2:megohm
  a ns2:PrefixedUnit ;
  rdfs:label "megohm"@en, "megohm"@nl ;
  ns2:alternativeLabel "megaohm"@en ;
  ns2:symbol "MΩ" ;
  ns2:hasPrefix ns2:mega ;
  ns2:hasUnit ns2:ohm ;
  ns2:hasDimension ns2:electricalResistance-Dimension .

ns2:gigaohm
  a ns2:PrefixedUnit ;
  rdfs:label "gigaohm"@en, "gigaohm"@nl ;
  ns2:symbol "GΩ" ;
  ns2:hasPrefix ns2:giga ;
  ns2:hasUnit ns2:ohm ;
  ns2:hasDimension ns2:electricalResistance-Dimension .

ns2:teraohm
  a ns2:PrefixedUnit ;
  rdfs:label "teraohm"@en, "teraohm"@nl ;
  ns2:symbol "TΩ" ;
  ns2:hasPrefix ns2:tera ;
  ns2:hasUnit ns2:ohm ;
  ns2:hasDimension ns2:electricalResistance-Dimension .

ns2:petaohm
  a ns2:PrefixedUnit ;
  rdfs:label "petaohm"@en, "petaohm"@nl ;
  ns2:symbol "PΩ" ;
  ns2:hasPrefix ns2:peta ;
  ns2:hasUnit ns2:ohm ;
  ns2:hasDimension ns2:electricalResistance-Dimension .

ns2:exaohm
  a ns2:PrefixedUnit ;
  rdfs:label "exaohm"@en, "exaohm"@nl ;
  ns2:symbol "EΩ" ;
  ns2:hasPrefix ns2:exa ;
  ns2:hasUnit ns2:ohm ;
  ns2:hasDimension ns2:electricalResistance-Dimension .

ns2:zettaohm
  a ns2:PrefixedUnit ;
  rdfs:label "zettaohm"@en, "zettaohm"@nl ;
  ns2:symbol "ZΩ" ;
  ns2:hasPrefix ns2:zetta ;
  ns2:hasUnit ns2:ohm ;
  ns2:hasDimension ns2:electricalResistance-Dimension .

ns2:yottaohm
  a ns2:PrefixedUnit ;
  rdfs:label "yottaohm"@en, "yottaohm"@nl ;
  ns2:symbol "YΩ" ;
  ns2:hasPrefix ns2:yotta ;
  ns2:hasUnit ns2:ohm ;
  ns2:hasDimension ns2:electricalResistance-Dimension .

ns2:amperePerVolt
  a ns2:UnitDivision ;
  rdfs:label "ampere per volt"@en, "ampère per volt"@nl ;
  ns2:symbol "A/V" ;
  ns2:alternativeSymbol "A V-1", "A·V-1" ;
  ns2:hasNumerator ns2:ampere ;
  ns2:hasDenominator ns2:volt ;
  ns2:hasDimension ns2:electricalConductance-Dimension .

ns2:ElectricalConductanceUnit
  a owl:Class ;
  rdfs:label "electrical conductance unit"@en ;
  rdfs:subClassOf ns2:Unit ;
  owl:equivalentClass [
    a owl:Class ;
    owl:unionOf (
     _:genid1174
     ns2:PrefixedSiemens
   )
  ] .

ns2:abmho
  a ns2:Unit, ns2:SingularUnit ;
  rdfs:label "abmho"@en, "abmho"@nl ;
  ns2:alternativeLabel "absiemens"@en, "absiemens"@nl ;
  rdfs:comment "The abmho is a unit of electrical conductance defined as 1.0e9 siemens."@en ;
  ns2:hasFactor "1.0e9"^^xsd:float ;
  ns2:hasUnit ns2:siemens ;
  ns2:hasDimension ns2:electricalConductance-Dimension .

ns2:mho
  a ns2:Unit, ns2:SingularUnit ;
  rdfs:label "mho"@en, "mho"@nl ;
  rdfs:comment "The mho is a unit of electrical conductance defined as 1 siemens."@en ;
  ns2:hasUnit ns2:siemens ;
  ns2:hasDimension ns2:electricalConductance-Dimension ;
  ns2:LaTeXCommand "\\mhoUnit" .

ns2:siemens
  a ns2:Unit, ns2:SingularUnit ;
  rdfs:label "siemens"@en, "siemens"@nl ;
  rdfs:comment "The siemens is a unit of electrical conductance defined as 1 divided by ohm = ampere divided by volt = coulomb squared times second divided by kilogram times square metre = ampere squared times second to the power 3 divided by kilogram times square metre."@en ;
  ns2:longcomment "The siemens is a unit of electrical conductance defined as 1 divided by ohm = ampere divided by volt = coulomb squared times second divided by kilogram times square metre = ampere squared times second to the power 3 divided by kilogram times square metre. The siemens is a derived unit in the International System of Units." ;
  ns2:symbol "S" ;
  ns2:hasUnit ns2:amperePerVolt ;
  ns2:hasDimension ns2:electricalConductance-Dimension .

ns2:statmho
  a ns2:Unit, ns2:SingularUnit ;
  rdfs:label "statmho"@en, "statmho"@nl ;
  ns2:alternativeLabel "statsiemens"@en, "statsiemens"@nl ;
  rdfs:comment "The statmho is a unit of electrical conductance defined as 1.112650e-12 siemens."@en ;
  ns2:hasFactor "1.112650e-12"^^xsd:float ;
  ns2:hasUnit ns2:siemens ;
  ns2:hasDimension ns2:electricalConductance-Dimension .

ns2:PrefixedSiemens
  a owl:Class ;
  rdfs:label "prefixed siemens"@en ;
  rdfs:subClassOf ns2:PrefixedUnit ;
  owl:equivalentClass [
    a owl:Class ;
    owl:intersectionOf (
     _:genid1185
     _:genid1187
     _:genid1189
     _:genid1191
   )
  ] .

ns2:yoctosiemens
  a ns2:PrefixedUnit ;
  rdfs:label "yoctosiemens"@en, "yoctosiemens"@nl ;
  ns2:symbol "yS" ;
  ns2:hasPrefix ns2:yocto ;
  ns2:hasUnit ns2:siemens ;
  ns2:hasDimension ns2:electricalConductance-Dimension .

ns2:zeptosiemens
  a ns2:PrefixedUnit ;
  rdfs:label "zeptosiemens"@en, "zeptosiemens"@nl ;
  ns2:symbol "zS" ;
  ns2:hasPrefix ns2:zepto ;
  ns2:hasUnit ns2:siemens ;
  ns2:hasDimension ns2:electricalConductance-Dimension .

ns2:attosiemens
  a ns2:PrefixedUnit ;
  rdfs:label "attosiemens"@en, "attosiemens"@nl ;
  ns2:symbol "aS" ;
  ns2:hasPrefix ns2:atto ;
  ns2:hasUnit ns2:siemens ;
  ns2:hasDimension ns2:electricalConductance-Dimension .

ns2:femtosiemens
  a ns2:PrefixedUnit ;
  rdfs:label "femtosiemens"@en, "femtosiemens"@nl ;
  ns2:symbol "fS" ;
  ns2:hasPrefix ns2:femto ;
  ns2:hasUnit ns2:siemens ;
  ns2:hasDimension ns2:electricalConductance-Dimension .

ns2:picosiemens
  a ns2:PrefixedUnit ;
  rdfs:label "picosiemens"@en, "picosiemens"@nl ;
  ns2:symbol "pS" ;
  ns2:hasPrefix ns2:pico ;
  ns2:hasUnit ns2:siemens ;
  ns2:hasDimension ns2:electricalConductance-Dimension .

ns2:nanosiemens
  a ns2:PrefixedUnit ;
  rdfs:label "nanosiemens"@en, "nanosiemens"@nl ;
  ns2:symbol "nS" ;
  ns2:hasPrefix ns2:nano ;
  ns2:hasUnit ns2:siemens ;
  ns2:hasDimension ns2:electricalConductance-Dimension .

ns2:microsiemens
  a ns2:PrefixedUnit ;
  rdfs:label "microsiemens"@en, "microsiemens"@nl ;
  ns2:symbol "μS" ;
  ns2:hasPrefix ns2:micro ;
  ns2:hasUnit ns2:siemens ;
  ns2:hasDimension ns2:electricalConductance-Dimension .

ns2:millisiemens
  a ns2:PrefixedUnit ;
  rdfs:label "millisiemens"@en, "millisiemens"@nl ;
  ns2:symbol "mS" ;
  ns2:hasPrefix ns2:milli ;
  ns2:hasUnit ns2:siemens ;
  ns2:hasDimension ns2:electricalConductance-Dimension .

ns2:centisiemens
  a ns2:PrefixedUnit ;
  rdfs:label "centisiemens"@en, "centisiemens"@nl ;
  ns2:symbol "cS" ;
  ns2:hasPrefix ns2:centi ;
  ns2:hasUnit ns2:siemens ;
  ns2:hasDimension ns2:electricalConductance-Dimension .

ns2:decisiemens
  a ns2:PrefixedUnit ;
  rdfs:label "decisiemens"@en, "decisiemens"@nl ;
  ns2:symbol "dS" ;
  ns2:hasPrefix ns2:deci ;
  ns2:hasUnit ns2:siemens ;
  ns2:hasDimension ns2:electricalConductance-Dimension .

ns2:decasiemens
  a ns2:PrefixedUnit ;
  rdfs:label "decasiemens"@en, "decasiemens"@nl ;
  ns2:symbol "daS" ;
  ns2:hasPrefix ns2:deca ;
  ns2:hasUnit ns2:siemens ;
  ns2:hasDimension ns2:electricalConductance-Dimension .

ns2:hectosiemens
  a ns2:PrefixedUnit ;
  rdfs:label "hectosiemens"@en, "hectosiemens"@nl ;
  ns2:symbol "hS" ;
  ns2:hasPrefix ns2:hecto ;
  ns2:hasUnit ns2:siemens ;
  ns2:hasDimension ns2:electricalConductance-Dimension .

ns2:kilosiemens
  a ns2:PrefixedUnit ;
  rdfs:label "kilosiemens"@en, "kilosiemens"@nl ;
  ns2:symbol "kS" ;
  ns2:hasPrefix ns2:kilo ;
  ns2:hasUnit ns2:siemens ;
  ns2:hasDimension ns2:electricalConductance-Dimension .

ns2:megasiemens
  a ns2:PrefixedUnit ;
  rdfs:label "megasiemens"@en, "megasiemens"@nl ;
  ns2:symbol "MS" ;
  ns2:hasPrefix ns2:mega ;
  ns2:hasUnit ns2:siemens ;
  ns2:hasDimension ns2:electricalConductance-Dimension .

ns2:gigasiemens
  a ns2:PrefixedUnit ;
  rdfs:label "gigasiemens"@en, "gigasiemens"@nl ;
  ns2:symbol "GS" ;
  ns2:hasPrefix ns2:giga ;
  ns2:hasUnit ns2:siemens ;
  ns2:hasDimension ns2:electricalConductance-Dimension .

ns2:terasiemens
  a ns2:PrefixedUnit ;
  rdfs:label "terasiemens"@en, "terasiemens"@nl ;
  ns2:symbol "TS" ;
  ns2:hasPrefix ns2:tera ;
  ns2:hasUnit ns2:siemens ;
  ns2:hasDimension ns2:electricalConductance-Dimension .

ns2:petasiemens
  a ns2:PrefixedUnit ;
  rdfs:label "petasiemens"@en, "petasiemens"@nl ;
  ns2:symbol "PS" ;
  ns2:hasPrefix ns2:peta ;
  ns2:hasUnit ns2:siemens ;
  ns2:hasDimension ns2:electricalConductance-Dimension .

ns2:exasiemens
  a ns2:PrefixedUnit ;
  rdfs:label "exasiemens"@en, "exasiemens"@nl ;
  ns2:symbol "ES" ;
  ns2:hasPrefix ns2:exa ;
  ns2:hasUnit ns2:siemens ;
  ns2:hasDimension ns2:electricalConductance-Dimension .

ns2:zettasiemens
  a ns2:PrefixedUnit ;
  rdfs:label "zettasiemens"@en, "zettasiemens"@nl ;
  ns2:symbol "ZS" ;
  ns2:hasPrefix ns2:zetta ;
  ns2:hasUnit ns2:siemens ;
  ns2:hasDimension ns2:electricalConductance-Dimension .

ns2:yottasiemens
  a ns2:PrefixedUnit ;
  rdfs:label "yottasiemens"@en, "yottasiemens"@nl ;
  ns2:symbol "YS" ;
  ns2:hasPrefix ns2:yotta ;
  ns2:hasUnit ns2:siemens ;
  ns2:hasDimension ns2:electricalConductance-Dimension .

ns2:newtonPerCoulomb
  a ns2:UnitDivision ;
  rdfs:label "newton per coulomb"@en, "newton per coulomb"@nl ;
  ns2:symbol "N/C" ;
  ns2:alternativeSymbol "N C-1", "N·C-1" ;
  ns2:hasNumerator ns2:newton ;
  ns2:hasDenominator ns2:coulomb ;
  ns2:hasDimension ns2:electricField-Dimension .

ns2:ElectricFieldUnit
  a owl:Class ;
  rdfs:label "electric field unit"@en ;
  rdfs:subClassOf ns2:Unit ;
  owl:equivalentClass [
    a owl:Class ;
    owl:oneOf (
     ns2:newtonPerCoulomb
     ns2:voltPerMetre
   )
  ] .

ns2:voltPerMetre
  a ns2:UnitDivision ;
  rdfs:label "volt per metre"@en, "volt per meter"@nl ;
  ns2:symbol "V/m" ;
  ns2:alternativeSymbol "V m-1", "V·m-1" ;
  ns2:hasNumerator ns2:volt ;
  ns2:hasDenominator ns2:metre ;
  ns2:hasDimension ns2:electricField-Dimension .

ns2:coulombPerCubicmetre
  a ns2:UnitDivision ;
  rdfs:label "coulomb per cubic metre"@en, "coulomb per kubieke meter"@nl ;
  ns2:symbol "C/m3" ;
  ns2:alternativeSymbol "C m-3", "C·m-3" ;
  ns2:hasNumerator ns2:coulomb ;
  ns2:hasDenominator ns2:cubicMetre ;
  ns2:hasDimension ns2:electricChargeDensity-Dimension .

ns2:ElectricChargeDensityUnit
  a owl:Class ;
  rdfs:label "electric charge density unit"@en ;
  rdfs:subClassOf ns2:Unit ;
  owl:equivalentClass [
    a owl:Class ;
    owl:oneOf ( ns2:coulombPerCubicmetre )
  ] .

ns2:coulombPerSquareMetre
  a ns2:UnitDivision ;
  rdfs:label "coulomb per square metre"@en, "coulomb per vierkante meter"@nl ;
  ns2:symbol "C/m2" ;
  ns2:alternativeSymbol "C m-2", "C·m-2" ;
  ns2:hasNumerator ns2:coulomb ;
  ns2:hasDenominator ns2:squareMetre ;
  ns2:hasDimension ns2:electricFluxDensity-Dimension .

ns2:ElectricFluxDensityUnit
  a owl:Class ;
  rdfs:label "electric flux density unit"@en ;
  rdfs:subClassOf ns2:Unit ;
  owl:equivalentClass [
    a owl:Class ;
    owl:oneOf ( ns2:coulombPerSquareMetre )
  ] .

ns2:voltSecond-Time
  a ns2:UnitMultiplication ;
  rdfs:label "volt second"@en, "volt seconde"@nl ;
  ns2:symbol "V s" ;
  ns2:alternativeSymbol "V·s" ;
  ns2:hasTerm1 ns2:volt ;
  ns2:hasTerm2 ns2:second-Time ;
  ns2:hasDimension ns2:magneticFlux-Dimension .

ns2:MagneticFluxUnit
  a owl:Class ;
  rdfs:label "magnetic flux unit"@en ;
  rdfs:subClassOf ns2:Unit ;
  owl:equivalentClass [
    a owl:Class ;
    owl:unionOf (
     _:genid1207
     ns2:PrefixedWeber
   )
  ] .

ns2:maxwell
  a ns2:Unit, ns2:SingularUnit ;
  rdfs:label "maxwell"@en, "maxwell"@nl ;
  rdfs:comment "The maxwell is a unit of magnetic flux defined as 1.0e-8 weber."@en ;
  ns2:symbol "Mx" ;
  ns2:hasFactor "1.0e-8"^^xsd:float ;
  ns2:hasUnit ns2:weber ;
  ns2:hasDimension ns2:magneticFlux-Dimension .

ns2:statweber
  a ns2:Unit, ns2:SingularUnit ;
  rdfs:label "statweber"@en, "statweber"@nl ;
  rdfs:comment "The statweber is a unit of magnetic flux defined as 2.9979e2 weber."@en ;
  ns2:symbol "statWb" ;
  ns2:hasFactor "2.9979e2"^^xsd:float ;
  ns2:hasUnit ns2:weber ;
  ns2:hasDimension ns2:magneticFlux-Dimension .

ns2:unitPole
  a ns2:Unit, ns2:SingularUnit ;
  rdfs:label "unit pole"@en ;
  rdfs:comment "The unit pole is a unit of magnetic flux defined as 1.256637e-7 weber."@en ;
  ns2:hasFactor "1.256637e-7"^^xsd:float ;
  ns2:hasUnit ns2:weber ;
  ns2:hasDimension ns2:magneticFlux-Dimension .

ns2:weber
  a ns2:Unit, ns2:SingularUnit ;
  rdfs:label "weber"@en, "weber"@nl ;
  rdfs:comment "The weber is a unit of magnetic flux defined as kilogram times square metre divided by second squared times ampere = volt times second = joule divided by ampere."@en ;
  ns2:longcomment "The weber is a unit of magnetic flux defined as kilogram times square metre divided by second squared times ampere = volt times second = joule divided by ampere. The weber is a derived unit in the International System of Units." ;
  ns2:symbol "Wb" ;
  ns2:hasUnit ns2:voltSecond-Time ;
  ns2:hasDimension ns2:magneticFlux-Dimension .

ns2:PrefixedWeber
  a owl:Class ;
  rdfs:label "prefixed weber"@en ;
  rdfs:subClassOf ns2:PrefixedUnit ;
  owl:equivalentClass [
    a owl:Class ;
    owl:intersectionOf (
     _:genid1218
     _:genid1220
     _:genid1222
     _:genid1224
   )
  ] .

ns2:yoctoweber
  a ns2:PrefixedUnit ;
  rdfs:label "yoctoweber"@en, "yoctoweber"@nl ;
  ns2:symbol "yWb" ;
  ns2:hasPrefix ns2:yocto ;
  ns2:hasUnit ns2:weber ;
  ns2:hasDimension ns2:magneticFlux-Dimension .

ns2:zeptoweber
  a ns2:PrefixedUnit ;
  rdfs:label "zeptoweber"@en, "zeptoweber"@nl ;
  ns2:symbol "zWb" ;
  ns2:hasPrefix ns2:zepto ;
  ns2:hasUnit ns2:weber ;
  ns2:hasDimension ns2:magneticFlux-Dimension .

ns2:attoweber
  a ns2:PrefixedUnit ;
  rdfs:label "attoweber"@en, "attoweber"@nl ;
  ns2:symbol "aWb" ;
  ns2:hasPrefix ns2:atto ;
  ns2:hasUnit ns2:weber ;
  ns2:hasDimension ns2:magneticFlux-Dimension .

ns2:femtoweber
  a ns2:PrefixedUnit ;
  rdfs:label "femtoweber"@en, "femtoweber"@nl ;
  ns2:symbol "fWb" ;
  ns2:hasPrefix ns2:femto ;
  ns2:hasUnit ns2:weber ;
  ns2:hasDimension ns2:magneticFlux-Dimension .

ns2:picoweber
  a ns2:PrefixedUnit ;
  rdfs:label "picoweber"@en, "picoweber"@nl ;
  ns2:symbol "pWb" ;
  ns2:hasPrefix ns2:pico ;
  ns2:hasUnit ns2:weber ;
  ns2:hasDimension ns2:magneticFlux-Dimension .

ns2:nanoweber
  a ns2:PrefixedUnit ;
  rdfs:label "nanoweber"@en, "nanoweber"@nl ;
  ns2:symbol "nWb" ;
  ns2:hasPrefix ns2:nano ;
  ns2:hasUnit ns2:weber ;
  ns2:hasDimension ns2:magneticFlux-Dimension .

ns2:microweber
  a ns2:PrefixedUnit ;
  rdfs:label "microweber"@en, "microweber"@nl ;
  ns2:symbol "μWb" ;
  ns2:hasPrefix ns2:micro ;
  ns2:hasUnit ns2:weber ;
  ns2:hasDimension ns2:magneticFlux-Dimension .

ns2:milliweber
  a ns2:PrefixedUnit ;
  rdfs:label "milliweber"@en, "milliweber"@nl ;
  ns2:symbol "mWb" ;
  ns2:hasPrefix ns2:milli ;
  ns2:hasUnit ns2:weber ;
  ns2:hasDimension ns2:magneticFlux-Dimension .

ns2:centiweber
  a ns2:PrefixedUnit ;
  rdfs:label "centiweber"@en, "centiweber"@nl ;
  ns2:symbol "cWb" ;
  ns2:hasPrefix ns2:centi ;
  ns2:hasUnit ns2:weber ;
  ns2:hasDimension ns2:magneticFlux-Dimension .

ns2:deciweber
  a ns2:PrefixedUnit ;
  rdfs:label "deciweber"@en, "deciweber"@nl ;
  ns2:symbol "dWb" ;
  ns2:hasPrefix ns2:deci ;
  ns2:hasUnit ns2:weber ;
  ns2:hasDimension ns2:magneticFlux-Dimension .

ns2:decaweber
  a ns2:PrefixedUnit ;
  rdfs:label "decaweber"@en, "decaweber"@nl ;
  ns2:symbol "daWb" ;
  ns2:hasPrefix ns2:deca ;
  ns2:hasUnit ns2:weber ;
  ns2:hasDimension ns2:magneticFlux-Dimension .

ns2:hectoweber
  a ns2:PrefixedUnit ;
  rdfs:label "hectoweber"@en, "hectoweber"@nl ;
  ns2:symbol "hWb" ;
  ns2:hasPrefix ns2:hecto ;
  ns2:hasUnit ns2:weber ;
  ns2:hasDimension ns2:magneticFlux-Dimension .

ns2:kiloweber
  a ns2:PrefixedUnit ;
  rdfs:label "kiloweber"@en, "kiloweber"@nl ;
  ns2:symbol "kWb" ;
  ns2:hasPrefix ns2:kilo ;
  ns2:hasUnit ns2:weber ;
  ns2:hasDimension ns2:magneticFlux-Dimension .

ns2:megaweber
  a ns2:PrefixedUnit ;
  rdfs:label "megaweber"@en, "megaweber"@nl ;
  ns2:symbol "MWb" ;
  ns2:hasPrefix ns2:mega ;
  ns2:hasUnit ns2:weber ;
  ns2:hasDimension ns2:magneticFlux-Dimension .

ns2:gigaweber
  a ns2:PrefixedUnit ;
  rdfs:label "gigaweber"@en, "gigaweber"@nl ;
  ns2:symbol "GWb" ;
  ns2:hasPrefix ns2:giga ;
  ns2:hasUnit ns2:weber ;
  ns2:hasDimension ns2:magneticFlux-Dimension .

ns2:teraweber
  a ns2:PrefixedUnit ;
  rdfs:label "teraweber"@en, "teraweber"@nl ;
  ns2:symbol "TWb" ;
  ns2:hasPrefix ns2:tera ;
  ns2:hasUnit ns2:weber ;
  ns2:hasDimension ns2:magneticFlux-Dimension .

ns2:petaweber
  a ns2:PrefixedUnit ;
  rdfs:label "petaweber"@en, "petaweber"@nl ;
  ns2:symbol "PWb" ;
  ns2:hasPrefix ns2:peta ;
  ns2:hasUnit ns2:weber ;
  ns2:hasDimension ns2:magneticFlux-Dimension .

ns2:exaweber
  a ns2:PrefixedUnit ;
  rdfs:label "exaweber"@en, "exaweber"@nl ;
  ns2:symbol "EWb" ;
  ns2:hasPrefix ns2:exa ;
  ns2:hasUnit ns2:weber ;
  ns2:hasDimension ns2:magneticFlux-Dimension .

ns2:zettaweber
  a ns2:PrefixedUnit ;
  rdfs:label "zettaweber"@en, "zettaweber"@nl ;
  ns2:symbol "ZWb" ;
  ns2:hasPrefix ns2:zetta ;
  ns2:hasUnit ns2:weber ;
  ns2:hasDimension ns2:magneticFlux-Dimension .

ns2:yottaweber
  a ns2:PrefixedUnit ;
  rdfs:label "yottaweber"@en, "yottaweber"@nl ;
  ns2:symbol "YWb" ;
  ns2:hasPrefix ns2:yotta ;
  ns2:hasUnit ns2:weber ;
  ns2:hasDimension ns2:magneticFlux-Dimension .

ns2:amperePerMetre
  a ns2:UnitDivision ;
  rdfs:label "ampere per metre"@en, "ampère per meter"@nl ;
  rdfs:comment "Ampere per metre is a unit of magnetic field defined as ampere divided by metre."@en ;
  ns2:longcomment "Ampere per metre is a unit of magnetic field defined as ampere divided by metre. Ampere per metre is a derived unit in the International System of Units." ;
  ns2:symbol "A/m" ;
  ns2:alternativeSymbol "A m-1", "A·m-1" ;
  ns2:hasNumerator ns2:ampere ;
  ns2:hasDenominator ns2:metre ;
  ns2:hasDimension ns2:MagneticField-Dimension .

ns2:MagneticFieldUnit
  a owl:Class ;
  rdfs:label "magnetic field unit"@en ;
  rdfs:subClassOf ns2:Unit ;
  owl:equivalentClass [
    a owl:Class ;
    owl:oneOf (
     ns2:oersted
     ns2:amperePerMetre
   )
  ] .

ns2:oersted
  a ns2:Unit, ns2:SingularUnit ;
  rdfs:label "oersted"@en ;
  rdfs:comment "The oersted is a unit of magnetic field defined as 7.957747e1 ampere per metre."@en ;
  ns2:symbol "Oe" ;
  ns2:hasFactor "7.957747e1"^^xsd:float ;
  ns2:hasUnit ns2:amperePerMetre ;
  ns2:hasDimension ns2:MagneticField-Dimension .

ns2:weberPerSquareMetre
  a ns2:UnitDivision ;
  rdfs:label "weber per square metre"@en, "weber per vierkante meter"@nl ;
  ns2:symbol "Wb/m2" ;
  ns2:alternativeSymbol "Wb m-2", "Wb·m-2" ;
  ns2:hasNumerator ns2:weber ;
  ns2:hasDenominator ns2:squareMetre ;
  ns2:hasDimension ns2:magneticFluxDensity-Dimension .

ns2:MagneticFluxDensityUnit
  a owl:Class ;
  rdfs:label "magnetic flux density unit"@en ;
  rdfs:subClassOf ns2:Unit ;
  owl:equivalentClass [
    a owl:Class ;
    owl:unionOf (
     _:genid1232
     ns2:PrefixedTesla
   )
  ] .

ns2:gamma
  a ns2:Unit, ns2:SingularUnit ;
  rdfs:label "gamma"@en, "gamma"@nl ;
  rdfs:comment "The gamma is a unit of magnetic flux density defined as 1.0e-9 tesla."@en ;
  ns2:LaTeXCommand "\\gammaUnit" ;
  ns2:symbol "γ" ;
  ns2:hasFactor "1.0e-9"^^xsd:float ;
  ns2:hasUnit ns2:tesla ;
  ns2:hasDimension ns2:magneticFluxDensity-Dimension .

ns2:gauss
  a ns2:Unit, ns2:SingularUnit ;
  rdfs:label "gauss"@en, "gauss"@nl ;
  ns2:alternativeLabel "abtesla"@en, "abtesla"@nl ;
  rdfs:comment "The gauss is a unit of magnetic flux density defined as 1.0e-4 tesla."@en ;
  ns2:symbol "G" ;
  ns2:alternativeSymbol "Gs" ;
  ns2:hasFactor "1.0e-4"^^xsd:float ;
  ns2:hasUnit ns2:tesla ;
  ns2:hasDimension ns2:magneticFluxDensity-Dimension .

ns2:stattesla
  a ns2:Unit, ns2:SingularUnit ;
  rdfs:label "stattesla"@en, "stattesla"@nl ;
  rdfs:comment "The stattesla is a unit of magnetic flux density defined as 2.9979e6 tesla."@en ;
  ns2:symbol "statT" ;
  ns2:hasFactor "2.9979e6"^^xsd:float ;
  ns2:hasUnit ns2:tesla ;
  ns2:hasDimension ns2:magneticFluxDensity-Dimension .

ns2:tesla
  a ns2:Unit, ns2:SingularUnit ;
  rdfs:label "tesla"@en, "tesla"@nl ;
  rdfs:comment "The tesla is a unit of magnetic flux density defined as volt times second divided by square metre = newton divided by ampere times metre = weber divided by square metre = kilogram divided by coulomb times second = kilogram divided by ampere times second squared."@en ;
  ns2:longcomment "The tesla is a unit of magnetic flux density defined as volt times second divided by square metre = newton divided by ampere times metre = weber divided by square metre = kilogram divided by coulomb times second = kilogram divided by ampere times second squared. The tesla is a derived unit in the International System of Units." ;
  ns2:symbol "T" ;
  ns2:hasUnit ns2:weberPerSquareMetre ;
  ns2:hasDimension ns2:magneticFluxDensity-Dimension .

ns2:milligauss
  a ns2:PrefixedUnit ;
  rdfs:label "milligauss"@en, "milligauss"@nl ;
  rdfs:comment "The milligauss is a unit of magnetic flux density defined as 1.0e-3 gauss."@en ;
  ns2:symbol "mG" ;
  ns2:hasPrefix ns2:milli ;
  ns2:hasUnit ns2:gauss ;
  ns2:hasDimension ns2:magneticFluxDensity-Dimension .

ns2:PrefixedTesla
  a owl:Class ;
  rdfs:label "prefixed tesla"@en ;
  rdfs:subClassOf ns2:PrefixedUnit ;
  owl:equivalentClass [
    a owl:Class ;
    owl:intersectionOf (
     _:genid1244
     _:genid1246
     _:genid1248
     _:genid1250
   )
  ] .

ns2:yoctotesla
  a ns2:PrefixedUnit ;
  rdfs:label "yoctotesla"@en, "yoctotesla"@nl ;
  ns2:symbol "yT" ;
  ns2:hasPrefix ns2:yocto ;
  ns2:hasUnit ns2:tesla ;
  ns2:hasDimension ns2:magneticFluxDensity-Dimension .

ns2:zeptotesla
  a ns2:PrefixedUnit ;
  rdfs:label "zeptotesla"@en, "zeptotesla"@nl ;
  ns2:symbol "zT" ;
  ns2:hasPrefix ns2:zepto ;
  ns2:hasUnit ns2:tesla ;
  ns2:hasDimension ns2:magneticFluxDensity-Dimension .

ns2:attotesla
  a ns2:PrefixedUnit ;
  rdfs:label "attotesla"@en, "attotesla"@nl ;
  ns2:symbol "aT" ;
  ns2:hasPrefix ns2:atto ;
  ns2:hasUnit ns2:tesla ;
  ns2:hasDimension ns2:magneticFluxDensity-Dimension .

ns2:femtotesla
  a ns2:PrefixedUnit ;
  rdfs:label "femtotesla"@en, "femtotesla"@nl ;
  ns2:symbol "fT" ;
  ns2:hasPrefix ns2:femto ;
  ns2:hasUnit ns2:tesla ;
  ns2:hasDimension ns2:magneticFluxDensity-Dimension .

ns2:picotesla
  a ns2:PrefixedUnit ;
  rdfs:label "picotesla"@en, "picotesla"@nl ;
  ns2:symbol "pT" ;
  ns2:hasPrefix ns2:pico ;
  ns2:hasUnit ns2:tesla ;
  ns2:hasDimension ns2:magneticFluxDensity-Dimension .

ns2:nanotesla
  a ns2:PrefixedUnit ;
  rdfs:label "nanotesla"@en, "nanotesla"@nl ;
  ns2:symbol "nT" ;
  ns2:hasPrefix ns2:nano ;
  ns2:hasUnit ns2:tesla ;
  ns2:hasDimension ns2:magneticFluxDensity-Dimension .

ns2:microtesla
  a ns2:PrefixedUnit ;
  rdfs:label "microtesla"@en, "microtesla"@nl ;
  ns2:symbol "μT" ;
  ns2:hasPrefix ns2:micro ;
  ns2:hasUnit ns2:tesla ;
  ns2:hasDimension ns2:magneticFluxDensity-Dimension .

ns2:millitesla
  a ns2:PrefixedUnit ;
  rdfs:label "millitesla"@en, "millitesla"@nl ;
  ns2:symbol "mT" ;
  ns2:hasPrefix ns2:milli ;
  ns2:hasUnit ns2:tesla ;
  ns2:hasDimension ns2:magneticFluxDensity-Dimension .

ns2:centitesla
  a ns2:PrefixedUnit ;
  rdfs:label "centitesla"@en, "centitesla"@nl ;
  ns2:symbol "cT" ;
  ns2:hasPrefix ns2:centi ;
  ns2:hasUnit ns2:tesla ;
  ns2:hasDimension ns2:magneticFluxDensity-Dimension .

ns2:decitesla
  a ns2:PrefixedUnit ;
  rdfs:label "decitesla"@en, "decitesla"@nl ;
  ns2:symbol "dT" ;
  ns2:hasPrefix ns2:deci ;
  ns2:hasUnit ns2:tesla ;
  ns2:hasDimension ns2:magneticFluxDensity-Dimension .

ns2:decatesla
  a ns2:PrefixedUnit ;
  rdfs:label "decatesla"@en, "decatesla"@nl ;
  ns2:symbol "daT" ;
  ns2:hasPrefix ns2:deca ;
  ns2:hasUnit ns2:tesla ;
  ns2:hasDimension ns2:magneticFluxDensity-Dimension .

ns2:hectotesla
  a ns2:PrefixedUnit ;
  rdfs:label "hectotesla"@en, "hectotesla"@nl ;
  ns2:symbol "hT" ;
  ns2:hasPrefix ns2:hecto ;
  ns2:hasUnit ns2:tesla ;
  ns2:hasDimension ns2:magneticFluxDensity-Dimension .

ns2:kilotesla
  a ns2:PrefixedUnit ;
  rdfs:label "kilotesla"@en, "kilotesla"@nl ;
  ns2:symbol "kT" ;
  ns2:hasPrefix ns2:kilo ;
  ns2:hasUnit ns2:tesla ;
  ns2:hasDimension ns2:magneticFluxDensity-Dimension .

ns2:megatesla
  a ns2:PrefixedUnit ;
  rdfs:label "megatesla"@en, "megatesla"@nl ;
  ns2:symbol "MT" ;
  ns2:hasPrefix ns2:mega ;
  ns2:hasUnit ns2:tesla ;
  ns2:hasDimension ns2:magneticFluxDensity-Dimension .

ns2:gigatesla
  a ns2:PrefixedUnit ;
  rdfs:label "gigatesla"@en, "gigatesla"@nl ;
  ns2:symbol "GT" ;
  ns2:hasPrefix ns2:giga ;
  ns2:hasUnit ns2:tesla ;
  ns2:hasDimension ns2:magneticFluxDensity-Dimension .

ns2:teratesla
  a ns2:PrefixedUnit ;
  rdfs:label "teratesla"@en, "teratesla"@nl ;
  ns2:symbol "TT" ;
  ns2:hasPrefix ns2:tera ;
  ns2:hasUnit ns2:tesla ;
  ns2:hasDimension ns2:magneticFluxDensity-Dimension .

ns2:petatesla
  a ns2:PrefixedUnit ;
  rdfs:label "petatesla"@en, "petatesla"@nl ;
  ns2:symbol "PT" ;
  ns2:hasPrefix ns2:peta ;
  ns2:hasUnit ns2:tesla ;
  ns2:hasDimension ns2:magneticFluxDensity-Dimension .

ns2:exatesla
  a ns2:PrefixedUnit ;
  rdfs:label "exatesla"@en, "exatesla"@nl ;
  ns2:symbol "ET" ;
  ns2:hasPrefix ns2:exa ;
  ns2:hasUnit ns2:tesla ;
  ns2:hasDimension ns2:magneticFluxDensity-Dimension .

ns2:zettatesla
  a ns2:PrefixedUnit ;
  rdfs:label "zettatesla"@en, "zettatesla"@nl ;
  ns2:symbol "ZT" ;
  ns2:hasPrefix ns2:zetta ;
  ns2:hasUnit ns2:tesla ;
  ns2:hasDimension ns2:magneticFluxDensity-Dimension .

ns2:yottatesla
  a ns2:PrefixedUnit ;
  rdfs:label "yottatesla"@en, "yottatesla"@nl ;
  ns2:symbol "YT" ;
  ns2:hasPrefix ns2:yotta ;
  ns2:hasUnit ns2:tesla ;
  ns2:hasDimension ns2:magneticFluxDensity-Dimension .

ns2:weberPerAmpere
  a ns2:UnitDivision ;
  rdfs:label "weber per ampere"@en, "weber per ampère"@nl ;
  ns2:symbol "Wb/A" ;
  ns2:alternativeSymbol "Wb A-1", "Wb·A-1" ;
  ns2:hasNumerator ns2:weber ;
  ns2:hasDenominator ns2:ampere ;
  ns2:hasDimension ns2:inductanceOrPermeance-Electromagnetic-Dimension .

ns2:InductanceUnit
  a owl:Class ;
  rdfs:label "inductance unit"@en ;
  rdfs:subClassOf ns2:Unit ;
  owl:equivalentClass [
    a owl:Class ;
    owl:unionOf (
     _:genid1253
     ns2:PrefixedHenry
   )
  ] .

ns2:abhenry
  a ns2:Unit, ns2:SingularUnit ;
  rdfs:label "abhenry"@en, "abhenry"@nl ;
  rdfs:comment "The abhenry is a unit of inductance defined as 1.0e-9 henry."@en ;
  ns2:symbol "abH" ;
  ns2:hasFactor "1.0e-9"^^xsd:float ;
  ns2:hasUnit ns2:henry ;
  ns2:hasDimension ns2:inductanceOrPermeance-Electromagnetic-Dimension .

ns2:henry
  a ns2:Unit, ns2:SingularUnit ;
  rdfs:label "henry"@en, "henry"@nl ;
  rdfs:comment "The henry is a unit of inductance defined as square metre times kilogram divided by second squared times ampere squared = weber divided by ampere = volt second divided by ampere = (joule divided by coulomb) times second divided by (coulomb divided by second) = joule times second squared divided by coulomb squared = square metre times kilogram divided by coulomb squared."@en ;
  ns2:longcomment "The henry is a unit of inductance defined as square metre times kilogram divided by second squared times ampere squared = weber divided by ampere = volt second divided by ampere = (joule divided by coulomb) times second divided by (coulomb divided by second) = joule times second squared divided by coulomb squared = square metre times kilogram divided by coulomb squared. The henry is a derived unit in the International System of Units." ;
  ns2:symbol "H" ;
  ns2:hasUnit ns2:weberPerAmpere ;
  ns2:hasDimension ns2:inductanceOrPermeance-Electromagnetic-Dimension .

ns2:stathenry
  a ns2:Unit, ns2:SingularUnit ;
  rdfs:label "stathenry"@en, "stathenry"@nl ;
  rdfs:comment "The stathenry is a unit of inductance defined as 8.987552e11 henry."@en ;
  ns2:symbol "statH" ;
  ns2:hasFactor "8.987552e11"^^xsd:float ;
  ns2:hasUnit ns2:henry ;
  ns2:hasDimension ns2:inductanceOrPermeance-Electromagnetic-Dimension .

ns2:PrefixedHenry
  a owl:Class ;
  rdfs:label "prefixed henry"@en ;
  rdfs:subClassOf ns2:PrefixedUnit ;
  owl:equivalentClass [
    a owl:Class ;
    owl:intersectionOf (
     _:genid1267
     _:genid1269
     _:genid1271
     _:genid1273
   )
  ] .

ns2:Permeance-ElectromagneticUnit
  a owl:Class ;
  rdfs:label "permeance (electromagnetic) unit"@en ;
  rdfs:subClassOf ns2:Unit ;
  owl:equivalentClass [
    a owl:Class ;
    owl:oneOf ( ns2:weberPerAmpere )
  ] .

ns2:yoctohenry
  a ns2:PrefixedUnit ;
  rdfs:label "yoctohenry"@en, "yoctohenry"@nl ;
  rdfs:comment "The yoctohenry is a unit of inductance defined as 1.0e-24 henry."@en ;
  ns2:symbol "yH" ;
  ns2:hasPrefix ns2:yocto ;
  ns2:hasUnit ns2:henry ;
  ns2:hasDimension ns2:inductanceOrPermeance-Electromagnetic-Dimension .

ns2:zeptohenry
  a ns2:PrefixedUnit ;
  rdfs:label "zeptohenry"@en, "zeptohenry"@nl ;
  rdfs:comment "The zepthenry is a unit of inductance defined as 1.0e-21 henry."@en ;
  ns2:symbol "zH" ;
  ns2:hasPrefix ns2:zepto ;
  ns2:hasUnit ns2:henry ;
  ns2:hasDimension ns2:inductanceOrPermeance-Electromagnetic-Dimension .

ns2:attohenry
  a ns2:PrefixedUnit ;
  rdfs:label "attohenry"@en, "attohenry"@nl ;
  rdfs:comment "The attohenry is a unit of inductance defined as 1.0e-18 henry."@en ;
  ns2:symbol "aH" ;
  ns2:hasPrefix ns2:atto ;
  ns2:hasUnit ns2:henry ;
  ns2:hasDimension ns2:inductanceOrPermeance-Electromagnetic-Dimension .

ns2:femtohenry
  a ns2:PrefixedUnit ;
  rdfs:label "femtohenry"@en, "femtohenry"@nl ;
  rdfs:comment "The femtohenry is a unit of inductance defined as 1.0e-15 henry."@en ;
  ns2:symbol "fH" ;
  ns2:hasPrefix ns2:femto ;
  ns2:hasUnit ns2:henry ;
  ns2:hasDimension ns2:inductanceOrPermeance-Electromagnetic-Dimension .

ns2:picohenry
  a ns2:PrefixedUnit ;
  rdfs:label "picohenry"@en, "picohenry"@nl ;
  rdfs:comment "The picohenry is a unit of inductance defined as 1.0e-12 henry."@en ;
  ns2:symbol "pH" ;
  ns2:hasPrefix ns2:pico ;
  ns2:hasUnit ns2:henry ;
  ns2:hasDimension ns2:inductanceOrPermeance-Electromagnetic-Dimension .

ns2:nanohenry
  a ns2:PrefixedUnit ;
  rdfs:label "nanohenry"@en, "nanohenry"@nl ;
  rdfs:comment "The nanohenry is a unit of inductance defined as 1.0e-9 henry."@en ;
  ns2:symbol "nH" ;
  ns2:hasPrefix ns2:nano ;
  ns2:hasUnit ns2:henry ;
  ns2:hasDimension ns2:inductanceOrPermeance-Electromagnetic-Dimension .

ns2:microhenry
  a ns2:PrefixedUnit ;
  rdfs:label "microhenry"@en, "microhenry"@nl ;
  rdfs:comment "The microhenry is a unit of inductance defined as 1.0e-6 henry."@en ;
  ns2:symbol "μH" ;
  ns2:hasPrefix ns2:micro ;
  ns2:hasUnit ns2:henry ;
  ns2:hasDimension ns2:inductanceOrPermeance-Electromagnetic-Dimension .

ns2:millihenry
  a ns2:PrefixedUnit ;
  rdfs:label "millihenry"@en, "millihenry"@nl ;
  rdfs:comment "The millihenry is a unit of inductance defined as 1.0e-3 henry."@en ;
  ns2:symbol "mH" ;
  ns2:hasPrefix ns2:milli ;
  ns2:hasUnit ns2:henry ;
  ns2:hasDimension ns2:inductanceOrPermeance-Electromagnetic-Dimension .

ns2:centihenry
  a ns2:PrefixedUnit ;
  rdfs:label "centihenry"@en, "centihenry"@nl ;
  rdfs:comment "The centihenry is a unit of inductance defined as 1.0e-2 henry."@en ;
  ns2:symbol "cH" ;
  ns2:hasPrefix ns2:centi ;
  ns2:hasUnit ns2:henry ;
  ns2:hasDimension ns2:inductanceOrPermeance-Electromagnetic-Dimension .

ns2:decihenry
  a ns2:PrefixedUnit ;
  rdfs:label "decihenry"@en, "decihenry"@nl ;
  rdfs:comment "The decihenry is a unit of inductance defined as 1.0e-1 henry."@en ;
  ns2:symbol "dH" ;
  ns2:hasPrefix ns2:deci ;
  ns2:hasUnit ns2:henry ;
  ns2:hasDimension ns2:inductanceOrPermeance-Electromagnetic-Dimension .

ns2:decahenry
  a ns2:PrefixedUnit ;
  rdfs:label "decahenry"@en, "decahenry"@nl ;
  rdfs:comment "The decahenry is a unit of inductance defined as 1.0e1 henry."@en ;
  ns2:symbol "daH" ;
  ns2:hasPrefix ns2:deca ;
  ns2:hasUnit ns2:henry ;
  ns2:hasDimension ns2:inductanceOrPermeance-Electromagnetic-Dimension .

ns2:hectohenry
  a ns2:PrefixedUnit ;
  rdfs:label "hectohenry"@en, "hectohenry"@nl ;
  rdfs:comment "The hectohenry is a unit of inductance defined as 1.0e2 henry."@en ;
  ns2:symbol "hH" ;
  ns2:hasPrefix ns2:hecto ;
  ns2:hasUnit ns2:henry ;
  ns2:hasDimension ns2:inductanceOrPermeance-Electromagnetic-Dimension .

ns2:kilohenry
  a ns2:PrefixedUnit ;
  rdfs:label "kilohenry"@en, "kilohenry"@nl ;
  rdfs:comment "The kilohenry is a unit of inductance defined as 1.0e3 henry."@en ;
  ns2:symbol "kH" ;
  ns2:hasPrefix ns2:kilo ;
  ns2:hasUnit ns2:henry ;
  ns2:hasDimension ns2:inductanceOrPermeance-Electromagnetic-Dimension .

ns2:megahenry
  a ns2:PrefixedUnit ;
  rdfs:label "megahenry"@en, "megahenry"@nl ;
  rdfs:comment "The megahenry is a unit of inductance defined as 1.0e6 henry."@en ;
  ns2:symbol "MH" ;
  ns2:hasPrefix ns2:mega ;
  ns2:hasUnit ns2:henry ;
  ns2:hasDimension ns2:inductanceOrPermeance-Electromagnetic-Dimension .

ns2:gigahenry
  a ns2:PrefixedUnit ;
  rdfs:label "gigahenry"@en, "gigahenry"@nl ;
  rdfs:comment "The gigahenry is a unit of inductance defined as 1.0e9 henry."@en ;
  ns2:symbol "GH" ;
  ns2:hasPrefix ns2:giga ;
  ns2:hasUnit ns2:henry ;
  ns2:hasDimension ns2:inductanceOrPermeance-Electromagnetic-Dimension .

ns2:terahenry
  a ns2:PrefixedUnit ;
  rdfs:label "terahenry"@en, "terahenry"@nl ;
  rdfs:comment "The terahenry is a unit of inductance defined as 1.0e12 henry."@en ;
  ns2:symbol "TH" ;
  ns2:hasPrefix ns2:tera ;
  ns2:hasUnit ns2:henry ;
  ns2:hasDimension ns2:inductanceOrPermeance-Electromagnetic-Dimension .

ns2:petahenry
  a ns2:PrefixedUnit ;
  rdfs:label "petahenry"@en, "petahenry"@nl ;
  rdfs:comment "The petahenry is a unit of inductance defined as 1.0e15 henry."@en ;
  ns2:symbol "PH" ;
  ns2:hasPrefix ns2:peta ;
  ns2:hasUnit ns2:henry ;
  ns2:hasDimension ns2:inductanceOrPermeance-Electromagnetic-Dimension .

ns2:exahenry
  a ns2:PrefixedUnit ;
  rdfs:label "exahenry"@en, "exahenry"@nl ;
  rdfs:comment "The exahenry is a unit of inductance defined as 1.0e18 henry."@en ;
  ns2:symbol "EH" ;
  ns2:hasPrefix ns2:exa ;
  ns2:hasUnit ns2:henry ;
  ns2:hasDimension ns2:inductanceOrPermeance-Electromagnetic-Dimension .

ns2:zettahenry
  a ns2:PrefixedUnit ;
  rdfs:label "zettahenry"@en, "zettahenry"@nl ;
  rdfs:comment "The zettahenry is a unit of inductance defined as 1.0e21 henry."@en ;
  ns2:symbol "ZH" ;
  ns2:hasPrefix ns2:zetta ;
  ns2:hasUnit ns2:henry ;
  ns2:hasDimension ns2:inductanceOrPermeance-Electromagnetic-Dimension .

ns2:yottahenry
  a ns2:PrefixedUnit ;
  rdfs:label "yottahenry"@en, "yottahenry"@nl ;
  rdfs:comment "The yottahenry is a unit of inductance defined as 1.0e24 henry."@en ;
  ns2:symbol "YH" ;
  ns2:hasPrefix ns2:yotta ;
  ns2:hasUnit ns2:henry ;
  ns2:hasDimension ns2:inductanceOrPermeance-Electromagnetic-Dimension .

ns2:henryPerMetre
  a ns2:UnitDivision ;
  rdfs:label "henry per metre"@en, "henry per meter"@nl ;
  ns2:symbol "H/m" ;
  ns2:alternativeSymbol "H m-1", "H·m-1" ;
  ns2:hasNumerator ns2:henry ;
  ns2:hasDenominator ns2:metre ;
  ns2:hasDimension ns2:permeabilityOfFreeSpace-Dimension .

ns2:PermeabilityOfFreeSpaceUnit
  a owl:Class ;
  rdfs:label "permeability of free space unit"@en ;
  rdfs:subClassOf ns2:Unit ;
  owl:equivalentClass [
    a owl:Class ;
    owl:oneOf ( ns2:henryPerMetre )
  ] .

ns2:faradPerMetre
  a ns2:UnitDivision ;
  rdfs:label "farad per metre"@en, "farad per meter"@nl ;
  ns2:symbol "F/m" ;
  ns2:alternativeSymbol "F m-1", "F·m-1" ;
  ns2:hasNumerator ns2:farad ;
  ns2:hasDenominator ns2:metre ;
  ns2:hasDimension ns2:permittivity-Dimension .

ns2:PermittivityUnit
  a owl:Class ;
  rdfs:label "permittivity unit"@en ;
  rdfs:subClassOf ns2:Unit ;
  owl:equivalentClass [
    a owl:Class ;
    owl:oneOf ( ns2:faradPerMetre )
  ] .

ns2:coulombMetre
  a ns2:UnitMultiplication ;
  rdfs:label "coulomb metre"@en, "coulomb meter"@nl ;
  ns2:symbol "C m" ;
  ns2:alternativeSymbol "C·m" ;
  ns2:hasTerm1 ns2:coulomb ;
  ns2:hasTerm2 ns2:metre ;
  ns2:hasDimension ns2:electricDipoleMoment-Dimension .

ns2:ElectricDipoleMomentUnit
  a owl:Class ;
  rdfs:label "electric dipole moment unit"@en ;
  rdfs:subClassOf ns2:Unit ;
  owl:equivalentClass [
    a owl:Class ;
    owl:oneOf (
     ns2:debye
     ns2:coulombMetre
   )
  ] .

ns2:debye
  a ns2:Unit, ns2:SingularUnit ;
  rdfs:label "debye"@en, "debye"@nl ;
  ns2:symbol "D" ;
  rdfs:comment "The debye is a unit of electric dipole moment defined as 3.33564e-30 coulomb metre."@en ;
  ns2:hasFactor "3.33564e-30"^^xsd:float ;
  ns2:hasUnit ns2:coulombMetre ;
  ns2:hasDimension ns2:electricDipoleMoment-Dimension .

ns2:reciprocalHenry
  a ns2:UnitExponentiation ;
  rdfs:label "reciprocal henry"@en, "omgekeerde henry"@nl ;
  ns2:symbol "H-1" ;
  ns2:hasBase ns2:henry ;
  ns2:hasExponent -1 ;
  ns2:hasDimension ns2:reluctance-Dimension .

ns2:ReluctanceUnit
  a owl:Class ;
  rdfs:label "reluctance unit"@en ;
  rdfs:subClassOf ns2:Unit ;
  owl:equivalentClass [
    a owl:Class ;
    owl:oneOf ( ns2:reciprocalHenry )
  ] .

ns2:ohmMetre
  a ns2:UnitMultiplication ;
  rdfs:label "ohm metre"@en, "ohm meter"@nl ;
  ns2:symbol "Ω m" ;
  ns2:alternativeSymbol "Ω·m" ;
  ns2:hasTerm1 ns2:ohm ;
  ns2:hasTerm2 ns2:metre ;
  ns2:hasDimension ns2:electricalResistivity-Dimension .

ns2:ElectricalResistivityUnit
  a owl:Class ;
  rdfs:label "electrical resistivity unit"@en ;
  rdfs:subClassOf ns2:Unit ;
  owl:equivalentClass [
    a owl:Class ;
    owl:oneOf ( ns2:ohmMetre )
  ] .

ns2:siemensPerMetre
  a ns2:UnitDivision ;
  rdfs:label "siemens per metre"@en, "siemens per meter"@nl ;
  ns2:symbol "S/m" ;
  ns2:alternativeSymbol "S m-1", "S·m-1" ;
  ns2:hasNumerator ns2:siemens ;
  ns2:hasDenominator ns2:metre ;
  ns2:hasDimension ns2:electricalConductivity-Dimension .

ns2:ElectricalConductivityUnit
  a owl:Class ;
  rdfs:label "electrical conductivity unit"@en ;
  rdfs:subClassOf ns2:Unit ;
  owl:equivalentClass [
    a owl:Class ;
    owl:oneOf ( ns2:siemensPerMetre )
  ] .

ns2:electricCurrent-Dimension
  a ns2:Dimension ;
  rdfs:label "electric current dimension"@en ;
  ns2:symbol "I" ;
  ns2:hasSILengthDimensionExponent 0 ;
  ns2:hasSIMassDimensionExponent 0 ;
  ns2:hasSITimeDimensionExponent 0 ;
  ns2:hasSIElectricCurrentDimensionExponent 1 ;
  ns2:hasSIThermodynamicTemperatureDimensionExponent 0 ;
  ns2:hasSIAmountOfSubstanceDimensionExponent 0 ;
  ns2:hasSILuminousIntensityDimensionExponent 0 .

ns2:currentDensity-Dimension
  a ns2:Dimension ;
  rdfs:label "current density dimension"@en ;
  ns2:hasSILengthDimensionExponent -2 ;
  ns2:hasSIMassDimensionExponent 0 ;
  ns2:hasSITimeDimensionExponent 0 ;
  ns2:hasSIElectricCurrentDimensionExponent 1 ;
  ns2:hasSIThermodynamicTemperatureDimensionExponent 0 ;
  ns2:hasSIAmountOfSubstanceDimensionExponent 0 ;
  ns2:hasSILuminousIntensityDimensionExponent 0 .

ns2:electricCharge-Dimension
  a ns2:Dimension ;
  rdfs:label "electric charge dimension"@en ;
  ns2:hasSILengthDimensionExponent 0 ;
  ns2:hasSIMassDimensionExponent 0 ;
  ns2:hasSITimeDimensionExponent 1 ;
  ns2:hasSIElectricCurrentDimensionExponent 1 ;
  ns2:hasSIThermodynamicTemperatureDimensionExponent 0 ;
  ns2:hasSIAmountOfSubstanceDimensionExponent 0 ;
  ns2:hasSILuminousIntensityDimensionExponent 0 .

ns2:electricPotential-Dimension
  a ns2:Dimension ;
  rdfs:label "electric potential dimension"@en ;
  ns2:hasSILengthDimensionExponent 2 ;
  ns2:hasSIMassDimensionExponent 1 ;
  ns2:hasSITimeDimensionExponent -3 ;
  ns2:hasSIElectricCurrentDimensionExponent -1 ;
  ns2:hasSIThermodynamicTemperatureDimensionExponent 0 ;
  ns2:hasSIAmountOfSubstanceDimensionExponent 0 ;
  ns2:hasSILuminousIntensityDimensionExponent 0 .

ns2:capacitance-Dimension
  a ns2:Dimension ;
  rdfs:label "capacitance dimension"@en ;
  ns2:hasSILengthDimensionExponent -2 ;
  ns2:hasSIMassDimensionExponent -1 ;
  ns2:hasSITimeDimensionExponent 4 ;
  ns2:hasSIElectricCurrentDimensionExponent 2 ;
  ns2:hasSIThermodynamicTemperatureDimensionExponent 0 ;
  ns2:hasSIAmountOfSubstanceDimensionExponent 0 ;
  ns2:hasSILuminousIntensityDimensionExponent 0 .

ns2:electricalResistance-Dimension
  a ns2:Dimension ;
  rdfs:label "electrical resistance dimension"@en ;
  ns2:hasSILengthDimensionExponent 2 ;
  ns2:hasSIMassDimensionExponent 1 ;
  ns2:hasSITimeDimensionExponent -3 ;
  ns2:hasSIElectricCurrentDimensionExponent -2 ;
  ns2:hasSIThermodynamicTemperatureDimensionExponent 0 ;
  ns2:hasSIAmountOfSubstanceDimensionExponent 0 ;
  ns2:hasSILuminousIntensityDimensionExponent 0 .

ns2:electricalConductance-Dimension
  a ns2:Dimension ;
  rdfs:label "electrical conductance dimension"@en ;
  ns2:hasSILengthDimensionExponent -2 ;
  ns2:hasSIMassDimensionExponent -1 ;
  ns2:hasSITimeDimensionExponent 3 ;
  ns2:hasSIElectricCurrentDimensionExponent 2 ;
  ns2:hasSIThermodynamicTemperatureDimensionExponent 0 ;
  ns2:hasSIAmountOfSubstanceDimensionExponent 0 ;
  ns2:hasSILuminousIntensityDimensionExponent 0 .

ns2:electricField-Dimension
  a ns2:Dimension ;
  rdfs:label "electric field dimension"@en ;
  ns2:hasSILengthDimensionExponent 1 ;
  ns2:hasSIMassDimensionExponent 1 ;
  ns2:hasSITimeDimensionExponent -3 ;
  ns2:hasSIElectricCurrentDimensionExponent -1 ;
  ns2:hasSIThermodynamicTemperatureDimensionExponent 0 ;
  ns2:hasSIAmountOfSubstanceDimensionExponent 0 ;
  ns2:hasSILuminousIntensityDimensionExponent 0 .

ns2:electricChargeDensity-Dimension
  a ns2:Dimension ;
  rdfs:label "electric charge density dimension"@en ;
  ns2:hasSILengthDimensionExponent -3 ;
  ns2:hasSIMassDimensionExponent 0 ;
  ns2:hasSITimeDimensionExponent 1 ;
  ns2:hasSIElectricCurrentDimensionExponent 1 ;
  ns2:hasSIThermodynamicTemperatureDimensionExponent 0 ;
  ns2:hasSIAmountOfSubstanceDimensionExponent 0 ;
  ns2:hasSILuminousIntensityDimensionExponent 0 .

ns2:electricFluxDensity-Dimension
  a ns2:Dimension ;
  rdfs:label "electric flux density dimension"@en ;
  ns2:hasSILengthDimensionExponent -2 ;
  ns2:hasSIMassDimensionExponent 0 ;
  ns2:hasSITimeDimensionExponent 1 ;
  ns2:hasSIElectricCurrentDimensionExponent 1 ;
  ns2:hasSIThermodynamicTemperatureDimensionExponent 0 ;
  ns2:hasSIAmountOfSubstanceDimensionExponent 0 ;
  ns2:hasSILuminousIntensityDimensionExponent 0 .

ns2:magneticFlux-Dimension
  a ns2:Dimension ;
  rdfs:label "magnetic flux dimension"@en ;
  ns2:hasSILengthDimensionExponent 2 ;
  ns2:hasSIMassDimensionExponent 1 ;
  ns2:hasSITimeDimensionExponent -2 ;
  ns2:hasSIElectricCurrentDimensionExponent -1 ;
  ns2:hasSIThermodynamicTemperatureDimensionExponent 0 ;
  ns2:hasSIAmountOfSubstanceDimensionExponent 0 ;
  ns2:hasSILuminousIntensityDimensionExponent 0 .

ns2:MagneticField-Dimension
  a ns2:Dimension ;
  rdfs:label "magnetic field dimension"@en ;
  ns2:hasSILengthDimensionExponent -1 ;
  ns2:hasSIMassDimensionExponent 0 ;
  ns2:hasSITimeDimensionExponent 0 ;
  ns2:hasSIElectricCurrentDimensionExponent 1 ;
  ns2:hasSIThermodynamicTemperatureDimensionExponent 0 ;
  ns2:hasSIAmountOfSubstanceDimensionExponent 0 ;
  ns2:hasSILuminousIntensityDimensionExponent 0 .

ns2:magneticFluxDensity-Dimension
  a ns2:Dimension ;
  rdfs:label "magnetic flux density dimension"@en ;
  ns2:hasSILengthDimensionExponent 0 ;
  ns2:hasSIMassDimensionExponent 1 ;
  ns2:hasSITimeDimensionExponent -2 ;
  ns2:hasSIElectricCurrentDimensionExponent -1 ;
  ns2:hasSIThermodynamicTemperatureDimensionExponent 0 ;
  ns2:hasSIAmountOfSubstanceDimensionExponent 0 ;
  ns2:hasSILuminousIntensityDimensionExponent 0 .

ns2:inductanceOrPermeance-Electromagnetic-Dimension
  a ns2:Dimension ;
  rdfs:label "inductance or permeance (electromagnetic) dimension"@en ;
  ns2:hasSILengthDimensionExponent 2 ;
  ns2:hasSIMassDimensionExponent 1 ;
  ns2:hasSITimeDimensionExponent -2 ;
  ns2:hasSIElectricCurrentDimensionExponent -2 ;
  ns2:hasSIThermodynamicTemperatureDimensionExponent 0 ;
  ns2:hasSIAmountOfSubstanceDimensionExponent 0 ;
  ns2:hasSILuminousIntensityDimensionExponent 0 .

ns2:permeabilityOfFreeSpace-Dimension
  a ns2:Dimension ;
  rdfs:label "permeability of free space dimension"@en ;
  ns2:hasSILengthDimensionExponent 1 ;
  ns2:hasSIMassDimensionExponent 1 ;
  ns2:hasSITimeDimensionExponent -2 ;
  ns2:hasSIElectricCurrentDimensionExponent -2 ;
  ns2:hasSIThermodynamicTemperatureDimensionExponent 0 ;
  ns2:hasSIAmountOfSubstanceDimensionExponent 0 ;
  ns2:hasSILuminousIntensityDimensionExponent 0 .

ns2:permittivity-Dimension
  a ns2:Dimension ;
  rdfs:label "permittivity dimension"@en ;
  ns2:hasSILengthDimensionExponent -3 ;
  ns2:hasSIMassDimensionExponent -1 ;
  ns2:hasSITimeDimensionExponent 4 ;
  ns2:hasSIElectricCurrentDimensionExponent 2 ;
  ns2:hasSIThermodynamicTemperatureDimensionExponent 0 ;
  ns2:hasSIAmountOfSubstanceDimensionExponent 0 ;
  ns2:hasSILuminousIntensityDimensionExponent 0 .

ns2:electricDipoleMoment-Dimension
  a ns2:Dimension ;
  rdfs:label "electric dipole moment dimension"@en ;
  ns2:hasSILengthDimensionExponent 1 ;
  ns2:hasSIMassDimensionExponent 0 ;
  ns2:hasSITimeDimensionExponent 1 ;
  ns2:hasSIElectricCurrentDimensionExponent 1 ;
  ns2:hasSIThermodynamicTemperatureDimensionExponent 0 ;
  ns2:hasSIAmountOfSubstanceDimensionExponent 0 ;
  ns2:hasSILuminousIntensityDimensionExponent 0 .

ns2:reluctance-Dimension
  a ns2:Dimension ;
  rdfs:label "reluctance dimension"@en ;
  ns2:hasSILengthDimensionExponent -2 ;
  ns2:hasSIMassDimensionExponent -1 ;
  ns2:hasSITimeDimensionExponent 2 ;
  ns2:hasSIElectricCurrentDimensionExponent 2 ;
  ns2:hasSIThermodynamicTemperatureDimensionExponent 0 ;
  ns2:hasSIAmountOfSubstanceDimensionExponent 0 ;
  ns2:hasSILuminousIntensityDimensionExponent 0 .

ns2:electricalResistivity-Dimension
  a ns2:Dimension ;
  rdfs:label "electrical resistivity dimension"@en ;
  ns2:hasSILengthDimensionExponent 3 ;
  ns2:hasSIMassDimensionExponent 1 ;
  ns2:hasSITimeDimensionExponent -3 ;
  ns2:hasSIElectricCurrentDimensionExponent -2 ;
  ns2:hasSIThermodynamicTemperatureDimensionExponent 0 ;
  ns2:hasSIAmountOfSubstanceDimensionExponent 0 ;
  ns2:hasSILuminousIntensityDimensionExponent 0 .

ns2:electricalConductivity-Dimension
  a ns2:Dimension ;
  rdfs:label "electrical conductivity dimension"@en ;
  ns2:hasSILengthDimensionExponent -3 ;
  ns2:hasSIMassDimensionExponent -1 ;
  ns2:hasSITimeDimensionExponent 3 ;
  ns2:hasSIElectricCurrentDimensionExponent 2 ;
  ns2:hasSIThermodynamicTemperatureDimensionExponent 0 ;
  ns2:hasSIAmountOfSubstanceDimensionExponent 0 ;
  ns2:hasSILuminousIntensityDimensionExponent 0 .

ns2:fluidMechanics
  a ns2:ApplicationArea ;
  rdfs:label "fluid mechanics"@en, "vloeistofmechanica"@nl ;
  ns2:usesQuantity ns2:ContactAngle, ns2:WettingAngle, ns2:Stress, ns2:CompressiveStress, ns2:NormalStress, ns2:ShearStress, ns2:StressTensor, ns2:ShearRate, ns2:Strain, ns2:LinearStrain, ns2:VolumeStrain, ns2:NormalStrain, ns2:ShearStrain, ns2:StrainTensor, ns2:DynamicModulus, ns2:ShearModulus, ns2:StorageModulus, ns2:ShearStorageModulus, ns2:LossModulus, ns2:ShearLossModulus, ns2:BulkModulus, ns2:ModulusOfElasticity, ns2:ElasticityTensor, ns2:SurfaceTension ;
  ns2:usesUnit ns2:attoradian, ns2:centiradian, ns2:deciradian, ns2:femtoradian, ns2:microradian, ns2:milliradian, ns2:nanoradian, ns2:picoradian, ns2:newtonPerSquareMetre, ns2:kilogramSecond-TimeToThePower-2ReciprocalMetre, ns2:pascal, ns2:attopascal, ns2:centipascal, ns2:decapascal, ns2:decipascal, ns2:exapascal, ns2:femtopascal, ns2:gigapascal, ns2:hectopascal, ns2:kilopascal, ns2:megapascal, ns2:micropascal, ns2:millipascal, ns2:nanopascal, ns2:petapascal, ns2:picopascal, ns2:terapascal, ns2:bar, ns2:decibar, ns2:microbar, ns2:millibar, ns2:metreOfMercury, ns2:centimetreOfMercury, ns2:millimetreOfMercury, ns2:atmosphere-Standard, ns2:atmosphere-Technical, ns2:barye, ns2:torr .

ns2:ContactAngle
  a owl:Class ;
  rdfs:label "contact angle"@en ;
  rdfs:subClassOf ns2:Angle ;
  ns2:commonlyHasUnit ns2:metrePerMetre, ns2:radian, ns2:attoradian, ns2:centiradian, ns2:deciradian, ns2:femtoradian, ns2:microradian, ns2:milliradian, ns2:nanoradian, ns2:picoradian, ns2:degree, ns2:gon, ns2:mil-Angle, ns2:minute-Angle, ns2:revolution, ns2:second-Angle, ns2:millisecond-Angle, ns2:microsecond-Angle .

ns2:WettingAngle
  a owl:Class ;
  rdfs:label "wetting angle"@en ;
  rdfs:subClassOf ns2:Angle ;
  ns2:commonlyHasUnit ns2:metrePerMetre, ns2:radian, ns2:attoradian, ns2:centiradian, ns2:deciradian, ns2:femtoradian, ns2:microradian, ns2:milliradian, ns2:nanoradian, ns2:picoradian, ns2:degree, ns2:gon, ns2:mil-Angle, ns2:minute-Angle, ns2:revolution, ns2:second-Angle, ns2:millisecond-Angle, ns2:microsecond-Angle .

ns2:CompressiveStress
  a owl:Class ;
  rdfs:label "compressive stress"@en ;
  rdfs:comment "Compressive stress is a stress that, when applied, acts towards the center of a material."@en ;
  rdfs:subClassOf ns2:Stress ;
  ns2:commonlyHasUnit ns2:newtonPerSquareMetre, ns2:kilogramSecond-TimeToThePower-2ReciprocalMetre, ns2:pascal, ns2:attopascal, ns2:centipascal, ns2:decapascal, ns2:decipascal, ns2:exapascal, ns2:femtopascal, ns2:gigapascal, ns2:hectopascal, ns2:kilopascal, ns2:megapascal, ns2:micropascal, ns2:millipascal, ns2:nanopascal, ns2:petapascal, ns2:picopascal, ns2:terapascal, ns2:bar, ns2:decibar, ns2:microbar, ns2:millibar, ns2:metreOfMercury, ns2:centimetreOfMercury, ns2:millimetreOfMercury, ns2:atmosphere-Standard, ns2:atmosphere-Technical, ns2:barye, ns2:torr .

ns2:NormalStress
  a owl:Class ;
  rdfs:label "normal stress"@en, "normaalspanning"@nl ;
  rdfs:subClassOf ns2:Stress ;
  ns2:commonlyHasUnit ns2:newtonPerSquareMetre, ns2:kilogramSecond-TimeToThePower-2ReciprocalMetre, ns2:pascal, ns2:attopascal, ns2:centipascal, ns2:decapascal, ns2:decipascal, ns2:exapascal, ns2:femtopascal, ns2:gigapascal, ns2:hectopascal, ns2:kilopascal, ns2:megapascal, ns2:micropascal, ns2:millipascal, ns2:nanopascal, ns2:petapascal, ns2:picopascal, ns2:terapascal, ns2:bar, ns2:decibar, ns2:microbar, ns2:millibar, ns2:metreOfMercury, ns2:centimetreOfMercury, ns2:millimetreOfMercury, ns2:atmosphere-Standard, ns2:atmosphere-Technical, ns2:barye, ns2:torr .

ns2:ShearStress
  a owl:Class ;
  rdfs:label "shear stress"@en, "schuifspanning"@nl ;
  rdfs:comment "Shear stress is a stress that is applied parallel or tangential to a face of a material."@en ;
  rdfs:subClassOf ns2:Stress ;
  ns2:symbol "τ" ;
  ns2:commonlyHasUnit ns2:newtonPerSquareMetre, ns2:kilogramSecond-TimeToThePower-2ReciprocalMetre, ns2:pascal, ns2:attopascal, ns2:centipascal, ns2:decapascal, ns2:decipascal, ns2:exapascal, ns2:femtopascal, ns2:gigapascal, ns2:hectopascal, ns2:kilopascal, ns2:megapascal, ns2:micropascal, ns2:millipascal, ns2:nanopascal, ns2:petapascal, ns2:picopascal, ns2:terapascal, ns2:bar, ns2:decibar, ns2:microbar, ns2:millibar, ns2:metreOfMercury, ns2:centimetreOfMercury, ns2:millimetreOfMercury, ns2:atmosphere-Standard, ns2:atmosphere-Technical, ns2:barye, ns2:torr .

ns2:StressTensor
  a owl:Class ;
  rdfs:label "stress tensor"@en, "mechanische-spanningstensor"@nl ;
  rdfs:subClassOf ns2:Stress ;
  ns2:symbol "τ_ij" ;
  ns2:commonlyHasUnit ns2:newtonPerSquareMetre, ns2:kilogramSecond-TimeToThePower-2ReciprocalMetre, ns2:pascal, ns2:attopascal, ns2:centipascal, ns2:decapascal, ns2:decipascal, ns2:exapascal, ns2:femtopascal, ns2:gigapascal, ns2:hectopascal, ns2:kilopascal, ns2:megapascal, ns2:micropascal, ns2:millipascal, ns2:nanopascal, ns2:petapascal, ns2:picopascal, ns2:terapascal, ns2:bar, ns2:decibar, ns2:microbar, ns2:millibar, ns2:metreOfMercury, ns2:centimetreOfMercury, ns2:millimetreOfMercury, ns2:atmosphere-Standard, ns2:atmosphere-Technical, ns2:barye, ns2:torr .

ns2:Strain
  a owl:Class ;
  rdfs:label "strain"@en, "vervorming"@nl ;
  rdfs:subClassOf ns2:Quantity, [
    a owl:Restriction ;
    owl:onProperty ns2:hasValue ;
    owl:allValuesFrom [
      a owl:Restriction ;
      owl:onProperty ns2:hasUnit ;
      owl:allValuesFrom ns2:StrainUnit
    ]
  ], [
    a owl:Restriction ;
    owl:onProperty ns2:hasDimension ;
    owl:hasValue ns2:dimensionOne
  ] ;
  ns2:symbol "ε" ;
  ns2:alternativeSymbol "γ" ;
  ns2:commonlyHasUnit ns2:one, ns2:percent .

ns2:StrainUnit
  a owl:Class ;
  rdfs:label "strain unit"@en ;
  rdfs:subClassOf ns2:Unit ;
  owl:equivalentClass [
    a owl:Class ;
    owl:oneOf (
     ns2:one
     ns2:percent
   )
  ] .

ns2:LinearStrain
  a owl:Class ;
  rdfs:label "linear strain"@en, "lineaire vervorming"@nl ;
  rdfs:subClassOf ns2:Strain ;
  ns2:alternativeSymbol "e" ;
  ns2:commonlyHasUnit ns2:one, ns2:percent .

ns2:VolumeStrain
  a owl:Class ;
  rdfs:label "volume strain"@en ;
  ns2:alternativeLabel "bulk strain"@en ;
  rdfs:subClassOf ns2:Strain ;
  ns2:symbol "θ" ;
  ns2:commonlyHasUnit ns2:one, ns2:percent .

ns2:NormalStrain
  a owl:Class ;
  rdfs:label "normal strain"@en, "normaalvervorming"@nl ;
  rdfs:subClassOf ns2:Strain ;
  ns2:commonlyHasUnit ns2:one, ns2:percent .

ns2:ShearStrain
  a owl:Class ;
  rdfs:label "shear strain"@en, "schuifvervorming"@nl ;
  rdfs:comment "Shear strain is a strain that acts parallel to the surface of a material that it acts on."@en ;
  rdfs:subClassOf ns2:Strain ;
  ns2:commonlyHasUnit ns2:one, ns2:percent .

ns2:StrainTensor
  a owl:Class ;
  rdfs:label "strain tensor"@en ;
  ns2:alternativeLabel "vervormingstensor"@nl, "rektensor"@nl ;
  rdfs:subClassOf ns2:Strain ;
  ns2:symbol "ε_ij" ;
  ns2:commonlyHasUnit ns2:one, ns2:percent .

ns2:ShearModulus
  a owl:Class ;
  rdfs:label "shear modulus"@en, "schuifmodulus"@nl ;
  rdfs:comment "Shear modulus is the ratio of shear stress to shear strain."@en ;
  rdfs:subClassOf ns2:DynamicModulus ;
  ns2:symbol "G" ;
  ns2:alternativeSymbol "S", "μ" ;
  ns2:commonlyHasUnit ns2:newtonPerSquareMetre, ns2:kilogramSecond-TimeToThePower-2ReciprocalMetre, ns2:pascal, ns2:attopascal, ns2:centipascal, ns2:decapascal, ns2:decipascal, ns2:exapascal, ns2:femtopascal, ns2:gigapascal, ns2:hectopascal, ns2:kilopascal, ns2:megapascal, ns2:micropascal, ns2:millipascal, ns2:nanopascal, ns2:petapascal, ns2:picopascal, ns2:terapascal, ns2:bar, ns2:decibar, ns2:microbar, ns2:millibar, ns2:metreOfMercury, ns2:centimetreOfMercury, ns2:millimetreOfMercury, ns2:atmosphere-Standard, ns2:atmosphere-Technical, ns2:barye, ns2:torr .

ns2:StorageModulus
  a owl:Class ;
  rdfs:label "storage modulus"@en ;
  rdfs:subClassOf ns2:DynamicModulus ;
  ns2:symbol "E'" ;
  ns2:commonlyHasUnit ns2:newtonPerSquareMetre, ns2:kilogramSecond-TimeToThePower-2ReciprocalMetre, ns2:pascal, ns2:attopascal, ns2:centipascal, ns2:decapascal, ns2:decipascal, ns2:exapascal, ns2:femtopascal, ns2:gigapascal, ns2:hectopascal, ns2:kilopascal, ns2:megapascal, ns2:micropascal, ns2:millipascal, ns2:nanopascal, ns2:petapascal, ns2:picopascal, ns2:terapascal, ns2:bar, ns2:decibar, ns2:microbar, ns2:millibar, ns2:metreOfMercury, ns2:centimetreOfMercury, ns2:millimetreOfMercury, ns2:atmosphere-Standard, ns2:atmosphere-Technical, ns2:barye, ns2:torr .

ns2:ShearStorageModulus
  a owl:Class ;
  rdfs:label "shear storage modulus"@en ;
  rdfs:subClassOf ns2:StorageModulus ;
  ns2:symbol "G'" ;
  ns2:commonlyHasUnit ns2:newtonPerSquareMetre, ns2:kilogramSecond-TimeToThePower-2ReciprocalMetre, ns2:pascal, ns2:attopascal, ns2:centipascal, ns2:decapascal, ns2:decipascal, ns2:exapascal, ns2:femtopascal, ns2:gigapascal, ns2:hectopascal, ns2:kilopascal, ns2:megapascal, ns2:micropascal, ns2:millipascal, ns2:nanopascal, ns2:petapascal, ns2:picopascal, ns2:terapascal, ns2:bar, ns2:decibar, ns2:microbar, ns2:millibar, ns2:metreOfMercury, ns2:centimetreOfMercury, ns2:millimetreOfMercury, ns2:atmosphere-Standard, ns2:atmosphere-Technical, ns2:barye, ns2:torr .

ns2:LossModulus
  a owl:Class ;
  rdfs:label "loss modulus"@en ;
  rdfs:subClassOf ns2:DynamicModulus ;
  ns2:symbol "E''" ;
  ns2:commonlyHasUnit ns2:newtonPerSquareMetre, ns2:kilogramSecond-TimeToThePower-2ReciprocalMetre, ns2:pascal, ns2:attopascal, ns2:centipascal, ns2:decapascal, ns2:decipascal, ns2:exapascal, ns2:femtopascal, ns2:gigapascal, ns2:hectopascal, ns2:kilopascal, ns2:megapascal, ns2:micropascal, ns2:millipascal, ns2:nanopascal, ns2:petapascal, ns2:picopascal, ns2:terapascal, ns2:bar, ns2:decibar, ns2:microbar, ns2:millibar, ns2:metreOfMercury, ns2:centimetreOfMercury, ns2:millimetreOfMercury, ns2:atmosphere-Standard, ns2:atmosphere-Technical, ns2:barye, ns2:torr .

ns2:ShearLossModulus
  a owl:Class ;
  rdfs:label "shear loss modulus"@en ;
  rdfs:subClassOf ns2:StorageModulus ;
  ns2:symbol "G''" ;
  ns2:commonlyHasUnit ns2:newtonPerSquareMetre, ns2:kilogramSecond-TimeToThePower-2ReciprocalMetre, ns2:pascal, ns2:attopascal, ns2:centipascal, ns2:decapascal, ns2:decipascal, ns2:exapascal, ns2:femtopascal, ns2:gigapascal, ns2:hectopascal, ns2:kilopascal, ns2:megapascal, ns2:micropascal, ns2:millipascal, ns2:nanopascal, ns2:petapascal, ns2:picopascal, ns2:terapascal, ns2:bar, ns2:decibar, ns2:microbar, ns2:millibar, ns2:metreOfMercury, ns2:centimetreOfMercury, ns2:millimetreOfMercury, ns2:atmosphere-Standard, ns2:atmosphere-Technical, ns2:barye, ns2:torr .

ns2:BulkModulus
  a owl:Class ;
  rdfs:label "bulk modulus"@en, "compressiemodulus"@nl ;
  rdfs:comment "Bulk modulus is a substance's resistance to uniform compression."@en ;
  rdfs:subClassOf ns2:DynamicModulus ;
  ns2:symbol "K" ;
  ns2:alternativeSymbol "κ" ;
  ns2:commonlyHasUnit ns2:newtonPerSquareMetre, ns2:kilogramSecond-TimeToThePower-2ReciprocalMetre, ns2:pascal, ns2:attopascal, ns2:centipascal, ns2:decapascal, ns2:decipascal, ns2:exapascal, ns2:femtopascal, ns2:gigapascal, ns2:hectopascal, ns2:kilopascal, ns2:megapascal, ns2:micropascal, ns2:millipascal, ns2:nanopascal, ns2:petapascal, ns2:picopascal, ns2:terapascal, ns2:bar, ns2:decibar, ns2:microbar, ns2:millibar, ns2:metreOfMercury, ns2:centimetreOfMercury, ns2:millimetreOfMercury, ns2:atmosphere-Standard, ns2:atmosphere-Technical, ns2:barye, ns2:torr .

ns2:ModulusOfElasticity
  a owl:Class ;
  rdfs:label "modulus of elasticity"@en, "elasticiteitsmodulus"@nl ;
  ns2:alternativeLabel "Young's modulus"@en ;
  rdfs:subClassOf ns2:DynamicModulus ;
  ns2:symbol "E" ;
  ns2:alternativeSymbol "Y" ;
  ns2:commonlyHasUnit ns2:newtonPerSquareMetre, ns2:kilogramSecond-TimeToThePower-2ReciprocalMetre, ns2:pascal, ns2:attopascal, ns2:centipascal, ns2:decapascal, ns2:decipascal, ns2:exapascal, ns2:femtopascal, ns2:gigapascal, ns2:hectopascal, ns2:kilopascal, ns2:megapascal, ns2:micropascal, ns2:millipascal, ns2:nanopascal, ns2:petapascal, ns2:picopascal, ns2:terapascal, ns2:bar, ns2:decibar, ns2:microbar, ns2:millibar, ns2:metreOfMercury, ns2:centimetreOfMercury, ns2:millimetreOfMercury, ns2:atmosphere-Standard, ns2:atmosphere-Technical, ns2:barye, ns2:torr .

ns2:ElasticityTensor
  a owl:Class ;
  rdfs:label "elasticity tensor"@en, "elasticiteitstensor"@nl ;
  ns2:alternativeLabel "stiffness tensor"@en ;
  rdfs:subClassOf ns2:DynamicModulus ;
  ns2:symbol "c_ijkl" ;
  ns2:commonlyHasUnit ns2:newtonPerSquareMetre, ns2:kilogramSecond-TimeToThePower-2ReciprocalMetre, ns2:pascal, ns2:attopascal, ns2:centipascal, ns2:decapascal, ns2:decipascal, ns2:exapascal, ns2:femtopascal, ns2:gigapascal, ns2:hectopascal, ns2:kilopascal, ns2:megapascal, ns2:micropascal, ns2:millipascal, ns2:nanopascal, ns2:petapascal, ns2:picopascal, ns2:terapascal, ns2:bar, ns2:decibar, ns2:microbar, ns2:millibar, ns2:metreOfMercury, ns2:centimetreOfMercury, ns2:millimetreOfMercury, ns2:atmosphere-Standard, ns2:atmosphere-Technical, ns2:barye, ns2:torr .

ns2:surfaceTension-Dimension
  a ns2:Dimension ;
  rdfs:label "surface tension dimension"@en, "oppervlaktespanningdimensie"@nl ;
  ns2:hasSILengthDimensionExponent 0 ;
  ns2:hasSIMassDimensionExponent 1 ;
  ns2:hasSITimeDimensionExponent -2 ;
  ns2:hasSIElectricCurrentDimensionExponent 0 ;
  ns2:hasSIThermodynamicTemperatureDimensionExponent 0 ;
  ns2:hasSIAmountOfSubstanceDimensionExponent 0 ;
  ns2:hasSILuminousIntensityDimensionExponent 0 .

ns2:fluidMechanicsDimensionlessNumbers
  a ns2:ApplicationArea ;
  rdfs:label "fluid mechanics dimensionless numbers"@en, "vloeistofmechanica dimensieloze getallen"@nl ;
  ns2:usesQuantity ns2:AlfvenNumber, ns2:CowlingNumber, ns2:EulerNumber, ns2:FirstCowlingNumber, ns2:FourierNumber, ns2:FourierNumberForMassTransfer, ns2:FroudeNumber, ns2:GrashofNumber, ns2:GrashofNumberForMassTransfer, ns2:HartmannNumber, ns2:KnudsenNumber, ns2:LewisNumber, ns2:MachNumber, ns2:MagneticReynoldsNumber, ns2:NusseltNumber, ns2:NusseltNumberForMassTransfer, ns2:PecletNumber, ns2:PecletNumberForMassTransfer, ns2:PrandtlNumber, ns2:RayleighNumber, ns2:ReynoldsNumber, ns2:SchmidtNumber, ns2:StantonNumber, ns2:StantonNumberForMassTransfer, ns2:StrouhalNumber, ns2:WeberNumber .

ns2:AlfvenNumber
  a owl:Class ;
  rdfs:label "Alfvén number"@en ;
  rdfs:subClassOf ns2:Quantity, [
    a owl:Restriction ;
    owl:onProperty ns2:hasValue ;
    owl:allValuesFrom [
      a owl:Restriction ;
      owl:onProperty ns2:hasUnit ;
      owl:allValuesFrom ns2:AlfvenNumberUnit
    ]
  ], [
    a owl:Restriction ;
    owl:onProperty ns2:hasDimension ;
    owl:hasValue ns2:dimensionOne
  ] ;
  ns2:symbol "Al" ;
  ns2:commonlyHasUnit ns2:one .

ns2:AlfvenNumberUnit
  a owl:Class ;
  rdfs:label "Alfvén number unit"@en ;
  rdfs:subClassOf ns2:Unit ;
  owl:equivalentClass [
    a owl:Class ;
    owl:oneOf ( ns2:one )
  ] .

ns2:CowlingNumber
  a owl:Class ;
  rdfs:label "Cowling number"@en ;
  ns2:alternativeLabel "second Cowling number"@en ;
  rdfs:subClassOf ns2:Quantity, [
    a owl:Restriction ;
    owl:onProperty ns2:hasValue ;
    owl:allValuesFrom [
      a owl:Restriction ;
      owl:onProperty ns2:hasUnit ;
      owl:allValuesFrom ns2:CowlingNumberUnit
    ]
  ], [
    a owl:Restriction ;
    owl:onProperty ns2:hasDimension ;
    owl:hasValue ns2:dimensionOne
  ] ;
  ns2:symbol "Co" ;
  ns2:alternativeSymbol "Co2" ;
  ns2:commonlyHasUnit ns2:one .

ns2:CowlingNumberUnit
  a owl:Class ;
  rdfs:label "Cowling number unit"@en ;
  rdfs:subClassOf ns2:Unit ;
  owl:equivalentClass [
    a owl:Class ;
    owl:oneOf ( ns2:one )
  ] .

ns2:EulerNumber
  a owl:Class ;
  rdfs:label "Euler number"@en, "getal van Euler"@nl ;
  rdfs:comment "The Euler number is a dimensionless number that expresses the relationship between a local pressure drop e.g. over a restriction and the kinetic energy per unit volume."@en ;
  rdfs:subClassOf ns2:Quantity, [
    a owl:Restriction ;
    owl:onProperty ns2:hasValue ;
    owl:allValuesFrom [
      a owl:Restriction ;
      owl:onProperty ns2:hasUnit ;
      owl:allValuesFrom ns2:EulerNumberUnit
    ]
  ], [
    a owl:Restriction ;
    owl:onProperty ns2:hasDimension ;
    owl:hasValue ns2:dimensionOne
  ] ;
  ns2:symbol "Eu" ;
  ns2:commonlyHasUnit ns2:one .

ns2:EulerNumberUnit
  a owl:Class ;
  rdfs:label "Euler number unit"@en ;
  rdfs:subClassOf ns2:Unit ;
  owl:equivalentClass [
    a owl:Class ;
    owl:oneOf ( ns2:one )
  ] .

ns2:FirstCowlingNumber
  a owl:Class ;
  rdfs:label "first Cowling number"@en ;
  rdfs:subClassOf ns2:Quantity, [
    a owl:Restriction ;
    owl:onProperty ns2:hasValue ;
    owl:allValuesFrom [
      a owl:Restriction ;
      owl:onProperty ns2:hasUnit ;
      owl:allValuesFrom ns2:FirstCowlingNumberUnit
    ]
  ], [
    a owl:Restriction ;
    owl:onProperty ns2:hasDimension ;
    owl:hasValue ns2:dimensionOne
  ] ;
  ns2:symbol "Co_1" ;
  ns2:commonlyHasUnit ns2:one .

ns2:FirstCowlingNumberUnit
  a owl:Class ;
  rdfs:label "first Cowling number unit"@en ;
  rdfs:subClassOf ns2:Unit ;
  owl:equivalentClass [
    a owl:Class ;
    owl:oneOf ( ns2:one )
  ] .

ns2:FourierNumber
  a owl:Class ;
  rdfs:label "Fourier number"@en, "getal van Fourier"@nl ;
  rdfs:comment "The Fourier number is a dimensionless number that characterises heat conduction. It is the ratio of heat conduction rate to rate of thermal energy storage. The Fourier number is a dimensionless time."@en ;
  rdfs:subClassOf ns2:Quantity, [
    a owl:Restriction ;
    owl:onProperty ns2:hasValue ;
    owl:allValuesFrom [
      a owl:Restriction ;
      owl:onProperty ns2:hasUnit ;
      owl:allValuesFrom ns2:FourierNumberUnit
    ]
  ], [
    a owl:Restriction ;
    owl:onProperty ns2:hasDimension ;
    owl:hasValue ns2:dimensionOne
  ] ;
  ns2:symbol "Fo" ;
  ns2:commonlyHasUnit ns2:one .

ns2:FourierNumberUnit
  a owl:Class ;
  rdfs:label "Fourier number unit"@en ;
  rdfs:subClassOf ns2:Unit ;
  owl:equivalentClass [
    a owl:Class ;
    owl:oneOf ( ns2:one )
  ] .

ns2:FourierNumberForMassTransfer
  a owl:Class ;
  rdfs:label "Fourier number for mass transfer"@en ;
  rdfs:subClassOf ns2:Quantity, [
    a owl:Restriction ;
    owl:onProperty ns2:hasValue ;
    owl:allValuesFrom [
      a owl:Restriction ;
      owl:onProperty ns2:hasUnit ;
      owl:allValuesFrom ns2:FourierNumberForMassTransferUnit
    ]
  ], [
    a owl:Restriction ;
    owl:onProperty ns2:hasDimension ;
    owl:hasValue ns2:dimensionOne
  ] ;
  ns2:symbol "Fo*" ;
  ns2:commonlyHasUnit ns2:one .

ns2:FourierNumberForMassTransferUnit
  a owl:Class ;
  rdfs:label "Fourier number for mass transfer unit"@en ;
  rdfs:subClassOf ns2:Unit ;
  owl:equivalentClass [
    a owl:Class ;
    owl:oneOf ( ns2:one )
  ] .

ns2:FroudeNumber
  a owl:Class ;
  rdfs:label "Froude number"@en, "getal van Froude"@nl ;
  rdfs:comment "The Froude number is a dimensionless number that compares inertial and gravitational forces. It may be used to quantify the resistance of an object moving through water, and compare objects of different sizes."@en ;
  rdfs:subClassOf ns2:Quantity, [
    a owl:Restriction ;
    owl:onProperty ns2:hasValue ;
    owl:allValuesFrom [
      a owl:Restriction ;
      owl:onProperty ns2:hasUnit ;
      owl:allValuesFrom ns2:FroudeNumberUnit
    ]
  ], [
    a owl:Restriction ;
    owl:onProperty ns2:hasDimension ;
    owl:hasValue ns2:dimensionOne
  ] ;
  ns2:symbol "Fr" ;
  ns2:commonlyHasUnit ns2:one .

ns2:FroudeNumberUnit
  a owl:Class ;
  rdfs:label "Froude number unit"@en ;
  rdfs:subClassOf ns2:Unit ;
  owl:equivalentClass [
    a owl:Class ;
    owl:oneOf ( ns2:one )
  ] .

ns2:GrashofNumber
  a owl:Class ;
  rdfs:label "Grashof number"@en, "getal van Grashof"@nl ;
  rdfs:comment "The Grashof number is a dimensionless number that approximates the ratio of buoyancy to viscous force that acts on a fluid."@en ;
  rdfs:subClassOf ns2:Quantity, [
    a owl:Restriction ;
    owl:onProperty ns2:hasValue ;
    owl:allValuesFrom [
      a owl:Restriction ;
      owl:onProperty ns2:hasUnit ;
      owl:allValuesFrom ns2:GrashofNumberUnit
    ]
  ], [
    a owl:Restriction ;
    owl:onProperty ns2:hasDimension ;
    owl:hasValue ns2:dimensionOne
  ] ;
  ns2:symbol "Gr" ;
  ns2:commonlyHasUnit ns2:one .

ns2:GrashofNumberUnit
  a owl:Class ;
  rdfs:label "Grashof number unit"@en ;
  rdfs:subClassOf ns2:Unit ;
  owl:equivalentClass [
    a owl:Class ;
    owl:oneOf ( ns2:one )
  ] .

ns2:GrashofNumberForMassTransfer
  a owl:Class ;
  rdfs:label "Grashof number for mass transfer"@en ;
  rdfs:subClassOf ns2:Quantity, [
    a owl:Restriction ;
    owl:onProperty ns2:hasValue ;
    owl:allValuesFrom [
      a owl:Restriction ;
      owl:onProperty ns2:hasUnit ;
      owl:allValuesFrom ns2:GrashofNumberForMassTransferUnit
    ]
  ], [
    a owl:Restriction ;
    owl:onProperty ns2:hasDimension ;
    owl:hasValue ns2:dimensionOne
  ] ;
  ns2:symbol "Gr*" ;
  ns2:commonlyHasUnit ns2:one .

ns2:GrashofNumberForMassTransferUnit
  a owl:Class ;
  rdfs:label "Grashof number for mass transfer unit"@en ;
  rdfs:subClassOf ns2:Unit ;
  owl:equivalentClass [
    a owl:Class ;
    owl:oneOf ( ns2:one )
  ] .

ns2:HartmannNumber
  a owl:Class ;
  rdfs:label "Hartmann number"@en, "getal van Hartmann"@nl ;
  rdfs:subClassOf ns2:Quantity, [
    a owl:Restriction ;
    owl:onProperty ns2:hasValue ;
    owl:allValuesFrom [
      a owl:Restriction ;
      owl:onProperty ns2:hasUnit ;
      owl:allValuesFrom ns2:HartmannNumberUnit
    ]
  ], [
    a owl:Restriction ;
    owl:onProperty ns2:hasDimension ;
    owl:hasValue ns2:dimensionOne
  ] ;
  ns2:symbol "Ha" ;
  ns2:commonlyHasUnit ns2:one .

ns2:HartmannNumberUnit
  a owl:Class ;
  rdfs:label "Hartmann number unit"@en ;
  rdfs:subClassOf ns2:Unit ;
  owl:equivalentClass [
    a owl:Class ;
    owl:oneOf ( ns2:one )
  ] .

ns2:KnudsenNumber
  a owl:Class ;
  rdfs:label "Knudsen number"@en, "getal van Knudsen"@nl ;
  rdfs:comment "The Knudsen number is a dimensionless number defined as the ratio of the molecular mean free path length to a representative physical length scale."@en ;
  rdfs:subClassOf ns2:Quantity, [
    a owl:Restriction ;
    owl:onProperty ns2:hasValue ;
    owl:allValuesFrom [
      a owl:Restriction ;
      owl:onProperty ns2:hasUnit ;
      owl:allValuesFrom ns2:KnudsenNumberUnit
    ]
  ], [
    a owl:Restriction ;
    owl:onProperty ns2:hasDimension ;
    owl:hasValue ns2:dimensionOne
  ] ;
  ns2:symbol "Kn" ;
  ns2:commonlyHasUnit ns2:one .

ns2:KnudsenNumberUnit
  a owl:Class ;
  rdfs:label "Knudsen number unit"@en ;
  rdfs:subClassOf ns2:Unit ;
  owl:equivalentClass [
    a owl:Class ;
    owl:oneOf ( ns2:one )
  ] .

ns2:LewisNumber
  a owl:Class ;
  rdfs:label "Lewis number"@en, "getal van Lewis"@nl ;
  rdfs:comment "The Lewis number is a dimensionless number defined as the ratio of thermal diffusivity to mass diffusivity."@en ;
  rdfs:subClassOf ns2:Quantity, [
    a owl:Restriction ;
    owl:onProperty ns2:hasValue ;
    owl:allValuesFrom [
      a owl:Restriction ;
      owl:onProperty ns2:hasUnit ;
      owl:allValuesFrom ns2:LewisNumberUnit
    ]
  ], [
    a owl:Restriction ;
    owl:onProperty ns2:hasDimension ;
    owl:hasValue ns2:dimensionOne
  ] ;
  ns2:symbol "Le" ;
  ns2:commonlyHasUnit ns2:one .

ns2:LewisNumberUnit
  a owl:Class ;
  rdfs:label "Lewis number unit"@en ;
  rdfs:subClassOf ns2:Unit ;
  owl:equivalentClass [
    a owl:Class ;
    owl:oneOf ( ns2:one )
  ] .

ns2:MachNumber
  a owl:Class ;
  rdfs:label "Mach number"@en, "Machgetal"@nl ;
  rdfs:comment "The Mach number is the speed of an object that moves through air, or any fluid substance, divided by the speed of sound as it is in that substance."@en ;
  rdfs:subClassOf ns2:Quantity, [
    a owl:Restriction ;
    owl:onProperty ns2:hasValue ;
    owl:allValuesFrom [
      a owl:Restriction ;
      owl:onProperty ns2:hasUnit ;
      owl:allValuesFrom ns2:MachNumberUnit
    ]
  ], [
    a owl:Restriction ;
    owl:onProperty ns2:hasDimension ;
    owl:hasValue ns2:dimensionOne
  ] ;
  ns2:symbol "Ma" ;
  ns2:commonlyHasUnit ns2:one .

ns2:MachNumberUnit
  a owl:Class ;
  rdfs:label "Mach number unit"@en ;
  rdfs:subClassOf ns2:Unit ;
  owl:equivalentClass [
    a owl:Class ;
    owl:oneOf ( ns2:one )
  ] .

ns2:MagneticReynoldsNumber
  a owl:Class ;
  rdfs:label "magnetic Reynolds number"@en, "magnetisch getal van Reynolds"@nl ;
  rdfs:subClassOf ns2:Quantity, [
    a owl:Restriction ;
    owl:onProperty ns2:hasValue ;
    owl:allValuesFrom [
      a owl:Restriction ;
      owl:onProperty ns2:hasUnit ;
      owl:allValuesFrom ns2:MagneticReynoldsNumberUnit
    ]
  ], [
    a owl:Restriction ;
    owl:onProperty ns2:hasDimension ;
    owl:hasValue ns2:dimensionOne
  ] ;
  ns2:symbol "Rm" ;
  ns2:commonlyHasUnit ns2:one .

ns2:MagneticReynoldsNumberUnit
  a owl:Class ;
  rdfs:label "magnetic Reynolds number unit"@en ;
  rdfs:subClassOf ns2:Unit ;
  owl:equivalentClass [
    a owl:Class ;
    owl:oneOf ( ns2:one )
  ] .

ns2:NusseltNumber
  a owl:Class ;
  rdfs:label "Nusselt number"@en, "getal van Nusselt"@nl ;
  rdfs:comment "The Nusselt number is the ratio of convective to conductive heat transfer across (normal to) the boundary."@en ;
  rdfs:subClassOf ns2:Quantity, [
    a owl:Restriction ;
    owl:onProperty ns2:hasValue ;
    owl:allValuesFrom [
      a owl:Restriction ;
      owl:onProperty ns2:hasUnit ;
      owl:allValuesFrom ns2:NusseltNumberUnit
    ]
  ], [
    a owl:Restriction ;
    owl:onProperty ns2:hasDimension ;
    owl:hasValue ns2:dimensionOne
  ] ;
  ns2:symbol "Nu" ;
  ns2:commonlyHasUnit ns2:one .

ns2:NusseltNumberUnit
  a owl:Class ;
  rdfs:label "Nusselt number unit"@en ;
  rdfs:subClassOf ns2:Unit ;
  owl:equivalentClass [
    a owl:Class ;
    owl:oneOf ( ns2:one )
  ] .

ns2:NusseltNumberForMassTransfer
  a owl:Class ;
  rdfs:label "Nusselt number for mass transfer"@en ;
  rdfs:subClassOf ns2:Quantity, [
    a owl:Restriction ;
    owl:onProperty ns2:hasValue ;
    owl:allValuesFrom [
      a owl:Restriction ;
      owl:onProperty ns2:hasUnit ;
      owl:allValuesFrom ns2:NusseltNumberForMassTransferUnit
    ]
  ], [
    a owl:Restriction ;
    owl:onProperty ns2:hasDimension ;
    owl:hasValue ns2:dimensionOne
  ] ;
  ns2:symbol "Nu*" ;
  ns2:commonlyHasUnit ns2:one .

ns2:NusseltNumberForMassTransferUnit
  a owl:Class ;
  rdfs:label "Nusselt number for mass transfer unit"@en ;
  rdfs:subClassOf ns2:Unit ;
  owl:equivalentClass [
    a owl:Class ;
    owl:oneOf ( ns2:one )
  ] .

ns2:PecletNumber
  a owl:Class ;
  rdfs:label "Péclet number"@en, "getal van Péclet"@nl ;
  rdfs:comment "The Péclet number is a dimensionless number that relates the rate of advection of a flow to its rate of diffusion, often thermal diffusion."@en ;
  rdfs:subClassOf ns2:Quantity, [
    a owl:Restriction ;
    owl:onProperty ns2:hasValue ;
    owl:allValuesFrom [
      a owl:Restriction ;
      owl:onProperty ns2:hasUnit ;
      owl:allValuesFrom ns2:PecletNumberUnit
    ]
  ], [
    a owl:Restriction ;
    owl:onProperty ns2:hasDimension ;
    owl:hasValue ns2:dimensionOne
  ] ;
  ns2:symbol "Pe" ;
  ns2:commonlyHasUnit ns2:one .

ns2:PecletNumberUnit
  a owl:Class ;
  rdfs:label "Péclet number unit"@en ;
  rdfs:subClassOf ns2:Unit ;
  owl:equivalentClass [
    a owl:Class ;
    owl:oneOf ( ns2:one )
  ] .

ns2:PecletNumberForMassTransfer
  a owl:Class ;
  rdfs:label "Péclet number for mass transfer"@en ;
  rdfs:subClassOf ns2:Quantity, [
    a owl:Restriction ;
    owl:onProperty ns2:hasValue ;
    owl:allValuesFrom [
      a owl:Restriction ;
      owl:onProperty ns2:hasUnit ;
      owl:allValuesFrom ns2:PecletNumberForMassTransferUnit
    ]
  ], [
    a owl:Restriction ;
    owl:onProperty ns2:hasDimension ;
    owl:hasValue ns2:dimensionOne
  ] ;
  ns2:symbol "Pe*" ;
  ns2:commonlyHasUnit ns2:one .

ns2:PecletNumberForMassTransferUnit
  a owl:Class ;
  rdfs:label "Péclet number for mass transfer unit"@en ;
  rdfs:subClassOf ns2:Unit ;
  owl:equivalentClass [
    a owl:Class ;
    owl:oneOf ( ns2:one )
  ] .

ns2:PrandtlNumber
  a owl:Class ;
  rdfs:label "Prandtl number"@en, "getal van Prandtl"@nl ;
  rdfs:subClassOf ns2:Quantity, [
    a owl:Restriction ;
    owl:onProperty ns2:hasValue ;
    owl:allValuesFrom [
      a owl:Restriction ;
      owl:onProperty ns2:hasUnit ;
      owl:allValuesFrom ns2:PrandtlNumberUnit
    ]
  ], [
    a owl:Restriction ;
    owl:onProperty ns2:hasDimension ;
    owl:hasValue ns2:dimensionOne
  ] ;
  ns2:symbol "Pr" ;
  ns2:commonlyHasUnit ns2:one .

ns2:PrandtlNumberUnit
  a owl:Class ;
  rdfs:label "Prandtl number unit"@en ;
  rdfs:subClassOf ns2:Unit ;
  owl:equivalentClass [
    a owl:Class ;
    owl:oneOf ( ns2:one )
  ] .

ns2:RayleighNumber
  a owl:Class ;
  rdfs:label "Rayleigh number"@en, "getal van Rayleigh"@nl ;
  rdfs:comment "The Rayleigh number for a fluid is a dimensionless number associated with buoyancy driven flow."@en ;
  rdfs:subClassOf ns2:Quantity, [
    a owl:Restriction ;
    owl:onProperty ns2:hasValue ;
    owl:allValuesFrom [
      a owl:Restriction ;
      owl:onProperty ns2:hasUnit ;
      owl:allValuesFrom ns2:RayleighNumberUnit
    ]
  ], [
    a owl:Restriction ;
    owl:onProperty ns2:hasDimension ;
    owl:hasValue ns2:dimensionOne
  ] ;
  ns2:symbol "Ra" ;
  ns2:commonlyHasUnit ns2:one .

ns2:RayleighNumberUnit
  a owl:Class ;
  rdfs:label "Rayleigh number unit"@en ;
  rdfs:subClassOf ns2:Unit ;
  owl:equivalentClass [
    a owl:Class ;
    owl:oneOf ( ns2:one )
  ] .

ns2:ReynoldsNumber
  a owl:Class ;
  rdfs:label "Reynolds number"@en, "getal van Reynolds"@nl ;
  rdfs:comment "The Reynolds number is a dimensionless number that gives a measure of the ratio of inertial forces to viscous forces and, consequently, quantifies the relative importance of these two types of forces for given flow conditions."@en ;
  rdfs:subClassOf ns2:Quantity, [
    a owl:Restriction ;
    owl:onProperty ns2:hasValue ;
    owl:allValuesFrom [
      a owl:Restriction ;
      owl:onProperty ns2:hasUnit ;
      owl:allValuesFrom ns2:ReynoldsNumberUnit
    ]
  ], [
    a owl:Restriction ;
    owl:onProperty ns2:hasDimension ;
    owl:hasValue ns2:dimensionOne
  ] ;
  ns2:symbol "Re" ;
  ns2:commonlyHasUnit ns2:one .

ns2:ReynoldsNumberUnit
  a owl:Class ;
  rdfs:label "Reynolds number unit"@en ;
  rdfs:subClassOf ns2:Unit ;
  owl:equivalentClass [
    a owl:Class ;
    owl:oneOf ( ns2:one )
  ] .

ns2:SchmidtNumber
  a owl:Class ;
  rdfs:label "Schmidt number"@en, "getal van Schmidt"@nl ;
  rdfs:subClassOf ns2:Quantity, [
    a owl:Restriction ;
    owl:onProperty ns2:hasValue ;
    owl:allValuesFrom [
      a owl:Restriction ;
      owl:onProperty ns2:hasUnit ;
      owl:allValuesFrom ns2:SchmidtNumberUnit
    ]
  ], [
    a owl:Restriction ;
    owl:onProperty ns2:hasDimension ;
    owl:hasValue ns2:dimensionOne
  ] ;
  ns2:symbol "Sc" ;
  ns2:commonlyHasUnit ns2:one .

ns2:SchmidtNumberUnit
  a owl:Class ;
  rdfs:label "Schmidt number unit"@en ;
  rdfs:subClassOf ns2:Unit ;
  owl:equivalentClass [
    a owl:Class ;
    owl:oneOf ( ns2:one )
  ] .

ns2:StantonNumber
  a owl:Class ;
  rdfs:label "Stanton number"@en, "getal van Stanton"@nl ;
  rdfs:comment "The Stanton number is a dimensionless number that measures the ratio of heat transferred into a fluid to the thermal capacity of fluid."@en ;
  rdfs:subClassOf ns2:Quantity, [
    a owl:Restriction ;
    owl:onProperty ns2:hasValue ;
    owl:allValuesFrom [
      a owl:Restriction ;
      owl:onProperty ns2:hasUnit ;
      owl:allValuesFrom ns2:StantonNumberUnit
    ]
  ], [
    a owl:Restriction ;
    owl:onProperty ns2:hasDimension ;
    owl:hasValue ns2:dimensionOne
  ] ;
  ns2:symbol "St" ;
  ns2:commonlyHasUnit ns2:one .

ns2:StantonNumberUnit
  a owl:Class ;
  rdfs:label "Stanton number unit"@en ;
  rdfs:subClassOf ns2:Unit ;
  owl:equivalentClass [
    a owl:Class ;
    owl:oneOf ( ns2:one )
  ] .

ns2:StantonNumberForMassTransfer
  a owl:Class ;
  rdfs:label "Stanton number for mass transfer"@en ;
  rdfs:subClassOf ns2:Quantity, [
    a owl:Restriction ;
    owl:onProperty ns2:hasValue ;
    owl:allValuesFrom [
      a owl:Restriction ;
      owl:onProperty ns2:hasUnit ;
      owl:allValuesFrom ns2:StantonNumberForMassTransferUnit
    ]
  ], [
    a owl:Restriction ;
    owl:onProperty ns2:hasDimension ;
    owl:hasValue ns2:dimensionOne
  ] ;
  ns2:symbol "St*" ;
  ns2:commonlyHasUnit ns2:one .

ns2:StantonNumberForMassTransferUnit
  a owl:Class ;
  rdfs:label "Stanton number for mass transfer unit"@en ;
  rdfs:subClassOf ns2:Unit ;
  owl:equivalentClass [
    a owl:Class ;
    owl:oneOf ( ns2:one )
  ] .

ns2:StrouhalNumber
  a owl:Class ;
  rdfs:label "Strouhal number"@en, "getal van Strouhal"@nl ;
  rdfs:comment "The Strouhal number is a dimensionless number that describes oscillating flow mechanisms."@en ;
  rdfs:subClassOf ns2:Quantity, [
    a owl:Restriction ;
    owl:onProperty ns2:hasValue ;
    owl:allValuesFrom [
      a owl:Restriction ;
      owl:onProperty ns2:hasUnit ;
      owl:allValuesFrom ns2:StrouhalNumberUnit
    ]
  ], [
    a owl:Restriction ;
    owl:onProperty ns2:hasDimension ;
    owl:hasValue ns2:dimensionOne
  ] ;
  ns2:symbol "Sr" ;
  ns2:commonlyHasUnit ns2:one .

ns2:StrouhalNumberUnit
  a owl:Class ;
  rdfs:label "Strouhal number unit"@en ;
  rdfs:subClassOf ns2:Unit ;
  owl:equivalentClass [
    a owl:Class ;
    owl:oneOf ( ns2:one )
  ] .

ns2:WeberNumber
  a owl:Class ;
  rdfs:label "Weber number"@en, "getal van Weber"@nl ;
  rdfs:subClassOf ns2:Quantity, [
    a owl:Restriction ;
    owl:onProperty ns2:hasValue ;
    owl:allValuesFrom [
      a owl:Restriction ;
      owl:onProperty ns2:hasUnit ;
      owl:allValuesFrom ns2:WeberNumberUnit
    ]
  ], [
    a owl:Restriction ;
    owl:onProperty ns2:hasDimension ;
    owl:hasValue ns2:dimensionOne
  ] ;
  ns2:symbol "We" ;
  ns2:commonlyHasUnit ns2:one .

ns2:WeberNumberUnit
  a owl:Class ;
  rdfs:label "Weber number unit"@en ;
  rdfs:subClassOf ns2:Unit ;
  owl:equivalentClass [
    a owl:Class ;
    owl:oneOf ( ns2:one )
  ] .

ns2:chemicalPhysics
  a ns2:ApplicationArea ;
  rdfs:label "chemical physics"@en, "fysische chemie"@nl ;
  ns2:usesQuantity ns2:AmountOfSubstance, ns2:AmountOfSubstanceConcentration, ns2:AmountOfSubstanceFraction, ns2:MolarEnergy, ns2:ResonanceEnergy, ns2:MolarEntropy, ns2:MolarHeatCapacity, ns2:AmountOfSubstanceFlow, ns2:Molality, ns2:MolarMass, ns2:MolarVolume, ns2:AmountOfSubstanceFractionFlow ;
  ns2:usesUnit ns2:one, ns2:partsPerMillion, ns2:percent, ns2:mole, ns2:attomole, ns2:centimole, ns2:decamole, ns2:decimole, ns2:examole, ns2:femtomole, ns2:gigamole, ns2:hectomole, ns2:kilomole, ns2:megamole, ns2:micromole, ns2:millimole, ns2:nanomole, ns2:petamole, ns2:picomole, ns2:teramole, ns2:molePerCubicmetre, ns2:molePerLitre, ns2:attomolePerLitre, ns2:centimolePerLitre, ns2:decamolePerLitre, ns2:decimolePerLitre, ns2:examolePerLitre, ns2:femtomolePerLitre, ns2:gigamolePerLitre, ns2:hectomolePerLitre, ns2:kilomolePerLitre, ns2:megamolePerLitre, ns2:micromolePerLitre, ns2:millimolePerLitre, ns2:nanomolePerLitre, ns2:petamolePerLitre, ns2:picomolePerLitre, ns2:teramolePerLitre, ns2:molePerAttolitre, ns2:molePerCentilitre, ns2:molePerDecalitre, ns2:molePerDecilitre, ns2:molePerExalitre, ns2:molePerFemtolitre, ns2:molePerGigalitre, ns2:molePerHectolitre, ns2:molePerKilolitre, ns2:molePerMegalitre, ns2:molePerMicrolitre, ns2:molePerMillilitre, ns2:molePerNanolitre, ns2:molePerPetalitre, ns2:molePerPicolitre, ns2:molePerTeralitre, ns2:molar, ns2:attomolar, ns2:femtomolar, ns2:megamolar, ns2:micromolar, ns2:millimolar, ns2:nanomolar, ns2:picomolar, ns2:molePerMole, ns2:micromolePerMole, ns2:joulePerMole, ns2:joulePerKelvinMole, ns2:molePerKilogram, ns2:kilogramPerMole, ns2:cubicMetrePerMole, ns2:litrePerMole, ns2:moleMicrometre, ns2:moleMicrometreReciprocalSquareCentimetre, ns2:moleMicrometreReciprocalSquareCentimetreReciprocalSecond-Time, ns2:molePerMetre, ns2:attomolePerMetre, ns2:femtomolePerMetre, ns2:picomolePerMetre, ns2:nanomolePerMetre, ns2:micromolePerMetre, ns2:millimolePerMetre, ns2:centimolePerMetre, ns2:decimolePerMetre, ns2:decamolePerMetre, ns2:hectomolePerMetre, ns2:kilomolePerMetre, ns2:megamolePerMetre, ns2:gigamolePerMetre, ns2:teramolePerMetre, ns2:petamolePerMetre, ns2:examolePerMetre, ns2:molePerYoctometre, ns2:molePerZeptometre, ns2:molePerAttometre, ns2:molePerFemtometre, ns2:molePerPicometre, ns2:molePerNanometre, ns2:molePerMicrometre, ns2:molePerMillimetre, ns2:molePerCentimetre, ns2:molePerDecimetre, ns2:molePerDecametre, ns2:molePerHectometre, ns2:molePerKilometre, ns2:molePermegametre, ns2:molePerGigametre, ns2:molePerTerametre, ns2:molePerPetametre, ns2:molePerExametre, ns2:molePerZettametre, ns2:molePerYottametre, ns2:kelvinMole, ns2:micromolePerSecond-TimeGram .

ns2:AmountOfSubstance
  a owl:Class ;
  rdfs:label "amount of substance"@en, "stofhoeveelheid"@nl ;
  rdfs:comment "Amount of substance is the number of elementary entities such as atoms, molecules, electrons, particles, etc. present in a phenomenon. It is a base quantity in the International System of Units."@en ;
  rdfs:subClassOf ns2:Quantity, [
    a owl:Restriction ;
    owl:onProperty ns2:hasValue ;
    owl:allValuesFrom [
      a owl:Restriction ;
      owl:onProperty ns2:hasUnit ;
      owl:allValuesFrom ns2:AmountOfSubstanceUnit
    ]
  ], [
    a owl:Restriction ;
    owl:onProperty ns2:hasDimension ;
    owl:hasValue ns2:amountOfSubstance-Dimension
  ] ;
  ns2:symbol "n" ;
  ns2:commonlyHasUnit ns2:mole, ns2:attomole, ns2:centimole, ns2:decamole, ns2:decimole, ns2:examole, ns2:femtomole, ns2:gigamole, ns2:hectomole, ns2:kilomole, ns2:megamole, ns2:micromole, ns2:millimole, ns2:nanomole, ns2:petamole, ns2:picomole, ns2:teramole .

ns2:AmountOfSubstanceConcentration
  a owl:Class ;
  rdfs:label "amount of substance concentration"@en ;
  ns2:alternativeLabel "molar concentration"@en, "molaire concentratie"@nl ;
  rdfs:subClassOf ns2:Quantity, [
    a owl:Restriction ;
    owl:onProperty ns2:hasValue ;
    owl:allValuesFrom [
      a owl:Restriction ;
      owl:onProperty ns2:hasUnit ;
      owl:allValuesFrom ns2:AmountOfSubstanceConcentrationUnit
    ]
  ], [
    a owl:Restriction ;
    owl:onProperty ns2:hasDimension ;
    owl:hasValue ns2:amountOfSubstanceConcentration-Dimension
  ] ;
  ns2:symbol "C" ;
  ns2:commonlyHasUnit ns2:molePerCubicmetre, ns2:molePerLitre, ns2:attomolePerLitre, ns2:centimolePerLitre, ns2:decamolePerLitre, ns2:decimolePerLitre, ns2:examolePerLitre, ns2:femtomolePerLitre, ns2:gigamolePerLitre, ns2:hectomolePerLitre, ns2:kilomolePerLitre, ns2:megamolePerLitre, ns2:micromolePerLitre, ns2:millimolePerLitre, ns2:nanomolePerLitre, ns2:petamolePerLitre, ns2:picomolePerLitre, ns2:teramolePerLitre, ns2:molePerAttolitre, ns2:molePerCentilitre, ns2:molePerDecalitre, ns2:molePerDecilitre, ns2:molePerExalitre, ns2:molePerFemtolitre, ns2:molePerGigalitre, ns2:molePerHectolitre, ns2:molePerKilolitre, ns2:molePerMegalitre, ns2:molePerMicrolitre, ns2:molePerMillilitre, ns2:molePerNanolitre, ns2:molePerPetalitre, ns2:molePerPicolitre, ns2:molePerTeralitre, ns2:molar, ns2:attomolar, ns2:femtomolar, ns2:megamolar, ns2:micromolar, ns2:millimolar, ns2:nanomolar, ns2:picomolar .

ns2:AmountOfSubstanceFraction
  a owl:Class ;
  rdfs:label "amount of substance fraction"@en ;
  ns2:alternativeLabel "amount-of-substance fraction"@en, "mole fraction"@en, "molfractie"@nl ;
  rdfs:subClassOf ns2:Quantity, [
    a owl:Restriction ;
    owl:onProperty ns2:hasDimension ;
    owl:hasValue ns2:dimensionOne
  ], [
    a owl:Restriction ;
    owl:onProperty ns2:hasValue ;
    owl:allValuesFrom [
      a owl:Restriction ;
      owl:onProperty ns2:hasUnit ;
      owl:allValuesFrom ns2:AmountOfSubstanceFractionUnit
    ]
  ] ;
  ns2:symbol "x" ;
  ns2:alternativeSymbol "y" ;
  ns2:commonlyHasUnit ns2:one, ns2:partsPerMillion, ns2:percent, ns2:molePerMole, ns2:micromolePerMole .

ns2:MolarEnergy
  a owl:Class ;
  rdfs:label "molar energy"@en, "molaire energie"@nl ;
  rdfs:subClassOf ns2:Quantity, [
    a owl:Restriction ;
    owl:onProperty ns2:hasValue ;
    owl:allValuesFrom [
      a owl:Restriction ;
      owl:onProperty ns2:hasUnit ;
      owl:allValuesFrom ns2:MolarEnergyUnit
    ]
  ], [
    a owl:Restriction ;
    owl:onProperty ns2:hasDimension ;
    owl:hasValue ns2:molarEnergy-Dimension
  ] ;
  ns2:commonlyHasUnit ns2:joulePerMole .

ns2:ResonanceEnergy
  a owl:Class ;
  rdfs:label "resonance energy"@en ;
  rdfs:subClassOf ns2:MolarEnergy ;
  ns2:commonlyHasUnit ns2:joulePerMole .

ns2:MolarEntropy
  a owl:Class ;
  rdfs:label "molar entropy"@en, "molaire entropie"@nl ;
  rdfs:subClassOf ns2:Quantity, [
    a owl:Restriction ;
    owl:onProperty ns2:hasValue ;
    owl:allValuesFrom [
      a owl:Restriction ;
      owl:onProperty ns2:hasUnit ;
      owl:allValuesFrom ns2:MolarEntropyUnit
    ]
  ], [
    a owl:Restriction ;
    owl:onProperty ns2:hasDimension ;
    owl:hasValue ns2:molarEntropyOrMolarHeatCapacityOrGasConstant-Dimension
  ] ;
  ns2:commonlyHasUnit ns2:joulePerKelvinMole .

ns2:MolarHeatCapacity
  a owl:Class ;
  rdfs:label "molar heat capacity"@en, "molaire warmtecapaciteit"@nl ;
  rdfs:subClassOf ns2:Quantity, [
    a owl:Restriction ;
    owl:onProperty ns2:hasValue ;
    owl:allValuesFrom [
      a owl:Restriction ;
      owl:onProperty ns2:hasUnit ;
      owl:allValuesFrom ns2:MolarHeatCapacityUnit
    ]
  ], [
    a owl:Restriction ;
    owl:onProperty ns2:hasDimension ;
    owl:hasValue ns2:molarEntropyOrMolarHeatCapacityOrGasConstant-Dimension
  ] ;
  ns2:commonlyHasUnit ns2:joulePerKelvinMole .

ns2:GasConstant
  a owl:Class ;
  rdfs:label "gas constant"@en, "gasconstante"@nl ;
  ns2:alternativeLabel "universal gas constant"@en, "universele gasconstante"@nl ;
  rdfs:subClassOf ns2:Quantity, [
    a owl:Restriction ;
    owl:onProperty ns2:hasValue ;
    owl:allValuesFrom [
      a owl:Restriction ;
      owl:onProperty ns2:hasUnit ;
      owl:allValuesFrom ns2:GasConstantUnit
    ]
  ], [
    a owl:Restriction ;
    owl:onProperty ns2:hasDimension ;
    owl:hasValue ns2:molarEntropyOrMolarHeatCapacityOrGasConstant-Dimension
  ] ;
  ns2:symbol "R" ;
  ns2:commonlyHasUnit ns2:joulePerKelvinMole .

ns2:AmountOfSubstanceFlow
  a owl:Class ;
  rdfs:label "amount of substance flow"@en ;
  ns2:alternativeLabel "amount-of-substance flow"@en, "molar flow"@en ;
  rdfs:subClassOf ns2:Quantity, [
    a owl:Restriction ;
    owl:onProperty ns2:hasValue ;
    owl:allValuesFrom [
      a owl:Restriction ;
      owl:onProperty ns2:hasUnit ;
      owl:allValuesFrom ns2:AmountOfSubstanceFlowUnit
    ]
  ] ;
  ns2:commonlyHasUnit ns2:molePerSecond-Time, ns2:micromolePerSecond-Time .

ns2:Molality
  a owl:Class ;
  rdfs:label "molality"@en, "molaliteit"@nl ;
  ns2:alternativeLabel "molality of solution"@en ;
  rdfs:comment "Molality is the number of moles of solute per kilogram of solvent."@en ;
  rdfs:subClassOf ns2:Quantity, [
    a owl:Restriction ;
    owl:onProperty ns2:hasValue ;
    owl:allValuesFrom [
      a owl:Restriction ;
      owl:onProperty ns2:hasUnit ;
      owl:allValuesFrom ns2:MolalityUnit
    ]
  ] ;
  ns2:symbol "b" ;
  ns2:alternativeSymbol "m" ;
  ns2:commonlyHasUnit ns2:molePerKilogram .

ns2:MolarMass
  a owl:Class ;
  rdfs:label "molar mass"@en, "molaire massa"@nl ;
  rdfs:subClassOf ns2:Quantity, [
    a owl:Restriction ;
    owl:onProperty ns2:hasValue ;
    owl:allValuesFrom [
      a owl:Restriction ;
      owl:onProperty ns2:hasUnit ;
      owl:allValuesFrom ns2:MolarMassUnit
    ]
  ] ;
  ns2:symbol "M" ;
  ns2:commonlyHasUnit ns2:kilogramPerMole .

ns2:MolarVolume
  a owl:Class ;
  rdfs:label "molar volume"@en, "molair volume"@nl ;
  rdfs:subClassOf ns2:Quantity, [
    a owl:Restriction ;
    owl:onProperty ns2:hasValue ;
    owl:allValuesFrom [
      a owl:Restriction ;
      owl:onProperty ns2:hasUnit ;
      owl:allValuesFrom ns2:MolarVolumeUnit
    ]
  ] ;
  ns2:symbol "V_m" ;
  ns2:commonlyHasUnit ns2:cubicMetrePerMole, ns2:litrePerMole .

ns2:AmountOfSubstanceFractionFlow
  a owl:Class ;
  rdfs:label "amount of substance fraction flow"@en ;
  ns2:alternativeLabel "amount-of-substance fraction flow"@en, "mole fraction flow"@en ;
  rdfs:subClassOf ns2:Quantity .

ns2:mole
  a ns2:Unit, ns2:SingularUnit ;
  rdfs:label "mole"@en, "mol"@nl ;
  ns2:symbol "mol" ;
  ns2:hasDimension ns2:amountOfSubstance-Dimension ;
  rdfs:comment "The mole is a unit of amount of substance defined as the amount of substance of a system that contains as many elementary entities as there are atoms in 0.012 kilogram of carbon 12."@en ;
  ns2:longcomment "The mole is a unit of amount of substance defined as the amount of substance of a system that contains as many elementary entities as there are atoms in 0.012 kilogram of carbon 12. The mole is a base unit in the International System of Units." ;
  ns2:hasQuantity ns2:amountOfSubstanceOfASystemThatContainsAsManyElementaryEntitiesAsThereAreAtomsIn0.012KilogramOfCarbon12 .

ns2:systemThatContainsAsManyElementaryEntitiesAsThereAreAtomsIn0.012KilogramOfCarbon12
  a owl:Thing ;
  rdfs:label "system that contains as many elementary entities as there are atoms in 0.012 kilogram of carbon 122"@en .

ns2:amountOfSubstanceOfASystemThatContainsAsManyElementaryEntitiesAsThereAreAtomsIn0.012KilogramOfCarbon12
  a ns2:AmountOfSubstance ;
  rdfs:label "amount of substance of a system that contains as many elementary entities as there are atoms in 0.012 kilogram of carbon 12"@en ;
  ns2:hasPhenomenon ns2:systemThatContainsAsManyElementaryEntitiesAsThereAreAtomsIn0.012KilogramOfCarbon12 .

ns2:AmountOfSubstanceUnit
  a owl:Class ;
  rdfs:label "amount of substance unit"@en ;
  rdfs:subClassOf ns2:Unit ;
  owl:equivalentClass [
    a owl:Class ;
    owl:unionOf (
     _:genid1463
     ns2:PrefixedMole
   )
  ] .

ns2:PrefixedMole
  a owl:Class ;
  rdfs:label "prefixed mole"@en ;
  rdfs:subClassOf ns2:PrefixedUnit ;
  owl:equivalentClass [
    a owl:Class ;
    owl:intersectionOf (
     _:genid1470
     _:genid1472
     _:genid1474
     _:genid1476
   )
  ] .

ns2:yoctomole
  a ns2:PrefixedUnit ;
  rdfs:label "yoctomole"@en, "yoctomol"@nl ;
  ns2:symbol "ymol" ;
  ns2:hasPrefix ns2:yocto ;
  ns2:hasUnit ns2:mole ;
  ns2:hasDimension ns2:amountOfSubstance-Dimension .

ns2:zeptomole
  a ns2:PrefixedUnit ;
  rdfs:label "zeptomole"@en, "zeptomol"@nl ;
  ns2:symbol "zmol" ;
  ns2:hasPrefix ns2:zepto ;
  ns2:hasUnit ns2:mole ;
  ns2:hasDimension ns2:amountOfSubstance-Dimension .

ns2:attomole
  a ns2:PrefixedUnit ;
  rdfs:label "attomole"@en, "attomol"@nl ;
  ns2:symbol "amol" ;
  ns2:hasPrefix ns2:atto ;
  ns2:hasUnit ns2:mole ;
  ns2:hasDimension ns2:amountOfSubstance-Dimension .

ns2:femtomole
  a ns2:PrefixedUnit ;
  rdfs:label "femtomole"@en, "femtomol"@nl ;
  ns2:symbol "fmol" ;
  ns2:hasPrefix ns2:femto ;
  ns2:hasUnit ns2:mole ;
  ns2:hasDimension ns2:amountOfSubstance-Dimension .

ns2:picomole
  a ns2:PrefixedUnit ;
  rdfs:label "picomole"@en, "picomol"@nl ;
  ns2:symbol "pmol" ;
  ns2:hasPrefix ns2:pico ;
  ns2:hasUnit ns2:mole ;
  ns2:hasDimension ns2:amountOfSubstance-Dimension .

ns2:nanomole
  a ns2:PrefixedUnit ;
  rdfs:label "nanomole"@en, "nanomol"@nl ;
  ns2:symbol "nmol" ;
  ns2:hasPrefix ns2:nano ;
  ns2:hasUnit ns2:mole ;
  ns2:hasDimension ns2:amountOfSubstance-Dimension .

ns2:micromole
  a ns2:PrefixedUnit ;
  rdfs:label "micromole"@en, "micromol"@nl ;
  ns2:symbol "μmol" ;
  ns2:hasPrefix ns2:micro ;
  ns2:hasUnit ns2:mole ;
  ns2:hasDimension ns2:amountOfSubstance-Dimension .

ns2:millimole
  a ns2:PrefixedUnit ;
  rdfs:label "millimole"@en, "millimol"@nl ;
  ns2:symbol "mmol" ;
  ns2:hasPrefix ns2:milli ;
  ns2:hasUnit ns2:mole ;
  ns2:hasDimension ns2:amountOfSubstance-Dimension .

ns2:centimole
  a ns2:PrefixedUnit ;
  rdfs:label "centimole"@en, "centimol"@nl ;
  ns2:symbol "cmol" ;
  ns2:hasPrefix ns2:centi ;
  ns2:hasUnit ns2:mole ;
  ns2:hasDimension ns2:amountOfSubstance-Dimension .

ns2:decimole
  a ns2:PrefixedUnit ;
  rdfs:label "decimole"@en, "decimol"@nl ;
  ns2:symbol "dmol" ;
  ns2:hasPrefix ns2:deci ;
  ns2:hasUnit ns2:mole ;
  ns2:hasDimension ns2:amountOfSubstance-Dimension .

ns2:decamole
  a ns2:PrefixedUnit ;
  rdfs:label "decamole"@en, "decamol"@nl ;
  ns2:symbol "damol" ;
  ns2:hasPrefix ns2:deca ;
  ns2:hasUnit ns2:mole ;
  ns2:hasDimension ns2:amountOfSubstance-Dimension .

ns2:hectomole
  a ns2:PrefixedUnit ;
  rdfs:label "hectomole"@en, "hectomol"@nl ;
  ns2:symbol "hmol" ;
  ns2:hasPrefix ns2:hecto ;
  ns2:hasUnit ns2:mole ;
  ns2:hasDimension ns2:amountOfSubstance-Dimension .

ns2:kilomole
  a ns2:PrefixedUnit ;
  rdfs:label "kilomole"@en, "kilomol"@nl ;
  ns2:symbol "kmol" ;
  ns2:hasPrefix ns2:kilo ;
  ns2:hasUnit ns2:mole ;
  ns2:hasDimension ns2:amountOfSubstance-Dimension .

ns2:megamole
  a ns2:PrefixedUnit ;
  rdfs:label "megamole"@en, "megamol"@nl ;
  ns2:symbol "Mmol" ;
  ns2:hasPrefix ns2:mega ;
  ns2:hasUnit ns2:mole ;
  ns2:hasDimension ns2:amountOfSubstance-Dimension .

ns2:gigamole
  a ns2:PrefixedUnit ;
  rdfs:label "gigamole"@en, "gigamol"@nl ;
  ns2:symbol "Gmol" ;
  ns2:hasPrefix ns2:giga ;
  ns2:hasUnit ns2:mole ;
  ns2:hasDimension ns2:amountOfSubstance-Dimension .

ns2:teramole
  a ns2:PrefixedUnit ;
  rdfs:label "teramole"@en, "teramol"@nl ;
  ns2:symbol "Tmol" ;
  ns2:hasPrefix ns2:tera ;
  ns2:hasUnit ns2:mole ;
  ns2:hasDimension ns2:amountOfSubstance-Dimension .

ns2:petamole
  a ns2:PrefixedUnit ;
  rdfs:label "petamole"@en, "petamol"@nl ;
  ns2:symbol "Pmol" ;
  ns2:hasPrefix ns2:peta ;
  ns2:hasUnit ns2:mole ;
  ns2:hasDimension ns2:amountOfSubstance-Dimension .

ns2:examole
  a ns2:PrefixedUnit ;
  rdfs:label "examole"@en, "examol"@nl ;
  ns2:symbol "Emol" ;
  ns2:hasPrefix ns2:exa ;
  ns2:hasUnit ns2:mole ;
  ns2:hasDimension ns2:amountOfSubstance-Dimension .

ns2:zettamole
  a ns2:PrefixedUnit ;
  rdfs:label "zettamole"@en, "zettamol"@nl ;
  ns2:symbol "Zmol" ;
  ns2:hasPrefix ns2:zetta ;
  ns2:hasUnit ns2:mole ;
  ns2:hasDimension ns2:amountOfSubstance-Dimension .

ns2:yottamole
  a ns2:PrefixedUnit ;
  rdfs:label "yottamole"@en, "yottamol"@nl ;
  ns2:symbol "Ymol" ;
  ns2:hasPrefix ns2:yotta ;
  ns2:hasUnit ns2:mole ;
  ns2:hasDimension ns2:amountOfSubstance-Dimension .

ns2:molePerCubicmetre
  a ns2:UnitDivision ;
  rdfs:label "mole per cubic metre"@en, "mol per kubieke meter"@nl ;
  rdfs:comment "Mole per cubic metre is a unit of amount of substance concentration defined as mole divided by cubic metre."@en ;
  ns2:longcomment "Mole per cubic metre is a unit of amount of substance concentration defined as mole divided by cubic metre. Mole per cubic metre is a derived unit in the International System of Units." ;
  ns2:symbol "mol/m3" ;
  ns2:alternativeSymbol "mol m-3", "mol·m-3" ;
  ns2:hasNumerator ns2:mole ;
  ns2:hasDenominator ns2:cubicMetre ;
  ns2:hasDimension ns2:amountOfSubstanceConcentration-Dimension .

ns2:AmountOfSubstanceConcentrationUnit
  a owl:Class ;
  rdfs:label "amount of substance concentration unit"@en ;
  rdfs:subClassOf ns2:Unit ;
  owl:equivalentClass [
    a owl:Class ;
    owl:unionOf (
     _:genid1479
     ns2:PrefixedMolar
     ns2:PrefixedMolePerLitre
     ns2:MolePerPrefixedLitre
     ns2:PrefixedMolePerPrefixedLitre
   )
  ] .

ns2:molar
  a ns2:Unit, ns2:SingularUnit ;
  rdfs:label "molar"@en, "molair"@nl ;
  rdfs:comment "Molar is a unit of amount of substance concentration defined as 1 mole per litre."@en ;
  ns2:symbol "M" ;
  ns2:hasUnit ns2:molePerLitre ;
  ns2:hasDimension ns2:amountOfSubstanceConcentration-Dimension .

ns2:molePerLitre
  a ns2:UnitDivision ;
  rdfs:label "mole per litre"@en, "mole per liter"@nl ;
  rdfs:comment "Mole per litre is a unit of amount of substance concentration defined as mole divided by litre."@en ;
  ns2:longcomment "Mole per litre is a unit of amount of substance concentration defined as mole divided by litre. Mole per litre is a derived unit in the International System of Units." ;
  ns2:symbol "mol/l" ;
  ns2:alternativeSymbol "mol l-1", "mol·l-1" ;
  ns2:hasNumerator ns2:mole ;
  ns2:hasDenominator ns2:litre ;
  ns2:hasDimension ns2:amountOfSubstanceConcentration-Dimension .

ns2:PrefixedMolar
  a owl:Class ;
  rdfs:label "prefixed molar"@en ;
  rdfs:subClassOf ns2:PrefixedUnit ;
  owl:equivalentClass [
    a owl:Class ;
    owl:intersectionOf (
     _:genid1518
     _:genid1520
     _:genid1522
     _:genid1524
   )
  ] .

ns2:PrefixedMolePerLitre
  a owl:Class ;
  rdfs:label "prefixed mole per litre"@en ;
  rdfs:subClassOf ns2:UnitDivision ;
  owl:equivalentClass [
    a owl:Class ;
    owl:intersectionOf (
     _:genid1491
     _:genid1493
     _:genid1495
     _:genid1497
   )
  ] .

ns2:MolePerPrefixedLitre
  a owl:Class ;
  rdfs:label "mole per prefixed litre"@en ;
  rdfs:subClassOf ns2:UnitDivision ;
  owl:equivalentClass [
    a owl:Class ;
    owl:intersectionOf (
     _:genid1500
     _:genid1502
     _:genid1504
     _:genid1506
   )
  ] .

ns2:PrefixedMolePerPrefixedLitre
  a owl:Class ;
  rdfs:label "prefixed mole per prefixed litre"@en ;
  rdfs:subClassOf ns2:UnitDivision ;
  owl:equivalentClass [
    a owl:Class ;
    owl:intersectionOf (
     _:genid1509
     _:genid1511
     _:genid1513
     _:genid1515
   )
  ] .

ns2:yoctomolePerLitre
  a ns2:PrefixedMolePerLitre ;
  rdfs:label "yoctomole per litre"@en, "yoctomole per liter"@nl ;
  rdfs:comment "Yoctomole per litre is a unit of amount of substance concentration defined as yoctomole divided by litre."@en ;
  ns2:symbol "ymol/l" ;
  ns2:alternativeSymbol "ymol l-1", "ymol·l-1" ;
  ns2:hasNumerator ns2:yoctomole ;
  ns2:hasDenominator ns2:litre ;
  ns2:hasDimension ns2:amountOfSubstanceConcentration-Dimension .

ns2:zeptomolePerLitre
  a ns2:PrefixedMolePerLitre ;
  rdfs:label "zeptomole per litre"@en, "zeptomole per liter"@nl ;
  rdfs:comment "Zeptomole per litre is a unit of amount of substance concentration defined as zeptomole divided by litre."@en ;
  ns2:symbol "zmol/l" ;
  ns2:alternativeSymbol "zmol l-1", "zmol·l-1" ;
  ns2:hasNumerator ns2:zeptomole ;
  ns2:hasDenominator ns2:litre ;
  ns2:hasDimension ns2:amountOfSubstanceConcentration-Dimension .

ns2:attomolePerLitre
  a ns2:PrefixedMolePerLitre ;
  rdfs:label "attomole per litre"@en, "attomole per liter"@nl ;
  rdfs:comment "Attomole per litre is a unit of amount of substance concentration defined as attomole divided by litre."@en ;
  ns2:symbol "amol/l" ;
  ns2:alternativeSymbol "amol l-1", "amol·l-1" ;
  ns2:hasNumerator ns2:attomole ;
  ns2:hasDenominator ns2:litre ;
  ns2:hasDimension ns2:amountOfSubstanceConcentration-Dimension .

ns2:femtomolePerLitre
  a ns2:PrefixedMolePerLitre ;
  rdfs:label "femtomole per litre"@en, "femtomole per liter"@nl ;
  rdfs:comment "Femtomole per litre is a unit of amount of substance concentration defined as femtomole divided by litre."@en ;
  ns2:symbol "fmol/l" ;
  ns2:alternativeSymbol "fm s-1", "fm·s-1" ;
  ns2:hasNumerator ns2:femtomole ;
  ns2:hasDenominator ns2:litre ;
  ns2:hasDimension ns2:amountOfSubstanceConcentration-Dimension .

ns2:picomolePerLitre
  a ns2:PrefixedMolePerLitre ;
  rdfs:label "picomole per litre"@en, "picomole per liter"@nl ;
  rdfs:comment "Picomole per litre is a unit of amount of substance concentration defined as picomole divided by litre."@en ;
  ns2:symbol "pmol/l" ;
  ns2:alternativeSymbol "pmol l-1", "pmol·l-1" ;
  ns2:hasNumerator ns2:picomole ;
  ns2:hasDenominator ns2:litre ;
  ns2:hasDimension ns2:amountOfSubstanceConcentration-Dimension .

ns2:nanomolePerLitre
  a ns2:PrefixedMolePerLitre ;
  rdfs:label "nanomole per litre"@en, "nanomole per liter"@nl ;
  rdfs:comment "Nanomole per litre is a unit of amount of substance concentration defined as nanomole divided by litre."@en ;
  ns2:symbol "nmol/l" ;
  ns2:alternativeSymbol "nmol l-1", "nmol·l-1" ;
  ns2:hasNumerator ns2:nanomole ;
  ns2:hasDenominator ns2:litre ;
  ns2:hasDimension ns2:amountOfSubstanceConcentration-Dimension .

ns2:micromolePerLitre
  a ns2:PrefixedMolePerLitre ;
  rdfs:label "micromole per litre"@en, "micromole per liter"@nl ;
  rdfs:comment "Micromole per litre is a unit of amount of substance concentration defined as micromole divided by litre."@en ;
  ns2:symbol "μmol/l" ;
  ns2:alternativeSymbol "μmol l-1", "μmol·l-1" ;
  ns2:hasNumerator ns2:micromole ;
  ns2:hasDenominator ns2:litre ;
  ns2:hasDimension ns2:amountOfSubstanceConcentration-Dimension .

ns2:millimolePerLitre
  a ns2:PrefixedMolePerLitre ;
  rdfs:label "millimole per litre"@en, "millimole per liter"@nl ;
  rdfs:comment "Millimole per litre is a unit of amount of substance concentration defined as millimole divided by litre."@en ;
  ns2:symbol "mmol/l" ;
  ns2:alternativeSymbol "mmol l-1", "mmol·l-1" ;
  ns2:hasNumerator ns2:millimole ;
  ns2:hasDenominator ns2:litre ;
  ns2:hasDimension ns2:amountOfSubstanceConcentration-Dimension .

ns2:centimolePerLitre
  a ns2:PrefixedMolePerLitre ;
  rdfs:label "centimole per litre"@en, "centimole per liter"@nl ;
  rdfs:comment "Centimole per litre is a unit of amount of substance concentration defined as centimole divided by litre."@en ;
  ns2:symbol "cmol/l" ;
  ns2:alternativeSymbol "cmol l-1", "cmol·l-1" ;
  ns2:hasNumerator ns2:centimole ;
  ns2:hasDenominator ns2:litre ;
  ns2:hasDimension ns2:amountOfSubstanceConcentration-Dimension .

ns2:decimolePerLitre
  a ns2:PrefixedMolePerLitre ;
  rdfs:label "decimole per litre"@en, "decimole per liter"@nl ;
  rdfs:comment "Decimole per litre is a unit of amount of substance concentration defined as decimole divided by litre."@en ;
  ns2:symbol "dmol/l" ;
  ns2:alternativeSymbol "dmol l-1", "dmol·l-1" ;
  ns2:hasNumerator ns2:decimole ;
  ns2:hasDenominator ns2:litre ;
  ns2:hasDimension ns2:amountOfSubstanceConcentration-Dimension .

ns2:decamolePerLitre
  a ns2:PrefixedMolePerLitre ;
  rdfs:label "decamole per litre"@en, "decamole per liter"@nl ;
  rdfs:comment "Decamole per litre is a unit of amount of substance concentration defined as decamole divided by litre."@en ;
  ns2:symbol "damol/l" ;
  ns2:alternativeSymbol "damol l-1", "damol·l-1" ;
  ns2:hasNumerator ns2:decamole ;
  ns2:hasDenominator ns2:litre ;
  ns2:hasDimension ns2:amountOfSubstanceConcentration-Dimension .

ns2:hectomolePerLitre
  a ns2:PrefixedMolePerLitre ;
  rdfs:label "hectomole per litre"@en, "hectomole per liter"@nl ;
  rdfs:comment "Hectomole per litre is a unit of amount of substance concentration defined as hectomole divided by litre."@en ;
  ns2:symbol "hmol/l" ;
  ns2:alternativeSymbol "hmol l-1", "hmol·l-1" ;
  ns2:hasNumerator ns2:hectomole ;
  ns2:hasDenominator ns2:litre ;
  ns2:hasDimension ns2:amountOfSubstanceConcentration-Dimension .

ns2:kilomolePerLitre
  a ns2:PrefixedMolePerLitre ;
  rdfs:label "kilomole per litre"@en, "kilomole per liter"@nl ;
  rdfs:comment "Kilomole per litre is a unit of amount of substance concentration defined as kilomole divided by litre."@en ;
  ns2:symbol "kmol/l" ;
  ns2:alternativeSymbol "kmol l-1", "kmol·l-1" ;
  ns2:hasNumerator ns2:kilomole ;
  ns2:hasDenominator ns2:litre ;
  ns2:hasDimension ns2:amountOfSubstanceConcentration-Dimension .

ns2:megamolePerLitre
  a ns2:PrefixedMolePerLitre ;
  rdfs:label "megamole per litre"@en, "megamole per liter"@nl ;
  rdfs:comment "Megamole per litre is a unit of amount of substance concentration defined as megamole divided by litre."@en ;
  ns2:symbol "Mmol/l" ;
  ns2:alternativeSymbol "Mmol l-1", "Mmol·l-1" ;
  ns2:hasNumerator ns2:megamole ;
  ns2:hasDenominator ns2:litre ;
  ns2:hasDimension ns2:amountOfSubstanceConcentration-Dimension .

ns2:gigamolePerLitre
  a ns2:PrefixedMolePerLitre ;
  rdfs:label "gigamole per litre"@en, "gigamole per liter"@nl ;
  rdfs:comment "Gigamole per litre is a unit of amount of substance concentration defined as gigamole divided by litre."@en ;
  ns2:symbol "Gmol/l" ;
  ns2:alternativeSymbol "Gmol l-1", "Gmol·l-1" ;
  ns2:hasNumerator ns2:gigamole ;
  ns2:hasDenominator ns2:litre ;
  ns2:hasDimension ns2:amountOfSubstanceConcentration-Dimension .

ns2:teramolePerLitre
  a ns2:PrefixedMolePerLitre ;
  rdfs:label "teramole per litre"@en, "teramole per liter"@nl ;
  rdfs:comment "Teramole per litre is a unit of amount of substance concentration defined as teramole divided by litre."@en ;
  ns2:symbol "Tmol/l" ;
  ns2:alternativeSymbol "Tmol l-1", "Tmol·l-1" ;
  ns2:hasNumerator ns2:teramole ;
  ns2:hasDenominator ns2:litre ;
  ns2:hasDimension ns2:amountOfSubstanceConcentration-Dimension .

ns2:petamolePerLitre
  a ns2:PrefixedMolePerLitre ;
  rdfs:label "petamole per litre"@en, "petamole per liter"@nl ;
  rdfs:comment "Petamole per litre is a unit of amount of substance concentration defined as petamole divided by litre."@en ;
  ns2:symbol "Pmol/l" ;
  ns2:alternativeSymbol "Pmol l-1", "Pmol·l-1" ;
  ns2:hasNumerator ns2:petamole ;
  ns2:hasDenominator ns2:litre ;
  ns2:hasDimension ns2:amountOfSubstanceConcentration-Dimension .

ns2:examolePerLitre
  a ns2:PrefixedMolePerLitre ;
  rdfs:label "examole per litre"@en, "examole per liter"@nl ;
  rdfs:comment "Examole per litre is a unit of amount of substance concentration defined as examole divided by litre."@en ;
  ns2:symbol "Emol/l" ;
  ns2:alternativeSymbol "Emol l-1", "Emol·l-1" ;
  ns2:hasNumerator ns2:examole ;
  ns2:hasDenominator ns2:litre ;
  ns2:hasDimension ns2:amountOfSubstanceConcentration-Dimension .

ns2:zettamolePerLitre
  a ns2:PrefixedMolePerLitre ;
  rdfs:label "zettamole per litre"@en, "zettamole per liter"@nl ;
  rdfs:comment "Zettamole per litre is a unit of amount of substance concentration defined as zettamole divided by litre."@en ;
  ns2:symbol "Zmol/l" ;
  ns2:alternativeSymbol "Zmol l-1", "Zmol·l-1" ;
  ns2:hasNumerator ns2:zettamole ;
  ns2:hasDenominator ns2:litre ;
  ns2:hasDimension ns2:amountOfSubstanceConcentration-Dimension .

ns2:yottamolePerLitre
  a ns2:PrefixedMolePerLitre ;
  rdfs:label "yottamole per litre"@en, "yottamole per liter"@nl ;
  rdfs:comment "Yottamole per litre is a unit of amount of substance concentration defined as yottamole divided by litre."@en ;
  ns2:symbol "Ymol/l" ;
  ns2:alternativeSymbol "Ymol l-1", "Ymol·l-1" ;
  ns2:hasNumerator ns2:yottamole ;
  ns2:hasDenominator ns2:litre ;
  ns2:hasDimension ns2:amountOfSubstanceConcentration-Dimension .

ns2:molePerYoctolitre
  a ns2:MolePerPrefixedLitre ;
  rdfs:label "mole per yoctolitre"@en, "mole per yoctoliter"@nl ;
  rdfs:comment "Mole per yoctolitre is a unit of amount of substance concentration defined as mole divided by yoctolitre."@en ;
  ns2:symbol "mol/yl" ;
  ns2:alternativeSymbol "mol yl-1", "mol·yl-1" ;
  ns2:hasNumerator ns2:mole ;
  ns2:hasDenominator ns2:yoctolitre ;
  ns2:hasDimension ns2:amountOfSubstanceConcentration-Dimension .

ns2:molePerZeptolitre
  a ns2:MolePerPrefixedLitre ;
  rdfs:label "mole per zeptolitre"@en, "mole per zeptoliter"@nl ;
  rdfs:comment "Mole per zeptolitre is a unit of amount of substance concentration defined as mole divided by zeptolitre."@en ;
  ns2:symbol "mol/zl" ;
  ns2:alternativeSymbol "mol zl-1", "mol·zl-1" ;
  ns2:hasNumerator ns2:mole ;
  ns2:hasDenominator ns2:zeptolitre ;
  ns2:hasDimension ns2:amountOfSubstanceConcentration-Dimension .

ns2:molePerAttolitre
  a ns2:MolePerPrefixedLitre ;
  rdfs:label "mole per attolitre"@en, "mole per attoliter"@nl ;
  rdfs:comment "Mole per attolitre is a unit of amount of substance concentration defined as mole divided by attolitre."@en ;
  ns2:symbol "mol/al" ;
  ns2:alternativeSymbol "mol al-1", "mol·al-1" ;
  ns2:hasNumerator ns2:mole ;
  ns2:hasDenominator ns2:attolitre ;
  ns2:hasDimension ns2:amountOfSubstanceConcentration-Dimension .

ns2:molePerFemtolitre
  a ns2:MolePerPrefixedLitre ;
  rdfs:label "mole per femtolitre"@en, "mole per femtoliter"@nl ;
  rdfs:comment "Mole per femtolitre is a unit of amount of substance concentration defined as mole divided by femtolitre."@en ;
  ns2:symbol "mol/fl" ;
  ns2:alternativeSymbol "mol fl-1", "mol·fl-1" ;
  ns2:hasNumerator ns2:mole ;
  ns2:hasDenominator ns2:femtolitre ;
  ns2:hasDimension ns2:amountOfSubstanceConcentration-Dimension .

ns2:molePerPicolitre
  a ns2:MolePerPrefixedLitre ;
  rdfs:label "mole per picolitre"@en, "mole per picoliter"@nl ;
  rdfs:comment "Mole per picolitre is a unit of amount of substance concentration defined as mole divided by picolitre."@en ;
  ns2:symbol "mol/pl" ;
  ns2:alternativeSymbol "mol pl-1", "mol·pl-1" ;
  ns2:hasNumerator ns2:mole ;
  ns2:hasDenominator ns2:picolitre ;
  ns2:hasDimension ns2:amountOfSubstanceConcentration-Dimension .

ns2:molePerNanolitre
  a ns2:MolePerPrefixedLitre ;
  rdfs:label "mole per nanolitre"@en, "mole per nanoliter"@nl ;
  rdfs:comment "Mole per nanolitre is a unit of amount of substance concentration defined as mole divided by nanolitre."@en ;
  ns2:symbol "mol/nl" ;
  ns2:alternativeSymbol "mol nl-1", "mol·nl-1" ;
  ns2:hasNumerator ns2:mole ;
  ns2:hasDenominator ns2:nanolitre ;
  ns2:hasDimension ns2:amountOfSubstanceConcentration-Dimension .

ns2:molePerMicrolitre
  a ns2:MolePerPrefixedLitre ;
  rdfs:label "mole per microlitre"@en, "mole per microliter"@nl ;
  rdfs:comment "Mole per microlitre is a unit of amount of substance concentration defined as mole divided by microlitre."@en ;
  ns2:symbol "mol/μl" ;
  ns2:alternativeSymbol "mol μl-1", "mol·μl-1" ;
  ns2:hasNumerator ns2:mole ;
  ns2:hasDenominator ns2:microlitre ;
  ns2:hasDimension ns2:amountOfSubstanceConcentration-Dimension .

ns2:molePerMillilitre
  a ns2:MolePerPrefixedLitre ;
  rdfs:label "mole per millilitre"@en, "mole per milliliter"@nl ;
  rdfs:comment "Mole per millilitre is a unit of amount of substance concentration defined as mole divided by millilitre."@en ;
  ns2:symbol "mol/ml" ;
  ns2:alternativeSymbol "mol ml-1", "mol·ml-1" ;
  ns2:hasNumerator ns2:mole ;
  ns2:hasDenominator ns2:millilitre ;
  ns2:hasDimension ns2:amountOfSubstanceConcentration-Dimension .

ns2:molePerCentilitre
  a ns2:MolePerPrefixedLitre ;
  rdfs:label "mole per centilitre"@en, "mole per centiliter"@nl ;
  rdfs:comment "Mole per centilitre is a unit of amount of substance concentration defined as mole divided by centilitre."@en ;
  ns2:symbol "mol/cl" ;
  ns2:alternativeSymbol "mol cl-1", "mol·cl-1" ;
  ns2:hasNumerator ns2:mole ;
  ns2:hasDenominator ns2:centilitre ;
  ns2:hasDimension ns2:amountOfSubstanceConcentration-Dimension .

ns2:molePerDecilitre
  a ns2:MolePerPrefixedLitre ;
  rdfs:label "mole per decilitre"@en, "mole per deciliter"@nl ;
  rdfs:comment "Mole per decilitre is a unit of amount of substance concentration defined as mole divided by decilitre."@en ;
  ns2:symbol "mol/dl" ;
  ns2:alternativeSymbol "mol dl-1", "mol·dl-1" ;
  ns2:hasNumerator ns2:mole ;
  ns2:hasDenominator ns2:decilitre ;
  ns2:hasDimension ns2:amountOfSubstanceConcentration-Dimension .

ns2:molePerDecalitre
  a ns2:MolePerPrefixedLitre ;
  rdfs:label "mole per decalitre"@en, "mole per decaliter"@nl ;
  rdfs:comment "Mole per decalitre is a unit of amount of substance concentration defined as mole divided by decalitre."@en ;
  ns2:symbol "mol/dal" ;
  ns2:alternativeSymbol "mol dal-1", "mol·dal-1" ;
  ns2:hasNumerator ns2:mole ;
  ns2:hasDenominator ns2:decalitre ;
  ns2:hasDimension ns2:amountOfSubstanceConcentration-Dimension .

ns2:molePerHectolitre
  a ns2:MolePerPrefixedLitre ;
  rdfs:label "mole per hectolitre"@en, "mole per hectoliter"@nl ;
  rdfs:comment "Mole per hectolitre is a unit of amount of substance concentration defined as mole divided by hectolitre."@en ;
  ns2:symbol "mol/hl" ;
  ns2:alternativeSymbol "mol hl-1", "mol·hl-1" ;
  ns2:hasNumerator ns2:mole ;
  ns2:hasDenominator ns2:hectolitre ;
  ns2:hasDimension ns2:amountOfSubstanceConcentration-Dimension .

ns2:molePerKilolitre
  a ns2:MolePerPrefixedLitre ;
  rdfs:label "mole per kilolitre"@en, "mole per kiloliter"@nl ;
  rdfs:comment "Mole per kilolitre is a unit of amount of substance concentration defined as mole divided by kilolitre."@en ;
  ns2:symbol "mol/kl" ;
  ns2:alternativeSymbol "mol kl-1", "mol·kl-1" ;
  ns2:hasNumerator ns2:mole ;
  ns2:hasDenominator ns2:kilolitre ;
  ns2:hasDimension ns2:amountOfSubstanceConcentration-Dimension .

ns2:molePerMegalitre
  a ns2:MolePerPrefixedLitre ;
  rdfs:label "mole per megalitre"@en, "mole per megaliter"@nl ;
  rdfs:comment "Mole per megalitre is a unit of amount of substance concentration defined as mole divided by megalitre."@en ;
  ns2:symbol "mol/Ml" ;
  ns2:alternativeSymbol "mol Ml-1", "mol·Ml-1" ;
  ns2:hasNumerator ns2:mole ;
  ns2:hasDenominator ns2:megalitre ;
  ns2:hasDimension ns2:amountOfSubstanceConcentration-Dimension .

ns2:molePerGigalitre
  a ns2:MolePerPrefixedLitre ;
  rdfs:label "mole per gigalitre"@en, "mole per gigaliter"@nl ;
  rdfs:comment "Mole per gigalitre is a unit of amount of substance concentration defined as mole divided by gigalitre."@en ;
  ns2:symbol "mol/Gl" ;
  ns2:alternativeSymbol "mol Gl-1", "mol·Gl-1" ;
  ns2:hasNumerator ns2:mole ;
  ns2:hasDenominator ns2:gigalitre ;
  ns2:hasDimension ns2:amountOfSubstanceConcentration-Dimension .

ns2:molePerTeralitre
  a ns2:MolePerPrefixedLitre ;
  rdfs:label "mole per teralitre"@en, "mole per teraliter"@nl ;
  rdfs:comment "Mole per teralitre is a unit of amount of substance concentration defined as mole divided by teralitre."@en ;
  ns2:symbol "mol/Tl" ;
  ns2:alternativeSymbol "mol Tl-1", "mol·Tl-1" ;
  ns2:hasNumerator ns2:mole ;
  ns2:hasDenominator ns2:teralitre ;
  ns2:hasDimension ns2:amountOfSubstanceConcentration-Dimension .

ns2:molePerPetalitre
  a ns2:MolePerPrefixedLitre ;
  rdfs:label "mole per petalitre"@en, "mole per petaliter"@nl ;
  rdfs:comment "Mole per petalitre is a unit of amount of substance concentration defined as mole divided by petalitre."@en ;
  ns2:symbol "mol/Pl" ;
  ns2:alternativeSymbol "mol Pl-1", "mol·Pl-1" ;
  ns2:hasNumerator ns2:mole ;
  ns2:hasDenominator ns2:petalitre ;
  ns2:hasDimension ns2:amountOfSubstanceConcentration-Dimension .

ns2:molePerExalitre
  a ns2:MolePerPrefixedLitre ;
  rdfs:label "mole per exalitre"@en, "mole per exaliter"@nl ;
  rdfs:comment "Mole per exalitre is a unit of amount of substance concentration defined as mole divided by exalitre."@en ;
  ns2:symbol "mol/El" ;
  ns2:alternativeSymbol "mol El-1", "mol·El-1" ;
  ns2:hasNumerator ns2:mole ;
  ns2:hasDenominator ns2:exalitre ;
  ns2:hasDimension ns2:amountOfSubstanceConcentration-Dimension .

ns2:molePerZettalitre
  a ns2:MolePerPrefixedLitre ;
  rdfs:label "mole per zettalitre"@en, "mole per zettaliter"@nl ;
  rdfs:comment "Mole per zettalitre is a unit of amount of substance concentration defined as mole divided by zettalitre."@en ;
  ns2:symbol "mol/Zl" ;
  ns2:alternativeSymbol "mol Zl-1", "mol·Zl-1" ;
  ns2:hasNumerator ns2:mole ;
  ns2:hasDenominator ns2:zettalitre ;
  ns2:hasDimension ns2:amountOfSubstanceConcentration-Dimension .

ns2:molePerYottalitre
  a ns2:MolePerPrefixedLitre ;
  rdfs:label "mole per yottalitre"@en, "mole per yottaliter"@nl ;
  rdfs:comment "Mole per yottalitre is a unit of amount of substance concentration defined as mole divided by yottalitre."@en ;
  ns2:symbol "mol/Yl" ;
  ns2:alternativeSymbol "mol Yl-1", "mol·Yl-1" ;
  ns2:hasNumerator ns2:mole ;
  ns2:hasDenominator ns2:yottalitre ;
  ns2:hasDimension ns2:amountOfSubstanceConcentration-Dimension .

ns2:yoctomolar
  a ns2:PrefixedUnit ;
  rdfs:label "yoctomolar"@en, "yoctomolair"@nl ;
  rdfs:comment "The yoctomolar is a unit of amount of substance concentration defined as 1.0e-24 molar."@en ;
  ns2:symbol "yM" ;
  ns2:hasPrefix ns2:yocto ;
  ns2:hasUnit ns2:molar ;
  ns2:hasDimension ns2:amountOfSubstanceConcentration-Dimension .

ns2:zeptomolar
  a ns2:PrefixedUnit ;
  rdfs:label "zeptomolar"@en, "zeptomolair"@nl ;
  rdfs:comment "The zeptmolar is a unit of amount of substance concentration defined as 1.0e-21 molar."@en ;
  ns2:symbol "zM" ;
  ns2:hasPrefix ns2:zepto ;
  ns2:hasUnit ns2:molar ;
  ns2:hasDimension ns2:amountOfSubstanceConcentration-Dimension .

ns2:attomolar
  a ns2:PrefixedUnit ;
  rdfs:label "attomolar"@en, "attomolair"@nl ;
  rdfs:comment "The attomolar is a unit of amount of substance concentration defined as 1.0e-18 molar."@en ;
  ns2:symbol "aM" ;
  ns2:hasPrefix ns2:atto ;
  ns2:hasUnit ns2:molar ;
  ns2:hasDimension ns2:amountOfSubstanceConcentration-Dimension .

ns2:femtomolar
  a ns2:PrefixedUnit ;
  rdfs:label "femtomolar"@en, "femtomolair"@nl ;
  rdfs:comment "The femtomolar is a unit of amount of substance concentration defined as 1.0e-15 molar."@en ;
  ns2:symbol "fM" ;
  ns2:hasPrefix ns2:femto ;
  ns2:hasUnit ns2:molar ;
  ns2:hasDimension ns2:amountOfSubstanceConcentration-Dimension .

ns2:picomolar
  a ns2:PrefixedUnit ;
  rdfs:label "picomolar"@en, "picomolair"@nl ;
  rdfs:comment "The picomolar is a unit of amount of substance concentration defined as 1.0e-12 molar."@en ;
  ns2:symbol "pM" ;
  ns2:hasPrefix ns2:pico ;
  ns2:hasUnit ns2:molar ;
  ns2:hasDimension ns2:amountOfSubstanceConcentration-Dimension .

ns2:nanomolar
  a ns2:PrefixedUnit ;
  rdfs:label "nanomolar"@en, "nanomolair"@nl ;
  rdfs:comment "The nanomolar is a unit of amount of substance concentration defined as 1.0e-9 molar."@en ;
  ns2:symbol "nM" ;
  ns2:hasPrefix ns2:nano ;
  ns2:hasUnit ns2:molar ;
  ns2:hasDimension ns2:amountOfSubstanceConcentration-Dimension .

ns2:micromolar
  a ns2:PrefixedUnit ;
  rdfs:label "micromolar"@en, "micromolair"@nl ;
  rdfs:comment "The micromolar is a unit of amount of substance concentration defined as 1.0e-6 molar."@en ;
  ns2:symbol "μM" ;
  ns2:hasPrefix ns2:micro ;
  ns2:hasUnit ns2:molar ;
  ns2:hasDimension ns2:amountOfSubstanceConcentration-Dimension .

ns2:millimolar
  a ns2:PrefixedUnit ;
  rdfs:label "millimolar"@en, "millimolair"@nl ;
  rdfs:comment "The millimolar is a unit of amount of substance concentration defined as 1.0e-3 molar."@en ;
  ns2:symbol "mM" ;
  ns2:hasPrefix ns2:milli ;
  ns2:hasUnit ns2:molar ;
  ns2:hasDimension ns2:amountOfSubstanceConcentration-Dimension .

ns2:centimolar
  a ns2:PrefixedUnit ;
  rdfs:label "centimolar"@en, "centimolair"@nl ;
  rdfs:comment "The centimolar is a unit of amount of substance concentration defined as 1.0e-2 molar."@en ;
  ns2:symbol "cM" ;
  ns2:hasPrefix ns2:centi ;
  ns2:hasUnit ns2:molar ;
  ns2:hasDimension ns2:amountOfSubstanceConcentration-Dimension .

ns2:decimolar
  a ns2:PrefixedUnit ;
  rdfs:label "decimolar"@en, "decimolair"@nl ;
  rdfs:comment "The decimolar is a unit of amount of substance concentration defined as 1.0e-1 molar."@en ;
  ns2:symbol "dM" ;
  ns2:hasPrefix ns2:deci ;
  ns2:hasUnit ns2:molar ;
  ns2:hasDimension ns2:amountOfSubstanceConcentration-Dimension .

ns2:decamolar
  a ns2:PrefixedUnit ;
  rdfs:label "decamolar"@en, "decamolair"@nl ;
  rdfs:comment "The decamolar is a unit of amount of substance concentration defined as 1.0e1 molar."@en ;
  ns2:symbol "daM" ;
  ns2:hasPrefix ns2:deca ;
  ns2:hasUnit ns2:molar ;
  ns2:hasDimension ns2:amountOfSubstanceConcentration-Dimension .

ns2:hectomolar
  a ns2:PrefixedUnit ;
  rdfs:label "hectomolar"@en, "hectomolair"@nl ;
  rdfs:comment "The hectomolar is a unit of amount of substance concentration defined as 1.0e2 molar."@en ;
  ns2:symbol "hM" ;
  ns2:hasPrefix ns2:hecto ;
  ns2:hasUnit ns2:molar ;
  ns2:hasDimension ns2:amountOfSubstanceConcentration-Dimension .

ns2:kilomolar
  a ns2:PrefixedUnit ;
  rdfs:label "kilomolar"@en, "kilomolair"@nl ;
  rdfs:comment "The kilomolar is a unit of amount of substance concentration defined as 1.0e3 molar."@en ;
  ns2:symbol "kM" ;
  ns2:hasPrefix ns2:kilo ;
  ns2:hasUnit ns2:molar ;
  ns2:hasDimension ns2:amountOfSubstanceConcentration-Dimension .

ns2:megamolar
  a ns2:PrefixedUnit ;
  rdfs:label "megamolar"@en, "megamolair"@nl ;
  rdfs:comment "The megamolar is a unit of amount of substance concentration defined as 1.0e6 molar."@en ;
  ns2:symbol "MM" ;
  ns2:hasPrefix ns2:mega ;
  ns2:hasUnit ns2:molar ;
  ns2:hasDimension ns2:amountOfSubstanceConcentration-Dimension .

ns2:gigamolar
  a ns2:PrefixedUnit ;
  rdfs:label "gigamolar"@en, "gigamolair"@nl ;
  rdfs:comment "The gigamolar is a unit of amount of substance concentration defined as 1.0e9 molar."@en ;
  ns2:symbol "GM" ;
  ns2:hasPrefix ns2:giga ;
  ns2:hasUnit ns2:molar ;
  ns2:hasDimension ns2:amountOfSubstanceConcentration-Dimension .

ns2:teramolar
  a ns2:PrefixedUnit ;
  rdfs:label "teramolar"@en, "teramolair"@nl ;
  rdfs:comment "The teramolar is a unit of amount of substance concentration defined as 1.0e12 molar."@en ;
  ns2:symbol "TM" ;
  ns2:hasPrefix ns2:tera ;
  ns2:hasUnit ns2:molar ;
  ns2:hasDimension ns2:amountOfSubstanceConcentration-Dimension .

ns2:petamolar
  a ns2:PrefixedUnit ;
  rdfs:label "petamolar"@en, "petamolair"@nl ;
  rdfs:comment "The petamolar is a unit of amount of substance concentration defined as 1.0e15 molar."@en ;
  ns2:symbol "PM" ;
  ns2:hasPrefix ns2:peta ;
  ns2:hasUnit ns2:molar ;
  ns2:hasDimension ns2:amountOfSubstanceConcentration-Dimension .

ns2:examolar
  a ns2:PrefixedUnit ;
  rdfs:label "examolar"@en, "examolair"@nl ;
  rdfs:comment "The examolar is a unit of amount of substance concentration defined as 1.0e18 molar."@en ;
  ns2:symbol "EM" ;
  ns2:hasPrefix ns2:exa ;
  ns2:hasUnit ns2:molar ;
  ns2:hasDimension ns2:amountOfSubstanceConcentration-Dimension .

ns2:zettamolar
  a ns2:PrefixedUnit ;
  rdfs:label "zettamolar"@en, "zettamolair"@nl ;
  rdfs:comment "The zettamolar is a unit of amount of substance concentration defined as 1.0e21 molar."@en ;
  ns2:symbol "ZM" ;
  ns2:hasPrefix ns2:zetta ;
  ns2:hasUnit ns2:molar ;
  ns2:hasDimension ns2:amountOfSubstanceConcentration-Dimension .

ns2:yottamolar
  a ns2:PrefixedUnit ;
  rdfs:label "yottamolar"@en, "yottamolair"@nl ;
  rdfs:comment "The yottamolar is a unit of amount of substance concentration defined as 1.0e24 molar."@en ;
  ns2:symbol "YM" ;
  ns2:hasPrefix ns2:yotta ;
  ns2:hasUnit ns2:molar ;
  ns2:hasDimension ns2:amountOfSubstanceConcentration-Dimension .

ns2:molePerMole
  a ns2:UnitDivision ;
  rdfs:label "mole per mole"@en, "mol per mol"@nl ;
  ns2:symbol "mol/mol" ;
  ns2:alternativeSymbol "mol mol-1", "mol·mol-1" ;
  ns2:hasNumerator ns2:mole ;
  ns2:hasDenominator ns2:mole ;
  ns2:hasDimension ns2:dimensionOne .

ns2:micromolePerMole
  a ns2:UnitDivision ;
  rdfs:label "micromole per mole"@en, "micromol per mol"@nl ;
  ns2:symbol "μmol/mol" ;
  ns2:alternativeSymbol "μmol mol-1", "μmol·mol-1" ;
  ns2:hasNumerator ns2:micromole ;
  ns2:hasDenominator ns2:mole ;
  ns2:hasDimension ns2:dimensionOne .

ns2:AmountOfSubstanceFractionUnit
  a owl:Class ;
  rdfs:label "amount of substance fraction unit"@en ;
  rdfs:subClassOf ns2:Unit ;
  owl:equivalentClass [
    a owl:Class ;
    owl:oneOf (
     ns2:one
     ns2:partsPerMillion
     ns2:percent
     ns2:molePerMole
     ns2:micromolePerMole
   )
  ] .

ns2:joulePerMole
  a ns2:UnitDivision ;
  rdfs:label "joule per mole"@en, "joule per mol"@nl ;
  ns2:symbol "J/mol" ;
  ns2:alternativeSymbol "J mol-1", "J·mol-1" ;
  ns2:hasNumerator ns2:joule ;
  ns2:hasDenominator ns2:mole ;
  ns2:hasDimension ns2:molarEnergy-Dimension .

ns2:MolarEnergyUnit
  a owl:Class ;
  rdfs:label "molar energy unit"@en ;
  rdfs:subClassOf ns2:Unit ;
  owl:equivalentClass [
    a owl:Class ;
    owl:oneOf ( ns2:joulePerMole )
  ] .

ns2:joulePerKelvinMole
  a ns2:UnitDivision ;
  rdfs:label "joule per kelvin mole"@en, "joule per kelvin mol"@nl ;
  ns2:symbol "J/(K mol)" ;
  ns2:alternativeSymbol "J/(K·mol)", "J K-1 mol-1", "J·K-1·mol-1" ;
  ns2:hasNumerator ns2:joule ;
  ns2:hasDenominator ns2:kelvinMole ;
  ns2:hasDimension ns2:molarEntropyOrMolarHeatCapacityOrGasConstant-Dimension .

ns2:MolarEntropyUnit
  a owl:Class ;
  rdfs:label "molar entropy unit"@en ;
  rdfs:subClassOf ns2:Unit ;
  owl:equivalentClass [
    a owl:Class ;
    owl:oneOf ( ns2:joulePerKelvinMole )
  ] .

ns2:MolarHeatCapacityUnit
  a owl:Class ;
  rdfs:label "molar heat capacity unit"@en ;
  rdfs:subClassOf ns2:Unit ;
  owl:equivalentClass [
    a owl:Class ;
    owl:oneOf ( ns2:joulePerKelvinMole )
  ] .

ns2:GasConstantUnit
  a owl:Class ;
  rdfs:label "gas constant unit"@en ;
  rdfs:subClassOf ns2:Unit ;
  owl:equivalentClass [
    a owl:Class ;
    owl:oneOf ( ns2:joulePerKelvinMole )
  ] .

ns2:molePerKilogram
  a ns2:UnitDivision ;
  rdfs:label "mole per kilogram"@en, "mol per kilogram"@nl ;
  ns2:symbol "mol/kg" ;
  ns2:alternativeSymbol "mol kg-1", "mol·kg-1" ;
  ns2:hasNumerator ns2:mole ;
  ns2:hasDenominator ns2:kilogram .

ns2:MolalityUnit
  a owl:Class ;
  rdfs:label "molality unit"@en ;
  rdfs:subClassOf ns2:Unit ;
  owl:equivalentClass [
    a owl:Class ;
    owl:oneOf ( ns2:molePerKilogram )
  ] .

ns2:kilogramPerMole
  a ns2:UnitDivision ;
  rdfs:label "kilogram per mole"@en, "kilogram per mol"@nl ;
  ns2:symbol "kg/mol" ;
  ns2:alternativeSymbol "kg mol-1", "kg·mol-1" ;
  ns2:hasNumerator ns2:kilogram ;
  ns2:hasDenominator ns2:mole .

ns2:MolarMassUnit
  a owl:Class ;
  rdfs:label "molar mass unit"@en ;
  rdfs:subClassOf ns2:Unit ;
  owl:equivalentClass [
    a owl:Class ;
    owl:oneOf ( ns2:kilogramPerMole )
  ] .

ns2:cubicMetrePerMole
  a ns2:UnitDivision ;
  rdfs:label "cubic metre per mole"@en, "kubieke meter per mol"@nl ;
  ns2:symbol "m3/mol" ;
  ns2:alternativeSymbol "m3 mol-1", "m3·mol-1" ;
  ns2:hasNumerator ns2:cubicMetre ;
  ns2:hasDenominator ns2:mole .

ns2:MolarVolumeUnit
  a owl:Class ;
  rdfs:label "molar volume unit"@en ;
  rdfs:subClassOf ns2:Unit ;
  owl:equivalentClass [
    a owl:Class ;
    owl:oneOf (
     ns2:cubicMetrePerMole
     ns2:litrePerMole
   )
  ] .

ns2:litrePerMole
  a ns2:UnitDivision ;
  rdfs:label "litre per mole"@en, "liter per mol"@nl ;
  ns2:symbol "l/mol" ;
  ns2:alternativeSymbol "l mol-1", "l·mol-1" ;
  ns2:hasNumerator ns2:litre ;
  ns2:hasDenominator ns2:mole .

ns2:moleMicrometre
  a ns2:UnitMultiplication ;
  rdfs:label "mole micrometre"@en, "mol micrometer"@nl ;
  ns2:symbol "mol μm" ;
  ns2:alternativeSymbol "mol·μm" ;
  ns2:hasTerm1 ns2:mole ;
  ns2:hasTerm2 ns2:micrometre .

ns2:moleMicrometreReciprocalSquareCentimetre
  a ns2:UnitMultiplication ;
  rdfs:label "mole micrometre reciprocal square centimetre"@en, "mol micrometer omgekeerde vierkante centimeter"@nl ;
  ns2:symbol "mol μm cm-2" ;
  ns2:alternativeSymbol "mol·μm·cm-2" ;
  ns2:hasTerm1 ns2:moleMicrometre ;
  ns2:hasTerm2 ns2:reciprocalSquareCentimetre .

ns2:moleMicrometreReciprocalSquareCentimetreReciprocalSecond-Time
  a ns2:UnitMultiplication ;
  rdfs:label "mole micrometre reciprocal square centimetre reciprocal second"@en, "mol micrometer omgekeerde vierkante centimeter omgekeerde seconde"@nl ;
  ns2:symbol "mol μm cm-2 s-1" ;
  ns2:alternativeSymbol "mol·μm·cm-2·s-1" ;
  ns2:hasTerm1 ns2:moleMicrometreReciprocalSquareCentimetre ;
  ns2:hasTerm2 ns2:reciprocalSecond-Time .

ns2:molePerMetre
  a ns2:UnitDivision ;
  rdfs:label "mole per metre"@en, "mole per meter"@nl ;
  ns2:symbol "mol/m" ;
  ns2:alternativeSymbol "mol m-1", "mol·m-1" ;
  ns2:hasNumerator ns2:mole ;
  ns2:hasDenominator ns2:metre .

ns2:yoctomolePerMetre
  a ns2:PrefixedMolePerMetre ;
  rdfs:label "yoctomole per metre"@en, "yoctomole per meter"@nl ;
  ns2:symbol "ymol/m" ;
  ns2:alternativeSymbol "ymol m-1", "ymol·m-1" ;
  ns2:hasNumerator ns2:yoctomole ;
  ns2:hasDenominator ns2:metre .

ns2:zeptomolePerMetre
  a ns2:PrefixedMolePerMetre ;
  rdfs:label "zeptomole per metre"@en, "zeptomole per meter"@nl ;
  ns2:symbol "zmol/m" ;
  ns2:alternativeSymbol "zmol m-1", "zmol·m-1" ;
  ns2:hasNumerator ns2:zeptomole ;
  ns2:hasDenominator ns2:metre .

ns2:attomolePerMetre
  a ns2:PrefixedMolePerMetre ;
  rdfs:label "attomole per metre"@en, "attomole per meter"@nl ;
  ns2:symbol "amol/m" ;
  ns2:alternativeSymbol "amol m-1", "amol·m-1" ;
  ns2:hasNumerator ns2:attomole ;
  ns2:hasDenominator ns2:metre .

ns2:femtomolePerMetre
  a ns2:PrefixedMolePerMetre ;
  rdfs:label "femtomole per metre"@en, "femtomole per meter"@nl ;
  ns2:symbol "fmol/m" ;
  ns2:alternativeSymbol "fm s-1", "fm·s-1" ;
  ns2:hasNumerator ns2:femtomole ;
  ns2:hasDenominator ns2:metre .

ns2:picomolePerMetre
  a ns2:PrefixedMolePerMetre ;
  rdfs:label "picomole per metre"@en, "picomole per meter"@nl ;
  ns2:symbol "pmol/m" ;
  ns2:alternativeSymbol "pmol m-1", "pmol·m-1" ;
  ns2:hasNumerator ns2:picomole ;
  ns2:hasDenominator ns2:metre .

ns2:nanomolePerMetre
  a ns2:PrefixedMolePerMetre ;
  rdfs:label "nanomole per metre"@en, "nanomole per meter"@nl ;
  ns2:symbol "nmol/m" ;
  ns2:alternativeSymbol "nmol m-1", "nmol·m-1" ;
  ns2:hasNumerator ns2:nanomole ;
  ns2:hasDenominator ns2:metre .

ns2:micromolePerMetre
  a ns2:PrefixedMolePerMetre ;
  rdfs:label "micromole per metre"@en, "micromole per meter"@nl ;
  ns2:symbol "μmol/m" ;
  ns2:alternativeSymbol "μmol m-1", "μmol·m-1" ;
  ns2:hasNumerator ns2:micromole ;
  ns2:hasDenominator ns2:metre .

ns2:millimolePerMetre
  a ns2:PrefixedMolePerMetre ;
  rdfs:label "millimole per metre"@en, "millimole per meter"@nl ;
  ns2:symbol "mmol/m" ;
  ns2:alternativeSymbol "mmol m-1", "mmol·m-1" ;
  ns2:hasNumerator ns2:millimole ;
  ns2:hasDenominator ns2:metre .

ns2:centimolePerMetre
  a ns2:PrefixedMolePerMetre ;
  rdfs:label "centimole per metre"@en, "centimole per meter"@nl ;
  ns2:symbol "cmol/m" ;
  ns2:alternativeSymbol "cmol m-1", "cmol·m-1" ;
  ns2:hasNumerator ns2:centimole ;
  ns2:hasDenominator ns2:metre .

ns2:decimolePerMetre
  a ns2:PrefixedMolePerMetre ;
  rdfs:label "decimole per metre"@en, "decimole per meter"@nl ;
  ns2:symbol "dmol/m" ;
  ns2:alternativeSymbol "dmol m-1", "dmol·m-1" ;
  ns2:hasNumerator ns2:decimole ;
  ns2:hasDenominator ns2:metre .

ns2:decamolePerMetre
  a ns2:PrefixedMolePerMetre ;
  rdfs:label "decamole per metre"@en, "decamole per meter"@nl ;
  ns2:symbol "damol/m" ;
  ns2:alternativeSymbol "damol m-1", "damol·m-1" ;
  ns2:hasNumerator ns2:decamole ;
  ns2:hasDenominator ns2:metre .

ns2:hectomolePerMetre
  a ns2:PrefixedMolePerMetre ;
  rdfs:label "hectomole per metre"@en, "hectomole per meter"@nl ;
  ns2:symbol "hmol/m" ;
  ns2:alternativeSymbol "hmol m-1", "hmol·m-1" ;
  ns2:hasNumerator ns2:hectomole ;
  ns2:hasDenominator ns2:metre .

ns2:kilomolePerMetre
  a ns2:PrefixedMolePerMetre ;
  rdfs:label "kilomole per metre"@en, "kilomole per meter"@nl ;
  ns2:symbol "kmol/m" ;
  ns2:alternativeSymbol "kmol m-1", "kmol·m-1" ;
  ns2:hasNumerator ns2:kilomole ;
  ns2:hasDenominator ns2:metre .

ns2:megamolePerMetre
  a ns2:PrefixedMolePerMetre ;
  rdfs:label "megamole per metre"@en, "megamole per meter"@nl ;
  ns2:symbol "Mmol/m" ;
  ns2:alternativeSymbol "Mmol m-1", "Mmol·m-1" ;
  ns2:hasNumerator ns2:megamole ;
  ns2:hasDenominator ns2:metre .

ns2:gigamolePerMetre
  a ns2:PrefixedMolePerMetre ;
  rdfs:label "gigamole per metre"@en, "gigamole per meter"@nl ;
  ns2:symbol "Gmol/m" ;
  ns2:alternativeSymbol "Gmol m-1", "Gmol·m-1" ;
  ns2:hasNumerator ns2:gigamole ;
  ns2:hasDenominator ns2:metre .

ns2:teramolePerMetre
  a ns2:PrefixedMolePerMetre ;
  rdfs:label "teramole per metre"@en, "teramole per meter"@nl ;
  ns2:symbol "Tmol/m" ;
  ns2:alternativeSymbol "Tmol m-1", "Tmol·m-1" ;
  ns2:hasNumerator ns2:teramole ;
  ns2:hasDenominator ns2:metre .

ns2:petamolePerMetre
  a ns2:PrefixedMolePerMetre ;
  rdfs:label "petamole per metre"@en, "petamole per meter"@nl ;
  ns2:symbol "Pmol/m" ;
  ns2:alternativeSymbol "Pmol m-1", "Pmol·m-1" ;
  ns2:hasNumerator ns2:petamole ;
  ns2:hasDenominator ns2:metre .

ns2:examolePerMetre
  a ns2:PrefixedMolePerMetre ;
  rdfs:label "examole per metre"@en, "examole per meter"@nl ;
  ns2:symbol "Emol/m" ;
  ns2:alternativeSymbol "Emol m-1", "Emol·m-1" ;
  ns2:hasNumerator ns2:examole ;
  ns2:hasDenominator ns2:metre .

ns2:zettamolePerMetre
  a ns2:PrefixedMolePerMetre ;
  rdfs:label "zettamole per metre"@en, "zettamole per meter"@nl ;
  ns2:symbol "Zmol/m" ;
  ns2:alternativeSymbol "Zmol m-1", "Zmol·m-1" ;
  ns2:hasNumerator ns2:zettamole ;
  ns2:hasDenominator ns2:metre .

ns2:yottamolePerMetre
  a ns2:PrefixedMolePerMetre ;
  rdfs:label "yottamole per metre"@en, "yottamole per meter"@nl ;
  ns2:symbol "Ymol/m" ;
  ns2:alternativeSymbol "Ymol m-1", "Ymol·m-1" ;
  ns2:hasNumerator ns2:yottamole ;
  ns2:hasDenominator ns2:metre .

ns2:molePerYoctometre
  a ns2:MolePerPrefixedMetre ;
  rdfs:label "mole per yoctometre"@en, "mole per yoctometer"@nl ;
  ns2:symbol "mol/ym" ;
  ns2:alternativeSymbol "mol ym-1", "mol·ym-1" ;
  ns2:hasNumerator ns2:mole ;
  ns2:hasDenominator ns2:yoctometre .

ns2:molePerZeptometre
  a ns2:MolePerPrefixedMetre ;
  rdfs:label "mole per zeptometre"@en, "mole per zeptometer"@nl ;
  ns2:symbol "mol/zm" ;
  ns2:alternativeSymbol "mol zm-1", "mol·zm-1" ;
  ns2:hasNumerator ns2:mole ;
  ns2:hasDenominator ns2:zeptometre .

ns2:molePerAttometre
  a ns2:MolePerPrefixedMetre ;
  rdfs:label "mole per attometre"@en, "mole per attometer"@nl ;
  ns2:symbol "mol/am" ;
  ns2:alternativeSymbol "mol am-1", "mol·am-1" ;
  ns2:hasNumerator ns2:mole ;
  ns2:hasDenominator ns2:attometre .

ns2:molePerFemtometre
  a ns2:MolePerPrefixedMetre ;
  rdfs:label "mole per femtometre"@en, "mole per femtometer"@nl ;
  ns2:symbol "mol/fm" ;
  ns2:alternativeSymbol "mol fm-1", "mol·fm-1" ;
  ns2:hasNumerator ns2:mole ;
  ns2:hasDenominator ns2:femtometre .

ns2:molePerPicometre
  a ns2:MolePerPrefixedMetre ;
  rdfs:label "mole per picometre"@en, "mole per picometer"@nl ;
  ns2:symbol "mol/pm" ;
  ns2:alternativeSymbol "mol pm-1", "mol·pm-1" ;
  ns2:hasNumerator ns2:mole ;
  ns2:hasDenominator ns2:picometre .

ns2:molePerNanometre
  a ns2:MolePerPrefixedMetre ;
  rdfs:label "mole per nanometre"@en, "mole per nanometer"@nl ;
  ns2:symbol "mol/nm" ;
  ns2:alternativeSymbol "mol nm-1", "mol·nm-1" ;
  ns2:hasNumerator ns2:mole ;
  ns2:hasDenominator ns2:nanometre .

ns2:molePerMicrometre
  a ns2:MolePerPrefixedMetre ;
  rdfs:label "mole per micrometre"@en, "mole per micrometer"@nl ;
  ns2:symbol "mol/μm" ;
  ns2:alternativeSymbol "mol μm-1", "mol·μm-1" ;
  ns2:hasNumerator ns2:mole ;
  ns2:hasDenominator ns2:micrometre .

ns2:molePerMillimetre
  a ns2:MolePerPrefixedMetre ;
  rdfs:label "mole per millimetre"@en, "mole per millimeter"@nl ;
  ns2:symbol "mol/mm" ;
  ns2:alternativeSymbol "mol mm-1", "mol·mm-1" ;
  ns2:hasNumerator ns2:mole ;
  ns2:hasDenominator ns2:millimetre .

ns2:molePerCentimetre
  a ns2:MolePerPrefixedMetre ;
  rdfs:label "mole per centimetre"@en, "mole per centimeter"@nl ;
  ns2:symbol "mol/cm" ;
  ns2:alternativeSymbol "mol cm-1", "mol·cm-1" ;
  ns2:hasNumerator ns2:mole ;
  ns2:hasDenominator ns2:centimetre .

ns2:molePerDecimetre
  a ns2:MolePerPrefixedMetre ;
  rdfs:label "mole per decimetre"@en, "mole per decimeter"@nl ;
  ns2:symbol "mol/dm" ;
  ns2:alternativeSymbol "mol dm-1", "mol·dm-1" ;
  ns2:hasNumerator ns2:mole ;
  ns2:hasDenominator ns2:decimetre .

ns2:molePerDecametre
  a ns2:MolePerPrefixedMetre ;
  rdfs:label "mole per decametre"@en, "mole per decameter"@nl ;
  ns2:symbol "mol/dam" ;
  ns2:alternativeSymbol "mol dam-1", "mol·dam-1" ;
  ns2:hasNumerator ns2:mole ;
  ns2:hasDenominator ns2:decametre .

ns2:molePerHectometre
  a ns2:MolePerPrefixedMetre ;
  rdfs:label "mole per hectometre"@en, "mole per hectometer"@nl ;
  ns2:symbol "mol/hm" ;
  ns2:alternativeSymbol "mol hm-1", "mol·hm-1" ;
  ns2:hasNumerator ns2:mole ;
  ns2:hasDenominator ns2:hectometre .

ns2:molePerKilometre
  a ns2:MolePerPrefixedMetre ;
  rdfs:label "mole per kilometre"@en, "mole per kilometer"@nl ;
  ns2:symbol "mol/km" ;
  ns2:alternativeSymbol "mol km-1", "mol·km-1" ;
  ns2:hasNumerator ns2:mole ;
  ns2:hasDenominator ns2:kilometre .

ns2:molePermegametre
  a ns2:MolePerPrefixedMetre ;
  rdfs:label "mole per megametre"@en, "mole per megameter"@nl ;
  ns2:symbol "mol/Mm" ;
  ns2:alternativeSymbol "mol Mm-1", "mol·Mm-1" ;
  ns2:hasNumerator ns2:mole ;
  ns2:hasDenominator ns2:megametre .

ns2:molePerGigametre
  a ns2:MolePerPrefixedMetre ;
  rdfs:label "mole per gigametre"@en, "mole per gigameter"@nl ;
  ns2:symbol "mol/Gm" ;
  ns2:alternativeSymbol "mol Gm-1", "mol·Gm-1" ;
  ns2:hasNumerator ns2:mole ;
  ns2:hasDenominator ns2:gigametre .

ns2:molePerTerametre
  a ns2:MolePerPrefixedMetre ;
  rdfs:label "mole per terametre"@en, "mole per terameter"@nl ;
  ns2:symbol "mol/Tm" ;
  ns2:alternativeSymbol "mol Tm-1", "mol·Tm-1" ;
  ns2:hasNumerator ns2:mole ;
  ns2:hasDenominator ns2:terametre .

ns2:molePerPetametre
  a ns2:MolePerPrefixedMetre ;
  rdfs:label "mole per petametre"@en, "mole per petameter"@nl ;
  ns2:symbol "mol/Pm" ;
  ns2:alternativeSymbol "mol Pm-1", "mol·Pm-1" ;
  ns2:hasNumerator ns2:mole ;
  ns2:hasDenominator ns2:petametre .

ns2:molePerExametre
  a ns2:MolePerPrefixedMetre ;
  rdfs:label "mole per exametre"@en, "mole per exameter"@nl ;
  ns2:symbol "mol/Em" ;
  ns2:alternativeSymbol "mol Em-1", "mol·Em-1" ;
  ns2:hasNumerator ns2:mole ;
  ns2:hasDenominator ns2:exametre .

ns2:molePerZettametre
  a ns2:MolePerPrefixedMetre ;
  rdfs:label "mole per zettametre"@en, "mole per zettameter"@nl ;
  ns2:symbol "mol/Zm" ;
  ns2:alternativeSymbol "mol Zm-1", "mol·Zm-1" ;
  ns2:hasNumerator ns2:mole ;
  ns2:hasDenominator ns2:zettametre .

ns2:molePerYottametre
  a ns2:MolePerPrefixedMetre ;
  rdfs:label "mole per yottametre"@en, "mole per yottameter"@nl ;
  ns2:symbol "mol/Ym" ;
  ns2:alternativeSymbol "mol Ym-1", "mol·Ym-1" ;
  ns2:hasNumerator ns2:mole ;
  ns2:hasDenominator ns2:yottametre .

ns2:PrefixedMolePerMetre
  a owl:Class ;
  rdfs:label "prefixed mole per metre"@en ;
  rdfs:subClassOf ns2:UnitDivision ;
  owl:equivalentClass [
    a owl:Class ;
    owl:intersectionOf (
     _:genid1564
     _:genid1566
     _:genid1568
     _:genid1570
   )
  ] .

ns2:MolePerPrefixedMetre
  a owl:Class ;
  rdfs:label "mole per prefixed metre"@en ;
  rdfs:subClassOf ns2:UnitDivision ;
  owl:equivalentClass [
    a owl:Class ;
    owl:intersectionOf (
     _:genid1573
     _:genid1575
     _:genid1577
     _:genid1579
   )
  ] .

ns2:PrefixedMolePerPrefixedMetre
  a owl:Class ;
  rdfs:label "prefixed mole per prefixed metre"@en ;
  rdfs:subClassOf ns2:UnitDivision ;
  owl:equivalentClass [
    a owl:Class ;
    owl:intersectionOf (
     _:genid1582
     _:genid1584
     _:genid1586
     _:genid1588
   )
  ] .

ns2:kelvinMole
  a ns2:UnitMultiplication ;
  rdfs:label "kelvin mole"@en, "kelvin mol"@nl ;
  ns2:symbol "K mol" ;
  ns2:alternativeSymbol "K·mol" ;
  ns2:hasTerm1 ns2:kelvin ;
  ns2:hasTerm2 ns2:mole .

ns2:micromolePerSecond-TimeGram
  a ns2:UnitDivision ;
  rdfs:label "micromole per second gram"@en ;
  ns2:symbol "μmol/(s g)" ;
  ns2:alternativeSymbol "μmol s-1 g-1", "μmol·s-1·g-1" ;
  ns2:hasNumerator ns2:micromolePerSecond-Time ;
  ns2:hasDenominator ns2:gram .

ns2:nanomolePerHour
  a ns2:UnitDivision ;
  rdfs:label "nanomole per hour"@en ;
  ns2:symbol "nmol/h" ;
  ns2:alternativeSymbol "nmol h-1", "nmol·h-1" ;
  ns2:hasNumerator ns2:nanomole ;
  ns2:hasDenominator ns2:hour .

ns2:nanomolePerHourMillilitre
  a ns2:UnitDivision ;
  rdfs:label "nanomole per hour millilitre"@en ;
  ns2:symbol "nmol/(h ml)" ;
  ns2:alternativeSymbol "nmol h-1 ml-1", "nmol·h-1·ml-1" ;
  ns2:hasNumerator ns2:nanomolePerHour ;
  ns2:hasDenominator ns2:millilitre .

ns2:amountOfSubstance-Dimension
  a ns2:Dimension ;
  rdfs:label "amount of substance dimension"@en, "stofhoeveelheiddimensie"@nl ;
  ns2:symbol "N" ;
  ns2:hasSILengthDimensionExponent 0 ;
  ns2:hasSIMassDimensionExponent 0 ;
  ns2:hasSITimeDimensionExponent 0 ;
  ns2:hasSIElectricCurrentDimensionExponent 0 ;
  ns2:hasSIThermodynamicTemperatureDimensionExponent 0 ;
  ns2:hasSIAmountOfSubstanceDimensionExponent 1 ;
  ns2:hasSILuminousIntensityDimensionExponent 0 .

ns2:amountOfSubstanceConcentration-Dimension
  a ns2:Dimension ;
  rdfs:label "amount of substance concentration dimension"@en ;
  ns2:hasSILengthDimensionExponent -3 ;
  ns2:hasSIMassDimensionExponent 0 ;
  ns2:hasSITimeDimensionExponent 0 ;
  ns2:hasSIElectricCurrentDimensionExponent 0 ;
  ns2:hasSIThermodynamicTemperatureDimensionExponent 0 ;
  ns2:hasSIAmountOfSubstanceDimensionExponent 1 ;
  ns2:hasSILuminousIntensityDimensionExponent 0 .

ns2:molarEnergy-Dimension
  a ns2:Dimension ;
  rdfs:label "molar energy dimension"@en, "molaire-energiedimensie"@nl ;
  ns2:hasSILengthDimensionExponent 2 ;
  ns2:hasSIMassDimensionExponent 1 ;
  ns2:hasSITimeDimensionExponent -2 ;
  ns2:hasSIElectricCurrentDimensionExponent 0 ;
  ns2:hasSIThermodynamicTemperatureDimensionExponent 0 ;
  ns2:hasSIAmountOfSubstanceDimensionExponent -1 ;
  ns2:hasSILuminousIntensityDimensionExponent 0 .

ns2:molarEntropyOrMolarHeatCapacityOrGasConstant-Dimension
  a ns2:Dimension ;
  rdfs:label "molar entropy, molar heat capacity, or gas constant dimension"@en ;
  ns2:hasSILengthDimensionExponent 2 ;
  ns2:hasSIMassDimensionExponent 1 ;
  ns2:hasSITimeDimensionExponent -2 ;
  ns2:hasSIElectricCurrentDimensionExponent 0 ;
  ns2:hasSIThermodynamicTemperatureDimensionExponent -1 ;
  ns2:hasSIAmountOfSubstanceDimensionExponent -1 ;
  ns2:hasSILuminousIntensityDimensionExponent 0 .

ns2:chemistry
  a ns2:ApplicationArea ;
  rdfs:label "chemistry"@en, "chemie"@nl ;
  ns2:usesQuantity ns2:CollisionFrequency, ns2:CatalyticActivity, ns2:CatalyticActivityConcentration, ns2:SpecificCatalyticActivity, ns2:SpecificAmylaseActivity, ns2:SpecificProteaseActivity, ns2:Acidity, ns2:Amphiphilicity, ns2:Hydrophilicity, ns2:Hydrophobicity, ns2:Lipophilicity, ns2:SaltStrength ;
  ns2:usesUnit ns2:molePerSecond-Time, ns2:micromolePerSecond-Time, ns2:katal, ns2:attokatal, ns2:centikatal, ns2:decakatal, ns2:decikatal, ns2:exakatal, ns2:femtokatal, ns2:gigakatal, ns2:hectokatal, ns2:kilokatal, ns2:megakatal, ns2:microkatal, ns2:millikatal, ns2:nanokatal, ns2:petakatal, ns2:picokatal, ns2:terakatal, ns2:amylaseUnit, ns2:deltaA450, ns2:deltaA450PerSecond-Time, ns2:katalPerCubicmetre, ns2:nanokatalPerMilligram, ns2:deltaA450PerSecond-TimePerMilligram .

ns2:CollisionFrequency
  a owl:Class ;
  rdfs:label "collision frequency"@en ;
  rdfs:comment "Collision frequency is the average number of collisions between reacting molecules per unit time."@en ;
  rdfs:subClassOf ns2:Frequency ;
  ns2:symbol "ν_coll" ;
  ns2:alternativeSymbol "ν_c" .

ns2:CatalyticActivity
  a owl:Class ;
  rdfs:label "catalytic activity"@en ;
  rdfs:subClassOf ns2:Quantity, [
    a owl:Restriction ;
    owl:onProperty ns2:hasValue ;
    owl:allValuesFrom [
      a owl:Restriction ;
      owl:onProperty ns2:hasUnit ;
      owl:allValuesFrom ns2:CatalyticActivityUnit
    ]
  ], [
    a owl:Restriction ;
    owl:onProperty ns2:hasDimension ;
    owl:hasValue ns2:catalyticActivity-Dimension
  ] ;
  ns2:commonlyHasUnit ns2:molePerSecond-Time, ns2:katal, ns2:attokatal, ns2:centikatal, ns2:decakatal, ns2:decikatal, ns2:exakatal, ns2:femtokatal, ns2:gigakatal, ns2:hectokatal, ns2:kilokatal, ns2:megakatal, ns2:microkatal, ns2:millikatal, ns2:nanokatal, ns2:petakatal, ns2:picokatal, ns2:terakatal, ns2:amylaseUnit, ns2:deltaA450PerSecond-Time .

ns2:CatalyticActivityConcentration
  a owl:Class ;
  rdfs:label "catalytic activity concentration"@en ;
  ns2:alternativeLabel "catalytic concentration"@en ;
  rdfs:subClassOf ns2:Quantity, [
    a owl:Restriction ;
    owl:onProperty ns2:hasValue ;
    owl:allValuesFrom [
      a owl:Restriction ;
      owl:onProperty ns2:hasUnit ;
      owl:allValuesFrom ns2:CatalyticActivityConcentrationUnit
    ]
  ], [
    a owl:Restriction ;
    owl:onProperty ns2:hasDimension ;
    owl:hasValue ns2:catalyticActivityConcentration-Dimension
  ] ;
  ns2:commonlyHasUnit ns2:katalPerCubicmetre .

ns2:SpecificCatalyticActivity
  a owl:Class ;
  rdfs:label "specific catalytic activity"@en ;
  rdfs:subClassOf ns2:Quantity, [
    a owl:Restriction ;
    owl:onProperty ns2:hasValue ;
    owl:allValuesFrom [
      a owl:Restriction ;
      owl:onProperty ns2:hasUnit ;
      owl:allValuesFrom ns2:SpecificCatalyticActivityUnit
    ]
  ], [
    a owl:Restriction ;
    owl:onProperty ns2:hasDimension ;
    owl:hasValue ns2:specificCatalyticActivity-Dimension
  ] ;
  ns2:commonlyHasUnit ns2:nanokatalPerMilligram, ns2:deltaA450PerSecond-TimePerMilligram .

ns2:SpecificAmylaseActivity
  a owl:Class ;
  rdfs:label "specific amylase activity"@en ;
  rdfs:subClassOf ns2:SpecificCatalyticActivity .

ns2:SpecificProteaseActivity
  a owl:Class ;
  rdfs:label "specific protease activity"@en ;
  rdfs:subClassOf ns2:SpecificCatalyticActivity .

ns2:Acidity
  a owl:Class ;
  rdfs:label "acidity"@en ;
  rdfs:subClassOf ns2:Quantity ;
  ns2:symbol "pH" .

ns2:Amphiphilicity
  a owl:Class ;
  rdfs:label "amphiphilicity"@en, "amfifiliciteit"@nl ;
  rdfs:subClassOf ns2:Quantity .

ns2:Hydrophilicity
  a owl:Class ;
  rdfs:label "hydrophilicity"@en, "hydrofiliciteit"@nl ;
  rdfs:subClassOf ns2:Quantity .

ns2:Hydrophobicity
  a owl:Class ;
  rdfs:label "hydrophobicity"@en, "hydrofobiciteit"@nl ;
  rdfs:subClassOf ns2:Quantity .

ns2:Lipophilicity
  a owl:Class ;
  rdfs:label "lipophilicity"@en, "lipofiliciteit"@nl ;
  rdfs:subClassOf ns2:Quantity .

ns2:SaltStrength
  a owl:Class ;
  rdfs:label "salt strength"@en, "zoutsterkte"@nl ;
  rdfs:subClassOf ns2:Quantity .

ns2:molePerSecond-Time
  a ns2:UnitDivision ;
  rdfs:label "mole per second"@en, "mol per seconde"@nl ;
  ns2:symbol "mol/s" ;
  ns2:alternativeSymbol "mol s-1", "mol·s-1" ;
  ns2:hasNumerator ns2:mole ;
  ns2:hasDenominator ns2:second-Time ;
  ns2:hasDimension ns2:catalyticActivity-Dimension .

ns2:micromolePerSecond-Time
  a ns2:UnitDivision ;
  rdfs:label "micromole per second"@en, "micromol per seconde"@nl ;
  ns2:symbol "μmol/s" ;
  ns2:alternativeSymbol "μmol s-1", "μmol·s-1" ;
  ns2:hasNumerator ns2:micromole ;
  ns2:hasDenominator ns2:second-Time ;
  ns2:hasDimension ns2:catalyticActivity-Dimension .

ns2:AmountOfSubstanceFlowUnit
  a owl:Class ;
  rdfs:label "amount of substance flow unit"@en ;
  rdfs:subClassOf ns2:Unit ;
  owl:equivalentClass [
    a owl:Class ;
    owl:oneOf (
     ns2:molePerSecond-Time
     ns2:micromolePerSecond-Time
   )
  ] .

ns2:CatalyticActivityUnit
  a owl:Class ;
  rdfs:label "catalytic activity unit"@en ;
  rdfs:subClassOf ns2:Unit ;
  owl:equivalentClass [
    a owl:Class ;
    owl:unionOf (
     _:genid1600
     ns2:PrefixedKatal
   )
  ] .

ns2:amylaseUnit
  a ns2:Unit, ns2:SingularUnit ;
  rdfs:label "amylase unit"@en ;
  rdfs:comment "The amylase unit is a unit of catalytic activity."@en ;
  ns2:symbol "AU" ;
  ns2:alternativeSymbol "U" ;
  ns2:hasDimension ns2:catalyticActivity-Dimension .

ns2:katal
  a ns2:Unit, ns2:SingularUnit ;
  rdfs:label "katal"@en, "katal"@nl ;
  rdfs:comment "The katal is a unit of catalytic activity defined as mole divided by second."@en ;
  ns2:longcomment "The katal is a unit of catalytic activity defined as mole divided by second. The katal is a derived unit in the International System of Units." ;
  ns2:symbol "kat" ;
  ns2:hasUnit ns2:molePerSecond-Time ;
  ns2:hasDimension ns2:catalyticActivity-Dimension .

ns2:deltaA450PerSecond-Time
  a ns2:UnitDivision ;
  rdfs:label "delta A450 per second"@en, "delta A450 per seconde"@nl ;
  ns2:hasNumerator ns2:deltaA450 ;
  ns2:hasDenominator ns2:second-Time ;
  ns2:hasDimension ns2:catalyticActivity-Dimension .

ns2:PrefixedKatal
  a owl:Class ;
  rdfs:label "prefixed katal"@en ;
  rdfs:subClassOf ns2:PrefixedUnit ;
  owl:equivalentClass [
    a owl:Class ;
    owl:intersectionOf (
     _:genid1612
     _:genid1614
     _:genid1616
     _:genid1618
   )
  ] .

ns2:yoctokatal
  a ns2:PrefixedUnit ;
  rdfs:label "yoctokatal"@en, "yoctokatal"@nl ;
  rdfs:comment "The yoctokatal is a unit of catalytic activity defined as 1.0e-24 katal."@en ;
  ns2:symbol "ykat" ;
  ns2:hasPrefix ns2:yocto ;
  ns2:hasUnit ns2:katal ;
  ns2:hasDimension ns2:catalyticActivity-Dimension .

ns2:zeptokatal
  a ns2:PrefixedUnit ;
  rdfs:label "zeptokatal"@en, "zeptokatal"@nl ;
  rdfs:comment "The zeptkatal is a unit of catalytic activity defined as 1.0e-21 katal."@en ;
  ns2:symbol "zkat" ;
  ns2:hasPrefix ns2:zepto ;
  ns2:hasUnit ns2:katal ;
  ns2:hasDimension ns2:catalyticActivity-Dimension .

ns2:attokatal
  a ns2:PrefixedUnit ;
  rdfs:label "attokatal"@en, "attokatal"@nl ;
  rdfs:comment "The attokatal is a unit of catalytic activity defined as 1.0e-18 katal."@en ;
  ns2:symbol "akat" ;
  ns2:hasPrefix ns2:atto ;
  ns2:hasUnit ns2:katal ;
  ns2:hasDimension ns2:catalyticActivity-Dimension .

ns2:femtokatal
  a ns2:PrefixedUnit ;
  rdfs:label "femtokatal"@en, "femtokatal"@nl ;
  rdfs:comment "The femtokatal is a unit of catalytic activity defined as 1.0e-15 katal."@en ;
  ns2:symbol "fkat" ;
  ns2:hasPrefix ns2:femto ;
  ns2:hasUnit ns2:katal ;
  ns2:hasDimension ns2:catalyticActivity-Dimension .

ns2:picokatal
  a ns2:PrefixedUnit ;
  rdfs:label "picokatal"@en, "picokatal"@nl ;
  rdfs:comment "The picokatal is a unit of catalytic activity defined as 1.0e-12 katal."@en ;
  ns2:symbol "pkat" ;
  ns2:hasPrefix ns2:pico ;
  ns2:hasUnit ns2:katal ;
  ns2:hasDimension ns2:catalyticActivity-Dimension .

ns2:nanokatal
  a ns2:PrefixedUnit ;
  rdfs:label "nanokatal"@en, "nanokatal"@nl ;
  rdfs:comment "The nanokatal is a unit of catalytic activity defined as 1.0e-9 katal."@en ;
  ns2:symbol "nkat" ;
  ns2:hasPrefix ns2:nano ;
  ns2:hasUnit ns2:katal ;
  ns2:hasDimension ns2:catalyticActivity-Dimension .

ns2:microkatal
  a ns2:PrefixedUnit ;
  rdfs:label "microkatal"@en, "microkatal"@nl ;
  rdfs:comment "The microkatal is a unit of catalytic activity defined as 1.0e-6 katal."@en ;
  ns2:symbol "μkat" ;
  ns2:hasPrefix ns2:micro ;
  ns2:hasUnit ns2:katal ;
  ns2:hasDimension ns2:catalyticActivity-Dimension .

ns2:millikatal
  a ns2:PrefixedUnit ;
  rdfs:label "millikatal"@en, "millikatal"@nl ;
  rdfs:comment "The millikatal is a unit of catalytic activity defined as 1.0e-3 katal."@en ;
  ns2:symbol "mkat" ;
  ns2:hasPrefix ns2:milli ;
  ns2:hasUnit ns2:katal ;
  ns2:hasDimension ns2:catalyticActivity-Dimension .

ns2:centikatal
  a ns2:PrefixedUnit ;
  rdfs:label "centikatal"@en, "centikatal"@nl ;
  rdfs:comment "The centikatal is a unit of catalytic activity defined as 1.0e-2 katal."@en ;
  ns2:symbol "ckat" ;
  ns2:hasPrefix ns2:centi ;
  ns2:hasUnit ns2:katal ;
  ns2:hasDimension ns2:catalyticActivity-Dimension .

ns2:decikatal
  a ns2:PrefixedUnit ;
  rdfs:label "decikatal"@en, "decikatal"@nl ;
  rdfs:comment "The decikatal is a unit of catalytic activity defined as 1.0e-1 katal."@en ;
  ns2:symbol "dkat" ;
  ns2:hasPrefix ns2:deci ;
  ns2:hasUnit ns2:katal ;
  ns2:hasDimension ns2:catalyticActivity-Dimension .

ns2:decakatal
  a ns2:PrefixedUnit ;
  rdfs:label "decakatal"@en, "decakatal"@nl ;
  rdfs:comment "The decakatal is a unit of catalytic activity defined as 1.0e1 katal."@en ;
  ns2:symbol "dakat" ;
  ns2:hasPrefix ns2:deca ;
  ns2:hasUnit ns2:katal ;
  ns2:hasDimension ns2:catalyticActivity-Dimension .

ns2:hectokatal
  a ns2:PrefixedUnit ;
  rdfs:label "hectokatal"@en, "hectokatal"@nl ;
  rdfs:comment "The hectokatal is a unit of catalytic activity defined as 1.0e2 katal."@en ;
  ns2:symbol "hkat" ;
  ns2:hasPrefix ns2:hecto ;
  ns2:hasUnit ns2:katal ;
  ns2:hasDimension ns2:catalyticActivity-Dimension .

ns2:kilokatal
  a ns2:PrefixedUnit ;
  rdfs:label "kilokatal"@en, "kilokatal"@nl ;
  rdfs:comment "The kilokatal is a unit of catalytic activity defined as 1.0e3 katal."@en ;
  ns2:symbol "kkat" ;
  ns2:hasPrefix ns2:kilo ;
  ns2:hasUnit ns2:katal ;
  ns2:hasDimension ns2:catalyticActivity-Dimension .

ns2:megakatal
  a ns2:PrefixedUnit ;
  rdfs:label "megakatal"@en, "megakatal"@nl ;
  rdfs:comment "The megakatal is a unit of catalytic activity defined as 1.0e6 katal."@en ;
  ns2:symbol "Mkat" ;
  ns2:hasPrefix ns2:mega ;
  ns2:hasUnit ns2:katal ;
  ns2:hasDimension ns2:catalyticActivity-Dimension .

ns2:gigakatal
  a ns2:PrefixedUnit ;
  rdfs:label "gigakatal"@en, "gigakatal"@nl ;
  rdfs:comment "The gigakatal is a unit of catalytic activity defined as 1.0e9 katal."@en ;
  ns2:symbol "Gkat" ;
  ns2:hasPrefix ns2:giga ;
  ns2:hasUnit ns2:katal ;
  ns2:hasDimension ns2:catalyticActivity-Dimension .

ns2:terakatal
  a ns2:PrefixedUnit ;
  rdfs:label "terakatal"@en, "terakatal"@nl ;
  rdfs:comment "The terakatal is a unit of catalytic activity defined as 1.0e12 katal."@en ;
  ns2:symbol "Tkat" ;
  ns2:hasPrefix ns2:tera ;
  ns2:hasUnit ns2:katal ;
  ns2:hasDimension ns2:catalyticActivity-Dimension .

ns2:petakatal
  a ns2:PrefixedUnit ;
  rdfs:label "petakatal"@en, "petakatal"@nl ;
  rdfs:comment "The petakatal is a unit of catalytic activity defined as 1.0e15 katal."@en ;
  ns2:symbol "Pkat" ;
  ns2:hasPrefix ns2:peta ;
  ns2:hasUnit ns2:katal ;
  ns2:hasDimension ns2:catalyticActivity-Dimension .

ns2:exakatal
  a ns2:PrefixedUnit ;
  rdfs:label "exakatal"@en, "exakatal"@nl ;
  rdfs:comment "The exakatal is a unit of catalytic activity defined as 1.0e18 katal."@en ;
  ns2:symbol "Ekat" ;
  ns2:hasPrefix ns2:exa ;
  ns2:hasUnit ns2:katal ;
  ns2:hasDimension ns2:catalyticActivity-Dimension .

ns2:zettakatal
  a ns2:PrefixedUnit ;
  rdfs:label "zettakatal"@en, "zettakatal"@nl ;
  rdfs:comment "The zettakatal is a unit of catalytic activity defined as 1.0e21 katal."@en ;
  ns2:symbol "Zkat" ;
  ns2:hasPrefix ns2:zetta ;
  ns2:hasUnit ns2:katal ;
  ns2:hasDimension ns2:catalyticActivity-Dimension .

ns2:yottakatal
  a ns2:PrefixedUnit ;
  rdfs:label "yottakatal"@en, "yottakatal"@nl ;
  rdfs:comment "The yottakatal is a unit of catalytic activity defined as 1.0e24 katal."@en ;
  ns2:symbol "Ykat" ;
  ns2:hasPrefix ns2:yotta ;
  ns2:hasUnit ns2:katal ;
  ns2:hasDimension ns2:catalyticActivity-Dimension .

ns2:deltaA450
  a ns2:Unit, ns2:SingularUnit ;
  rdfs:label "delta A450"@en .

ns2:katalPerCubicmetre
  a ns2:UnitDivision ;
  rdfs:label "katal per cubic metre"@en, "katal per kubieke meter"@nl ;
  ns2:symbol "kat/m3" ;
  ns2:alternativeSymbol "kat m-3", "kat·m-3" ;
  ns2:hasNumerator ns2:katal ;
  ns2:hasDenominator ns2:cubicMetre ;
  ns2:hasDimension ns2:catalyticActivityConcentration-Dimension .

ns2:CatalyticActivityConcentrationUnit
  a owl:Class ;
  rdfs:label "catalytic activity concentration unit"@en ;
  rdfs:subClassOf ns2:Unit ;
  owl:equivalentClass [
    a owl:Class ;
    owl:oneOf ( ns2:katalPerCubicmetre )
  ] .

ns2:nanokatalPerMilligram
  a ns2:UnitDivision ;
  rdfs:label "nanokatal per milligram"@en, "nanokatal per milligram"@nl ;
  ns2:symbol "nkat/mg" ;
  ns2:alternativeSymbol "nkat mg-1", "nkat·mg-1" ;
  ns2:hasNumerator ns2:nanokatal ;
  ns2:hasDenominator ns2:milligram ;
  ns2:hasDimension ns2:specificCatalyticActivity-Dimension .

ns2:deltaA450PerSecond-TimePerMilligram
  a ns2:UnitDivision ;
  rdfs:label "delta A450 per second per milligram"@en, "delta A450 per seconde per milligram"@nl ;
  ns2:hasNumerator ns2:deltaA450PerSecond-Time ;
  ns2:hasDenominator ns2:milligram ;
  ns2:hasDimension ns2:specificCatalyticActivity-Dimension .

ns2:SpecificCatalyticActivityUnit
  a owl:Class ;
  rdfs:label "specific catalytic activity unit"@en ;
  rdfs:subClassOf ns2:Unit ;
  owl:equivalentClass [
    a owl:Class ;
    owl:oneOf (
     ns2:nanokatalPerMilligram
     ns2:deltaA450PerSecond-TimePerMilligram
   )
  ] .

ns2:catalyticActivity-Dimension
  a ns2:Dimension ;
  rdfs:label "catalytic activity dimension"@en ;
  ns2:hasSILengthDimensionExponent 0 ;
  ns2:hasSIMassDimensionExponent 0 ;
  ns2:hasSITimeDimensionExponent -1 ;
  ns2:hasSIElectricCurrentDimensionExponent 0 ;
  ns2:hasSIThermodynamicTemperatureDimensionExponent 0 ;
  ns2:hasSIAmountOfSubstanceDimensionExponent 1 ;
  ns2:hasSILuminousIntensityDimensionExponent 0 .

ns2:catalyticActivityConcentration-Dimension
  a ns2:Dimension ;
  rdfs:label "catalytic activity concentration dimension"@en ;
  ns2:hasSILengthDimensionExponent -3 ;
  ns2:hasSIMassDimensionExponent 0 ;
  ns2:hasSITimeDimensionExponent -1 ;
  ns2:hasSIElectricCurrentDimensionExponent 0 ;
  ns2:hasSIThermodynamicTemperatureDimensionExponent 0 ;
  ns2:hasSIAmountOfSubstanceDimensionExponent 1 ;
  ns2:hasSILuminousIntensityDimensionExponent 0 .

ns2:specificCatalyticActivity-Dimension
  a ns2:Dimension ;
  rdfs:label "specific catalytic activity dimension"@en ;
  ns2:hasSILengthDimensionExponent 0 ;
  ns2:hasSIMassDimensionExponent -2 ;
  ns2:hasSITimeDimensionExponent -1 ;
  ns2:hasSIElectricCurrentDimensionExponent 0 ;
  ns2:hasSIThermodynamicTemperatureDimensionExponent 0 ;
  ns2:hasSIAmountOfSubstanceDimensionExponent 1 ;
  ns2:hasSILuminousIntensityDimensionExponent 0 .

ns2:photometry
  a ns2:ApplicationArea ;
  rdfs:label "photometry"@en, "fotometrie"@nl ;
  ns2:usesQuantity ns2:LuminousIntensity, ns2:Luminance, ns2:LuminousFlux, ns2:LuminousEnergy, ns2:Illuminance, ns2:Exposure, ns2:LuminousEfficacy ;
  ns2:usesUnit ns2:candela, ns2:attocandela, ns2:centicandela, ns2:decacandela, ns2:decicandela, ns2:exacandela, ns2:femtocandela, ns2:gigacandela, ns2:hectocandela, ns2:kilocandela, ns2:megacandela, ns2:microcandela, ns2:millicandela, ns2:nanocandela, ns2:petacandela, ns2:picocandela, ns2:teracandela, ns2:candelaPerSquareMetre, ns2:candelaPerSquareCentimetre, ns2:footlambert, ns2:lambert, ns2:stilb, ns2:candelaSteradian, ns2:lumen, ns2:attolumen, ns2:centilumen, ns2:decalumen, ns2:decilumen, ns2:exalumen, ns2:femtolumen, ns2:gigalumen, ns2:hectolumen, ns2:kilolumen, ns2:megalumen, ns2:microlumen, ns2:millilumen, ns2:nanolumen, ns2:petalumen, ns2:picolumen, ns2:teralumen, ns2:lumenPerSquareMetre, ns2:lux, ns2:attolux, ns2:centilux, ns2:decalux, ns2:decilux, ns2:exalux, ns2:femtolux, ns2:gigalux, ns2:hectolux, ns2:kilolux, ns2:megalux, ns2:microlux, ns2:millilux, ns2:nanolux, ns2:petalux, ns2:picolux, ns2:teralux, ns2:footcandle, ns2:phot, ns2:lumenSecond-Time, ns2:luxSecond-Time, ns2:lumenPerWatt .

ns2:LuminousIntensity
  a owl:Class ;
  rdfs:label "luminous intensity"@en, "lichtsterkte"@nl ;
  rdfs:comment "Luminous intensity is the wavelength-weighted power emitted by a light source in a particular direction per unit solid angle. It is a base quantity in the International System of Units. Luminous intensity is luminous flux divided by solid angle."@en ;
  rdfs:subClassOf ns2:Quantity, [
    a owl:Restriction ;
    owl:onProperty ns2:hasValue ;
    owl:allValuesFrom [
      a owl:Restriction ;
      owl:onProperty ns2:hasUnit ;
      owl:allValuesFrom ns2:LuminousIntensityUnit
    ]
  ], [
    a owl:Restriction ;
    owl:onProperty ns2:hasDimension ;
    owl:hasValue ns2:luminousIntensity-Dimension
  ] ;
  ns2:symbol "I" ;
  ns2:alternativeSymbol "I_v" ;
  ns2:commonlyHasUnit ns2:candela, ns2:attocandela, ns2:centicandela, ns2:decacandela, ns2:decicandela, ns2:exacandela, ns2:femtocandela, ns2:gigacandela, ns2:hectocandela, ns2:kilocandela, ns2:megacandela, ns2:microcandela, ns2:millicandela, ns2:nanocandela, ns2:petacandela, ns2:picocandela, ns2:teracandela .

ns2:Luminance
  a owl:Class ;
  rdfs:label "luminance"@en ;
  rdfs:comment "Luminous flux is the total visible energy emitted by a source per unit time."@en ;
  rdfs:subClassOf ns2:Quantity, [
    a owl:Restriction ;
    owl:onProperty ns2:hasValue ;
    owl:allValuesFrom [
      a owl:Restriction ;
      owl:onProperty ns2:hasUnit ;
      owl:allValuesFrom ns2:LuminanceUnit
    ]
  ], [
    a owl:Restriction ;
    owl:onProperty ns2:hasDimension ;
    owl:hasValue ns2:luminance-Dimension
  ] ;
  ns2:symbol "L" ;
  ns2:alternativeSymbol "L_v" ;
  ns2:commonlyHasUnit ns2:candelaPerSquareMetre, ns2:candelaPerSquareCentimetre, ns2:footlambert, ns2:lambert, ns2:stilb .

ns2:LuminousFlux
  a owl:Class ;
  rdfs:label "luminous flux"@en ;
  rdfs:comment "Luminous flux is the total visible energy emitted by a source per unit time."@en ;
  rdfs:subClassOf ns2:Quantity, [
    a owl:Restriction ;
    owl:onProperty ns2:hasValue ;
    owl:allValuesFrom [
      a owl:Restriction ;
      owl:onProperty ns2:hasUnit ;
      owl:allValuesFrom ns2:LuminousFluxUnit
    ]
  ], [
    a owl:Restriction ;
    owl:onProperty ns2:hasDimension ;
    owl:hasValue ns2:luminousFlux-Dimension
  ] ;
  ns2:symbol "F" ;
  ns2:commonlyHasUnit ns2:candelaSteradian, ns2:lumen, ns2:attolumen, ns2:centilumen, ns2:decalumen, ns2:decilumen, ns2:exalumen, ns2:femtolumen, ns2:gigalumen, ns2:hectolumen, ns2:kilolumen, ns2:megalumen, ns2:microlumen, ns2:millilumen, ns2:nanolumen, ns2:petalumen, ns2:picolumen, ns2:teralumen .

ns2:LuminousEnergy
  a owl:Class ;
  rdfs:label "luminous energy"@en ;
  rdfs:subClassOf ns2:Quantity, [
    a owl:Restriction ;
    owl:onProperty ns2:hasValue ;
    owl:allValuesFrom [
      a owl:Restriction ;
      owl:onProperty ns2:hasUnit ;
      owl:allValuesFrom ns2:LuminousEnergyUnit
    ]
  ], [
    a owl:Restriction ;
    owl:onProperty ns2:hasDimension ;
    owl:hasValue ns2:luminousEnergy-Dimension
  ] ;
  ns2:symbol "F" ;
  ns2:commonlyHasUnit ns2:lumenSecond-Time .

ns2:Illuminance
  a owl:Class ;
  rdfs:label "illuminance"@en ;
  ns2:alternativeLabel "illumination"@en ;
  rdfs:comment "Illuminance is the total luminous flux incident on a surface per unit area."@en ;
  rdfs:subClassOf ns2:Quantity, [
    a owl:Restriction ;
    owl:onProperty ns2:hasValue ;
    owl:allValuesFrom [
      a owl:Restriction ;
      owl:onProperty ns2:hasUnit ;
      owl:allValuesFrom ns2:IlluminanceUnit
    ]
  ], [
    a owl:Restriction ;
    owl:onProperty ns2:hasDimension ;
    owl:hasValue ns2:illuminance-Dimension
  ] ;
  ns2:symbol "Φ" ;
  ns2:alternativeSymbol "Φ_v" ;
  ns2:commonlyHasUnit ns2:lumenPerSquareMetre, ns2:lux, ns2:attolux, ns2:centilux, ns2:decalux, ns2:decilux, ns2:exalux, ns2:femtolux, ns2:gigalux, ns2:hectolux, ns2:kilolux, ns2:megalux, ns2:microlux, ns2:millilux, ns2:nanolux, ns2:petalux, ns2:picolux, ns2:teralux, ns2:footcandle, ns2:phot .

ns2:Exposure
  a owl:Class ;
  rdfs:label "exposure"@en ;
  rdfs:subClassOf ns2:Quantity, [
    a owl:Restriction ;
    owl:onProperty ns2:hasValue ;
    owl:allValuesFrom [
      a owl:Restriction ;
      owl:onProperty ns2:hasUnit ;
      owl:allValuesFrom ns2:ExposureUnit
    ]
  ], [
    a owl:Restriction ;
    owl:onProperty ns2:hasDimension ;
    owl:hasValue ns2:exposure-Dimension
  ] ;
  ns2:commonlyHasUnit ns2:luxSecond-Time .

ns2:LuminousEfficacy
  a owl:Class ;
  rdfs:label "luminous efficacy"@en ;
  rdfs:subClassOf ns2:Quantity, [
    a owl:Restriction ;
    owl:onProperty ns2:hasValue ;
    owl:allValuesFrom [
      a owl:Restriction ;
      owl:onProperty ns2:hasUnit ;
      owl:allValuesFrom ns2:LuminousEfficacyUnit
    ]
  ], [
    a owl:Restriction ;
    owl:onProperty ns2:hasDimension ;
    owl:hasValue ns2:luminousEfficacy-Dimension
  ] ;
  ns2:commonlyHasUnit ns2:lumenPerWatt .

ns2:candela
  a ns2:Unit, ns2:SingularUnit ;
  rdfs:label "candela"@en, "candela"@nl, "坎德拉"@zh ;
  ns2:symbol "cd" ;
  ns2:hasDimension ns2:luminousIntensity-Dimension ;
  rdfs:comment "The candela is a unit of luminous intensity defined as the luminous intensity, in a given direction, of a source that emits monochromatic radiation of frequency 540e12 hertz and that has a radiant intensity in that direction of 1/683 watt per steradian."@en ;
  ns2:longcomment "The candela is a unit of luminous intensity defined as the luminous intensity, in a given direction, of a source that emits monochromatic radiation of frequency 540e12 hertz and that has a radiant intensity in that direction of 1/683 watt per steradian. The candela is a base unit in the International System of Units." ;
  ns2:hasQuantity ns2:luminousIntensityInAGivenDirectionOfASourceThatEmitsMonochromaticRadiationOfFrequency540e12HertzAndThatHasARadiantIntensityInThatDirectionOf1683WattPerSteradian .

ns2:luminousIntensityInAGivenDirectionOfASourceThatEmitsMonochromaticRadiationOfFrequency540e12HertzAndThatHasARadiantIntensityInThatDirectionOf1683WattPerSteradian
  a ns2:LuminousIntensity ;
  rdfs:label "luminous intensity, in a given direction, of a source that emits monochromatic radiation of frequency 540e12 hertz and that has a radiant intensity in that direction of 1/683 watt per steradian"@en .

ns2:LuminousIntensityUnit
  a owl:Class ;
  rdfs:label "luminous intensity unit"@en ;
  rdfs:subClassOf ns2:Unit ;
  owl:equivalentClass [
    a owl:Class ;
    owl:unionOf (
     _:genid1633
     ns2:PrefixedCandela
   )
  ] .

ns2:PrefixedCandela
  a owl:Class ;
  rdfs:label "prefixed candela"@en ;
  rdfs:subClassOf ns2:PrefixedUnit ;
  owl:equivalentClass [
    a owl:Class ;
    owl:intersectionOf (
     _:genid1640
     _:genid1642
     _:genid1644
     _:genid1646
   )
  ] .

ns2:yoctocandela
  a ns2:PrefixedUnit ;
  rdfs:label "yoctocandela"@en, "yoctocandela"@nl ;
  rdfs:comment "The yoctocandela is a unit of luminous intensity defined as 1.0e-24 candela."@en ;
  ns2:symbol "ycd" ;
  ns2:hasPrefix ns2:yocto ;
  ns2:hasUnit ns2:candela ;
  ns2:hasDimension ns2:luminousIntensity-Dimension .

ns2:zeptocandela
  a ns2:PrefixedUnit ;
  rdfs:label "zeptocandela"@en, "zeptocandela"@nl ;
  rdfs:comment "The zeptcandela is a unit of luminous intensity defined as 1.0e-21 candela."@en ;
  ns2:symbol "zcd" ;
  ns2:hasPrefix ns2:zepto ;
  ns2:hasUnit ns2:candela ;
  ns2:hasDimension ns2:luminousIntensity-Dimension .

ns2:attocandela
  a ns2:PrefixedUnit ;
  rdfs:label "attocandela"@en, "attocandela"@nl ;
  rdfs:comment "The attocandela is a unit of luminous intensity defined as 1.0e-18 candela."@en ;
  ns2:symbol "acd" ;
  ns2:hasPrefix ns2:atto ;
  ns2:hasUnit ns2:candela ;
  ns2:hasDimension ns2:luminousIntensity-Dimension .

ns2:femtocandela
  a ns2:PrefixedUnit ;
  rdfs:label "femtocandela"@en, "femtocandela"@nl ;
  rdfs:comment "The femtocandela is a unit of luminous intensity defined as 1.0e-15 candela."@en ;
  ns2:symbol "fcd" ;
  ns2:hasPrefix ns2:femto ;
  ns2:hasUnit ns2:candela ;
  ns2:hasDimension ns2:luminousIntensity-Dimension .

ns2:picocandela
  a ns2:PrefixedUnit ;
  rdfs:label "picocandela"@en, "picocandela"@nl ;
  rdfs:comment "The picocandela is a unit of luminous intensity defined as 1.0e-12 candela."@en ;
  ns2:symbol "pcd" ;
  ns2:hasPrefix ns2:pico ;
  ns2:hasUnit ns2:candela ;
  ns2:hasDimension ns2:luminousIntensity-Dimension .

ns2:nanocandela
  a ns2:PrefixedUnit ;
  rdfs:label "nanocandela"@en, "nanocandela"@nl ;
  rdfs:comment "The nanocandela is a unit of luminous intensity defined as 1.0e-9 candela."@en ;
  ns2:symbol "ncd" ;
  ns2:hasPrefix ns2:nano ;
  ns2:hasUnit ns2:candela ;
  ns2:hasDimension ns2:luminousIntensity-Dimension .

ns2:microcandela
  a ns2:PrefixedUnit ;
  rdfs:label "microcandela"@en, "microcandela"@nl ;
  rdfs:comment "The microcandela is a unit of luminous intensity defined as 1.0e-6 candela."@en ;
  ns2:symbol "μcd" ;
  ns2:hasPrefix ns2:micro ;
  ns2:hasUnit ns2:candela ;
  ns2:hasDimension ns2:luminousIntensity-Dimension .

ns2:millicandela
  a ns2:PrefixedUnit ;
  rdfs:label "millicandela"@en, "millicandela"@nl ;
  rdfs:comment "The millicandela is a unit of luminous intensity defined as 1.0e-3 candela."@en ;
  ns2:symbol "mcd" ;
  ns2:hasPrefix ns2:milli ;
  ns2:hasUnit ns2:candela ;
  ns2:hasDimension ns2:luminousIntensity-Dimension .

ns2:centicandela
  a ns2:PrefixedUnit ;
  rdfs:label "centicandela"@en, "centicandela"@nl ;
  rdfs:comment "The centicandela is a unit of luminous intensity defined as 1.0e-2 candela."@en ;
  ns2:symbol "ccd" ;
  ns2:hasPrefix ns2:centi ;
  ns2:hasUnit ns2:candela ;
  ns2:hasDimension ns2:luminousIntensity-Dimension .

ns2:decicandela
  a ns2:PrefixedUnit ;
  rdfs:label "decicandela"@en, "decicandela"@nl ;
  rdfs:comment "The decicandela is a unit of luminous intensity defined as 1.0e-1 candela."@en ;
  ns2:symbol "dcd" ;
  ns2:hasPrefix ns2:deci ;
  ns2:hasUnit ns2:candela ;
  ns2:hasDimension ns2:luminousIntensity-Dimension .

ns2:decacandela
  a ns2:PrefixedUnit ;
  rdfs:label "decacandela"@en, "decacandela"@nl ;
  rdfs:comment "The decacandela is a unit of luminous intensity defined as 1.0e1 candela."@en ;
  ns2:symbol "dacd" ;
  ns2:hasPrefix ns2:deca ;
  ns2:hasUnit ns2:candela ;
  ns2:hasDimension ns2:luminousIntensity-Dimension .

ns2:hectocandela
  a ns2:PrefixedUnit ;
  rdfs:label "hectocandela"@en, "hectocandela"@nl ;
  rdfs:comment "The hectocandela is a unit of luminous intensity defined as 1.0e2 candela."@en ;
  ns2:symbol "hcd" ;
  ns2:hasPrefix ns2:hecto ;
  ns2:hasUnit ns2:candela ;
  ns2:hasDimension ns2:luminousIntensity-Dimension .

ns2:kilocandela
  a ns2:PrefixedUnit ;
  rdfs:label "kilocandela"@en, "kilocandela"@nl ;
  rdfs:comment "The kilocandela is a unit of luminous intensity defined as 1.0e3 candela."@en ;
  ns2:symbol "kcd" ;
  ns2:hasPrefix ns2:kilo ;
  ns2:hasUnit ns2:candela ;
  ns2:hasDimension ns2:luminousIntensity-Dimension .

ns2:megacandela
  a ns2:PrefixedUnit ;
  rdfs:label "megacandela"@en, "megacandela"@nl ;
  rdfs:comment "The megacandela is a unit of luminous intensity defined as 1.0e6 candela."@en ;
  ns2:symbol "Mcd" ;
  ns2:hasPrefix ns2:mega ;
  ns2:hasUnit ns2:candela ;
  ns2:hasDimension ns2:luminousIntensity-Dimension .

ns2:gigacandela
  a ns2:PrefixedUnit ;
  rdfs:label "gigacandela"@en, "gigacandela"@nl ;
  rdfs:comment "The gigacandela is a unit of luminous intensity defined as 1.0e9 candela."@en ;
  ns2:symbol "Gcd" ;
  ns2:hasPrefix ns2:giga ;
  ns2:hasUnit ns2:candela ;
  ns2:hasDimension ns2:luminousIntensity-Dimension .

ns2:teracandela
  a ns2:PrefixedUnit ;
  rdfs:label "teracandela"@en, "teracandela"@nl ;
  rdfs:comment "The teracandela is a unit of luminous intensity defined as 1.0e12 candela."@en ;
  ns2:symbol "Tcd" ;
  ns2:hasPrefix ns2:tera ;
  ns2:hasUnit ns2:candela ;
  ns2:hasDimension ns2:luminousIntensity-Dimension .

ns2:petacandela
  a ns2:PrefixedUnit ;
  rdfs:label "petacandela"@en, "petacandela"@nl ;
  rdfs:comment "The petacandela is a unit of luminous intensity defined as 1.0e15 candela."@en ;
  ns2:symbol "Pcd" ;
  ns2:hasPrefix ns2:peta ;
  ns2:hasUnit ns2:candela ;
  ns2:hasDimension ns2:luminousIntensity-Dimension .

ns2:exacandela
  a ns2:PrefixedUnit ;
  rdfs:label "exacandela"@en, "exacandela"@nl ;
  rdfs:comment "The exacandela is a unit of luminous intensity defined as 1.0e18 candela."@en ;
  ns2:symbol "Ecd" ;
  ns2:hasPrefix ns2:exa ;
  ns2:hasUnit ns2:candela ;
  ns2:hasDimension ns2:luminousIntensity-Dimension .

ns2:zettacandela
  a ns2:PrefixedUnit ;
  rdfs:label "zettacandela"@en, "zettacandela"@nl ;
  rdfs:comment "The zettacandela is a unit of luminous intensity defined as 1.0e21 candela."@en ;
  ns2:symbol "Zcd" ;
  ns2:hasPrefix ns2:zetta ;
  ns2:hasUnit ns2:candela ;
  ns2:hasDimension ns2:luminousIntensity-Dimension .

ns2:yottacandela
  a ns2:PrefixedUnit ;
  rdfs:label "yottacandela"@en, "yottacandela"@nl ;
  rdfs:comment "The yottacandela is a unit of luminous intensity defined as 1.0e24 candela."@en ;
  ns2:symbol "Ycd" ;
  ns2:hasPrefix ns2:yotta ;
  ns2:hasUnit ns2:candela ;
  ns2:hasDimension ns2:luminousIntensity-Dimension .

ns2:candelaPerSquareMetre
  a ns2:UnitDivision ;
  rdfs:label "candela per square metre"@en, "candela per vierkante meter"@nl ;
  rdfs:comment "Candela per square metre is a unit of luminance defined as candela divided by square metre."@en ;
  ns2:longcomment "Candela per square metre is a unit of luminance defined as candela divided by square metre. Candela per square metre is a derived unit in the Internationa; System of Units." ;
  ns2:symbol "cd/m" ;
  ns2:alternativeSymbol "cd m-1", "cd·m-1" ;
  ns2:hasNumerator ns2:candela ;
  ns2:hasDenominator ns2:squareMetre ;
  ns2:hasDimension ns2:luminance-Dimension .

ns2:LuminanceUnit
  a owl:Class ;
  rdfs:label "luminance unit"@en ;
  rdfs:subClassOf ns2:Unit ;
  owl:equivalentClass [
    a owl:Class ;
    owl:oneOf (
     ns2:footlambert
     ns2:lambert
     ns2:stilb
     ns2:candelaPerSquareMetre
     ns2:candelaPerSquareCentimetre
   )
  ] .

ns2:footlambert
  a ns2:Unit, ns2:SingularUnit ;
  rdfs:label "footlambert"@en ;
  rdfs:comment "The footlambert is a unit of luminance defined as 3.426259 candela per square metre."@en ;
  ns2:hasFactor "3.426259"^^xsd:float ;
  ns2:hasUnit ns2:candelaPerSquareMetre ;
  ns2:hasDimension ns2:luminance-Dimension .

ns2:lambert
  a ns2:Unit, ns2:SingularUnit ;
  rdfs:label "lambert"@en, "lambert"@nl ;
  rdfs:comment "The lambert is a unit of luminance defined as 3.183099e3 candela per square metre."@en ;
  ns2:hasFactor "3.183099e3"^^xsd:float ;
  ns2:hasUnit ns2:candelaPerSquareMetre ;
  ns2:hasDimension ns2:luminance-Dimension .

ns2:stilb
  a ns2:Unit, ns2:SingularUnit ;
  rdfs:label "stilb"@en, "stilb"@nl ;
  rdfs:comment "The stilb is a unit of luminance defined as 1.0e4 candela per square metre."@en ;
  ns2:symbol "sb" ;
  ns2:hasFactor "1.0e4"^^xsd:float ;
  ns2:hasUnit ns2:candelaPerSquareMetre ;
  ns2:hasDimension ns2:luminance-Dimension .

ns2:candelaPerSquareCentimetre
  a ns2:UnitDivision ;
  rdfs:label "candela per square centimetre"@en, "candela per vierkante centimeter"@nl ;
  ns2:symbol "cd/cm" ;
  ns2:alternativeSymbol "cd cm-1", "cd·cm-1" ;
  ns2:hasNumerator ns2:candela ;
  ns2:hasDenominator ns2:squareCentimetre ;
  ns2:hasDimension ns2:luminance-Dimension .

ns2:candelaSteradian
  a ns2:UnitMultiplication ;
  rdfs:label "candela steradian"@en, "candela steradiaal"@nl ;
  ns2:symbol "cd sr" ;
  ns2:alternativeSymbol "cd·sr" ;
  ns2:hasTerm1 ns2:candela ;
  ns2:hasTerm2 ns2:steradian ;
  ns2:hasDimension ns2:luminousFlux-Dimension .

ns2:LuminousFluxUnit
  a owl:Class ;
  rdfs:label "luminous flux unit"@en ;
  rdfs:subClassOf ns2:Unit ;
  owl:equivalentClass [
    a owl:Class ;
    owl:unionOf (
     _:genid1657
     ns2:PrefixedLumen
   )
  ] .

ns2:lumen
  a ns2:Unit, ns2:SingularUnit ;
  rdfs:label "lumen"@en, "lumen"@nl ;
  rdfs:comment "The lumen is a unit of luminous flux defined as candela times steradian = lux times square metre."@en ;
  ns2:longcomment "The lumen is a unit of luminous flux defined as candela times steradian = lux times square metre. The lumen is a derived unit in the International System of Units." ;
  ns2:symbol "lm" ;
  ns2:hasUnit ns2:candelaSteradian ;
  ns2:hasDimension ns2:luminousFlux-Dimension .

ns2:PrefixedLumen
  a owl:Class ;
  rdfs:label "prefixed lumen"@en ;
  rdfs:subClassOf ns2:PrefixedUnit ;
  owl:equivalentClass [
    a owl:Class ;
    owl:intersectionOf (
     _:genid1665
     _:genid1667
     _:genid1669
     _:genid1671
   )
  ] .

ns2:yoctolumen
  a ns2:PrefixedUnit ;
  rdfs:label "yoctolumen"@en, "yoctolumen"@nl ;
  ns2:symbol "ylm" ;
  ns2:hasPrefix ns2:yocto ;
  ns2:hasUnit ns2:lumen ;
  ns2:hasDimension ns2:luminousFlux-Dimension .

ns2:zeptolumen
  a ns2:PrefixedUnit ;
  rdfs:label "zeptolumen"@en, "zeptolumen"@nl ;
  ns2:symbol "zlm" ;
  ns2:hasPrefix ns2:zepto ;
  ns2:hasUnit ns2:lumen ;
  ns2:hasDimension ns2:luminousFlux-Dimension .

ns2:attolumen
  a ns2:PrefixedUnit ;
  rdfs:label "attolumen"@en, "attolumen"@nl ;
  ns2:symbol "alm" ;
  ns2:hasPrefix ns2:atto ;
  ns2:hasUnit ns2:lumen ;
  ns2:hasDimension ns2:luminousFlux-Dimension .

ns2:femtolumen
  a ns2:PrefixedUnit ;
  rdfs:label "femtolumen"@en, "femtolumen"@nl ;
  ns2:symbol "flm" ;
  ns2:hasPrefix ns2:femto ;
  ns2:hasUnit ns2:lumen ;
  ns2:hasDimension ns2:luminousFlux-Dimension .

ns2:picolumen
  a ns2:PrefixedUnit ;
  rdfs:label "picolumen"@en, "picolumen"@nl ;
  ns2:symbol "plm" ;
  ns2:hasPrefix ns2:pico ;
  ns2:hasUnit ns2:lumen ;
  ns2:hasDimension ns2:luminousFlux-Dimension .

ns2:nanolumen
  a ns2:PrefixedUnit ;
  rdfs:label "nanolumen"@en, "nanolumen"@nl ;
  ns2:symbol "nlm" ;
  ns2:hasPrefix ns2:nano ;
  ns2:hasUnit ns2:lumen ;
  ns2:hasDimension ns2:luminousFlux-Dimension .

ns2:microlumen
  a ns2:PrefixedUnit ;
  rdfs:label "microlumen"@en, "microlumen"@nl ;
  ns2:symbol "μlm" ;
  ns2:hasPrefix ns2:micro ;
  ns2:hasUnit ns2:lumen ;
  ns2:hasDimension ns2:luminousFlux-Dimension .

ns2:millilumen
  a ns2:PrefixedUnit ;
  rdfs:label "millilumen"@en, "millilumen"@nl ;
  ns2:symbol "mlm" ;
  ns2:hasPrefix ns2:milli ;
  ns2:hasUnit ns2:lumen ;
  ns2:hasDimension ns2:luminousFlux-Dimension .

ns2:centilumen
  a ns2:PrefixedUnit ;
  rdfs:label "centilumen"@en, "centilumen"@nl ;
  ns2:symbol "clm" ;
  ns2:hasPrefix ns2:centi ;
  ns2:hasUnit ns2:lumen ;
  ns2:hasDimension ns2:luminousFlux-Dimension .

ns2:decilumen
  a ns2:PrefixedUnit ;
  rdfs:label "decilumen"@en, "decilumen"@nl ;
  ns2:symbol "dlm" ;
  ns2:hasPrefix ns2:deci ;
  ns2:hasUnit ns2:lumen ;
  ns2:hasDimension ns2:luminousFlux-Dimension .

ns2:decalumen
  a ns2:PrefixedUnit ;
  rdfs:label "decalumen"@en, "decalumen"@nl ;
  ns2:symbol "dalm" ;
  ns2:hasPrefix ns2:deca ;
  ns2:hasUnit ns2:lumen ;
  ns2:hasDimension ns2:luminousFlux-Dimension .

ns2:hectolumen
  a ns2:PrefixedUnit ;
  rdfs:label "hectolumen"@en, "hectolumen"@nl ;
  ns2:symbol "hlm" ;
  ns2:hasPrefix ns2:hecto ;
  ns2:hasUnit ns2:lumen ;
  ns2:hasDimension ns2:luminousFlux-Dimension .

ns2:kilolumen
  a ns2:PrefixedUnit ;
  rdfs:label "kilolumen"@en, "kilolumen"@nl ;
  ns2:symbol "klm" ;
  ns2:hasPrefix ns2:kilo ;
  ns2:hasUnit ns2:lumen ;
  ns2:hasDimension ns2:luminousFlux-Dimension .

ns2:megalumen
  a ns2:PrefixedUnit ;
  rdfs:label "megalumen"@en, "megalumen"@nl ;
  ns2:symbol "Mlm" ;
  ns2:hasPrefix ns2:mega ;
  ns2:hasUnit ns2:lumen ;
  ns2:hasDimension ns2:luminousFlux-Dimension .

ns2:gigalumen
  a ns2:PrefixedUnit ;
  rdfs:label "gigalumen"@en, "gigalumen"@nl ;
  ns2:symbol "Glm" ;
  ns2:hasPrefix ns2:giga ;
  ns2:hasUnit ns2:lumen ;
  ns2:hasDimension ns2:luminousFlux-Dimension .

ns2:teralumen
  a ns2:PrefixedUnit ;
  rdfs:label "teralumen"@en, "teralumen"@nl ;
  ns2:symbol "Tlm" ;
  ns2:hasPrefix ns2:tera ;
  ns2:hasUnit ns2:lumen ;
  ns2:hasDimension ns2:luminousFlux-Dimension .

ns2:petalumen
  a ns2:PrefixedUnit ;
  rdfs:label "petalumen"@en, "petalumen"@nl ;
  ns2:symbol "Plm" ;
  ns2:hasPrefix ns2:peta ;
  ns2:hasUnit ns2:lumen ;
  ns2:hasDimension ns2:luminousFlux-Dimension .

ns2:exalumen
  a ns2:PrefixedUnit ;
  rdfs:label "exalumen"@en, "exalumen"@nl ;
  ns2:symbol "Elm" ;
  ns2:hasPrefix ns2:exa ;
  ns2:hasUnit ns2:lumen ;
  ns2:hasDimension ns2:luminousFlux-Dimension .

ns2:zettalumen
  a ns2:PrefixedUnit ;
  rdfs:label "zettalumen"@en, "zettalumen"@nl ;
  ns2:symbol "Zlm" ;
  ns2:hasPrefix ns2:zetta ;
  ns2:hasUnit ns2:lumen ;
  ns2:hasDimension ns2:luminousFlux-Dimension .

ns2:yottalumen
  a ns2:PrefixedUnit ;
  rdfs:label "yottalumen"@en, "yottalumen"@nl ;
  ns2:symbol "Ylm" ;
  ns2:hasPrefix ns2:yotta ;
  ns2:hasUnit ns2:lumen ;
  ns2:hasDimension ns2:luminousFlux-Dimension .

ns2:lumenSecond-Time
  a ns2:UnitMultiplication ;
  rdfs:label "lumen second"@en, "lumen seconde"@nl ;
  ns2:symbol "lm s" ;
  ns2:alternativeSymbol "lm·s" ;
  ns2:hasTerm1 ns2:lumen ;
  ns2:hasTerm2 ns2:second-Time ;
  ns2:hasDimension ns2:luminousEnergy-Dimension .

ns2:LuminousEnergyUnit
  a owl:Class ;
  rdfs:label "luminous energy unit"@en ;
  rdfs:subClassOf ns2:Unit ;
  owl:equivalentClass [
    a owl:Class ;
    owl:unionOf ( _:genid1674 )
  ] .

ns2:lumenPerSquareMetre
  a ns2:UnitDivision ;
  rdfs:label "lumen per square metre"@en, "lumen per vierkante meter"@nl ;
  ns2:symbol "lm/m2" ;
  ns2:alternativeSymbol "lm m-2", "lm·m-2" ;
  ns2:hasNumerator ns2:lumen ;
  ns2:hasDenominator ns2:squareMetre ;
  ns2:hasDimension ns2:illuminance-Dimension .

ns2:IlluminanceUnit
  a owl:Class ;
  rdfs:label "illuminance unit"@en ;
  rdfs:subClassOf ns2:Unit ;
  owl:equivalentClass [
    a owl:Class ;
    owl:unionOf (
     _:genid1680
     ns2:PrefixedLux
   )
  ] .

ns2:footcandle
  a ns2:Unit, ns2:SingularUnit ;
  rdfs:label "footcandle"@en ;
  rdfs:comment "The footcandle is a unit of illuminance defined as 1.076391e1 lux."@en ;
  ns2:hasFactor "1.076391e1"^^xsd:float ;
  ns2:hasUnit ns2:lux ;
  ns2:hasDimension ns2:illuminance-Dimension .

ns2:lux
  a ns2:Unit, ns2:SingularUnit ;
  rdfs:label "lux"@en, "lux"@nl ;
  rdfs:comment "The lux is a unit of illuminance defined as lumen divided by square metre = candela times steradian divided by square metre."@en ;
  ns2:longcomment "The lux is a unit of illuminance defined as lumen divided by square metre = candela times steradian divided by square metre. The lux is a derived unit in the International System of Units." ;
  ns2:symbol "lx" ;
  ns2:hasUnit ns2:lumenPerSquareMetre ;
  ns2:hasDimension ns2:illuminance-Dimension .

ns2:phot
  a ns2:Unit, ns2:SingularUnit ;
  rdfs:label "phot"@en, "phot"@nl ;
  rdfs:comment "The phot is a unit of illuminance defined as 1.0e4 lux."@en ;
  ns2:symbol "ph" ;
  ns2:hasFactor "1.0e4"^^xsd:float ;
  ns2:hasUnit ns2:lux ;
  ns2:hasDimension ns2:illuminance-Dimension .

ns2:PrefixedLux
  a owl:Class ;
  rdfs:label "prefixed lux"@en ;
  rdfs:subClassOf ns2:PrefixedUnit ;
  owl:equivalentClass [
    a owl:Class ;
    owl:intersectionOf (
     _:genid1690
     _:genid1692
     _:genid1694
     _:genid1696
   )
  ] .

ns2:yoctolux
  a ns2:PrefixedUnit ;
  rdfs:label "yoctolux"@en, "yoctolux"@nl ;
  ns2:symbol "ylx" ;
  ns2:hasPrefix ns2:yocto ;
  ns2:hasUnit ns2:lux ;
  ns2:hasDimension ns2:illuminance-Dimension .

ns2:zeptolux
  a ns2:PrefixedUnit ;
  rdfs:label "zeptolux"@nl, "zeptolux"@en ;
  ns2:symbol "zlx" ;
  ns2:hasPrefix ns2:zepto ;
  ns2:hasUnit ns2:lux ;
  ns2:hasDimension ns2:illuminance-Dimension .

ns2:attolux
  a ns2:PrefixedUnit ;
  rdfs:label "attolux"@en, "attolux"@nl ;
  ns2:symbol "alx" ;
  ns2:hasPrefix ns2:atto ;
  ns2:hasUnit ns2:lux ;
  ns2:hasDimension ns2:illuminance-Dimension .

ns2:femtolux
  a ns2:PrefixedUnit ;
  rdfs:label "femtolux"@en, "femtolux"@nl ;
  ns2:symbol "flx" ;
  ns2:hasPrefix ns2:femto ;
  ns2:hasUnit ns2:lux ;
  ns2:hasDimension ns2:illuminance-Dimension .

ns2:picolux
  a ns2:PrefixedUnit ;
  rdfs:label "picolux"@en, "picolux"@nl ;
  ns2:symbol "plx" ;
  ns2:hasPrefix ns2:pico ;
  ns2:hasUnit ns2:lux ;
  ns2:hasDimension ns2:illuminance-Dimension .

ns2:nanolux
  a ns2:PrefixedUnit ;
  rdfs:label "nanolux"@en, "nanolux"@nl ;
  ns2:symbol "nlx" ;
  ns2:hasPrefix ns2:nano ;
  ns2:hasUnit ns2:lux ;
  ns2:hasDimension ns2:illuminance-Dimension .

ns2:microlux
  a ns2:PrefixedUnit ;
  rdfs:label "microlux"@en, "microlux"@nl ;
  ns2:symbol "μlx" ;
  ns2:hasPrefix ns2:micro ;
  ns2:hasUnit ns2:lux ;
  ns2:hasDimension ns2:illuminance-Dimension .

ns2:millilux
  a ns2:PrefixedUnit ;
  rdfs:label "millilux"@en, "millilux"@nl ;
  ns2:symbol "mlx" ;
  ns2:hasPrefix ns2:milli ;
  ns2:hasUnit ns2:lux ;
  ns2:hasDimension ns2:illuminance-Dimension .

ns2:centilux
  a ns2:PrefixedUnit ;
  rdfs:label "centilux"@en, "centilux"@nl ;
  ns2:symbol "clx" ;
  ns2:hasPrefix ns2:centi ;
  ns2:hasUnit ns2:lux ;
  ns2:hasDimension ns2:illuminance-Dimension .

ns2:decilux
  a ns2:PrefixedUnit ;
  rdfs:label "decilux"@en, "decilux"@nl ;
  ns2:symbol "dlx" ;
  ns2:hasPrefix ns2:deci ;
  ns2:hasUnit ns2:lux ;
  ns2:hasDimension ns2:illuminance-Dimension .

ns2:decalux
  a ns2:PrefixedUnit ;
  rdfs:label "decalux"@en, "decalux"@nl ;
  ns2:symbol "dalx" ;
  ns2:hasPrefix ns2:deca ;
  ns2:hasUnit ns2:lux ;
  ns2:hasDimension ns2:illuminance-Dimension .

ns2:hectolux
  a ns2:PrefixedUnit ;
  rdfs:label "hectolux"@en, "hectolux"@nl ;
  ns2:symbol "hlx" ;
  ns2:hasPrefix ns2:hecto ;
  ns2:hasUnit ns2:lux ;
  ns2:hasDimension ns2:illuminance-Dimension .

ns2:kilolux
  a ns2:PrefixedUnit ;
  rdfs:label "kilolux"@en, "kilolux"@nl ;
  ns2:symbol "klx" ;
  ns2:hasPrefix ns2:kilo ;
  ns2:hasUnit ns2:lux ;
  ns2:hasDimension ns2:illuminance-Dimension .

ns2:megalux
  a ns2:PrefixedUnit ;
  rdfs:label "megalux"@en, "megalux"@nl ;
  ns2:symbol "Mlx" ;
  ns2:hasPrefix ns2:mega ;
  ns2:hasUnit ns2:lux ;
  ns2:hasDimension ns2:illuminance-Dimension .

ns2:gigalux
  a ns2:PrefixedUnit ;
  rdfs:label "gigalux"@en, "gigalux"@nl ;
  ns2:symbol "Glx" ;
  ns2:hasPrefix ns2:giga ;
  ns2:hasUnit ns2:lux ;
  ns2:hasDimension ns2:illuminance-Dimension .

ns2:teralux
  a ns2:PrefixedUnit ;
  rdfs:label "teralux"@en, "teralux"@nl ;
  ns2:symbol "Tlx" ;
  ns2:hasPrefix ns2:tera ;
  ns2:hasUnit ns2:lux ;
  ns2:hasDimension ns2:illuminance-Dimension .

ns2:petalux
  a ns2:PrefixedUnit ;
  rdfs:label "petalux"@en, "petalux"@nl ;
  ns2:symbol "Plx" ;
  ns2:hasPrefix ns2:peta ;
  ns2:hasUnit ns2:lux ;
  ns2:hasDimension ns2:illuminance-Dimension .

ns2:exalux
  a ns2:PrefixedUnit ;
  rdfs:label "exalux"@en, "exalux"@nl ;
  ns2:symbol "Elx" ;
  ns2:hasPrefix ns2:exa ;
  ns2:hasUnit ns2:lux ;
  ns2:hasDimension ns2:illuminance-Dimension .

ns2:zettalux
  a ns2:PrefixedUnit ;
  rdfs:label "zettalux"@en, "zettalux"@nl ;
  ns2:symbol "Zlx" ;
  ns2:hasPrefix ns2:zetta ;
  ns2:hasUnit ns2:lux ;
  ns2:hasDimension ns2:illuminance-Dimension .

ns2:yottalux
  a ns2:PrefixedUnit ;
  rdfs:label "yottalux"@en, "yottalux"@nl ;
  ns2:symbol "Ylx" ;
  ns2:hasPrefix ns2:yotta ;
  ns2:hasUnit ns2:lux ;
  ns2:hasDimension ns2:illuminance-Dimension .

ns2:luxSecond-Time
  a ns2:UnitMultiplication ;
  rdfs:label "lux second"@en, "lux seconde"@nl ;
  ns2:symbol "lx s" ;
  ns2:alternativeSymbol "lx·s" ;
  ns2:hasTerm1 ns2:lux ;
  ns2:hasTerm2 ns2:second-Time ;
  ns2:hasDimension ns2:exposure-Dimension .

ns2:ExposureUnit
  a owl:Class ;
  rdfs:label "exposure unit"@en ;
  rdfs:subClassOf ns2:Unit ;
  owl:equivalentClass [
    a owl:Class ;
    owl:unionOf ( _:genid1699 )
  ] .

ns2:lumenPerWatt
  a ns2:UnitDivision ;
  rdfs:label "lumen per watt"@en, "lumen per watt"@nl ;
  ns2:symbol "lm/W" ;
  ns2:alternativeSymbol "lm W-1", "lm·W-1" ;
  ns2:hasNumerator ns2:lumen ;
  ns2:hasDenominator ns2:watt ;
  ns2:hasDimension ns2:luminousEfficacy-Dimension .

ns2:LuminousEfficacyUnit
  a owl:Class ;
  rdfs:label "luminous efficacy unit"@en ;
  rdfs:subClassOf ns2:Unit ;
  owl:equivalentClass [
    a owl:Class ;
    owl:unionOf ( _:genid1705 )
  ] .

ns2:luminousIntensity-Dimension
  a ns2:Dimension ;
  rdfs:label "luminous intensity dimension"@en, "lichtsterktedimensie"@nl ;
  ns2:symbol "J" ;
  ns2:hasSILengthDimensionExponent 0 ;
  ns2:hasSIMassDimensionExponent 0 ;
  ns2:hasSITimeDimensionExponent 0 ;
  ns2:hasSIElectricCurrentDimensionExponent 0 ;
  ns2:hasSIThermodynamicTemperatureDimensionExponent 0 ;
  ns2:hasSIAmountOfSubstanceDimensionExponent 0 ;
  ns2:hasSILuminousIntensityDimensionExponent 1 .

ns2:luminance-Dimension
  a ns2:Dimension ;
  rdfs:label "luminance dimension"@en ;
  ns2:hasSILengthDimensionExponent -2 ;
  ns2:hasSIMassDimensionExponent 0 ;
  ns2:hasSITimeDimensionExponent 0 ;
  ns2:hasSIElectricCurrentDimensionExponent 0 ;
  ns2:hasSIThermodynamicTemperatureDimensionExponent 0 ;
  ns2:hasSIAmountOfSubstanceDimensionExponent 0 ;
  ns2:hasSILuminousIntensityDimensionExponent 1 .

ns2:luminousFlux-Dimension
  a ns2:Dimension ;
  rdfs:label "luminous flux dimension"@en ;
  ns2:hasSILengthDimensionExponent 0 ;
  ns2:hasSIMassDimensionExponent 0 ;
  ns2:hasSITimeDimensionExponent 0 ;
  ns2:hasSIElectricCurrentDimensionExponent 0 ;
  ns2:hasSIThermodynamicTemperatureDimensionExponent 0 ;
  ns2:hasSIAmountOfSubstanceDimensionExponent 0 ;
  ns2:hasSILuminousIntensityDimensionExponent 1 .

ns2:luminousEnergy-Dimension
  a ns2:Dimension ;
  rdfs:label "luminous energy dimension"@en ;
  ns2:hasSILengthDimensionExponent 0 ;
  ns2:hasSIMassDimensionExponent 0 ;
  ns2:hasSITimeDimensionExponent 1 ;
  ns2:hasSIElectricCurrentDimensionExponent 0 ;
  ns2:hasSIThermodynamicTemperatureDimensionExponent 0 ;
  ns2:hasSIAmountOfSubstanceDimensionExponent 0 ;
  ns2:hasSILuminousIntensityDimensionExponent 1 .

ns2:illuminance-Dimension
  a ns2:Dimension ;
  rdfs:label "illuminance dimension"@en ;
  ns2:hasSILengthDimensionExponent -2 ;
  ns2:hasSIMassDimensionExponent 0 ;
  ns2:hasSITimeDimensionExponent 0 ;
  ns2:hasSIElectricCurrentDimensionExponent 0 ;
  ns2:hasSIThermodynamicTemperatureDimensionExponent 0 ;
  ns2:hasSIAmountOfSubstanceDimensionExponent 0 ;
  ns2:hasSILuminousIntensityDimensionExponent 1 .

ns2:exposure-Dimension
  a ns2:Dimension ;
  rdfs:label "exposure dimension"@en ;
  ns2:hasSILengthDimensionExponent -2 ;
  ns2:hasSIMassDimensionExponent 0 ;
  ns2:hasSITimeDimensionExponent 1 ;
  ns2:hasSIElectricCurrentDimensionExponent 0 ;
  ns2:hasSIThermodynamicTemperatureDimensionExponent 0 ;
  ns2:hasSIAmountOfSubstanceDimensionExponent 0 ;
  ns2:hasSILuminousIntensityDimensionExponent 1 .

ns2:luminousEfficacy-Dimension
  a ns2:Dimension ;
  rdfs:label "luminous efficacy dimension"@en ;
  ns2:hasSILengthDimensionExponent -2 ;
  ns2:hasSIMassDimensionExponent -1 ;
  ns2:hasSITimeDimensionExponent 3 ;
  ns2:hasSIElectricCurrentDimensionExponent 0 ;
  ns2:hasSIThermodynamicTemperatureDimensionExponent 0 ;
  ns2:hasSIAmountOfSubstanceDimensionExponent 0 ;
  ns2:hasSILuminousIntensityDimensionExponent 1 .

ns2:radiometryAndRadiobiology
  a ns2:ApplicationArea ;
  rdfs:label "radiometry and radiobiology"@en, "radiometrie en radiobiologie"@nl ;
  ns2:usesQuantity ns2:AbsorbedDose, ns2:Kerma, ns2:SpecificEnergyImparted, ns2:DoseEquivalent, ns2:AmbientDoseEquivalent, ns2:DirectionalDoseEquivalent, ns2:OrganDoseEquivalent, ns2:PersonalDoseEquivalent, ns2:Activity, ns2:RadiantFlux, ns2:Irradiance, ns2:RadiantIntensity, ns2:Radiance, ns2:ExposureToXAndGammaRays, ns2:AbsorbedDoseRate, ns2:RadiantEnergy ;
  ns2:usesUnit ns2:gray, ns2:attogray, ns2:centigray, ns2:decagray, ns2:decigray, ns2:exagray, ns2:femtogray, ns2:gigagray, ns2:hectogray, ns2:kilogray, ns2:megagray, ns2:microgray, ns2:milligray, ns2:nanogray, ns2:petagray, ns2:picogray, ns2:teragray, ns2:rad, ns2:sievert, ns2:attosievert, ns2:centisievert, ns2:decasievert, ns2:decisievert, ns2:exasievert, ns2:femtosievert, ns2:gigasievert, ns2:hectosievert, ns2:kilosievert, ns2:megasievert, ns2:microsievert, ns2:millisievert, ns2:nanosievert, ns2:petasievert, ns2:picosievert, ns2:terasievert, ns2:rem, ns2:becquerel, ns2:attobecquerel, ns2:centibecquerel, ns2:decabecquerel, ns2:decibecquerel, ns2:exabecquerel, ns2:femtobecquerel, ns2:gigabecquerel, ns2:hectobecquerel, ns2:kilobecquerel, ns2:megabecquerel, ns2:microbecquerel, ns2:millibecquerel, ns2:nanobecquerel, ns2:petabecquerel, ns2:picobecquerel, ns2:terabecquerel, ns2:curie, ns2:coulombPerKilogram, ns2:röntgen, ns2:grayPerSecond-Time, ns2:milligrayPerSecond-Time .

ns2:AbsorbedDose
  a owl:Class ;
  rdfs:label "absorbed dose"@en ;
  ns2:alternativeLabel "total ionizing dose"@en ;
  rdfs:comment "Absorbed dose is the energy deposited in a medium by ionizing radiation. It is a derived quantity in the International System of Units. Absorbed dose is energy divided by mass."@en ;
  rdfs:subClassOf ns2:Quantity, [
    a owl:Restriction ;
    owl:onProperty ns2:hasValue ;
    owl:allValuesFrom [
      a owl:Restriction ;
      owl:onProperty ns2:hasUnit ;
      owl:allValuesFrom ns2:AbsorbedDoseUnit
    ]
  ], [
    a owl:Restriction ;
    owl:onProperty ns2:hasDimension ;
    owl:hasValue ns2:specificEnergyOrAbsorbedDoseOrDoseEquivalent-Dimension
  ] ;
  ns2:commonlyHasUnit ns2:joulePerKilogram, ns2:gray, ns2:attogray, ns2:centigray, ns2:decagray, ns2:decigray, ns2:exagray, ns2:femtogray, ns2:gigagray, ns2:hectogray, ns2:kilogray, ns2:megagray, ns2:microgray, ns2:milligray, ns2:nanogray, ns2:petagray, ns2:picogray, ns2:teragray, ns2:rad .

ns2:AbsorbedDoseUnit
  a owl:Class ;
  rdfs:label "absorbed dose unit"@en ;
  rdfs:subClassOf ns2:Unit ;
  owl:equivalentClass [
    a owl:Class ;
    owl:unionOf (
     _:genid1718
     ns2:PrefixedGray
   )
  ] .

ns2:gray
  a ns2:Unit, ns2:SingularUnit ;
  rdfs:label "gray"@en, "gray"@nl ;
  rdfs:comment "The gray is a unit of absorbed dose defined as joule divided by kilogram = square metre divided by second squared."@en ;
  ns2:longcomment "The gray is a unit of absorbed dose defined as joule divided by kilogram = square metre divided by second squared. The gray is a derived unit is the International System of Units." ;
  ns2:symbol "Gy" ;
  ns2:hasUnit ns2:joulePerKilogram ;
  ns2:hasDimension ns2:specificEnergyOrAbsorbedDoseOrDoseEquivalent-Dimension .

ns2:rad
  a ns2:Unit, ns2:SingularUnit ;
  rdfs:label "rad"@en, "rad"@nl ;
  rdfs:comment "The rad is a unit of absorbed dose defined as 1.0e-2 gray."@en ;
  ns2:symbol "rad" ;
  ns2:hasFactor "1.0e-2"^^xsd:float ;
  ns2:hasUnit ns2:gray ;
  ns2:hasDimension ns2:specificEnergyOrAbsorbedDoseOrDoseEquivalent-Dimension .

ns2:PrefixedGray
  a owl:Class ;
  rdfs:label "prefixed gray"@en ;
  rdfs:subClassOf ns2:PrefixedUnit ;
  owl:equivalentClass [
    a owl:Class ;
    owl:intersectionOf (
     _:genid1731
     _:genid1733
     _:genid1735
     _:genid1737
   )
  ] .

ns2:Kerma
  a owl:Class ;
  rdfs:label "kerma"@en ;
  rdfs:subClassOf ns2:AbsorbedDose ;
  ns2:commonlyHasUnit ns2:joulePerKilogram, ns2:gray, ns2:attogray, ns2:centigray, ns2:decagray, ns2:decigray, ns2:exagray, ns2:femtogray, ns2:gigagray, ns2:hectogray, ns2:kilogray, ns2:megagray, ns2:microgray, ns2:milligray, ns2:nanogray, ns2:petagray, ns2:picogray, ns2:teragray, ns2:rad .

ns2:SpecificEnergyImparted
  a owl:Class ;
  rdfs:label "specific energy imparted"@en ;
  ns2:alternativeLabel "specific energy (imparted)"@en ;
  rdfs:subClassOf ns2:AbsorbedDose ;
  ns2:commonlyHasUnit ns2:joulePerKilogram, ns2:gray, ns2:attogray, ns2:centigray, ns2:decagray, ns2:decigray, ns2:exagray, ns2:femtogray, ns2:gigagray, ns2:hectogray, ns2:kilogray, ns2:megagray, ns2:microgray, ns2:milligray, ns2:nanogray, ns2:petagray, ns2:picogray, ns2:teragray, ns2:rad .

ns2:DoseEquivalent
  a owl:Class ;
  rdfs:label "dose equivalent"@en ;
  rdfs:comment "Dose equivalent is a measure of the radiation dose to tissue where an attempt has been made to allow for the different relative biological effects of different types of ionizing radiation."@en ;
  rdfs:subClassOf ns2:Quantity, [
    a owl:Restriction ;
    owl:onProperty ns2:hasDimension ;
    owl:hasValue ns2:specificEnergyOrAbsorbedDoseOrDoseEquivalent-Dimension
  ], [
    a owl:Restriction ;
    owl:onProperty ns2:hasValue ;
    owl:allValuesFrom [
      a owl:Restriction ;
      owl:onProperty ns2:hasUnit ;
      owl:allValuesFrom ns2:DoseEquivalentUnit
    ]
  ] ;
  ns2:commonlyHasUnit ns2:sievert, ns2:attosievert, ns2:centisievert, ns2:decasievert, ns2:decisievert, ns2:exasievert, ns2:femtosievert, ns2:gigasievert, ns2:hectosievert, ns2:kilosievert, ns2:megasievert, ns2:microsievert, ns2:millisievert, ns2:nanosievert, ns2:petasievert, ns2:picosievert, ns2:terasievert, ns2:rem .

ns2:AmbientDoseEquivalent
  a owl:Class ;
  rdfs:label "ambient dose equivalent"@en ;
  rdfs:subClassOf ns2:DoseEquivalent ;
  ns2:commonlyHasUnit ns2:sievert, ns2:attosievert, ns2:centisievert, ns2:decasievert, ns2:decisievert, ns2:exasievert, ns2:femtosievert, ns2:gigasievert, ns2:hectosievert, ns2:kilosievert, ns2:megasievert, ns2:microsievert, ns2:millisievert, ns2:nanosievert, ns2:petasievert, ns2:picosievert, ns2:terasievert, ns2:rem .

ns2:DirectionalDoseEquivalent
  a owl:Class ;
  rdfs:label "directional dose equivalent"@en ;
  rdfs:subClassOf ns2:DoseEquivalent ;
  ns2:commonlyHasUnit ns2:sievert, ns2:attosievert, ns2:centisievert, ns2:decasievert, ns2:decisievert, ns2:exasievert, ns2:femtosievert, ns2:gigasievert, ns2:hectosievert, ns2:kilosievert, ns2:megasievert, ns2:microsievert, ns2:millisievert, ns2:nanosievert, ns2:petasievert, ns2:picosievert, ns2:terasievert, ns2:rem .

ns2:OrganDoseEquivalent
  a owl:Class ;
  rdfs:label "organ dose equivalent"@en ;
  rdfs:subClassOf ns2:DoseEquivalent ;
  ns2:commonlyHasUnit ns2:sievert, ns2:attosievert, ns2:centisievert, ns2:decasievert, ns2:decisievert, ns2:exasievert, ns2:femtosievert, ns2:gigasievert, ns2:hectosievert, ns2:kilosievert, ns2:megasievert, ns2:microsievert, ns2:millisievert, ns2:nanosievert, ns2:petasievert, ns2:picosievert, ns2:terasievert, ns2:rem .

ns2:PersonalDoseEquivalent
  a owl:Class ;
  rdfs:label "personal dose equivalent"@en ;
  rdfs:subClassOf ns2:DoseEquivalent ;
  ns2:commonlyHasUnit ns2:sievert, ns2:attosievert, ns2:centisievert, ns2:decasievert, ns2:decisievert, ns2:exasievert, ns2:femtosievert, ns2:gigasievert, ns2:hectosievert, ns2:kilosievert, ns2:megasievert, ns2:microsievert, ns2:millisievert, ns2:nanosievert, ns2:petasievert, ns2:picosievert, ns2:terasievert, ns2:rem .

ns2:Activity
  a owl:Class ;
  rdfs:label "activity"@en, "activiteit"@nl ;
  ns2:alternativeLabel "activity (of a radionuclide)"@en, "activity of a radionuclide"@en ;
  rdfs:comment "Activity is the decay rate of a radioactive substance. It is a derived quantity in the International System of Units. Activity is 1 divided by time."@en ;
  rdfs:subClassOf ns2:Quantity, [
    a owl:Restriction ;
    owl:onProperty ns2:hasDimension ;
    owl:hasValue ns2:frequency-Dimension
  ], [
    a owl:Restriction ;
    owl:onProperty ns2:hasValue ;
    owl:allValuesFrom [
      a owl:Restriction ;
      owl:onProperty ns2:hasUnit ;
      owl:allValuesFrom ns2:ActivityUnit
    ]
  ] ;
  ns2:symbol "A" ;
  ns2:commonlyHasUnit ns2:reciprocalSecond-Time, ns2:becquerel, ns2:curie, ns2:attobecquerel, ns2:centibecquerel, ns2:decabecquerel, ns2:decibecquerel, ns2:exabecquerel, ns2:femtobecquerel, ns2:gigabecquerel, ns2:hectobecquerel, ns2:kilobecquerel, ns2:megabecquerel, ns2:microbecquerel, ns2:millibecquerel, ns2:nanobecquerel, ns2:petabecquerel, ns2:picobecquerel, ns2:terabecquerel .

ns2:ExposureToXAndGammaRays
  a owl:Class ;
  rdfs:label "exposure to x and γ rays"@en ;
  ns2:alternativeLabel "exposure to x and gamma rays"@en, "exposure (to x and γ rays)"@en, "exposure (to x and gamma rays)"@en, "exposure"@en ;
  rdfs:subClassOf ns2:Quantity, [
    a owl:Restriction ;
    owl:onProperty ns2:hasValue ;
    owl:allValuesFrom [
      a owl:Restriction ;
      owl:onProperty ns2:hasUnit ;
      owl:allValuesFrom ns2:ExposureToXAndGammaRaysUnit
    ]
  ], [
    a owl:Restriction ;
    owl:onProperty ns2:hasDimension ;
    owl:hasValue ns2:exposureToXAndGammaRays-Dimension
  ] ;
  ns2:commonlyHasUnit ns2:coulombPerKilogram, ns2:röntgen .

ns2:AbsorbedDoseRate
  a owl:Class ;
  rdfs:label "absorbed dose rate"@en ;
  rdfs:subClassOf ns2:Quantity, [
    a owl:Restriction ;
    owl:onProperty ns2:hasValue ;
    owl:allValuesFrom [
      a owl:Restriction ;
      owl:onProperty ns2:hasUnit ;
      owl:allValuesFrom ns2:AbsorbedDoseRateUnit
    ]
  ], [
    a owl:Restriction ;
    owl:onProperty ns2:hasDimension ;
    owl:hasValue ns2:absorbedDoseRate-Dimension
  ] ;
  ns2:commonlyHasUnit ns2:grayPerSecond-Time, ns2:milligrayPerSecond-Time .

ns2:RadiantEnergy
  a owl:Class ;
  rdfs:label "radiant energy"@en ;
  rdfs:subClassOf ns2:Energy ;
  ns2:symbol "Q" ;
  ns2:alternativeSymbol "Q_e", "W" ;
  ns2:commonlyHasUnit ns2:newtonMetre, ns2:micronewtonMetre, ns2:millinewtonMetre, ns2:joule, ns2:attojoule, ns2:centijoule, ns2:decajoule, ns2:decijoule, ns2:exajoule, ns2:femtojoule, ns2:gigajoule, ns2:hectojoule, ns2:kilojoule, ns2:megajoule, ns2:microjoule, ns2:millijoule, ns2:nanojoule, ns2:petajoule, ns2:picojoule, ns2:terajoule, ns2:electronvolt, ns2:gigaelectronvolt, ns2:kiloelectronvolt, ns2:megaelectronvolt, ns2:calorie-Mean, ns2:kilocalorie-Mean, ns2:BritishThermalUnit-39F, ns2:BritishThermalUnit-59F, ns2:BritishThermalUnit-60F, ns2:BritishThermalUnit-InternationalTable, ns2:BritishThermalUnit-Mean, ns2:BritishThermalUnit-Thermochemical, ns2:calorie-15C, ns2:calorie-20C, ns2:calorie-InternationalTable, ns2:calorie-Thermochemical, ns2:erg, ns2:footPoundal, ns2:quad, ns2:wattHour, ns2:kilowattHour, ns2:megawattHour, ns2:gigawattHour, ns2:terawattHour, ns2:therm-EC, ns2:therm-US, ns2:tonOfTNT, ns2:megaerg .

ns2:yoctogray
  a ns2:PrefixedUnit ;
  rdfs:label "yoctogray"@en, "yoctogray"@nl ;
  rdfs:comment "The yoctogray is a unit of absorbed dose defined as 1.0e-24 gray."@en ;
  ns2:symbol "yGy" ;
  ns2:hasPrefix ns2:yocto ;
  ns2:hasUnit ns2:gray ;
  ns2:hasDimension ns2:specificEnergyOrAbsorbedDoseOrDoseEquivalent-Dimension .

ns2:zeptogray
  a ns2:PrefixedUnit ;
  rdfs:label "zeptogray"@en, "zeptogray"@nl ;
  rdfs:comment "The zeptgray is a unit of absorbed dose defined as 1.0e-21 gray."@en ;
  ns2:symbol "zGy" ;
  ns2:hasPrefix ns2:zepto ;
  ns2:hasUnit ns2:gray ;
  ns2:hasDimension ns2:specificEnergyOrAbsorbedDoseOrDoseEquivalent-Dimension .

ns2:attogray
  a ns2:PrefixedUnit ;
  rdfs:label "attogray"@en, "attogray"@nl ;
  rdfs:comment "The attogray is a unit of absorbed dose defined as 1.0e-18 gray."@en ;
  ns2:symbol "aGy" ;
  ns2:hasPrefix ns2:atto ;
  ns2:hasUnit ns2:gray ;
  ns2:hasDimension ns2:specificEnergyOrAbsorbedDoseOrDoseEquivalent-Dimension .

ns2:femtogray
  a ns2:PrefixedUnit ;
  rdfs:label "femtogray"@en, "femtogray"@nl ;
  rdfs:comment "The femtogray is a unit of absorbed dose defined as 1.0e-15 gray."@en ;
  ns2:symbol "fGy" ;
  ns2:hasPrefix ns2:femto ;
  ns2:hasUnit ns2:gray ;
  ns2:hasDimension ns2:specificEnergyOrAbsorbedDoseOrDoseEquivalent-Dimension .

ns2:picogray
  a ns2:PrefixedUnit ;
  rdfs:label "picogray"@en, "picogray"@nl ;
  rdfs:comment "The picogray is a unit of absorbed dose defined as 1.0e-12 gray."@en ;
  ns2:symbol "pGy" ;
  ns2:hasPrefix ns2:pico ;
  ns2:hasUnit ns2:gray ;
  ns2:hasDimension ns2:specificEnergyOrAbsorbedDoseOrDoseEquivalent-Dimension .

ns2:nanogray
  a ns2:PrefixedUnit ;
  rdfs:label "nanogray"@en, "nanogray"@nl ;
  rdfs:comment "The nanogray is a unit of absorbed dose defined as 1.0e-9 gray."@en ;
  ns2:symbol "nGy" ;
  ns2:hasPrefix ns2:nano ;
  ns2:hasUnit ns2:gray ;
  ns2:hasDimension ns2:specificEnergyOrAbsorbedDoseOrDoseEquivalent-Dimension .

ns2:microgray
  a ns2:PrefixedUnit ;
  rdfs:label "microgray"@en, "microgray"@nl ;
  rdfs:comment "The microgray is a unit of absorbed dose defined as 1.0e-6 gray."@en ;
  ns2:symbol "μGy" ;
  ns2:hasPrefix ns2:micro ;
  ns2:hasUnit ns2:gray ;
  ns2:hasDimension ns2:specificEnergyOrAbsorbedDoseOrDoseEquivalent-Dimension .

ns2:milligray
  a ns2:PrefixedUnit ;
  rdfs:label "milligray"@en, "milligray"@nl ;
  rdfs:comment "The milligray is a unit of absorbed dose defined as 1.0e-3 gray."@en ;
  ns2:symbol "mGy" ;
  ns2:hasPrefix ns2:milli ;
  ns2:hasUnit ns2:gray ;
  ns2:hasDimension ns2:specificEnergyOrAbsorbedDoseOrDoseEquivalent-Dimension .

ns2:centigray
  a ns2:PrefixedUnit ;
  rdfs:label "centigray"@en, "centigray"@nl ;
  rdfs:comment "The centigray is a unit of absorbed dose defined as 1.0e-2 gray."@en ;
  ns2:symbol "cGy" ;
  ns2:hasPrefix ns2:centi ;
  ns2:hasUnit ns2:gray ;
  ns2:hasDimension ns2:specificEnergyOrAbsorbedDoseOrDoseEquivalent-Dimension .

ns2:decigray
  a ns2:PrefixedUnit ;
  rdfs:label "decigray"@en, "decigray"@nl ;
  rdfs:comment "The decigray is a unit of absorbed dose defined as 1.0e-1 gray."@en ;
  ns2:symbol "dGy" ;
  ns2:hasPrefix ns2:deci ;
  ns2:hasUnit ns2:gray ;
  ns2:hasDimension ns2:specificEnergyOrAbsorbedDoseOrDoseEquivalent-Dimension .

ns2:decagray
  a ns2:PrefixedUnit ;
  rdfs:label "decagray"@en, "decagray"@nl ;
  rdfs:comment "The decagray is a unit of absorbed dose defined as 1.0e1 gray."@en ;
  ns2:symbol "daGy" ;
  ns2:hasPrefix ns2:deca ;
  ns2:hasUnit ns2:gray ;
  ns2:hasDimension ns2:specificEnergyOrAbsorbedDoseOrDoseEquivalent-Dimension .

ns2:hectogray
  a ns2:PrefixedUnit ;
  rdfs:label "hectogray"@en, "hectogray"@nl ;
  rdfs:comment "The hectogray is a unit of absorbed dose defined as 1.0e2 gray."@en ;
  ns2:symbol "hGy" ;
  ns2:hasPrefix ns2:hecto ;
  ns2:hasUnit ns2:gray ;
  ns2:hasDimension ns2:specificEnergyOrAbsorbedDoseOrDoseEquivalent-Dimension .

ns2:kilogray
  a ns2:PrefixedUnit ;
  rdfs:label "kilogray"@en, "kilogray"@nl ;
  rdfs:comment "The kilogray is a unit of absorbed dose defined as 1.0e3 gray."@en ;
  ns2:symbol "kGy" ;
  ns2:hasPrefix ns2:kilo ;
  ns2:hasUnit ns2:gray ;
  ns2:hasDimension ns2:specificEnergyOrAbsorbedDoseOrDoseEquivalent-Dimension .

ns2:megagray
  a ns2:PrefixedUnit ;
  rdfs:label "megagray"@en, "megagray"@nl ;
  rdfs:comment "The megagray is a unit of absorbed dose defined as 1.0e6 gray."@en ;
  ns2:symbol "MGy" ;
  ns2:hasPrefix ns2:mega ;
  ns2:hasUnit ns2:gray ;
  ns2:hasDimension ns2:specificEnergyOrAbsorbedDoseOrDoseEquivalent-Dimension .

ns2:gigagray
  a ns2:PrefixedUnit ;
  rdfs:label "gigagray"@en, "gigagray"@nl ;
  rdfs:comment "The gigagray is a unit of absorbed dose defined as 1.0e9 gray."@en ;
  ns2:symbol "GGy" ;
  ns2:hasPrefix ns2:giga ;
  ns2:hasUnit ns2:gray ;
  ns2:hasDimension ns2:specificEnergyOrAbsorbedDoseOrDoseEquivalent-Dimension .

ns2:teragray
  a ns2:PrefixedUnit ;
  rdfs:label "teragray"@en, "teragray"@nl ;
  rdfs:comment "The teragray is a unit of absorbed dose defined as 1.0e12 gray."@en ;
  ns2:symbol "TGy" ;
  ns2:hasPrefix ns2:tera ;
  ns2:hasUnit ns2:gray ;
  ns2:hasDimension ns2:specificEnergyOrAbsorbedDoseOrDoseEquivalent-Dimension .

ns2:petagray
  a ns2:PrefixedUnit ;
  rdfs:label "petagray"@en, "petagray"@nl ;
  rdfs:comment "The petagray is a unit of absorbed dose defined as 1.0e15 gray."@en ;
  ns2:symbol "PGy" ;
  ns2:hasPrefix ns2:peta ;
  ns2:hasUnit ns2:gray ;
  ns2:hasDimension ns2:specificEnergyOrAbsorbedDoseOrDoseEquivalent-Dimension .

ns2:exagray
  a ns2:PrefixedUnit ;
  rdfs:label "exagray"@en, "exagray"@nl ;
  rdfs:comment "The exagray is a unit of absorbed dose defined as 1.0e18 gray."@en ;
  ns2:symbol "EGy" ;
  ns2:hasPrefix ns2:exa ;
  ns2:hasUnit ns2:gray ;
  ns2:hasDimension ns2:specificEnergyOrAbsorbedDoseOrDoseEquivalent-Dimension .

ns2:zettagray
  a ns2:PrefixedUnit ;
  rdfs:label "zettagray"@en, "zettagray"@nl ;
  rdfs:comment "The zettagray is a unit of absorbed dose defined as 1.0e21 gray."@en ;
  ns2:symbol "ZGy" ;
  ns2:hasPrefix ns2:zetta ;
  ns2:hasUnit ns2:gray ;
  ns2:hasDimension ns2:specificEnergyOrAbsorbedDoseOrDoseEquivalent-Dimension .

ns2:yottagray
  a ns2:PrefixedUnit ;
  rdfs:label "yottagray"@en, "yottagray"@nl ;
  rdfs:comment "The yottagray is a unit of absorbed dose defined as 1.0e24 gray."@en ;
  ns2:symbol "YGy" ;
  ns2:hasPrefix ns2:yotta ;
  ns2:hasUnit ns2:gray ;
  ns2:hasDimension ns2:specificEnergyOrAbsorbedDoseOrDoseEquivalent-Dimension .

ns2:sievert
  a ns2:Unit, ns2:SingularUnit ;
  rdfs:label "sievert"@en, "sievert"@nl ;
  rdfs:comment "The sievert is a unit of dose equivalent defined as joule divided by kilogram = square metre divided by second squared."@en ;
  ns2:longcomment "The sievert is a unit of dose equivalent defined as joule divided by kilogram = square metre divided by second squared. The sievert is a derived unit is the International System of Units." ;
  ns2:symbol "Sv" ;
  ns2:hasUnit ns2:joulePerKilogram ;
  ns2:hasDimension ns2:specificEnergyOrAbsorbedDoseOrDoseEquivalent-Dimension .

ns2:DoseEquivalentUnit
  a owl:Class ;
  rdfs:label "dose equivalent unit"@en ;
  rdfs:subClassOf ns2:Unit ;
  owl:equivalentClass [
    a owl:Class ;
    owl:unionOf (
     _:genid1740
     ns2:PrefixedSievert
   )
  ] .

ns2:rem
  a ns2:Unit, ns2:SingularUnit ;
  rdfs:label "rem"@en, "rem"@nl ;
  rdfs:comment "The rem is a unit of dose equivalent defined as 1.0e-2 sievert."@en ;
  ns2:symbol "rem" ;
  ns2:hasFactor "1.0e-2"^^xsd:float ;
  ns2:hasUnit ns2:sievert ;
  ns2:hasDimension ns2:specificEnergyOrAbsorbedDoseOrDoseEquivalent-Dimension .

ns2:PrefixedSievert
  a owl:Class ;
  rdfs:label "prefixed sievert"@en ;
  rdfs:subClassOf ns2:PrefixedUnit ;
  owl:equivalentClass [
    a owl:Class ;
    owl:intersectionOf (
     _:genid1750
     _:genid1752
     _:genid1754
     _:genid1756
   )
  ] .

ns2:yoctosievert
  a ns2:PrefixedUnit ;
  rdfs:label "yoctosievert"@en, "yoctosievert"@nl ;
  ns2:symbol "ySv" ;
  ns2:hasPrefix ns2:yocto ;
  ns2:hasUnit ns2:sievert ;
  ns2:hasDimension ns2:specificEnergyOrAbsorbedDoseOrDoseEquivalent-Dimension .

ns2:zeptosievert
  a ns2:PrefixedUnit ;
  rdfs:label "zeptosievert"@en, "zeptosievert"@nl ;
  ns2:symbol "zSv" ;
  ns2:hasPrefix ns2:zepto ;
  ns2:hasUnit ns2:sievert ;
  ns2:hasDimension ns2:specificEnergyOrAbsorbedDoseOrDoseEquivalent-Dimension .

ns2:attosievert
  a ns2:PrefixedUnit ;
  rdfs:label "attosievert"@en, "attosievert"@nl ;
  ns2:symbol "aSv" ;
  ns2:hasPrefix ns2:atto ;
  ns2:hasUnit ns2:sievert ;
  ns2:hasDimension ns2:specificEnergyOrAbsorbedDoseOrDoseEquivalent-Dimension .

ns2:femtosievert
  a ns2:PrefixedUnit ;
  rdfs:label "femtosievert"@en, "femtosievert"@nl ;
  ns2:symbol "fSv" ;
  ns2:hasPrefix ns2:femto ;
  ns2:hasUnit ns2:sievert ;
  ns2:hasDimension ns2:specificEnergyOrAbsorbedDoseOrDoseEquivalent-Dimension .

ns2:picosievert
  a ns2:PrefixedUnit ;
  rdfs:label "picosievert"@en, "picosievert"@nl ;
  ns2:symbol "pSv" ;
  ns2:hasPrefix ns2:pico ;
  ns2:hasUnit ns2:sievert ;
  ns2:hasDimension ns2:specificEnergyOrAbsorbedDoseOrDoseEquivalent-Dimension .

ns2:nanosievert
  a ns2:PrefixedUnit ;
  rdfs:label "nanosievert"@en, "nanosievert"@nl ;
  ns2:symbol "nSv" ;
  ns2:hasPrefix ns2:nano ;
  ns2:hasUnit ns2:sievert ;
  ns2:hasDimension ns2:specificEnergyOrAbsorbedDoseOrDoseEquivalent-Dimension .

ns2:microsievert
  a ns2:PrefixedUnit ;
  rdfs:label "microsievert"@en, "microsievert"@nl ;
  ns2:symbol "μSv" ;
  ns2:hasPrefix ns2:micro ;
  ns2:hasUnit ns2:sievert ;
  ns2:hasDimension ns2:specificEnergyOrAbsorbedDoseOrDoseEquivalent-Dimension .

ns2:millisievert
  a ns2:PrefixedUnit ;
  rdfs:label "millisievert"@en, "millisievert"@nl ;
  ns2:symbol "mSv" ;
  ns2:hasPrefix ns2:milli ;
  ns2:hasUnit ns2:sievert ;
  ns2:hasDimension ns2:specificEnergyOrAbsorbedDoseOrDoseEquivalent-Dimension .

ns2:centisievert
  a ns2:PrefixedUnit ;
  rdfs:label "centisievert"@en, "centisievert"@nl ;
  ns2:symbol "cSv" ;
  ns2:hasPrefix ns2:centi ;
  ns2:hasUnit ns2:sievert ;
  ns2:hasDimension ns2:specificEnergyOrAbsorbedDoseOrDoseEquivalent-Dimension .

ns2:decisievert
  a ns2:PrefixedUnit ;
  rdfs:label "decisievert"@en, "decisievert"@nl ;
  ns2:symbol "dSv" ;
  ns2:hasPrefix ns2:deci ;
  ns2:hasUnit ns2:sievert ;
  ns2:hasDimension ns2:specificEnergyOrAbsorbedDoseOrDoseEquivalent-Dimension .

ns2:decasievert
  a ns2:PrefixedUnit ;
  rdfs:label "decasievert"@en, "decasievert"@nl ;
  ns2:symbol "daSv" ;
  ns2:hasPrefix ns2:deca ;
  ns2:hasUnit ns2:sievert ;
  ns2:hasDimension ns2:specificEnergyOrAbsorbedDoseOrDoseEquivalent-Dimension .

ns2:hectosievert
  a ns2:PrefixedUnit ;
  rdfs:label "hectosievert"@en, "hectosievert"@nl ;
  ns2:symbol "hSv" ;
  ns2:hasPrefix ns2:hecto ;
  ns2:hasUnit ns2:sievert ;
  ns2:hasDimension ns2:specificEnergyOrAbsorbedDoseOrDoseEquivalent-Dimension .

ns2:kilosievert
  a ns2:PrefixedUnit ;
  rdfs:label "kilosievert"@en, "kilosievert"@nl ;
  ns2:symbol "kSv" ;
  ns2:hasPrefix ns2:kilo ;
  ns2:hasUnit ns2:sievert ;
  ns2:hasDimension ns2:specificEnergyOrAbsorbedDoseOrDoseEquivalent-Dimension .

ns2:megasievert
  a ns2:PrefixedUnit ;
  rdfs:label "megasievert"@en, "megasievert"@nl ;
  ns2:symbol "MSv" ;
  ns2:hasPrefix ns2:mega ;
  ns2:hasUnit ns2:sievert ;
  ns2:hasDimension ns2:specificEnergyOrAbsorbedDoseOrDoseEquivalent-Dimension .

ns2:gigasievert
  a ns2:PrefixedUnit ;
  rdfs:label "gigasievert"@en, "gigasievert"@nl ;
  ns2:symbol "GSv" ;
  ns2:hasPrefix ns2:giga ;
  ns2:hasUnit ns2:sievert ;
  ns2:hasDimension ns2:specificEnergyOrAbsorbedDoseOrDoseEquivalent-Dimension .

ns2:terasievert
  a ns2:PrefixedUnit ;
  rdfs:label "terasievert"@en, "terasievert"@nl ;
  ns2:symbol "TSv" ;
  ns2:hasPrefix ns2:tera ;
  ns2:hasUnit ns2:sievert ;
  ns2:hasDimension ns2:specificEnergyOrAbsorbedDoseOrDoseEquivalent-Dimension .

ns2:petasievert
  a ns2:PrefixedUnit ;
  rdfs:label "petasievert"@en, "petasievert"@nl ;
  ns2:symbol "PSv" ;
  ns2:hasPrefix ns2:peta ;
  ns2:hasUnit ns2:sievert ;
  ns2:hasDimension ns2:specificEnergyOrAbsorbedDoseOrDoseEquivalent-Dimension .

ns2:exasievert
  a ns2:PrefixedUnit ;
  rdfs:label "exasievert"@en, "exasievert"@nl ;
  ns2:symbol "ESv" ;
  ns2:hasPrefix ns2:exa ;
  ns2:hasUnit ns2:sievert ;
  ns2:hasDimension ns2:specificEnergyOrAbsorbedDoseOrDoseEquivalent-Dimension .

ns2:zettasievert
  a ns2:PrefixedUnit ;
  rdfs:label "zettasievert"@en, "zettasievert"@nl ;
  ns2:symbol "ZSv" ;
  ns2:hasPrefix ns2:zetta ;
  ns2:hasUnit ns2:sievert ;
  ns2:hasDimension ns2:specificEnergyOrAbsorbedDoseOrDoseEquivalent-Dimension .

ns2:yottasievert
  a ns2:PrefixedUnit ;
  rdfs:label "yottasievert"@en, "yottasievert"@nl ;
  ns2:symbol "YSv" ;
  ns2:hasPrefix ns2:yotta ;
  ns2:hasUnit ns2:sievert ;
  ns2:hasDimension ns2:specificEnergyOrAbsorbedDoseOrDoseEquivalent-Dimension .

ns2:becquerel
  a ns2:Unit, ns2:SingularUnit ;
  rdfs:label "becquerel"@en, "becquerel"@nl ;
  rdfs:comment "The becquerel is a unit of activity defined as the activity of a quantity of radioactive material in which one nucleus decays per second. Algebraically it is defined as 1 divided by second."@en ;
  ns2:longcomment "The becquerel is a unit of activity defined as the activity of a quantity of radioactive material in which one nucleus decays per second. Algebraically it is defined as 1 divided by second. The becquerel is a derived unit in the International System of Units." ;
  ns2:symbol "Bq" ;
  ns2:hasUnit ns2:reciprocalSecond-Time ;
  ns2:hasDimension ns2:frequency-Dimension .

ns2:ActivityUnit
  a owl:Class ;
  rdfs:label "activity unit"@en ;
  rdfs:subClassOf ns2:Unit ;
  owl:equivalentClass [
    a owl:Class ;
    owl:unionOf (
     _:genid1759
     ns2:PrefixedBecquerel
   )
  ] .

ns2:curie
  a ns2:Unit, ns2:SingularUnit ;
  rdfs:label "curie"@en, "curie"@nl ;
  rdfs:comment "The curie is a unit of activity defined as 3.7e10 becquerel."@en ;
  ns2:symbol "Ci" ;
  ns2:hasFactor "3.7e10"^^xsd:float ;
  ns2:hasUnit ns2:becquerel ;
  ns2:hasDimension ns2:frequency-Dimension .

ns2:PrefixedBecquerel
  a owl:Class ;
  rdfs:label "prefixed becquerel"@en ;
  rdfs:subClassOf ns2:PrefixedUnit ;
  owl:equivalentClass [
    a owl:Class ;
    owl:intersectionOf (
     _:genid1768
     _:genid1770
     _:genid1772
     _:genid1774
   )
  ] .

ns2:yoctobecquerel
  a ns2:PrefixedUnit ;
  rdfs:label "yoctobecquerel"@en, "yoctobecquerel"@nl ;
  rdfs:comment "The yoctobecquerel is a unit of activity defined as 1.0e-24 becquerel."@en ;
  ns2:symbol "yBq" ;
  ns2:hasPrefix ns2:yocto ;
  ns2:hasUnit ns2:becquerel ;
  ns2:hasDimension ns2:frequency-Dimension .

ns2:zeptobecquerel
  a ns2:PrefixedUnit ;
  rdfs:label "zeptobecquerel"@en, "zeptobecquerel"@nl ;
  rdfs:comment "The zeptbecquerel is a unit of activity defined as 1.0e-21 becquerel."@en ;
  ns2:symbol "zBq" ;
  ns2:hasPrefix ns2:zepto ;
  ns2:hasUnit ns2:becquerel ;
  ns2:hasDimension ns2:frequency-Dimension .

ns2:attobecquerel
  a ns2:PrefixedUnit ;
  rdfs:label "attobecquerel"@en, "attobecquerel"@nl ;
  rdfs:comment "The attobecquerel is a unit of activity defined as 1.0e-18 becquerel."@en ;
  ns2:symbol "aBq" ;
  ns2:hasPrefix ns2:atto ;
  ns2:hasUnit ns2:becquerel ;
  ns2:hasDimension ns2:frequency-Dimension .

ns2:femtobecquerel
  a ns2:PrefixedUnit ;
  rdfs:label "femtobecquerel"@en, "femtobecquerel"@nl ;
  rdfs:comment "The femtobecquerel is a unit of activity defined as 1.0e-15 becquerel."@en ;
  ns2:symbol "fBq" ;
  ns2:hasPrefix ns2:femto ;
  ns2:hasUnit ns2:becquerel ;
  ns2:hasDimension ns2:frequency-Dimension .

ns2:picobecquerel
  a ns2:PrefixedUnit ;
  rdfs:label "picobecquerel"@en, "picobecquerel"@nl ;
  rdfs:comment "The picobecquerel is a unit of activity defined as 1.0e-12 becquerel."@en ;
  ns2:symbol "pBq" ;
  ns2:hasPrefix ns2:pico ;
  ns2:hasUnit ns2:becquerel ;
  ns2:hasDimension ns2:frequency-Dimension .

ns2:nanobecquerel
  a ns2:PrefixedUnit ;
  rdfs:label "nanobecquerel"@en, "nanobecquerel"@nl ;
  rdfs:comment "The nanobecquerel is a unit of activity defined as 1.0e-9 becquerel."@en ;
  ns2:symbol "nBq" ;
  ns2:hasPrefix ns2:nano ;
  ns2:hasUnit ns2:becquerel ;
  ns2:hasDimension ns2:frequency-Dimension .

ns2:microbecquerel
  a ns2:PrefixedUnit ;
  rdfs:label "microbecquerel"@en, "microbecquerel"@nl ;
  rdfs:comment "The microbecquerel is a unit of activity defined as 1.0e-6 becquerel."@en ;
  ns2:symbol "μBq" ;
  ns2:hasPrefix ns2:micro ;
  ns2:hasUnit ns2:becquerel ;
  ns2:hasDimension ns2:frequency-Dimension .

ns2:millibecquerel
  a ns2:PrefixedUnit ;
  rdfs:label "millibecquerel"@en, "millibecquerel"@nl ;
  rdfs:comment "The millibecquerel is a unit of activity defined as 1.0e-3 becquerel."@en ;
  ns2:symbol "mBq" ;
  ns2:hasPrefix ns2:milli ;
  ns2:hasUnit ns2:becquerel ;
  ns2:hasDimension ns2:frequency-Dimension .

ns2:centibecquerel
  a ns2:PrefixedUnit ;
  rdfs:label "centibecquerel"@en, "centibecquerel"@nl ;
  rdfs:comment "The centibecquerel is a unit of activity defined as 1.0e-2 becquerel."@en ;
  ns2:symbol "cBq" ;
  ns2:hasPrefix ns2:centi ;
  ns2:hasUnit ns2:becquerel ;
  ns2:hasDimension ns2:frequency-Dimension .

ns2:decibecquerel
  a ns2:PrefixedUnit ;
  rdfs:label "decibecquerel"@en, "decibecquerel"@nl ;
  rdfs:comment "The decibecquerel is a unit of activity defined as 1.0e-1 becquerel."@en ;
  ns2:symbol "dBq" ;
  ns2:hasPrefix ns2:deci ;
  ns2:hasUnit ns2:becquerel ;
  ns2:hasDimension ns2:frequency-Dimension .

ns2:decabecquerel
  a ns2:PrefixedUnit ;
  rdfs:label "decabecquerel"@en, "decabecquerel"@nl ;
  rdfs:comment "The decabecquerel is a unit of activity defined as 1.0e1 becquerel."@en ;
  ns2:symbol "daBq" ;
  ns2:hasPrefix ns2:deca ;
  ns2:hasUnit ns2:becquerel ;
  ns2:hasDimension ns2:frequency-Dimension .

ns2:hectobecquerel
  a ns2:PrefixedUnit ;
  rdfs:label "hectobecquerel"@en, "hectobecquerel"@nl ;
  rdfs:comment "The hectobecquerel is a unit of activity defined as 1.0e2 becquerel."@en ;
  ns2:symbol "hBq" ;
  ns2:hasPrefix ns2:hecto ;
  ns2:hasUnit ns2:becquerel ;
  ns2:hasDimension ns2:frequency-Dimension .

ns2:kilobecquerel
  a ns2:PrefixedUnit ;
  rdfs:label "kilobecquerel"@en, "kilobecquerel"@nl ;
  rdfs:comment "The kilobecquerel is a unit of activity defined as 1.0e3 becquerel."@en ;
  ns2:symbol "kBq" ;
  ns2:hasPrefix ns2:kilo ;
  ns2:hasUnit ns2:becquerel ;
  ns2:hasDimension ns2:frequency-Dimension .

ns2:megabecquerel
  a ns2:PrefixedUnit ;
  rdfs:label "megabecquerel"@en, "megabecquerel"@nl ;
  rdfs:comment "The megabecquerel is a unit of activity defined as 1.0e6 becquerel."@en ;
  ns2:symbol "MBq" ;
  ns2:hasPrefix ns2:mega ;
  ns2:hasUnit ns2:becquerel ;
  ns2:hasDimension ns2:frequency-Dimension .

ns2:gigabecquerel
  a ns2:PrefixedUnit ;
  rdfs:label "gigabecquerel"@en, "gigabecquerel"@nl ;
  rdfs:comment "The gigabecquerel is a unit of activity defined as 1.0e9 becquerel."@en ;
  ns2:symbol "GBq" ;
  ns2:hasPrefix ns2:giga ;
  ns2:hasUnit ns2:becquerel ;
  ns2:hasDimension ns2:frequency-Dimension .

ns2:terabecquerel
  a ns2:PrefixedUnit ;
  rdfs:label "terabecquerel"@en, "terabecquerel"@nl ;
  rdfs:comment "The terabecquerel is a unit of activity defined as 1.0e12 becquerel."@en ;
  ns2:symbol "TBq" ;
  ns2:hasPrefix ns2:tera ;
  ns2:hasUnit ns2:becquerel ;
  ns2:hasDimension ns2:frequency-Dimension .

ns2:petabecquerel
  a ns2:PrefixedUnit ;
  rdfs:label "petabecquerel"@en, "petabecquerel"@nl ;
  rdfs:comment "The petabecquerel is a unit of activity defined as 1.0e15 becquerel."@en ;
  ns2:symbol "PBq" ;
  ns2:hasPrefix ns2:peta ;
  ns2:hasUnit ns2:becquerel ;
  ns2:hasDimension ns2:frequency-Dimension .

ns2:exabecquerel
  a ns2:PrefixedUnit ;
  rdfs:label "exabecquerel"@en, "exabecquerel"@nl ;
  rdfs:comment "The exabecquerel is a unit of activity defined as 1.0e18 becquerel."@en ;
  ns2:symbol "EBq" ;
  ns2:hasPrefix ns2:exa ;
  ns2:hasUnit ns2:becquerel ;
  ns2:hasDimension ns2:frequency-Dimension .

ns2:zettabecquerel
  a ns2:PrefixedUnit ;
  rdfs:label "zettabecquerel"@en, "zettabecquerel"@nl ;
  rdfs:comment "The zettabecquerel is a unit of activity defined as 1.0e21 becquerel."@en ;
  ns2:symbol "ZBq" ;
  ns2:hasPrefix ns2:zetta ;
  ns2:hasUnit ns2:becquerel ;
  ns2:hasDimension ns2:frequency-Dimension .

ns2:yottabecquerel
  a ns2:PrefixedUnit ;
  rdfs:label "yottabecquerel"@en, "yottabecquerel"@nl ;
  rdfs:comment "The yottabecquerel is a unit of activity defined as 1.0e24 becquerel."@en ;
  ns2:symbol "YBq" ;
  ns2:hasPrefix ns2:yotta ;
  ns2:hasUnit ns2:becquerel ;
  ns2:hasDimension ns2:frequency-Dimension .

ns2:coulombPerKilogram
  a ns2:UnitDivision ;
  rdfs:label "coulomb per kilogram"@en, "coulomb per kilogram"@nl ;
  ns2:symbol "C/kg" ;
  ns2:alternativeSymbol "C kg-1", "C·kg-1" ;
  ns2:hasNumerator ns2:coulomb ;
  ns2:hasDenominator ns2:kilogram ;
  ns2:hasDimension ns2:exposureToXAndGammaRays-Dimension .

ns2:röntgen
  a ns2:Unit, ns2:SingularUnit ;
  rdfs:label "röntgen"@en, "röntgen"@nl ;
  rdfs:comment "The röntgen is a unit of exposure to x and γ rays defined as 2.58e-4 coulomb per kilogram."@en ;
  ns2:symbol "R" ;
  ns2:hasFactor "2.58e-4"^^xsd:float ;
  ns2:hasUnit ns2:coulombPerKilogram ;
  ns2:hasDimension ns2:exposureToXAndGammaRays-Dimension .

ns2:ExposureToXAndGammaRaysUnit
  a owl:Class ;
  rdfs:label "exposure to x and γ rays unit"@en ;
  rdfs:subClassOf ns2:Unit ;
  owl:equivalentClass [
    a owl:Class ;
    owl:oneOf (
     ns2:röntgen
     ns2:coulombPerKilogram
   )
  ] .

ns2:grayPerSecond-Time
  a ns2:UnitDivision ;
  rdfs:label "gray per second"@en, "gray per seconde"@nl ;
  ns2:symbol "Gy/s" ;
  ns2:alternativeSymbol "Gy s-1", "Gy·s-1" ;
  ns2:hasNumerator ns2:gray ;
  ns2:hasDenominator ns2:second-Time ;
  ns2:hasDimension ns2:absorbedDoseRate-Dimension .

ns2:milligrayPerSecond-Time
  a ns2:UnitDivision ;
  rdfs:label "milligray per second"@en, "milligray per seconde"@nl ;
  ns2:symbol "mGy/s" ;
  ns2:alternativeSymbol "mGy s-1", "mGy·s-1" ;
  ns2:hasNumerator ns2:milligray ;
  ns2:hasDenominator ns2:second-Time ;
  ns2:hasDimension ns2:absorbedDoseRate-Dimension .

ns2:AbsorbedDoseRateUnit
  a owl:Class ;
  rdfs:label "absorbed dose rate unit"@en ;
  rdfs:subClassOf ns2:Unit ;
  owl:equivalentClass [
    a owl:Class ;
    owl:oneOf (
     ns2:grayPerSecond-Time
     ns2:milligrayPerSecond-Time
   )
  ] .

ns2:exposureToXAndGammaRays-Dimension
  a ns2:Dimension ;
  rdfs:label "exposure to x and γ rays dimension"@en ;
  ns2:hasSILengthDimensionExponent 0 ;
  ns2:hasSIMassDimensionExponent -1 ;
  ns2:hasSITimeDimensionExponent 1 ;
  ns2:hasSIElectricCurrentDimensionExponent 1 ;
  ns2:hasSIThermodynamicTemperatureDimensionExponent 0 ;
  ns2:hasSIAmountOfSubstanceDimensionExponent 0 ;
  ns2:hasSILuminousIntensityDimensionExponent 0 .

ns2:absorbedDoseRate-Dimension
  a ns2:Dimension ;
  rdfs:label "absorbed dose rate dimension"@en ;
  ns2:hasSILengthDimensionExponent 2 ;
  ns2:hasSIMassDimensionExponent 0 ;
  ns2:hasSITimeDimensionExponent -3 ;
  ns2:hasSIElectricCurrentDimensionExponent 0 ;
  ns2:hasSIThermodynamicTemperatureDimensionExponent 0 ;
  ns2:hasSIAmountOfSubstanceDimensionExponent 0 ;
  ns2:hasSILuminousIntensityDimensionExponent 0 .

ns2:radiance-Dimension
  a ns2:Dimension ;
  rdfs:label "radiance dimension"@en ;
  ns2:hasSILengthDimensionExponent 0 ;
  ns2:hasSIMassDimensionExponent 1 ;
  ns2:hasSITimeDimensionExponent -3 ;
  ns2:hasSIElectricCurrentDimensionExponent 0 ;
  ns2:hasSIThermodynamicTemperatureDimensionExponent 0 ;
  ns2:hasSIAmountOfSubstanceDimensionExponent 0 ;
  ns2:hasSILuminousIntensityDimensionExponent 0 .

ns2:Half-Life
  a owl:Class ;
  rdfs:label "half-life"@en ;
  rdfs:subClassOf ns2:Time ;
  ns2:symbol "t_½" ;
  ns2:LaTeXSymbol "T_{\\frac{1}{2}}" ;
  ns2:LaTeXCommand "\\Halflife" ;
  ns2:alternativeSymbol "t_1/2", "T_½", "τ_½" ;
  ns2:commonlyHasUnit ns2:second-Time, ns2:attosecond-Time, ns2:centisecond-Time, ns2:decasecond-Time, ns2:decisecond-Time, ns2:exasecond-Time, ns2:femtosecond-Time, ns2:gigasecond-Time, ns2:hectosecond-Time, ns2:kilosecond-Time, ns2:megasecond-Time, ns2:microsecond-Time, ns2:millisecond-Time, ns2:nanosecond-Time, ns2:petasecond-Time, ns2:picosecond-Time, ns2:terasecond-Time, ns2:day, ns2:hour, ns2:minute-Time, ns2:shake, ns2:year, ns2:day-Sidereal, ns2:gigayear, ns2:hour-Sidereal, ns2:minute-Sidereal, ns2:second-Sidereal, ns2:year-Sidereal, ns2:year-Tropical .

ns2:astronomyAndAstrophysics
  a ns2:ApplicationArea ;
  rdfs:label "astronomy and astrophysics"@en, "astronomie en astrofysica"@nl ;
  ns2:usesQuantity ns2:Aberration, ns2:AberrationInLatitude, ns2:AberrationInLongitude, ns2:AbsoluteMagnitude, ns2:AbsoluteBolometricMagnitude, ns2:Albedo, ns2:Altitude, ns2:Amplitude, ns2:VAmplitude, ns2:PhotographicAmplitude, ns2:AngularSize, ns2:AnnualAberration, ns2:ApparentDiameter, ns2:ApparentDistanceModulus, ns2:ApparentMagnitude, ns2:Azimuth, ns2:BMagnitude, ns2:BMagnitudeAtMaximumBrightness, ns2:BMagnitudeAtMinimumBrightness, ns2:BolometricCorrection, ns2:BolometricMagnitude, ns2:BondAlbedo, ns2:BrightnessTemperature, ns2:Co-RotationRadius, ns2:ColdGasMassFraction, ns2:ColourIndex, ns2:ColourTemperature, ns2:Cut-OffWavelength, ns2:DarkNoise, ns2:Declination, ns2:DetectiveQuantumEfficiency, ns2:Detectivity, ns2:Diameter-Angle, ns2:DistanceModulus, ns2:DiurnalAberration, ns2:DynamicRange, ns2:Eccentricity, ns2:EclipticLatitude, ns2:EclipticLongitude, ns2:ElectronTemperature, ns2:Ellipticity, ns2:Extinction, ns2:GalacticCylindricalPolarAngleCoordinate, ns2:GalacticLatitude, ns2:GalacticLongitude, ns2:GeometricalAlbedo, ns2:HourAngle, ns2:InitialMassFunction, ns2:IntegratedMagnitude, ns2:IntrinsicColourIndex, ns2:IonizationTemperature, ns2:JeansMass, ns2:LightTime, ns2:LimitingMagnitude, ns2:LuminosityFunction, ns2:Epoch, ns2:EpochAtMaximumBrightness, ns2:ExtinctionAtWavelength, ns2:ExtinctionAtWaveband, ns2:ExtinctionInV, ns2:ExtinctionInB, ns2:ExtinctionInU, ns2:Magnitude, ns2:MagnitudeAtMaximumBrightness, ns2:MagnitudeAtMinimumBrightness, ns2:Metallicity, ns2:NoiseEquivalentPower, ns2:NormalAlbedo, ns2:NormalisedDetectivity, ns2:PeakWavelength, ns2:PhotographicMagnitude, ns2:PhotographicMagnitudeAtMaximumBrightness, ns2:PhotographicMagnitudeAtMinimumBrightness, ns2:PlanetaryAberration, ns2:QuantumEfficiency, ns2:Radius-Angle, ns2:RedMagnitude, ns2:Reddening, ns2:ReddeningB-V, ns2:ReddeningU-B, ns2:Responsivity, ns2:RightAscension, ns2:ScaleHeight, ns2:ScaleLength, ns2:SecularAberration, ns2:SpectralResponse, ns2:StellarAberration, ns2:SupergalacticLatitude, ns2:SupergalacticLongitude, ns2:TimeConstant, ns2:TrueDistanceModulus, ns2:TychoBroadbandMagnitude, ns2:JohnsonMagnitude, ns2:StroemgrenMagnitude, ns2:CousinsMagnitude, ns2:ThuanAndGunnMagnitude, ns2:UMagnitude, ns2:VMagnitude, ns2:VMagnitudeAtMaximumBrightness, ns2:VMagnitudeAtMinimumBrightness, ns2:VisualAlbedo, ns2:WhiteLightMagnitude, ns2:WhiteLightMagnitudeAtMaximumBrightness, ns2:WhiteLightMagnitudeAtMinimumBrightness, ns2:ZenithDistance, ns2:_1040NanometreLockwoodMagnitude, ns2:uMagnitude, ns2:vMagnitude, ns2:bMagnitude, ns2:yMagnitude, ns2:BetaNarrowMagnitude, ns2:BetaWideMagnitude, ns2:IMagnitude, ns2:RMagnitude, ns2:gMagnitude ;
  ns2:usesUnit ns2:amperePerWatt, ns2:angstrom, ns2:bitPerSecond-Time, ns2:candelaPerSquareMetre, ns2:centimetre, ns2:cubicParsec, ns2:day, ns2:degreeSquared, ns2:gigaelectronvolt, ns2:gigaparsec, ns2:hour-HourAngle, ns2:jansky, ns2:kelvin, ns2:kiloelectronvolt, ns2:kiloparsec, ns2:kilometrePerSecond-TimePerMegaparsec, ns2:lightYear, ns2:magnitude, ns2:magnitudePerSecond-AngleSquared, ns2:megaelectronvolt, ns2:megaparsec, ns2:metreKilogramPerSecond-Time, ns2:metrePerSecond-TimePerMetre, ns2:micromagnitude, ns2:microsecond-Angle, ns2:millimagnitude, ns2:millisecond-Angle, ns2:millisecond-AnglePerYear, ns2:minute-HourAngle, ns2:minute-Angle, ns2:nanometre, ns2:one, ns2:percent, ns2:radian, ns2:reciprocalCubicMetre, ns2:reciprocalCubicParsec, ns2:second-HourAngle, ns2:second-Angle, ns2:second-AngleSquared, ns2:second-Time, ns2:solarMass, ns2:solarMassPerCubicParsec, ns2:solarMassPerGigayearCubicKiloparsec, ns2:solarMassPerGigayearCubicParsec, ns2:solarLuminosity, ns2:solarRadius, ns2:voltPerWatt, ns2:watt, ns2:wattPerCubicmetre, ns2:wattPerHertz, ns2:wattPerNanometre, ns2:wattPerSecond-AngleSquared, ns2:wattPerSquareMetreHertz, ns2:wattPerSquareMetreNanometre, ns2:wattPerSteradianSquareMetre, ns2:wattPerSteradianSquareMetreHertz, ns2:year .

ns2:Co-RotationRadius
  a owl:Class ;
  rdfs:label "co-rotation radius"@en ;
  rdfs:subClassOf ns2:Radius ;
  rdfs:comment "The radius (distance from the galaxy's centre) at which the stars move at the same speed as the spiral pattern or bar in a galaxy."@en ;
  ns2:symbol "r_c" ;
  ns2:commonlyHasUnit ns2:parsec, ns2:astronomicalUnit, ns2:lightYear, ns2:kiloparsec .

ns2:Cut-OffWavelength
  a owl:Class ;
  rdfs:label "cut-off wavelength"@en ;
  rdfs:comment "Either: wavelengths at which the detectivity (D) falls to 0, or the wavelengths at which the detectivity falls to 1% of the peak value, or the wavelengths at which the normalised detectivity (D*) has fallen to half its peak value."@en ;
  rdfs:subClassOf ns2:Wavelength ;
  ns1:reference ns1:Astrophysical_Techniques_chapter1 ;
  ns2:symbol "λ_c" ;
  ns2:commonlyHasUnit ns2:metre, ns2:attometre, ns2:centimetre, ns2:decametre, ns2:decimetre, ns2:exametre, ns2:femtometre, ns2:gigametre, ns2:hectometre, ns2:kilometre, ns2:megametre, ns2:micrometre, ns2:millimetre, ns2:nanometre, ns2:petametre, ns2:picometre, ns2:terametre, ns2:angstrom, ns2:chain, ns2:fathom-USSurvey, ns2:fermi, ns2:foot-International, ns2:foot-USSurvey, ns2:furlong-International, ns2:inch-International, ns2:micron, ns2:mil-Length, ns2:mile-Statute, ns2:mile-USSurvey, ns2:nauticalMile-International, ns2:rod-US, ns2:yard-International, ns2:astronomicalUnit, ns2:lightYear, ns2:parsec, ns2:solarRadius, ns2:gigaparsec, ns2:kiloparsec, ns2:megaparsec, ns2:cicero, ns2:pica-ATA, ns2:pica-Postscript, ns2:pica-TeX, ns2:point-ATA, ns2:point-Didot, ns2:point-Postscript, ns2:point-TeX .

ns2:PeakWavelength
  a owl:Class ;
  rdfs:label "peak wavelength"@en ;
  rdfs:comment "Wavelength for which the detectivity is at a maximum."@en ;
  rdfs:subClassOf ns2:Wavelength ;
  ns2:symbol "λ_m" ;
  ns1:reference ns1:Astrophysical_Techniques_chapter1 ;
  ns2:commonlyHasUnit ns2:metre, ns2:attometre, ns2:centimetre, ns2:decametre, ns2:decimetre, ns2:exametre, ns2:femtometre, ns2:gigametre, ns2:hectometre, ns2:kilometre, ns2:megametre, ns2:micrometre, ns2:millimetre, ns2:nanometre, ns2:petametre, ns2:picometre, ns2:terametre, ns2:angstrom, ns2:chain, ns2:fathom-USSurvey, ns2:fermi, ns2:foot-International, ns2:foot-USSurvey, ns2:furlong-International, ns2:inch-International, ns2:micron, ns2:mil-Length, ns2:mile-Statute, ns2:mile-USSurvey, ns2:nauticalMile-International, ns2:rod-US, ns2:yard-International, ns2:astronomicalUnit, ns2:lightYear, ns2:parsec, ns2:solarRadius, ns2:gigaparsec, ns2:kiloparsec, ns2:megaparsec, ns2:cicero, ns2:pica-ATA, ns2:pica-Postscript, ns2:pica-TeX, ns2:point-ATA, ns2:point-Didot, ns2:point-Postscript, ns2:point-TeX .

ns2:ScaleHeight
  a owl:Class ;
  rdfs:label "scale height"@en ;
  rdfs:comment "The scale height of a feature (such as the thin galactic disk) is the height (or position) at which the number density of the feature (for instance of the number of Population II stars) is equal to 1/e times the number density at the origin (for instance the Galactic Plane)."@en ;
  rdfs:subClassOf ns2:Length ;
  ns2:symbol "h_z" ;
  ns2:commonlyHasUnit ns2:parsec, ns2:kiloparsec .

ns2:ScaleLength
  a owl:Class ;
  rdfs:label "scale length"@en ;
  ns2:alternativeLabel "scale radius"@en ;
  rdfs:comment "The radial distance from a galaxy's core at which the average intensity has fallen to 1/e of the intensity at the centre of the galaxy."@en ;
  rdfs:subClassOf ns2:Length ;
  ns2:symbol "r" ;
  ns2:commonlyHasUnit ns2:kiloparsec .

ns2:Epoch
  a owl:Class ;
  rdfs:label "epoch"@en ;
  rdfs:subClassOf ns2:Date ;
  ns2:commonlyHasUnit ns2:second-Time, ns2:year .

ns2:EpochAtMaximumBrightness
  a owl:Class ;
  rdfs:label "epoch at maximum brightness"@en ;
  rdfs:comment "A moment when the object (i.e. a variable star) was at maximum brightness."@en ;
  rdfs:subClassOf ns2:Epoch ;
  ns2:commonlyHasUnit ns2:second-Time, ns2:year .

ns2:PeriodOfVariability
  a owl:Class ;
  rdfs:label "period of variability"@en ;
  rdfs:comment "The duration of one cycle in a (semi) periodical star."@en ;
  rdfs:subClassOf ns2:Time ;
  ns2:symbol "P" ;
  ns2:commonlyHasUnit ns2:second-Time, ns2:attosecond-Time, ns2:centisecond-Time, ns2:decasecond-Time, ns2:decisecond-Time, ns2:exasecond-Time, ns2:femtosecond-Time, ns2:gigasecond-Time, ns2:hectosecond-Time, ns2:kilosecond-Time, ns2:megasecond-Time, ns2:microsecond-Time, ns2:millisecond-Time, ns2:nanosecond-Time, ns2:petasecond-Time, ns2:picosecond-Time, ns2:terasecond-Time, ns2:day, ns2:hour, ns2:minute-Time, ns2:shake, ns2:year, ns2:day-Sidereal, ns2:gigayear, ns2:hour-Sidereal, ns2:minute-Sidereal, ns2:second-Sidereal, ns2:year-Sidereal, ns2:year-Tropical .

ns2:LightTime
  a owl:Class ;
  rdfs:label "light time"@en ;
  rdfs:comment "The time electromagnetic radiation takes to reach Earth from a distant source. Often the correction in light time is needed to accurately calculate the apparent position of solar system objects or to calculate the period of variable stars (different times are observed when the Earth is at a different position in its orbit)."@en ;
  rdfs:subClassOf ns2:Time ;
  ns2:symbol "τ" ;
  ns2:commonlyHasUnit ns2:second-Time .

ns2:TimeConstant
  a owl:Class ;
  rdfs:label "time constant"@en ;
  rdfs:comment "Time required to approach (1-1/e) of the final output value of a detector (about 63%) (Kitchin, Astrophysical Techniques, IoP, Table 1.1.2)."@en ;
  rdfs:subClassOf ns2:Time ;
  ns2:symbol "τ" ;
  ns2:commonlyHasUnit ns2:second-Time .

ns2:JeansMass
  a owl:Class ;
  rdfs:label "Jeans mass"@en ;
  rdfs:comment "The critical mass of a molecular cloud, above which it will be unstable to collapse."@en ;
  rdfs:subClassOf ns2:Mass ;
  ns2:symbol "M_J" ;
  ns2:commonlyHasUnit ns2:kilogram, ns2:solarMass .

ns2:BrightnessTemperature
  a owl:Class ;
  rdfs:label "brightness temperature"@en ;
  rdfs:comment "The temperature that a blackbody would need to have in order to emit radiation of the observed intensity at a given wavelength (mostly used in radio astronomy)."@en ;
  rdfs:subClassOf ns2:ThermodynamicTemperature ;
  ns2:commonlyHasUnit ns2:kelvin .

ns2:ColourTemperature
  a owl:Class ;
  rdfs:label "colour temperature"@en ;
  rdfs:comment "The temperature of a blackbody that has the same colour index as a given star."@en ;
  rdfs:subClassOf ns2:ThermodynamicTemperature ;
  ns2:commonlyHasUnit ns2:kelvin .

ns2:ElectronTemperature
  a owl:Class ;
  rdfs:label "electron temperature"@en ;
  ns2:alternativeLabel "kinetic temperature"@en ;
  rdfs:comment "The temperature determined by the mean kinetic energy of free electrons in a plasma; also known as kinetic temperature."@en ;
  rdfs:subClassOf ns2:ThermodynamicTemperature ;
  ns2:symbol "T_e" ;
  ns2:alternativeSymbol "T_k" ;
  ns2:commonlyHasUnit ns2:kelvin .

ns2:IonizationTemperature
  a owl:Class ;
  rdfs:label "ionization temperature"@en ;
  rdfs:comment "The temperature of a gas or plasma derived from the relative numbers of neutral atoms and ions. Specifically, it is the temperature for which the Saha equations would predict these relative numbers, assuming the atoms and ions are in thermodynamic equilibrium."@en ;
  rdfs:subClassOf ns2:ThermodynamicTemperature ;
  ns2:symbol "T_ion" ;
  ns2:commonlyHasUnit ns2:kelvin .

ns2:Albedo
  a owl:Class ;
  rdfs:label "albedo"@en, "albedo"@nl ;
  rdfs:comment "Ratio between radiation falling onto an object and the radiation reflected or scattered back. Or the ratio between the illumination and observed brightness."@en ;
  rdfs:subClassOf ns2:QuantityOfDimensionOne ;
  ns2:symbol "α" ;
  ns2:commonlyHasUnit ns2:one .

ns2:NormalAlbedo
  a owl:Class ;
  rdfs:label "normal albedo"@en ;
  rdfs:comment "Ratio between radiation falling vertically onto an object and the radiation radiated back vertically."@en ;
  rdfs:subClassOf ns2:Albedo ;
  ns2:commonlyHasUnit ns2:one .

ns2:VisualAlbedo
  a owl:Class ;
  rdfs:label "visual albedo"@en ;
  rdfs:comment "The albedo only for radiation in the visual part of the spectrum."@en ;
  rdfs:subClassOf ns2:Albedo ;
  ns2:commonlyHasUnit ns2:one .

ns2:GeometricalAlbedo
  a owl:Class ;
  rdfs:label "geometrical albedo"@en ;
  ns2:alternativeLabel "astronomical albedo"@en, "physical albedo"@en ;
  rdfs:comment "Ratio between the brightness of an object as seen from the direction of a hypothetical white, diffusely reflecting sphere of the same size and at the same distance."@en ;
  rdfs:subClassOf ns2:Albedo ;
  ns2:symbol "A" ;
  ns2:commonlyHasUnit ns2:one .

ns2:BondAlbedo
  a owl:Class ;
  rdfs:label "bond albedo"@en ;
  ns2:alternativeLabel "spherical albedo"@en ;
  rdfs:comment "Is the fraction of the total incident solar radiation - the radiation at all wavelengths - that is reflected or scattered by an object in all directions."@en ;
  rdfs:subClassOf ns2:Albedo ;
  ns2:commonlyHasUnit ns2:one .

ns2:Ellipticity
  a owl:Class ;
  rdfs:label "ellipticity"@en ;
  ns2:alternativeLabel "oblateness"@en, "flattening"@en ;
  rdfs:comment "A measure of the amount by which an object, such as a planet or a galaxy, deviates from a perfect sphere."@en ;
  rdfs:subClassOf ns2:QuantityOfDimensionOne ;
  ns2:symbol "f" ;
  ns2:commonlyHasUnit ns2:one .

ns2:Eccentricity
  a owl:Class ;
  rdfs:label "eccentricity"@en, "eccentriciteit"@nl ;
  rdfs:comment "A measure of the deviation from a circle for an orbit."@en ;
  rdfs:subClassOf ns2:QuantityOfDimensionOne ;
  ns2:symbol "e" ;
  ns2:commonlyHasUnit ns2:one .

ns2:Metallicity
  a owl:Class ;
  rdfs:label "metallicity"@en ;
  rdfs:comment "The log of the ratio between the ratios of the observed Fe and H quantities in a star and the same ratio in the Sun. This is a very important quantity that is often used in astronomy as an indicator of the age of a star."@en ;
  rdfs:subClassOf ns2:QuantityOfDimensionOne ;
  ns2:commonlyHasUnit ns2:one .

ns2:DynamicRange
  a owl:Class ;
  ns2:commonlyHasUnit ns2:one ;
  rdfs:subClassOf [
    a owl:Restriction ;
    owl:onProperty ns2:hasValue ;
    owl:allValuesFrom [
      a owl:Restriction ;
      owl:onProperty ns2:hasUnit ;
      owl:allValuesFrom ns2:DynamicRangeUnit
    ]
  ], ns2:Quantity, [
    a owl:Restriction ;
    owl:onProperty ns2:hasDimension ;
    owl:hasValue ns2:dimensionOne
  ] ;
  rdfs:label "dynamic range"@en ;
  rdfs:comment "Ratio between the saturation output and the dark signal, sometimes only over the region of linearity."@en ;
  ns1:reference ns1:Astrophysical_Techniques_chapter1 .

ns2:QuantumEfficiency
  a owl:Class ;
  ns2:commonlyHasUnit ns2:one ;
  rdfs:subClassOf [
    a owl:Restriction ;
    owl:onProperty ns2:hasValue ;
    owl:allValuesFrom [
      a owl:Restriction ;
      owl:onProperty ns2:hasUnit ;
      owl:allValuesFrom ns2:QuantumEfficiencyUnit
    ]
  ], ns2:Quantity, [
    a owl:Restriction ;
    owl:onProperty ns2:hasDimension ;
    owl:hasValue ns2:dimensionOne
  ] ;
  rdfs:label "quantum efficiency"@en ;
  rdfs:comment "Ratio (of a detector such as a CCD) of actual number of detected photons and the number of incident photons."@en ;
  ns2:symbol "QE" ;
  ns1:reference ns1:Astrophysical_Techniques_chapter1 .

ns2:TotalDensityParameter
  a owl:Class ;
  ns2:commonlyHasUnit ns2:one ;
  rdfs:label "total density parameter"@en ;
  rdfs:comment "The total density parameter."@en ;
  rdfs:subClassOf ns2:DensityParameter ;
  ns2:symbol "Ω_T" .

ns2:Magnitude
  a owl:Class ;
  ns2:commonlyHasUnit ns2:one, ns2:magnitude, ns2:millimagnitude, ns2:micromagnitude ;
  rdfs:label "magnitude"@en, "magnitude"@nl ;
  rdfs:comment "Reverse logarithmic measure of the brightness of an object."@en ;
  ns2:longcomment """The magnitude scale was originally created by Hipparchos of Nicea (160-127 BCE) and was measured by comparing the brightness between stars. Initially this was done inaccurately by eye but is currently done by using photoelectric photometers or even more recently by CCDs. Hipparchos divided the stars into six magnitude (brightness classes), the brightest stars being assigned to the first class and the faintest to the sixth class. By about the middle 1800s it became apparent that the traditional magnitude scale is close to a logarithmic scale with base 2.5. This is due to the fact that the response of the eye is nearly logarithmic. N.R. Pogson formalised the magnitude scale to closely match the traditional (visual) scale. It is now defined as:  
    <math xmlns="http://www.w3.org/1998/Math/MathML" ="block">
   		<msub><mi>m</mi><mn>1</mn></msub> <mo>-</mo> <msub><mi>m</mi><mn>2</mn>  </msub><mo>=</mo> 
   		<mn>-2.5</mn><mi>log</mi>
    	<mfrac ="1">
    		<mrow>
    			<msub><mi>f</mi><mn>1</mn></msub>
    		</mrow>
    		<mrow><msub><mi>f</mi><mn>2</mn></msub>
    		</mrow>
    	</mfrac>
    </math>
    where <math ="inline"><msub><mi>m</mi><mn>1</mn></msub> <mo>-</mo> <msub><mi>m</mi><mn>2</mn>  </msub></math> is the magnitude difference between two objects, and <math ="inline"><msub><mi>f</mi><mn>1</mn></msub></math> and <math ="inline"><msub><mi>f</mi><mn>2</mn></msub></math> are the luminous fluxes of the two objects. The magnitude of Vega (α Lyrae, HD 172167) is defined to be 0 in all wavelengths and passbands, although in practice this can only be an approximation. The zero point is now defined using multiple standard stars from the north polar sequence (non-variable stars within 2 degrees of the north celestial pole) or secondary standard stars from other parts of the sky. Please note that the scale is inverted, objects of magnitude 1 have a higher luminous flux than objects of magnitude 5. Stars of magnitude 6 are just visible to the naked eye under good observing conditions.
    The units of magnitude, also called magnitude, are usually not indicated except when indicating small magnitude differences when milli- or micromagnitudes are used."""^^rdf:XMLLiteral ;
  rdfs:subClassOf ns2:Quantity, [
    a owl:Restriction ;
    owl:onProperty ns2:hasDimension ;
    owl:hasValue ns2:dimensionOne
  ], [
    a owl:Restriction ;
    owl:onProperty ns2:hasValue ;
    owl:allValuesFrom [
      a owl:Restriction ;
      owl:onProperty ns2:hasUnit ;
      owl:allValuesFrom ns2:MagnitudeUnit
    ]
  ] ;
  ns2:symbol "m" ;
  ns1:reference ns1:Astrophysical_Techniques_chapter3, ns1:IntroAstronomicalPhotometry_chapter_2 .

ns2:AbsoluteMagnitude
  a owl:Class ;
  ns2:commonlyHasUnit ns2:one, ns2:magnitude, ns2:millimagnitude, ns2:micromagnitude ;
  rdfs:label "absolute magnitude"@en, "absolute magnitude"@nl ;
  rdfs:comment "Logarithmic measure of the brightness of an object as seen from a standard distance of 10 pc. Units usually not indicated (http://en.wikipedia.org/wiki/Magnitude_(astronomy)."@en ;
  rdfs:subClassOf ns2:Magnitude ;
  ns2:symbol "M" .

ns2:ApparentMagnitude
  a owl:Class ;
  ns2:commonlyHasUnit ns2:one, ns2:magnitude, ns2:millimagnitude, ns2:micromagnitude ;
  rdfs:label "apparent magnitude"@en, "schijnbare magnitude"@nl ;
  rdfs:comment "Logarithmic measure of the apparent brightness of an object. Units usually not indicated(http://en.wikipedia.org/wiki/Magnitude_(astronomy)."@en ;
  rdfs:subClassOf ns2:Magnitude ;
  ns2:symbol "m" .

ns2:BMagnitude
  a owl:Class ;
  ns2:commonlyHasUnit ns2:one, ns2:magnitude, ns2:millimagnitude, ns2:micromagnitude ;
  rdfs:label "B magnitude"@en ;
  rdfs:comment "Johnson B magnitude. The Johnson B band is a standard filter in the blue area. The central wavelength is 440nm and the bandwidth is 100nm.  The filter to be used is the Corning 5030 filter plus the Schott GG13 filter."@en ;
  rdfs:subClassOf ns2:JohnsonMagnitude ;
  ns2:symbol "B" ;
  ns2:alternativeSymbol "m_B" ;
  ns1:reference ns1:Astrophysical_Techniques_chapter3 .

ns2:BMagnitudeAtMaximumBrightness
  a owl:Class ;
  ns2:commonlyHasUnit ns2:one, ns2:magnitude ;
  rdfs:label "B magnitude at maximum brightness"@en ;
  rdfs:comment "Johnson B magnitude at maximum brightness (i.e. for a variable star). The Johnson B band is a standard filter in the blue area. The central wavelength is 440nm and the bandwidth is 100nm.  The filter to be used is the Corning 5030 filter plus the Schott GG13 filter."@en ;
  rdfs:subClassOf ns2:BMagnitude, ns2:MagnitudeAtMaximumBrightness ;
  ns2:symbol "B_max" ;
  ns1:reference ns1:Astrophysical_Techniques_chapter3 .

ns2:BMagnitudeAtMinimumBrightness
  a owl:Class ;
  ns2:commonlyHasUnit ns2:one, ns2:magnitude ;
  rdfs:label "B magnitude at minimum brightness"@en ;
  rdfs:comment "Johnson B magnitude at minimum brightness (i.e. for a variable star). The Johnson B band is a standard filter in the blue area. The central wavelength is 440nm and the bandwidth is 100nm.  The filter to be used is the Corning 5030 filter plus the Schott GG13 filter."@en ;
  rdfs:subClassOf ns2:BMagnitude, ns2:MagnitudeAtMinimumBrightness ;
  ns2:symbol "B_min" ;
  ns1:reference ns1:Astrophysical_Techniques_chapter3 .

ns2:MagnitudeAtMaximumBrightness
  a owl:Class ;
  ns2:commonlyHasUnit ns2:one, ns2:magnitude ;
  rdfs:label "magnitude at maximum brightness"@en ;
  rdfs:comment "The magnitude at maximum brightness of a variable star."@en ;
  rdfs:subClassOf ns2:Magnitude ;
  ns2:symbol "m_max" .

ns2:MagnitudeAtMinimumBrightness
  a owl:Class ;
  ns2:commonlyHasUnit ns2:one, ns2:magnitude ;
  rdfs:label "magnitude at minimum brightness"@en ;
  rdfs:comment "The magnitude at minimum brightness of a variable star."@en ;
  rdfs:subClassOf ns2:Magnitude ;
  ns2:symbol "m_min" .

ns2:PhotographicMagnitude
  a owl:Class ;
  ns2:commonlyHasUnit ns2:one, ns2:magnitude ;
  rdfs:label "photographic magnitude"@en ;
  rdfs:subClassOf ns2:Magnitude ;
  ns2:symbol "m_photo" .

ns2:PhotographicMagnitudeAtMaximumBrightness
  a owl:Class ;
  ns2:commonlyHasUnit ns2:one, ns2:magnitude ;
  rdfs:label "photographic magnitude at maximum brightness"@en ;
  rdfs:subClassOf ns2:PhotographicMagnitude, ns2:MagnitudeAtMaximumBrightness ;
  ns2:symbol "m_p,max" .

ns2:PhotographicMagnitudeAtMinimumBrightness
  a owl:Class ;
  ns2:commonlyHasUnit ns2:one, ns2:magnitude ;
  rdfs:label "photographic magnitude at minimum brightness"@en ;
  rdfs:subClassOf ns2:PhotographicMagnitude, ns2:MagnitudeAtMinimumBrightness ;
  ns2:symbol "m_p,min" .

ns2:UMagnitude
  a owl:Class ;
  ns2:commonlyHasUnit ns2:one, ns2:magnitude, ns2:millimagnitude, ns2:micromagnitude ;
  rdfs:label "U magnitude"@en ;
  rdfs:comment "Johnson U magnitude. The Johnson U band is a standard passband in the ultraviolet area. The central wavelength is 365nm and the bandwidth is 70nm.  The filter to be used is the Corning 9863 filter."@en ;
  rdfs:subClassOf ns2:JohnsonMagnitude ;
  ns2:symbol "U" ;
  ns2:alternativeSymbol "m_U" ;
  ns1:reference ns1:Astrophysical_Techniques_chapter3 .

ns2:VMagnitude
  a owl:Class ;
  ns2:commonlyHasUnit ns2:one, ns2:magnitude, ns2:millimagnitude, ns2:micromagnitude ;
  rdfs:label "V magnitude"@en ;
  rdfs:comment "Johnson V magnitude. The Johnson V band is a standard passband in the visual area, matching the response curve of the human eye. The central wavelength is 550nm and the bandwidth is 90nm.  The filter to be used is the Corning 3384 filter."@en ;
  rdfs:subClassOf ns2:JohnsonMagnitude ;
  ns2:symbol "V" ;
  ns2:alternativeSymbol "m_V" ;
  ns1:reference ns1:Astrophysical_Techniques_chapter3 .

ns2:VMagnitudeAtMaximumBrightness
  a owl:Class ;
  ns2:commonlyHasUnit ns2:one, ns2:magnitude ;
  rdfs:label "V magnitude at maximum brightness"@en ;
  rdfs:comment "Johnson V magnitude (apparent) at maximum brightness (i.e. for a variable star). The Johnson V band is a standard filter in the visual area, matching the response curve of the human eye. The central wavelength is 550nm and the bandwidth is 90nm.  The filter to be used is the Corning 3384 filter."@en ;
  rdfs:subClassOf ns2:VMagnitude, ns2:MagnitudeAtMaximumBrightness ;
  ns2:symbol "V_max" ;
  ns1:reference ns1:Astrophysical_Techniques_chapter3 .

ns2:VMagnitudeAtMinimumBrightness
  a owl:Class ;
  ns2:commonlyHasUnit ns2:one, ns2:magnitude ;
  rdfs:label "V magnitude at minimum brightness"@en ;
  rdfs:comment "Johnson V magnitude (apparent) at minimum brightness (i.e. for a variable star). The Johnson V band is a standard filter in the visual area, matching the response curve of the human eye. The central wavelength is 550nm and the bandwidth is 90nm.  The filter to be used is the Corning 3384 filter."@en ;
  rdfs:subClassOf ns2:VMagnitude, ns2:MagnitudeAtMinimumBrightness ;
  ns2:symbol "V_min" ;
  ns1:reference ns1:Astrophysical_Techniques_chapter3 .

ns2:WhiteLightMagnitude
  a owl:Class ;
  ns2:commonlyHasUnit ns2:one, ns2:magnitude ;
  rdfs:label "white light magnitude"@en ;
  rdfs:subClassOf ns2:Magnitude ;
  ns2:symbol "m" .

ns2:WhiteLightMagnitudeAtMaximumBrightness
  a owl:Class ;
  ns2:commonlyHasUnit ns2:one, ns2:magnitude ;
  rdfs:label "white light magnitude at maximum brightness"@en ;
  rdfs:subClassOf ns2:WhiteLightMagnitude, ns2:MagnitudeAtMaximumBrightness ;
  ns2:symbol "m_max" .

ns2:WhiteLightMagnitudeAtMinimumBrightness
  a owl:Class ;
  ns2:commonlyHasUnit ns2:one, ns2:magnitude ;
  rdfs:label "white light magnitude at minimum brightness"@en ;
  rdfs:subClassOf ns2:WhiteLightMagnitude, ns2:MagnitudeAtMinimumBrightness ;
  ns2:symbol "m_min" .

ns2:DetectiveQuantumEfficiency
  a owl:Class ;
  ns2:commonlyHasUnit ns2:one ;
  rdfs:label "detective quantum efficiency"@en ;
  rdfs:comment "Square of ratio between the output signal noise ratio and the input signal noise ratio."@en ;
  rdfs:subClassOf ns2:QuantumEfficiency ;
  ns2:symbol "DQE" ;
  ns1:reference ns1:Astrophysical_Techniques_chapter1 .

ns2:DynamicRangeUnit
  a owl:Class ;
  rdfs:label "dynamic range unit"@en ;
  rdfs:subClassOf ns2:Unit ;
  owl:equivalentClass [
    a owl:Class ;
    owl:oneOf ( ns2:one )
  ] .

ns2:QuantumEfficiencyUnit
  a owl:Class ;
  rdfs:label "quantum efficiency unit"@en ;
  rdfs:subClassOf ns2:Unit ;
  owl:equivalentClass [
    a owl:Class ;
    owl:oneOf ( ns2:one )
  ] .

ns2:Radius-Angle
  a owl:Class ;
  rdfs:label "radius (angle)"@en, "radius (hoek)"@nl ;
  rdfs:subClassOf ns2:Angle ;
  ns2:commonlyHasUnit ns2:degree, ns2:microsecond-Angle, ns2:millisecond-Angle, ns2:minute-Angle, ns2:second-Angle .

ns2:Diameter-Angle
  a owl:Class ;
  rdfs:label "diameter (angle)"@en, "diameter (hoek)"@nl ;
  rdfs:subClassOf ns2:Angle ;
  ns2:commonlyHasUnit ns2:degree, ns2:microsecond-Angle, ns2:millisecond-Angle, ns2:minute-Angle, ns2:second-Angle .

ns2:Altitude
  a owl:Class ;
  rdfs:label "altitude"@en ;
  ns2:alternativeLabel "elevation"@en ;
  rdfs:comment "The angular distance of a celestial body above or below the horizon, measured along the great circle passing through the body and the zenith."@en ;
  rdfs:subClassOf ns2:Angle ;
  ns2:symbol "h" ;
  ns2:alternativeSymbol "Alt" ;
  ns1:reference ns1:Glossary_Astronomical_Almanac ;
  ns2:commonlyHasUnit ns2:degree, ns2:minute-Angle, ns2:second-Angle .

ns2:ApparentDiameter
  a owl:Class ;
  rdfs:label "apparent diameter"@en ;
  rdfs:comment "The angle that the actual diameter of an object makes in the sky; also known as angular size. Most often small, so units are mostly arcminutes, arcseconds, or even milli- or microarcseconds."@en ;
  rdfs:subClassOf ns2:Angle ;
  ns2:commonlyHasUnit ns2:degree, ns2:minute-Angle, ns2:second-Angle, ns2:millisecond-Angle, ns2:microsecond-Angle, ns2:radian .

ns2:Azimuth
  a owl:Class ;
  rdfs:label "azimuth"@en, "azimut"@nl ;
  rdfs:comment "The angular distance measured clockwise along the horizon from a specified reference point (usually north) to the intersection with the great circle drawn from the zenith through a body on the celestial sphere."@en ;
  rdfs:subClassOf ns2:Angle ;
  ns2:symbol "A" ;
  ns2:alternativeSymbol "Az" ;
  ns1:reference ns1:Glossary_Astronomical_Almanac ;
  ns2:commonlyHasUnit ns2:degree, ns2:minute-Angle, ns2:second-Angle .

ns2:Declination
  a owl:Class ;
  rdfs:label "declination"@en, "declinatie"@nl ;
  rdfs:comment "The angular distance on the celestial sphere north or south of the celestial equator. It is measured along the hour circle passing through the celestial object. Declination is usually given in combination with right ascension or hour angle."@en ;
  rdfs:subClassOf ns2:Angle ;
  ns2:symbol "δ" ;
  ns2:alternativeSymbol "dec" ;
  ns1:reference ns1:Glossary_Astronomical_Almanac ;
  ns2:commonlyHasUnit ns2:degree, ns2:minute-Angle, ns2:second-Angle .

ns2:EclipticLatitude
  a owl:Class ;
  rdfs:label "ecliptic latitude"@en ;
  rdfs:comment "The angular distance on the celestial sphere north or south of the ecliptic (the path of the Sun on the celestial sphere during one year). It is measured along the great circle passing through the object and the ecliptic poles and perpendicular to the ecliptic."@en ;
  rdfs:subClassOf ns2:Angle ;
  ns2:symbol "β" ;
  ns1:reference ns1:chapter13_Astronomical_Algorithms ;
  ns2:commonlyHasUnit ns2:degree, ns2:minute-Angle, ns2:second-Angle .

ns2:EclipticLongitude
  a owl:Class ;
  rdfs:label "ecliptic longitude"@en ;
  rdfs:comment "The angular distance on the celestial sphere measured clockwise from the vernal equinox along the ecliptic (the path of the Sun on the celestial sphere during one year) to the intersection with the great circle drawn from the ecliptical north pole through the object."@en ;
  rdfs:subClassOf ns2:Angle ;
  ns2:symbol "λ" ;
  ns1:reference ns1:chapter13_Astronomical_Algorithms ;
  ns2:commonlyHasUnit ns2:degree, ns2:minute-Angle, ns2:second-Angle .

ns2:GalacticCylindricalPolarAngleCoordinate
  a owl:Class ;
  rdfs:label "galactic cylindrical polar angle coordinate"@en ;
  rdfs:comment "The angle from the Galactic centre between the perpendicular projection of the Sun on the Galactic plane and the projection of the object. This is one of the three Galactic Cylindrical Polar Coordinates."@en ;
  rdfs:subClassOf ns2:Angle ;
  ns2:symbol "φ" ;
  ns2:commonlyHasUnit ns2:degree, ns2:radian .

ns2:GalacticLatitude
  a owl:Class ;
  rdfs:label "galactic latitude"@en ;
  rdfs:comment "The angular distance on the celestial sphere north or south of the galactic equator. It is measured along the great circle passing through the object and the galactic poles and perpendicular to the galactic equator."@en ;
  rdfs:subClassOf ns2:Angle ;
  ns2:symbol "b" ;
  ns1:reference ns1:chapter13_Astronomical_Algorithms ;
  ns2:commonlyHasUnit ns2:degree, ns2:minute-Angle, ns2:second-Angle .

ns2:GalacticLongitude
  a owl:Class ;
  rdfs:label "galactic longitude"@en ;
  rdfs:comment "The angular distance on the celestial sphere measured clockwise from the galactic centre (as defined by the International Astronomical Union (IAU)) along the galactic equator to the intersection with the great circle drawn from the galactic north pole through the object."@en ;
  rdfs:subClassOf ns2:Angle ;
  ns2:symbol "l" ;
  ns1:reference ns1:chapter13_Astronomical_Algorithms ;
  ns2:commonlyHasUnit ns2:degree, ns2:minute-Angle, ns2:second-Angle .

ns2:HourAngle
  a owl:Class ;
  rdfs:label "hour angle"@en, "uurhoek"@nl ;
  rdfs:comment "The angular distance on the celestial sphere measured westward along the celestial equator from the meridian to the hour circle that passes through the celestial object."@en ;
  rdfs:subClassOf ns2:Angle ;
  ns2:symbol "H" ;
  ns1:reference ns1:Glossary_Astronomical_Almanac ;
  ns2:commonlyHasUnit ns2:hour-HourAngle, ns2:minute-HourAngle, ns2:second-HourAngle .

ns2:RightAscension
  a owl:Class ;
  rdfs:label "right ascension"@en, "rechte klimming"@nl ;
  rdfs:comment "The angular distance on the celestial sphere measured eastward along the celestial equator from the equinox to the great circle passing through the celestial object and the celestial north pole."@en ;
  rdfs:subClassOf ns2:Angle ;
  ns2:symbol "α" ;
  ns2:alternativeSymbol "ra" ;
  ns1:reference ns1:Glossary_Astronomical_Almanac ;
  ns2:commonlyHasUnit ns2:degree, ns2:hour-HourAngle, ns2:minute-HourAngle, ns2:second-HourAngle .

ns2:SupergalacticLatitude
  a owl:Class ;
  rdfs:label "supergalactic latitude"@en ;
  rdfs:comment "The angular distance on the celestial sphere north or south of the supergalactic equator. It is measured along the great circle passing through the object and the supergalactic poles and perpendicular to the supergalactic equator."@en ;
  rdfs:subClassOf ns2:Angle ;
  ns2:symbol "SGB" ;
  ns2:commonlyHasUnit ns2:degree, ns2:minute-Angle, ns2:second-Angle .

ns2:SupergalacticLongitude
  a owl:Class ;
  rdfs:label "supergalactic longitude"@en ;
  rdfs:comment "The angular distance on the celestial sphere measured clockwise from the supergalactic centre (as defined by the International Astronomical Union (IAU)) along the supergalactic equator to the intersection with the great circle drawn from the supergalactic north pole through the object."@en ;
  rdfs:subClassOf ns2:Angle ;
  ns2:symbol "SGL" ;
  ns2:commonlyHasUnit ns2:degree, ns2:minute-Angle, ns2:second-Angle .

ns2:ZenithDistance
  a owl:Class ;
  rdfs:label "zenith distance"@en, "zenitafstand"@nl ;
  ns2:alternativeLabel "zenith angle"@en, "zenithoek"@nl ;
  rdfs:comment "The angular distance on the celestial sphere measured along the great circle from the zenith to the celestial object. z = 90° - h."@en ;
  rdfs:subClassOf ns2:Angle ;
  ns2:symbol "z" ;
  ns1:reference ns1:Glossary_Astronomical_Almanac ;
  ns2:commonlyHasUnit ns2:degree, ns2:minute-Angle, ns2:second-Angle .

ns2:Aberration
  a owl:Class ;
  rdfs:label "aberration"@en ;
  rdfs:comment "The apparent angular displacement of the observed position of a celestial object from its geometric position, caused by the finite velocity of light in combination with the motions of the observer and of the observed object."@en ;
  rdfs:subClassOf ns2:AngularDisplacement ;
  ns1:reference ns1:Glossary_Astronomical_Almanac ;
  ns2:commonlyHasUnit ns2:degree, ns2:second-Angle, ns2:millisecond-Angle, ns2:microsecond-Angle .

ns2:PlanetaryAberration
  a owl:Class ;
  rdfs:label "planetary aberration"@en ;
  rdfs:comment "The apparent angular displacement of the observed position of a celestial object produced by the motion of the observer and the actual motion of the observed object."@en ;
  rdfs:subClassOf ns2:Aberration ;
  ns1:reference ns1:Glossary_Astronomical_Almanac ;
  ns2:commonlyHasUnit ns2:degree, ns2:second-Angle, ns2:millisecond-Angle, ns2:microsecond-Angle .

ns2:StellarAberration
  a owl:Class ;
  rdfs:label "stellar aberration"@en ;
  rdfs:comment "The apparent angular displacement of the observed position of a celestial object resulting from the motion of the observer. Stellar aberration is divided into diurnal, annual, and secular components."@en ;
  rdfs:subClassOf ns2:Aberration ;
  ns1:reference ns1:Glossary_Astronomical_Almanac ;
  ns2:commonlyHasUnit ns2:degree, ns2:second-Angle, ns2:millisecond-Angle, ns2:microsecond-Angle .

ns2:AnnualAberration
  a owl:Class ;
  rdfs:label "annual aberration"@en ;
  rdfs:comment "The component of the stellar abberation resulting from the motion of the Earth about the Sun. The abberation is the apparent angular displacement of the observed position of a celestial object from its geometric position, caused by the finite velocity of light in combination with the motions of the observer and of the observed object."@en ;
  rdfs:subClassOf ns2:AngularDisplacement ;
  ns1:reference ns1:Glossary_Astronomical_Almanac ;
  ns2:commonlyHasUnit ns2:degree, ns2:second-Angle, ns2:millisecond-Angle, ns2:microsecond-Angle .

ns2:DiurnalAberration
  a owl:Class ;
  rdfs:label "diurnal aberration"@en ;
  rdfs:comment "The component of the stellar abberation resulting from the diurnal motion of the observer around the centre of the Earth. The abberation is the apparent angular displacement of the observed position of a celestial object from its geometric position, caused by the finite velocity of light in combination with the motions of the observer and of the observed object."@en ;
  rdfs:subClassOf ns2:AngularDisplacement ;
  ns1:reference ns1:Glossary_Astronomical_Almanac ;
  ns2:commonlyHasUnit ns2:degree, ns2:second-Angle, ns2:millisecond-Angle, ns2:microsecond-Angle .

ns2:SecularAberration
  a owl:Class ;
  rdfs:label "secular aberration"@en ;
  rdfs:comment "The component of the stellar abberation resulting from the motion of the solar system in space. This component is usually ignored. The abberation is the apparent angular displacement of the observed position of a celestial object from its geometric position, caused by the finite velocity of light in combination with the motions of the observer and of the observed object."@en ;
  rdfs:subClassOf ns2:AngularDisplacement ;
  ns1:reference ns1:Glossary_Astronomical_Almanac ;
  ns2:commonlyHasUnit ns2:degree, ns2:second-Anglee, ns2:millisecond-Angle, ns2:microsecond-Angle .

ns2:AberrationInLongitude
  a owl:Class ;
  rdfs:label "aberration in longitude"@en ;
  rdfs:comment "The apparent angular displacement in ecliptical longitude of the observed position of a celestial object from its geometric position, caused by the finite velocity of light in combination with the motions of the observer and of the observed object."@en ;
  rdfs:subClassOf ns2:AngularDisplacement ;
  ns2:symbol "Δλ" ;
  ns1:reference ns1:chapter23_Astronomical_Algorithms ;
  ns2:commonlyHasUnit ns2:degree, ns2:second-Anglee, ns2:millisecond-Angle, ns2:microsecond-Angle .

ns2:AberrationInLatitude
  a owl:Class ;
  rdfs:label "aberration in latitude"@en ;
  rdfs:comment "The apparent angular displacement in ecliptical latitude of the observed position of a celestial object from its geometric position, caused by the finite velocity of light in combination with the motions of the observer and of the observed object."@en ;
  rdfs:subClassOf ns2:AngularDisplacement ;
  ns2:symbol "Δβ" ;
  ns1:reference ns1:chapter23_Astronomical_Algorithms ;
  ns2:commonlyHasUnit ns2:degree, ns2:second-Angle, ns2:millisecond-Angle, ns2:microsecond-Angle .

ns2:InitialMassFunction
  a owl:Class ;
  rdfs:label "initial mass function"@en ;
  rdfs:comment "The number of stars in mass fraction dM around mass M. Used in Salpeter's Initial Mass Function (IMF)."@en ;
  rdfs:subClassOf ns2:NumberDensity ;
  ns2:symbol "IMF" ;
  ns2:commonlyHasUnit ns2:reciprocalCubicParsec .

ns2:LuminosityFunction
  a owl:Class ;
  rdfs:label "luminosity function"@en ;
  rdfs:comment "The number of stars of absolute magnitudes between Mv and Mv+ΔMv per cubic parsec."@en ;
  rdfs:subClassOf ns2:NumberDensity ;
  ns2:commonlyHasUnit ns2:reciprocalCubicParsec .

ns2:NoiseEquivalentPower
  a owl:Class ;
  rdfs:label "noise equivalent power"@en ;
  rdfs:comment "Radiative flux on a detector needed for a signal/noise ratio of 1 (Kitchin, Astrophysical Techniques, IoP, Table 1.1.2)."@en ;
  rdfs:subClassOf ns2:Power ;
  ns1:reference ns1:Astrophysical_Techniques_chapter1 ;
  ns2:symbol "NEP" ;
  ns2:commonlyHasUnit ns2:watt .

ns2:ColdGasMassFraction
  a owl:Class ;
  rdfs:label "cold gas mass fraction"@en ;
  rdfs:comment "The fraction of the mass of a galaxy that is in the form of cold gas ~10s K."@en ;
  rdfs:subClassOf ns2:MassFraction ;
  ns2:commonlyHasUnit ns2:one .

ns2:SpectralResponse
  a owl:Class ;
  rdfs:label "spectral response"@en ;
  rdfs:comment "The change in output signal as a function of changes in the wavelength of the input signal."@en ;
  rdfs:subClassOf ns2:Quantity ;
  ns1:reference ns1:Astrophysical_Techniques_chapter1 .

ns2:ApparentDistanceModulus
  a owl:Class ;
  rdfs:label "apparent distance modulus"@en ;
  rdfs:subClassOf ns2:DistanceModulus ;
  ns2:commonlyHasUnit ns2:magnitude .

ns2:Amplitude
  a owl:Class ;
  rdfs:label "amplitude"@en ;
  rdfs:comment "The difference between the maximum and minimum magnitudes of a variable star, i.e., the total range of its brightness."@en ;
  rdfs:subClassOf ns2:Quantity ;
  ns2:commonlyHasUnit ns2:magnitude .

ns2:BolometricMagnitude
  a owl:Class ;
  rdfs:label "bolometric magnitude"@en ;
  rdfs:comment "The magnitude of a star measured across all wavelengths, so that it takes into account the total amount of energy radiated. If a star is a strong infrared or ultraviolet emitter, its bolometric magnitude  will differ greatly from its visual magnitude."@en ;
  rdfs:subClassOf ns2:Magnitude ;
  ns2:symbol "m_bol" ;
  ns2:commonlyHasUnit ns2:magnitude .

ns2:AbsoluteBolometricMagnitude
  a owl:Class ;
  rdfs:label "absolute bolometric magnitude"@en ;
  rdfs:comment "The absolute magnitude (see absolute magnitude) of a star is a measure of its total energy emission per second, or luminosity, i.e., the bolometric magnitude from a standard distance (10 pc)."@en ;
  rdfs:subClassOf ns2:BolometricMagnitude ;
  ns2:symbol "M_bol" ;
  ns2:commonlyHasUnit ns2:magnitude .

ns2:BolometricCorrection
  a owl:Class ;
  rdfs:label "bolometric correction"@en ;
  rdfs:comment "The visual magnitude of an object minus its bolometric magnitude."@en ;
  rdfs:subClassOf ns2:Quantity ;
  ns2:symbol "BC" ;
  ns2:commonlyHasUnit ns2:magnitude .

ns2:ColourIndex
  a owl:Class ;
  rdfs:label "colour index"@en, "kleurindex"@nl ;
  rdfs:comment "The difference between the apparent magnitude of a star at two different wavelengths (always the shorter-wavelength magnitude minus the longer-wavelength magnitude) to give a quantification of the star's colour. The magnitude of an object at different wavelengths are measured by using different filters before the detector. Often the Johnson system with UBV passbands are used. Other passbands may also be used (for instance g-r)."@en ;
  rdfs:subClassOf ns2:Quantity ;
  ns2:commonlyHasUnit ns2:magnitude .

ns2:IntrinsicColourIndex
  a owl:Class ;
  rdfs:label "intrinsic colour index"@en ;
  rdfs:comment "The colour index a star would have in the absence of interstellar extinction (reddening). It is assumed that all stars of the same spectral type and luminosity class have the same colour index."@en ;
  rdfs:subClassOf ns2:ColourIndex ;
  ns2:commonlyHasUnit ns2:magnitude .

ns2:DistanceModulus
  a owl:Class ;
  rdfs:label "distance modulus"@en ;
  rdfs:comment """The difference between the apparent magnitude (m) of an astronomical object, such as a star, and its absolute magnitude (M), used as a distance measurement. Distances can be expressed in distance modulii as $$m-M = 5\\log d + 10 = 10-5 log \\varpi$$ where \\(d\\) is the distance in kiloparsec and \\(\\varpi\\) is the parallax in milliarcseconds.
    """@en ;
  rdfs:subClassOf ns2:Distance ;
  ns2:symbol "m-M" ;
  ns2:commonlyHasUnit ns2:magnitude .

ns2:Extinction
  a owl:Class ;
  rdfs:label "extinction"@en, "extinctie"@nl ;
  rdfs:comment "Total extinction at a specific wavelength. The extinction is caused by dust and gas between a star and the observer. It is the difference between the observed magnitude and the magnitude the source would have had if no extinction had taken place."@en ;
  rdfs:subClassOf ns2:Quantity ;
  ns2:symbol "A" ;
  ns2:commonlyHasUnit ns2:magnitude .

ns2:ExtinctionAtWavelength
  a owl:Class ;
  rdfs:label "extinction at wavelength"@en ;
  rdfs:subClassOf ns2:Extinction ;
  ns2:symbol "A_λ" ;
  ns2:commonlyHasUnit ns2:magnitude .

ns2:ExtinctionAtWaveband
  a owl:Class ;
  rdfs:label "extinction at waveband"@en ;
  rdfs:subClassOf ns2:Extinction ;
  ns2:symbol "A_X" ;
  ns2:commonlyHasUnit ns2:magnitude .

ns2:ExtinctionInV
  a owl:Class ;
  rdfs:label "extinction in V"@en ;
  rdfs:subClassOf ns2:ExtinctionAtWaveband ;
  ns2:symbol "A_V" ;
  ns2:commonlyHasUnit ns2:magnitude .

ns2:ExtinctionInB
  a owl:Class ;
  rdfs:label "extinction in B"@en ;
  rdfs:subClassOf ns2:ExtinctionAtWaveband ;
  ns2:symbol "A_B" ;
  ns2:commonlyHasUnit ns2:magnitude .

ns2:ExtinctionInU
  a owl:Class ;
  rdfs:label "extinction in U"@en ;
  rdfs:subClassOf ns2:ExtinctionAtWaveband ;
  ns2:symbol "A_U" ;
  ns2:commonlyHasUnit ns2:magnitude .

ns2:IntegratedMagnitude
  a owl:Class ;
  rdfs:label "integrated magnitude"@en ;
  rdfs:comment "The apparent magnitude that an extended object, such as a nebula or galaxy, would have if all its light were concentrated at a starlike point."@en ;
  rdfs:subClassOf ns2:Magnitude ;
  ns2:commonlyHasUnit ns2:magnitude .

ns2:LimitingMagnitude
  a owl:Class ;
  rdfs:label "limiting magnitude"@en ;
  rdfs:comment "The magnitude of the faintest object (star) that can be detected by a telescope or other instrument. Depends not only on the telescope but also on the detector and on the observing method."@en ;
  rdfs:subClassOf ns2:Magnitude ;
  ns2:commonlyHasUnit ns2:magnitude .

ns2:PhotographicAmplitude
  a owl:Class ;
  rdfs:label "photographic amplitude"@en ;
  rdfs:comment "Amplitude of the light variation in photographic magnitude."@en ;
  rdfs:subClassOf ns2:Amplitude ;
  ns2:symbol "A_V" ;
  ns2:commonlyHasUnit ns2:magnitude .

ns2:RedMagnitude
  a owl:Class ;
  rdfs:label "red magnitude"@en ;
  rdfs:comment "A red magnitude not specified for a specific photometric system."@en ;
  rdfs:subClassOf ns2:Magnitude ;
  ns2:symbol "r" ;
  ns2:alternativeSymbol "m_r" ;
  ns2:commonlyHasUnit ns2:magnitude .

ns2:Reddening
  a owl:Class ;
  rdfs:label "reddening"@en ;
  ns2:alternativeLabel "colour excess"@en, "wavelength-selective extinction"@en ;
  rdfs:comment "Reddening causes the star to appear redder if more dust or gas is between the star and the observer."@en ;
  rdfs:subClassOf ns2:Quantity ;
  ns2:symbol "E" ;
  ns2:commonlyHasUnit ns2:magnitude .

ns2:ReddeningB-V
  a owl:Class ;
  rdfs:label "reddening (B-V)"@en ;
  ns2:alternativeLabel "colour excess (B-V)"@en, "wavelength-selective extinction (B-V)"@en ;
  rdfs:comment "Reddening causes the star to appear redder if more dust or gas is between the star and the observer. The standard reddening is measured using the B and V passbands."@en ;
  rdfs:subClassOf ns2:Reddening ;
  ns2:symbol "E_B-V" ;
  ns2:LaTeXSymbol "E_{\\mathit{B-V}}" ;
  ns2:commonlyHasUnit ns2:magnitude .

ns2:ReddeningU-B
  a owl:Class ;
  rdfs:label "reddening (U-B)"@en ;
  ns2:alternativeLabel "colour excess (U-B)"@en, "wavelength-selective extinction (U-B)"@en ;
  rdfs:comment "Reddening measured with the U and B passbands."@en ;
  rdfs:subClassOf ns2:Reddening ;
  ns2:symbol "E_U-B" ;
  ns2:LaTeXSymbol "E_{\\mathit{U-B}}" ;
  ns2:commonlyHasUnit ns2:magnitude .

ns2:TrueDistanceModulus
  a owl:Class ;
  rdfs:label "true distance modulus"@en ;
  rdfs:subClassOf ns2:DistanceModulus ;
  ns2:commonlyHasUnit ns2:magnitude .

ns2:TychoBroadbandMagnitude
  a owl:Class ;
  rdfs:label "Tycho broadband magnitude"@en ;
  rdfs:comment "Broadband Tycho magnitude (formed from B and V magintude measurements."@en ;
  rdfs:subClassOf ns2:Magnitude ;
  ns2:symbol "T" ;
  ns2:alternativeSymbol "m_T" ;
  ns2:commonlyHasUnit ns2:magnitude .

ns2:JohnsonMagnitude
  a owl:Class ;
  rdfs:label "Johnson magnitude"@en ;
  rdfs:comment "A magnitude measured in one of Johnson's standard passbands (using a standard filter, i.e. U, B, or V)."@en ;
  ns2:longcomment "For accurate photometry the magnitude needs to be determined over well-defined spectral regions as the spectrum of to objects may be quite different. These magnitudes are measured using filters that allows only radiation within specific spectral regions (passbands) to pass through to the detector. These filters have accurately defined transmission curves characterised by a central wavelength and a bandwidth. The UBV system devised by Harold Johnson and William Morgan has been the most important general system until recently. The precise definition requires a reflecting telescope with aluminised mirrors fitted with an RCA 1P21 photomultiplier. The U region corresponds to a region in the violet and ultraviolet, the B region corresponds to typical photographic response and the V region to the visual response region (approximating the eye's response curve)."^^rdf:XMLLiteral ;
  rdfs:subClassOf ns2:Magnitude ;
  ns1:reference ns1:Astrophysical_Techniques_chapter3 .

ns2:StroemgrenMagnitude
  a owl:Class ;
  rdfs:label "Strömgren magnitude"@en ;
  rdfs:comment "A magnitude measured in one of Strömgren's standard passbands (using a standard filter, u, b, v, or y) or in the passbands defined by Crawford (β_narrow or β_wide)."@en ;
  rdfs:subClassOf ns2:Magnitude ;
  ns1:reference ns1:Astrophysical_Techniques_chapter3, ns1:Stroemgren1956, ns1:Crawford1958 .

ns2:CousinsMagnitude
  a owl:Class ;
  rdfs:label "Cousins magnitude"@en ;
  rdfs:comment "A magnitude measured in one of Cousins standard passbands (using a standard filter, i.e. I or R)."@en ;
  rdfs:subClassOf ns2:Magnitude .

ns2:ThuanAndGunnMagnitude
  a owl:Class ;
  rdfs:label "Thuan and Gunn magnitude"@en ;
  rdfs:comment "A magnitude measured in one of Thuan and Gunn's standard passbands (using a standard filter, i.e. g)."@en ;
  rdfs:subClassOf ns2:Magnitude .

ns2:VAmplitude
  a owl:Class ;
  rdfs:label "V amplitude"@en ;
  rdfs:comment "Amplitude of the light variation in Johnson V magnitude. The Johnson V band is a standard passband in the visual area, matching the response curve of the human eye. The central wavelength is 550nm and the bandwidth is 90nm.  The filter to be used is the Corning 3384 filter."@en ;
  rdfs:subClassOf ns2:Amplitude ;
  ns1:reference ns1:Astrophysical_Techniques_chapter3 ;
  ns2:symbol "A_V" ;
  ns2:commonlyHasUnit ns2:magnitude .

ns2:_1040NanometreLockwoodMagnitude
  a owl:Class ;
  rdfs:label "1040 nm Lockwood magnitude"@en ;
  rdfs:comment "A magnitude in the 1.04 micrometre band of the photometric system introduced by G.W. Lockwood."@en ;
  rdfs:subClassOf ns2:Magnitude ;
  ns2:symbol "m_L1040" ;
  ns2:commonlyHasUnit ns2:magnitude .

ns2:uMagnitude
  a owl:Class ;
  rdfs:label "u magnitude"@en ;
  rdfs:comment "u Magnitude in the Strömgren photometric system with a peak wavelength at 350 nm and a peak-half-width of 30 nm."@en ;
  rdfs:subClassOf ns2:StroemgrenMagnitude ;
  ns2:symbol "u" ;
  ns2:alternativeSymbol "m_u" ;
  ns1:reference ns1:Astrophysical_Techniques_chapter3, ns1:Stroemgren1956, ns1:Crawford1958 ;
  ns2:commonlyHasUnit ns2:magnitude .

ns2:vMagnitude
  a owl:Class ;
  rdfs:label "v magnitude"@en ;
  rdfs:comment "v Magnitude in the Strömgren photometric system with a peak wavelength at 411 nm and a peak-half-width of 19 nm."@en ;
  rdfs:subClassOf ns2:StroemgrenMagnitude ;
  ns2:symbol "v" ;
  ns2:alternativeSymbol "m_v" ;
  ns1:reference ns1:Astrophysical_Techniques_chapter3, ns1:Stroemgren1956, ns1:Crawford1958 ;
  ns2:commonlyHasUnit ns2:magnitude .

ns2:bMagnitude
  a owl:Class ;
  rdfs:label "b magnitude"@en ;
  rdfs:comment "b Magnitude in the Strömgren photometric system with a peak wavelength at 467 nm and a peak-half-width of 18 nm."@en ;
  rdfs:subClassOf ns2:StroemgrenMagnitude ;
  ns2:symbol "b" ;
  ns2:alternativeSymbol "m_b" ;
  ns1:reference ns1:Astrophysical_Techniques_chapter3, ns1:Stroemgren1956, ns1:Crawford1958 ;
  ns2:commonlyHasUnit ns2:magnitude .

ns2:yMagnitude
  a owl:Class ;
  rdfs:label "y magnitude"@en ;
  rdfs:comment "y Magnitude in the Strömgren photometric system with a peak wavelength at 547 nm and a peak-half-width of 23 nm."@en ;
  rdfs:subClassOf ns2:StroemgrenMagnitude ;
  ns2:symbol "y" ;
  ns2:alternativeSymbol "m_y" ;
  ns1:reference ns1:Astrophysical_Techniques_chapter3, ns1:Stroemgren1956, ns1:Crawford1958 ;
  ns2:commonlyHasUnit ns2:magnitude .

ns2:BetaNarrowMagnitude
  a owl:Class ;
  rdfs:label "β_narrow magnitude"@en ;
  rdfs:comment "β_narrow  Magnitude in the Strömgren-Crawford photometric system with a peak wavelength at 485.8 nm and a peak-half-width of 2.9 nm."@en ;
  rdfs:subClassOf ns2:StroemgrenMagnitude ;
  ns2:symbol "β_n" ;
  ns2:alternativeSymbol "β_narrow" ;
  ns1:reference ns1:Astrophysical_Techniques_chapter3, ns1:Crawford1958 ;
  ns2:commonlyHasUnit ns2:magnitude .

ns2:BetaWideMagnitude
  a owl:Class ;
  rdfs:label "β_wide magnitude"@en ;
  rdfs:comment "β_wide  Magnitude in the Strömgren-Crawford photometric system with a peak wavelength at 485 nm and a peak-half-width of 12.9 nm."@en ;
  rdfs:subClassOf ns2:StroemgrenMagnitude ;
  ns2:symbol "β_w" ;
  ns2:alternativeSymbol "β_wide" ;
  ns1:reference ns1:Astrophysical_Techniques_chapter3, ns1:Crawford1958 ;
  ns2:commonlyHasUnit ns2:magnitude .

ns2:IMagnitude
  a owl:Class ;
  rdfs:label "I magnitude"@en ;
  rdfs:comment "I magnitude in the Cousins photometric system."@en ;
  rdfs:subClassOf ns2:CousinsMagnitude ;
  ns2:symbol "I" ;
  ns2:alternativeSymbol "m_I" ;
  ns2:commonlyHasUnit ns2:magnitude .

ns2:RMagnitude
  a owl:Class ;
  rdfs:label "R magnitude"@en ;
  rdfs:comment "R magnitude in the Cousins photometric system."@en ;
  rdfs:subClassOf ns2:CousinsMagnitude ;
  ns2:symbol "R" ;
  ns2:alternativeSymbol "m_R" ;
  ns2:commonlyHasUnit ns2:magnitude .

ns2:gMagnitude
  a owl:Class ;
  rdfs:label "g magnitude"@en ;
  rdfs:comment "g Magnitude in the Thuan and Gunn photometric system."@en ;
  rdfs:subClassOf ns2:ThuanAndGunnMagnitude ;
  ns2:symbol "g" ;
  ns2:alternativeSymbol "m_g" ;
  ns2:commonlyHasUnit ns2:magnitude .

ns2:DarkNoise
  a owl:Class ;
  rdfs:label "dark noise"@en ;
  rdfs:comment "Output from a detector when unilluminated - usually as RMS voltage or current (Kitchin, Astrophysical Techniques, IoP, Table 1.1.2)."@en ;
  rdfs:subClassOf ns2:Quantity ;
  ns1:reference ns1:Astrophysical_Techniques_chapter1 .

ns2:NormalisedDetectivity
  a owl:Class ;
  rdfs:label "normalised detectivity"@en ;
  rdfs:comment "The detectivity normalised by multiplying by the square root of the detector area, and by the electrical bandwidth. The units cm Hz(1/2)/W are commonly used and it then represents the signal-to-noise ratio when 1 W of radiation is incident on a detector with an area of 1 cm2, and the electrical bandwidth is 1 Hz."@en ;
  rdfs:subClassOf ns2:Quantity ;
  ns1:reference ns1:Astrophysical_Techniques_chapter1 ;
  ns2:symbol "D*" .

ns2:Responsivity
  a owl:Class ;
  rdfs:label "responsivity"@en ;
  rdfs:comment "Detector output for unit intensity input. Units are usually volts per watt or amps per watt."@en ;
  rdfs:subClassOf ns2:Quantity, [
    a owl:Restriction ;
    owl:onProperty ns2:hasValue ;
    owl:allValuesFrom [
      a owl:Restriction ;
      owl:onProperty ns2:hasUnit ;
      owl:allValuesFrom ns2:ResponsivityUnit
    ]
  ] ;
  ns1:reference ns1:Astrophysical_Techniques_chapter1 ;
  ns2:symbol "R" ;
  ns2:commonlyHasUnit ns2:voltPerWatt, ns2:amperePerWatt .

ns2:hour-HourAngle
  a ns2:Unit, ns2:SingularUnit ;
  rdfs:label "hour (hour angle)"@en, "uur (uurhoek)"@nl ;
  rdfs:comment "Wordt gebruikt als hoek (360°=24) voor o.a. rechte klimming. De h wordt meestal als superscript achter de waarde gezet gevolgd door de verdere opdeling naar minuten en seconden. Zoals in 5h34m12s09. Vaak wordt de fractie in seconden zonder punt geschreven, de s wordt als afscheiding gebruikt (http://en.wikipedia.org/wiki/Right_ascension)."@nl ;
  ns2:symbol "h" ;
  ns2:hasFactor "15"^^xsd:float ;
  ns2:hasUnit ns2:degree ;
  ns2:hasDimension ns2:dimensionOne .

ns2:minute-HourAngle
  a ns2:Unit, ns2:SingularUnit ;
  rdfs:label "minute (hour angle)"@en, "minuut (uurhoek)"@nl ;
  rdfs:comment "Wordt gebruikt als hoek (360°=1440) voor o.a. rechte klimming. De m wordt meestal als superscript achter de waarde gezet gevolgd door de verdere opdeling naar seconden. Zoals in 5h34m12s09. Vaak wordt de fractie in seconden zonder punt geschreven, de s wordt als afscheiding gebruikt (http://en.wikipedia.org/wiki/Right_ascension)."@nl ;
  ns2:symbol "m" ;
  ns2:hasFactor "0.25"^^xsd:float ;
  ns2:hasUnit ns2:degree ;
  ns2:hasDimension ns2:dimensionOne .

ns2:second-HourAngle
  a ns2:Unit, ns2:SingularUnit ;
  rdfs:label "second (hour angle)"@en, "seconde (uurhoek)"@nl ;
  rdfs:comment "Wordt gebruikt als hoek (360°=864000) voor o.a. rechte klimming. De s wordt meestal als superscript achter de waarde gezet. Zoals in 5h34m12s09. Vaak wordt de fractie in seconden zonder punt geschreven, de s wordt als afscheiding gebruikt (http://en.wikipedia.org/wiki/Right_ascension)."@nl ;
  ns2:symbol "s" ;
  ns2:hasFactor "4.1666667e-3"^^xsd:float ;
  ns2:hasUnit ns2:degree ;
  ns2:hasDimension ns2:dimensionOne .

ns2:magnitude
  a ns2:Unit, ns2:SingularUnit ;
  rdfs:label "magnitude"@en, "magnitude"@nl ;
  rdfs:comment "Eenheid waarmee de helderheid van sterren wordt aangegeven. Meestal wordt het symbool niet aangeduid (http://en.wikipedia.org/wiki/Magnitude_(astronomy))."@en ;
  ns2:symbol "mag" ;
  ns2:hasUnit ns2:one ;
  ns2:hasDimension ns2:dimensionOne .

ns2:MagnitudeUnit
  a owl:Class ;
  rdfs:label "magnitude unit"@en ;
  rdfs:subClassOf ns2:Unit ;
  owl:equivalentClass [
    a owl:Class ;
    owl:oneOf (
     ns2:one
     ns2:magnitude
     ns2:millimagnitude
     ns2:micromagnitude
   )
  ] .

ns2:millimagnitude
  a ns2:PrefixedUnit ;
  rdfs:label "millimagnitude"@en, "millimagnitude"@nl ;
  rdfs:comment "The millimagnitude is a unit of magnitude defined as 1.0e-3 magnitude."@en ;
  ns2:symbol "mmag" ;
  ns2:hasPrefix ns2:milli ;
  ns2:hasUnit ns2:magnitude ;
  ns2:hasDimension ns2:dimensionOne .

ns2:micromagnitude
  a ns2:PrefixedUnit ;
  rdfs:label "micromagnitude"@en, "micromagnitude"@nl ;
  rdfs:comment "The micromagnitude is a unit of magnitude defined as 1.0e-6 magnitude."@en ;
  ns2:symbol "μmag" ;
  ns2:hasPrefix ns2:micro ;
  ns2:hasUnit ns2:magnitude ;
  ns2:hasDimension ns2:dimensionOne .

ns2:voltPerWatt
  a ns2:UnitDivision ;
  rdfs:label "volt per watt"@en, "volt per watt"@nl ;
  ns2:symbol "V/W" ;
  ns2:alternativeSymbol "V W-1", "V·W-1" ;
  ns2:hasNumerator ns2:volt ;
  ns2:hasDenominator ns2:watt .

ns2:ResponsivityUnit
  a owl:Class ;
  rdfs:label "responsivity unit"@en ;
  rdfs:subClassOf ns2:Unit ;
  owl:equivalentClass [
    a owl:Class ;
    owl:oneOf (
     ns2:voltPerWatt
     ns2:amperePerWatt
   )
  ] ;
  ns1:reference ns1:Astrophysical_Techniques_chapter1 .

ns2:amperePerWatt
  a ns2:UnitDivision ;
  rdfs:label "ampere per watt"@en, "ampere per watt"@nl ;
  ns2:symbol "A/W" ;
  ns2:alternativeSymbol "A W-1", "A·W-1" ;
  ns2:hasNumerator ns2:ampere ;
  ns2:hasDenominator ns2:watt .

ns2:jansky
  a ns2:Unit, ns2:SingularUnit ;
  rdfs:label "jansky"@en, "jansky"@nl ;
  ns2:alternativeLabel "flux unit"@en ;
  ns2:symbol "Jy" .

ns2:magnitudePerSecond-AngleSquared
  a ns2:UnitDivision ;
  rdfs:label "magnitude per second (angle) squared"@en ;
  rdfs:comment "The brightness (in magnitudes) of an area on the celestial sphere of 1 arcsecond by 1 arcsecond."@en ;
  ns2:symbol "mag/arcsec2" ;
  ns2:alternativeSymbol "mag arcsec-2", "mag·arcsec-2" ;
  ns2:hasNumerator ns2:magnitude ;
  ns2:hasDenominator ns2:second-AngleSquared .

ns2:wattPerSecond-AngleSquared
  a ns2:UnitDivision ;
  rdfs:label "watt per second (angle) squared"@en ;
  rdfs:comment "The radiative intensity (in watts) of an area on the celestial sphere of 1 arcsecond by 1 arcsecond."@en ;
  ns2:symbol "W/arcsec2" ;
  ns2:alternativeSymbol "W arcsec-2", "W·arcsec-2" ;
  ns2:hasNumerator ns2:watt ;
  ns2:hasDenominator ns2:second-AngleSquared .

ns2:gigayearCubicParsec
  a ns2:UnitMultiplication ;
  rdfs:label "gigayear cubic parsec"@en, "gigajaar kubieke parsec"@nl ;
  ns2:symbol "Gyr pc3" ;
  ns2:alternativeSymbol "Gyr·pc3" ;
  ns2:hasTerm1 ns2:gigayear ;
  ns2:hasTerm2 ns2:cubicParsec .

ns2:gigayearCubicKiloparsec
  a ns2:UnitMultiplication ;
  rdfs:label "gigayear cubic kiloparsec"@en, "gigajaar kubieke kiloparsec"@nl ;
  ns2:symbol "Gyr kpc3" ;
  ns2:alternativeSymbol "Gyr·kpc3" ;
  ns2:hasTerm1 ns2:gigayear ;
  ns2:hasTerm2 ns2:cubicKiloparsec .

ns2:solarMassPerGigayearCubicParsec
  a ns2:UnitDivision ;
  rdfs:label "solar mass per gigayear cubic parsec"@en ;
  rdfs:comment "The amount of stellar mass created per cubic parsec in each billion years."@en ;
  ns2:symbol "M_☉/(Gyr pc3)" ;
  ns2:alternativeSymbol "M_☉ Gyr-1 pc-3", "M_☉·Gyr-1·pc-3" ;
  ns2:hasNumerator ns2:solarMass ;
  ns2:hasDenominator ns2:gigayearCubicParsec .

ns2:solarMassPerGigayearCubicKiloparsec
  a ns2:UnitDivision ;
  rdfs:label "solar mass per gigayear cubic kiloparsec"@en ;
  rdfs:comment "The amount of stellar mass created per cubic kiloparsec in each billion years."@en ;
  ns2:symbol "M_☉/(Gyr kpc3)" ;
  ns2:alternativeSymbol "M_☉ Gyr-1 kpc-3", "M_☉·Gyr-1·kpc-3" ;
  ns2:LaTeXSymbol "M_{\\astrosun}Gyr^{-1}kpc^{-1}" ;
  ns2:hasNumerator ns2:solarMass ;
  ns2:hasDenominator ns2:gigayearCubicKiloparsec .

ns2:cosmology
  a ns2:ApplicationArea ;
  rdfs:label "cosmology"@en, "kosmologie"@nl ;
  ns2:usesQuantity ns2:CosmologicalConstant, ns2:CriticalDensity, ns2:CurvatureConstant, ns2:DecelerationParameter, ns2:DensityParameter, ns2:DensityParameterForMatter, ns2:DensityParameterForBaryonicMatter, ns2:DensityParameterForRadiation, ns2:DensityParameterForVacuum, ns2:HubbleConstant, ns2:HubbleConstantAtPresentEpoch, ns2:ScaleFactor, ns2:TotalDensityParameter ;
  ns2:usesUnit ns2:gigaelectronvolt, ns2:gigaparsec, ns2:kiloelectronvolt, ns2:megaelectronvolt, ns2:megaparsec .

ns2:CriticalDensity
  a owl:Class ;
  rdfs:label "critical density"@en, "kritieke dichtheid"@nl ;
  rdfs:comment "The density needed for a closed universe."@en ;
  rdfs:subClassOf ns2:Density ;
  ns2:symbol "ρ_c" ;
  ns2:commonlyHasUnit ns2:kilogramPerCubicmetre, ns2:gramPerCubicmetre, ns2:milligramPerCubicmetre, ns2:gramPerCubicCentimetre, ns2:microgramPerCubicCentimetre, ns2:kilogramPerCubicDecimetre .

ns2:CurvatureConstant
  a owl:Class ;
  rdfs:label "curvature constant"@en ;
  rdfs:comment "The curvature constant k=-1, 0, or 1."@en ;
  rdfs:subClassOf ns2:Quantity, [
    a owl:Restriction ;
    owl:onProperty ns2:hasValue ;
    owl:allValuesFrom [
      a owl:Restriction ;
      owl:onProperty ns2:hasUnit ;
      owl:allValuesFrom ns2:CurvatureConstantUnit
    ]
  ], [
    a owl:Restriction ;
    owl:onProperty ns2:hasDimension ;
    owl:hasValue ns2:dimensionOne
  ] ;
  ns2:symbol "k" ;
  ns2:commonlyHasUnit ns2:one .

ns2:CurvatureConstantUnit
  a owl:Class ;
  rdfs:label "curvature constant unit"@en ;
  rdfs:subClassOf ns2:Unit ;
  owl:equivalentClass [
    a owl:Class ;
    owl:oneOf ( ns2:one )
  ] .

ns2:DecelerationParameter
  a owl:Class ;
  rdfs:label "deceleration parameter"@en ;
  rdfs:subClassOf ns2:Quantity, [
    a owl:Restriction ;
    owl:onProperty ns2:hasValue ;
    owl:allValuesFrom [
      a owl:Restriction ;
      owl:onProperty ns2:hasUnit ;
      owl:allValuesFrom ns2:DecelerationParameterUnit
    ]
  ] ;
  ns2:symbol "q" ;
  ns2:commonlyHasUnit ns2:one .

ns2:DecelerationParameterUnit
  a owl:Class ;
  rdfs:label "deceleration parameter unit"@en ;
  rdfs:subClassOf ns2:Unit ;
  owl:equivalentClass [
    a owl:Class ;
    owl:oneOf ( ns2:one )
  ] .

ns2:DensityParameter
  a owl:Class ;
  rdfs:label "density parameter"@en ;
  rdfs:comment "Ratio of the average density and the critical density."@en ;
  rdfs:subClassOf ns2:Quantity, [
    a owl:Restriction ;
    owl:onProperty ns2:hasValue ;
    owl:allValuesFrom [
      a owl:Restriction ;
      owl:onProperty ns2:hasUnit ;
      owl:allValuesFrom ns2:DensityParameterUnit
    ]
  ], [
    a owl:Restriction ;
    owl:onProperty ns2:hasDimension ;
    owl:hasValue ns2:dimensionOne
  ] ;
  ns2:symbol "Ω" ;
  ns2:commonlyHasUnit ns2:one .

ns2:DensityParameterUnit
  a owl:Class ;
  rdfs:label "density parameter unit"@en ;
  rdfs:subClassOf ns2:Unit ;
  owl:equivalentClass [
    a owl:Class ;
    owl:oneOf ( ns2:one )
  ] .

ns2:DensityParameterForMatter
  a owl:Class ;
  rdfs:label "density parameter for matter"@en ;
  rdfs:comment "The density parameter for matter (either baryonic or dark)."@en ;
  rdfs:subClassOf ns2:DensityParameter ;
  ns2:symbol "Ω_M" ;
  ns2:commonlyHasUnit ns2:one .

ns2:DensityParameterForBaryonicMatter
  a owl:Class ;
  rdfs:label "density parameter for baryonic matter"@en ;
  rdfs:comment "The density parameter for baryonic (oridnary) matter."@en ;
  rdfs:subClassOf ns2:DensityParameter ;
  ns2:symbol "Ω_B" ;
  ns2:commonlyHasUnit ns2:one .

ns2:DensityParameterForRadiation
  a owl:Class ;
  rdfs:label "density parameter for radiation"@en ;
  rdfs:comment "The density parameter for radiation."@en ;
  rdfs:subClassOf ns2:DensityParameter ;
  ns2:symbol "Ω_R" ;
  ns2:commonlyHasUnit ns2:one .

ns2:DensityParameterForVacuum
  a owl:Class ;
  rdfs:label "density parameter for vacuum"@en ;
  rdfs:comment "The density parameter for vacuum."@en ;
  rdfs:subClassOf ns2:DensityParameter ;
  ns2:symbol "Ω_Λ" ;
  ns2:commonlyHasUnit ns2:one .

ns2:HubbleConstant
  a owl:Class ;
  rdfs:label "Hubble constant"@en, "constante van Hubble"@nl ;
  rdfs:comment "The Hubble constant (NOT a constant over time)."@en ;
  rdfs:subClassOf ns2:Quantity, [
    a owl:Restriction ;
    owl:onProperty ns2:hasValue ;
    owl:allValuesFrom [
      a owl:Restriction ;
      owl:onProperty ns2:hasUnit ;
      owl:allValuesFrom ns2:HubbleConstantUnit
    ]
  ] ;
  ns2:commonlyHasUnit ns2:metrePerSecond-TimePerMetre, ns2:kilometrePerSecond-TimePerMegaparsec .

ns2:HubbleConstantUnit
  a owl:Class ;
  rdfs:label "Hubble constant unit"@en ;
  rdfs:subClassOf ns2:Unit ;
  owl:equivalentClass [
    a owl:Class ;
    owl:oneOf (
     ns2:kilometrePerSecond-TimePerMegaparsec
     ns2:metrePerSecond-TimePerMetre
   )
  ] .

ns2:kilometrePerSecond-TimePerMegaparsec
  a ns2:UnitDivision ;
  rdfs:label "kilometre per second per megaparsec"@en, "kilometer per seconde per megaparsec"@nl ;
  rdfs:comment "De eenheid van de Hubble constante (die niet constant is!) (http://en.wikipedia.org/wiki/Hubble_constant)."@en ;
  ns2:symbol "km s-1 Mpc-1" ;
  ns2:hasNumerator ns2:kilometrePerSecond-Time ;
  ns2:hasDenominator ns2:megaparsec .

ns2:HubbleConstantAtPresentEpoch
  a owl:Class ;
  rdfs:label "Hubble constant at present epoch"@en, "constante van Hubble tijdens het huidige epoch"@nl ;
  rdfs:comment "The Hubble constant at the present epoch (a constant)."@en ;
  rdfs:subClassOf ns2:HubbleConstant ;
  ns2:symbol "H_0" ;
  ns2:commonlyHasUnit ns2:metrePerSecond-TimePerMetre, ns2:kilometrePerSecond-TimePerMegaparsec .

ns2:CosmologicalConstant
  a owl:Class ;
  rdfs:label "cosmological constant"@en, "kosmologische constante"@nl ;
  rdfs:comment "The cosmological constant."@en ;
  rdfs:subClassOf ns2:Quantity ;
  ns2:symbol "Λ" .

ns2:ScaleFactor
  a owl:Class ;
  rdfs:label "scale factor"@en, "schaalfactor"@nl ;
  rdfs:subClassOf ns2:Quantity .

ns2:Permeability-EarthScience
  a owl:Class ;
  rdfs:label "permeability (earth science)"@en, "permeabiliteit (aardwetenschappen)"@nl ;
  ns2:alternativeLabel "intrinsic permeability"@en, "intrinsieke permeabiliteit"@nl ;
  rdfs:subClassOf ns2:Quantity, [
    a owl:Restriction ;
    owl:onProperty ns2:hasDimension ;
    owl:hasValue ns2:area-Dimension
  ], [
    a owl:Restriction ;
    owl:onProperty ns2:hasValue ;
    owl:allValuesFrom [
      a owl:Restriction ;
      owl:onProperty ns2:hasUnit ;
      owl:allValuesFrom ns2:Permeability-EarthScienceUnit
    ]
  ] ;
  ns2:symbol "κ" ;
  ns2:alternativeSymbol "k" ;
  ns2:commonlyHasUnit ns2:squareMetre, ns2:squareAttometre, ns2:squareCentimetre, ns2:squareDecametre, ns2:squareDecimetre, ns2:squareExametre, ns2:squareFemtometre, ns2:squareGigametre, ns2:squareHectometre, ns2:squareKilometre, ns2:squareMegametre, ns2:squareMicrometre, ns2:squareMillimetre, ns2:squareNanometre, ns2:squarePetametre, ns2:squarePicometre, ns2:squareTerametre, ns2:darcy .

ns2:darcy
  a ns2:Unit, ns2:SingularUnit ;
  rdfs:label "darcy"@en, "darcy"@nl ;
  rdfs:comment "The darcy is a unit of area defined as 9.869233e-13 square metre."@en ;
  ns2:hasFactor "9.869233e-13"^^xsd:float ;
  ns2:hasUnit ns2:squareMetre ;
  ns2:hasDimension ns2:area-Dimension .

ns2:Permeability-EarthScienceUnit
  a owl:Class ;
  rdfs:label "permeability (earth science) unit"@en ;
  rdfs:subClassOf ns2:Unit ;
  owl:equivalentClass [
    a owl:Class ;
    owl:unionOf (
     _:genid1833
     ns2:SquarePrefixedMetre
   )
  ] .

ns2:Permeance-MaterialsScience
  a owl:Class ;
  rdfs:label "permeance (materials science)"@en ;
  rdfs:comment "Permeance is the degree to which a material transmits another substance."@en ;
  rdfs:subClassOf ns2:Quantity, [
    a owl:Restriction ;
    owl:onProperty ns2:hasValue ;
    owl:allValuesFrom [
      a owl:Restriction ;
      owl:onProperty ns2:hasUnit ;
      owl:allValuesFrom ns2:Permeance-MaterialsScienceUnit
    ]
  ], [
    a owl:Restriction ;
    owl:onProperty ns2:hasDimension ;
    owl:hasValue ns2:permeance-MaterialsScience-Dimension
  ] ;
  ns2:symbol "Λ" ;
  ns2:commonlyHasUnit ns2:kilogramPerPascalSecond-TimeSquareMetre, ns2:perm-0C, ns2:perm-23C .

ns2:kilogramPerPascalSecond-TimeSquareMetre
  a ns2:UnitDivision ;
  rdfs:label "kilogram per pascal second square metre"@en, "kilogram per pascal seconde vierkante meter"@nl ;
  ns2:symbol "kg Pa-1 s-1 m-2" ;
  ns2:alternativeSymbol "kg·Pa-1·s-1·m-2", "kg/(Pa s m2)", "kg/(Pa·s·m2)" ;
  ns2:hasNumerator ns2:kilogram ;
  ns2:hasDenominator ns2:pascalSecond-TimeSquareMetre ;
  ns2:hasDimension ns2:permeance-MaterialsScience-Dimension .

ns2:Permeance-MaterialsScienceUnit
  a owl:Class ;
  rdfs:label "permeance (materials science) unit"@en ;
  rdfs:subClassOf ns2:Unit ;
  owl:equivalentClass [
    a owl:Class ;
    owl:oneOf (
     ns2:perm-0C
     ns2:perm-23C
     ns2:kilogramPerPascalSecond-TimeSquareMetre
   )
  ] .

ns2:perm-0C
  a ns2:Unit, ns2:SingularUnit ;
  rdfs:label "perm (0 °C)"@en, "perm (0 °C)"@nl ;
  ns2:alternativeLabel "0 °C perm"@en, "0 °C perm"@nl ;
  rdfs:comment "The 0 °C perm is a unit ofpermeance defined as 5.72135e-11 kilogram per pascal second (time) square metre."@en ;
  ns2:hasFactor "5.72135e-11"^^xsd:float ;
  ns2:hasUnit ns2:kilogramPerPascalSecond-TimeSquareMetre ;
  ns2:hasDimension ns2:permeance-MaterialsScience-Dimension .

ns2:perm-23C
  a ns2:Unit, ns2:SingularUnit ;
  rdfs:label "perm (23 °C)"@en, "perm (23 °C)"@nl ;
  ns2:alternativeLabel "23 °C perm"@en, "23 °C perm"@nl ;
  rdfs:comment "The 23 °C perm is a unit of permeance defined as 5.74525e-11 kilogram per pascal second (time) square metre."@en ;
  ns2:hasFactor "5.74525e-11"^^xsd:float ;
  ns2:hasUnit ns2:kilogramPerPascalSecond-TimeSquareMetre ;
  ns2:hasDimension ns2:permeance-MaterialsScience-Dimension .

ns2:permeance-MaterialsScience-Dimension
  a ns2:Dimension ;
  rdfs:label "permeance (materials science) dimension"@en ;
  ns2:hasSILengthDimensionExponent -1 ;
  ns2:hasSIMassDimensionExponent 0 ;
  ns2:hasSITimeDimensionExponent 1 ;
  ns2:hasSIElectricCurrentDimensionExponent 0 ;
  ns2:hasSIThermodynamicTemperatureDimensionExponent 0 ;
  ns2:hasSIAmountOfSubstanceDimensionExponent 0 ;
  ns2:hasSILuminousIntensityDimensionExponent 0 .

ns2:ViableCount
  a owl:Class ;
  rdfs:label "viable count"@en ;
  rdfs:subClassOf ns2:Quantity, [
    a owl:Restriction ;
    owl:onProperty ns2:hasValue ;
    owl:allValuesFrom [
      a owl:Restriction ;
      owl:onProperty ns2:hasUnit ;
      owl:allValuesFrom ns2:ViableCountUnit
    ]
  ] ;
  ns2:commonlyHasUnit ns2:colonyFormingUnit, ns2:_1000ColonyFormingUnit .

ns2:VolumetricViableCount
  a owl:Class ;
  rdfs:label "viable count (volumetric)"@en ;
  rdfs:subClassOf ns2:Quantity, [
    a owl:Restriction ;
    owl:onProperty ns2:hasValue ;
    owl:allValuesFrom [
      a owl:Restriction ;
      owl:onProperty ns2:hasUnit ;
      owl:allValuesFrom ns2:VolumetricViableCountUnit
    ]
  ] ;
  ns2:commonlyHasUnit ns2:colonyFormingUnitPerMillilitre, ns2:colonyFormingUnitPer25Millilitre, ns2:_1000ColonyFormingUnitPerMillilitre .

ns2:VolumetricColiformBacterieCount
  a owl:Class ;
  rdfs:label "coliform bacteria count (volumetric)"@en ;
  rdfs:subClassOf ns2:VolumetricViableCount ;
  ns2:commonlyHasUnit ns2:colonyFormingUnitPerMillilitre, ns2:colonyFormingUnitPer25Millilitre, ns2:_1000ColonyFormingUnitPerMillilitre .

ns2:VolumetricCorynebacteriumCount
  a owl:Class ;
  rdfs:label "Corynebacterium count (volumetric)"@en ;
  ns2:alternativeLabel "Arcanobacterium count (volumetric)"@en ;
  rdfs:subClassOf ns2:VolumetricViableCount ;
  ns2:commonlyHasUnit ns2:colonyFormingUnitPerMillilitre, ns2:colonyFormingUnitPer25Millilitre, ns2:_1000ColonyFormingUnitPerMillilitre .

ns2:VolumetricCorynebacteriumBovisCount
  a owl:Class ;
  rdfs:label "Corynebacterium bovis count (volumetric)"@en ;
  rdfs:subClassOf ns2:VolumetricViableCount ;
  ns2:commonlyHasUnit ns2:colonyFormingUnitPerMillilitre, ns2:colonyFormingUnitPer25Millilitre, ns2:_1000ColonyFormingUnitPerMillilitre .

ns2:VolumetricEnterobacteriaceaeCount
  a owl:Class ;
  rdfs:label "Enterobacteriaceae count (volumetric)"@en ;
  rdfs:subClassOf ns2:VolumetricViableCount ;
  ns2:commonlyHasUnit ns2:colonyFormingUnitPerMillilitre, ns2:colonyFormingUnitPer25Millilitre, ns2:_1000ColonyFormingUnitPerMillilitre .

ns2:VolumetricEnterococcusCount
  a owl:Class ;
  rdfs:label "Enterococcus count (volumetric)"@en ;
  rdfs:subClassOf ns2:VolumetricViableCount ;
  ns2:commonlyHasUnit ns2:colonyFormingUnitPerMillilitre, ns2:colonyFormingUnitPer25Millilitre, ns2:_1000ColonyFormingUnitPerMillilitre .

ns2:VolumetricEscherichiaColiCount
  a owl:Class ;
  rdfs:label "Escherichia coli count (volumetric)"@en ;
  rdfs:subClassOf ns2:VolumetricViableCount ;
  ns2:commonlyHasUnit ns2:colonyFormingUnitPerMillilitre, ns2:colonyFormingUnitPer25Millilitre, ns2:_1000ColonyFormingUnitPerMillilitre .

ns2:VolumetricKlebsiellaCount
  a owl:Class ;
  rdfs:label "Klebsiella count (volumetric)"@en ;
  rdfs:subClassOf ns2:VolumetricViableCount ;
  ns2:commonlyHasUnit ns2:colonyFormingUnitPerMillilitre, ns2:colonyFormingUnitPer25Millilitre, ns2:_1000ColonyFormingUnitPerMillilitre .

ns2:VolumetricListeriaMonocytogenesCount
  a owl:Class ;
  rdfs:label "Listeria monocytogenes count (volumetric)"@en ;
  rdfs:subClassOf ns2:VolumetricViableCount ;
  ns2:commonlyHasUnit ns2:colonyFormingUnitPerMillilitre, ns2:colonyFormingUnitPer25Millilitre, ns2:_1000ColonyFormingUnitPerMillilitre .

ns2:VolumetricSalmonellaCount
  a owl:Class ;
  rdfs:label "Salmonella count (volumetric)"@en ;
  rdfs:subClassOf ns2:VolumetricViableCount ;
  ns2:commonlyHasUnit ns2:colonyFormingUnitPerMillilitre, ns2:colonyFormingUnitPer25Millilitre, ns2:_1000ColonyFormingUnitPerMillilitre .

ns2:VolumetricSerratiaMarcescensCount
  a owl:Class ;
  rdfs:label "Serratia marcescens count (volumetric)"@en ;
  rdfs:subClassOf ns2:VolumetricViableCount ;
  ns2:commonlyHasUnit ns2:colonyFormingUnitPerMillilitre, ns2:colonyFormingUnitPer25Millilitre, ns2:_1000ColonyFormingUnitPerMillilitre .

ns2:VolumetricStaphylococcusAureusCount
  a owl:Class ;
  rdfs:label "Staphylococcus aureus count (volumetric)"@en ;
  rdfs:subClassOf ns2:VolumetricViableCount ;
  ns2:commonlyHasUnit ns2:colonyFormingUnitPerMillilitre, ns2:colonyFormingUnitPer25Millilitre, ns2:_1000ColonyFormingUnitPerMillilitre .

ns2:VolumetricStreptococcusAgalactiaeCount
  a owl:Class ;
  rdfs:label "Streptococcus agalactiae count (volumetric)"@en ;
  rdfs:subClassOf ns2:VolumetricViableCount ;
  ns2:commonlyHasUnit ns2:colonyFormingUnitPerMillilitre, ns2:colonyFormingUnitPer25Millilitre, ns2:_1000ColonyFormingUnitPerMillilitre .

ns2:VolumetricStreptococcusDysgalactiaeCount
  a owl:Class ;
  rdfs:label "Streptococcus dysgalactiae count (volumetric)"@en ;
  rdfs:subClassOf ns2:VolumetricViableCount ;
  ns2:commonlyHasUnit ns2:colonyFormingUnitPerMillilitre, ns2:colonyFormingUnitPer25Millilitre, ns2:_1000ColonyFormingUnitPerMillilitre .

ns2:VolumetricStreptococcusUberisCount
  a owl:Class ;
  rdfs:label "Streptococcus uberis count (volumetric)"@en ;
  rdfs:subClassOf ns2:VolumetricViableCount ;
  ns2:commonlyHasUnit ns2:colonyFormingUnitPerMillilitre, ns2:colonyFormingUnitPer25Millilitre, ns2:_1000ColonyFormingUnitPerMillilitre .

ns2:VolumetricYeastAndFungiCount
  a owl:Class ;
  rdfs:label "yeast and fungi count (volumetric)"@en ;
  rdfs:subClassOf ns2:VolumetricViableCount ;
  ns2:commonlyHasUnit ns2:colonyFormingUnitPerMillilitre, ns2:colonyFormingUnitPer25Millilitre, ns2:_1000ColonyFormingUnitPerMillilitre .

ns2:SpecificViableCount
  a owl:Class ;
  rdfs:label "viable count (specific)"@en ;
  rdfs:subClassOf ns2:Quantity, [
    a owl:Restriction ;
    owl:onProperty ns2:hasValue ;
    owl:allValuesFrom [
      a owl:Restriction ;
      owl:onProperty ns2:hasUnit ;
      owl:allValuesFrom ns2:SpecificViableCountUnit
    ]
  ] ;
  ns2:commonlyHasUnit ns2:colonyFormingUnitPerGram .

ns2:SpecificColiformBacterieCount
  a owl:Class ;
  rdfs:label "coliform bacteria count (specific)"@en ;
  rdfs:subClassOf ns2:SpecificViableCount ;
  ns2:commonlyHasUnit ns2:colonyFormingUnitPerGram .

ns2:SpecificCorynebacteriumCount
  a owl:Class ;
  rdfs:label "Corynebacterium count (specific)"@en ;
  ns2:alternativeLabel "Arcanobacterium count (specific)"@en ;
  rdfs:subClassOf ns2:SpecificViableCount ;
  ns2:commonlyHasUnit ns2:colonyFormingUnitPerGram .

ns2:SpecificCorynebacteriumBovisCount
  a owl:Class ;
  rdfs:label "Corynebacterium bovis count (specific)"@en ;
  rdfs:subClassOf ns2:SpecificViableCount ;
  ns2:commonlyHasUnit ns2:colonyFormingUnitPerGram .

ns2:SpecificEnterobacteriaceaeCount
  a owl:Class ;
  rdfs:label "Enterobacteriaceae count (specific)"@en ;
  rdfs:subClassOf ns2:SpecificViableCount ;
  ns2:commonlyHasUnit ns2:colonyFormingUnitPerGram .

ns2:SpecificEnterococcusCount
  a owl:Class ;
  rdfs:label "Enterococcus count (specific)"@en ;
  rdfs:subClassOf ns2:SpecificViableCount ;
  ns2:commonlyHasUnit ns2:colonyFormingUnitPerGram .

ns2:SpecificEscherichiaColiCount
  a owl:Class ;
  rdfs:label "Escherichia coli count (specific)"@en ;
  rdfs:subClassOf ns2:SpecificViableCount ;
  ns2:commonlyHasUnit ns2:colonyFormingUnitPerGram .

ns2:SpecificKlebsiellaCount
  a owl:Class ;
  rdfs:label "Klebsiella count (specific)"@en ;
  rdfs:subClassOf ns2:SpecificViableCount ;
  ns2:commonlyHasUnit ns2:colonyFormingUnitPerGram .

ns2:SpecificListeriaMonocytogenesCount
  a owl:Class ;
  rdfs:label "Listeria monocytogenes count (specific)"@en ;
  rdfs:subClassOf ns2:SpecificViableCount ;
  ns2:commonlyHasUnit ns2:colonyFormingUnitPerGram .

ns2:SpecificSalmonellaCount
  a owl:Class ;
  rdfs:label "Salmonella count (specific)"@en ;
  rdfs:subClassOf ns2:SpecificViableCount ;
  ns2:commonlyHasUnit ns2:colonyFormingUnitPerGram .

ns2:SpecificSerratiaMarcescensCount
  a owl:Class ;
  rdfs:label "Serratia marcescens count (specific)"@en ;
  rdfs:subClassOf ns2:SpecificViableCount ;
  ns2:commonlyHasUnit ns2:colonyFormingUnitPerGram .

ns2:SpecificStaphylococcusAureusCount
  a owl:Class ;
  rdfs:label "Staphylococcus aureus count (specific)"@en ;
  rdfs:subClassOf ns2:SpecificViableCount ;
  ns2:commonlyHasUnit ns2:colonyFormingUnitPerGram .

ns2:SpecificStreptococcusAgalactiaeCount
  a owl:Class ;
  rdfs:label "Streptococcus agalactiae count (specific)"@en ;
  rdfs:subClassOf ns2:SpecificViableCount ;
  ns2:commonlyHasUnit ns2:colonyFormingUnitPerGram .

ns2:SpecificStreptococcusDysgalactiaeCount
  a owl:Class ;
  rdfs:label "Streptococcus dysgalactiae count (specific)"@en ;
  rdfs:subClassOf ns2:SpecificViableCount ;
  ns2:commonlyHasUnit ns2:colonyFormingUnitPerGram .

ns2:SpecificStreptococcusUberisCount
  a owl:Class ;
  rdfs:label "Streptococcus uberis count (specific)"@en ;
  rdfs:subClassOf ns2:SpecificViableCount ;
  ns2:commonlyHasUnit ns2:colonyFormingUnitPerGram .

ns2:SpecificYeastAndFungiCount
  a owl:Class ;
  rdfs:label "yeast and fungi count (specific)"@en ;
  rdfs:subClassOf ns2:SpecificViableCount ;
  ns2:commonlyHasUnit ns2:colonyFormingUnitPerGram .

ns2:colonyFormingUnit
  a ns2:Unit, ns2:SingularUnit, ns2:UnitDivision ;
  rdfs:label "colony forming unit"@en ;
  ns2:symbol "CFU" .

ns2:_1000ColonyFormingUnit
  a ns2:UnitMultiple, ns2:UnitDivision ;
  rdfs:label "1000 colony forming unit"@en ;
  ns2:symbol "1000 CFU" ;
  ns2:hasFactor "1000"^^xsd:float ;
  ns2:hasUnit ns2:colonyFormingUnit .

ns2:colonyFormingUnitPerGram
  a ns2:UnitDivision ;
  rdfs:label "colony forming unit per gram"@en ;
  ns2:symbol "CFU/g" ;
  ns2:hasNumerator ns2:colonyFormingUnit ;
  ns2:hasDenominator ns2:gram .

ns2:colonyFormingUnitPerMillilitre
  a ns2:UnitDivision ;
  rdfs:label "colony forming unit per millilitre"@en ;
  ns2:symbol "CFU/ml" ;
  ns2:hasNumerator ns2:colonyFormingUnit ;
  ns2:hasDenominator ns2:millilitre .

ns2:colonyFormingUnitPer25Millilitre
  a ns2:UnitDivision ;
  rdfs:label "colony forming unit per 25 millilitre"@en ;
  ns2:symbol "CFU/ml" ;
  ns2:hasNumerator ns2:colonyFormingUnit ;
  ns2:hasDenominator ns2:_25Millilitre .

ns2:_1000ColonyFormingUnitPerMillilitre
  a ns2:UnitDivision ;
  rdfs:label "1000 colony forming unit per millilitre"@en ;
  ns2:unofficialAbbreviation "1000 CFU/ml" ;
  ns2:symbol "1000 CFU/ml" ;
  ns2:hasNumerator ns2:_1000ColonyFormingUnit ;
  ns2:hasDenominator ns2:millilitre .

ns2:ViableCountUnit
  a owl:Class ;
  rdfs:label "viable count unit"@en ;
  rdfs:subClassOf ns2:Unit ;
  owl:equivalentClass [
    a owl:Class ;
    owl:oneOf (
     ns2:colonyFormingUnit
     ns2:_1000ColonyFormingUnit
   )
  ] .

ns2:VolumetricViableCountUnit
  a owl:Class ;
  rdfs:label "volumetric viable count unit"@en ;
  rdfs:subClassOf ns2:Unit ;
  owl:equivalentClass [
    a owl:Class ;
    owl:oneOf (
     ns2:colonyFormingUnitPerMillilitre
     ns2:colonyFormingUnitPer25Millilitre
     ns2:_1000ColonyFormingUnitPerMillilitre
   )
  ] .

ns2:SpecificViableCountUnit
  a owl:Class ;
  rdfs:label "specific viable count unit"@en ;
  rdfs:subClassOf ns2:Unit ;
  owl:equivalentClass [
    a owl:Class ;
    owl:oneOf ( ns2:colonyFormingUnitPerGram )
  ] .

ns2:acoustics
  a ns2:ApplicationArea ;
  rdfs:label "acoustics"@en, "akoestiek"@nl ;
  ns2:usesUnit ns2:bel, ns2:decibel .

ns2:bel
  a ns2:Unit, ns2:SingularUnit ;
  rdfs:label "bel"@en, "bel"@nl ;
  ns2:symbol "B" .

ns2:decibel
  a ns2:PrefixedUnit ;
  rdfs:label "decibel"@en, "decibel"@nl ;
  ns2:symbol "dB" ;
  ns2:hasPrefix ns2:deci ;
  ns2:hasUnit ns2:bel .

ns2:sustainability
  a ns2:ApplicationArea ;
  rdfs:label "sustainability"@en, "duurzaamheid"@nl ;
  ns2:usesQuantity ns2:CarbonDioxideEquivalentMass, ns2:CarbonDioxideEquivalentMassPerEnergy ;
  ns2:usesUnit ns2:gramOfCarbonDioxideEquivalent, ns2:kilogramOfCarbonDioxideEquivalent, ns2:tonneOfCarbonDioxideEquivalent, ns2:gramOfCarbonDioxideEquivalentPerKilowattHour, ns2:kilogramOfCarbonDioxideEquivalentPerMegaWattHour, ns2:tonneOfCarbonDioxideEquivalentPerGigaWattHour .

ns2:CarbonDioxideEquivalentMass
  a owl:Class ;
  rdfs:label "carbon dioxide equivalent mass"@en ;
  rdfs:subClassOf ns2:Mass, [
    a owl:Restriction ;
    owl:onProperty ns2:hasValue ;
    owl:allValuesFrom [
      a owl:Restriction ;
      owl:onProperty ns2:hasUnit ;
      owl:allValuesFrom ns2:CarbonDioxideEquivalentMassUnit
    ]
  ] ;
  ns2:commonlyHasUnit ns2:gramOfCarbonDioxideEquivalent, ns2:kilogramOfCarbonDioxideEquivalent, ns2:tonneOfCarbonDioxideEquivalent .

ns2:CarbonDioxideEquivalentMassPerEnergy
  a owl:Class ;
  rdfs:label "carbon dioxide equivalent mass per energy"@en ;
  rdfs:subClassOf ns2:MassPerEnergy, [
    a owl:Restriction ;
    owl:onProperty ns2:hasValue ;
    owl:allValuesFrom [
      a owl:Restriction ;
      owl:onProperty ns2:hasUnit ;
      owl:allValuesFrom ns2:CarbonDioxideEquivalentMassPerEnergyUnit
    ]
  ] ;
  ns2:commonlyHasUnit ns2:gramOfCarbonDioxideEquivalentPerKilowattHour, ns2:kilogramOfCarbonDioxideEquivalentPerMegaWattHour, ns2:tonneOfCarbonDioxideEquivalentPerGigawattHour .

ns2:gramOfCarbonDioxideEquivalent
  a ns2:Unit, ns2:SingularUnit ;
  rdfs:label "gram of carbon dioxide equivalent"@en ;
  ns2:symbol "gCO2eq" ;
  ns2:hasFactor "1"^^xsd:float ;
  ns2:hasUnit ns2:gram .

ns2:kilogramOfCarbonDioxideEquivalent
  a ns2:PrefixedUnit ;
  rdfs:label "kilogram of carbon dioxide equivalent"@en ;
  ns2:symbol "kgCO2eq" ;
  ns2:hasPrefix ns2:kilo ;
  ns2:hasUnit ns2:gramOfCarbonDioxideEquivalent .

ns2:tonneOfCarbonDioxideEquivalent
  a ns2:Unit, ns2:SingularUnit ;
  rdfs:label "tonne of carbon dioxide equivalent"@en ;
  ns2:symbol "tCO2eq" ;
  ns2:hasFactor "1"^^xsd:float ;
  ns2:hasUnit ns2:tonne .

ns2:CarbonDioxideEquivalentMassUnit
  a owl:Class ;
  rdfs:label "carbon dioxide equivalent mass unit"@en ;
  rdfs:subClassOf ns2:MassUnit ;
  owl:equivalentClass [
    a owl:Class ;
    owl:oneOf (
     ns2:gramOfCarbonDioxideEquivalent
     ns2:kilogramOfCarbonDioxideEquivalent
     ns2:tonneOfCarbonDioxideEquivalent
   )
  ] .

ns2:gramOfCarbonDioxideEquivalentPerKilowattHour
  a ns2:UnitDivision, ns2:Unit ;
  rdfs:label "gram of carbon dioxide equivalent per kilowatt hour"@en ;
  ns2:symbol "gCO2eq/kWh" ;
  ns2:hasNumerator ns2:gramOfCarbonDioxideEquivalent ;
  ns2:hasDenominator ns2:kilowattHour .

ns2:kilogramOfCarbonDioxideEquivalentPerMegawattHour
  a ns2:UnitDivision, ns2:PrefixedUnit ;
  rdfs:label "kilogram of carbon dioxide equivalent per megawatt hour"@en ;
  ns2:symbol "kgCO2eq/MWh" ;
  ns2:hasNumerator ns2:kilogramOfCarbonDioxideEquivalent ;
  ns2:hasDenominator ns2:megawattHour .

ns2:tonneOfCarbonDioxideEquivalentPerGigawattHour
  a ns2:UnitDivision, ns2:Unit ;
  rdfs:label "tonne of carbon dioxide equivalent per gigawatt hour"@en ;
  ns2:symbol "tCO2eq/GWh" ;
  ns2:hasNumerator ns2:tonneOfCarbonDioxideEquivalent ;
  ns2:hasDenominator ns2:gigawattHour .

ns2:CarbonDioxideEquivalentMassPerEnergyUnit
  a owl:Class ;
  rdfs:label "carbon dioxide equivalent mass per energy unit"@en ;
  rdfs:subClassOf ns2:MassPerEnergyUnit ;
  owl:equivalentClass [
    a owl:Class ;
    owl:oneOf (
     ns2:gramOfCarbonDioxideEquivalentPerKilowattHour
     ns2:kilogramOfCarbonDioxideEquivalentPerMegawattHour
     ns2:tonneOfCarbonDioxideEquivalentPerGigawattHour
   )
  ] .

ns2:economics
  a ns2:ApplicationArea ;
  rdfs:label "economics"@en, "economie"@nl ;
  ns2:usesQuantity ns2:AmountOfMoney, ns2:SpecificAmountOfMoney, ns2:Cost ;
  ns2:usesUnit ns2:UnitedStatesDollar, ns2:euro, ns2:JapaneseYen, ns2:poundSterling, ns2:AustralianDollar, ns2:SwissFranc, ns2:CanadianDollar, ns2:MexicanPeso, ns2:ChineseYuan, ns2:NewZealandDollar, ns2:SwedishKrona, ns2:RussianRuble, ns2:HongKongDollar, ns2:NorwegianKrone, ns2:SingaporeDollar, ns2:TurkishLira, ns2:SouthKoreanWon, ns2:SouthAfricanRand, ns2:BrazilianReal, ns2:IndianRupee, ns2:megaeuro, ns2:euroPerTonne, ns2:megaeuroPerMegatonne .

ns2:AmountOfMoney
  a owl:Class ;
  rdfs:label "amount of money"@en ;
  rdfs:subClassOf ns2:Quantity, [
    a owl:Restriction ;
    owl:onProperty ns2:hasValue ;
    owl:allValuesFrom [
      a owl:Restriction ;
      owl:onProperty ns2:hasUnit ;
      owl:allValuesFrom ns2:AmountOfMoneyUnit
    ]
  ] ;
  ns2:commonlyHasUnit ns2:euro, ns2:megaeuro, ns2:UnitedStatesDollar, ns2:JapaneseYen, ns2:poundSterling, ns2:AustralianDollar, ns2:SwissFranc, ns2:CanadianDollar, ns2:MexicanPeso, ns2:ChineseYuan, ns2:NewZealandDollar, ns2:SwedishKrona, ns2:RussianRuble, ns2:HongKongDollar, ns2:NorwegianKrone, ns2:SingaporeDollar, ns2:TurkishLira, ns2:SouthKoreanWon, ns2:SouthAfricanRand, ns2:BrazilianReal, ns2:IndianRupee .

ns2:Cost
  a owl:Class ;
  rdfs:label "cost"@en ;
  rdfs:subClassOf ns2:AmountOfMoney ;
  ns2:commonlyHasUnit ns2:euro, ns2:megaeuro, ns2:UnitedStatesDollar, ns2:JapaneseYen, ns2:poundSterling, ns2:AustralianDollar, ns2:SwissFranc, ns2:CanadianDollar, ns2:MexicanPeso, ns2:ChineseYuan, ns2:NewZealandDollar, ns2:SwedishKrona, ns2:RussianRuble, ns2:HongKongDollar, ns2:NorwegianKrone, ns2:SingaporeDollar, ns2:TurkishLira, ns2:SouthKoreanWon, ns2:SouthAfricanRand, ns2:BrazilianReal, ns2:IndianRupee .

ns2:SpecificAmountOfMoney
  a owl:Class ;
  rdfs:label "specific amount of money"@en ;
  rdfs:subClassOf ns2:Quantity, [
    a owl:Restriction ;
    owl:onProperty ns2:hasValue ;
    owl:allValuesFrom [
      a owl:Restriction ;
      owl:onProperty ns2:hasUnit ;
      owl:allValuesFrom ns2:SpecificAmountOfMoneyUnit
    ]
  ] ;
  ns2:commonlyHasUnit ns2:euroPerTonne, ns2:megaeuroPerMegatonne .

ns2:SpecificCost
  a owl:Class ;
  rdfs:label "specific cost"@en ;
  rdfs:subClassOf ns2:SpecificAmountOfMoney ;
  ns2:commonlyHasUnit ns2:euroPerTonne, ns2:megaeuroPerMegatonne .

ns2:euro
  a ns2:Unit, ns2:SingularUnit ;
  rdfs:label "euro"@en, "欧元"@zh .

ns2:megaeuro
  a ns2:PrefixedUnit ;
  rdfs:label "megaeuro"@en ;
  ns2:hasPrefix ns2:mega ;
  ns2:hasUnit ns2:euro .

ns2:UnitedStatesDollar
  a ns2:Unit, ns2:SingularUnit ;
  rdfs:label "United States dollar"@en, "美国美元"@zh .

ns2:JapaneseYen
  a ns2:Unit, ns2:SingularUnit ;
  rdfs:label "Japanese yen"@en, "日元"@zh .

ns2:poundSterling
  a ns2:Unit, ns2:SingularUnit ;
  rdfs:label "pound sterling"@en, "英镑"@zh .

ns2:AustralianDollar
  a ns2:Unit, ns2:SingularUnit ;
  rdfs:label "Australian dollar"@en, "澳元"@zh .

ns2:SwissFranc
  a ns2:Unit, ns2:SingularUnit ;
  rdfs:label "Swiss franc"@en, "瑞士法郎"@zh .

ns2:CanadianDollar
  a ns2:Unit, ns2:SingularUnit ;
  rdfs:label "Canadian dollar"@en, "加元"@zh .

ns2:MexicanPeso
  a ns2:Unit, ns2:SingularUnit ;
  rdfs:label "Mexican peso"@en, "墨西哥比索"@zh .

ns2:ChineseYuan
  a ns2:Unit, ns2:SingularUnit ;
  rdfs:label "Chinese yuan"@en, "中国元"@zh .

ns2:NewZealandDollar
  a ns2:Unit, ns2:SingularUnit ;
  rdfs:label "New Zealand dollar"@en, "新西兰美元"@zh .

ns2:SwedishKrona
  a ns2:Unit, ns2:SingularUnit ;
  rdfs:label "Swedish krona"@en, "瑞典克朗"@zh .

ns2:RussianRuble
  a ns2:Unit, ns2:SingularUnit ;
  rdfs:label "RussianRuble"@en, "俄罗斯卢布"@zh .

ns2:HongKongDollar
  a ns2:Unit, ns2:SingularUnit ;
  rdfs:label "Hong Kong dollar"@en, "港元"@zh .

ns2:NorwegianKrone
  a ns2:Unit, ns2:SingularUnit ;
  rdfs:label "Norwegian krone"@en, "挪威克朗"@zh .

ns2:SingaporeDollar
  a ns2:Unit, ns2:SingularUnit ;
  rdfs:label "Singapore dollar"@en, "新加坡元"@zh .

ns2:TurkishLira
  a ns2:Unit, ns2:SingularUnit ;
  rdfs:label "Turkish lira"@en, "土耳其里拉"@zh .

ns2:SouthKoreanWon
  a ns2:Unit, ns2:SingularUnit ;
  rdfs:label "South Korean won"@en, "韩元"@zh .

ns2:SouthAfricanRand
  a ns2:Unit, ns2:SingularUnit ;
  rdfs:label "South African rand"@en, "南非兰特"@zh .

ns2:BrazilianReal
  a ns2:Unit, ns2:SingularUnit ;
  rdfs:label "Brazilian real"@en, "巴西里拉"@zh .

ns2:IndianRupee
  a ns2:Unit, ns2:SingularUnit ;
  rdfs:label "Indian rupee"@en, "印度卢比"@zh .

ns2:AmountOfMoneyUnit
  a owl:Class ;
  rdfs:label "amount of money unit"@en ;
  rdfs:subClassOf ns2:Unit ;
  owl:equivalentClass [
    a owl:Class ;
    owl:oneOf (
     ns2:UnitedStatesDollar
     ns2:euro
     ns2:JapaneseYen
     ns2:poundSterling
     ns2:AustralianDollar
     ns2:SwissFranc
     ns2:CanadianDollar
     ns2:MexicanPeso
     ns2:ChineseYuan
     ns2:NewZealandDollar
     ns2:SwedishKrona
     ns2:RussianRuble
     ns2:HongKongDollar
     ns2:NorwegianKrone
     ns2:SingaporeDollar
     ns2:TurkishLira
     ns2:SouthKoreanWon
     ns2:SouthAfricanRand
     ns2:BrazilianReal
     ns2:IndianRupee
     ns2:megaeuro
   )
  ] .

ns2:euroPerTonne
  a ns2:UnitDivision ;
  rdfs:label "euro per tonne"@en ;
  ns2:hasNumerator ns2:euro ;
  ns2:hasDenominator ns2:tonne .

ns2:megaeuroPerMegatonne
  a ns2:UnitDivision ;
  rdfs:label "megaeuro per megatonne"@en ;
  ns2:hasNumerator ns2:megaeuro ;
  ns2:hasDenominator ns2:megatonne .

ns2:SpecificAmountOfMoneyUnit
  a owl:Class ;
  rdfs:label "specific amount of money unit"@en ;
  rdfs:subClassOf ns2:Unit ;
  owl:equivalentClass [
    a owl:Class ;
    owl:oneOf (
     ns2:euroPerTonne
     ns2:megaeuroPerMegatonne
   )
  ] .

ns2:informationTechnology
  a ns2:ApplicationArea ;
  rdfs:label "information technology"@en, "informatietechnologie"@nl ;
  ns2:usesQuantity ns2:InformationCapacity, ns2:SymbolRate, ns2:PixelCount ;
  ns2:usesUnit ns2:bit, ns2:byte, ns2:hartley, ns2:shannon, ns2:kibibit, ns2:mebibit, ns2:gibibit, ns2:tebibit, ns2:pebibit, ns2:exbibit, ns2:zebibit, ns2:yobibit, ns2:kilobit, ns2:megabit, ns2:gigabit, ns2:terabit, ns2:petabit, ns2:exabit, ns2:zettabit, ns2:yottabit, ns2:bitPerSecond-Time, ns2:pixel .

ns2:InformationCapacity
  a owl:Class ;
  rdfs:label "information capacity"@en, "informatiecapaciteit"@nl ;
  rdfs:subClassOf ns2:Quantity, [
    a owl:Restriction ;
    owl:onProperty ns2:hasValue ;
    owl:allValuesFrom [
      a owl:Restriction ;
      owl:onProperty ns2:hasUnit ;
      owl:allValuesFrom ns2:InformationCapacityUnit
    ]
  ] ;
  ns2:commonlyHasUnit ns2:bit, ns2:kibibit, ns2:mebibit, ns2:gibibit, ns2:tebibit, ns2:pebibit, ns2:exbibit, ns2:zebibit, ns2:yobibit, ns2:kilobit, ns2:megabit, ns2:gigabit, ns2:terabit, ns2:petabit, ns2:exabit, ns2:zettabit, ns2:yottabit, ns2:byte, ns2:kibibyte, ns2:mebibyte, ns2:gibibyte, ns2:tebibyte, ns2:pebibyte, ns2:exbibyte, ns2:zebibyte, ns2:yobibyte, ns2:kilobyte, ns2:megabyte, ns2:gigabyte, ns2:terabyte, ns2:petabyte, ns2:exabyte, ns2:zettabyte, ns2:yottabyte, ns2:hartley, ns2:shannon .

ns2:SymbolRate
  a owl:Class ;
  rdfs:label "symbol rate"@en ;
  ns2:alternativeLabel "baud rate"@en, "modulation rate"@en ;
  rdfs:comment "Symbol rate is the number of symbol changes (signalling events) made to the transmission medium per second using a digitally modulated signal or a line code."@en ;
  rdfs:subClassOf ns2:Quantity, [
    a owl:Restriction ;
    owl:onProperty ns2:hasValue ;
    owl:allValuesFrom [
      a owl:Restriction ;
      owl:onProperty ns2:hasUnit ;
      owl:allValuesFrom ns2:SymbolRateUnit
    ]
  ] ;
  ns2:commonlyHasUnit ns2:baud .

ns2:PixelCount
  a owl:Class ;
  rdfs:label "pixel count"@en ;
  rdfs:subClassOf ns2:Quantity, [
    a owl:Restriction ;
    owl:onProperty ns2:hasValue ;
    owl:allValuesFrom [
      a owl:Restriction ;
      owl:onProperty ns2:hasUnit ;
      owl:allValuesFrom ns2:PixelCountUnit
    ]
  ] .

ns2:BinaryPrefix
  a owl:Class ;
  rdfs:label "binary prefix"@en ;
  rdfs:comment "IEC prefix"@en ;
  rdfs:subClassOf ns2:Prefix .

ns2:kibi
  a ns2:BinaryPrefix ;
  rdfs:label "kibi"@en, "kibi"@nl ;
  ns2:alternativeLabel "kilobinary"@en ;
  rdfs:comment "IEC prefix"@en ;
  ns2:symbol "Ki" ;
  ns2:hasFactor "1.024e3"^^xsd:float .

ns2:mebi
  a ns2:BinaryPrefix ;
  rdfs:label "mebi"@en, "mebi"@nl ;
  ns2:alternativeLabel "megabinary"@en ;
  rdfs:comment "IEC prefix"@en ;
  ns2:symbol "Mi" ;
  ns2:hasFactor "1.048576e6"^^xsd:float .

ns2:gibi
  a ns2:BinaryPrefix ;
  rdfs:label "gibi"@en, "gibi"@nl ;
  ns2:alternativeLabel "gigabinary"@en ;
  rdfs:comment "IEC prefix"@en ;
  ns2:symbol "Gi" ;
  ns2:hasFactor "1.073741824e9"^^xsd:float .

ns2:tebi
  a ns2:BinaryPrefix ;
  rdfs:label "tebi"@en, "tebi"@nl ;
  ns2:alternativeLabel "terabinary"@en ;
  rdfs:comment "IEC prefix"@en ;
  ns2:symbol "Ti" ;
  ns2:hasFactor "1.099511627776e12"^^xsd:float .

ns2:pebi
  a ns2:BinaryPrefix ;
  rdfs:label "pebi"@en, "pebi"@nl ;
  ns2:alternativeLabel "petabinary"@en ;
  rdfs:comment "IEC prefix"@en ;
  ns2:symbol "Pi" ;
  ns2:hasFactor "1.125899906842624e15"^^xsd:float .

ns2:exbi
  a ns2:BinaryPrefix ;
  rdfs:label "exbi"@en, "exbi"@nl ;
  ns2:alternativeLabel "exabinary"@en ;
  rdfs:comment "IEC prefix"@en ;
  ns2:symbol "Ei" ;
  ns2:hasFactor "1.152921504606846976e18"^^xsd:float .

ns2:zebi
  a ns2:BinaryPrefix ;
  rdfs:label "zebi"@en, "zebi"@nl ;
  rdfs:comment "IEC prefix"@en ;
  ns2:symbol "Zi" ;
  ns2:hasFactor "1.180591620717411303424e21"^^xsd:float .

ns2:yobi
  a ns2:BinaryPrefix ;
  rdfs:label "yobi"@en, "yobi"@nl ;
  rdfs:comment "IEC prefix"@en ;
  ns2:symbol "Yi" ;
  ns2:hasFactor "1.208925819614629174706176e24"^^xsd:float .

ns2:bit
  a ns2:Unit, ns2:SingularUnit ;
  rdfs:label "bit"@en, "bit"@nl, "指二进制中的一位"@zh ;
  ns2:symbol "bit" ;
  rdfs:comment "The bit is a unit of information capacity defined as the information capacity of one binary digit."@en ;
  ns2:hasQuantity ns2:informationCapacityOfOneBinaryDigit .

ns2:oneBinaryDigit
  a owl:Thing ;
  rdfs:label "one binary digit"@en .

ns2:informationCapacityOfOneBinaryDigit
  a ns2:InformationCapacity ;
  rdfs:label "information capacity of one binary digit"@en ;
  ns2:hasPhenomenon ns2:oneBinaryDigit .

ns2:InformationCapacityUnit
  a owl:Class ;
  rdfs:label "information capacity unit"@en ;
  rdfs:subClassOf ns2:Unit ;
  owl:equivalentClass [
    a owl:Class ;
    owl:unionOf (
     _:genid1904
     ns2:PrefixedBit
     ns2:PrefixedByte
   )
  ] .

ns2:byte
  a ns2:Unit, ns2:SingularUnit ;
  rdfs:label "byte"@en, "byte"@nl, "字节"@zh ;
  rdfs:comment "The byte is a unit of information capacity defined as 8 bit."@en ;
  ns2:symbol "B" ;
  ns2:hasFactor "8"^^xsd:float ;
  ns2:hasUnit ns2:bit .

ns2:hartley
  a ns2:Unit, ns2:SingularUnit ;
  rdfs:label "hartley"@en, "hartley"@nl ;
  rdfs:comment "The hartley is a unit of information capacity defined as 3.321928095 bit."@en ;
  ns2:symbol "Hart" ;
  ns2:hasFactor "3.321928095"^^xsd:float ;
  ns2:hasUnit ns2:bit .

ns2:shannon
  a ns2:Unit, ns2:SingularUnit ;
  rdfs:label "shannon"@en, "shannon"@nl ;
  rdfs:comment "The shannon is a unit of information capacity defined as 1 bit."@en ;
  ns2:symbol "Sh" ;
  ns2:hasUnit ns2:bit .

ns2:PrefixedBit
  a owl:Class ;
  rdfs:label "prefixed bit"@en ;
  rdfs:subClassOf ns2:PrefixedUnit ;
  owl:equivalentClass [
    a owl:Class ;
    owl:intersectionOf (
     _:genid1915
     _:genid1917
     _:genid1919
     _:genid1921
   )
  ] .

ns2:PrefixedByte
  a owl:Class ;
  rdfs:label "prefixed byte"@en ;
  rdfs:subClassOf ns2:PrefixedUnit ;
  owl:equivalentClass [
    a owl:Class ;
    owl:intersectionOf (
     _:genid1924
     _:genid1926
     _:genid1928
     _:genid1930
   )
  ] .

ns2:kibibit
  a ns2:PrefixedUnit ;
  rdfs:label "kibibit"@en, "kibibit"@nl ;
  ns2:symbol "Kibit" ;
  ns2:hasPrefix ns2:kibi ;
  ns2:hasUnit ns2:bit .

ns2:mebibit
  a ns2:PrefixedUnit ;
  rdfs:label "mebibit"@en, "mebibit"@nl ;
  ns2:symbol "Mibit" ;
  ns2:hasPrefix ns2:mebi ;
  ns2:hasUnit ns2:bit .

ns2:gibibit
  a ns2:PrefixedUnit ;
  rdfs:label "gibibit"@en, "gibibit"@nl ;
  ns2:symbol "Gibit" ;
  ns2:hasPrefix ns2:gibi ;
  ns2:hasUnit ns2:bit .

ns2:tebibit
  a ns2:PrefixedUnit ;
  rdfs:label "tebibit"@en, "tebibit"@nl ;
  ns2:symbol "Tibit" ;
  ns2:hasPrefix ns2:tebi ;
  ns2:hasUnit ns2:bit .

ns2:pebibit
  a ns2:PrefixedUnit ;
  rdfs:label "pebibit"@en, "pebibit"@nl ;
  ns2:symbol "Pibit" ;
  ns2:hasPrefix ns2:pebi ;
  ns2:hasUnit ns2:bit .

ns2:exbibit
  a ns2:PrefixedUnit ;
  rdfs:label "exbibit"@en, "exbibit"@nl ;
  ns2:symbol "Eibit" ;
  ns2:hasPrefix ns2:exbi ;
  ns2:hasUnit ns2:bit .

ns2:zebibit
  a ns2:PrefixedUnit ;
  rdfs:label "zebibit"@en, "zebibit"@nl ;
  ns2:symbol "Zibit" ;
  ns2:hasPrefix ns2:zebi ;
  ns2:hasUnit ns2:bit .

ns2:yobibit
  a ns2:PrefixedUnit ;
  rdfs:label "yobibit"@en, "yobibit"@nl ;
  ns2:symbol "Yibit" ;
  ns2:hasPrefix ns2:yobi ;
  ns2:hasUnit ns2:bit .

ns2:kilobit
  a ns2:PrefixedUnit ;
  rdfs:label "kilobit"@en, "kilobit"@nl ;
  ns2:symbol "kbit" ;
  ns2:hasPrefix ns2:kilo ;
  ns2:hasUnit ns2:bit .

ns2:megabit
  a ns2:PrefixedUnit ;
  rdfs:label "megabit"@en, "megabit"@nl ;
  ns2:symbol "Mbit" ;
  ns2:hasPrefix ns2:mega ;
  ns2:hasUnit ns2:bit .

ns2:gigabit
  a ns2:PrefixedUnit ;
  rdfs:label "gigabit"@en, "gigabit"@nl ;
  ns2:symbol "Gbit" ;
  ns2:hasPrefix ns2:giga ;
  ns2:hasUnit ns2:bit .

ns2:terabit
  a ns2:PrefixedUnit ;
  rdfs:label "terabit"@en, "terabit"@nl ;
  ns2:symbol "Tbit" ;
  ns2:hasPrefix ns2:tera ;
  ns2:hasUnit ns2:bit .

ns2:petabit
  a ns2:PrefixedUnit ;
  rdfs:label "petabit"@en, "petabit"@nl ;
  ns2:symbol "Pbit" ;
  ns2:hasPrefix ns2:peta ;
  ns2:hasUnit ns2:bit .

ns2:exabit
  a ns2:PrefixedUnit ;
  rdfs:label "exabit"@en, "exabit"@nl ;
  ns2:symbol "Ebit" ;
  ns2:hasPrefix ns2:exa ;
  ns2:hasUnit ns2:bit .

ns2:zettabit
  a ns2:PrefixedUnit ;
  rdfs:label "zettabit"@en, "zettabit"@nl ;
  ns2:symbol "Zbit" ;
  ns2:hasPrefix ns2:zetta ;
  ns2:hasUnit ns2:bit .

ns2:yottabit
  a ns2:PrefixedUnit ;
  rdfs:label "yottabit"@en, "yottabit"@nl ;
  ns2:symbol "Ybit" ;
  ns2:hasPrefix ns2:yotta ;
  ns2:hasUnit ns2:bit .

ns2:kibibyte
  a ns2:PrefixedUnit ;
  rdfs:label "kibibyte"@en, "kibibyte"@nl ;
  ns2:symbol "KiB" ;
  ns2:hasPrefix ns2:kibi ;
  ns2:hasUnit ns2:byte .

ns2:mebibyte
  a ns2:PrefixedUnit ;
  rdfs:label "mebibyte"@en, "mebibyte"@nl ;
  ns2:symbol "MiB" ;
  ns2:hasPrefix ns2:mebi ;
  ns2:hasUnit ns2:byte .

ns2:gibibyte
  a ns2:PrefixedUnit ;
  rdfs:label "gibibyte"@en, "gibibyte"@nl ;
  ns2:symbol "GiB" ;
  ns2:hasPrefix ns2:gibi ;
  ns2:hasUnit ns2:byte .

ns2:tebibyte
  a ns2:PrefixedUnit ;
  rdfs:label "tebibyte"@en, "tebibyte"@nl ;
  ns2:symbol "TiB" ;
  ns2:hasPrefix ns2:tebi ;
  ns2:hasUnit ns2:byte .

ns2:pebibyte
  a ns2:PrefixedUnit ;
  rdfs:label "pebibyte"@en, "pebibyte"@nl ;
  ns2:symbol "PiB" ;
  ns2:hasPrefix ns2:pebi ;
  ns2:hasUnit ns2:byte .

ns2:exbibyte
  a ns2:PrefixedUnit ;
  rdfs:label "exbibyte"@en, "exbibyte"@nl ;
  ns2:symbol "EiB" ;
  ns2:hasPrefix ns2:exbi ;
  ns2:hasUnit ns2:byte .

ns2:zebibyte
  a ns2:PrefixedUnit ;
  rdfs:label "zebibyte"@en, "zebibyte"@nl ;
  ns2:symbol "ZiB" ;
  ns2:hasPrefix ns2:zebi ;
  ns2:hasUnit ns2:byte .

ns2:yobibyte
  a ns2:PrefixedUnit ;
  rdfs:label "yobibyte"@en, "yobibyte"@nl ;
  ns2:symbol "YiB" ;
  ns2:hasPrefix ns2:yobi ;
  ns2:hasUnit ns2:byte .

ns2:kilobyte
  a ns2:PrefixedUnit ;
  rdfs:label "kilobyte"@en, "kilobyte"@nl ;
  ns2:symbol "kB" ;
  ns2:hasPrefix ns2:kilo ;
  ns2:hasUnit ns2:byte .

ns2:megabyte
  a ns2:PrefixedUnit ;
  rdfs:label "megabyte"@en, "megabyte"@nl, "百万字节"@zh ;
  ns2:symbol "MB" ;
  ns2:hasPrefix ns2:mega ;
  ns2:hasUnit ns2:byte .

ns2:gigabyte
  a ns2:PrefixedUnit ;
  rdfs:label "gigabyte"@en, "gigabyte"@nl ;
  ns2:symbol "GB" ;
  ns2:hasPrefix ns2:giga ;
  ns2:hasUnit ns2:byte .

ns2:terabyte
  a ns2:PrefixedUnit ;
  rdfs:label "terabyte"@en, "terabyte"@nl, "10^12字节"@zh ;
  ns2:symbol "TB" ;
  ns2:hasPrefix ns2:tera ;
  ns2:hasUnit ns2:byte .

ns2:petabyte
  a ns2:PrefixedUnit ;
  rdfs:label "petabyte"@en, "petabyte"@nl, "10^15字节"@zh ;
  ns2:symbol "PB" ;
  ns2:hasPrefix ns2:peta ;
  ns2:hasUnit ns2:byte .

ns2:exabyte
  a ns2:PrefixedUnit ;
  rdfs:label "exabyte"@en, "exabyte"@nl, "千兆兆字节"@zh ;
  ns2:symbol "EB" ;
  ns2:hasPrefix ns2:exa ;
  ns2:hasUnit ns2:byte .

ns2:zettabyte
  a ns2:PrefixedUnit ;
  rdfs:label "zettabyte"@en, "zettabyte"@nl, "10^21字节"@zh ;
  ns2:symbol "ZB" ;
  ns2:hasPrefix ns2:zetta ;
  ns2:hasUnit ns2:byte .

ns2:yottabyte
  a ns2:PrefixedUnit ;
  rdfs:label "yottabyte"@en, "yottabyte"@nl, "10^24字节"@zh ;
  ns2:symbol "YB" ;
  ns2:hasPrefix ns2:yotta ;
  ns2:hasUnit ns2:byte .

ns2:baud
  a ns2:Unit, ns2:SingularUnit ;
  rdfs:label "baud"@en, "baud"@nl ;
  ns2:symbol "Bd" ;
  rdfs:comment "The baud is a unit of symbol rate defined as one distinct symbol change or signalling event made to the transmission medium per second in a digitally modulated signal or a line code."@en ;
  ns2:hasQuantity ns2:oneDistinctSymbolChangeOrSignallingEventMadeToTheTransmissionMediumPerSecondInADigitallyModulatedSignalOrALineCode .

ns2:oneDistinctSymbolChangeOrSignallingEventMadeToTheTransmissionMediumPerSecondInADigitallyModulatedSignalOrALineCode a ns2:SymbolRate .
ns2:SymbolRateUnit
  a owl:Class ;
  rdfs:label "symbol rate unit"@en ;
  rdfs:subClassOf ns2:Unit ;
  owl:equivalentClass [
    a owl:Class ;
    owl:oneOf ( ns2:baud )
  ] .

ns2:bitPerSecond-Time
  a ns2:UnitDivision ;
  rdfs:label "bit per second"@en, "bit per seconde"@nl ;
  ns2:symbol "bit/s" ;
  ns2:alternativeSymbol "bit s-1", "bit·s-1" ;
  ns2:hasNumerator ns2:bit ;
  ns2:hasDenominator ns2:second-Time .

ns2:pixel
  a ns2:Unit, ns2:SingularUnit ;
  rdfs:label "pixel"@en, "pixel"@nl .

ns2:PixelCountUnit
  a owl:Class ;
  rdfs:label "pixel count unit"@en ;
  rdfs:subClassOf ns2:Unit ;
  owl:equivalentClass [
    a owl:Class ;
    owl:oneOf ( ns2:pixel )
  ] .

ns2:typography
  a ns2:ApplicationArea ;
  rdfs:label "typography"@en, "typografie"@nl ;
  ns2:usesQuantity ns2:FontSize ;
  ns2:usesUnit ns2:cicero, ns2:pica-ATA, ns2:pica-Postscript, ns2:pica-TeX, ns2:point-ATA, ns2:point-Didot, ns2:point-Postscript, ns2:point-TeX .

ns2:FontSize
  a owl:Class ;
  rdfs:label "font size"@en, "fontgrootte"@nl ;
  rdfs:subClassOf ns2:Length, [
    a owl:Restriction ;
    owl:onProperty ns2:hasValue ;
    owl:allValuesFrom [
      a owl:Restriction ;
      owl:onProperty ns2:hasUnit ;
      owl:allValuesFrom ns2:FontSizeUnit
    ]
  ] ;
  ns2:commonlyHasUnit ns2:metre, ns2:attometre, ns2:centimetre, ns2:decametre, ns2:decimetre, ns2:exametre, ns2:femtometre, ns2:gigametre, ns2:hectometre, ns2:kilometre, ns2:megametre, ns2:micrometre, ns2:millimetre, ns2:nanometre, ns2:petametre, ns2:picometre, ns2:terametre, ns2:angstrom, ns2:chain, ns2:fathom-USSurvey, ns2:fermi, ns2:foot-International, ns2:foot-USSurvey, ns2:furlong-International, ns2:inch-International, ns2:micron, ns2:mil-Length, ns2:mile-Statute, ns2:mile-USSurvey, ns2:nauticalMile-International, ns2:rod-US, ns2:yard-International, ns2:cicero, ns2:pica-ATA, ns2:pica-Postscript, ns2:pica-TeX, ns2:point-ATA, ns2:point-Didot, ns2:point-Postscript, ns2:point-TeX .

ns2:FontSizeUnit
  a owl:Class ;
  rdfs:label "font size unit"@en ;
  rdfs:subClassOf ns2:LengthUnit ;
  owl:equivalentClass [
    a owl:Class ;
    owl:oneOf (
     ns2:cicero
     ns2:pica-ATA
     ns2:pica-Postscript
     ns2:pica-TeX
     ns2:point-ATA
     ns2:point-Didot
     ns2:point-Postscript
     ns2:point-TeX
   )
  ] .

ns2:shipping
  a ns2:ApplicationArea ;
  rdfs:label "shipping"@en, "shipping"@nl ;
  ns2:usesQuantity ns2:Length, ns2:Speed ;
  ns2:usesUnit ns2:nauticalMile-International, ns2:knot-International, ns2:nauticalMile-InternationalPerHour .

ns2:AceticAcidMassFraction
  a owl:Class ;
  rdfs:label "acetic acid mass fraction"@en ;
  rdfs:comment "The fraction of the mass of acetic acid in a phenomenon"@en ;
  rdfs:subClassOf ns2:MassFraction ;
  ns2:commonlyHasUnit ns2:one, ns2:percent, ns2:gramPerGram .

ns2:DisodiumEthyleneDiamineTetreAcetateMassFraction
  a owl:Class ;
  rdfs:label "disodium ethylene diamine tetra acetate mass fraction"@en ;
  ns2:alternativeLabel "NaEDTA mass fraction"@en ;
  rdfs:comment "The fraction of the mass of disodium ethylene diamine tetra acetate in a phenomenon"@en ;
  rdfs:subClassOf ns2:MassFraction ;
  ns2:commonlyHasUnit ns2:one, ns2:percent, ns2:gramPerGram .

ns2:DryMatterMassFraction
  a owl:Class ;
  rdfs:label "dry matter mass fraction"@en ;
  rdfs:comment "The fraction of the mass of dry matter in a phenomenon"@en ;
  rdfs:subClassOf ns2:MassFraction ;
  ns2:commonlyHasUnit ns2:one, ns2:percent, ns2:gramPerGram .

ns2:EggMassFraction
  a owl:Class ;
  rdfs:label "egg mass fraction"@en ;
  rdfs:comment "The fraction of the mass of egg in a phenomenon"@en ;
  rdfs:subClassOf ns2:MassFraction ;
  ns2:commonlyHasUnit ns2:one, ns2:percent, ns2:gramPerGram .

ns2:FatMassFraction
  a owl:Class ;
  rdfs:label "fat mass fraction"@en ;
  rdfs:comment "The fraction of the mass of fat in a phenomenon"@en ;
  rdfs:subClassOf ns2:MassFraction ;
  ns2:commonlyHasUnit ns2:one, ns2:percent, ns2:gramPerGram .

ns2:GelatinMassFraction
  a owl:Class ;
  rdfs:label "gelatin mass fraction"@en ;
  rdfs:comment "The fraction of the mass of gelatin in a phenomenon"@en ;
  rdfs:subClassOf ns2:MassFraction ;
  ns2:commonlyHasUnit ns2:one, ns2:percent, ns2:gramPerGram .

ns2:GuarGumMassFraction
  a owl:Class ;
  rdfs:label "guar gum mass fraction"@en ;
  rdfs:comment "The fraction of the mass of guar gum in a phenomenon"@en ;
  rdfs:subClassOf ns2:MassFraction ;
  ns2:commonlyHasUnit ns2:one, ns2:percent, ns2:gramPerGram .

ns2:LactoseMassFraction
  a owl:Class ;
  rdfs:label "lactose mass fraction"@en ;
  rdfs:comment "The fraction of the mass of lactose in a phenomenon"@en ;
  rdfs:subClassOf ns2:MassFraction ;
  ns2:commonlyHasUnit ns2:one, ns2:percent, ns2:gramPerGram .

ns2:LocustBeanGumMassFraction
  a owl:Class ;
  rdfs:label "locust bean gum mass fraction"@en ;
  rdfs:comment "The fraction of the mass of locust bean gum in a phenomenon"@en ;
  rdfs:subClassOf ns2:MassFraction ;
  ns2:commonlyHasUnit ns2:one, ns2:percent, ns2:gramPerGram .

ns2:ModeratedStarchMassFraction
  a owl:Class ;
  rdfs:label "moderated starch mass fraction"@en ;
  rdfs:comment "The fraction of the mass of moderated starch in a phenomenon"@en ;
  rdfs:subClassOf ns2:MassFraction ;
  ns2:commonlyHasUnit ns2:one, ns2:percent, ns2:gramPerGram .

ns2:MustardPowderMassFraction
  a owl:Class ;
  rdfs:label "mustard powder mass fraction"@en ;
  rdfs:comment "The fraction of the mass of mustard powder in a phenomenon"@en ;
  rdfs:subClassOf ns2:MassFraction ;
  ns2:commonlyHasUnit ns2:one, ns2:percent, ns2:gramPerGram .

ns2:PotassiumSorbateMassFraction
  a owl:Class ;
  rdfs:label "potassium sorbate mass fraction"@en ;
  rdfs:comment "The fraction of the mass of potassium sorbate in a phenomenon"@en ;
  rdfs:subClassOf ns2:MassFraction ;
  ns2:commonlyHasUnit ns2:one, ns2:percent, ns2:gramPerGram .

ns2:ProteinMassFraction
  a owl:Class ;
  rdfs:label "protein mass fraction"@en ;
  rdfs:comment "The fraction of the mass of protein in a phenomenon"@en ;
  rdfs:subClassOf ns2:MassFraction ;
  ns2:commonlyHasUnit ns2:one, ns2:percent, ns2:gramPerGram .

ns2:SaltMassFraction
  a owl:Class ;
  rdfs:label "salt mass fraction"@en ;
  rdfs:comment "The fraction of the mass of salt in a phenomenon"@en ;
  rdfs:subClassOf ns2:MassFraction ;
  ns2:commonlyHasUnit ns2:one, ns2:percent, ns2:gramPerGram .

ns2:SoyBeanMassFraction
  a owl:Class ;
  rdfs:label "soy bean mass fraction"@en ;
  rdfs:comment "The fraction of the mass of soy bean oil in a phenomenon"@en ;
  rdfs:subClassOf ns2:MassFraction ;
  ns2:commonlyHasUnit ns2:one, ns2:percent, ns2:gramPerGram .

ns2:StarchMassFraction
  a owl:Class ;
  rdfs:label "starch mass fraction"@en ;
  rdfs:comment "The fraction of the mass of starch in a phenomenon"@en ;
  rdfs:subClassOf ns2:MassFraction ;
  ns2:commonlyHasUnit ns2:one, ns2:percent, ns2:gramPerGram .

ns2:StarchVA40MassFraction
  a owl:Class ;
  rdfs:label "starch VA40 mass fraction"@en ;
  rdfs:comment "The fraction of the mass of starch VA40 in a phenomenon"@en ;
  rdfs:subClassOf ns2:MassFraction ;
  ns2:commonlyHasUnit ns2:one, ns2:percent, ns2:gramPerGram .

ns2:StarchVA85MassFraction
  a owl:Class ;
  rdfs:label "starch VA85 mass fraction"@en ;
  rdfs:comment "The fraction of the mass of starch VA85 in a phenomenon"@en ;
  rdfs:subClassOf ns2:MassFraction ;
  ns2:commonlyHasUnit ns2:one, ns2:percent, ns2:gramPerGram .

ns2:SugarMassFraction
  a owl:Class ;
  rdfs:label "sugar mass fraction"@en ;
  rdfs:comment "The fraction of the mass of sugar in a phenomenon"@en ;
  rdfs:subClassOf ns2:MassFraction ;
  ns2:commonlyHasUnit ns2:one, ns2:percent, ns2:gramPerGram .

ns2:TweenMassFraction
  a owl:Class ;
  rdfs:label "tween mass fraction"@en ;
  rdfs:comment "The fraction of the mass of tween in a phenomenon"@en ;
  rdfs:subClassOf ns2:MassFraction ;
  ns2:commonlyHasUnit ns2:one, ns2:percent, ns2:gramPerGram .

ns2:WaterMassFraction
  a owl:Class ;
  rdfs:label "water mass fraction"@en ;
  rdfs:comment "The fraction of the mass of water in a phenomenon"@en ;
  rdfs:subClassOf ns2:MassFraction ;
  ns2:commonlyHasUnit ns2:one, ns2:percent, ns2:gramPerGram .

ns2:WheyProteinMassFraction
  a owl:Class ;
  rdfs:label "whey protein mass fraction"@en ;
  rdfs:comment "The fraction of the mass of whey protein in a phenomenon"@en ;
  rdfs:subClassOf ns2:MassFraction ;
  ns2:commonlyHasUnit ns2:one, ns2:percent, ns2:gramPerGram .

ns2:WheyProteinAggregateMassFraction
  a owl:Class ;
  rdfs:label "whey protein aggregate mass fraction"@en ;
  rdfs:comment "The fraction of the mass of whey protein aggregate in a phenomenon"@en ;
  rdfs:subClassOf ns2:MassFraction ;
  ns2:commonlyHasUnit ns2:one, ns2:percent, ns2:gramPerGram .

ns2:WheyProteinBeadsMassFraction
  a owl:Class ;
  rdfs:label "whey protein beads mass fraction"@en ;
  rdfs:comment "The fraction of the mass of whey protein beads in a phenomenon"@en ;
  rdfs:subClassOf ns2:MassFraction ;
  ns2:commonlyHasUnit ns2:one, ns2:percent, ns2:gramPerGram .

ns2:XanthanMassFraction
  a owl:Class ;
  rdfs:label "xanthan mass fraction"@en ;
  rdfs:comment "The fraction of the mass of xanthan in a phenomenon"@en ;
  rdfs:subClassOf ns2:MassFraction ;
  ns2:commonlyHasUnit ns2:one, ns2:percent, ns2:gramPerGram .

ns2:VaseLife
  a owl:Class ;
  rdfs:label "vase life"@en, "vaasleven"@nl ;
  rdfs:comment "Aantal dagen op de vaas tot onvoldoende."@nl ;
  rdfs:subClassOf ns2:Time ;
  ns2:commonlyHasUnit ns2:day .

ns2:NumberBudStadium
  a owl:Class ;
  rdfs:label "number bud stadium"@en, "aantal knopstadium"@nl ;
  rdfs:subClassOf ns2:Number ;
  ns2:commonlyHasUnit ns2:one .

ns2:NumberBudStadium1
  a owl:Class ;
  rdfs:label "number bud stadium 1"@en, "aantal knopstadium 1"@nl ;
  ns2:alternativeLabel "s1"@en ;
  rdfs:comment "Roos aantal in knopstadium 1: spitse knop."@nl ;
  rdfs:subClassOf ns2:NumberBudStadium ;
  ns2:commonlyHasUnit ns2:one .

ns2:NumberBudStadium2
  a owl:Class ;
  rdfs:label "number bud stadium 2"@en, "aantal knopstadium 2"@nl ;
  ns2:alternativeLabel "s2"@en ;
  rdfs:comment "Roos aantal in knopstadium 2: spitse knop."@nl ;
  rdfs:subClassOf ns2:NumberBudStadium ;
  ns2:commonlyHasUnit ns2:one .

ns2:NumberBudStadium3
  a owl:Class ;
  rdfs:label "number bud stadium 3"@en, "aantal knopstadium 3"@nl ;
  ns2:alternativeLabel "s3"@en ;
  rdfs:comment "Roos aantal in knopstadium 3: spitse knop."@nl ;
  rdfs:subClassOf ns2:NumberBudStadium ;
  ns2:commonlyHasUnit ns2:one .

ns2:NumberBudStadium4
  a owl:Class ;
  rdfs:label "number bud stadium 4"@en, "aantal knopstadium 4"@nl ;
  ns2:alternativeLabel "s4"@en ;
  rdfs:comment "Roos aantal in knopstadium 4: spitse knop."@nl ;
  rdfs:subClassOf ns2:NumberBudStadium ;
  ns2:commonlyHasUnit ns2:one .

ns2:NumberBudStadium5
  a owl:Class ;
  rdfs:label "number bud stadium 5"@en, "aantal knopstadium 5"@nl ;
  ns2:alternativeLabel "s5"@en ;
  rdfs:comment "Roos aantal in knopstadium 5: spitse knop."@nl ;
  rdfs:subClassOf ns2:NumberBudStadium ;
  ns2:commonlyHasUnit ns2:one .

ns2:BudStadium
  a owl:Class ;
  rdfs:label "bud stadium"@en, "knopstadium"@nl ;
  rdfs:subClassOf ns2:Quantity ;
  ns2:commonlyHasUnit ns2:_1-5 .

ns2:BudStadiumDay0
  a owl:Class ;
  rdfs:label "bud stadium day 0"@en, "knopstadium dag 0"@nl ;
  ns2:alternativeLabel "sday0"@en ;
  rdfs:comment "Knopstadium vaasdag 0 (start vaasleven) (code)."@nl ;
  rdfs:subClassOf ns2:BudStadium ;
  ns2:commonlyHasUnit ns2:_1-5 .

ns2:BudStadiumDay4
  a owl:Class ;
  rdfs:label "bud stadium day 4"@en, "knopstadium dag 4"@nl ;
  ns2:alternativeLabel "sday4"@en ;
  rdfs:comment "Knopstadium vaasdag 4 (code)."@nl ;
  rdfs:subClassOf ns2:BudStadium ;
  ns2:commonlyHasUnit ns2:_1-5 .

ns2:BudStadiumDay7
  a owl:Class ;
  rdfs:label "bud stadium day 7"@en, "knopstadium dag 7"@nl ;
  ns2:alternativeLabel "sday7"@en ;
  rdfs:comment "Knopstadium vaasdag 7 (code)."@nl ;
  rdfs:subClassOf ns2:BudStadium ;
  ns2:commonlyHasUnit ns2:_1-5 .

ns2:_1-5
  a ns2:Unit, ns2:SingularUnit ;
  rdfs:label "1-5"@en, "1-5"@nl ;
  ns2:hasDimension ns2:dimensionOne .

ns2:NumberBotrytis
  a owl:Class ;
  rdfs:label "number Botrytis"@en, "aantal Botrytis"@nl ;
  rdfs:subClassOf ns2:Number ;
  ns2:commonlyHasUnit ns2:one .

ns2:NumberBotrytis0
  a owl:Class ;
  rdfs:label "number Botrytis 0"@en, "aantal Botrytis 0"@nl ;
  ns2:alternativeLabel "b0"@en ;
  rdfs:comment "Aantal bloemen zonder Botrytis."@nl ;
  rdfs:subClassOf ns2:NumberBotrytis ;
  ns2:commonlyHasUnit ns2:one .

ns2:NumberBotrytis1
  a owl:Class ;
  rdfs:label "number Botrytis 1"@en, "aantal Botrytis 1"@nl ;
  ns2:alternativeLabel "b1"@en ;
  rdfs:comment "Aantal bloemen met Botrytis 1: enkele laesies: max 3 op één petaal of max 5 op meerdere plekken."@nl ;
  rdfs:subClassOf ns2:NumberBotrytis ;
  ns2:commonlyHasUnit ns2:one .

ns2:NumberBotrytis2
  a owl:Class ;
  rdfs:label "number Botrytis 2"@en, "aantal Botrytis 2"@nl ;
  ns2:alternativeLabel "b2"@en ;
  rdfs:comment "Aantal bloemen met Botrytis 2: grotere vlek(ken) op één petaal."@nl ;
  rdfs:subClassOf ns2:NumberBotrytis ;
  ns2:commonlyHasUnit ns2:one .

ns2:NumberBotrytis3
  a owl:Class ;
  rdfs:label "number Botrytis 3"@en, "aantal Botrytis 3"@nl ;
  ns2:alternativeLabel "b3"@en ;
  rdfs:comment "Aantal bloemen met Botrytis 3: één bruin petaal of vlekken op meer petalen."@nl ;
  rdfs:subClassOf ns2:NumberBotrytis ;
  ns2:commonlyHasUnit ns2:one .

ns2:NumberBotrytis4
  a owl:Class ;
  rdfs:label "number Botrytis 4"@en, "aantal Botrytis 4"@nl ;
  ns2:alternativeLabel "b4"@en ;
  rdfs:comment "Aantal bloemen met Botrytis 4: minimaal één bruin petaal en hart aangetast."@nl ;
  rdfs:subClassOf ns2:NumberBotrytis ;
  ns2:commonlyHasUnit ns2:one .

ns2:CauseEndOfVaseLifeBotrytis
  a owl:Class ;
  rdfs:label "cause end of vase life Botrytis"@en, "oorzaak einde vaasleven Botrytis"@nl ;
  ns2:alternativeLabel "bot"@en ;
  rdfs:comment "Oorzaak einde vaasleven Botrytis (b3 of b4) (1/0)."@nl ;
  rdfs:subClassOf ns2:Quantity ;
  ns2:commonlyHasUnit ns2:_1-0 .

ns2:_1-0
  a ns2:Unit, ns2:SingularUnit ;
  rdfs:label "1/0"@en, "1/0"@nl ;
  ns2:hasDimension ns2:dimensionOne .

ns2:NumberFlowers
  a owl:Class ;
  rdfs:label "number flowers"@en, "aantal bloemen"@nl ;
  rdfs:subClassOf ns2:Number ;
  ns2:commonlyHasUnit ns2:one .

ns2:TotalNumberFlowers
  a owl:Class ;
  rdfs:label "total number flowers"@en, "totaal aantal bloemen"@nl ;
  ns2:alternativeLabel "#flowers"@en ;
  rdfs:comment "Totaal aantal bloemen."@nl ;
  rdfs:subClassOf ns2:NumberFlowers ;
  ns2:commonlyHasUnit ns2:one .

ns2:NumberBlue-DiscoloredFlowers
  a owl:Class ;
  rdfs:label "number blue-discolored flowers"@en, "aantal blauwverkleurde bloemen"@nl ;
  ns2:alternativeLabel "#blue flowers"@en ;
  rdfs:comment "Aantal blauwverkleurde bloemen."@nl ;
  rdfs:subClassOf ns2:NumberFlowers ;
  ns2:commonlyHasUnit ns2:one .

ns2:NumberAbscisedFlowers
  a owl:Class ;
  rdfs:label "number abscised flowers"@en, "aantal gevallen bloemen"@nl ;
  ns2:alternativeLabel "#abscised flowers"@en ;
  rdfs:comment "Aantal gevallen bloemen."@nl ;
  rdfs:subClassOf ns2:NumberFlowers ;
  ns2:commonlyHasUnit ns2:one .

ns2:NumberWiltedFlowers
  a owl:Class ;
  rdfs:label "number wilted flowers"@en, "aantal verwelkte bloemen"@nl ;
  ns2:alternativeLabel "#wilted flowers"@en ;
  rdfs:comment "Aantal verwelkte bloemen."@nl ;
  rdfs:subClassOf ns2:NumberFlowers ;
  ns2:commonlyHasUnit ns2:one .

ns2:NumberRottenFlowers
  a owl:Class ;
  rdfs:label "number rotten flowers"@en, "aantal rotte bloemen"@nl ;
  ns2:alternativeLabel "#rotten flowers"@en ;
  rdfs:comment "Aantal rotte bloemen."@nl ;
  rdfs:subClassOf ns2:NumberFlowers ;
  ns2:commonlyHasUnit ns2:one .

ns2:NumberDryFlowers
  a owl:Class ;
  rdfs:label "number dry flowers"@en, "aantal verdroogde bloemen"@nl ;
  ns2:alternativeLabel "#dry flowers"@en ;
  rdfs:comment "Aantal verdroogde bloemen."@nl ;
  rdfs:subClassOf ns2:NumberFlowers ;
  ns2:commonlyHasUnit ns2:one .

ns2:NumberMalformedFlowers
  a owl:Class ;
  rdfs:label "number malformed flowers"@en, "aantal misvormde bloemen"@nl ;
  ns2:alternativeLabel "#malformed flowers"@en ;
  rdfs:comment "Aantal misvormde bloemen."@nl ;
  rdfs:subClassOf ns2:NumberFlowers ;
  ns2:commonlyHasUnit ns2:one .

ns2:NumberNonturgidFlowers
  a owl:Class ;
  rdfs:label "number nonturgid flowers"@en, "aantal slappe bloemen"@nl ;
  ns2:alternativeLabel "#nonturgid flowers"@en ;
  rdfs:comment "Aantal slappe bloemen."@nl ;
  rdfs:subClassOf ns2:NumberFlowers ;
  ns2:commonlyHasUnit ns2:one .

ns2:CauseEndOfVaseLifeBlueFlowers
  a owl:Class ;
  rdfs:label "cause end of vase life blue flowers"@en, "oorzaak einde vaasleven blauwe bloemen"@nl ;
  ns2:alternativeLabel "blue flowers"@en ;
  rdfs:comment "Oorzaak einde vaasleven blauwe bloemen (1/0)."@nl ;
  rdfs:subClassOf ns2:Quantity ;
  ns2:commonlyHasUnit ns2:_1-0 .

ns2:CauseEndOfVaseLifeAbscisedFlowers
  a owl:Class ;
  rdfs:label "cause end of vase life abscised flowers"@en, "oorzaak einde vaasleven bloemval"@nl ;
  ns2:alternativeLabel "abscised flowers"@en ;
  rdfs:comment "Oorzaak einde vaasleven bloemval (1/0)."@nl ;
  rdfs:subClassOf ns2:Quantity ;
  ns2:commonlyHasUnit ns2:_1-0 .

ns2:CauseEndOfVaseLifeWiltedFlowers
  a owl:Class ;
  rdfs:label "cause end of vase life wilted flowers"@en, "oorzaak einde vaasleven bloemverwelking"@nl ;
  ns2:alternativeLabel "wilted flowers"@en ;
  rdfs:comment "Oorzaak einde vaasleven bloemverwelking (1/0)."@nl ;
  rdfs:subClassOf ns2:Quantity ;
  ns2:commonlyHasUnit ns2:_1-0 .

ns2:CauseEndOfVaseLifeRottenFlowers
  a owl:Class ;
  rdfs:label "cause end of vase life rotten flowers"@en, "oorzaak einde vaasleven bloemrot"@nl ;
  ns2:alternativeLabel "rotten flowers"@en ;
  rdfs:comment "Oorzaak einde vaasleven bloemrot (1/0)."@nl ;
  rdfs:subClassOf ns2:Quantity ;
  ns2:commonlyHasUnit ns2:_1-0 .

ns2:CauseEndOfVaseLifeDryFlowers
  a owl:Class ;
  rdfs:label "cause end of vase life dry flowers"@en, "oorzaak einde vaasleven bloemverdroging"@nl ;
  ns2:alternativeLabel "dry flowers"@en ;
  rdfs:comment "Oorzaak einde vaasleven bloemverdroging (1/0)."@nl ;
  rdfs:subClassOf ns2:Quantity ;
  ns2:commonlyHasUnit ns2:_1-0 .

ns2:CauseEndOfVaseLifeMalformedFlowers
  a owl:Class ;
  rdfs:label "cause end of vase life malformed flowers"@en, "oorzaak einde vaasleven misvormde bloemen"@nl ;
  ns2:alternativeLabel "malformed flowers"@en ;
  rdfs:comment "Oorzaak einde vaasleven misvormde bloemen (1/0)."@nl ;
  rdfs:subClassOf ns2:Quantity ;
  ns2:commonlyHasUnit ns2:_1-0 .

ns2:CauseEndOfVaseLifeNonturgidFlowers
  a owl:Class ;
  rdfs:label "cause end of vase life nonturgid flowers"@en, "oorzaak einde vaasleven slappe bloemen"@nl ;
  ns2:alternativeLabel "nonturgid flowers"@en ;
  rdfs:comment "Oorzaak einde vaasleven slappe bloemen (1/0)."@nl ;
  rdfs:subClassOf ns2:Quantity ;
  ns2:commonlyHasUnit ns2:_1-0 .

ns2:NumberLeaves
  a owl:Class ;
  rdfs:label "number leaves"@en, "aantal bladeren"@nl ;
  rdfs:subClassOf ns2:Number ;
  ns2:commonlyHasUnit ns2:one .

ns2:TotalNumberLeaves
  a owl:Class ;
  rdfs:label "total number leaves"@en, "totaal aantal bladeren"@nl ;
  ns2:alternativeLabel "#leaves"@en ;
  rdfs:comment "Totaal aantal bladeren."@nl ;
  rdfs:subClassOf ns2:NumberLeaves ;
  ns2:commonlyHasUnit ns2:one .

ns2:NumberDryLeaves
  a owl:Class ;
  rdfs:label "number dry leaves"@en, "aantal verdroogde bladeren"@nl ;
  ns2:alternativeLabel "#dry leaves"@en ;
  rdfs:comment "Aantal verdroogde bladeren."@nl ;
  rdfs:subClassOf ns2:NumberLeaves ;
  ns2:commonlyHasUnit ns2:one .

ns2:NumberYellowLeaves
  a owl:Class ;
  rdfs:label "number yellow leaves"@en, "aantal vergeelde bladeren"@nl ;
  ns2:alternativeLabel "#yellow leaves"@en ;
  rdfs:comment "Aantal yellow bladeren."@nl ;
  rdfs:subClassOf ns2:NumberLeaves ;
  ns2:commonlyHasUnit ns2:one .

ns2:NumberAbscisedLeaves
  a owl:Class ;
  rdfs:label "number abscised leaves"@en, "aantal gevallen bladeren"@nl ;
  ns2:alternativeLabel "#abscised leaves"@en ;
  rdfs:comment "Aantal gevallen bladeren."@nl ;
  rdfs:subClassOf ns2:NumberLeaves ;
  ns2:commonlyHasUnit ns2:one .

ns2:NumberWiltedLeaves
  a owl:Class ;
  rdfs:label "number wilted leaves"@en, "aantal verwelkte bladeren"@nl ;
  ns2:alternativeLabel "#wilted leaves"@en ;
  rdfs:comment "Aantal verwelkte bladeren."@nl ;
  rdfs:subClassOf ns2:NumberLeaves ;
  ns2:commonlyHasUnit ns2:one .

ns2:NumberRottenLeaves
  a owl:Class ;
  rdfs:label "number rotten leaves"@en, "aantal rotte bladeren"@nl ;
  ns2:alternativeLabel "#rotten leaves"@en ;
  rdfs:comment "Aantal rotte bladeren."@nl ;
  rdfs:subClassOf ns2:NumberLeaves ;
  ns2:commonlyHasUnit ns2:one .

ns2:NumberNonturgidLeaves
  a owl:Class ;
  rdfs:label "number nonturgid leaves"@en, "aantal slappe bladeren"@nl ;
  ns2:alternativeLabel "#nonturgid leaves"@en ;
  rdfs:comment "Aantal slappe bladeren."@nl ;
  rdfs:subClassOf ns2:NumberLeaves ;
  ns2:commonlyHasUnit ns2:one .

ns2:CauseEndOfVaseLifeDryLeaves
  a owl:Class ;
  rdfs:label "cause end of vase life dry leaves"@en, "oorzaak einde vaasleven bladverdroging"@nl ;
  ns2:alternativeLabel "dry leaves"@en ;
  rdfs:comment "Oorzaak einde vaasleven bladverdroging (1/0)."@nl ;
  rdfs:subClassOf ns2:Quantity ;
  ns2:commonlyHasUnit ns2:_1-0 .

ns2:CauseEndOfVaseLifeYellowLeaves
  a owl:Class ;
  rdfs:label "cause end of vase life yellow leaves"@en, "oorzaak einde vaasleven bladvergeling"@nl ;
  ns2:alternativeLabel "yellow leaves"@en ;
  rdfs:comment "Oorzaak einde vaasleven bladvergeling (1/0)."@nl ;
  rdfs:subClassOf ns2:Quantity ;
  ns2:commonlyHasUnit ns2:_1-0 .

ns2:CauseEndOfVaseLifeAbscisedLeaves
  a owl:Class ;
  rdfs:label "cause end of vase life abscised leaves"@en, "oorzaak einde vaasleven bladval"@nl ;
  ns2:alternativeLabel "abscised leaves"@en ;
  rdfs:comment "Oorzaak einde vaasleven bladval (1/0)."@nl ;
  rdfs:subClassOf ns2:Quantity ;
  ns2:commonlyHasUnit ns2:_1-0 .

ns2:CauseEndOfVaseLifeWiltedLeaves
  a owl:Class ;
  rdfs:label "cause end of vase life wilted leaves"@en, "oorzaak einde vaasleven bladverwelking"@nl ;
  ns2:alternativeLabel "wilted leaves"@en ;
  rdfs:comment "Oorzaak einde vaasleven bladverwelking (1/0)."@nl ;
  rdfs:subClassOf ns2:Quantity ;
  ns2:commonlyHasUnit ns2:_1-0 .

ns2:CauseEndOfVaseLifeRottenLeaves
  a owl:Class ;
  rdfs:label "cause end of vase life rotten leaves"@en, "oorzaak einde vaasleven rotte bladeren"@nl ;
  ns2:alternativeLabel "rotten leaves"@en ;
  rdfs:comment "Oorzaak einde vaasleven rotte bladeren (1/0)."@nl ;
  rdfs:subClassOf ns2:Quantity ;
  ns2:commonlyHasUnit ns2:_1-0 .

ns2:CauseEndOfVaseLifeNonturgidLeaves
  a owl:Class ;
  rdfs:label "cause end of vase life nonturgid leaves"@en, "oorzaak einde vaasleven slappe bladeren"@nl ;
  ns2:alternativeLabel "nonturgid leaves"@en ;
  rdfs:comment "Oorzaak einde vaasleven slappe bladeren (1/0)."@nl ;
  rdfs:subClassOf ns2:Quantity ;
  ns2:commonlyHasUnit ns2:_1-0 .

ns2:NumberBuds
  a owl:Class ;
  rdfs:label "number buds"@en, "aantal knoppen"@nl ;
  rdfs:subClassOf ns2:Number ;
  ns2:commonlyHasUnit ns2:one .

ns2:TotalNumberBuds
  a owl:Class ;
  rdfs:label "total number buds"@en, "totaal aantal knoppen"@nl ;
  ns2:alternativeLabel "#buds"@en ;
  rdfs:comment "Totaal aantal knoppen."@nl ;
  rdfs:subClassOf ns2:NumberBuds ;
  ns2:commonlyHasUnit ns2:one .

ns2:NumberDryBuds
  a owl:Class ;
  rdfs:label "number dry buds"@en, "aantal verdroogde knoppen"@nl ;
  ns2:alternativeLabel "#dry buds"@en ;
  rdfs:comment "Aantal verdroogde knoppen."@nl ;
  rdfs:subClassOf ns2:NumberBuds ;
  ns2:commonlyHasUnit ns2:one .

ns2:NumberMalformedBuds
  a owl:Class ;
  rdfs:label "number malformed buds"@en, "aantal misvormde knoppen"@nl ;
  ns2:alternativeLabel "#malformed buds"@en ;
  rdfs:comment "Aantal misvormde knoppen."@nl ;
  rdfs:subClassOf ns2:NumberBuds ;
  ns2:commonlyHasUnit ns2:one .

ns2:NumberAbscisedBuds
  a owl:Class ;
  rdfs:label "number abscised buds"@en, "aantal gevallen knoppen"@nl ;
  ns2:alternativeLabel "#abscised buds"@en ;
  rdfs:comment "Aantal gevallen knoppen."@nl ;
  rdfs:subClassOf ns2:NumberBuds ;
  ns2:commonlyHasUnit ns2:one .

ns2:CauseEndOfVaseLifeDryBuds
  a owl:Class ;
  rdfs:label "cause end of vase life dry buds"@en, "oorzaak einde vaasleven knopverdroging"@nl ;
  ns2:alternativeLabel "dry buds"@en ;
  rdfs:comment "Oorzaak einde vaasleven knopverdroging (1/0)."@nl ;
  rdfs:subClassOf ns2:Quantity ;
  ns2:commonlyHasUnit ns2:_1-0 .

ns2:CauseEndOfVaseLifeMalformedBuds
  a owl:Class ;
  rdfs:label "cause end of vase life malformed buds"@en, "oorzaak einde vaasleven misvormde knoppen"@nl ;
  ns2:alternativeLabel "malformed buds"@en ;
  rdfs:comment "Oorzaak einde vaasleven misvormde knoppen (1/0)."@nl ;
  rdfs:subClassOf ns2:Quantity ;
  ns2:commonlyHasUnit ns2:_1-0 .

ns2:CauseEndOfVaseLifeAbscisedBuds
  a owl:Class ;
  rdfs:label "cause end of vase life abscised buds"@en, "oorzaak einde vaasleven knopval"@nl ;
  ns2:alternativeLabel "abscised buds"@en ;
  rdfs:comment "Oorzaak einde vaasleven knopval (1/0)."@nl ;
  rdfs:subClassOf ns2:Quantity ;
  ns2:commonlyHasUnit ns2:_1-0 .

ns2:QualityMark
  a owl:Class ;
  rdfs:label "quality mark"@en, "kwaliteitscijfer"@nl ;
  ns2:alternativeLabel "Qcijfer"@nl ;
  rdfs:subClassOf ns2:Quantity ;
  ns2:commonlyHasUnit ns2:_1-10 .

ns2:QualityMarkFlower
  a owl:Class ;
  rdfs:label "quality mark flower(s)"@en, "kwaliteitscijfer bloem(en)"@nl ;
  ns2:alternativeLabel "Qcijfer flower"@nl ;
  rdfs:subClassOf ns2:QualityMark ;
  ns2:commonlyHasUnit ns2:_1-10 .

ns2:QualityMarkLeaf
  a owl:Class ;
  rdfs:label "quality mark leafs"@en, "kwaliteitscijfer bladeren"@nl ;
  ns2:alternativeLabel "Qcijfer leaf"@nl ;
  rdfs:subClassOf ns2:QualityMark ;
  ns2:commonlyHasUnit ns2:_1-10 .

ns2:QualityMarkTotal
  a owl:Class ;
  rdfs:label "quality mark total"@en, "kwaliteitscijfer total"@nl ;
  ns2:alternativeLabel "Qcijfer total"@nl ;
  rdfs:subClassOf ns2:QualityMark ;
  ns2:commonlyHasUnit ns2:_1-10 .

ns2:_1-10
  a ns2:Unit, ns2:SingularUnit ;
  rdfs:label "1-10"@en, "1-10"@nl ;
  ns2:hasDimension ns2:dimensionOne .

ns2:_0-100
  a ns2:Unit, ns2:SingularUnit ;
  rdfs:label "0-100"@en, "0-100"@nl ;
  ns2:hasDimension ns2:dimensionOne .

ns2:VasePlusWaterMass
  a owl:Class ;
  rdfs:label "vase plus water mass"@en, "vaas- plus watermassa"@nl ;
  ns2:alternativeLabel "vase plus water weight"@en, "weight vase"@en ;
  rdfs:comment "Gewicht vaas plus water."@nl ;
  rdfs:subClassOf ns2:Mass ;
  ns2:commonlyHasUnit ns2:gram .

ns2:VasePlusWaterPlusFlowerMass
  a owl:Class ;
  rdfs:label "vase plus water plus flower mass"@en, "vaas- plus water- plus bloemmassa"@nl ;
  ns2:alternativeLabel "vase plus water plus flower weight"@en, "weight flo and vase"@en ;
  rdfs:comment "Gewicht vaas plus water plus bloem (= steel plus blad plus bloem)."@nl ;
  rdfs:subClassOf ns2:Mass ;
  ns2:commonlyHasUnit ns2:gram .

ns2:NumberColor
  a owl:Class ;
  rdfs:label "number color"@en, "aantal kleur"@nl ;
  rdfs:subClassOf ns2:Number ;
  ns2:commonlyHasUnit ns2:one .

ns2:NumberColor1
  a owl:Class ;
  rdfs:label "number color 1"@en, "aantal kleur 1"@nl ;
  ns2:alternativeLabel "color_1"@en ;
  rdfs:comment "Voorbeeld avocado Hass: code 1 poster (vrijwel) geheel groen."@nl ;
  rdfs:subClassOf ns2:NumberColor ;
  ns2:commonlyHasUnit ns2:one .

ns2:NumberColor2
  a owl:Class ;
  rdfs:label "number color 2"@en, "aantal kleur 2"@nl ;
  ns2:alternativeLabel "color_2"@en ;
  rdfs:comment "Voorbeeld avocado Hass: code 2 poster meer groen dan donker."@nl ;
  rdfs:subClassOf ns2:NumberColor ;
  ns2:commonlyHasUnit ns2:one .

ns2:NumberColor3
  a owl:Class ;
  rdfs:label "number color 3"@en, "aantal kleur 3"@nl ;
  ns2:alternativeLabel "color_3"@en ;
  rdfs:comment "Voorbeeld avocado Hass: code 3 poster 50% groen."@nl ;
  rdfs:subClassOf ns2:NumberColor ;
  ns2:commonlyHasUnit ns2:one .

ns2:NumberColor4
  a owl:Class ;
  rdfs:label "number color 4"@en, "aantal kleur 4"@nl ;
  ns2:alternativeLabel "color_4"@en ;
  rdfs:comment "Voorbeeld avocado Hass: code 4 poster meer donker dan groen."@nl ;
  rdfs:subClassOf ns2:NumberColor ;
  ns2:commonlyHasUnit ns2:one .

ns2:NumberColor5
  a owl:Class ;
  rdfs:label "number color 5"@en, "aantal kleur 5"@nl ;
  ns2:alternativeLabel "color_5"@en ;
  rdfs:comment "Voorbeeld avocado Hass: code 5 poster (vrijwel) geheel donker."@nl ;
  rdfs:subClassOf ns2:NumberColor ;
  ns2:commonlyHasUnit ns2:one .

ns2:ColorAreaFraction
  a owl:Class ;
  rdfs:label "color area fraction"@en, "kleuroppervlaktefractie"@nl ;
  ns2:alternativeLabel "color%"@en ;
  rdfs:comment "Voorbeeld avocado Hass: percentage oppervlak donker."@nl ;
  rdfs:subClassOf ns2:AreaFraction ;
  ns2:commonlyHasUnit ns2:percent .

ns2:NumberExternalBrowning
  a owl:Class ;
  rdfs:label "number external browning"@en ;
  rdfs:subClassOf ns2:Number ;
  ns2:commonlyHasUnit ns2:one .

ns2:NumberExternalBrowning1
  a owl:Class ;
  rdfs:label "number external browning 1"@en ;
  ns2:alternativeLabel "ext_brown_1"@en ;
  rdfs:comment "Voorbeeld avocado Hass: code 1 poster."@nl ;
  rdfs:subClassOf ns2:NumberColor ;
  ns2:commonlyHasUnit ns2:one .

ns2:NumberExternalBrowning2
  a owl:Class ;
  rdfs:label "number external browning 2"@en ;
  ns2:alternativeLabel "ext_brown_2"@en ;
  rdfs:comment "Voorbeeld avocado Hass: code 2 poster."@nl ;
  rdfs:subClassOf ns2:NumberColor ;
  ns2:commonlyHasUnit ns2:one .

ns2:NumberExternalBrowning3
  a owl:Class ;
  rdfs:label "number external browning 3"@en ;
  ns2:alternativeLabel "ext_brown_3"@en ;
  rdfs:comment "Voorbeeld avocado Hass: code 3 poster."@nl ;
  rdfs:subClassOf ns2:NumberColor ;
  ns2:commonlyHasUnit ns2:one .

ns2:NumberExternalBrowning4
  a owl:Class ;
  rdfs:label "number external browning 4"@en ;
  ns2:alternativeLabel "ext_brown_4"@en ;
  rdfs:comment "Voorbeeld avocado Hass: code 4 poster."@nl ;
  rdfs:subClassOf ns2:NumberColor ;
  ns2:commonlyHasUnit ns2:one .

ns2:NumberExternalBrowning5
  a owl:Class ;
  rdfs:label "number external browning 5"@en ;
  ns2:alternativeLabel "ext_brown_5"@en ;
  rdfs:comment "Voorbeeld avocado Hass: code 5 poster."@nl ;
  rdfs:subClassOf ns2:NumberColor ;
  ns2:commonlyHasUnit ns2:one .

ns2:ExternalBrowning
  a owl:Class ;
  rdfs:label "external browning"@en ;
  ns2:alternativeLabel "ext_brown"@en ;
  rdfs:comment "Voorbeeld avocado Hass: poster (code)."@nl ;
  rdfs:subClassOf ns2:Quantity ;
  ns2:commonlyHasUnit ns2:_1-5 .

ns2:NumberVascularBrowning
  a owl:Class ;
  rdfs:label "number vascular browning"@en ;
  rdfs:subClassOf ns2:Number ;
  ns2:commonlyHasUnit ns2:one .

ns2:NumberVascularBrowning1
  a owl:Class ;
  rdfs:label "number vascular browning 1"@en ;
  ns2:alternativeLabel "vascular_1"@en ;
  rdfs:comment "Voorbeeld avocado Hass: code 1 poster vascular browning."@nl ;
  rdfs:subClassOf ns2:NumberColor ;
  ns2:commonlyHasUnit ns2:one .

ns2:NumberVascularBrowning2
  a owl:Class ;
  rdfs:label "number vascular browning 2"@en ;
  ns2:alternativeLabel "vascular_2"@en ;
  rdfs:comment "Voorbeeld avocado Hass: code 2 poster vascular browning."@nl ;
  rdfs:subClassOf ns2:NumberColor ;
  ns2:commonlyHasUnit ns2:one .

ns2:NumberVascularBrowning3
  a owl:Class ;
  rdfs:label "number vascular browning 3"@en ;
  ns2:alternativeLabel "vascular_3"@en ;
  rdfs:comment "Voorbeeld avocado Hass: code 3 poster vascular browning."@nl ;
  rdfs:subClassOf ns2:NumberColor ;
  ns2:commonlyHasUnit ns2:one .

ns2:NumberVascularBrowning4
  a owl:Class ;
  rdfs:label "number vascular browning 4"@en ;
  ns2:alternativeLabel "vascular_4"@en ;
  rdfs:comment "Voorbeeld avocado Hass: code 4 poster vascular browning."@nl ;
  rdfs:subClassOf ns2:NumberColor ;
  ns2:commonlyHasUnit ns2:one .

ns2:NumberVascularBrowning5
  a owl:Class ;
  rdfs:label "number vascular browning 5"@en ;
  ns2:alternativeLabel "vascular_5"@en ;
  rdfs:comment "Voorbeeld avocado Hass: code 5 poster vascular browning."@nl ;
  rdfs:subClassOf ns2:NumberColor ;
  ns2:commonlyHasUnit ns2:one .

ns2:VascularBrowning
  a owl:Class ;
  rdfs:label "vascular browning"@en ;
  ns2:alternativeLabel "vascular"@en ;
  rdfs:comment "Voorbeeld avocado Hass: poster (code)."@nl ;
  rdfs:subClassOf ns2:Quantity ;
  ns2:commonlyHasUnit ns2:_1-5 .

ns2:NumberPulpBrowning
  a owl:Class ;
  rdfs:label "number pulp browning"@en ;
  rdfs:subClassOf ns2:Number ;
  ns2:commonlyHasUnit ns2:one .

ns2:NumberPulpBrowning1
  a owl:Class ;
  rdfs:label "number pulp browning 1"@en ;
  ns2:alternativeLabel "pulp_1"@en ;
  rdfs:comment "Voorbeeld avocado Hass: code 1 poster pulp browning."@nl ;
  rdfs:subClassOf ns2:NumberColor ;
  ns2:commonlyHasUnit ns2:one .

ns2:NumberPulpBrowning2
  a owl:Class ;
  rdfs:label "number pulp browning 2"@en ;
  ns2:alternativeLabel "pulp_2"@en ;
  rdfs:comment "Voorbeeld avocado Hass: code 2 poster pulp browning."@nl ;
  rdfs:subClassOf ns2:NumberColor ;
  ns2:commonlyHasUnit ns2:one .

ns2:NumberPulpBrowning3
  a owl:Class ;
  rdfs:label "number pulp browning 3"@en ;
  ns2:alternativeLabel "pulp_3"@en ;
  rdfs:comment "Voorbeeld avocado Hass: code 3 poster pulp browning."@nl ;
  rdfs:subClassOf ns2:NumberColor ;
  ns2:commonlyHasUnit ns2:one .

ns2:NumberPulpBrowning4
  a owl:Class ;
  rdfs:label "number pulp browning 4"@en ;
  ns2:alternativeLabel "pulp_4"@en ;
  rdfs:comment "Voorbeeld avocado Hass: code 4 poster pulp browning."@nl ;
  rdfs:subClassOf ns2:NumberColor ;
  ns2:commonlyHasUnit ns2:one .

ns2:NumberPulpBrowning5
  a owl:Class ;
  rdfs:label "number pulp browning 5"@en ;
  ns2:alternativeLabel "pulp_5"@en ;
  rdfs:comment "Voorbeeld avocado Hass: code 5 poster pulp browning."@nl ;
  rdfs:subClassOf ns2:NumberColor ;
  ns2:commonlyHasUnit ns2:one .

ns2:PulpBrowning
  a owl:Class ;
  rdfs:label "pulp browning"@en ;
  ns2:alternativeLabel "pulp"@en ;
  rdfs:comment "Voorbeeld avocado Hass: poster (code)."@nl ;
  rdfs:subClassOf ns2:Quantity ;
  ns2:commonlyHasUnit ns2:_1-5 .

ns2:StemEndRot
  a owl:Class ;
  rdfs:label "stem end rot"@en ;
  ns2:alternativeLabel "stemendrot"@en ;
  rdfs:comment "Aanwezigheid stem end rot (1/0)."@nl ;
  rdfs:subClassOf ns2:Quantity ;
  ns2:commonlyHasUnit ns2:_1-0 .

ns2:StemEndRotAreaFraction
  a owl:Class ;
  rdfs:label "stem end rot area fraction"@en, "stem-end-rot-oppervlaktefractie"@nl ;
  ns2:alternativeLabel "stemendrot%"@en ;
  rdfs:comment "Percentage van het oppervlak stem end rot."@nl ;
  rdfs:subClassOf ns2:AreaFraction ;
  ns2:commonlyHasUnit ns2:percent .

ns2:StickStone
  a owl:Class ;
  rdfs:label "stick stone"@en ;
  ns2:alternativeLabel "stickstone"@en ;
  rdfs:comment "Kleefpit of niet (1/0)."@nl ;
  rdfs:subClassOf ns2:Quantity ;
  ns2:commonlyHasUnit ns2:_1-0 .

ns2:AcousticFirmness
  a owl:Class ;
  rdfs:label "acoustic firmness"@en, "akoestische stevigheid"@nl ;
  ns2:alternativeLabel "firmness_ac"@en ;
  rdfs:comment "Stevigheid gemeten met AWETA (acoustic firmness value). AFS value."@nl ;
  rdfs:subClassOf ns2:Quantity ;
  ns2:commonlyHasUnit ns2:AFS .

ns2:AFS
  a ns2:Unit, ns2:SingularUnit ;
  rdfs:label "AFS"@en ;
  ns2:hasDimension ns2:dimensionOne .

ns2:Firmness-Penetrometer-Method1
  a owl:Class ;
  rdfs:label "firmness (penetrometer) (method 1)"@en, "stevigheid (penetrometer) (methode 1)"@nl ;
  ns2:alternativeLabel "firmness_pen_1"@en ;
  rdfs:comment "Stevigheid gemeten met penetrometer methode 1."@nl ;
  rdfs:subClassOf ns2:Quantity ;
  ns2:commonlyHasUnit ns2:kilogramPerSquareMetre .

ns2:Firmness-Penetrometer-Method2
  a owl:Class ;
  rdfs:label "firmness (penetrometer) (method 2)"@en, "stevigheid (penetrometer) (methode 2)"@nl ;
  ns2:alternativeLabel "firmness_pen_2"@en ;
  rdfs:comment "Stevigheid gemeten met penetrometer methode 2."@nl ;
  rdfs:subClassOf ns2:Quantity ;
  ns2:commonlyHasUnit ns2:kilogramPerSquareMetre .

ns2:NumberManualFirmness
  a owl:Class ;
  rdfs:label "number manual firmness"@en, "aantal manuele stevigheid"@nl ;
  rdfs:subClassOf ns2:Number ;
  ns2:commonlyHasUnit ns2:one .

ns2:NumberManualFirmness0
  a owl:Class ;
  rdfs:label "number manual firmness 0"@en, "aantal manuele stevigheid 0"@nl ;
  ns2:alternativeLabel "firmness_m_0"@en ;
  rdfs:comment "Firmness manueel: 0 = steenhard."@nl ;
  rdfs:subClassOf ns2:NumberManualFirmness ;
  ns2:commonlyHasUnit ns2:one .

ns2:NumberManualFirmness0.5
  a owl:Class ;
  rdfs:label "number manual firmness 0.5"@en, "aantal manuele stevigheid 0.5"@nl ;
  ns2:alternativeLabel "firmness_m_0.5"@en ;
  rdfs:comment "Firmness manueel: 0.5 = hard."@nl ;
  rdfs:subClassOf ns2:NumberManualFirmness ;
  ns2:commonlyHasUnit ns2:one .

ns2:NumberManualFirmness1
  a owl:Class ;
  rdfs:label "number manual firmness 1"@en, "aantal manuele stevigheid 1"@nl ;
  ns2:alternativeLabel "firmness_m_1"@en ;
  rdfs:comment "Firmness manueel: 1 = zeer stevig."@nl ;
  rdfs:subClassOf ns2:NumberManualFirmness ;
  ns2:commonlyHasUnit ns2:one .

ns2:NumberManualFirmness1.5
  a owl:Class ;
  rdfs:label "number manual firmness 1.5"@en, "aantal manuele stevigheid 1.5"@nl ;
  ns2:alternativeLabel "firmness_m_1.5"@en ;
  rdfs:comment "Firmness manueel: 1.5 = stevig."@nl ;
  rdfs:subClassOf ns2:NumberManualFirmness ;
  ns2:commonlyHasUnit ns2:one .

ns2:NumberManualFirmness2
  a owl:Class ;
  rdfs:label "number manual firmness 2"@en, "aantal manuele stevigheid 2"@nl ;
  ns2:alternativeLabel "firmness_m_2"@en ;
  rdfs:comment "Firmness manueel: 2 = halfzacht."@nl ;
  rdfs:subClassOf ns2:NumberManualFirmness ;
  ns2:commonlyHasUnit ns2:one .

ns2:NumberManualFirmness2.5
  a owl:Class ;
  rdfs:label "number manual firmness 2.5"@en, "aantal manuele stevigheid 2.5"@nl ;
  ns2:alternativeLabel "firmness_m_2.5"@en ;
  rdfs:comment "Firmness manueel: 2.5 = eetrijp."@nl ;
  rdfs:subClassOf ns2:NumberManualFirmness ;
  ns2:commonlyHasUnit ns2:one .

ns2:NumberManualFirmness3
  a owl:Class ;
  rdfs:label "number manual firmness 3"@en, "aantal manuele stevigheid 3"@nl ;
  ns2:alternativeLabel "firmness_m_3"@en ;
  rdfs:comment "Firmness manueel: 3 = zacht."@nl ;
  rdfs:subClassOf ns2:NumberManualFirmness ;
  ns2:commonlyHasUnit ns2:one .

ns2:NumberManualFirmness3.5
  a owl:Class ;
  rdfs:label "number manual firmness 3.5"@en, "aantal manuele stevigheid 3.5"@nl ;
  ns2:alternativeLabel "firmness_m_3.5"@en ;
  rdfs:comment "Firmness manueel: 3.5 = te zacht."@nl ;
  rdfs:subClassOf ns2:NumberManualFirmness ;
  ns2:commonlyHasUnit ns2:one .

ns2:NumberManualFirmness4
  a owl:Class ;
  rdfs:label "number manual firmness 4"@en, "aantal manuele stevigheid 4"@nl ;
  ns2:alternativeLabel "firmness_m_4"@en ;
  rdfs:comment "Firmness manueel: 4 = week."@nl ;
  rdfs:subClassOf ns2:NumberManualFirmness ;
  ns2:commonlyHasUnit ns2:one .

ns2:NumberManualFirmness4.5
  a owl:Class ;
  rdfs:label "number manual firmness 4.5"@en, "aantal manuele stevigheid 4.5"@nl ;
  ns2:alternativeLabel "firmness_m_4.5"@en ;
  rdfs:comment "Firmness manueel: 4.5 = vies."@nl ;
  rdfs:subClassOf ns2:NumberManualFirmness ;
  ns2:commonlyHasUnit ns2:one .

ns2:NumberManualFirmness5
  a owl:Class ;
  rdfs:label "number manual firmness 5"@en, "aantal manuele stevigheid 5"@nl ;
  ns2:alternativeLabel "firmness_m_5"@en ;
  rdfs:comment "Firmness manueel: 5 = zeer vies."@nl ;
  rdfs:subClassOf ns2:NumberManualFirmness ;
  ns2:commonlyHasUnit ns2:one .

ns2:ManualFirmness
  a owl:Class ;
  rdfs:label "manual firmness"@en, "manuele stevigheid"@nl ;
  ns2:alternativeLabel "firmness_m"@en ;
  rdfs:comment "Firmness manueel: code 0 - 5."@nl ;
  rdfs:subClassOf ns2:Quantity ;
  ns2:commonlyHasUnit ns2:_0-5 .

ns2:_0-5
  a ns2:Unit, ns2:SingularUnit ;
  rdfs:label "0-5"@en, "0-5"@nl ;
  ns2:hasDimension ns2:dimensionOne .

ns2:xRange
  a owl:Class ;
  rdfs:label "x range"@en ;
  rdfs:subClassOf ns2:Length ;
  ns2:commonlyHasUnit ns2:metre, ns2:attometre, ns2:centimetre, ns2:decametre, ns2:decimetre, ns2:exametre, ns2:femtometre, ns2:gigametre, ns2:hectometre, ns2:kilometre, ns2:megametre, ns2:micrometre, ns2:millimetre, ns2:nanometre, ns2:petametre, ns2:picometre, ns2:terametre, ns2:angstrom, ns2:astronomicalUnit, ns2:chain, ns2:cicero, ns2:fathom-USSurvey, ns2:fermi, ns2:foot-International, ns2:foot-USSurvey, ns2:furlong-International, ns2:inch-International, ns2:lightYear, ns2:micron, ns2:mil-Length, ns2:mile-USSurvey, ns2:nauticalMile-International, ns2:parsec, ns2:pica-ATA, ns2:pica-Postscript, ns2:pica-TeX, ns2:point-ATA, ns2:point-Didot, ns2:point-Postscript, ns2:point-TeX, ns2:rod-US, ns2:mile-Statute, ns2:yard-International, ns2:megaparsec .

ns2:yRange
  a owl:Class ;
  rdfs:label "y range"@en ;
  rdfs:subClassOf ns2:Length ;
  ns2:commonlyHasUnit ns2:metre, ns2:attometre, ns2:centimetre, ns2:decametre, ns2:decimetre, ns2:exametre, ns2:femtometre, ns2:gigametre, ns2:hectometre, ns2:kilometre, ns2:megametre, ns2:micrometre, ns2:millimetre, ns2:nanometre, ns2:petametre, ns2:picometre, ns2:terametre, ns2:angstrom, ns2:astronomicalUnit, ns2:chain, ns2:cicero, ns2:fathom-USSurvey, ns2:fermi, ns2:foot-International, ns2:foot-USSurvey, ns2:furlong-International, ns2:inch-International, ns2:lightYear, ns2:micron, ns2:mil-Length, ns2:mile-USSurvey, ns2:nauticalMile-International, ns2:parsec, ns2:pica-ATA, ns2:pica-Postscript, ns2:pica-TeX, ns2:point-ATA, ns2:point-Didot, ns2:point-Postscript, ns2:point-TeX, ns2:rod-US, ns2:mile-Statute, ns2:yard-International, ns2:megaparsec .

ns2:zRange
  a owl:Class ;
  rdfs:label "z range"@en ;
  rdfs:subClassOf ns2:Length ;
  ns2:commonlyHasUnit ns2:metre, ns2:attometre, ns2:centimetre, ns2:decametre, ns2:decimetre, ns2:exametre, ns2:femtometre, ns2:gigametre, ns2:hectometre, ns2:kilometre, ns2:megametre, ns2:micrometre, ns2:millimetre, ns2:nanometre, ns2:petametre, ns2:picometre, ns2:terametre, ns2:angstrom, ns2:astronomicalUnit, ns2:chain, ns2:cicero, ns2:fathom-USSurvey, ns2:fermi, ns2:foot-International, ns2:foot-USSurvey, ns2:furlong-International, ns2:inch-International, ns2:lightYear, ns2:micron, ns2:mil-Length, ns2:mile-USSurvey, ns2:nauticalMile-International, ns2:parsec, ns2:pica-ATA, ns2:pica-Postscript, ns2:pica-TeX, ns2:point-ATA, ns2:point-Didot, ns2:point-Postscript, ns2:point-TeX, ns2:rod-US, ns2:mile-Statute, ns2:yard-International, ns2:megaparsec .

ns2:Total3DStartEndDistance
  a owl:Class ;
  rdfs:label "total 3D start-end distance"@en ;
  rdfs:subClassOf ns2:Distance ;
  ns2:commonlyHasUnit ns2:metre, ns2:attometre, ns2:centimetre, ns2:decametre, ns2:decimetre, ns2:exametre, ns2:femtometre, ns2:gigametre, ns2:hectometre, ns2:kilometre, ns2:megametre, ns2:micrometre, ns2:millimetre, ns2:nanometre, ns2:petametre, ns2:picometre, ns2:terametre, ns2:angstrom, ns2:astronomicalUnit, ns2:chain, ns2:cicero, ns2:fathom-USSurvey, ns2:fermi, ns2:foot-International, ns2:foot-USSurvey, ns2:furlong-International, ns2:inch-International, ns2:lightYear, ns2:micron, ns2:mil-Length, ns2:mile-USSurvey, ns2:nauticalMile-International, ns2:parsec, ns2:pica-ATA, ns2:pica-Postscript, ns2:pica-TeX, ns2:point-ATA, ns2:point-Didot, ns2:point-Postscript, ns2:point-TeX, ns2:rod-US, ns2:mile-Statute, ns2:yard-International, ns2:megaparsec .

ns2:xy2DStartEndDistance
  a owl:Class ;
  rdfs:label "xy 2D start-end distance"@en ;
  rdfs:subClassOf ns2:Distance ;
  ns2:commonlyHasUnit ns2:metre, ns2:attometre, ns2:centimetre, ns2:decametre, ns2:decimetre, ns2:exametre, ns2:femtometre, ns2:gigametre, ns2:hectometre, ns2:kilometre, ns2:megametre, ns2:micrometre, ns2:millimetre, ns2:nanometre, ns2:petametre, ns2:picometre, ns2:terametre, ns2:angstrom, ns2:astronomicalUnit, ns2:chain, ns2:cicero, ns2:fathom-USSurvey, ns2:fermi, ns2:foot-International, ns2:foot-USSurvey, ns2:furlong-International, ns2:inch-International, ns2:lightYear, ns2:micron, ns2:mil-Length, ns2:mile-USSurvey, ns2:nauticalMile-International, ns2:parsec, ns2:pica-ATA, ns2:pica-Postscript, ns2:pica-TeX, ns2:point-ATA, ns2:point-Didot, ns2:point-Postscript, ns2:point-TeX, ns2:rod-US, ns2:mile-Statute, ns2:yard-International, ns2:megaparsec .

ns2:TotalDistanceTravelled
  a owl:Class ;
  rdfs:label "total distance travelled"@en ;
  rdfs:subClassOf ns2:Distance ;
  ns2:commonlyHasUnit ns2:metre, ns2:attometre, ns2:centimetre, ns2:decametre, ns2:decimetre, ns2:exametre, ns2:femtometre, ns2:gigametre, ns2:hectometre, ns2:kilometre, ns2:megametre, ns2:micrometre, ns2:millimetre, ns2:nanometre, ns2:petametre, ns2:picometre, ns2:terametre, ns2:angstrom, ns2:astronomicalUnit, ns2:chain, ns2:cicero, ns2:fathom-USSurvey, ns2:fermi, ns2:foot-International, ns2:foot-USSurvey, ns2:furlong-International, ns2:inch-International, ns2:lightYear, ns2:micron, ns2:mil-Length, ns2:mile-USSurvey, ns2:nauticalMile-International, ns2:parsec, ns2:pica-ATA, ns2:pica-Postscript, ns2:pica-TeX, ns2:point-ATA, ns2:point-Didot, ns2:point-Postscript, ns2:point-TeX, ns2:rod-US, ns2:mile-Statute, ns2:yard-International, ns2:megaparsec .

ns2:xyDistanceTravelled
  a owl:Class ;
  rdfs:label "xy distance travelled"@en ;
  rdfs:subClassOf ns2:Distance ;
  ns2:commonlyHasUnit ns2:metre, ns2:attometre, ns2:centimetre, ns2:decametre, ns2:decimetre, ns2:exametre, ns2:femtometre, ns2:gigametre, ns2:hectometre, ns2:kilometre, ns2:megametre, ns2:micrometre, ns2:millimetre, ns2:nanometre, ns2:petametre, ns2:picometre, ns2:terametre, ns2:angstrom, ns2:astronomicalUnit, ns2:chain, ns2:cicero, ns2:fathom-USSurvey, ns2:fermi, ns2:foot-International, ns2:foot-USSurvey, ns2:furlong-International, ns2:inch-International, ns2:lightYear, ns2:micron, ns2:mil-Length, ns2:mile-USSurvey, ns2:nauticalMile-International, ns2:parsec, ns2:pica-ATA, ns2:pica-Postscript, ns2:pica-TeX, ns2:point-ATA, ns2:point-Didot, ns2:point-Postscript, ns2:point-TeX, ns2:rod-US, ns2:mile-Statute, ns2:yard-International, ns2:megaparsec .

ns2:BodyMass
  a owl:Class ;
  rdfs:label "body mass"@en ;
  ns2:unofficialLabel "body weight" ;
  rdfs:subClassOf ns2:Mass ;
  ns2:commonlyHasUnit ns2:gram, ns2:kilogram, ns2:tonne .

ns2:CapMass
  a owl:Class ;
  rdfs:label "cap mass"@en ;
  ns2:unofficialLabel "cap weight" ;
  rdfs:subClassOf ns2:Mass ;
  ns2:commonlyHasUnit ns2:gram, ns2:kilogram, ns2:tonne .

ns2:CartonMass
  a owl:Class ;
  rdfs:label "carton mass"@en ;
  ns2:unofficialLabel "carton weight" ;
  rdfs:subClassOf ns2:Mass ;
  ns2:commonlyHasUnit ns2:gram, ns2:kilogram, ns2:tonne .

ns2:DryMass
  a owl:Class ;
  rdfs:label "dry mass"@en ;
  ns2:unofficialLabel "dry weight" ;
  rdfs:subClassOf ns2:Mass ;
  ns2:commonlyHasUnit ns2:gram, ns2:kilogram, ns2:tonne .

ns2:DryBodyMass
  a owl:Class ;
  rdfs:label "dry body mass"@en ;
  ns2:unofficialLabel "dry body weight" ;
  rdfs:subClassOf ns2:DryMass ;
  ns2:commonlyHasUnit ns2:gram, ns2:kilogram, ns2:tonne .

ns2:FlowpackMass
  a owl:Class ;
  rdfs:label "flowpack mass"@en ;
  ns2:unofficialLabel "flowpack weight" ;
  rdfs:subClassOf ns2:Mass ;
  ns2:commonlyHasUnit ns2:gram, ns2:kilogram, ns2:tonne .

ns2:LabelMass
  a owl:Class ;
  rdfs:label "label mass"@en ;
  ns2:unofficialLabel "label weight" ;
  rdfs:subClassOf ns2:Mass ;
  ns2:commonlyHasUnit ns2:gram, ns2:kilogram, ns2:tonne .

ns2:BodyLabelMass
  a owl:Class ;
  rdfs:label "body label mass"@en ;
  ns2:unofficialLabel "body label weight" ;
  rdfs:subClassOf ns2:LabelMass ;
  ns2:commonlyHasUnit ns2:gram, ns2:kilogram, ns2:tonne .

ns2:NeckRingMass
  a owl:Class ;
  rdfs:label "neck ring mass"@en ;
  ns2:unofficialLabel "neck ring weight" ;
  rdfs:subClassOf ns2:Mass ;
  ns2:commonlyHasUnit ns2:gram, ns2:kilogram, ns2:tonne .

ns2:StrawMass
  a owl:Class ;
  rdfs:label "straw mass"@en ;
  ns2:unofficialLabel "straw weight" ;
  rdfs:subClassOf ns2:Mass ;
  ns2:commonlyHasUnit ns2:gram, ns2:kilogram, ns2:tonne .

ns2:TopMass
  a owl:Class ;
  rdfs:label "top mass"@en ;
  ns2:unofficialLabel "top weight" ;
  rdfs:subClassOf ns2:Mass ;
  ns2:commonlyHasUnit ns2:gram, ns2:kilogram, ns2:tonne .

ns2:commonApplicationArea
  a ns2:ApplicationArea ;
  rdfs:label "common application area"@en, "algemeen toepassingsgebied"@nl ;
  ns2:usesQuantity ns2:Length, ns2:Mass, ns2:Time, ns2:Temperature, ns2:Area, ns2:Volume, ns2:Speed, ns2:Frequency, ns2:Energy, ns2:Power, ns2:Force, ns2:ElectricCurrent, ns2:ElectricPotential, ns2:MassFraction, ns2:Density ;
  ns2:usesUnit ns2:metre, ns2:kilometre, ns2:centimetre, ns2:millimetre, ns2:inch-International, ns2:foot-International, ns2:mile-Statute, ns2:yard-International, ns2:kilogram, ns2:gram, ns2:milligram, ns2:poundAvoirdupois, ns2:ounceAvoirdupois, ns2:second-Time, ns2:millisecond-Time, ns2:minute-Time, ns2:hour, ns2:day, ns2:week, ns2:month, ns2:year, ns2:kelvin, ns2:degreeCelsius, ns2:degreeFahrenheit, ns2:squareMetre, ns2:squareCentimetre, ns2:squareKilometre, ns2:are, ns2:hectare, ns2:acre-International, ns2:acre-USSurvey, ns2:cubicMetre, ns2:cubicCentimetre, ns2:litre, ns2:decilitre, ns2:centilitre, ns2:millilitre, ns2:pint-Imperial, ns2:liquidPint-US, ns2:gallon-Imperial, ns2:gallon-US, ns2:metrePerSecond-Time, ns2:kilometrePerHour, ns2:mile-StatutePerHour, ns2:hertz, ns2:kilohertz, ns2:megahertz, ns2:joule, ns2:kilojoule, ns2:kilocalorie-Mean, ns2:kilowattHour, ns2:watt, ns2:milliwatt, ns2:kilowatt, ns2:megawatt, ns2:newton, ns2:kilonewton, ns2:pound-Force, ns2:ampere, ns2:milliampere, ns2:volt, ns2:millivolt, ns2:gramPerKilogram, ns2:percent, ns2:gramPerLitre, ns2:milligramPerLitre .

ns1:reference
  a owl:ObjectProperty, owl:FunctionalProperty ;
  rdfs:label "reference"@en ;
  rdfs:domain bibo:Document .

ns1:Hajo_Rijgersberg
  a foaf:Person ;
  foaf:name "Hajo Rijgersberg" .

ns1:VU
  a foaf:Organization ;
  foaf:name "Vrije Universiteit" ;
  foaf:based_near "Amsterdam, The Netherlands" .

<http://www.openisbn.com/isbn/9789462280618/>
  a bibo:Thesis ;
  dc11:title "Semantic Support of Quantitative Research" ;
  dc11:date "2013" ;
  dc11:creator ns1:Hajo_Rijgersberg ;
  bibo:issuer ns1:VU ;
  bibo:degree <http://purl.org/bibo/degrees/phd> ;
  bibo:uri "http://www.openisbn.com/isbn/9789462280618/" ;
  bibo:isbn13 "978-94-6228-061-8" .

ns1:Jean_Meeus
  a foaf:Person ;
  foaf:name "Jean Meeus" .

ns1:Willmann_Bell
  a foaf:Organization ;
  foaf:name "Willmann-Bell Inc." .

<urn:isbn:0943396611>
  a bibo:Book ;
  dc11:title "Astronomical Algorithms" ;
  dc11:date "1998" ;
  dc11:creator ns1:Jean_Meeus ;
  dc11:publisher ns1:Willmann_Bell ;
  bibo:edition "2" ;
  dc11:subject "Astronomy - Data processing", "Astronomy - Problems, exercises", "Algorithms" ;
  bibo:isbn10 "0943396611" ;
  bibo:uri "http://www.willbell.com/math/mc1.htm" .

ns1:chapter13_Astronomical_Algorithms
  a bibo:Chapter ;
  dc11:title "Transformation of Coordinates" ;
  bibo:chapter "13" ;
  bibo:pageStart "92" ;
  bibo:pageEnd "96" ;
  bibo:reproducedIn <urn:isbn:0943396611> .

ns1:chapter23_Astronomical_Algorithms
  a bibo:Chapter ;
  dc11:title "Apparent place of a star" ;
  bibo:chapter "23" ;
  bibo:pageStart "149" ;
  bibo:pageEnd "158" ;
  bibo:reproducedIn <urn:isbn:0943396611> .

ns1:Kenneth_Siedelmann
  a foaf:Person ;
  foaf:name "Kenneth Siedelmann" .

ns1:University_Science_Books
  a foaf:Organization ;
  foaf:name "University Science Books" ;
  foaf:based_near "Sausalito, California" .

<http://www.openisbn.com/isbn/1891389459/>
  a bibo:Book ;
  dc11:title "Explanatory Supplement to the Astronomical Almanac" ;
  dc11:date "1992" ;
  dc11:creator ns1:Kenneth_Siedelmann ;
  dc11:publisher ns1:University_Science_Books ;
  bibo:uri "http://www.openisbn.com/isbn/1891389459/" ;
  bibo:isbn10 "1891389459" .

ns1:Glossary_Astronomical_Almanac
  a bibo:BookSection ;
  dc11:title "Glossary" ;
  bibo:pageStart "721" ;
  bibo:pageEnd "739" ;
  bibo:reproducedIn <http://www.openisbn.com/isbn/1891389459/> .

ns1:CR_Kitchin
  a foaf:Person ;
  foaf:name "C.R. Kitchin" .

ns1:Institute_of_Physics_Publishing
  a foaf:Organization ;
  foaf:name "Institute of Physics Publishing" ;
  foaf:based_near "Bristol, UK" .

ns1:Astrophysical_Techniques
  a bibo:Book ;
  dc11:title "Astrophysical Techniques" ;
  dc11:date "2003" ;
  bibo:edition "5" ;
  dc11:creator ns1:CR_Kitchin ;
  dc11:publisher ns1:Institute_of_Physics_Publishing ;
  bibo:uri "http://www.crcpress.com/product/isbn/9781466511156" ;
  bibo:isbn13 "9781466511156" .

ns1:Astrophysical_Techniques_chapter1
  a bibo:Chapter ;
  dc11:title "Detectors" ;
  bibo:chapter "1" ;
  bibo:pageStart "1" ;
  bibo:pageEnd "185" ;
  bibo:reproducedIn ns1:Astrophysical_Techniques .

ns1:Astrophysical_Techniques_chapter3
  a bibo:Chapter ;
  dc11:title "Photometry" ;
  bibo:chapter "3" ;
  bibo:pageStart "329" ;
  bibo:pageEnd "365" ;
  bibo:reproducedIn ns1:Astrophysical_Techniques .

ns1:Edwin_Budding
  a foaf:Person ;
  foaf:name "Edwin Budding" .

ns1:Osman_Demircan
  a foaf:Person ;
  foaf:name "Osman Demircan" .

ns1:Cambridge_University_Press
  a foaf:Organization ;
  foaf:name "Cambridge University Press" ;
  foaf:based_near "Cambridge, UK" .

ns1:IntroAstronomicalPhotometry
  a bibo:Book ;
  dc11:title "Introduction to Astronomical Photometry" ;
  dc11:date "2007" ;
  bibo:edition "2" ;
  dc11:creator ns1:Edwin_Budding, ns1:Osman_Demircan ;
  bibo:authorList ns1:IntroAstronomicalPhotometryAuthors ;
  dc11:publisher ns1:Cambridge_University_Press ;
  bibo:uri "http://ebooks.cambridge.org/ebook.jsf?bid=CBO9780511536175" ;
  bibo:isbn13 "9780521847117" .

ns1:IntroAstronomicalPhotometry_chapter_2
  a bibo:Chapter ;
  dc11:title "Introduction" ;
  bibo:chapter "2" ;
  bibo:pageStart "11" ;
  bibo:pageEnd "38" ;
  bibo:reproducedIn ns1:IntroAstronomicalPhotometry .

ns1:IntroAstronomicalPhotometryAuthors
  a rdf:Seq ;
  rdf:_1 ns1:Edwin_Budding ;
  rdf:_2 ns1:Osman_Demircan .

ns1:IAUDiv1WG
  a foaf:Organization ;
  foaf:name "IAU Division I Working Group Numerical Standards" .

ns1:International_Astronomical_Union
  a foaf:Organization ;
  foaf:name "International Astronomical Union" .

<http://www.iau.org/static/resolutions/IAU2012_English.pdf>
  a bibo:Standard ;
  dc11:date "2012" ;
  dc11:title "IAU 2012" ;
  dc11:creator ns1:IAUDiv1WG ;
  dc11:publisher ns1:International_Astronomical_Union ;
  bibo:uri "http://www.iau.org/static/resolutions/IAU2012_English.pdf" .

ns1:IAU_2012_Resolution_B2
  a bibo:Chapter ;
  dc11:title "Resolution B2" ;
  bibo:reproducedIn <http://www.iau.org/static/resolutions/IAU2012_English.pdf> .

ns1:Brengt_Stroemgren
  a foaf:Person ;
  foaf:name "Brengt Strömgren" .

ns1:Stroemgren1956
  a bibo:Article ;
  dc11:title "Two-dimensional spectral classification of F stars through photoelectric photometry with interference filters" ;
  dc11:date "1956" ;
  dc11:creator ns1:Brengt_Stroemgren ;
  dc11:subject "Astronomy", "Distance Measurement" ;
  dc11:isPartOf ns1:VistasAstronomy ;
  bibo:volume "2" ;
  bibo:pageStart "1336" ;
  bibo:pageEnd "1346" ;
  bibo:authorList ns1:Stroemgren1956Authors ;
  bibo:uri "http://www.sciencedirect.com/science/article/pii/0083665656900605" .

ns1:VistasAstronomy
  a bibo:Journal ;
  dc11:title "Vistas in Astronomy" .

ns1:Stroemgren1956Authors
  a rdf:Seq ;
  rdf:_1 ns1:Brengt_Stroemgren .

ns1:DLCrawford
  a foaf:Person ;
  foaf:name "David L. Crawford" .

ns1:Crawford1958
  a bibo:Article ;
  dc11:title "Two-dimensional spectral classification by narrow-band photometry for B stars in clusters and associations" ;
  dc11:date "1958" ;
  dc11:creator ns1:DLCrawford ;
  dc11:subject "Astronomy", "Distance Measurement" ;
  dc11:isPartOf ns1:ApJ ;
  bibo:volume "128" ;
  bibo:pageStart "185" ;
  bibo:pageEnd "206" ;
  bibo:authorList ns1:Crawford1958Authors ;
  bibo:uri "http://articles.adsabs.harvard.edu/cgi-bin/nph-iarticle_query?1958ApJ...128..185C&data_type=PDF_HIGH&whole_paper=YES&type=PRINTER&filetype=.pdf" .

ns1:ApJ
  a bibo:Journal ;
  dc11:title "Astrophysical Journal" ;
  bibo:shortTitle "ApJ" ;
  bibo:uri "http://iopscience.iop.org/0004-637X/" .

ns1:Crawford1958Authors
  a rdf:Seq ;
  rdf:_1 ns1:DLCrawford .

_:genid40
  a owl:Class ;
  owl:oneOf (
   ns2:angstrom
   ns2:astronomicalUnit
   ns2:BirminghamGauge
   ns2:chain
   ns2:cicero
   ns2:fathom-USSurvey
   ns2:fermi
   ns2:foot-International
   ns2:foot-USSurvey
   ns2:FrenchGauge
   ns2:furlong-International
   ns2:inch-International
   ns2:lightYear
   ns2:metre
   ns2:micron
   ns2:mil-Length
   ns2:mile-Statute
   ns2:mile-USSurvey
   ns2:nauticalMile-International
   ns2:parsec
   ns2:pica-ATA
   ns2:pica-Postscript
   ns2:pica-TeX
   ns2:point-ATA
   ns2:point-Didot
   ns2:point-Postscript
   ns2:point-TeX
   ns2:rod-US
   ns2:solarRadius
   ns2:yard-International
   ns2:gigaparsec
   ns2:kiloparsec
   ns2:megaparsec
 ) .

_:genid79
  a owl:Restriction ;
  owl:onProperty ns2:hasUnit ;
  owl:hasValue ns2:metre .

_:genid81
  a owl:Restriction ;
  owl:onProperty ns2:hasUnit ;
  owl:cardinality "1"^^xsd:nonNegativeInteger .

_:genid83
  a owl:Restriction ;
  owl:onProperty ns2:hasPrefix ;
  owl:allValuesFrom ns2:SIPrefix .

_:genid85
  a owl:Restriction ;
  owl:onProperty ns2:hasPrefix ;
  owl:cardinality "1"^^xsd:nonNegativeInteger .

_:genid88
  a owl:Class ;
  owl:oneOf (
   ns2:acre-International
   ns2:acre-USSurvey
   ns2:are
   ns2:barn
   ns2:circularMil
   ns2:squareMetre
   ns2:squareInch-International
   ns2:squareFoot-International
   ns2:squareYard-International
   ns2:squareMile-International
 ) .

_:genid105
  a owl:Restriction ;
  owl:onProperty ns2:hasBase ;
  owl:allValuesFrom ns2:PrefixedMetre .

_:genid107
  a owl:Restriction ;
  owl:onProperty ns2:hasBase ;
  owl:cardinality "1"^^xsd:nonNegativeInteger .

_:genid109
  a owl:Restriction ;
  owl:onProperty ns2:hasExponent ;
  owl:hasValue "2"^^xsd:nonNegativeInteger .

_:genid111
  a owl:Restriction ;
  owl:onProperty ns2:hasExponent ;
  owl:cardinality "1"^^xsd:nonNegativeInteger .

_:genid114
  a owl:Restriction ;
  owl:onProperty ns2:hasUnit ;
  owl:hasValue ns2:are .

_:genid116
  a owl:Restriction ;
  owl:onProperty ns2:hasUnit ;
  owl:cardinality "1"^^xsd:nonNegativeInteger .

_:genid118
  a owl:Restriction ;
  owl:onProperty ns2:hasPrefix ;
  owl:allValuesFrom ns2:SIPrefix .

_:genid120
  a owl:Restriction ;
  owl:onProperty ns2:hasPrefix ;
  owl:cardinality "1"^^xsd:nonNegativeInteger .

_:genid123
  a owl:Class ;
  owl:oneOf (
   ns2:acreFoot
   ns2:barrel-US
   ns2:bushel-US
   ns2:cord
   ns2:cup-USCustomary
   ns2:dryGallon-US
   ns2:dryPint-US
   ns2:dryQuart-US
   ns2:fluidOunce-Imperial
   ns2:fluidOunce-US
   ns2:gallon-Imperial
   ns2:gallon-US
   ns2:gill-Imperial
   ns2:gill-US
   ns2:litre
   ns2:liquidPint-US
   ns2:liquidQuart-US
   ns2:peck-US
   ns2:pint-Imperial
   ns2:quart-Imperial
   ns2:stere
   ns2:tablespoon-US
   ns2:teaspoon-US
   ns2:dessertspoon
   ns2:ton-Register
   ns2:cubicMetre
   ns2:cubicParsec
   ns2:cubicKiloparsec
 ) .

_:genid158
  a owl:Restriction ;
  owl:onProperty ns2:hasBase ;
  owl:allValuesFrom ns2:PrefixedMetre .

_:genid160
  a owl:Restriction ;
  owl:onProperty ns2:hasBase ;
  owl:cardinality "1"^^xsd:nonNegativeInteger .

_:genid162
  a owl:Restriction ;
  owl:onProperty ns2:hasExponent ;
  owl:hasValue "3"^^xsd:nonNegativeInteger .

_:genid164
  a owl:Restriction ;
  owl:onProperty ns2:hasExponent ;
  owl:cardinality "1"^^xsd:nonNegativeInteger .

_:genid167
  a owl:Restriction ;
  owl:onProperty ns2:hasUnit ;
  owl:hasValue ns2:litre .

_:genid169
  a owl:Restriction ;
  owl:onProperty ns2:hasUnit ;
  owl:cardinality "1"^^xsd:nonNegativeInteger .

_:genid171
  a owl:Restriction ;
  owl:onProperty ns2:hasPrefix ;
  owl:allValuesFrom ns2:SIPrefix .

_:genid173
  a owl:Restriction ;
  owl:onProperty ns2:hasPrefix ;
  owl:cardinality "1"^^xsd:nonNegativeInteger .

_:genid176
  a owl:Class ;
  owl:oneOf (
   ns2:degree
   ns2:gon
   ns2:mil-Angle
   ns2:minute-Angle
   ns2:radian
   ns2:revolution
   ns2:second-Angle
   ns2:millisecond-Angle
   ns2:microsecond-Angle
   ns2:metrePerMetre
 ) .

_:genid192
  a owl:Restriction ;
  owl:onProperty ns2:hasUnit ;
  owl:hasValue ns2:radian .

_:genid194
  a owl:Restriction ;
  owl:onProperty ns2:hasUnit ;
  owl:cardinality "1"^^xsd:nonNegativeInteger .

_:genid196
  a owl:Restriction ;
  owl:onProperty ns2:hasPrefix ;
  owl:allValuesFrom ns2:SIPrefix .

_:genid198
  a owl:Restriction ;
  owl:onProperty ns2:hasPrefix ;
  owl:cardinality "1"^^xsd:nonNegativeInteger .

_:genid201
  a owl:Class ;
  owl:oneOf (
   ns2:steradian
   ns2:squareMetrePerSquareMetre
   ns2:degreeSquared
   ns2:second-AngleSquared
 ) .

_:genid211
  a owl:Restriction ;
  owl:onProperty ns2:hasUnit ;
  owl:hasValue ns2:steradian .

_:genid213
  a owl:Restriction ;
  owl:onProperty ns2:hasUnit ;
  owl:cardinality "1"^^xsd:nonNegativeInteger .

_:genid215
  a owl:Restriction ;
  owl:onProperty ns2:hasPrefix ;
  owl:allValuesFrom ns2:SIPrefix .

_:genid217
  a owl:Restriction ;
  owl:onProperty ns2:hasPrefix ;
  owl:cardinality "1"^^xsd:nonNegativeInteger .

_:genid228
  a owl:Restriction ;
  owl:onProperty ns2:hasAggregateFunction ;
  owl:hasValue ns2:average .

_:genid235
  a owl:Class ;
  owl:oneOf (
   ns2:day
   ns2:day-Sidereal
   ns2:hour
   ns2:hour-Sidereal
   ns2:minute-Time
   ns2:minute-Sidereal
   ns2:second-Sidereal
   ns2:second-Time
   ns2:shake
   ns2:year
   ns2:year-Sidereal
   ns2:year-Tropical
   ns2:gigayear
 ) .

_:genid254
  a owl:Restriction ;
  owl:onProperty ns2:hasUnit ;
  owl:hasValue ns2:second-Time .

_:genid256
  a owl:Restriction ;
  owl:onProperty ns2:hasUnit ;
  owl:cardinality "1"^^xsd:nonNegativeInteger .

_:genid258
  a owl:Restriction ;
  owl:onProperty ns2:hasPrefix ;
  owl:allValuesFrom ns2:SIPrefix .

_:genid260
  a owl:Restriction ;
  owl:onProperty ns2:hasPrefix ;
  owl:cardinality "1"^^xsd:nonNegativeInteger .

_:genid263
  a owl:Class ;
  owl:oneOf (
   ns2:carat-Mass
   ns2:grain
   ns2:gram
   ns2:hundredweight-British
   ns2:hundredweight-US
   ns2:InternationalUnit
   ns2:milligramRAE
   ns2:ounceApothecaries
   ns2:ounceAvoirdupois
   ns2:pennyweight-Troy
   ns2:poundApothecaries
   ns2:poundAvoirdupois
   ns2:slug
   ns2:solarMass
   ns2:ton-ShortAssay
   ns2:ton-Long
   ns2:ton-Short
   ns2:tonne
   ns2:unifiedAtomicMassUnit
 ) .

_:genid290
  a owl:Restriction ;
  owl:onProperty ns2:hasUnit ;
  owl:hasValue ns2:gram .

_:genid292
  a owl:Restriction ;
  owl:onProperty ns2:hasUnit ;
  owl:cardinality "1"^^xsd:nonNegativeInteger .

_:genid294
  a owl:Restriction ;
  owl:onProperty ns2:hasPrefix ;
  owl:allValuesFrom ns2:SIPrefix .

_:genid296
  a owl:Restriction ;
  owl:onProperty ns2:hasPrefix ;
  owl:cardinality "1"^^xsd:nonNegativeInteger .

_:genid299
  a owl:Restriction ;
  owl:onProperty ns2:hasUnit ;
  owl:hasValue ns2:tonne .

_:genid301
  a owl:Restriction ;
  owl:onProperty ns2:hasUnit ;
  owl:cardinality "1"^^xsd:nonNegativeInteger .

_:genid303
  a owl:Restriction ;
  owl:onProperty ns2:hasPrefix ;
  owl:allValuesFrom ns2:SIPrefix .

_:genid305
  a owl:Restriction ;
  owl:onProperty ns2:hasPrefix ;
  owl:cardinality "1"^^xsd:nonNegativeInteger .

_:genid308
  a owl:Restriction ;
  owl:onProperty ns2:hasUnit ;
  owl:hasValue ns2:unifiedAtomicMassUnit .

_:genid310
  a owl:Restriction ;
  owl:onProperty ns2:hasUnit ;
  owl:cardinality "1"^^xsd:nonNegativeInteger .

_:genid312
  a owl:Restriction ;
  owl:onProperty ns2:hasPrefix ;
  owl:allValuesFrom ns2:SIPrefix .

_:genid314
  a owl:Restriction ;
  owl:onProperty ns2:hasPrefix ;
  owl:cardinality "1"^^xsd:nonNegativeInteger .

_:genid381
  a owl:Class ;
  owl:oneOf (
   ns2:hertz
   ns2:reciprocalSecond-Time
   ns2:reciprocalMinute-Time
   ns2:reciprocalHour
   ns2:reciprocalDay
   ns2:reciprocalYear
 ) .

_:genid393
  a owl:Restriction ;
  owl:onProperty ns2:hasUnit ;
  owl:hasValue ns2:hertz .

_:genid395
  a owl:Restriction ;
  owl:onProperty ns2:hasUnit ;
  owl:cardinality "1"^^xsd:nonNegativeInteger .

_:genid397
  a owl:Restriction ;
  owl:onProperty ns2:hasPrefix ;
  owl:allValuesFrom ns2:SIPrefix .

_:genid399
  a owl:Restriction ;
  owl:onProperty ns2:hasPrefix ;
  owl:cardinality "1"^^xsd:nonNegativeInteger .

_:genid414
  a owl:Class ;
  owl:oneOf (
   ns2:gal
   ns2:metrePerSecond-TimeSquared
 ) .

_:genid424
  a owl:Restriction ;
  owl:onProperty ns2:hasNumerator ;
  owl:allValuesFrom ns2:PrefixedMetre .

_:genid426
  a owl:Restriction ;
  owl:onProperty ns2:hasNumerator ;
  owl:cardinality "1"^^xsd:nonNegativeInteger .

_:genid428
  a owl:Restriction ;
  owl:onProperty ns2:hasDenominator ;
  owl:hasValue ns2:second-TimeSquared .

_:genid430
  a owl:Restriction ;
  owl:onProperty ns2:hasDenominator ;
  owl:cardinality "1"^^xsd:nonNegativeInteger .

_:genid433
  a owl:Restriction ;
  owl:onProperty ns2:hasNumerator ;
  owl:hasValue ns2:metre .

_:genid435
  a owl:Restriction ;
  owl:onProperty ns2:hasNumerator ;
  owl:cardinality "1"^^xsd:nonNegativeInteger .

_:genid437
  a owl:Restriction ;
  owl:onProperty ns2:hasDenominator ;
  owl:allValuesFrom ns2:PrefixedSecond-TimeSquared .

_:genid439
  a owl:Restriction ;
  owl:onProperty ns2:hasDenominator ;
  owl:cardinality "1"^^xsd:nonNegativeInteger .

_:genid442
  a owl:Restriction ;
  owl:onProperty ns2:hasNumerator ;
  owl:allValuesFrom ns2:PrefixedMetre .

_:genid444
  a owl:Restriction ;
  owl:onProperty ns2:hasNumerator ;
  owl:cardinality "1"^^xsd:nonNegativeInteger .

_:genid446
  a owl:Restriction ;
  owl:onProperty ns2:hasDenominator ;
  owl:allValuesFrom ns2:PrefixedSecond-TimeSquared .

_:genid448
  a owl:Restriction ;
  owl:onProperty ns2:hasDenominator ;
  owl:cardinality "1"^^xsd:nonNegativeInteger .

_:genid451
  a owl:Class ;
  owl:oneOf (
   ns2:gramPerCubicmetre
   ns2:milligramPerCubicmetre
   ns2:gramPerCubicCentimetre
   ns2:microgramPerCubicCentimetre
   ns2:kilogramPerCubicmetre
   ns2:kilogramPerCubicDecimetre
   ns2:gramPerLitre
   ns2:solarMassPerCubicParsec
 ) .

_:genid467
  a owl:Restriction ;
  owl:onProperty ns2:hasNumerator ;
  owl:allValuesFrom ns2:PrefixedGram .

_:genid469
  a owl:Restriction ;
  owl:onProperty ns2:hasNumerator ;
  owl:cardinality "1"^^xsd:nonNegativeInteger .

_:genid471
  a owl:Restriction ;
  owl:onProperty ns2:hasDenominator ;
  owl:hasValue ns2:litre .

_:genid473
  a owl:Restriction ;
  owl:onProperty ns2:hasDenominator ;
  owl:cardinality "1"^^xsd:nonNegativeInteger .

_:genid476
  a owl:Restriction ;
  owl:onProperty ns2:hasNumerator ;
  owl:hasValue ns2:gram .

_:genid478
  a owl:Restriction ;
  owl:onProperty ns2:hasNumerator ;
  owl:cardinality "1"^^xsd:nonNegativeInteger .

_:genid480
  a owl:Restriction ;
  owl:onProperty ns2:hasDenominator ;
  owl:allValuesFrom ns2:PrefixedLitre .

_:genid482
  a owl:Restriction ;
  owl:onProperty ns2:hasDenominator ;
  owl:cardinality "1"^^xsd:nonNegativeInteger .

_:genid485
  a owl:Restriction ;
  owl:onProperty ns2:hasNumerator ;
  owl:allValuesFrom ns2:PrefixedGram .

_:genid487
  a owl:Restriction ;
  owl:onProperty ns2:hasNumerator ;
  owl:cardinality "1"^^xsd:nonNegativeInteger .

_:genid489
  a owl:Restriction ;
  owl:onProperty ns2:hasDenominator ;
  owl:allValuesFrom ns2:PrefixedLitre .

_:genid491
  a owl:Restriction ;
  owl:onProperty ns2:hasDenominator ;
  owl:cardinality "1"^^xsd:nonNegativeInteger .

_:genid499
  a owl:Class ;
  owl:oneOf (
   ns2:knot-International
   ns2:millimetrePerHour
   ns2:kilometrePerHour
   ns2:centimetrePerDay
   ns2:metrePerDay
   ns2:millimetrePerDay
   ns2:metrePerSecond-Time
   ns2:mile-StatutePerHour
   ns2:nauticalMile-InternationalPerHour
 ) .

_:genid516
  a owl:Restriction ;
  owl:onProperty ns2:hasNumerator ;
  owl:allValuesFrom ns2:PrefixedMetre .

_:genid518
  a owl:Restriction ;
  owl:onProperty ns2:hasNumerator ;
  owl:cardinality "1"^^xsd:nonNegativeInteger .

_:genid520
  a owl:Restriction ;
  owl:onProperty ns2:hasDenominator ;
  owl:hasValue ns2:second-Time .

_:genid522
  a owl:Restriction ;
  owl:onProperty ns2:hasDenominator ;
  owl:cardinality "1"^^xsd:nonNegativeInteger .

_:genid525
  a owl:Restriction ;
  owl:onProperty ns2:hasNumerator ;
  owl:hasValue ns2:metre .

_:genid527
  a owl:Restriction ;
  owl:onProperty ns2:hasNumerator ;
  owl:cardinality "1"^^xsd:nonNegativeInteger .

_:genid529
  a owl:Restriction ;
  owl:onProperty ns2:hasDenominator ;
  owl:allValuesFrom ns2:PrefixedSecond-Time .

_:genid531
  a owl:Restriction ;
  owl:onProperty ns2:hasDenominator ;
  owl:cardinality "1"^^xsd:nonNegativeInteger .

_:genid534
  a owl:Restriction ;
  owl:onProperty ns2:hasNumerator ;
  owl:allValuesFrom ns2:PrefixedMetre .

_:genid536
  a owl:Restriction ;
  owl:onProperty ns2:hasNumerator ;
  owl:cardinality "1"^^xsd:nonNegativeInteger .

_:genid538
  a owl:Restriction ;
  owl:onProperty ns2:hasDenominator ;
  owl:allValuesFrom ns2:PrefixedSecond-Time .

_:genid540
  a owl:Restriction ;
  owl:onProperty ns2:hasDenominator ;
  owl:cardinality "1"^^xsd:nonNegativeInteger .

_:genid543
  a owl:Class ;
  owl:oneOf (
   ns2:dyne
   ns2:kip
   ns2:newton
   ns2:poundal
   ns2:pound-Force
   ns2:ton-Force-Short
   ns2:metreKilogramPerSecond-TimeSquared
 ) .

_:genid556
  a owl:Restriction ;
  owl:onProperty ns2:hasUnit ;
  owl:hasValue ns2:newton .

_:genid558
  a owl:Restriction ;
  owl:onProperty ns2:hasUnit ;
  owl:cardinality "1"^^xsd:nonNegativeInteger .

_:genid560
  a owl:Restriction ;
  owl:onProperty ns2:hasPrefix ;
  owl:allValuesFrom ns2:SIPrefix .

_:genid562
  a owl:Restriction ;
  owl:onProperty ns2:hasPrefix ;
  owl:cardinality "1"^^xsd:nonNegativeInteger .

_:genid565
  a owl:Class ;
  owl:oneOf (
   ns2:atmosphere-Standard
   ns2:atmosphere-Technical
   ns2:bar
   ns2:barye
   ns2:metreOfMercury
   ns2:pascal
   ns2:torr
   ns2:decibar
   ns2:microbar
   ns2:millibar
   ns2:centimetreOfMercury
   ns2:millimetreOfMercury
   ns2:kilogramSecond-TimeToThePower-2ReciprocalMetre
   ns2:newtonPerSquareMetre
 ) .

_:genid583
  a owl:Class ;
  owl:oneOf (
   ns2:atmosphere-Standard
   ns2:atmosphere-Technical
   ns2:bar
   ns2:barye
   ns2:metreOfMercury
   ns2:pascal
   ns2:torr
   ns2:decibar
   ns2:microbar
   ns2:millibar
   ns2:centimetreOfMercury
   ns2:millimetreOfMercury
   ns2:kilogramSecond-TimeToThePower-2ReciprocalMetre
   ns2:newtonPerSquareMetre
 ) .

_:genid607
  a owl:Restriction ;
  owl:onProperty ns2:hasUnit ;
  owl:hasValue ns2:pascal .

_:genid609
  a owl:Restriction ;
  owl:onProperty ns2:hasUnit ;
  owl:cardinality "1"^^xsd:nonNegativeInteger .

_:genid611
  a owl:Restriction ;
  owl:onProperty ns2:hasPrefix ;
  owl:allValuesFrom ns2:SIPrefix .

_:genid613
  a owl:Restriction ;
  owl:onProperty ns2:hasPrefix ;
  owl:cardinality "1"^^xsd:nonNegativeInteger .

_:genid628
  a owl:Class ;
  owl:oneOf (
   ns2:BritishThermalUnit-39F
   ns2:BritishThermalUnit-59F
   ns2:BritishThermalUnit-60F
   ns2:BritishThermalUnit-InternationalTable
   ns2:BritishThermalUnit-Mean
   ns2:BritishThermalUnit-Thermochemical
   ns2:calorie-15C
   ns2:calorie-20C
   ns2:calorie-InternationalTable
   ns2:calorie-Mean
   ns2:calorie-Thermochemical
   ns2:electronvolt
   ns2:erg
   ns2:footPoundal
   ns2:joule
   ns2:quad
   ns2:gigaelectronvolt
   ns2:kiloelectronvolt
   ns2:megaelectronvolt
   ns2:wattHour
   ns2:kilowattHour
   ns2:terawattHour
   ns2:therm-EC
   ns2:therm-US
   ns2:tonOfTNT
   ns2:newtonMetre
   ns2:micronewtonMetre
   ns2:millinewtonMetre
 ) .

_:genid664
  a owl:Restriction ;
  owl:onProperty ns2:hasUnit ;
  owl:hasValue ns2:joule .

_:genid666
  a owl:Restriction ;
  owl:onProperty ns2:hasUnit ;
  owl:cardinality "1"^^xsd:nonNegativeInteger .

_:genid668
  a owl:Restriction ;
  owl:onProperty ns2:hasPrefix ;
  owl:allValuesFrom ns2:SIPrefix .

_:genid670
  a owl:Restriction ;
  owl:onProperty ns2:hasPrefix ;
  owl:cardinality "1"^^xsd:nonNegativeInteger .

_:genid673
  a owl:Restriction ;
  owl:onProperty ns2:hasUnit ;
  owl:hasValue ns2:electronvolt .

_:genid675
  a owl:Restriction ;
  owl:onProperty ns2:hasUnit ;
  owl:cardinality "1"^^xsd:nonNegativeInteger .

_:genid677
  a owl:Restriction ;
  owl:onProperty ns2:hasPrefix ;
  owl:allValuesFrom ns2:SIPrefix .

_:genid679
  a owl:Restriction ;
  owl:onProperty ns2:hasPrefix ;
  owl:cardinality "1"^^xsd:nonNegativeInteger .

_:genid682
  a owl:Restriction ;
  owl:onProperty ns2:hasUnit ;
  owl:hasValue ns2:calorie-Mean .

_:genid684
  a owl:Restriction ;
  owl:onProperty ns2:hasUnit ;
  owl:cardinality "1"^^xsd:nonNegativeInteger .

_:genid686
  a owl:Restriction ;
  owl:onProperty ns2:hasPrefix ;
  owl:allValuesFrom ns2:SIPrefix .

_:genid688
  a owl:Restriction ;
  owl:onProperty ns2:hasPrefix ;
  owl:cardinality "1"^^xsd:nonNegativeInteger .

_:genid691
  a owl:Class ;
  owl:oneOf (
   ns2:horsepower-Boiler
   ns2:horsepower-British
   ns2:horsepower-Electric
   ns2:horsepower-Metric
   ns2:horsepower-Water
   ns2:kilocalorie-MeanPerDay
   ns2:solarLuminosity
   ns2:tonOfRefrigeration
   ns2:watt
   ns2:joulePerSecond-Time
 ) .

_:genid707
  a owl:Restriction ;
  owl:onProperty ns2:hasUnit ;
  owl:hasValue ns2:watt .

_:genid709
  a owl:Restriction ;
  owl:onProperty ns2:hasUnit ;
  owl:cardinality "1"^^xsd:nonNegativeInteger .

_:genid711
  a owl:Restriction ;
  owl:onProperty ns2:hasPrefix ;
  owl:allValuesFrom ns2:SIPrefix .

_:genid713
  a owl:Restriction ;
  owl:onProperty ns2:hasPrefix ;
  owl:cardinality "1"^^xsd:nonNegativeInteger .

_:genid731
  a owl:Class ;
  owl:oneOf (
   ns2:poise
   ns2:pascalSecond-Time
 ) .

_:genid739
  a owl:Restriction ;
  owl:onProperty ns2:hasUnit ;
  owl:hasValue ns2:poise .

_:genid741
  a owl:Restriction ;
  owl:onProperty ns2:hasUnit ;
  owl:cardinality "1"^^xsd:nonNegativeInteger .

_:genid743
  a owl:Restriction ;
  owl:onProperty ns2:hasPrefix ;
  owl:allValuesFrom ns2:SIPrefix .

_:genid745
  a owl:Restriction ;
  owl:onProperty ns2:hasPrefix ;
  owl:cardinality "1"^^xsd:nonNegativeInteger .

_:genid748
  a owl:Class ;
  owl:oneOf (
   ns2:stokes
   ns2:squareMetrePerSecond-Time
 ) .

_:genid756
  a owl:Restriction ;
  owl:onProperty ns2:hasUnit ;
  owl:hasValue ns2:stokes .

_:genid758
  a owl:Restriction ;
  owl:onProperty ns2:hasUnit ;
  owl:cardinality "1"^^xsd:nonNegativeInteger .

_:genid760
  a owl:Restriction ;
  owl:onProperty ns2:hasPrefix ;
  owl:allValuesFrom ns2:SIPrefix .

_:genid762
  a owl:Restriction ;
  owl:onProperty ns2:hasPrefix ;
  owl:cardinality "1"^^xsd:nonNegativeInteger .

_:genid828
  a owl:Restriction ;
  owl:onProperty ns2:hasTerm1 ;
  owl:allValuesFrom ns2:PrefixedMetre .

_:genid830
  a owl:Restriction ;
  owl:onProperty ns2:hasTerm1 ;
  owl:cardinality "1"^^xsd:nonNegativeInteger .

_:genid832
  a owl:Restriction ;
  owl:onProperty ns2:hasTerm2 ;
  owl:allValuesFrom ns2:PrefixedGram .

_:genid834
  a owl:Restriction ;
  owl:onProperty ns2:hasTerm2 ;
  owl:cardinality "1"^^xsd:nonNegativeInteger .

_:genid843
  a owl:Class ;
  owl:oneOf (
   ns2:gramPerSquareMetre
   ns2:kilogramPerSquareMetre
   ns2:kilogramPerHectare
   ns2:ounceAvoirdupoisPerSquareYard-International
 ) .

_:genid852
  a owl:Class ;
  owl:oneOf ( ns2:kilogramPerHectareDay ) .

_:genid863
  a owl:Restriction ;
  owl:onProperty ns2:hasBase ;
  owl:allValuesFrom ns2:PrefixedSecond-Time .

_:genid865
  a owl:Restriction ;
  owl:onProperty ns2:hasBase ;
  owl:cardinality "1"^^xsd:nonNegativeInteger .

_:genid867
  a owl:Restriction ;
  owl:onProperty ns2:hasExponent ;
  owl:hasValue "2"^^xsd:nonNegativeInteger .

_:genid869
  a owl:Restriction ;
  owl:onProperty ns2:hasExponent ;
  owl:cardinality "1"^^xsd:nonNegativeInteger .

_:genid904
  a owl:Class ;
  owl:oneOf ( ns2:kelvin ) .

_:genid909
  a owl:Class ;
  owl:oneOf (
   ns2:degreeCelsius
   ns2:degreeFahrenheit
   ns2:degreeRankine
   ns2:degreeReaumur
   ns2:kelvin
 ) .

_:genid919
  a owl:Restriction ;
  owl:onProperty ns2:hasUnit ;
  owl:hasValue ns2:kelvin .

_:genid921
  a owl:Restriction ;
  owl:onProperty ns2:hasUnit ;
  owl:cardinality "1"^^xsd:nonNegativeInteger .

_:genid923
  a owl:Restriction ;
  owl:onProperty ns2:hasPrefix ;
  owl:allValuesFrom ns2:SIPrefix .

_:genid925
  a owl:Restriction ;
  owl:onProperty ns2:hasPrefix ;
  owl:cardinality "1"^^xsd:nonNegativeInteger .

_:genid928
  a owl:Class ;
  owl:oneOf ( ns2:degreeCelsius ) .

_:genid933
  a owl:Restriction ;
  owl:onProperty ns2:hasUnit ;
  owl:hasValue ns2:degreeCelsius .

_:genid935
  a owl:Restriction ;
  owl:onProperty ns2:hasUnit ;
  owl:cardinality "1"^^xsd:nonNegativeInteger .

_:genid937
  a owl:Restriction ;
  owl:onProperty ns2:hasPrefix ;
  owl:allValuesFrom ns2:SIPrefix .

_:genid939
  a owl:Restriction ;
  owl:onProperty ns2:hasPrefix ;
  owl:cardinality "1"^^xsd:nonNegativeInteger .

_:genid942
  a owl:Class ;
  owl:oneOf ( ns2:degreeFahrenheit ) .

_:genid946
  a owl:Class ;
  owl:oneOf ( ns2:degreeRankine ) .

_:genid950
  a owl:Class ;
  owl:oneOf ( ns2:degreeReaumur ) .

_:genid1064
  a owl:Class ;
  owl:oneOf (
   ns2:abampere
   ns2:ampere
   ns2:biot
   ns2:statampere
 ) .

_:genid1072
  a owl:Class ;
  owl:oneOf ( ns2:gilbert ) .

_:genid1081
  a owl:Restriction ;
  owl:onProperty ns2:hasUnit ;
  owl:hasValue ns2:ampere .

_:genid1083
  a owl:Restriction ;
  owl:onProperty ns2:hasUnit ;
  owl:cardinality "1"^^xsd:nonNegativeInteger .

_:genid1085
  a owl:Restriction ;
  owl:onProperty ns2:hasPrefix ;
  owl:allValuesFrom ns2:SIPrefix .

_:genid1087
  a owl:Restriction ;
  owl:onProperty ns2:hasPrefix ;
  owl:cardinality "1"^^xsd:nonNegativeInteger .

_:genid1094
  a owl:Class ;
  owl:oneOf (
   ns2:abcoulomb
   ns2:coulomb
   ns2:faraday
   ns2:franklin
   ns2:statcoulomb
   ns2:second-TimeAmpere
   ns2:ampereHour
   ns2:milliampereHour
 ) .

_:genid1108
  a owl:Restriction ;
  owl:onProperty ns2:hasUnit ;
  owl:hasValue ns2:coulomb .

_:genid1110
  a owl:Restriction ;
  owl:onProperty ns2:hasUnit ;
  owl:cardinality "1"^^xsd:nonNegativeInteger .

_:genid1112
  a owl:Restriction ;
  owl:onProperty ns2:hasPrefix ;
  owl:allValuesFrom ns2:SIPrefix .

_:genid1114
  a owl:Restriction ;
  owl:onProperty ns2:hasPrefix ;
  owl:cardinality "1"^^xsd:nonNegativeInteger .

_:genid1117
  a owl:Class ;
  owl:oneOf (
   ns2:abvolt
   ns2:statvolt
   ns2:volt
   ns2:wattPerAmpere
 ) .

_:genid1127
  a owl:Restriction ;
  owl:onProperty ns2:hasUnit ;
  owl:hasValue ns2:volt .

_:genid1129
  a owl:Restriction ;
  owl:onProperty ns2:hasUnit ;
  owl:cardinality "1"^^xsd:nonNegativeInteger .

_:genid1131
  a owl:Restriction ;
  owl:onProperty ns2:hasPrefix ;
  owl:allValuesFrom ns2:SIPrefix .

_:genid1133
  a owl:Restriction ;
  owl:onProperty ns2:hasPrefix ;
  owl:cardinality "1"^^xsd:nonNegativeInteger .

_:genid1136
  a owl:Class ;
  owl:oneOf (
   ns2:abfarad
   ns2:farad
   ns2:statfarad
   ns2:coulombPerVolt
 ) .

_:genid1146
  a owl:Restriction ;
  owl:onProperty ns2:hasUnit ;
  owl:hasValue ns2:farad .

_:genid1148
  a owl:Restriction ;
  owl:onProperty ns2:hasUnit ;
  owl:cardinality "1"^^xsd:nonNegativeInteger .

_:genid1150
  a owl:Restriction ;
  owl:onProperty ns2:hasPrefix ;
  owl:allValuesFrom ns2:SIPrefix .

_:genid1152
  a owl:Restriction ;
  owl:onProperty ns2:hasPrefix ;
  owl:cardinality "1"^^xsd:nonNegativeInteger .

_:genid1155
  a owl:Class ;
  owl:oneOf (
   ns2:abohm
   ns2:ohm
   ns2:statohm
   ns2:voltPerAmpere
 ) .

_:genid1165
  a owl:Restriction ;
  owl:onProperty ns2:hasUnit ;
  owl:hasValue ns2:ohm .

_:genid1167
  a owl:Restriction ;
  owl:onProperty ns2:hasUnit ;
  owl:cardinality "1"^^xsd:nonNegativeInteger .

_:genid1169
  a owl:Restriction ;
  owl:onProperty ns2:hasPrefix ;
  owl:allValuesFrom ns2:SIPrefix .

_:genid1171
  a owl:Restriction ;
  owl:onProperty ns2:hasPrefix ;
  owl:cardinality "1"^^xsd:nonNegativeInteger .

_:genid1174
  a owl:Class ;
  owl:oneOf (
   ns2:abmho
   ns2:mho
   ns2:siemens
   ns2:statmho
   ns2:amperePerVolt
 ) .

_:genid1185
  a owl:Restriction ;
  owl:onProperty ns2:hasUnit ;
  owl:hasValue ns2:siemens .

_:genid1187
  a owl:Restriction ;
  owl:onProperty ns2:hasUnit ;
  owl:cardinality "1"^^xsd:nonNegativeInteger .

_:genid1189
  a owl:Restriction ;
  owl:onProperty ns2:hasPrefix ;
  owl:allValuesFrom ns2:SIPrefix .

_:genid1191
  a owl:Restriction ;
  owl:onProperty ns2:hasPrefix ;
  owl:cardinality "1"^^xsd:nonNegativeInteger .

_:genid1207
  a owl:Class ;
  owl:oneOf (
   ns2:maxwell
   ns2:statweber
   ns2:unitPole
   ns2:weber
   ns2:voltSecond-Time
 ) .

_:genid1218
  a owl:Restriction ;
  owl:onProperty ns2:hasUnit ;
  owl:hasValue ns2:weber .

_:genid1220
  a owl:Restriction ;
  owl:onProperty ns2:hasUnit ;
  owl:cardinality "1"^^xsd:nonNegativeInteger .

_:genid1222
  a owl:Restriction ;
  owl:onProperty ns2:hasPrefix ;
  owl:allValuesFrom ns2:SIPrefix .

_:genid1224
  a owl:Restriction ;
  owl:onProperty ns2:hasPrefix ;
  owl:cardinality "1"^^xsd:nonNegativeInteger .

_:genid1232
  a owl:Class ;
  owl:oneOf (
   ns2:gamma
   ns2:gauss
   ns2:stattesla
   ns2:tesla
   ns2:weberPerSquareMetre
   ns2:milligauss
 ) .

_:genid1244
  a owl:Restriction ;
  owl:onProperty ns2:hasUnit ;
  owl:hasValue ns2:tesla .

_:genid1246
  a owl:Restriction ;
  owl:onProperty ns2:hasUnit ;
  owl:cardinality "1"^^xsd:nonNegativeInteger .

_:genid1248
  a owl:Restriction ;
  owl:onProperty ns2:hasPrefix ;
  owl:allValuesFrom ns2:SIPrefix .

_:genid1250
  a owl:Restriction ;
  owl:onProperty ns2:hasPrefix ;
  owl:cardinality "1"^^xsd:nonNegativeInteger .

_:genid1253
  a owl:Class ;
  owl:oneOf (
   ns2:abhenry
   ns2:henry
   ns2:stathenry
   ns2:weberPerAmpere
 ) .

_:genid1267
  a owl:Restriction ;
  owl:onProperty ns2:hasUnit ;
  owl:hasValue ns2:henry .

_:genid1269
  a owl:Restriction ;
  owl:onProperty ns2:hasUnit ;
  owl:cardinality "1"^^xsd:nonNegativeInteger .

_:genid1271
  a owl:Restriction ;
  owl:onProperty ns2:hasPrefix ;
  owl:allValuesFrom ns2:SIPrefix .

_:genid1273
  a owl:Restriction ;
  owl:onProperty ns2:hasPrefix ;
  owl:cardinality "1"^^xsd:nonNegativeInteger .

_:genid1463
  a owl:Class ;
  owl:oneOf ( ns2:mole ) .

_:genid1470
  a owl:Restriction ;
  owl:onProperty ns2:hasUnit ;
  owl:hasValue ns2:mole .

_:genid1472
  a owl:Restriction ;
  owl:onProperty ns2:hasUnit ;
  owl:cardinality "1"^^xsd:nonNegativeInteger .

_:genid1474
  a owl:Restriction ;
  owl:onProperty ns2:hasPrefix ;
  owl:allValuesFrom ns2:SIPrefix .

_:genid1476
  a owl:Restriction ;
  owl:onProperty ns2:hasPrefix ;
  owl:cardinality "1"^^xsd:nonNegativeInteger .

_:genid1479
  a owl:Class ;
  owl:oneOf (
   ns2:molar
   ns2:molePerCubicmetre
   ns2:molePerLitre
 ) .

_:genid1491
  a owl:Restriction ;
  owl:onProperty ns2:hasNumerator ;
  owl:allValuesFrom ns2:PrefixedMole .

_:genid1493
  a owl:Restriction ;
  owl:onProperty ns2:hasNumerator ;
  owl:cardinality "1"^^xsd:nonNegativeInteger .

_:genid1495
  a owl:Restriction ;
  owl:onProperty ns2:hasDenominator ;
  owl:hasValue ns2:litre .

_:genid1497
  a owl:Restriction ;
  owl:onProperty ns2:hasDenominator ;
  owl:cardinality "1"^^xsd:nonNegativeInteger .

_:genid1500
  a owl:Restriction ;
  owl:onProperty ns2:hasNumerator ;
  owl:hasValue ns2:mole .

_:genid1502
  a owl:Restriction ;
  owl:onProperty ns2:hasNumerator ;
  owl:cardinality "1"^^xsd:nonNegativeInteger .

_:genid1504
  a owl:Restriction ;
  owl:onProperty ns2:hasDenominator ;
  owl:allValuesFrom ns2:PrefixedLitre .

_:genid1506
  a owl:Restriction ;
  owl:onProperty ns2:hasDenominator ;
  owl:cardinality "1"^^xsd:nonNegativeInteger .

_:genid1509
  a owl:Restriction ;
  owl:onProperty ns2:hasNumerator ;
  owl:allValuesFrom ns2:PrefixedMole .

_:genid1511
  a owl:Restriction ;
  owl:onProperty ns2:hasNumerator ;
  owl:cardinality "1"^^xsd:nonNegativeInteger .

_:genid1513
  a owl:Restriction ;
  owl:onProperty ns2:hasDenominator ;
  owl:allValuesFrom ns2:PrefixedLitre .

_:genid1515
  a owl:Restriction ;
  owl:onProperty ns2:hasDenominator ;
  owl:cardinality "1"^^xsd:nonNegativeInteger .

_:genid1518
  a owl:Restriction ;
  owl:onProperty ns2:hasUnit ;
  owl:hasValue ns2:molar .

_:genid1520
  a owl:Restriction ;
  owl:onProperty ns2:hasUnit ;
  owl:cardinality "1"^^xsd:nonNegativeInteger .

_:genid1522
  a owl:Restriction ;
  owl:onProperty ns2:hasPrefix ;
  owl:allValuesFrom ns2:SIPrefix .

_:genid1524
  a owl:Restriction ;
  owl:onProperty ns2:hasPrefix ;
  owl:cardinality "1"^^xsd:nonNegativeInteger .

_:genid1564
  a owl:Restriction ;
  owl:onProperty ns2:hasNumerator ;
  owl:allValuesFrom ns2:PrefixedMole .

_:genid1566
  a owl:Restriction ;
  owl:onProperty ns2:hasNumerator ;
  owl:cardinality "1"^^xsd:nonNegativeInteger .

_:genid1568
  a owl:Restriction ;
  owl:onProperty ns2:hasDenominator ;
  owl:hasValue ns2:metre .

_:genid1570
  a owl:Restriction ;
  owl:onProperty ns2:hasDenominator ;
  owl:cardinality "1"^^xsd:nonNegativeInteger .

_:genid1573
  a owl:Restriction ;
  owl:onProperty ns2:hasNumerator ;
  owl:hasValue ns2:mole .

_:genid1575
  a owl:Restriction ;
  owl:onProperty ns2:hasNumerator ;
  owl:cardinality "1"^^xsd:nonNegativeInteger .

_:genid1577
  a owl:Restriction ;
  owl:onProperty ns2:hasDenominator ;
  owl:allValuesFrom ns2:PrefixedMetre .

_:genid1579
  a owl:Restriction ;
  owl:onProperty ns2:hasDenominator ;
  owl:cardinality "1"^^xsd:nonNegativeInteger .

_:genid1582
  a owl:Restriction ;
  owl:onProperty ns2:hasNumerator ;
  owl:allValuesFrom ns2:PrefixedMole .

_:genid1584
  a owl:Restriction ;
  owl:onProperty ns2:hasNumerator ;
  owl:cardinality "1"^^xsd:nonNegativeInteger .

_:genid1586
  a owl:Restriction ;
  owl:onProperty ns2:hasDenominator ;
  owl:allValuesFrom ns2:PrefixedMetre .

_:genid1588
  a owl:Restriction ;
  owl:onProperty ns2:hasDenominator ;
  owl:cardinality "1"^^xsd:nonNegativeInteger .

_:genid1600
  a owl:Class ;
  owl:oneOf (
   ns2:amylaseUnit
   ns2:katal
   ns2:molePerSecond-Time
   ns2:deltaA450PerSecond-Time
 ) .

_:genid1612
  a owl:Restriction ;
  owl:onProperty ns2:hasUnit ;
  owl:hasValue ns2:katal .

_:genid1614
  a owl:Restriction ;
  owl:onProperty ns2:hasUnit ;
  owl:cardinality "1"^^xsd:nonNegativeInteger .

_:genid1616
  a owl:Restriction ;
  owl:onProperty ns2:hasPrefix ;
  owl:allValuesFrom ns2:SIPrefix .

_:genid1618
  a owl:Restriction ;
  owl:onProperty ns2:hasPrefix ;
  owl:cardinality "1"^^xsd:nonNegativeInteger .

_:genid1633
  a owl:Class ;
  owl:oneOf ( ns2:candela ) .

_:genid1640
  a owl:Restriction ;
  owl:onProperty ns2:hasUnit ;
  owl:hasValue ns2:candela .

_:genid1642
  a owl:Restriction ;
  owl:onProperty ns2:hasUnit ;
  owl:cardinality "1"^^xsd:nonNegativeInteger .

_:genid1644
  a owl:Restriction ;
  owl:onProperty ns2:hasPrefix ;
  owl:allValuesFrom ns2:SIPrefix .

_:genid1646
  a owl:Restriction ;
  owl:onProperty ns2:hasPrefix ;
  owl:cardinality "1"^^xsd:nonNegativeInteger .

_:genid1657
  a owl:Class ;
  owl:oneOf (
   ns2:lumen
   ns2:candelaSteradian
 ) .

_:genid1665
  a owl:Restriction ;
  owl:onProperty ns2:hasUnit ;
  owl:hasValue ns2:lumen .

_:genid1667
  a owl:Restriction ;
  owl:onProperty ns2:hasUnit ;
  owl:cardinality "1"^^xsd:nonNegativeInteger .

_:genid1669
  a owl:Restriction ;
  owl:onProperty ns2:hasPrefix ;
  owl:allValuesFrom ns2:SIPrefix .

_:genid1671
  a owl:Restriction ;
  owl:onProperty ns2:hasPrefix ;
  owl:cardinality "1"^^xsd:nonNegativeInteger .

_:genid1674
  a owl:Class ;
  owl:oneOf ( ns2:lumenSecond-Time ) .

_:genid1680
  a owl:Class ;
  owl:oneOf (
   ns2:footcandle
   ns2:lux
   ns2:phot
   ns2:lumenPerSquareMetre
 ) .

_:genid1690
  a owl:Restriction ;
  owl:onProperty ns2:hasUnit ;
  owl:hasValue ns2:lux .

_:genid1692
  a owl:Restriction ;
  owl:onProperty ns2:hasUnit ;
  owl:cardinality "1"^^xsd:nonNegativeInteger .

_:genid1694
  a owl:Restriction ;
  owl:onProperty ns2:hasPrefix ;
  owl:allValuesFrom ns2:SIPrefix .

_:genid1696
  a owl:Restriction ;
  owl:onProperty ns2:hasPrefix ;
  owl:cardinality "1"^^xsd:nonNegativeInteger .

_:genid1699
  a owl:Class ;
  owl:oneOf ( ns2:luxSecond-Time ) .

_:genid1705
  a owl:Class ;
  owl:oneOf ( ns2:lumenPerWatt ) .

_:genid1718
  a owl:Class ;
  owl:oneOf (
   ns2:gray
   ns2:rad
   ns2:joulePerKilogram
   ns2:kilojoulePerHectogram
 ) .

_:genid1731
  a owl:Restriction ;
  owl:onProperty ns2:hasUnit ;
  owl:hasValue ns2:gray .

_:genid1733
  a owl:Restriction ;
  owl:onProperty ns2:hasUnit ;
  owl:cardinality "1"^^xsd:nonNegativeInteger .

_:genid1735
  a owl:Restriction ;
  owl:onProperty ns2:hasPrefix ;
  owl:allValuesFrom ns2:SIPrefix .

_:genid1737
  a owl:Restriction ;
  owl:onProperty ns2:hasPrefix ;
  owl:cardinality "1"^^xsd:nonNegativeInteger .

_:genid1740
  a owl:Class ;
  owl:oneOf (
   ns2:rem
   ns2:sievert
   ns2:joulePerKilogram
   ns2:kilojoulePerHectogram
 ) .

_:genid1750
  a owl:Restriction ;
  owl:onProperty ns2:hasUnit ;
  owl:hasValue ns2:sievert .

_:genid1752
  a owl:Restriction ;
  owl:onProperty ns2:hasUnit ;
  owl:cardinality "1"^^xsd:nonNegativeInteger .

_:genid1754
  a owl:Restriction ;
  owl:onProperty ns2:hasPrefix ;
  owl:allValuesFrom ns2:SIPrefix .

_:genid1756
  a owl:Restriction ;
  owl:onProperty ns2:hasPrefix ;
  owl:cardinality "1"^^xsd:nonNegativeInteger .

_:genid1759
  a owl:Class ;
  owl:oneOf (
   ns2:becquerel
   ns2:curie
   ns2:reciprocalSecond-Time
 ) .

_:genid1768
  a owl:Restriction ;
  owl:onProperty ns2:hasUnit ;
  owl:hasValue ns2:becquerel .

_:genid1770
  a owl:Restriction ;
  owl:onProperty ns2:hasUnit ;
  owl:cardinality "1"^^xsd:nonNegativeInteger .

_:genid1772
  a owl:Restriction ;
  owl:onProperty ns2:hasPrefix ;
  owl:allValuesFrom ns2:SIPrefix .

_:genid1774
  a owl:Restriction ;
  owl:onProperty ns2:hasPrefix ;
  owl:cardinality "1"^^xsd:nonNegativeInteger .

_:genid1833
  a owl:Class ;
  owl:oneOf (
   ns2:darcy
   ns2:squareMetre
 ) .

_:genid1904
  a owl:Class ;
  owl:oneOf (
   ns2:bit
   ns2:byte
   ns2:hartley
   ns2:shannon
 ) .

_:genid1915
  a owl:Restriction ;
  owl:onProperty ns2:hasUnit ;
  owl:hasValue ns2:bit .

_:genid1917
  a owl:Restriction ;
  owl:onProperty ns2:hasUnit ;
  owl:cardinality "1"^^xsd:nonNegativeInteger .

_:genid1919
  a owl:Restriction ;
  owl:onProperty ns2:hasPrefix ;
  owl:allValuesFrom ns2:Prefix .

_:genid1921
  a owl:Restriction ;
  owl:onProperty ns2:hasPrefix ;
  owl:cardinality "1"^^xsd:nonNegativeInteger .

_:genid1924
  a owl:Restriction ;
  owl:onProperty ns2:hasUnit ;
  owl:hasValue ns2:byte .

_:genid1926
  a owl:Restriction ;
  owl:onProperty ns2:hasUnit ;
  owl:cardinality "1"^^xsd:nonNegativeInteger .

_:genid1928
  a owl:Restriction ;
  owl:onProperty ns2:hasPrefix ;
  owl:allValuesFrom ns2:Prefix .

_:genid1930
  a owl:Restriction ;
  owl:onProperty ns2:hasPrefix ;
  owl:cardinality "1"^^xsd:nonNegativeInteger .

